@prefix rdf: <http://www.w3.org/1999/02/22-rdf-syntax-ns#> .
@prefix : <https://www.ica.org/standards/RiC/ontology#> .
@prefix cc: <http://creativecommons.org/ns#> .
@prefix dc: <http://purl.org/dc/elements/1.1/> .
@prefix dcat: <http://www.w3.org/ns/dcat#> .
@prefix dcterms: <http://purl.org/dc/terms/> .
@prefix html: <http://www.w3.org/1999/xhtml> .
@prefix owl: <http://www.w3.org/2002/07/owl#> .
@prefix rdfs: <http://www.w3.org/2000/01/rdf-schema#> .
@prefix ric-dft: <https://www.ica.org/standards/RiC/vocabularies/documentaryFormTypes#> .
@prefix ric-rst: <https://www.ica.org/standards/RiC/vocabularies/recordSetTypes#> .
@prefix skos: <http://www.w3.org/2004/02/skos/core#> .
@prefix vann: <http://purl.org/vocab/vann/> .
@prefix voaf: <http://purl.org/vocommons/voaf#> .
@prefix xs: <http://www.w3.org/2001/XMLSchema> .
@prefix xsd: <http://www.w3.org/2001/XMLSchema#> .

cc:license
    a owl:AnnotationProperty ;
    rdfs:isDefinedBy <http://creativecommons.org/ns#> .

dc:contributor
    a owl:AnnotationProperty ;
    rdfs:isDefinedBy <http://purl.org/dc/elements/1.1/> .

dc:creator
    a owl:AnnotationProperty ;
    rdfs:isDefinedBy <http://purl.org/dc/elements/1.1/> .

dc:date
    a owl:AnnotationProperty ;
    rdfs:isDefinedBy <http://purl.org/dc/elements/1.1/> .

dc:language
    a owl:AnnotationProperty ;
    rdfs:isDefinedBy <http://purl.org/dc/elements/1.1/> .

dc:publisher
    a owl:AnnotationProperty ;
    rdfs:isDefinedBy <http://purl.org/dc/elements/1.1/> .

dc:rights
    a owl:AnnotationProperty ;
    rdfs:isDefinedBy <http://purl.org/dc/elements/1.1/> .

dc:title
    a owl:AnnotationProperty ;
    rdfs:isDefinedBy <http://purl.org/dc/elements/1.1/> .

dcterms:abstract
    a owl:AnnotationProperty ;
    rdfs:isDefinedBy <http://purl.org/dc/terms/> .

dcterms:contributor
    a owl:AnnotationProperty ;
    rdfs:isDefinedBy <http://purl.org/dc/terms/> .

dcterms:description
    a owl:AnnotationProperty ;
    rdfs:isDefinedBy <http://purl.org/dc/terms/> .

dcterms:publisher
    a owl:AnnotationProperty ;
    rdfs:isDefinedBy <http://purl.org/dc/terms/> .

dcterms:title
    a owl:AnnotationProperty ;
    rdfs:isDefinedBy <http://purl.org/dc/terms/> .

vann:preferredNamespacePrefix
    a owl:AnnotationProperty ;
    rdfs:isDefinedBy <http://purl.org/vocab/vann/> .

vann:preferredNamespaceUri
    a owl:AnnotationProperty ;
    rdfs:isDefinedBy <http://purl.org/vocab/vann/> .

voaf:Vocabulary
    a owl:Class ;
    rdfs:isDefinedBy <http://purl.org/vocommons/voaf> .

rdf:value
    a owl:AnnotationProperty ;
    rdfs:isDefinedBy <http://www.w3.org/1999/02/22-rdf-syntax-ns#> .

skos:Concept
    a owl:Class ;
    rdfs:isDefinedBy <http://www.w3.org/2004/02/skos/core> .

skos:ConceptScheme
    a owl:Class ;
    rdfs:isDefinedBy <http://www.w3.org/2004/02/skos/core> .

skos:broader
    a owl:ObjectProperty ;
    rdfs:isDefinedBy <http://www.w3.org/2004/02/skos/core> ;
    owl:inverseOf skos:narrower .

skos:changeNote
    a owl:AnnotationProperty ;
    rdfs:isDefinedBy <http://www.w3.org/2004/02/skos/core> ;
    rdfs:subPropertyOf skos:note .

skos:definition
    a owl:AnnotationProperty ;
    rdfs:isDefinedBy <http://www.w3.org/2004/02/skos/core> ;
    rdfs:subPropertyOf skos:note .

skos:example
    a owl:AnnotationProperty ;
    rdfs:isDefinedBy <http://www.w3.org/2004/02/skos/core> ;
    rdfs:subPropertyOf skos:note .

skos:hasTopConcept
    a owl:ObjectProperty ;
    rdfs:isDefinedBy <http://www.w3.org/2004/02/skos/core> ;
    owl:inverseOf skos:topConceptOf .

skos:historyNote
    a owl:AnnotationProperty ;
    rdfs:isDefinedBy <http://www.w3.org/2004/02/skos/core> ;
    rdfs:subPropertyOf skos:note .

skos:inScheme
    a owl:ObjectProperty ;
    rdfs:isDefinedBy <http://www.w3.org/2004/02/skos/core> .

skos:narrower
    a owl:ObjectProperty ;
    rdfs:isDefinedBy <http://www.w3.org/2004/02/skos/core> ;
    owl:inverseOf skos:broader .

skos:note
    a owl:AnnotationProperty ;
    rdfs:isDefinedBy <http://www.w3.org/2004/02/skos/core> .

skos:scopeNote
    a owl:AnnotationProperty ;
    rdfs:isDefinedBy <http://www.w3.org/2004/02/skos/core> ;
    rdfs:subPropertyOf skos:note .

skos:topConceptOf
    a owl:ObjectProperty ;
    rdfs:isDefinedBy <http://www.w3.org/2004/02/skos/core> ;
    owl:inverseOf skos:hasTopConcept .

dcat:version
    a owl:DatatypeProperty ;
    rdfs:isDefinedBy <http://www.w3.org/ns/dcat> .

<https://www.ica.org/standards/RiC/ontology>
    cc:license <https://creativecommons.org/licenses/by/4.0/> ;
    dc:contributor """Aaron Rubinstein (University of Massachusetts Amherst, USA),
         member of EGAD and EGAD RiC-O team from 2012 to 2022"""@en, """Daniel Pitti (University of Virginia, USA), chair of EGAD from
         2012"""@en, """Florence Clavaud (Archives nationales de France), member of EGAD
         and lead of EGAD RiC-O team from 2012"""@en, """Ivo Zandhuis (Consultant Digital Cultural Heritage, The
         Netherlands), member of EGAD and EGAD RiC-O team from 2023"""@en, """Jan Krause-Bilvin (docuteam, Switzerland), member of EGAD and
         EGAD RiC-O team from 2023"""@en, """Miia Herrala (National Archives of Finland), member of EGAD and
         EGAD RiC-O team from 2016 to 2022"""@en, """Regine I. Heberlein (University of Princeton, USA), member of EGAD and EGAD
         RiC-O team from 2023 to 2024""", """Richard David Williamson (National Archives of Norway), member
         of EGAD and of EGAD RiC-O team from 2024"""@en, """Tobias Wildi (docuteam, Switzerland), member of EGAD and EGAD
         RiC-O team from 2019"""@en ;
    dc:creator """International Council on Archives Expert Group on Archival
         Description (ICA EGAD)"""@en ;
    dc:publisher "International Council on Archives"@en ;
    dc:rights "Copyright 2019-, International Council on Archives (ICA)"@en ;
    dcterms:abstract """
         <html:div xmlns:html=\"http://www.w3.org/1999/xhtml\" xml:lang=\"en\">
            <html:p>RiC-O (Records in Contexts-Ontology) is an OWL ontology for describing archival
               record resources. As the third part of Records in Contexts standard, it is a formal
               representation of Records in Contexts Conceptual Model (RiC-CM).</html:p>
            <html:p>RiC-O provides a generic vocabulary and formal rules for creating RDF datasets
               to describe any kind of archival record resource, whether natively or by transforming
               existing metadata (or generating them from existing archival metadata). It supports
               publishing RDF datasets as Linked Data, querying them using SPARQL, and making
               inferences.</html:p>
            <html:p>The current version is <html:strong>v1.1</html:strong>; <html:strong>it is
                  compliant with RiC-CM 1.0</html:strong>, which was published by EGAD on November
               30, 2023.</html:p>
         </html:div>
      """^^rdf:XMLLiteral ;
    dcterms:contributor <https://orcid.org/0000-0001-6743-9622>, <https://orcid.org/0000-0001-9375-2102>, <https://orcid.org/0000-0001-9938-6502>, <https://orcid.org/0000-0002-0803-8025>, <https://orcid.org/0000-0002-5681-4850>, <https://orcid.org/0000-0003-0165-8341>, <https://orcid.org/0009-0004-3219-2534> ;
    dcterms:description """
         <html:div xmlns:html=\"http://www.w3.org/1999/xhtml\" id=\"introduction\" xml:lang=\"en\">
            <html:h3>Introduction</html:h3>
            <html:p>RiC-O (Records in Contexts-Ontology) is an OWL ontology for describing archival
               record resources. As the third part of Records in Contexts standard, it is a formal
               representation of Records in Contexts Conceptual Model (RiC-CM). This version, which
               is v1.1, is the latest official release. It is compliant with RiC-CM v1.0.</html:p>
            <html:p>The following diagram shows the main RiC-CM 1.0 entities and a few relations
               between them: <html:img alt=\"A partial overview of RiC-CM 1.0 main entities\" class=\"diagram\" src=\"https://github.com/ICA-EGAD/RiC-O/blob/7bc6d5d59ecc85a4b901cc79d649ae50209fd69e/diagrams/diagrams_v1-0/RiC-CM-overview/diagram_RiC-CM-overview-RiC-v1-0.jpg?raw=true\"></html:img>
            </html:p>
            <html:div id=\"design-principles\">
               <html:h4>RiC-O design principles</html:h4>
               <html:p>The following design principles were followed when developing RiC-O.</html:p>
               <html:p>
                  <html:strong>1. RiC-O is a domain and reference ontology</html:strong>.</html:p>
               <html:p>RiC-O provides <html:strong>a generic vocabulary and formal rules for
                     creating RDF datasets (or generating them from existing archival metadata) that
                     describe in a consistent way any kind of archival record
                  resource</html:strong>. It supports publishing RDF datasets as Linked Data,
                  querying them using SPARQL, and making inferences using the logic of the
                  ontology.</html:p>
               <html:p>While some projects have built some specific ontologies for describing
                  archives, in 2013 no generic domain ontology existed for the specific needs of the
                  archival community. This is why EGAD decided to develop RiC-O as a part of RiC
                  standard.</html:p>
               <html:p>Apart from this first, main target, <html:strong>RiC-O, as a technical
                     implementation of RiC-CM that also extends and refines it and that includes
                     formal logic, can guide or inspire, in many ways, the development of any tool
                     or system that manages (i.e. stores, enables to edit or processes) and
                     publishes descriptive archival metadata.</html:strong>. Of course, other
                  technical implementations of RiC-CM may be developed later on. Also, the current
                  technical implementations of the former ICA standards, e.g. EAD and EAC-CPF XML
                  schemas, should be made closer to RiC-CM in the future; on this topic, see <html:a href=\"https://www2.archivists.org/groups/technical-subcommittee-on-encoded-archival-standards-ts-eas\">the news and announcements of the Technical Subcommittee on Encoded Archival
                     Standards (TS-EAS) of the Society of American Archivists</html:a>.</html:p>
               <html:p>As RiC-O is a generic, domain ontology, <html:strong>it does not address by
                     itself every specific need or expectation</html:strong> that may occur in every
                  archival institution or project. It is rather <html:strong>a high level
                     framework</html:strong> and an institution or project implementing RiC-O can
                  apply only such a subset of properties as meets their needs, or extend the
                  specification according to their particular requirements, or do both.</html:p>
               <html:p>As a domain ontology, RiC-O, at this stage, does not borrow from other
                  existing ontologies (such as the cultural heritage models – IFLA-LRM and
                  CIDOC-CRM, PREMIS, or PROV-O). It should therefore be easier, for an archival
                  institution or archival project, to understand, implement and maintain RiC-O
                  within its system.</html:p>
               <html:p>Alignment with those and other models, where possible, will be undertaken in
                  a future revision cycle to support the interconnected nature of resource
                  description across the domains. This is of course essential for interconnecting
                  RDF datasets conforming to RiC-O with other datasets, or for using parts of RiC-O
                  in other contexts than the archival or records management realm.</html:p>
               <html:p>
                  <html:strong>2. RiC-O is immediately usable.</html:strong>
               </html:p>
               <html:p>
                  <html:strong>This is a key feature</html:strong>. <html:strong>Metadata conforming
                     to superseded ICA standards can be transformed to RiC-O
                     successfully</html:strong>. Converting existing archival metadata created or
                  generated in current information systems and compliant with ICA standards to
                  RDF/RiC-O is possible without losing data or structure.</html:p>
               <html:p>During the ongoing development process of RiC-O, intensive conversion
                  testing, either by hand or using scripts, was conducted on XML/EAD finding aids
                  and XML/EAC-CPF authority records to ensure that RiC-O is usable with existing
                  descriptive metadata. An <html:a href=\"https://github.com/ArchivesNationalesFR/rico-converter\">open source
                     conversion software</html:a> was also developed, whose first version was
                  published in April 2020.</html:p>
               <html:p>While some existing metadata sets may have a very fine level of granularity
                  and accuracy, already using, for example, controlled vocabularies, or describing
                  curation events separately, often these metadata don’t have the very precise
                  structure that RiC-CM recommends. Even then, such a conversion process remains
                  possible. In order to allow this, RiC-O sometimes provides several methods for
                  representing information (as described below). From this point of view, RiC-O 1.1
                  may be considered a transitional ontology, in which some components may be
                  deprecated later on.</html:p>
               <html:p>The usability of a model also depends on its documentation. RiC-O is
                  documented extensively. The documentation will be reviewed and updated on a
                  continuing basis.</html:p>
               <html:p>
                  <html:strong>3. RiC-O provides a flexible framework</html:strong>.</html:p>
               <html:p>
                  <html:strong>This is a very important principle too</html:strong>. It is related
                  with the usability principle quoted above. Moreover, <html:strong>archival
                     description is flexible by essence</html:strong>. It is quite commonly noted
                  that today the level of granularity of information varies from one finding aid to
                  another (or from one authority record to another), or even within the same finding
                  aid. Some series or agents are described summarily because little is known about
                  them and there is little time for extensive research, while other series, even
                  records, or agents are described in detail; some relations (e.g. that relating to
                  provenance) may be described without any detail while others may be thoroughly
                  documented, as ISAAR(CPF) and EAC-CPF allow it.</html:p>
               <html:p>Being generally flexible, for an OWL ontology, depends first on the
                  polyhierarchical systems of classes and properties it provides. A superproperty or
                  superclass, more general or generic than its subproperties or subclasses, must
                  exist and be available for handling information, while at the same time more
                  accurate subcomponents must be there for handling more accurate description. Also,
                  RiC-O provides methods for describing relations as full entities, as well as
                  direct and short paths between entities.</html:p>
               <html:p>
                  <html:strong>4. RiC-O opens new potential for archival description.</html:strong>
               </html:p>
               <html:p>
                  <html:strong>Linked Data tools and interfaces enable end users to go through
                     RDF/RiC-O graphs, query them using SPARQL, and make inferences. This means a
                     completely new way of consulting archival metadata and their multiple
                     contexts.</html:strong> An end user should be able to ask of any given data
                  set, for example, “What are (according to your dataset) the corporate bodies that
                  succeeded a given entity from its end of existence to now (as concerns this given
                  activity)?”, or “what instantiations of this photograph exist?”, or “what are the
                  existing copies of this original charter?”, and get a list of these entities. This
                  means that institutions or projects that invest in the implementation of RiC-O
                  will be able to query their data in ways not possible with the previous ICA
                  standards, and will get new insight into the content and context of their archives
                  that wasn’t visible with the existing ICA-standards. What is more, repositories
                  using RiC-O may infer new assertions from the RDF datasets and link them to other
                  resources outside their institution, thereby amplifying the query and inferencing
                  possibilities manifold.</html:p>
               <html:p>
                  <html:strong>5. RiC-O is extensible.</html:strong>
               </html:p>
               <html:p>Institutions with descriptive needs beyond what RiC-O provides out-of-the-box
                  have the option of extending the ontology by adding new subclasses or
                  subproperties as needed. Also, the concepts defined in existing SKOS vocabularies
                  (e.g. a list of documentary form types) can also be connected to RiC-O based
                  graphs (using the *Type classes, and properties which are in the domain or range
                  of these classes).</html:p>
               <html:p>RiC-O has also the potential to be usable in other contexts than purely
                  archival ones. It can be used to “hook” archival description to descriptive
                  metadata in other domains (e.g. bibliographic or museum metadata). As said above,
                  alignment with other models will be undertaken by EGAD in a future revision cycle,
                  facilitating such connections.</html:p>
            </html:div>
            <html:div id=\"understanding-RiCO\">
               <html:h4>Understanding RiC-O: a quick overview of some features</html:h4>
               <html:div id=\"fromRiCCM-to-RiCO\">
                  <html:h5>From RiC-CM to RiC-O</html:h5>
                  <html:div id=\"From_RiC-CM_components_to_RiC-O_classes\">
                     <html:h6>1. From RiC-CM components to RiC-O classes</html:h6>
                     <html:p>
                        <html:strong>Each RiC-CM entity has a corresponding class in
                           RiC-O</html:strong>. These classes are organized according to the same
                        hierarchy as in RiC-CM. Some projects may need very few of them (e.g. Agent,
                        Record Resource and Activity only), while others may need more (e.g.
                        Corporate Body and Person; Record; Place).</html:p>
                     <html:p>
                        <html:strong>Many classes only exist in RiC-O and not in
                           RiC-CM</html:strong>. These additional classes address special
                        needs:</html:p>
                     <html:ul>
                        <html:li>
                           <html:strong>some correspond to RiC-CM attributes</html:strong>, when it
                           may be considered necessary to handle them as full entities. This is the
                           case for <html:a href=\"#rico:Type\">Type</html:a> and its subclasses, that
                           correspond to RiC-CM attributes that contain controlled values, and that
                           can help to articulate RiC-O with external RDF resources like SKOS
                           vocabularies; and also for <html:a href=\"#rico:Language\">Language</html:a>, <html:a href=\"#rico:Name\">Name</html:a> and
                              <html:a href=\"#rico:Identifier\">Identifier</html:a>, that can be
                           considered as full entities and as key linking nodes in a RDF graph. All
                           these classes have been grouped under a <html:a href=\"#rico:Concept\">Concept</html:a> class.</html:li>
                        <html:li>
                           <html:strong>some classes have been added in order to provide a more
                              accurate definition and model for some entities</html:strong>. For
                           example, <html:a href=\"#rico:Place\">Place</html:a> comes along with a
                              <html:a href=\"#rico:PhysicalLocation\">Physical Location
                           class</html:a>, and with a <html:a href=\"#rico:Coordinates\">Coordinates
                              class</html:a>. A Place is considered both a geographical and
                           historical entity. As a historical entity, among other features, it has a
                           history, and may be preceded or succeeded by other Places. A Place also
                           may have zero to many Physical Location through time (for instance, its
                           boundaries, if it is an administrative area or a country, may change).
                           Each Physical Location may be connected to zero to many Coordinates. This
                           model is quite close to the Linked Places Format (<html:a href=\"https://github.com/LinkedPasts/linked-places\">https://github.com/LinkedPasts/linked-places</html:a>).</html:li>
                        <html:li>Another example of such an addition is the <html:a href=\"#rico:Proxy\">Proxy class</html:a>, that represents (stands for)
                           a Record Resource as it exists in a specific other Record Resource, and
                           may therefore be useful when you describe records which are
                           simultaneously included in several distinct record resources.</html:li>
                        <html:li>
                           <html:strong>finally, a system of n-ary classes helps to implement the
                              Relations section of RiC-CM</html:strong>. While these relations also
                           are represented as simple, binary object properties (e.g. <html:a href=\"#rico:hasOrganicProvenance\">hasOrganicProvenance</html:a> that
                           corresponds to RiC-R026 relation), you may need to assign different
                           attributes to a relation, e.g. a date, certainty or description, as it is
                           already possible, and quite often done, in a XML/EAC-CPF file. One of the
                           standard available methods for representing such a documented relation in
                           RDF for now is to use a class. Thus, for example, in RiC-O a <html:a href=\"#rico:OrganicProvenanceRelation\">OrganicProvenanceRelation
                              class</html:a> exists. Instances of this class can connect one to many
                           Agents to one to many created or accumulated Record Resources or
                           Instantiations, which actually is a quite common situation. In addition
                           to properties that can be used for any Thing, they may have some specific
                           object properties, like <html:a href=\"#rico:relationHasDate\">rico:relationHasDate</html:a> that was added in RiC-O 1.1, or <html:a href=\"#rico:relationCertainty\">rico:relationCertainty</html:a>,
                              <html:a href=\"#rico:relationSource\">rico:relationSource</html:a>,
                              <html:a href=\"#rico:relationState\">rico:relationState</html:a>). Back
                           to the <html:a href=\"#rico:hasOrganicProvenance\">hasOrganicProvenance</html:a> object property, let us add that it is
                           formally defined in RiC-O, using OWL 2 property chain axiom (see <html:a href=\"https://www.w3.org/TR/owl2-new-features/#F8:_Property_Chain_Inclusion\">https://www.w3.org/TR/owl2-new-features/#F8:_Property_Chain_Inclusion</html:a>),
                           as a ‘shortcut’ for the longer path
                           ‘thingIsSourceOfRelation/organicProvenanceRelation_role/relationHasTarget’,
                           where the intermediate node is an instance of OrganicProvenanceRelation:<html:br></html:br>
                           <html:img alt=\"rico:hasOrganicProvenance object property as a shortcut\" class=\"code\" src=\"https://github.com/ICA-EGAD/RiC-O/blob/master/ontology/current-version/HTML_view/rico_hasOrganicProvenance.png?raw=true\"></html:img>
                           <html:br></html:br>A triplestore, with the appropriate configuration, may thus
                           infer the direct ‘hasOrganicProvenance’ assertion from this long
                           path.</html:li>
                     </html:ul>
                  </html:div>
                  <html:div id=\"about_RiC-O_datatype-properties\">
                     <html:h6>2. About RiC-O datatype properties (relations whose object is a
                        literal)</html:h6>
                     <html:p>
                        <html:strong>Most of the datatype properties in RiC-O correspond to RiC-CM
                           attributes that contain free, plain text</html:strong>. See for example
                           <html:a href=\"#rico:generalDescription\">rico:generalDescription</html:a>,
                           <html:a href=\"#rico:history\">rico:history</html:a> and <html:a href=\"#scopeAndContent\">rico:scopeAndContent</html:a>.</html:p>
                     <html:p>In many simple use cases it’s sufficent to just use the <html:a href=\"#rico:identifier\">rico:identifier</html:a> or <html:a href=\"#rico:name\">rico:name</html:a> datatype properties. However, as
                        already said, in addition to these datatype properties, the Name and
                        Identifier RiC-CM attributes also have corresponding classes (subclasses of
                           <html:a href=\"#rico:Appellation\">rico:Appellation</html:a>). A resource
                        may have several Identifiers (e.g. archival reference code, system number,
                        digital object identifier) or Names and each comes with different
                        attributes; in this case instances of classes are needed. The Location
                        RiC-CM attribute also has a <html:a href=\"#rico:PhysicalLocation\">rico:PhysicalLocation</html:a> corresponding class (for users who want
                        to use Place, Physical Location and Coordinates for handling
                        places).</html:p>
                     <html:p>As already said too, every RiC-CM attribute that has ‘controlled value’
                        or ‘rule-based’ as a schema value, has a class as corresponding component in
                        RiC-O. <html:strong>However, for these CM attributes that correspond to a
                           RiC-O class, as it is necessary to provide an immediately usable
                           ontology, two supplementary datatype properties exist that allow not to
                           use the classes, at least for a while, if you want to implement RiC-O and
                           create RiC-O/RDF datasets from existing archival metadata without being
                           able to handle URIs for the information you have</html:strong>.</html:p>
                     <html:p>For example, you may not be able to handle and maintain URIs for some
                        controlled values you use in EAD finding aids for carrier types: maybe your
                        information system does not use a vocabulary for this, and you cannot for a
                        while consider these carrier types as full entities. Nevertheless you want
                        to produce RiC-O datasets where every piece of information is kept, and you
                        want to avoid blank nodes. If RiC-O would only provide the Carrier Type
                        class, it would be an issue for you.</html:p>
                     <html:p>So RiC-O provides a <html:a href=\"#rico:type\">rico:type</html:a>
                        datatype property, with range rdfs:literal, which allows you to move
                        forward. For RiC-CM Coordinates attribute, you also have the <html:a href=\"#rico:geographicalCoordinates\">rico:geographicalCoordinates</html:a> datatype property.</html:p>
                     <html:p>These datatype properties have a skos:scopeNote which says (for
                        example) \"Provided for usability reasons. May be made deprecated or removed
                        later on. Use only if you don’t use Physical Location and Coordinates
                        classes with Place.\"</html:p>
                     <html:p>
                        <html:strong>The same key design principle (RiC-O must be immediately
                           usable) led us to define some datatype properties that would enable users
                           to use RiC-O in simple use cases where they do not want to consider dates
                           and rules as full entities</html:strong>. Thus, there of course is Date
                        and Rule classes in RiC-O (since there are Date and Rule entities in
                        RiC-CM). And <html:strong>you also have a <html:a href=\"#rico:date\">rico:date</html:a> datatype property, which has several
                           subproperties; plus a <html:a href=\"#rico:ruleFollowed\">rico:ruleFollowed</html:a> datatype property</html:strong>. The same
                        analysis led us to keep the <html:a href=\"#rico:history\">rico:history</html:a> datatype property in RiC-O (same as RiC-CM history
                        attribute), while RiC-CM and RiC-O also provide the <html:a href=\"#rico:Event\">Event</html:a> class, and using a series of Events may
                        of course be a better method, easier to query, link and display, than simply
                        using a history prose discourse. The two methods may be used in parallel
                        within the same dataset by an institution that, for example, would decide to
                        emphasize only the accession, appraisal and description events among the
                        whole history of Record Resources.</html:p>
                     <html:p>These datatype properties have the same kind of skos:scopeNote as
                        above.</html:p>
                     <html:p>Finally, <html:strong>we have introduced a few datatype properties that
                           do not correspond to any RiC-CM attribute</html:strong>.</html:p>
                     <html:p>Some are superproperties, and thus group datatype properties: <html:a href=\"#rico:physicalOrLogicalExtent\">rico:physicalOrLogicalExtent</html:a>, with rico:carrierExtent,
                        rico:instantiationExtent and rico:recordResourceExtent as subproperties;
                           <html:a href=\"#rico:textualValue\">rico:textualValue</html:a>, with
                        rico:expressedDate, rico:normalizedValue and rico:quantity as subproperties;
                           <html:a href=\"#rico:measure\">rico:measure</html:a>; <html:a href=\"#rico:referenceSystem\">rico:referenceSystem</html:a>; <html:a href=\"#rico:note\">rico:note</html:a> (added in RiC-O 1.1), with
                        rico:authenticityNote, rico:integrityNote and
                        rico:physicalCharacteristicsNote as subproperties.</html:p>
                     <html:p>Some are simply more specific properties, like: <html:a href=\"#rico:accrualsStatus\">rico:accrualsStatus</html:a>; <html:a href=\"#rico:recordResourceStructure\">rico:recordResourceStructure</html:a> and <html:a href=\"#rico:instantiationStructure\">rico:instantiationStructure</html:a>,
                        subproperties of rico:structure; <html:a href=\"#rico:title\">rico:title</html:a> (subproperty of rico:name); <html:a href=\"#rico:altitude\"> &gt;rico:altitude</html:a>, <html:a href=\"#rico:height\">rico:height</html:a>, <html:a href=\"#rico:latitude\">rico:latitude</html:a>, <html:a href=\"#rico:length\">rico:length</html:a>, <html:a href=\"#rico:longitude\">rico:longitude</html:a>, <html:a href=\"#rico:width\">rico:width</html:a>
                        (subproperties of rico:measure), <html:a href=\"#rico:geodesicSystem\">rico:geodesicSystem</html:a> and <html:a href=\"#rico:altimetricSystem\">rico:altimetricSystem</html:a> (subproperties of rico:referenceSystem);
                           <html:a href=\"#rico:sentimentOrEmotionExpressed\">rico:sentimentOrEmotionExpressed</html:a> (added in RiC-O 1.1),
                        subproperty of rico:scopeAndContent.</html:p>
                  </html:div>
                  <html:div id=\"about_RiC-O_object-properties\">
                     <html:h6>3. About RiC-O object properties (relations between two
                        entities)</html:h6>
                     <html:p>In order to connect all the classes created, <html:strong>a significant
                           number of object properties have been defined, in addition to the 85
                           relations defined in RiC-CM 1.0.</html:strong>
                     </html:p>
                     <html:p>While the 'flat' list of object properties is a long one,
                           <html:strong>the object properties are grouped
                           hierarchically</html:strong>, so that one can use the upper to
                        intermediate level ones for simplicity sake, or choose the most accurate and
                        expressive ones, or extend the system adding a subproperty easily. It is
                        expected that, in most use cases, a subset of these properties only will be
                        needed.</html:p>
                     <html:p>Below we just give a few details on certain specific sets of
                        properties.</html:p>
                     <html:p>While in RiC-CM it was not possible to achieve such a level of
                        precision with simple attributes, <html:strong>RiC-O includes object
                           properties to assert that a <html:a href=\"#rico:RecordSet\">rico:RecordSet</html:a> has or had members (either all of them, or
                           some of them) that share some characteristics</html:strong>, like
                        Language, ContentType, DocumentaryFormType, LegalStatus, RecordState, and
                        (added recently) accumulation or creation Date, or a subject (as a
                        rico:Thing). See for example <html:a href=\"#rico:hasOrHadAllMembersWithType\">rico:hasOrHadAllMembersWithType</html:a>, or <html:a href=\"#rico:hasOrHadSomeMembersWithSubject\">rico:hasOrHadSomeMembersWithSubject</html:a> and its
                        subproperties.</html:p>
                     <html:p>
                        <html:strong>Some of the object properties are formally defined as
                           shortcuts</html:strong>: they can be inferred if you create triples that
                        include instances of the Relation classes. See the example explained above
                        in the <html:a href=\"#RiC-O_classes\">section dedicated to classes</html:a>.
                        In RiC-O 1.1, some object properties that connect a RecordResource or an
                        Agent to a Date are also now defined as shortcuts, like <html:a href=\"#rico:isOrWasActiveAtDate\">rico:isOrWasActiveAtDate</html:a> or
                           <html:a href=\"#rico:hasCreationDate\">rico:hasCreationDate</html:a>.</html:p>
                     <html:p>
                        <html:strong>Many properties, added in RiC-O 1.0 and later, are
                           transitive</html:strong>, as explained in the <html:a href=\"#history-note\">history note</html:a>.</html:p>
                  </html:div>
                  <html:div id=\"named-individuals\">
                     <html:h6>4. Named Individuals</html:h6>
                     <html:p>RiC-O adds seven individuals to address current and frequent
                        needs:</html:p>
                     <html:ul>
                        <html:li>
                           <html:a href=\"#FindingAid\">FindingAid</html:a>, <html:a href=\"#AuthorityRecord\">AuthorityRecord</html:a>, and <html:a href=\"#IIIFManifest\">IIIFManifest</html:a> (added in RiC-O 1.1), which
                           are instances of both RiC-O Documentary Form Type and SKOS Concept, and
                           can be used for categorizing finding aids, authority records and IIIF
                           manifests, which can be considered as Records. For example, a Record with
                           Documentary Form Type ‘Finding Aid’ may be connected to one to many
                           Record Resources using the ‘rico:describes’ object property.</html:li>
                        <html:li>
                           <html:a href=\"#Fonds\">Fonds</html:a>, <html:a href=\"#Series\">Series</html:a>, <html:a href=\"#File\">File</html:a>, and <html:a href=\"#Collection\">Collection</html:a> are instances of both Record
                           Set Type class and skos:Concept. Their definition is taken from the
                           ISAD(G) glossary. They can be used for categorizing Record
                           Sets.</html:li>
                     </html:ul>
                     <html:p>We expect other categories to be defined by the archival community as
                        RiC-O matures, forming rich, hopefully multilingual, SKOS vocabularies that
                        support rich description (for example, allowing an instance of the <html:a href=\"#rico:DocumentaryFormType\">Documentary Form Type class</html:a> to
                        have a history and temporal relations to other documentary form
                        types).</html:p>
                  </html:div>
               </html:div>
               <html:div id=\"RiCO-documentation\">
                  <html:h5>RiC-O documentation and annotation properties</html:h5>
                  <html:p>Each class, property and individual has an English, a French and a Spanish
                     label (rdfs:label), and a description (rdfs:comment). Each class also has been
                     assigned a German label in RiC-O 1.1. Some components also have a
                     skos:scopeNote or a skos:example.</html:p>
                  <html:p>When a RiC-O class or property corresponds to a RiC-CM component in any
                     way, its description and scope note are either the same as or derived from
                     their RiC-CM definition and scope note.</html:p>
                  <html:p>RiC-O provides two annotation properties (subproperties of rdfs:comment)
                     for handling:</html:p>
                  <html:ul>
                     <html:li>information about the corresponding RiC-CM component when applicable
                           (<html:a href=\"#rico:RiCCMCorrespondingComponent\">rico:RiCCMCorrespondingComponent</html:a>). Various phrasings are used
                        in this property depending on the rule applied for defining the RiC-CM
                        component.</html:li>
                     <html:li>information about possible mappings with other models or ontologies
                           (<html:a href=\"#rico:closeTo\">rico:closeTo</html:a>, rarely used in this
                        1.1 version)).</html:li>
                  </html:ul>
                  <html:p>Any change in the definition of a class or property made since December
                     2019 is documented using a skos:changeNote.</html:p>
               </html:div>
            </html:div>
            <html:div id=\"next-steps\">
               <html:h4>Next steps</html:h4>
               <html:p>The following is a non exhaustive list of known issues, topics or tasks on
                  which EGAD has begun to work and will continue to work in the next months. These
                  topics are part of the roadmap for RiC-O 2.0.</html:p>
               <html:ul>
                  <html:li>articulate the Event and Activity classes, and the Relation system of
                     classes</html:li>
                  <html:li>add suggestions of mappings (in rico:closeTo) and OWL equivalences
                     between some classes or properties and components in other models (among which
                     - this is not an exhaustive list- PREMIS, Schema.org, PROV-O, IFLA-LRM and RDA,
                     CIDOC-CRM), or document how these models can be used together. </html:li>
                  <html:li>develop multilingual vocabularies in order to provide users with means to
                     populate RiC-CM attributes that have a controlled value, and to use shared
                     instances of RiC-O *Type classes, so that their RDF datasets would be easier to
                     query using SPARQL federated queries or portals, and to link to each other.
                     Such a task will probably start with curation Activity Types and Rule Types, in
                     addition to more Record Set Types and Documentary Form Types than the seven
                     ones already defined.</html:li>
               </html:ul>
            </html:div>
         </html:div>
      """^^rdf:XMLLiteral ;
    dcterms:publisher <http://www.wikidata.org/entity/Q1421986> ;
    dcterms:title """International Council on Archives Records in Contexts Ontology
         (ICA RiC-O) version 1.1"""@en ;
    vann:preferredNamespacePrefix "rico" ;
    vann:preferredNamespaceUri "https://www.ica.org/standards/RiC/ontology#" ;
    a voaf:Vocabulary, owl:NamedIndividual, owl:Ontology ;
    rdfs:label """International Council on Archives Records in Contexts Ontology (ICA
         RiC-O) version 1.1"""@en ;
    owl:incompatibleWith <https://raw.githubusercontent.com/ICA-EGAD/RiC-O/master/ontology/previous-versions/RiC-O_v0-2_release/RiC-O_v0-2.rdf> ;
    owl:priorVersion <https://raw.githubusercontent.com/ICA-EGAD/RiC-O/master/ontology/previous-versions/RiC-O_v0-2_release/RiC-O_v0-2.rdf>, <https://raw.githubusercontent.com/ICA-EGAD/RiC-O/master/ontology/previous-versions/RiC-O_v1-0-1_release/RiC-O_1-0-1.rdf>, <https://raw.githubusercontent.com/ICA-EGAD/RiC-O/master/ontology/previous-versions/RiC-O_v1-0-beta_release/RiC-O_1-0-beta.rdf>, <https://raw.githubusercontent.com/ICA-EGAD/RiC-O/master/ontology/previous-versions/RiC-O_v1-0_release/RiC-O_1-0.rdf>, <https://www.ica.org/standards/RiC/ontology/1.0.2> ;
    owl:versionIRI <https://www.ica.org/standards/RiC/ontology/1.1> ;
    owl:versionInfo "Version 1.1 - 2025-05-22."@en ;
    skos:historyNote """
         <html:div xmlns:html=\"http://www.w3.org/1999/xhtml\" xml:lang=\"en\">
            <html:div id=\"history-note\">
               <html:h3>History note</html:h3>
               <html:p>A first beta version of RiC-O was developed in 2017 and used by the National
                  Archives of France for building a proof of concept (<html:a href=\"https://piaaf.demo.logilab.fr\">https://piaaf.demo.logilab.fr</html:a>).</html:p>
               <html:p>EGAD continued to develop the ontology, and this process entered a very
                  active period in 2019, while RiC-CM v0.2 was being designed and edited. From
                  December 2018 to November 2019, about 65 persons that responded to a call for
                  reviewers, received successive beta versions of RiC-O and sent a few first
                  comments. While EGAD RiC-O team could not answer to each of these comments, each
                  was taken into account. RiC-O v0.1 was released on December 2019, at the same time
                  as RiC-CM v0.2 preview.</html:p>
               <html:p>The Git repository that is used for handling RiC-O was made public in March
                  2020 (see <html:a href=\"https://github.com/ICA-EGAD/RiC-O\">https://github.com/ICA-EGAD/RiC-O</html:a>).</html:p>
               <html:p>In 2020, RiC-CM v0.2 preview was significantly updated: the textual
                  definitions of many entities were changed, as well as the specifications of many
                  attributes; and the IRIs of lot of relations were changed, in order to take into
                  account past situations and to adopt some simple naming rules. As a consequence,
                  RiC-O had to be updated in order to remain compliant with RiC-CM. These changes
                  could not be made before the end of 2020, when RiC-CM could be considered stable.
                  EGAD also decided to make other changes in RiC-O, among which the most important
                  are mentioned in bold in the following list.</html:p>
               <html:p>RiC-O 0.2 results from these updates and changes. It was released in February
                  2021, and is fully compliant with RiC-CM 0.2, which was released in July
                  2021.</html:p>
               <html:p>
                  <html:strong>At the end of 2022</html:strong>, while the EGAD group, as part of
                  the development of version 1.0 of RiC-CM, was working on analyzing and taking into
                  account the very numerous comments relating to RiC-CM 0.2 received, <html:strong>a
                     new active phase of development started for RiC-O. A team of no longer three,
                     but six people prepared this version.</html:strong> It was then absolutely not
                  a question of breaking with the principles and methods already used; the work was
                  a continuation of what had already been done. It was a matter of
                     <html:strong>improving what had already been done, by simplifying wherever
                     possible the specifications, by adding some properties and taking into account
                     the needs that a growing community of users was expressing</html:strong>. On
                  the other hand, it was obviously a question of <html:strong>making RiC-O 1.0
                     compliant with RiC-CM 1.0</html:strong>.</html:p>
               <html:p><html:strong>After the release of RiC-O 1.0 in December 2023, the development
                     team continued to improve the ontology</html:strong>. Bugs were fixed and a few
                  adjustments made to RiC-O documentation in v1.0.1 and 1.0.2. Then version 1.1
                  introduced, in addition to some corrections and adjustments, several significant
                  additions or modifications, the majority of which concern the rico:RecordResource
                  class and/or its subclasses.</html:p>
               <html:p>
                  <html:strong>As the result of this work, RiC-O 1.1 defines:</html:strong>
               </html:p>
               <html:ul>
                  <html:li>
                     <html:strong>107 classes</html:strong>. As in RiC-CM 1.0, the modeling of dates
                     had been modified, this led to the removal of the three subclasses of <html:a href=\"#rico:Date\">rico:Date</html:a> in RiC-O 1.0. It was also necessary to
                     add a <html:a href=\"#rico:MandateType\">rico:MandateType</html:a> class,
                     corresponding to the new RiC-A44 Mandate Type attribute of RiC-CM 1.0. A
                     generic <html:a href=\"#rico:OrganicOrFunctionalProvenanceRelation\">rico:OrganicOrFunctionalProvenanceRelation</html:a> class was also added.
                     In RiC-O 1.1, a new <html:a href=\"#rico:TitleType\">rico:TitleType</html:a>
                     class was added, as well as a <html:a href=\"#rico:StudyAtRelation\">rico:StudyAtRelation</html:a> class.</html:li>
                  <html:li>
                     <html:strong>75 datatype properties</html:strong>. Several properties had been
                     renamed in RiC-O 1.0, to make the ontology compliant with RiC-CM 1.0 (so
                     rico:descriptiveNote has become <html:a href=\"#rico:generalDescription\">rico:generalDescription</html:a>, whose definition is a little different).
                     A <html:a href=\"#rico:length\">rico:length</html:a> property had also been
                     added; rico:calendar and rico:dateStandard were removed. The hierarchy of
                        <html:a href=\"#rico:date\">rico:date</html:a> subproperties had been revised.
                     Some properties had been made subproperties of others (like <html:a href=\"#rico:scopeAndContent\">rico:scopeAndContent</html:a>, now a
                     subproperty of <html:a href=\"#rico:generalDescription\">rico:generalDescription</html:a>). Then in RiC-O 1.1, 14 datatype
                     properties were added, among which 9 are direct or indirect subproperties of
                        <html:a href=\"#rico:date\">rico:date</html:a>. Also, a <html:a href=\"#rico:note\">rico:note</html:a> datatype property was added,
                     superproperty of the already existing *note properties, with domain rico:Thing.
                     A new datatype property, <html:a href=\"#rico:sentimentOrEmotionExpressed\">rico:sentimentOrEmotionExpressed</html:a>, subproperty of
                     rico:scopeAndContent, was created, with domain Record or Record Part. A <html:a href=\"#rico:recordResourceSourceOfInformation\">rico:recordResourceSourceOfInformation</html:a> datatype property was added
                     to connect a Record Resource to a source on which its content is based. Two
                     datatype properties with domain RecordResource or Proxy (<html:a href=\"#rico:rankInSequence\">rico:rankInSequence</html:a> and <html:a href=\"#rico:rankInHierarchy\">rico:rankInHierarchy</html:a>), were added, to
                     be used in addition only (never independently) to the object properties defined
                     for representing sequences and hierarchies of record resources.</html:li>
                  <html:li>
                     <html:strong>480 object properties</html:strong>, compared to 400 in RiC-O 1.0
                     and 423 in RiC-O 0.2. <html:br></html:br> In RiC-O 1.0, <html:strong>significant
                        modifications had been made to the object properties of RiC-O
                        0.2</html:strong>. On the one hand, <html:strong>a certain number of
                        properties had been added to make RiC-O compliant with RiC-CM
                        1.0</html:strong>: addition of properties whose domain or range are <html:a href=\"#rico:Date\">rico:Date</html:a> or <html:a href=\"#rico:Event\">rico:Event</html:a>; addition of <html:a href=\"#rico:hasOrHadMandateType\">rico:hasOrHadMandateType</html:a> and <html:a href=\"#rico:isOrWasMandateTypeOf\">rico:isOrWasMandateTypeOf</html:a>,
                     properties related to the new <html:a href=\"#rico:MandateType\">rico:MandateType</html:a> class. On the other hand, <html:strong>to meet
                        the needs expressed by RiC-O users, other properties had been
                        added</html:strong>: <html:a href=\"#rico:isAgentAssociatedWithPlace\">rico:isAgentAssociatedWithPlace</html:a>, <html:a href=\"#rico:isOrWasEmployerOf\">rico:isOrWasEmployerOf</html:a>, <html:a href=\"#rico:wasMergedInto\">rico:wasMergedInto</html:a>, <html:a href=\"#rico:wasSplitInto\">rico:wasSplitInto</html:a>, <html:a href=\"#rico:hasDeathPlace\">rico:hasDeathPlace</html:a>, <html:a href=\"#rico:hasBirthPlace\">rico:hasBirthPlace</html:a>, <html:a href=\"#rico:hasOrHadAnalogueInstantiation\">rico:hasOrHadAnalogueInstantiation</html:a>, <html:a href=\"#rico:hasOrHadDigitalInstantiation\">rico:hasOrHadDigitalInstantiation</html:a>, and their inverse properties.
                     Furthermore, <html:strong>a significant number of properties had been added to
                        allow the expression of indirect relationships</html:strong>. Thus, it is
                     now possible, for instance, to specify that a <html:a href=\"#rico:Record\">rico:Record</html:a> is included indirectly in a <html:a href=\"#rico:RecordSet\">rico:RecordSet</html:a> such as a fonds, using
                        <html:a href=\"#rico:isIncludedInTransitive\">rico:isIncludedInTransitive</html:a>, or to infer this relation, which is
                     the super property of the new <html:a href=\"#rico:isDirectlyIncludedIn\">rico:isDirectlyIncludedIn</html:a> property. <html:strong>The addition of
                        such transitive properties concerned partitive (sub-properties of <html:a href=\"#rico:hasOrHadPart\">rico:hasOrHadPart</html:a>), sequential
                        (sub-properties of <html:a href=\"#rico:precedesOrPreceded\">rico:precedesOrPreceded</html:a>) and authority (sub-properties of
                           <html:a href=\"#rico:hasOrHadSubordinate\">rico:hasOrHadSubordinate</html:a>) relations</html:strong>, and the
                     inverse properties. It was accompanied by the creation of properties specifying
                     past relations. <html:br></html:br> Finally, <html:strong>in order to simplify their
                        maintenance, the n-ary Relation classes had been rolified</html:strong>. 48
                     new object properties had been created to do this, such as for example <html:a href=\"#rico:leadershipRelation_role\">rico:leadershipRelation_role</html:a>;
                     the definition of n-ary Relation classes (such as <html:a href=\"#rico:LeadershipRelation\">rico:LeadershipRelation</html:a>) was
                     revised to introduce an equivalence with these properties when they have the
                     same source and the same target, and the property chain axioms of the
                     corresponding binary properties (such as <html:a href=\"#rico:hasOrHadLeader\">rico:hasOrHadLeader</html:a>) were revised. 166 object properties, which
                     existed in RiC-O 0.2 and were specific to each of the n-ary relations, could
                     then be deleted. A full accounting of the rolification of n-ary relations may
                     be found at <html:a href=\"https://github.com/ICA-EGAD/RiC-O/issues/67\">https://github.com/ICA-EGAD/RiC-O/issues/67</html:a>).
                        <html:br></html:br><html:strong>In RiC-O 1.1, 80 object properties were added, whose
                        domain or range are most often rico:RecordResource (or its subclasses),
                        rico:Proxy, rico:Instantiation, rico:Date or rico:Relation</html:strong>.
                     The following list describes the main additions made.<html:ul>
                        <html:li>as a rico:TitleType class was added, the object properties needed
                           to connect it to rico:Title were also created. <html:strong>The names of
                              the higher level 'hasOrHadCategory' and 'isOrWasCategoryOf' object
                              properties have been changed to 'hasOrHadType' and
                              'isOrWasTypeOf'</html:strong>.</html:li>
                        <html:li>a <html:a href=\"#rico:studiesOrStudiedAt\">rico:studiesOrStudiedAt</html:a> object property - and the inverse
                           one, <html:a href=\"#rico:isOrWasAttendedByStudent\">rico:isOrWasAttendedByStudent</html:a> - was added, subproperty of
                           rico:isOrWasMemberOf, to connect a Person to a Corporate Body at which
                           the person studies or studied; as already said above, the corresponding
                              <html:a href=\"#rico:StudyAtRelation\">rico:StudyAtRelation</html:a>
                           n-ary class was also created;</html:li>
                        <html:li>object properties were added to be used for accumulation dates,
                           with domain the union of rico:RecordResource and rico:Instantiation (for
                              <html:a href=\"#rico:hasAccumulationDate\">rico:hasAccumulationDate</html:a>), or RecordSet (for <html:a href=\"#rico:hasOrHadAllMembersWithAccumulationDate\">rico:hasOrHadAllMembersWithAccumulationDate</html:a>, <html:a href=\"#rico:hasOrHadSomeMembersWithAccumulationDate\">rico:hasOrHadSomeMembersWithAccumulationDate</html:a>, <html:a href=\"#rico:hasOrHadMostMembersWithAccumulationDate\">rico:hasOrHadMostMembersWithAccumulationDate</html:a>), along with
                           the inverse properties. Note that a parallel rico:accumulationDate
                           datatype property was also created, along with its variants for
                           rico:RecordSet. Rico:hasAccumulationDate and rico:hasCreationDate were
                           made subproperties of a new <html:a href=\"#rico:hasOrganicProvenanceDate\">rico:hasOrganicProvenanceDate</html:a> object property.</html:li>
                        <html:li><html:strong>the textual definitions (rdfs:comment) of several
                              object properties (rico:isPublicationDateOf, rico:isCreationDateOf,
                              rico:isAccumulationDateOf, rico:isDestructionDateOf) and of their
                              variants, related to the lifecycle of records and instantiations, were
                              modified so that they can now be used for describing planned events or
                              activities</html:strong>. New <html:a href=\"#rico:isDerivationDateOf\">rico:isDerivationDateOf</html:a> and <html:a href=\"#rico:isMigrationDateOf\">rico:isMigrationDateOf</html:a> object
                           properties, with domain Instantiation, and their inverse properties, also
                           were added, with the same broader temporal coverage.</html:li>
                        <html:li>a <html:a href=\"#rico:relationHasDate\">rico:relationHasDate</html:a> object property (and its inverse
                           property) was created, <html:strong>and new chain property axioms could
                              be specified, using this new property, for connecting Record Resources
                              or Instantiations to a Date, through the n-ary provenance Relation
                              classes</html:strong> (rico:OrganicProvenanceRelation,
                           rico:CreationRelation and rico:AccumulationRelation) and the
                           Instantiation to Instantiation relations (rico:DerivationRelation and
                           rico:MigrationRelation).</html:li>
                        <html:li>a <html:a href=\"#rico:isOrWasActiveAtDate\">rico:isOrWasActiveAtDate</html:a> object property (and its inverse
                           property) was added, defined as a shortcut for 'thingIsTargetOfRelation o
                           performanceRelation_role o relationHasDate'.</html:li>
                        <html:li><html:strong>a new property was added to connect a Record Resource
                              to a Record Resource on which its content is based</html:strong>:
                              <html:a href=\"#rico:recordResourceHasSourceOfInformation\">rico:recordResourceHasSourceOfInformation</html:a> (and the inverse
                              <html:a href=\"#rico:isSourceOfInformationOfRecordResource\">rico:isSourceOfInformationOfRecordResource</html:a> object property).
                           These properties replace, as concerns Record Resource, the 'source'
                           datatype property and the 'hasSource'/'isSourceOf' object properties,
                           which had been created in RiC-O 0.1 and removed in RiC-O 1.0;</html:li>
                        <html:li><html:strong>new properties, some of which being transitive, were
                              added in order to complete the model as concerns the representation of
                              sequences and hierarchies of record resources</html:strong>. In
                           particular, this resulted in <html:strong>a significant set of object
                              properties in order to allow the use of rico:Proxy in such sequences
                              and hierarchies</html:strong>.</html:li>
                        <html:li><html:strong>two properties (<html:a href=\"#rico:hasContentWhichRepresents\">rico:hasContentWhichRepresents</html:a> and <html:a href=\"#rico:hasContentWhichMainlyRepresents\">rico:hasContentWhichMainlyRepresents</html:a>) were added as
                              subproperties of rico:hasOrHadSubject and
                              rico:hasOrHadMainSubject</html:strong>, in order to connect Records or
                           Record Parts and the Things they represent. Variants of those properties
                           were created in order to connect a Record Set and the Things that some or
                           all of its members are about or represent. The inverse properties were
                           also created.</html:li>
                     </html:ul>
                  </html:li>
                  <html:li><html:strong>7 named individuals</html:strong>, all of which are
                     instances of both skos:Concept and of, either rico:RecordSetType, or
                     rico:DocumentaryFormType. Six of those indivivuals had been defined in RiC-O
                     0.1. In RiC-O 1.1, a new individual, <html:a href=\"#IIIFManifest\">IIIFManifest</html:a>, instance of skos:Concept and of
                     rico:DocumentaryFormType, was added, to enable users to describe a IIIF
                     manifest in a RiC-O knowledge graph. Those individuals are part of two SKOS
                     vocabularies (<html:a href=\"#documentaryFormTypes\">documentaryFormTypes</html:a> and <html:a href=\"#recordSetTypes\">recordSetTypes</html:a>), which have also been available from v1.0 as
                     separate files, in the modularized version of RiC-O.</html:li>
               </html:ul>
               <html:p>Finally, significant efforts were made since the release of RiC-O 0.2
                  regarding the documentation of the ontology. In particular, <html:strong>the
                     labels of each class and property (rdfs:label annotations) are now available in
                     French and Spanish as well as in English</html:strong>. We would like to thank
                  our French-speaking and Spanish-speaking colleagues, members or not of the
                  ICA/EGAD group, who contributed to this translation work. <html:strong>In RiC-O
                     1.1, German labels were added to the 107 classes defined by the
                     ontology</html:strong>, thanks to the work of several German-speaking members
                  of ICA/EGAD.</html:p>
               <html:p><html:strong>RiC-O 1.1 therefore presents itself as an ontology richer than
                     RiC-O 0.2 and RiC-O 1.0, particularly as concerns record resources,
                     instantiations and agents, technically opening up new possibilities (with
                     transitive relations and shortcuts) and preserving or extending the semantics
                     defined previously</html:strong>.</html:p>
               <html:p>A running list of changes since v0.1 may be found in <html:a href=\"#appendix-I\">Appendix I</html:a>. <html:strong>Note that from October
                     2020 any change on a component is described and dated in the specification of
                     this component, using skos:changeNote</html:strong>.</html:p>
            </html:div>
            <html:div id=\"appendix-I\">
               <html:h3>Appendix I: list of the changes made since the release of RiC-O
                  v0.1</html:h3>
               <html:p>The following is a list of the changes made to RiC-O since the release of
                  RiC-O v0.1 in December 2019. The most important changes are mentioned in bold.
                     <html:strong>Note that from October 2020 any change on a component is described
                     and dated in the specification of this component, using
                     skos:changeNote</html:strong>.</html:p>
               <html:ul>
                  <html:li>Fixed a bug in the documentation of rico:PerformanceRelation and its
                     object properties.</html:li>
                  <html:li>Renamed the file and updated the ontology metadata.</html:li>
                  <html:li>OccupationType made a subclass of ActivityType.</html:li>
                  <html:li>Changed the domain and range of rico:hasOriginal and rico:hasDraft (it is
                     now Record or Record Part); same for their inverse properties.</html:li>
                  <html:li>Fixed a bug in the definition of rico:provenanceRelationHasTarget
                     (removed the owl:propertyChainAxiom).</html:li>
                  <html:li>Changed the name of rico:leadBy object property (grammatical mistake) to
                     rico:ledBy. </html:li>
                  <html:li>2020, October 19: Added a vann:preferredNamespaceUri and
                     vann:preferredNamespacePrefix property to the ontology metadata</html:li>
                  <html:li>2020, October 19 : created RuleType and IdentifierType classes, along
                     with the associated object properties.</html:li>
                  <html:li>2020, October 23: <html:strong>updated the text definition and/or scope
                        note of 33 classes, that correspond to RiC-CM entities or attributes, in
                        order to make them compliant with RiC-CM v0.2</html:strong>. Added a few
                     owl:disjointWith properties.</html:li>
                  <html:li>2020, November 1: <html:strong>updated the text definition and/or scope
                        note of, and/or added examples for, 27 datatype properties, that correspond
                        to RiC-CM attributes, in order to make them compliant with RiC-CM
                        v0.2</html:strong>.</html:li>
                  <html:li>2020, November 20: <html:strong>created new classes and properties for
                        handling an accurate description of instantation and record resource
                        extent</html:strong>: Extent, Carrier Extent, Instantiation Extent, Record
                     Resource Extent, Unit of measurement, Extent Type classes; unit of measurement
                     and quantity datatype properties; has Extent, is Extent Of, has Extent Type, is
                     Extent Type Of, has Unit Of Measurement, is Unit of Measurement Of, object
                     properties.</html:li>
                  <html:li>2020, December 28: changed the IRIs and definition of RecordResourceState
                     class and of the associated object properties; <html:strong>changed the domain
                        or ranges and textual definitions of properties associated with Language,
                        LegalStatus, ContentType, DocumentaryFormType; added new object properties
                        for handling the description of some or all members of Record
                        Set</html:strong>. Added the corresponding change notes.</html:li>
                  <html:li>2020, December 29: deleted the isSuperiorTo and isInferiorTo object
                     properties, as well as the AgentSubordinationRelation and its object properties
                     (as the RiC-R043 relation has been removed from RiC-CM 0.2). Added the
                     hasAuthor/isAuthorOf object properties, plus an AuthorshipRelation class and
                     its specific object properties (as the RiC-R079 relation has been added to
                     RiC-CM 0.2). Added the corresponding change notes.</html:li>
                  <html:li>2021, January 22: <html:strong>changed the IRI, label, and/or
                        superproperties or inverse property IRI, and/or textual definition, and/or
                        domain or range, of 152 object properties. Among them, changed the IRI of
                        119 object properties; 85 correspond to RiC-CM relations whose name has been
                        changed in RiC-CM 0.2</html:strong>. Added the corresponding change
                     notes.</html:li>
                  <html:li>2021, January 27: added an rdfs:isDefinedBy to the specification of each
                     RiC-O class and property and made the last changes to the ontology metadata
                     (mainly in the history note).</html:li>
                  <html:li>2021, February 1: last small changes in the ontology metadata (mainly in
                     the abstract).</html:li>
                  <html:li>2021, February 1: 'hasOrHadPhysicalLocation' made a subproperty of
                     'isPlaceAssociatedWith'; 'isOrWasPhysicalLocationOf' made a subproperty of
                     'isAssociatedWithPlace'.</html:li>
                  <html:li>2021, February 1: reordered everything with Protégé without changing the
                     content</html:li>
                  <html:li>2021, February 4: checked and fixed the language of the
                     examples.</html:li>
                  <html:li>2021, February 8: removed a few Restriction classes
                     (rdfs:subClassOf/owl:Restriction) in the definition of classes; completed the
                     textual definition and scope note of the Relation class.</html:li>
                  <html:li>2021, February 9: added a link to RiC-CM 0.2 diagram overview in the
                     introduction; fixed some typos.</html:li>
                  <html:li>2021, February 11: added an @xml:lang='en' on a few labels; updated the
                     definition (rdfs:comment) and scope note of the Rule class, as they were
                     recently changed in RiC-CM 0.2 full draft.</html:li>
                  <html:li>2023, April 17: renamed the file (moving to RiC-O 1.0) and started to
                     update the ontology metadata.</html:li>
                  <html:li>2023, April 19: <html:strong>removed the unnecessary restrictions
                        specified for a significant number of classes</html:strong>, among which
                     most of the subclasses of Type, plus Activity, AgentTemporalRelation,
                     Coordinates, CreationRelation, Event, Identifier, Instantiation,
                     MandateRelation, Person, PhysicalLocation, Place, RecordResource, RecordSet,
                     Rule.</html:li>
                  <html:li>2023, April 21: removed an unnecessary restriction that remained on
                     Mandate class.</html:li>
                  <html:li>2023, end of May-June 5: fixed some typos in the introduction and
                     definition of entities, including the use of \"data property\" term instead of
                     the correct \"datatype property\" one.</html:li>
                  <html:li>2023, June 5: <html:strong>made includesOrIncluded object property a
                        subproperty of hasOrHadPart in addition to
                        isRecordResourceAssociatedToRecordResource</html:strong>.</html:li>
                  <html:li>2023, June 21: <html:strong>added two object properties, sub-properties
                        of hasSuccessor: wasMergedInto and wasSplitInto</html:strong>, with
                     Corporate Body as domain and range, and their inverse ones.</html:li>
                  <html:li>2023, July 25: adjusted definition of hasOrHadLanguage</html:li>
                  <html:li>2023, August 25: added French labels to the descriptions of classes and
                     of datatype properties</html:li>
                  <html:li>2023, August 28: added French labels to the descriptions of 250 object
                     properties; added an xml:lang attribute with value 'en' on rdfs:comment when it
                     was missing. Also added French labels to the two RiC-O annotation properties
                     and to the few named individuals already defined.</html:li>
                  <html:li>2023, August 28: changed the domain of hasExtent (from Instantiation or
                     RecordResource to Thing), same for the range of isExtentOf; added a length
                     datatype property under measure.</html:li>
                  <html:li>2023, August 29: <html:strong>updated hasInstantiation and
                        hasDerivedInstantiation</html:strong>, and the inverse properties (changed
                     their IRIs, labels, definitions, inverse properties, according to RiC-CM 1.0).
                     As a consequence, also updated the superproperties of migratedInto and
                     migratedFrom. <html:strong>Created four new object properties:
                        hasOrHadDigitalInstantiation, hasOrHadAnalogueInstantiation, and the inverse
                        ones</html:strong>.</html:li>
                  <html:li>2023, August 29: fixed some typos in the English labels of a few object
                     properties and added the past tense to the English label of
                     hasOrHadCoordinates.</html:li>
                  <html:li>2023, September 13: added 54 new object properties under 'hasorhadpart',
                     in order to extend the following nine existing properties:
                     'containsOrContained', 'hasOrHadComponent', 'hasOrHadConstituent',
                     'includesOrIncluded', 'hasOrHadSubdivision', 'hasOrHadSubevent'. Also did the
                     same for 'followsInTime', 'followsOrFollowed', 'isOrWasSubordinateto'. For each
                     listed property, one was added to express past partitive relations, and 2 other
                     ones for present partitive relations, the first one being transitive and the
                     superproperty of the second one. Added the inverse properties as well. Made
                     'hasDescendant' and 'hasAncestor' transitive.</html:li>
                  <html:li>2023, September 20: <html:strong>began to review and adjust the object
                        properties added on September 13, starting with the properties under
                        hasOrHadPart, and under the inverse isOrWasPartOf property. Among the
                        changes made: adjusted the change notes, added a few 'this is a transitive
                        relation' when missing in the rdfs:comment, and fixed the hierarchy of the
                        properties. Also, every past relation (e.g. contained) also made a
                        subproperty of hadPart. Every current transitive relation (e.g.
                        containsTransitive) made a subproperty of hasPartTransitive. Every current
                        direct relation (e.g. directlyContains) made a subproperty of
                        hasDirectPart</html:strong>. Fixed a syntaxic bug on the ontology history
                     note.</html:li>
                  <html:li>2023, September 22: finished to check and fix the object properties added
                     on September 13, working on hasOrHadSubordinate/isOrWasSubordinateTo
                     subproperties and on precedesOrPreceded/followsOrFollowed
                     subproperties.</html:li>
                  <html:li>2023, September 22: <html:strong>removed DateSingle, DateRange, DateSet
                        and added datatype and properties for dates</html:strong>.</html:li>
                  <html:li>2023, October 10: began to complete the updates made for date and its
                     properties. work done for Date Type, hasDateType, is dateTypeOf, expressedDate,
                     normalizedDateValue and dateQualifier. Also made isCreationDateOfMostMembersOf
                     a subproperty of isCreationDateOfSomeMembersOf; same for the inverse object
                     properties.</html:li>
                  <html:li>2023, October 12: <html:strong>finished to complete the updates made for
                        date and its properties</html:strong>. updated isCreationDateOf,
                     isCreationDateOfSomeMembersOf, isCreationDateOfMostMembersOf,
                     isCreationDateOfAllMembersOf, isPublicationDateOf and the inverse properties.
                     Also, renamed isDeletionDateOf into isDestructionDateOf, and applied the same
                     change to hasDeletiondate. Created isOccurrenceOf, isWithin, intersects ant the
                     inverse properties.</html:li>
                  <html:li>2023, October 13: adjusted a few details on date object properties
                     (renamed some of them to correct the spelling or take past members of record
                     sets into account; added a few subPropertyOf; adjusted the annotations
                     accordingly). Fixed a syntax problem on the history note of the
                     ontology.</html:li>
                  <html:li>2023, October 14: reintroduced the certainty datatype property with
                     domain Event and Relation. Adjusted a few details in the annotations of the
                     date properties.</html:li>
                  <html:li>2023, October 16: fixed several bugs while resolving conflicts before
                     merging, including bad IRIs.</html:li>
                  <html:li>2023, October 17: made occurredAtDate and isDateOfOccurenceof
                     subproperties of isEventAssociatedWith and isAssociatedWithEvent</html:li>
                  <html:li>2023, October 19: made rico:wasUsedFromDate and rico:wasUsedToDate (and
                     its inverses) sub-properties of rico:hasBeginningDate and rico:hasEndDate (and
                     its inverses) respectively</html:li>
                  <html:li>2023, October 19: added RecordPart to domain of hasOrHadConstituent and
                     to the range of the inverse property as well.</html:li>
                  <html:li>2023, October 20: <html:strong>created the following new properties
                        isAgentAssociatedWithPlace, hasDeathPlace, hasBirthPlace,
                        agentHasOrHadLocation, hasOrHadEmployer and their inverse
                        properties</html:strong> as well.</html:li>
                  <html:li>2023, October 26: added Record Part to the domain of hadOrhadConstituent
                     subproperties, and RecordPart to the range of the inverse ones. Changed the
                     definitions of these properties accordingly. Fixed a bug in the history note of
                     the ontology. Regenerated the inverse properties.</html:li>
                  <html:li>2023, October 26: changed the domain and range of 'is or was employer
                     of', removed 'has or had member' super-property of the propertyn added an
                     rdfs:comment to it. Same for the inverse property.</html:li>
                  <html:li>2023, October 26: added rdfs:comments, fixed one IRI, French labels, some
                     domains and range, to the recently added isPlaceAssociatedWithAgent,
                     isBirthPlaceOf, isDeathPlaceOf, isOrWasLocationOfAgent, and their inverse
                     properties. Fixed a bug in the history note of the ontology. Regenerated the
                     inverse properties.</html:li>
                  <html:li>2023, November 2: <html:strong>added Spanish labels to 59 datatype
                        properties, 103 classes and 277 object properties</html:strong>.</html:li>
                  <html:li>2023, November 7: added property chain axioms that were missing, in order
                     to define the following properties as shortcuts: isChildOf, hasOrHadPosition,
                     isOrWasAppellationOf, isOrWasDerivedFromInstantiation, hasOrHadWorkRelationWith
                     and hasGeneticLinkToRecordResource.</html:li>
                  <html:li>2023, November 7: added a hasOrganicOrFunctionalProvenance property,
                     superproperty of documents and of hasOrganicProvenance (new name of
                     hasProvenance); added the shortcut. Same for the inverse property. Added a
                     OrganicAndFunctionalProvenanceRelation, superclass of OrganicProvenanceRelation
                     (new name of AgentOriginationRelation) and ActivityDocumentationRelation;
                     created the needed object properties. Adjusted the names of the properties of
                     OrganicProvenanceRelation.</html:li>
                  <html:li>2023, November 8: <html:strong>rolifying the Relation classes, step
                        1</html:strong>: created 48 reflexive object properties that rolify the
                     classes; modified the specifications of the Relation classes; modified the
                     property chain axioms of the corresponding shortcuts. Fixed the range of
                     isExtentOf.</html:li>
                  <html:li>2023, November 8, later: <html:strong>rolifying the Relation classes,
                        step 2</html:strong>: deleted 166 object properties that had become
                     unnecessary.</html:li>
                  <html:li>2023, November 12: <html:strong>updated the datatype properties in order
                        to make them compliant with RiC-CM 1.0 attributes</html:strong>. Changed the
                     IRIS of accrual (to accruals), accrualStatus (to accrualsStatus),
                     descriptiveNote (to generalDescription), integrity (to integrityNote),
                     physicalCharacteristics (to physicalCharacteristicsNote),
                     qualityOfRepresentation (to qualityOfRepresentationNote). Made scopeAndContent
                     a subproperty of generalDescription, and expressedDate a subproperty of name.
                     Updated or added a few domains and many rdfs:comment, skos:scopeNote,
                     skos:example. Also made usedFromDate a subproperty of beginningDate, and
                     usedToDate a subproperty of endDate.</html:li>
                  <html:li>2023, November 12: <html:strong>updated the classes in order to make them
                        compliant with RiC-CM 1.0 entities and attributes</html:strong>. Updated or
                     added many rdfs:comment and skos:scopeNote, taking into account, as concerns
                     the Relation classes, the fact that they are n-ary. Created a new MandateType
                     class, corresponding to RiC-A44 attribute in RiC-CM 1.0. Also added a
                     rdfs:isDefinedBy to skos:Concept, skos:ConceptScheme and
                     voaf:Vocabulary.</html:li>
                  <html:li>2023, November 12 and 13: <html:strong>updated 35 object properties in
                        order to make them compliant with RiC-CM 1.0 relations. Added labels or
                        modified rdfs:comment of 65 other object properties. Added
                        hasOrHadMandateType and isOrWasMandateType of.</html:strong>
                  </html:li>
                  <html:li>2023, November 13: added or modified a few French or Spanish
                     labels.</html:li>
                  <html:li>2023, November 13: updated the ontology metadata.</html:li>
                  <html:li>2023, November 14: fixed some typos in the ontology metadata.</html:li>
                  <html:li>2023, November 24: started to work on v1.0, after releasing v 1.0-beta:
                     renamed the file and updated a few metadata.</html:li>
                  <html:li>2023, November 25: fixed three French labels; added Spanish labels to the
                     annotation properties and named individuals.</html:li>
                  <html:li>2023, November 27: added Spanish labels to the 93 object properties which
                     were missing one.</html:li>
                  <html:li>2023, December 6: <html:strong>improved the description (rdfs:comment) of
                        the 48 n-ary Relation classes by clearly specifying how they are
                        directed</html:strong>.</html:li>
                  <html:li>2023, December 13: Completed the metadata of the vocabulary: added
                     dc:language, a history note and a scope note.</html:li>
                  <html:li>2023, December 21: <html:strong>revised and updated the ontology metadata
                        and introduction, and the HTML view.</html:strong>.</html:li>
                  <html:li>2023, December 27: in order to make the ontology clearer and more
                     consistent, renamed the certainty and source datatype properties to
                     relationCertainty and relationSource and reduced their domain to Relation.
                     Renamed the 'hasSource' object property to 'isEvidencedBy' and reduced its
                     domain to Relation and range to RecordResource; same for the inverse property,
                     'isSourceOf', renamed to 'evidences'. Updated the specifications of these
                     properties accordingly.</html:li>
                  <html:li>2023, December 27: added rdfs:isDefinedBy to all the properties not
                     defined in RiC-O itself.</html:li>
                  <html:li>2023, December 28: made a few changes in the ontology introduction
                     (dcterms:description) and metadata.</html:li>
                  <html:li>2023, December 29: Added the property chain axiom on
                     'hasCreator'.</html:li>
                  <html:li>2023, December 30: Fixed a typo in five French labels.</html:li>
                  <html:li>2024, February 21: Fixed a typo in the rdfs:comment of rico:RoleType
                     class.</html:li>
                  <html:li>2024, April 10: <html:strong>Fixed the IRI of
                        'hasOrHadSomeMemberswithDocumentaryFormType' object property (changed to
                        'hasOrHadSomeMembersWithDocumentaryFormType')</html:strong> and corrected
                     several typos.</html:li>
                  <html:li>2024, April 12: Replaced the code illustrating the shortcut by an image,
                     change the headers of the subsections in 'From RiC-CM to RiC-O'; added a few
                     details to an sentence in the section on Ric-O properties; adjusted the
                     metadata, mainly moved to v1.0.1.</html:li>
                  <html:li>2024, May 2: Added Richard David Williamson to the list of contributors
                     and set the date of v1.0.1 to May 2, 2024.</html:li>
                  <html:li>2024, May 13: Added Richard Williamson's ORCID number, changed the
                     affiliation of T. Wildi and J. Krause-Bilvin, and set the date of v1.0.1 to May
                     13, 2024.</html:li>
                  <html:li><html:strong>2024, August 2: Removed global reflexivity from the object
                        properties that rolify the Relation classes, to fix a source of
                        inconsistency</html:strong> (they still satisfy local reflexivity, i.e.
                     reflexivity for each of these object properties can be inferred for all
                     individuals in their domain).</html:li>
                  <html:li>2024, September 2: Fixed the French label (rdfs:label) of the following
                     object properties: rico:isOrWasEnforcedBy; rico:isOrWasResponsibleForEnforcing;
                     rico:hasOrHadIntellectualPropertyRightsHolder; rico:hasOrHadController;
                     rico:isOrWasControllerOf; rico:isOrWasJurisdictionOf.</html:li>
                  <html:li>2024, September 2: Moved to v1.0.2: updated the metadata, and
                        <html:strong>added a owl:versionIRI to this new version</html:strong>. Moved
                     v1.0.1 to the previous-versions subfolder.</html:li>
                  <html:li>2024, September 2: Fixed a typo in two of the EDTF examples for
                     rico:normalizedDateValue.</html:li>
                  <html:li>2024, September 4: Fixed a few typos in Appendix 1 and in a change note.
                     Changed the date of the release (it is 2024 September 4th now).</html:li>
                  <html:li>2024, October 4: Added TitleType, hasTitleType and isTitleTypeOf;
                        <html:strong>Changed hasOrHadCategory et al. into
                     hasOrHadType</html:strong></html:li>
                  <html:li>2024, October 10: changed the French and/or Spanish labels of the
                     DemographicGroup class and of the 2 properties used with it,
                     hasOrHadDemographicGroup and isOrWasDemographicGroupOf.</html:li>
                  <html:li>2024, October 14: <html:strong>added the following object properties
                        under isDateAssociatedWith: isAccumulationDateOf,
                        isOrWasAccumulationDateOfAllMembersOf,
                        isOrWasAccumulationDateOfSomeMembersOf (and its
                        isOrWasAccumulationDateOfMostMembersOf subproperty)</html:strong>, and also
                     created the inverse properties under isAssociatedWithDate.</html:li>
                  <html:li>2024, October 16: started to move to v2.0.0: modified some of the
                     ontology metadata (versionIRI, versionInfo, rdfs:label, dcterms:title). Removed
                     the declarations of the two not used dcterms:creator and dcterms:rights
                     annotations. Checked the annotation properties. Renamed the file.</html:li>
                  <html:li>2024, October 21: fixed the Spanish label of 'hasSubeventTransitive'.
                     Added @xml:lang to 5 rdf:value and removed it from 9 dc:date in
                     skos:changeNote. Automatically reordered everything in the file, including the
                     labels and the change notes; regenerated the inverse properties. </html:li>
                  <html:li>2024, October 22: went back from 2.0.0 to v1.1, following a decision made
                     by the RiC-O team today. Modified the ontology metadata (owl:versionInfo,
                     rdfs:label, dcterms:title). Renamed the file.</html:li>
                  <html:li>2024, December 19: <html:strong>added relationHasDate and
                        isDateAssociatedWithRelation object properties, to connect n-ary Relation
                        classes and Dates. Added hasOrganicProvenanceDate and
                        isOrganicProvenanceDateOf object properties (with property chain axioms to
                        connect those properties to the OrganicProvenanceRelation). Added property
                        chain axioms to hasCreationDate, hasAccumulationDate, and to their inverse
                        properties</html:strong>.</html:li>
                  <html:li>2024, December 23: added the following datatype properties:
                     accumulationDate, allMembersWithAccumulationDate,
                     someMembersWithAccumulationDate (subproperties of date);
                     mostMembersWithAccumulationDate (subproperty of
                     someMembersWithAccumulationDate); allMembersWithCreationDate and
                     someMembersWithCreationDate (subproperties of beginningDate);
                     mostMembersWithCreationDate (subproperty of someMembersWithCreationDate).
                     Narrowed the domain of creationDate.</html:li>
                  <html:li>2024, December 24: <html:strong>added two new object properties,
                        studiesOrStudiedAt and isOrWasAttendedByStudent, plus a StudyAtRelation
                        n-ary Relation class</html:strong>, and studyAtRelation_role accompanyning
                     property.</html:li>
                  <html:li>2025, January 17: <html:strong>added a
                        'recordResourceSourceOfInformation' datatype property, and the
                        'recordResourceHasSourceOfInformation' and
                        'isSourceOfInformationOfRecordResource' object properties</html:strong>.
                     These properties replace, as concerns Record Resource, the 'source' datatype
                     property and the 'hasSource'/'isSourceOf' object properties, which had been
                     created in RC-O 0.1 and removed in RiC-O 1.0.</html:li>
                  <html:li>2025, January 17: <html:strong>added a 'note' datatype
                        property</html:strong>, superproperty of the existing 'integrityNote',
                     'authenticityNote' and 'physicalCharacteristicsNote' properties.</html:li>
                  <html:li>2025, January 30: <html:strong>added a 'IIIFManifest' SKOS Concept, RiC-O
                        Documentary Form Type, to the named individuals</html:strong>. Made it a
                     concept of the vocabulary on documentary form types and a narrower concept of
                     FindingAid.</html:li>
                  <html:li>2025, February 19: <html:strong>changed definitions so that dates for
                        destruction, accumulation, creation and publication could be in the future.
                        Added hasMigrationDate, isMigrationDateOf and migrationDate. Restricted the
                        domain of hasDestructionDate and of destructionDate</html:strong></html:li>
                  <html:li>2025, March 1st: fixed a bug (made isPublicationDateOf a subproperty of
                     isDateAssociatedWith, instead of isBeginningDateOf). <html:strong>Added
                        'hasDerivationDate', 'isDerivationDateOf' and
                     'derivationDate'</html:strong>. Changed the rdfs:subpropertyOf of
                     hasMigrationDate, isMigrationDateOf and of migrationDate accordingly. Removed
                     the mention of Record Resource from the rdfs:comment of isMigrationDateOf and
                     migrationDate.</html:li>
                  <html:li>2025, March 4th: <html:strong>introduced datatype properties
                        rankInSequence and rankInHierarchy, expanded the range of proxyIn to any
                        RecordResource and tweaked the definition of it and proxyFor accordingly,
                        added an inverse property hasProxy for proxyFor, added two new
                        sub-properties proxyInRecord and proxyInRecordSet of ProxyIn, introduced 36
                        object properties pertaining to use of Proxy in sequences or hierarchies,
                        and added one or two property chain axioms involving rico:Proxy to a few
                        object properties used to define sequences or
                     hierarchies</html:strong>.</html:li>
                  <html:li>2025, March 6th: added a new object property 'isOrWasActiveAtDate' and an
                     inverse.</html:li>
                  <html:li>2025, March 13: added French and Spanish labels to the object properties
                     that connect Date and Relation, and to the
                     isOrganicProvenanceDateOf/hasOrganicProvenanceDate properties. Fixed the domain
                     and a rdfs:subPropertyOf of isDateAssociatedWithRelation. Also added property
                     chain axioms to hasDerivationDate, hasMigrationDate and to their inverse
                     properties.</html:li>
                  <html:li>2025, April 2nd: reviewed the new properties for Proxies, hierarchies and
                     sequences. Fixed a few owl:inverseOf, owl:subPropertyOf and a property chain
                     axiom. Modified a few details in the rdfs:comment of those properties. Added
                     French and Spanish labels to these new properties.</html:li>
                  <html:li>2025, April 3rd: renamed the inverse property of 'isOrWasActiveAtDate',
                     adjusted the rdfs:comment of the two properties, added a chain property axiom
                     and French and Spanish labels.</html:li>
                  <html:li>2025, April 5th: <html:strong>added hasContentWhichRepresents and
                        hasContentWhichMainlyRepresents properties</html:strong>, with domain Record
                     or Record Part, and the inverse properties.</html:li>
                  <html:li>2025, April 6th: Added the sentimentOrEmotionExpressed datatype property,
                     with domain Record or Record Part. <html:strong>Added the object properties
                        needed to connect a Record Set, some or all of whose members have subject or
                        main subject a Thing, or represent a Thing, and this Thing, plus the inverse
                        properties</html:strong>. Adjusted the Spanish labels of several existing
                     object properties.</html:li>
                  <html:li>2025, April 8th: <html:strong>Added German labels to the 107 RiC-O
                        classes</html:strong>.</html:li>
                  <html:li>2025, May 12th: revised and updated the ontology metadata.</html:li>
                  <html:li>2025, May 14th: added a dcat:version to the two skos:ConceptScheme named
                     individuals.</html:li>
               </html:ul>
            </html:div>
         </html:div>
      """^^rdf:XMLLiteral .

:AccumulationRelation
    a owl:Class ;
    rdfs:comment """Connects at least one Record Resource or Instantiation to at least
         one Agent, when the Record Resource or Instantiation is or was accumulated by the Agent, be
         it intentionally (collecting it) or not (receiving it in the course of its activities). The
         Record Resource(s) or Instantiation(s) is the source of the Relation, and the Agent(s) is
         the target."""@en ;
    rdfs:isDefinedBy <https://www.ica.org/standards/RiC/ontology> ;
    rdfs:label "Accumulation Relation"@en, "Recordressource/Instanz-Akteur-Bestandsbildung"@de, "Relación de acumulación"@es, "Relation d’accumulation"@fr ;
    rdfs:subClassOf :OrganicProvenanceRelation, [
        a owl:Restriction ;
        owl:minQualifiedCardinality "1"^^xsd:nonNegativeInteger ;
        owl:onClass [
            a owl:Class ;
            owl:unionOf (:Instantiation
                :RecordResource
            )
        ] ;
        owl:onProperty :relationHasSource
    ], [
        a owl:Restriction ;
        owl:minQualifiedCardinality "1"^^xsd:nonNegativeInteger ;
        owl:onClass :Agent ;
        owl:onProperty :relationHasTarget
    ] ;
    owl:equivalentClass [
        a owl:Restriction ;
        owl:hasSelf true ;
        owl:onProperty :accumulationRelation_role
    ] ;
    skos:changeNote [
        dc:date "2025-04-08" ;
        rdf:value "Added a new rdfs:label in German."@en
    ], [
        dc:date "2023-12-06" ;
        rdf:value """Improved the description of the Relation class (rdfs:comment)
               by clearly specifying how it is directed."""@en
    ], [
        dc:date "2023-11-12" ;
        rdf:value """Aligned with RiC-CM 1.0: updated the description
               (rdfs:comment)."""@en
    ], [
        dc:date "2023-11-08" ;
        rdf:value """In order to get a system of rolified Relation classes: added an
               equivalentClass object property; replaced the specific object properties by the
               generic ones in the subClassOf declarations."""@en
    ], [
        dc:date "2023-11-02" ;
        rdf:value "Added a new rdfs:label in Spanish."@en
    ], [
        dc:date "2023-08-25" ;
        rdf:value "Added a new rdfs:label in French."@en
    ] ;
    :RiCCMCorrespondingComponent """Class implementation of RiC-R028 and RiC-R028i
         relations"""@en .

:Activity
    a owl:Class ;
    rdfs:comment "The doing of something for some human purpose."@en ;
    rdfs:isDefinedBy <https://www.ica.org/standards/RiC/ontology> ;
    rdfs:label "Actividad"@es, "Activity"@en, "Activité"@fr, "Aktivität"@de ;
    rdfs:subClassOf :Event ;
    skos:changeNote [
        dc:date "2025-04-08" ;
        rdf:value "Added a new rdfs:label in German."@en
    ], [
        dc:date "2023-11-02" ;
        rdf:value "Added a new rdfs:label in Spanish."@en
    ], [
        dc:date "2023-08-25" ;
        rdf:value "Added a new rdfs:label in French."@en
    ], [
        dc:date "2023-04-19" ;
        rdf:value "Removed the 0.2 existing unnecessary restriction."@en
    ], [
        dc:date "2020-10-23" ;
        rdf:value """Scope note: made separate paragraphs and updated. Objective: to
               make RiC-O compliant with RiC-CM v0.2."""@en
    ] ;
    skos:scopeNote """Activity is a kind of Event. Activity is specifically used to
         designate purposeful human activity. Activity may be understood from two perspectives.
         First it can be understood as leading to an end. The end is the purpose of the Activity, or
         why the Activity is performed. Second, it can be understood in terms of the processes that
         lead to achieving the end, how the end is realized through coordinated actions. Purpose and
         process are complementary understandings of Activity. Together the two perspectives address
         why the Activity is performed, the expected ends or outcomes; and how the Activity fulfills
         the purpose. While activity has an intended end, it also has unintended consequences and
         results, or side-effects. By and large, these may not be the focus of the description, but
         they are, unquestionably, context. |In a corporate or government context an Activity may
         also be called a 'function'. An Activity exists in a specific social and cultural context,
         and within that context is subject to change over time. An Activity may be composed of
         other Activities."""@en ;
    :RiCCMCorrespondingComponent """Corresponds to RiC-E15 (Activity
         entity)"""@en .

:ActivityDocumentationRelation
    a owl:Class ;
    rdfs:comment """Connects at least one Record Resource or Instantiation to at least
         one Activity, when the Record Resource or Instantiation results from the Activity. The
         Record Resource(s) or Instantiation(s) is the source of the Relation, and the
         Activity(-ies) is the target."""@en ;
    rdfs:isDefinedBy <https://www.ica.org/standards/RiC/ontology> ;
    rdfs:label "Activity Documentation Relation"@en, "Recordressource/Instanz-Aktivität"@de, "Relación de procedencia funcional"@es, "Relation entre activités et ressources archivistiques"@fr ;
    rdfs:subClassOf :EventRelation, :OrganicOrFunctionalProvenanceRelation, [
        a owl:Restriction ;
        owl:minQualifiedCardinality "1"^^xsd:nonNegativeInteger ;
        owl:onClass [
            a owl:Class ;
            owl:unionOf (:Instantiation
                :RecordResource
            )
        ] ;
        owl:onProperty :relationHasSource
    ], [
        a owl:Restriction ;
        owl:minQualifiedCardinality "1"^^xsd:nonNegativeInteger ;
        owl:onClass :Activity ;
        owl:onProperty :relationHasTarget
    ] ;
    owl:equivalentClass [
        a owl:Restriction ;
        owl:hasSelf true ;
        owl:onProperty :activityDocumentationRelation_role
    ] ;
    skos:changeNote [
        dc:date "2025-04-08" ;
        rdf:value "Added a new rdfs:label in German."@en
    ], [
        dc:date "2023-12-06" ;
        rdf:value """Improved the description of the Relation class (rdfs:comment)
               by clearly specifying how it is directed."""@en
    ], [
        dc:date "2023-11-12" ;
        rdf:value "Aligned with RiC-CM 1.0: updated the ."@en
    ], [
        dc:date "2023-11-08" ;
        rdf:value """In order to get a system of rolified Relation classes: added an
               equivalentClass object property; replaced the specific object properties by the
               generic ones in the subClassOf declarations."""@en
    ], [
        dc:date "2023-11-08" ;
        rdf:value "Made this relation a subclass of EventRelation."@en
    ], [
        dc:date "2023-11-02" ;
        rdf:value "Added a new rdfs:label in Spanish."@en
    ], [
        dc:date "2023-08-25" ;
        rdf:value "Added a new rdfs:label in French."@en
    ] ;
    :RiCCMCorrespondingComponent """Class implementation of RiC-R033 and RiC-R033
         relations"""@en .

:ActivityType
    a owl:Class ;
    rdfs:comment "Categorization of an Activity."@en ;
    rdfs:isDefinedBy <https://www.ica.org/standards/RiC/ontology> ;
    rdfs:label "Activity Type"@en, "Aktivitätskategorie"@de, "Tipo de actividad"@es, "Type d’activité"@fr ;
    rdfs:subClassOf :Type ;
    skos:changeNote [
        dc:date "2025-04-08" ;
        rdf:value "Added a new rdfs:label in German."@en
    ], [
        dc:date "2023-11-02" ;
        rdf:value "Added a new rdfs:label in Spanish."@en
    ], [
        dc:date "2023-08-25" ;
        rdf:value "Added a new rdfs:label in French."@en
    ], [
        dc:date "2023-04-19" ;
        rdf:value "Removed the 0.2 existing unnecessary restriction."@en
    ], [
        dc:date "2020-10-23" ;
        rdf:value """Scope note: updated (different from RiC-CM scope note).
               Objective: to make RiC-O compliant with RiC-CM v0.2."""@en
    ] ;
    skos:scopeNote """Can be extended with any number of subclasses, e.g.
         “function/action” and “activity domain”. This allows for a faceted approach that enables an
         Activity to be categorized using a combination of components, general or more specific. For
         example, “monitoring” can be used in combination with “election polls” or “water
         resources”."""@en ;
    :RiCCMCorrespondingComponent """Corresponds to RiC-A02 (Activity Type
         attribute)"""@en .

:Agent
    a owl:Class ;
    rdfs:comment """A Person, or Group, or an entity created by a Person or Group
         (Mechanism), or a Position, that acts in the world."""@en ;
    rdfs:isDefinedBy <https://www.ica.org/standards/RiC/ontology> ;
    rdfs:label "Agent"@en, "Agent"@fr, "Agente"@es, "Akteur"@de ;
    rdfs:subClassOf :Thing ;
    skos:changeNote [
        dc:date "2025-04-08" ;
        rdf:value "Added a new rdfs:label in German."@en
    ], [
        dc:date "2023-11-02" ;
        rdf:value "Added a new rdfs:label in Spanish."@en
    ], [
        dc:date "2023-08-25" ;
        rdf:value "Added a new rdfs:label in French."@en
    ], [
        dc:date "2021-02-08" ;
        rdf:value "removed the Restrictions"@en
    ], [
        dc:date "2020-10-23" ;
        rdf:value """Comment: updated. Scope note: updated and made several
               paragraphs. Objective: to make RiC-O compliant with RiC-CM v0.2."""@en
    ] ;
    skos:scopeNote """An Agent may have one or more identities; an identity is a
         constellation of properties or relations that together “identify” the Agent. A Person or
         Group commonly has one identity, though each also may have one or more alternative
         identities. Such alternative identities may be shared by more than one Person or Group.
         Alternative identities include but are not limited to pseudonyms, heteronyms, DBA (Doing
         Business As), and trade identities. An alternative identity should not be confused with a
         Position in a Group, for example, presidents, prime ministers, governors, popes, royalty,
         or bishops. Nor should an alternative identity be confused with a variant name or
         identifier of the same identity. Agent also includes entities created by a Person or Group
         that act on behalf of the creating Agent in an autonomous or semi-autonomous manner.
         Examples of a Mechanism include software agents, robots, and space and underwater probes
         that generate data (records) in the course of Activity assigned to and in conformance with
         the instructions given to them by the creating Person or Group."""@en ;
    :RiCCMCorrespondingComponent """Corresponds to RiC-E07 (Agent
         entity)"""@en .

:AgentControlRelation
    a owl:Class ;
    rdfs:comment """Connects at least one Agent, to at least another Agent, when the
         first one(s) control(s) or controlled in a way the activities of the second one(s). The
         Relation is oriented from the controlling agent to the controlled one: the controlling
         Agent(s) is the source of the Relation, and the controlled Agent(s) is the
         target."""@en ;
    rdfs:isDefinedBy <https://www.ica.org/standards/RiC/ontology> ;
    rdfs:label "Agent Control Relation"@en, "Akteur-Kontrolle-Akteur"@de, "Relación de control entre agentes"@es, "Relation de contrôle entre agents"@fr ;
    rdfs:subClassOf :AgentHierarchicalRelation, :AuthorityRelation, [
        a owl:Restriction ;
        owl:minQualifiedCardinality "1"^^xsd:nonNegativeInteger ;
        owl:onClass :Agent ;
        owl:onProperty :relationHasSource
    ], [
        a owl:Restriction ;
        owl:minQualifiedCardinality "1"^^xsd:nonNegativeInteger ;
        owl:onClass :Agent ;
        owl:onProperty :relationHasTarget
    ] ;
    owl:equivalentClass [
        a owl:Restriction ;
        owl:hasSelf true ;
        owl:onProperty :agentControlRelation_role
    ] ;
    skos:changeNote [
        dc:date "2025-04-08" ;
        rdf:value "Added a new rdfs:label in German."@en
    ], [
        dc:date "2023-12-06" ;
        rdf:value """Improved the description of the Relation class (rdfs:comment)
               by clearly specifying how it is directed."""@en
    ], [
        dc:date "2023-11-12" ;
        rdf:value """Aligned with RiC-CM 1.0: updated the description
               (rdfs:comment)."""@en
    ], [
        dc:date "2023-11-08" ;
        rdf:value """In order to get a system of rolified Relation classes: added an
               equivalentClass object property; replaced the specific object properties by the
               generic ones in the subClassOf declarations."""@en
    ], [
        dc:date "2023-11-02" ;
        rdf:value "Added a new rdfs:label in Spanish."@en
    ], [
        dc:date "2023-08-25" ;
        rdf:value "Added a new rdfs:label in French."@en
    ] ;
    :RiCCMCorrespondingComponent """Class implementation of RiC-R041 and RiC-R041i
         relations"""@en .

:AgentHierarchicalRelation
    a owl:Class ;
    rdfs:comment """Connects at least one Agent to at least another Agent, when the
         first one is or was hierarchically superior to the second one. The Relation is oriented
         towards the 'bottom' of the hierarchical tree: the superior Agent(s) is the source of the
         Relation, and the inferior Agent(s) is the target."""@en ;
    rdfs:isDefinedBy <https://www.ica.org/standards/RiC/ontology> ;
    rdfs:label "Agent Hierarchical Relation"@en, "Akteur-Hierarchie-Akteur"@de, "Relación jerárquica entre agentes"@es, "Relation hiérarchique entre agents"@fr ;
    rdfs:subClassOf :AgentToAgentRelation, [
        a owl:Restriction ;
        owl:minQualifiedCardinality "1"^^xsd:nonNegativeInteger ;
        owl:onClass :Agent ;
        owl:onProperty :relationHasSource
    ], [
        a owl:Restriction ;
        owl:minQualifiedCardinality "1"^^xsd:nonNegativeInteger ;
        owl:onClass :Agent ;
        owl:onProperty :relationHasTarget
    ] ;
    owl:equivalentClass [
        a owl:Restriction ;
        owl:hasSelf true ;
        owl:onProperty :agentHierarchicalRelation_role
    ] ;
    skos:changeNote [
        dc:date "2025-04-08" ;
        rdf:value "Added a new rdfs:label in German."@en
    ], [
        dc:date "2023-12-06" ;
        rdf:value """Improved the description of the Relation class (rdfs:comment)
               by clearly specifying how it is directed."""@en
    ], [
        dc:date "2023-11-12" ;
        rdf:value """Aligned with RiC-CM 1.0: updated the description
               (rdfs:comment), skos:scopeNote."""@en
    ], [
        dc:date "2023-11-08" ;
        rdf:value """In order to get a system of rolified Relation classes: added an
               equivalentClass object property; replaced the specific object properties by the
               generic ones in the subClassOf declarations."""@en
    ], [
        dc:date "2023-11-02" ;
        rdf:value "Added a new rdfs:label in Spanish."@en
    ], [
        dc:date "2023-08-25" ;
        rdf:value "Added a new rdfs:label in French."@en
    ] ;
    skos:scopeNote """The hierarchical relation can be an authority relation, or a
         whole/part relation between two agents."""@en ;
    :RiCCMCorrespondingComponent """Class implementation of RiC-R045 and RiC-R045i
         relations"""@en .

:AgentName
    a owl:Class ;
    rdfs:comment """A label, title or term designating an Agent in order to make it
         distinguishable from other similar entities."""@en ;
    rdfs:isDefinedBy <https://www.ica.org/standards/RiC/ontology> ;
    rdfs:label "Agent Name"@en, "Akteursname"@de, "Nom d’agent"@fr, "Nombre de Agente"@es ;
    rdfs:subClassOf :Name ;
    skos:changeNote [
        dc:date "2025-04-08" ;
        rdf:value "Added a new rdfs:label in German."@en
    ], [
        dc:date "2023-11-02" ;
        rdf:value "Added a new rdfs:label in Spanish."@en
    ], [
        dc:date "2023-08-25" ;
        rdf:value "Added a new rdfs:label in French."@en
    ] ;
    :RiCCMCorrespondingComponent """Class implementation of a specialization of RiC-A28
         (Name attribute)"""@en .

:AgentTemporalRelation
    a owl:Class ;
    rdfs:comment """Connects at least one Agent to at least another Agent that
         succeeds it chronologically for, for instance, fullfilling some functions or performing
         some activities. The Relation is oriented chronologically, from the predecessor to the
         successor: the predecessor Agent(s) is the source of the Relation, and the successor
         Agent(s) is the target."""@en ;
    rdfs:isDefinedBy <https://www.ica.org/standards/RiC/ontology> ;
    rdfs:label "Agent Temporal Relation"@en, "Akteur-Nachfolge"@de, "Relación temporal entre agentes"@es, "Relation temporelle entre agents"@fr ;
    rdfs:subClassOf :AgentToAgentRelation, :TemporalRelation, [
        a owl:Restriction ;
        owl:minQualifiedCardinality "1"^^xsd:nonNegativeInteger ;
        owl:onClass :Agent ;
        owl:onProperty :relationHasSource
    ], [
        a owl:Restriction ;
        owl:minQualifiedCardinality "1"^^xsd:nonNegativeInteger ;
        owl:onClass :Agent ;
        owl:onProperty :relationHasTarget
    ] ;
    owl:equivalentClass [
        a owl:Restriction ;
        owl:hasSelf true ;
        owl:onProperty :agentTemporalRelation_role
    ] ;
    skos:changeNote [
        dc:date "2025-04-08" ;
        rdf:value "Added a new rdfs:label in German."@en
    ], [
        dc:date "2023-12-06" ;
        rdf:value """Improved the description of the Relation class (rdfs:comment)
               by clearly specifying how it is directed."""@en
    ], [
        dc:date "2023-11-12" ;
        rdf:value """Aligned with RiC-CM 1.0: updated the
               skos:scopeNote."""@en
    ], [
        dc:date "2023-11-08" ;
        rdf:value """In order to get a system of rolified Relation classes: added an
               equivalentClass object property; replaced the specific object properties by the
               generic ones in the subClassOf declarations."""@en
    ], [
        dc:date "2023-11-02" ;
        rdf:value "Added a new rdfs:label in Spanish."@en
    ], [
        dc:date "2023-08-25" ;
        rdf:value "Added a new rdfs:label in French."@en
    ], [
        dc:date "2023-04-19" ;
        rdf:value "Removed the 0.2 existing unnecessary restriction."@en
    ] ;
    skos:scopeNote """There may be zero to many intermediate agents, ignored or
         unknown, between the two connected agents. Can be used when there is a transfer of function
         from the first agent to the second agent."""@en ;
    :RiCCMCorrespondingComponent """Class implementation of RiC-R016 and RiC-016i
         relations"""@en .

:AgentToAgentRelation
    a owl:Class ;
    rdfs:comment """Connects at least two Agents. This Relation is a generic, not
         oriented one."""@en ;
    rdfs:isDefinedBy <https://www.ica.org/standards/RiC/ontology> ;
    rdfs:label "Agent Relation"@en, "Akteur-Akteur"@de, "Relación entre agentes"@es, "Relation entre agents"@fr ;
    rdfs:subClassOf :Relation, [
        a owl:Restriction ;
        owl:minQualifiedCardinality "2"^^xsd:nonNegativeInteger ;
        owl:onClass :Agent ;
        owl:onProperty :relationConnects
    ] ;
    owl:equivalentClass [
        a owl:Restriction ;
        owl:hasSelf true ;
        owl:onProperty :agentToAgentRelation_role
    ] ;
    skos:changeNote [
        dc:date "2025-04-08" ;
        rdf:value "Added a new rdfs:label in German."@en
    ], [
        dc:date "2023-12-06" ;
        rdf:value """Improved the description of the Relation class (rdfs:comment)
               by clearly specifying how it is directed."""@en
    ], [
        dc:date "2023-11-12" ;
        rdf:value """Aligned with RiC-CM 1.0: updated the
               skos:scopeNote."""@en
    ], [
        dc:date "2023-11-08" ;
        rdf:value """In order to get a system of rolified Relation classes: added an
               equivalentClass object property; replaced the specific object properties by the
               generic ones in the subClassOf declarations."""@en
    ], [
        dc:date "2023-11-02" ;
        rdf:value "Added a new rdfs:label in Spanish."@en
    ], [
        dc:date "2023-08-25" ;
        rdf:value "Added a new rdfs:label in French."@en
    ] ;
    skos:scopeNote """Use only if it is not possible to specify a narrower agent to
         agent relation, for example a WorkRelation."""@en ;
    :RiCCMCorrespondingComponent """Class implementation of RiC-R044 and RiC-044i
         relations"""@en .

:Appellation
    a owl:Class ;
    rdfs:comment """A concept of any kind that is used for designating an Entity and
         referring to it."""@en ;
    rdfs:isDefinedBy <https://www.ica.org/standards/RiC/ontology> ;
    rdfs:label "Appellation"@en, "Appellation"@fr, "Bezeichnung"@de, "Denominación"@es ;
    rdfs:subClassOf :Concept ;
    skos:changeNote [
        dc:date "2025-04-08" ;
        rdf:value "Added a new rdfs:label in German."@en
    ], [
        dc:date "2023-11-02" ;
        rdf:value "Added a new rdfs:label in Spanish."@en
    ], [
        dc:date "2023-08-25" ;
        rdf:value "Added a new rdfs:label in French."@en
    ] .

:AppellationRelation
    a owl:Class ;
    rdfs:comment """Connects an Appellation and at least one Thing that the
         Appellation designates or designated. The Appellation is the source of the Relation and the
         Thing(s) is the target."""@en ;
    rdfs:isDefinedBy <https://www.ica.org/standards/RiC/ontology> ;
    rdfs:label "Appellation Relation"@en, "Bezeichnung-Ding"@de, "Relación de denominación"@es, "Relation d’appellation"@fr ;
    rdfs:subClassOf :Relation, [
        a owl:Restriction ;
        owl:onClass :Appellation ;
        owl:onProperty :relationHasSource ;
        owl:qualifiedCardinality "1"^^xsd:nonNegativeInteger
    ], [
        a owl:Restriction ;
        owl:minQualifiedCardinality "1"^^xsd:nonNegativeInteger ;
        owl:onClass :Thing ;
        owl:onProperty :relationHasTarget
    ] ;
    owl:equivalentClass [
        a owl:Restriction ;
        owl:hasSelf true ;
        owl:onProperty :appellationRelation_role
    ] ;
    skos:changeNote [
        dc:date "2025-04-08" ;
        rdf:value "Added a new rdfs:label in German."@en
    ], [
        dc:date "2023-12-06" ;
        rdf:value """Improved the description of the Relation class (rdfs:comment)
               by clearly specifying how it is directed."""@en
    ], [
        dc:date "2023-11-12" ;
        rdf:value """Aligned with RiC-CM 1.0: updated the description
               (rdfs:comment)."""@en
    ], [
        dc:date "2023-11-08" ;
        rdf:value """In order to get a system of rolified Relation classes: added an
               equivalentClass object property; replaced the specific object properties by the
               generic ones in the subClassOf declarations."""@en
    ], [
        dc:date "2023-11-02" ;
        rdf:value "Added a new rdfs:label in Spanish."@en
    ], [
        dc:date "2023-08-25" ;
        rdf:value "Added a new rdfs:label in French."@en
    ] .

:AuthorityRelation
    a owl:Class ;
    rdfs:comment """Connects at least one Agent and at least one Thing over which the
         Agent has or had some authority. The Agent(s) is the source of the relation, and the
         Thing(s) is the target."""@en ;
    rdfs:isDefinedBy <https://www.ica.org/standards/RiC/ontology> ;
    rdfs:label "Akteur-Autorität-Ding"@de, "Authority Relation"@en, "Relación de control por parte de agentes"@es, "Relation d’autorité"@fr ;
    rdfs:subClassOf :Relation, [
        a owl:Restriction ;
        owl:minQualifiedCardinality "1"^^xsd:nonNegativeInteger ;
        owl:onClass :Agent ;
        owl:onProperty :relationHasSource
    ], [
        a owl:Restriction ;
        owl:minQualifiedCardinality "1"^^xsd:nonNegativeInteger ;
        owl:onClass :Thing ;
        owl:onProperty :relationHasTarget
    ] ;
    owl:equivalentClass [
        a owl:Restriction ;
        owl:hasSelf true ;
        owl:onProperty :authorityRelation_role
    ] ;
    skos:changeNote [
        dc:date "2025-04-08" ;
        rdf:value "Added a new rdfs:label in German."@en
    ], [
        dc:date "2023-12-06" ;
        rdf:value """Improved the description of the Relation class (rdfs:comment)
               by clearly specifying how it is directed."""@en
    ], [
        dc:date "2023-11-12" ;
        rdf:value """Aligned with RiC-CM 1.0: updated the description
               (rdfs:comment), skos:scopeNote."""@en
    ], [
        dc:date "2023-11-08" ;
        rdf:value """In order to get a system of rolified Relation classes: added an
               equivalentClass object property; replaced the specific object properties by the
               generic ones in the subClassOf declarations."""@en
    ], [
        dc:date "2023-11-02" ;
        rdf:value "Added a new rdfs:label in Spanish."@en
    ], [
        dc:date "2023-08-25" ;
        rdf:value "Added a new rdfs:label in French."@en
    ] ;
    skos:scopeNote """Use only if it is not possible to specify a narrower authority
         relation, for example OwnershipRelation."""@en ;
    :RiCCMCorrespondingComponent """Class implementation of RiC-R036 and RiC-R036i
         relations"""@en .

:AuthorshipRelation
    a owl:Class ;
    rdfs:comment """Connects at least one Record to at least one Person, Group or
         Position that is or was responsible for conceiving and formulating the information
         contained in the Record. The Record is the source of the Relation and the Person(s),
         Group(s) or Position(s) is the target. """@en ;
    rdfs:isDefinedBy <https://www.ica.org/standards/RiC/ontology> ;
    rdfs:label "Authorship Relation"@en, "Record-Autor-Akteur"@de, "Relación de autoría"@es, "Relation de responsabilité intellectuelle"@fr ;
    rdfs:subClassOf :CreationRelation, [
        a owl:Restriction ;
        owl:minQualifiedCardinality "1"^^xsd:nonNegativeInteger ;
        owl:onClass :Record ;
        owl:onProperty :relationHasSource
    ], [
        a owl:Restriction ;
        owl:minQualifiedCardinality "1"^^xsd:nonNegativeInteger ;
        owl:onClass [
            a owl:Class ;
            owl:unionOf (:Group
                :Person
                :Position
            )
        ] ;
        owl:onProperty :relationHasTarget
    ] ;
    owl:equivalentClass [
        a owl:Restriction ;
        owl:hasSelf true ;
        owl:onProperty :authorshipRelation_role
    ] ;
    skos:changeNote [
        dc:date "2025-04-08" ;
        rdf:value "Added a new rdfs:label in German."@en
    ], [
        dc:date "2023-12-06" ;
        rdf:value """Improved the description of the Relation class (rdfs:comment)
               by clearly specifying how it is directed."""@en
    ], [
        dc:date "2023-11-12" ;
        rdf:value """Aligned with RiC-CM 1.0: updated the description
               (rdfs:comment), skos:scopeNote."""@en
    ], [
        dc:date "2023-11-08" ;
        rdf:value """In order to get a system of rolified Relation classes: added an
               equivalentClass object property; replaced the specific object properties by the
               generic ones in the subClassOf declarations."""@en
    ], [
        dc:date "2023-11-02" ;
        rdf:value "Added a new rdfs:label in Spanish."@en
    ], [
        dc:date "2023-08-25" ;
        rdf:value "Added a new rdfs:label in French."@en
    ], [
        dc:date "2020-12-29" ;
        rdf:value """Created following the addition of RiC-R079 relation in RiC-CM
               0.2"""@en
    ] ;
    skos:scopeNote """To be used for a person, group or position that makes any
         contribution to the content of a record. Includes the person, group or position in whose
         name or by whose command the content may have been formulated and first instantiated (for
         example the person who signed the record). """@en ;
    :RiCCMCorrespondingComponent """Class implementation of RiC-R079 and RiC-R079i
         relations"""@en .

:CarrierExtent
    a owl:Class ;
    rdfs:comment """Number of physical units and/or physical dimensions of the carrier
         of an Instantiation."""@en ;
    rdfs:isDefinedBy <https://www.ica.org/standards/RiC/ontology> ;
    rdfs:label "Carrier Extent"@en, "Datenträgerumfang"@de, "Extensión del soporte"@es, "Mesure d’un support"@fr ;
    rdfs:subClassOf :Extent ;
    skos:changeNote [
        dc:date "2025-04-08" ;
        rdf:value "Added a new rdfs:label in German."@en
    ], [
        dc:date "2023-11-12" ;
        rdf:value """Aligned with RiC-CM 1.0: updated the description
               (rdfs:comment), skos:scopeNote."""@en
    ], [
        dc:date "2023-11-02" ;
        rdf:value "Added a new rdfs:label in Spanish."@en
    ], [
        dc:date "2023-08-25" ;
        rdf:value "Added a new rdfs:label in French."@en
    ], [
        dc:date "2020-11-21" ;
        rdf:value """Changed a bit the definition and added change
               notes."""@en
    ], [
        dc:date "2020-10-28" ;
        rdf:value """Class added in order to handle an accurate description of a
               carrier extent"""@en
    ] ;
    skos:scopeNote """In order to manage an instantiation of a record resource it is
         necessary to note the extent of the carrier as well as that of the instantiation itself.
         Whether it is necessary to note dimensions, the number of relevant units or both depends on
         the nature of the carrier and particular business needs."""@en ;
    :RiCCMCorrespondingComponent """Class implementation of RiC-A04 (Carrier Extent)
         attribute"""@en .

:CarrierType
    a owl:Class ;
    rdfs:comment """Categorization of physical material on which information is
         represented."""@en ;
    rdfs:isDefinedBy <https://www.ica.org/standards/RiC/ontology> ;
    rdfs:label "Carrier Type"@en, "Datenträgerkategorie"@de, "Tipo de soporte"@es, "Type de support"@fr ;
    rdfs:subClassOf :Type ;
    skos:changeNote [
        dc:date "2025-04-08" ;
        rdf:value "Added a new rdfs:label in German."@en
    ], [
        dc:date "2023-11-12" ;
        rdf:value """Aligned with RiC-CM 1.0: updated the description
               (rdfs:comment), skos:scopeNote."""@en
    ], [
        dc:date "2023-11-02" ;
        rdf:value "Added a new rdfs:label in Spanish."@en
    ], [
        dc:date "2023-08-25" ;
        rdf:value "Added a new rdfs:label in French."@en
    ], [
        dc:date "2023-04-19" ;
        rdf:value "Removed the 0.2 existing unnecessary restriction."@en
    ], [
        dc:date "2020-10-23" ;
        rdf:value """Scope note: updated (quite the same as RiC-CM definition).
               Objective: to make RiC-O compliant with RiC-CM v0.2."""@en
    ] ;
    skos:scopeNote """In order to manage an instantiation of a record resource, it is
         necessary to note the type of carrier on which the record resource is instantiated as its
         nature will determine the environmental storage conditions and the prerequisites for and
         possible ways of accessing and using the record resource."""@en ;
    :RiCCMCorrespondingComponent """Corresponds to RiC-A05 (Carrier Type
         attribute)"""@en .

:ChildRelation
    a owl:Class ;
    rdfs:comment """Connects at least one Person to at least another Person, when the
         first has(ave) child(s) the second one(s). The Relation is oriented from the parent to the
         child: the parent is the source of the relation, and the child(ren) is the
         target."""@en ;
    rdfs:isDefinedBy <https://www.ica.org/standards/RiC/ontology> ;
    rdfs:label "Child Relation"@en, "Person-Kind"@de, "Relación de filiación"@es, "Relation de filiation"@fr ;
    rdfs:subClassOf :DescendanceRelation, [
        a owl:Restriction ;
        owl:minQualifiedCardinality "1"^^xsd:nonNegativeInteger ;
        owl:onClass :Person ;
        owl:onProperty :relationHasSource
    ], [
        a owl:Restriction ;
        owl:minQualifiedCardinality "1"^^xsd:nonNegativeInteger ;
        owl:onClass :Person ;
        owl:onProperty :relationHasTarget
    ] ;
    owl:equivalentClass [
        a owl:Restriction ;
        owl:hasSelf true ;
        owl:onProperty :childRelation_role
    ] ;
    skos:changeNote [
        dc:date "2025-04-08" ;
        rdf:value "Added a new rdfs:label in German."@en
    ], [
        dc:date "2023-12-06" ;
        rdf:value """Improved the description of the Relation class (rdfs:comment)
               by clearly specifying how it is directed."""@en
    ], [
        dc:date "2023-11-12" ;
        rdf:value """Aligned with RiC-CM 1.0: updated the description
               (rdfs:comment)."""@en
    ], [
        dc:date "2023-11-08" ;
        rdf:value """In order to get a system of rolified Relation classes: added an
               equivalentClass object property; replaced the specific object properties by the
               generic ones in the subClassOf declarations."""@en
    ], [
        dc:date "2023-11-02" ;
        rdf:value "Added a new rdfs:label in Spanish."@en
    ], [
        dc:date "2023-08-25" ;
        rdf:value "Added a new rdfs:label in French."@en
    ] ;
    :RiCCMCorrespondingComponent """Class implementation of RiC-R018 and RiC-R018i
         relations"""@en .

:Concept
    a owl:Class ;
    rdfs:comment """An idea, unit of thought, abstract cultural object or
         category"""@en ;
    rdfs:isDefinedBy <https://www.ica.org/standards/RiC/ontology> ;
    rdfs:label "Concept"@en, "Concept"@fr, "Concepto"@es, "Konzept"@de ;
    rdfs:subClassOf :Thing ;
    skos:changeNote [
        dc:date "2025-04-08" ;
        rdf:value "Added a new rdfs:label in German."@en
    ], [
        dc:date "2023-11-02" ;
        rdf:value "Added a new rdfs:label in Spanish."@en
    ], [
        dc:date "2023-08-25" ;
        rdf:value "Added a new rdfs:label in French."@en
    ] .

:ContentType
    a owl:Class ;
    rdfs:comment """The fundamental form of communication in which a Record or Record
         Part is expressed."""@en ;
    rdfs:isDefinedBy <https://www.ica.org/standards/RiC/ontology> ;
    rdfs:label "Content Type"@en, "Inhaltskategorie"@de, "Tipo de contenido"@es, "Type de contenu"@fr ;
    rdfs:subClassOf :Type ;
    skos:changeNote [
        dc:date "2025-04-08" ;
        rdf:value "Added a new rdfs:label in German."@en
    ], [
        dc:date "2023-11-12" ;
        rdf:value """Aligned with RiC-CM 1.0: updated the description
               (rdfs:comment), skos:scopeNote."""@en
    ], [
        dc:date "2023-11-02" ;
        rdf:value "Added a new rdfs:label in Spanish."@en
    ], [
        dc:date "2023-08-25" ;
        rdf:value "Added a new rdfs:label in French."@en
    ], [
        dc:date "2023-04-19" ;
        rdf:value "Removed the 0.2 existing unnecessary restriction."@en
    ], [
        dc:date "2020-10-23" ;
        rdf:value """Scope note: added (quite the same as RiC-CM
               definition)."""@en
    ] ;
    skos:scopeNote """Content Type should not be confused with Representation Type or
         Carrier Type that would concern a related Instantiation since the form of communication can
         be independent of the representation or carrier, for example a map (content type
         \"cartographic image\") may be represented as a sketch (representation type \"visual\")
         recorded as a physical document (carrier type \"paper\"). It also should not be confused with
         the Documentary Form Type of a Record, or Record Part, which describes a specific document
         form (for example a deed of sale)."""@en ;
    :RiCCMCorrespondingComponent """Corresponds to RiC-A10 (Content Type
         attribute)"""@en .

:Coordinates
    a owl:Class ;
    rdfs:comment """Longitudinal and latitudinal information about a
         Place."""@en ;
    rdfs:isDefinedBy <https://www.ica.org/standards/RiC/ontology> ;
    rdfs:label "Coordenadas de lugar"@es, "Coordinates"@en, "Coordonnées géographiques"@fr, "Koordinaten"@de ;
    rdfs:subClassOf :Thing ;
    skos:changeNote [
        dc:date "2025-04-08" ;
        rdf:value "Added a new rdfs:label in German."@en
    ], [
        dc:date "2023-11-12" ;
        rdf:value """Aligned with RiC-CM 1.0: updated the description
               (rdfs:comment)."""@en
    ], [
        dc:date "2023-11-02" ;
        rdf:value "Added a new rdfs:label in Spanish."@en
    ], [
        dc:date "2023-08-25" ;
        rdf:value "Added a new rdfs:label in French."@en
    ], [
        dc:date "2023-04-19" ;
        rdf:value "Removed the 0.2 existing unnecessary restriction."@en
    ], [
        dc:date "2021-02-08" ;
        rdf:value """Removed the cardinality Restrictions when the range is a
               datatype property"""@en
    ] ;
    :RiCCMCorrespondingComponent """Class implementation of RiC-A11 (Coordinates
         attribute)"""@en .

:CorporateBody
    a owl:Class ;
    rdfs:comment """An organized group of persons that act together as an Agent, and
         that has a recognized legal or social status."""@en ;
    rdfs:isDefinedBy <https://www.ica.org/standards/RiC/ontology> ;
    rdfs:label "Collectivité"@fr, "Corporate Body"@en, "Institución"@es, "Körperschaft"@de ;
    rdfs:subClassOf :Group ;
    skos:changeNote [
        dc:date "2025-04-08" ;
        rdf:value "Added a new rdfs:label in German."@en
    ], [
        dc:date "2023-11-12" ;
        rdf:value """Aligned with RiC-CM 1.0: updated the description
               (rdfs:comment), skos:scopeNote."""@en
    ], [
        dc:date "2023-11-02" ;
        rdf:value "Added a new rdfs:label in Spanish."@en
    ], [
        dc:date "2023-08-25" ;
        rdf:value "Added a new rdfs:label in French."@en
    ], [
        dc:date "2023-08-25" ;
        rdf:value "Added a new rdfs:label in French."@en
    ], [
        dc:date "2020-10-23" ;
        rdf:value """scope note: updated. Objective: to make RiC-O compliant with
               RiC-CM v0.2."""@en
    ] ;
    skos:scopeNote """Corporate body is a kind of Group (RiC-E09). By exception,
         within some legal contexts, a sole trader or sole proprietor may be recognized as a
         corporate body, even when the economic enterprise does not have additional members.
         Corporate bodies often have a mandate giving them the authority to act within their area(s)
         of competence. They will also usually act within a particular jurisdiction being governed
         by legal and other rule-based frameworks. A corporate body though may be constituted in a
         more informal manner and exist as an entity by virtue of its recognition as such by its
         members."""@en ;
    :RiCCMCorrespondingComponent """Corresponds to RiC-E11 (Corporate Body
         entity)"""@en .

:CorporateBodyType
    a owl:Class ;
    rdfs:comment "Categorization of a Corporate Body."@en ;
    rdfs:isDefinedBy <https://www.ica.org/standards/RiC/ontology> ;
    rdfs:label "Corporate Body Type"@en, "Körperschaftskategorie"@de, "Tipo de institución"@es, "Type de collectivité"@fr ;
    rdfs:subClassOf :Type ;
    skos:changeNote [
        dc:date "2025-04-08" ;
        rdf:value "Added a new rdfs:label in German."@en
    ], [
        dc:date "2023-11-02" ;
        rdf:value "Added a new rdfs:label in Spanish."@en
    ], [
        dc:date "2023-08-25" ;
        rdf:value "Added a new rdfs:label in French."@en
    ], [
        dc:date "2023-04-19" ;
        rdf:value "Removed the 0.2 existing unnecessary restriction."@en
    ] ;
    :RiCCMCorrespondingComponent """Corresponds to RiC-A12 (Corporate Body Type
         attribute)"""@en .

:CorrespondenceRelation
    a owl:Class ;
    rdfs:comment """Connects at least two Persons, when they correspond or
         corresponded to each other. This Relation is not oriented."""@en ;
    rdfs:isDefinedBy <https://www.ica.org/standards/RiC/ontology> ;
    rdfs:label "Correspondence Relation"@en, "Person-Korrespondenz-Person"@de, "Relación entre personas por correspondencia"@es, "Relation épistolaire"@fr ;
    rdfs:subClassOf :KnowingRelation, [
        a owl:Restriction ;
        owl:minQualifiedCardinality "2"^^xsd:nonNegativeInteger ;
        owl:onClass :Person ;
        owl:onProperty :relationConnects
    ] ;
    owl:equivalentClass [
        a owl:Restriction ;
        owl:hasSelf true ;
        owl:onProperty :correspondenceRelation_role
    ] ;
    skos:changeNote [
        dc:date "2025-04-08" ;
        rdf:value "Added a new rdfs:label in German."@en
    ], [
        dc:date "2023-12-06" ;
        rdf:value """Improved the description of the Relation class (rdfs:comment)
               by clearly specifying how it is directed."""@en
    ], [
        dc:date "2023-11-12" ;
        rdf:value """Aligned with RiC-CM 1.0: updated the description
               (rdfs:comment)."""@en
    ], [
        dc:date "2023-11-08" ;
        rdf:value """In order to get a system of rolified Relation classes: added an
               equivalentClass object property; replaced the specific object properties by the
               generic ones in the subClassOf declarations."""@en
    ], [
        dc:date "2023-11-02" ;
        rdf:value "Added a new rdfs:label in Spanish."@en
    ], [
        dc:date "2023-08-25" ;
        rdf:value "Added a new rdfs:label in French."@en
    ] ;
    :RiCCMCorrespondingComponent """Class implementation of RiC-R052 and Ri052i
         relations"""@en .

:CreationRelation
    a owl:Class ;
    rdfs:comment """Connects at least one Record Resource or Instantiation to at least
         one Agent, when the Agent is either responsible for all or some of the content of the
         Record Resource, or is a contributor to the genesis or production of the Instantiation. The
         Record Resource or Instantiation is the source of the Relation, and the Agent(s) is the
         target. """@en ;
    rdfs:isDefinedBy <https://www.ica.org/standards/RiC/ontology> ;
    rdfs:label "Creation Relation"@en, "Recordressource/Instanz-Erstellung-Akteur"@de, "Relación de creación"@es, "Relation de création"@fr ;
    rdfs:subClassOf :OrganicProvenanceRelation, [
        a owl:Restriction ;
        owl:minQualifiedCardinality "1"^^xsd:nonNegativeInteger ;
        owl:onClass [
            a owl:Class ;
            owl:unionOf (:Instantiation
                :RecordResource
            )
        ] ;
        owl:onProperty :relationHasSource
    ], [
        a owl:Restriction ;
        owl:minQualifiedCardinality "1"^^xsd:nonNegativeInteger ;
        owl:onClass :Agent ;
        owl:onProperty :relationHasTarget
    ] ;
    owl:equivalentClass [
        a owl:Restriction ;
        owl:hasSelf true ;
        owl:onProperty :creationRelation_role
    ] ;
    skos:changeNote [
        dc:date "2025-04-08" ;
        rdf:value "Added a new rdfs:label in German."@en
    ], [
        dc:date "2023-12-06" ;
        rdf:value """Improved the description of the Relation class (rdfs:comment)
               by clearly specifying how it is directed."""@en
    ], [
        dc:date "2023-11-12" ;
        rdf:value """Aligned with RiC-CM 1.0: updated the
               skos:scopeNote."""@en
    ], [
        dc:date "2023-11-08" ;
        rdf:value """In order to get a system of rolified Relation classes: added an
               equivalentClass object property; replaced the specific object properties by the
               generic ones in the subClassOf declarations."""@en
    ], [
        dc:date "2023-11-02" ;
        rdf:value "Added a new rdfs:label in Spanish."@en
    ], [
        dc:date "2023-08-25" ;
        rdf:value "Added a new rdfs:label in French."@en
    ], [
        dc:date "2023-04-19" ;
        rdf:value "Removed a 0.2 existing unnecessary restriction."@en
    ] ;
    skos:scopeNote """Covers the definition of \"author\" in diplomatics, and any agent
         that makes a contribution to the intellectual content of a record resource. Can also be
         used for any agent that was involved in the genesis (e.g. with the role of witness,
         representative of the author etc.) or in the production (e.g. with the role of scribe,
         secretary, notary, printer etc.) of the record resource or instantiation."""@en ;
    :RiCCMCorrespondingComponent """Class implementation of RiC-R027 and RiC-R027i
         relations"""@en .

:Date
    a owl:Class ;
    rdfs:comment """Chronological information associated with an entity that
         contributes to its identification and contextualization."""@en ;
    rdfs:isDefinedBy <https://www.ica.org/standards/RiC/ontology> ;
    rdfs:label "Date"@en, "Date"@fr, "Datum"@de, "Fecha"@es ;
    rdfs:subClassOf :Thing ;
    skos:changeNote [
        dc:date "2025-04-08" ;
        rdf:value "Added a new rdfs:label in German."@en
    ], [
        dc:date "2023-11-12" ;
        rdf:value """Aligned with RiC-CM 1.0: updated the
               skos:scopeNote."""@en
    ], [
        dc:date "2023-11-02" ;
        rdf:value "Added a new rdfs:label in Spanish."@en
    ], [
        dc:date "2023-08-25" ;
        rdf:value "Added a new rdfs:label in French."@en
    ], [
        dc:date "2020-10-23" ;
        rdf:value "Scope note: made separate paragraphs."@en
    ] ;
    skos:scopeNote """A Date may be represented in natural language, based on a
         digital standard, or both. Digital standard dates will typically be based on ISO 8601, or
         Extended Date-Time Format (EDTF)"""@en ;
    :RiCCMCorrespondingComponent """Corresponds to RiC-E18 (Date
         entity)"""@en .

:DateType
    a owl:Class ;
    rdfs:comment "Categorization of a Date."@en ;
    rdfs:isDefinedBy <https://www.ica.org/standards/RiC/ontology> ;
    rdfs:label "Date Type"@en, "Datumskategorie"@de, "Tipo de fecha"@es, "Type de date"@fr ;
    rdfs:subClassOf :Type ;
    skos:changeNote [
        dc:date "2025-04-08" ;
        rdf:value "Added a new rdfs:label in German."@en
    ], [
        dc:date "2023-11-12" ;
        rdf:value """Aligned with RiC-CM 1.0: updated the description
               (rdfs:comment), skos:scopeNote. Added a label in Spanish."""@en
    ], [
        dc:date "2023-10-10" ;
        rdf:value """Added the rdfs:comment, a French rdfs:label, and adjusted the
               rico:RiCCMCorrespondingComponent annotation."""@en
    ], [
        dc:date "2023-09-22" ;
        rdf:value "Added in RiC-O 1.0."@en
    ] ;
    skos:scopeNote """May be used to categorize a Date as a single date, a date range
         or a date set or sub-categories of these broad types. This attribute should not be confused
         with the date relations defined to connect a Date entity and any other entity (such as
         RiC-R069 ‘is beginning date of’)."""@en ;
    :RiCCMCorrespondingComponent """Corresponds to RiC-A42 (Date Type attribute) (new
         in RiC-CM 1.0)."""@en .

:DemographicGroup
    a owl:Class ;
    rdfs:comment """Categorization of a Person or Group based on shared
         characteristics."""@en ;
    rdfs:isDefinedBy <https://www.ica.org/standards/RiC/ontology> ;
    rdfs:label "Demographic Group"@en, "Demographische Gruppe"@de, "Groupe démographique"@fr, "Grupo demográfico"@es ;
    rdfs:subClassOf :Type ;
    skos:changeNote [
        dc:date "2025-04-08" ;
        rdf:value "Added a new rdfs:label in German."@en
    ], [
        dc:date "2024-10-10" ;
        rdf:value """Changed the French and Spanish labels (replaced 'catégorie' and
               'categoria' with 'groupe' and 'grupo')."""@en
    ], [
        dc:date "2023-11-12" ;
        rdf:value """Aligned with RiC-CM 1.0: updated the description
               (rdfs:comment), skos:scopeNote."""@en
    ], [
        dc:date "2023-11-02" ;
        rdf:value "Added a new rdfs:label in Spanish."@en
    ], [
        dc:date "2023-08-25" ;
        rdf:value "Added a new rdfs:label in French."@en
    ], [
        dc:date "2021-02-08" ;
        rdf:value "Removed the Restriction."@en
    ], [
        dc:date "2020-10-23" ;
        rdf:value """Comment: updated. Scope note: updated and made several
               paragraphs. Objective: to make RiC-O compliant with RiC-CM v0.2."""@en
    ] ;
    skos:scopeNote """Can be extended with any number of specific subclasses. Among
         possible specific demographic groups are gender, (biological) sex, education, identity,
         place, ancestry, ethnic/cultural identification, and religion."""@en ;
    :RiCCMCorrespondingComponent """Corresponds to RiC-A15 (Demographic Group
         attribute)"""@en .

:DerivationRelation
    a owl:Class ;
    rdfs:comment """Connects an Instantiation to at least one Instantiation that is
         derived from it, whether it exists or has been lost or destroyed. The Relation is oriented
         chronologically, from the first Instantiation in time to the derived Instantiation: the
         first Instantiation is the source of the Relation, and the derived Instantiation(s) is the
         target."""@en ;
    rdfs:isDefinedBy <https://www.ica.org/standards/RiC/ontology> ;
    rdfs:label "Derivation Relation"@en, "Instanz-Derivat-Instanz"@de, "Relación de derivación"@es, "Relation de dérivation"@fr ;
    rdfs:subClassOf :InstantiationToInstantiationRelation, :TemporalRelation, [
        a owl:Restriction ;
        owl:onClass :Instantiation ;
        owl:onProperty :relationHasSource ;
        owl:qualifiedCardinality "1"^^xsd:nonNegativeInteger
    ], [
        a owl:Restriction ;
        owl:minQualifiedCardinality "1"^^xsd:nonNegativeInteger ;
        owl:onClass :Instantiation ;
        owl:onProperty :relationHasTarget
    ] ;
    owl:equivalentClass [
        a owl:Restriction ;
        owl:hasSelf true ;
        owl:onProperty :derivationRelation_role
    ] ;
    skos:changeNote [
        dc:date "2025-04-08" ;
        rdf:value "Added a new rdfs:label in German."@en
    ], [
        dc:date "2023-12-06" ;
        rdf:value """Improved the description of the Relation class (rdfs:comment)
               by clearly specifying how it is directed."""@en
    ], [
        dc:date "2023-11-12" ;
        rdf:value """Aligned with RiC-CM 1.0: updated the description
               (rdfs:comment), skos:scopeNote."""@en
    ], [
        dc:date "2023-11-08" ;
        rdf:value """In order to get a system of rolified Relation classes: added an
               equivalentClass object property; replaced the specific object properties by the
               generic ones in the subClassOf declarations."""@en
    ], [
        dc:date "2023-11-02" ;
        rdf:value "Added a new rdfs:label in Spanish."@en
    ], [
        dc:date "2023-08-25" ;
        rdf:value "Added a new rdfs:label in French."@en
    ] ;
    skos:scopeNote """In some situations, it may be useful or necessary to connect an
         instantiation to an instantiation that was derived from it but no longer exists or has been
         lost."""@en ;
    :RiCCMCorrespondingComponent """Class implementation of RiC-R014 and RiR014i
         relations"""@en .

:DescendanceRelation
    a owl:Class ;
    rdfs:comment """Connects at least one Person to at least another Person, when the
         first has/have descendant the second one(s). The Relation is oriented from the ascendant to
         the descendant: the ascendant Person(s) is the source of the Relation, and the descendant
         Person(s) is the target."""@en ;
    rdfs:isDefinedBy <https://www.ica.org/standards/RiC/ontology> ;
    rdfs:label "Descendance Relation"@en, "Person-Nachkommen"@de, "Relación de descendencia"@es, "Relation de descendance"@fr ;
    rdfs:subClassOf :AgentTemporalRelation, :FamilyRelation, [
        a owl:Restriction ;
        owl:minQualifiedCardinality "1"^^xsd:nonNegativeInteger ;
        owl:onClass :Person ;
        owl:onProperty :relationHasSource
    ], [
        a owl:Restriction ;
        owl:minQualifiedCardinality "1"^^xsd:nonNegativeInteger ;
        owl:onClass :Person ;
        owl:onProperty :relationHasTarget
    ] ;
    owl:equivalentClass [
        a owl:Restriction ;
        owl:hasSelf true ;
        owl:onProperty :descendanceRelation_role
    ] ;
    skos:changeNote [
        dc:date "2025-04-08" ;
        rdf:value "Added a new rdfs:label in German."@en
    ], [
        dc:date "2023-12-06" ;
        rdf:value """Improved the description of the Relation class (rdfs:comment)
               by clearly specifying how it is directed."""@en
    ], [
        dc:date "2023-11-08" ;
        rdf:value """In order to get a system of rolified Relation classes: added an
               equivalentClass object property; replaced the specific object properties by the
               generic ones in the subClassOf declarations."""@en
    ], [
        dc:date "2023-11-02" ;
        rdf:value "Added a new rdfs:label in Spanish."@en
    ], [
        dc:date "2023-08-25" ;
        rdf:value "Added a new rdfs:label in French."@en
    ] ;
    :RiCCMCorrespondingComponent """Class implementation of RiC-R017 and RiC-R017i
         relations"""@en .

:DocumentaryFormType
    a owl:Class ;
    rdfs:comment """Categorization of a Record or Record Part with respect to its
         extrinsic and intrinsic elements that together communicate its content, administrative and
         documentary context, and authority."""@en ;
    rdfs:isDefinedBy <https://www.ica.org/standards/RiC/ontology> ;
    rdfs:label "Documentary Form Type"@en, "Dokumentenkategorie"@de, "Tipo documental"@es, "Type de document"@fr ;
    rdfs:subClassOf :Type ;
    skos:changeNote [
        dc:date "2025-04-08" ;
        rdf:value "Added a new rdfs:label in German."@en
    ], [
        dc:date "2023-11-12" ;
        rdf:value """Aligned with RiC-CM 1.0: updated the description
               (rdfs:comment)."""@en
    ], [
        dc:date "2023-11-02" ;
        rdf:value "Added a new rdfs:label in Spanish."@en
    ], [
        dc:date "2023-08-25" ;
        rdf:value "Added a new rdfs:label in French."@en
    ], [
        dc:date "2023-04-19" ;
        rdf:value "Removed the 0.2 existing unnecessary restriction."@en
    ], [
        dc:date "2020-10-23" ;
        rdf:value """Comment: updated. Scope note: made several paragraphs.
               Objective: to make RiC-O compliant with RiC-CM v0.2."""@en
    ] ;
    skos:scopeNote """Documentary Form Type plays an important role in determining the
         type of information a Record may comprise, its status of perfection, and its authenticity
         and reliability. Documentary form types exist in a specific social and cultural context,
         and within that context, are subject to change over time."""@en ;
    :RiCCMCorrespondingComponent """Corresponds to RiC-A17 (Documentary Form Type
         attribute)"""@en .

:Event
    a owl:Class ;
    rdfs:comment "Something that happens or occurs in time and space."@en ;
    rdfs:isDefinedBy <https://www.ica.org/standards/RiC/ontology> ;
    rdfs:label "Ereignis"@de, "Event"@en, "Evento"@es, "Événement"@fr ;
    rdfs:subClassOf :Thing ;
    skos:changeNote [
        dc:date "2025-04-08" ;
        rdf:value "Added a new rdfs:label in German."@en
    ], [
        dc:date "2023-11-12" ;
        rdf:value """Aligned with RiC-CM 1.0: updated the description
               (rdfs:comment), skos:scopeNote."""@en
    ], [
        dc:date "2023-11-02" ;
        rdf:value "Added a new rdfs:label in Spanish."@en
    ], [
        dc:date "2023-08-25" ;
        rdf:value "Added a new rdfs:label in French."@en
    ], [
        dc:date "2023-04-19" ;
        rdf:value "Removed the 0.2 existing unnecessary restriction."@en
    ], [
        dc:date "2020-10-23" ;
        rdf:value """Scope note: made separate paragraphs and some
               changes."""@en
    ] ;
    skos:scopeNote """An event may be caused by nature, an agent, or a combination of
         nature and agent. Events have temporal and spatial boundaries. An event may actively
         involve some agent(s) and affect any entity. An event may be discrete, happening at a
         specific moment in time, or may occur over an extended period of time. Events may have
         events as parts, and events may precede or follow one another. Multiple agents may
         participate in the same event, and in different roles."""@en ;
    :RiCCMCorrespondingComponent """Corresponds to RiC-E14 (Event
         entity)"""@en ;
    :closeTo "LODE Event class (http://linkedevents.org/ontology/#Event)"@en .

:EventRelation
    a owl:Class ;
    rdfs:comment """Connects at least one Event to at least one Thing, when the first
         is associated with the existence and lifecycle of the second one. The Event(s) is the
         source of the Relation, and the Thing(s) is the target."""@en ;
    rdfs:isDefinedBy <https://www.ica.org/standards/RiC/ontology> ;
    rdfs:label "Ereignis-Ding"@de, "Event Relation"@en, "Relación con un evento"@es, "Relation impliquant un événement"@fr ;
    rdfs:subClassOf :Relation, [
        a owl:Restriction ;
        owl:minQualifiedCardinality "1"^^xsd:nonNegativeInteger ;
        owl:onClass :Event ;
        owl:onProperty :relationHasSource
    ], [
        a owl:Restriction ;
        owl:minQualifiedCardinality "1"^^xsd:nonNegativeInteger ;
        owl:onClass :Thing ;
        owl:onProperty :relationHasTarget
    ] ;
    owl:equivalentClass [
        a owl:Restriction ;
        owl:hasSelf true ;
        owl:onProperty :eventRelation_role
    ] ;
    skos:changeNote [
        dc:date "2025-04-08" ;
        rdf:value "Added a new rdfs:label in German."@en
    ], [
        dc:date "2023-12-06" ;
        rdf:value """Improved the description of the Relation class (rdfs:comment)
               by clearly specifying how it is directed."""@en
    ], [
        dc:date "2023-11-12" ;
        rdf:value """Aligned with RiC-CM 1.0: updated the
               skos:scopeNote."""@en
    ], [
        dc:date "2023-11-08" ;
        rdf:value """In order to get a system of rolified Relation classes: added an
               equivalentClass object property; replaced the specific object properties by the
               generic ones in the subClassOf declarations."""@en
    ], [
        dc:date "2023-11-02" ;
        rdf:value "Added a new rdfs:label in Spanish."@en
    ], [
        dc:date "2023-08-25" ;
        rdf:value "Added a new rdfs:label in French."@en
    ] ;
    skos:scopeNote """Use to connect an event and an entity only if it is not possible
         to specify a narrower event relation, for example a PerformanceRelation."""@en ;
    :RiCCMCorrespondingComponent """Class implementation of RiC-R057 and RiC-R057i
         relations"""@en .

:EventType
    a owl:Class ;
    rdfs:comment "Categorization of an Event."@en ;
    rdfs:isDefinedBy <https://www.ica.org/standards/RiC/ontology> ;
    rdfs:label "Ereigniskategorie"@de, "Event Type"@en, "Tipo de evento"@es, "Type d’événement"@fr ;
    rdfs:subClassOf :Type ;
    skos:changeNote [
        dc:date "2025-04-08" ;
        rdf:value "Added a new rdfs:label in German."@en
    ], [
        dc:date "2023-11-12" ;
        rdf:value """Aligned with RiC-CM 1.0: updated the
               skos:scopeNote."""@en
    ], [
        dc:date "2023-11-02" ;
        rdf:value "Added a new rdfs:label in Spanish."@en
    ], [
        dc:date "2023-08-25" ;
        rdf:value "Added a new rdfs:label in French."@en
    ], [
        dc:date "2023-04-19" ;
        rdf:value "Removed the 0.2 existing unnecessary restriction."@en
    ], [
        dc:date "2020-10-23" ;
        rdf:value """Scope note: updated and made several paragraphs. Objective: to
               make RiC-O compliant with RiC-CM v0.2."""@en
    ] ;
    skos:scopeNote """Events of all kinds can be categorized. Curation event types
         include creation; acquisition; transfer; arrangement; description; digitization, etc.
         Biographical event types include birth, marriage, death, etc."""@en ;
    :RiCCMCorrespondingComponent """Corresponds to RiC-A18 (Event Type
         attribute)"""@en .

:Extent
    a owl:Class ;
    rdfs:comment """Countable characteristics of the content of an entity expressed as
         a quantity."""@en ;
    rdfs:isDefinedBy <https://www.ica.org/standards/RiC/ontology> ;
    rdfs:label "Extensión"@es, "Extent"@en, "Mesure"@fr, "Umfang "@de ;
    rdfs:subClassOf :Thing ;
    skos:changeNote [
        dc:date "2025-04-08" ;
        rdf:value "Added a new rdfs:label in German."@en
    ], [
        dc:date "2023-11-02" ;
        rdf:value "Added a new rdfs:label in Spanish."@en
    ], [
        dc:date "2023-08-25" ;
        rdf:value "Added a new rdfs:label in French."@en
    ], [
        dc:date "2020-10-28" ;
        rdf:value """Class added together with three subclasses and hasExtent and
               isExtentOf Object properties"""@en
    ] ;
    skos:scopeNote "Physical or logical extent of a resource"@en .

:ExtentType
    a owl:Class ;
    rdfs:comment """Categorization of the extent that is being
         measured."""@en ;
    rdfs:isDefinedBy <https://www.ica.org/standards/RiC/ontology> ;
    rdfs:label "Extent Type"@en, "Tipo de Extensión"@es, "Type de mesure"@fr, "Umfangskategorie"@de ;
    rdfs:subClassOf :Type ;
    skos:changeNote [
        dc:date "2025-04-08" ;
        rdf:value "Added a new rdfs:label in German."@en
    ], [
        dc:date "2023-11-02" ;
        rdf:value "Added a new rdfs:label in Spanish."@en
    ], [
        dc:date "2023-08-28" ;
        rdf:value "Added an xml:lang attribute to the rdfs:comment."@en
    ], [
        dc:date "2023-08-25" ;
        rdf:value "Added a new rdfs:label in French."@en
    ], [
        dc:date "2020-11-01" ;
        rdf:value """Added to specify the dimension that is being
               measured"""@en
    ] .

:Family
    a owl:Class ;
    rdfs:comment """Two or more persons related by birth, or through marriage,
         adoption, civil union, or other social conventions that bind them together as a socially
         recognized familial group."""@en ;
    rdfs:isDefinedBy <https://www.ica.org/standards/RiC/ontology> ;
    rdfs:label "Familia"@es, "Familie"@de, "Famille"@fr, "Family"@en ;
    rdfs:subClassOf :Group ;
    skos:changeNote [
        dc:date "2025-04-08" ;
        rdf:value "Added a new rdfs:label in German."@en
    ], [
        dc:date "2023-11-02" ;
        rdf:value "Added a new rdfs:label in Spanish."@en
    ], [
        dc:date "2023-08-25" ;
        rdf:value "Added a new rdfs:label in French."@en
    ], [
        dc:date "2020-10-23" ;
        rdf:value """Scope note: made separate paragraphs and some
               changes."""@en
    ] ;
    skos:scopeNote """Family is a kind of Group. “Family” is used here as a general
         term that encompasses a wide variety of familial groups. Other types of familial groups
         include Dynasty, Clan, House, Tribe and others. Though family may be a recognized legal
         group in specific contexts, the term may also be used for groups that are socially
         recognized as families. A family may be a group of persons related either by consanguinity
         or affinity or cohabitation or other social conventions. In some context, a Family may be
         legally recognized as Corporate Body. For example, certain North American peoples (tribes)
         retain self-government rights and have jurisdiction over defined tribal
         lands."""@en ;
    :RiCCMCorrespondingComponent """Corresponds to RiC-E10 (Family
         entity)"""@en .

:FamilyRelation
    a owl:Class ;
    rdfs:comment """Connects at least two Persons, when they have some family link,
         i.e. belong to the same family. This Relation is a generic, not oriented
         one."""@en ;
    rdfs:isDefinedBy <https://www.ica.org/standards/RiC/ontology> ;
    rdfs:label "Family Relation"@en, "Person-Familie-Person"@de, "Relación familiar"@es, "Relation familiale"@fr ;
    rdfs:subClassOf :AgentToAgentRelation, [
        a owl:Restriction ;
        owl:minQualifiedCardinality "2"^^xsd:nonNegativeInteger ;
        owl:onClass :Person ;
        owl:onProperty :relationConnects
    ] ;
    owl:equivalentClass [
        a owl:Restriction ;
        owl:hasSelf true ;
        owl:onProperty :familyRelation_role
    ] ;
    skos:changeNote [
        dc:date "2025-04-08" ;
        rdf:value "Added a new rdfs:label in German."@en
    ], [
        dc:date "2023-12-06" ;
        rdf:value """Improved the description of the Relation class (rdfs:comment)
               by clearly specifying how it is directed."""@en
    ], [
        dc:date "2023-11-12" ;
        rdf:value """Aligned with RiC-CM 1.0: updated the
               skos:scopeNote."""@en
    ], [
        dc:date "2023-11-08" ;
        rdf:value """In order to get a system of rolified Relation classes: added an
               equivalentClass object property; replaced the specific object properties by the
               generic ones in the subClassOf declarations."""@en
    ], [
        dc:date "2023-11-02" ;
        rdf:value "Added a new rdfs:label in Spanish."@en
    ], [
        dc:date "2023-08-25" ;
        rdf:value "Added a new rdfs:label in French."@en
    ] ;
    skos:scopeNote """Use the MembershipRelation class for connecting a family and a
         person."""@en ;
    :RiCCMCorrespondingComponent """Class implementation of RiC-R047 and RiC-R047i
         relations"""@en .

:FamilyType
    a owl:Class ;
    rdfs:comment "Categorization of a Family."@en ;
    rdfs:isDefinedBy <https://www.ica.org/standards/RiC/ontology> ;
    rdfs:label "Familienkategorie"@de, "Family Type"@en, "Tipo de familia"@es, "Type de famille"@fr ;
    rdfs:subClassOf :Type ;
    skos:changeNote [
        dc:date "2025-04-08" ;
        rdf:value "Added a new rdfs:label in German."@en
    ], [
        dc:date "2023-11-12" ;
        rdf:value """Aligned with RiC-CM 1.0: updated the
               skos:scopeNote."""@en
    ], [
        dc:date "2023-11-02" ;
        rdf:value "Added a new rdfs:label in Spanish."@en
    ], [
        dc:date "2023-08-25" ;
        rdf:value "Added a new rdfs:label in French."@en
    ], [
        dc:date "2023-04-19" ;
        rdf:value "Removed the 0.2 existing unnecessary restriction."@en
    ], [
        dc:date "2020-10-23" ;
        rdf:value "Comment: slighty changed."@en
    ] ;
    skos:scopeNote """Encompasses a wide variety of familial groups related by
         consanguinity, affinity, cohabitation, or other social conventions."""@en ;
    :RiCCMCorrespondingComponent """Corresponds to RiC-A20 (Family Type
         attribute)"""@en .

:FunctionalEquivalenceRelation
    a owl:Class ;
    rdfs:comment """Connects at least two Instantiations which may be considered as
         equivalent. This Relation is not oriented."""@en ;
    rdfs:isDefinedBy <https://www.ica.org/standards/RiC/ontology> ;
    rdfs:label "Functional Equivalence Relation"@en, "Relación de equivalencia funcional"@es, "Relation d’équivalence fonctionnelle"@fr, "Repräsentation-Äquivalent-Repräsentation"@de ;
    rdfs:subClassOf :InstantiationToInstantiationRelation, [
        a owl:Restriction ;
        owl:minQualifiedCardinality "2"^^xsd:nonNegativeInteger ;
        owl:onClass :Instantiation ;
        owl:onProperty :relationConnects
    ] ;
    owl:equivalentClass [
        a owl:Restriction ;
        owl:hasSelf true ;
        owl:onProperty :functionalEquivalenceRelation_role
    ] ;
    skos:changeNote [
        dc:date "2025-04-08" ;
        rdf:value "Added a new rdfs:label in German."@en
    ], [
        dc:date "2023-12-06" ;
        rdf:value """Improved the description of the Relation class (rdfs:comment)
               by clearly specifying how it is directed."""@en
    ], [
        dc:date "2023-11-12" ;
        rdf:value """Aligned with RiC-CM 1.0: updated the
               skos:scopeNote."""@en
    ], [
        dc:date "2023-11-08" ;
        rdf:value """In order to get a system of rolified Relation classes: added an
               equivalentClass object property; replaced the specific object properties by the
               generic ones in the subClassOf declarations."""@en
    ], [
        dc:date "2023-11-02" ;
        rdf:value "Added a new rdfs:label in Spanish."@en
    ], [
        dc:date "2023-08-25" ;
        rdf:value "Added a new rdfs:label in French."@en
    ] ;
    skos:scopeNote """Two instantiations, from some point of view, may be considered
         as equivalent. This equivalence is usually based upon the fact that the instantiations have
         at least the same intellectual content (they instantiate the same record
         resource)."""@en ;
    :RiCCMCorrespondingComponent """Class implementation of RiC-R035 and RiC-R035i
         relations"""@en .

:Group
    a owl:Class ;
    rdfs:comment "Two or more Agents that act together as an Agent."@en ;
    rdfs:isDefinedBy <https://www.ica.org/standards/RiC/ontology> ;
    rdfs:label "Group"@en, "Groupe d’agents"@fr, "Grupo de agentes"@es, "Gruppe"@de ;
    rdfs:subClassOf :Agent ;
    owl:disjointWith :Mechanism, :Person, :Position ;
    skos:changeNote [
        dc:date "2025-04-08" ;
        rdf:value "Added a new rdfs:label in German."@en
    ], [
        dc:date "2023-11-02" ;
        rdf:value "Added a new rdfs:label in Spanish."@en
    ], [
        dc:date "2023-08-25" ;
        rdf:value "Added a new rdfs:label in French."@en
    ], [
        dc:date "2020-10-23" ;
        rdf:value """Scope note: made separate paragraphs plus very few changes.
               Disjoint with: enriched."""@en
    ] ;
    skos:scopeNote """Group is a kind of Agent. A Group has a socially recognized
         identity. Each member of the Group plays a particular role or roles (that is has a
         particular Position) in the coordinated activity of the Group. Corporate bodies and
         families are kinds of groups, though other kinds of groups are possible. For example, the
         “electorate” -- all of the voters in a given election. Complex, large groups may be
         subdivided into other groups."""@en ;
    :RiCCMCorrespondingComponent """Corresponds to RiC-E09 (Group
         Entity)"""@en .

:GroupSubdivisionRelation
    a owl:Class ;
    rdfs:comment """Connects a Group and at least another Group, when the first one
         has or had the second one(s) among its subdivisions. The Relation is oriented from the
         Group to its subdivision(s): the parent Group is the source and the subdivision Group(s) is
         the target."""@en ;
    rdfs:isDefinedBy <https://www.ica.org/standards/RiC/ontology> ;
    rdfs:label "Group Subdivision Relation"@en, "Gruppe-Untergruppe"@de, "Relación de subdivisión entre grupos de agentes"@es, "Relation de subdivision entre groupes d’agents"@fr ;
    rdfs:subClassOf :AgentHierarchicalRelation, :WholePartRelation, [
        a owl:Restriction ;
        owl:onClass :Group ;
        owl:onProperty :relationHasSource ;
        owl:qualifiedCardinality "1"^^xsd:nonNegativeInteger
    ], [
        a owl:Restriction ;
        owl:minQualifiedCardinality "1"^^xsd:nonNegativeInteger ;
        owl:onClass :Group ;
        owl:onProperty :relationHasTarget
    ] ;
    owl:equivalentClass [
        a owl:Restriction ;
        owl:hasSelf true ;
        owl:onProperty :groupSubdivisionRelation_role
    ] ;
    skos:changeNote [
        dc:date "2025-04-08" ;
        rdf:value "Added a new rdfs:label in German."@en
    ], [
        dc:date "2023-12-06" ;
        rdf:value """Improved the description of the Relation class (rdfs:comment)
               by clearly specifying how it is directed."""@en
    ], [
        dc:date "2023-11-12" ;
        rdf:value """Aligned with RiC-CM 1.0: updated the description
               (rdfs:comment)."""@en
    ], [
        dc:date "2023-11-08" ;
        rdf:value """In order to get a system of rolified Relation classes: added an
               equivalentClass object property; replaced the specific object properties by the
               generic ones in the subClassOf declarations."""@en
    ], [
        dc:date "2023-11-02" ;
        rdf:value "Added a new rdfs:label in Spanish."@en
    ], [
        dc:date "2023-08-25" ;
        rdf:value "Added a new rdfs:label in French."@en
    ] ;
    :RiCCMCorrespondingComponent """Class implementation of RiC-R005 and RiC-R005i
         relations"""@en .

:Identifier
    a owl:Class ;
    rdfs:comment """A word, number, letter, symbol, or any combination of these used
         to uniquely identify or reference an individual instance of an entity within a specific
         information domain."""@en ;
    rdfs:isDefinedBy <https://www.ica.org/standards/RiC/ontology> ;
    rdfs:label "Identifiant"@fr, "Identificador"@es, "Identifier"@en, "Identifikator"@de ;
    rdfs:subClassOf :Appellation ;
    skos:changeNote [
        dc:date "2025-04-08" ;
        rdf:value "Added a new rdfs:label in German."@en
    ], [
        dc:date "2023-11-12" ;
        rdf:value """Aligned with RiC-CM 1.0: updated the
               skos:scopeNote."""@en
    ], [
        dc:date "2023-11-02" ;
        rdf:value "Added a new rdfs:label in Spanish."@en
    ], [
        dc:date "2023-08-25" ;
        rdf:value "Added a new rdfs:label in French."@en
    ], [
        dc:date "2023-04-19" ;
        rdf:value "Removed the 0.2 existing unnecessary restriction."@en
    ] ;
    skos:scopeNote """Can include Global Persistent Identifiers (globally unique and
         persistently resolvable identifier for the entity) and/or Local Identifiers. Both the
         domain within which the identifier is unique, and the rules used in forming the identifier
         value should be provided with the identifier value."""@en ;
    :RiCCMCorrespondingComponent """Class implementation of RiC-A22 (Identifier
         attribute) (see also the identifier datatype property)"""@en .

:IdentifierType
    a owl:Class ;
    rdfs:comment "Categorization of an Identifier."@en ;
    rdfs:isDefinedBy <https://www.ica.org/standards/RiC/ontology> ;
    rdfs:label "Identifier Type"@en, "Identifikatorenkategorie"@de, "Tipo de identificador"@es, "Type d’identifiant"@fr ;
    rdfs:subClassOf :Type ;
    skos:changeNote [
        dc:date "2025-04-08" ;
        rdf:value "Added a new rdfs:label in German."@en
    ], [
        dc:date "2023-11-02" ;
        rdf:value "Added a new rdfs:label in Spanish."@en
    ], [
        dc:date "2023-08-25" ;
        rdf:value "Added a new rdfs:label in French."@en
    ], [
        dc:date "2023-04-19" ;
        rdf:value "Removed the 0.2 existing unnecessary restriction."@en
    ], [
        dc:date "2020-10-19" ;
        rdf:value """Class added along with hasIdentifierType and isIdentifierTypeOf
               object properties."""@en
    ] ;
    skos:scopeNote """For example, 'old identifier' ; 'ISNI' (for a person or
         corporate body), etc."""@en .

:Instantiation
    a owl:Class ;
    rdfs:comment """The inscription of information made by an Agent on a physical
         carrier in any persistent, recoverable form as a means of communicating information through
         time and space."""@en ;
    rdfs:isDefinedBy <https://www.ica.org/standards/RiC/ontology> ;
    rdfs:label "Instanciación"@es, "Instanciation"@fr, "Instantiation"@en, "Repräsentation oder Instanz"@de ;
    rdfs:subClassOf :Thing ;
    skos:changeNote [
        dc:date "2025-04-08" ;
        rdf:value "Added a new rdfs:label in German."@en
    ], [
        dc:date "2023-11-02" ;
        rdf:value "Added a new rdfs:label in Spanish."@en
    ], [
        dc:date "2023-08-25" ;
        rdf:value "Added a new rdfs:label in French."@en
    ], [
        dc:date "2023-04-19" ;
        rdf:value "Removed the 0.2 existing unnecessary restrictions."@en
    ], [
        dc:date "2020-10-23" ;
        rdf:value """Comment: updated. Scope note: updated and made several
               paragraphs. Objective: to make RiC-O compliant with RiC-CM v0.2."""@en
    ] ;
    skos:scopeNote """A Record or Record Part must have been instantiated at least
         once, though this instantiation may no longer exist at the moment of description. An
         instantiation might also exist at the moment of description, but be destroyed at a later
         moment in time, when, for example, a derived instantiation might become the only remaining
         instantiation. A Record Set may have an instantiation, which is to say that it is not a
         necessary condition. An Instantiation may be derived from another Instantiation. A Record
         Resource may have many Instantiations simultaneously (for instance, a record printed and
         saved in the same time as DOCX and PDF/A would have 3 concurrent instantiations) or through
         time (for example, copy of a record). Depending on the context, a new instantiation may be
         seen as a new or as the same record resource. During in the process of re-instantiation
         something is lost and something is preserved, but it is up to the context and the Agent
         that produces or uses that Instantiation to assess whether the two instantiations are
         functionally equivalent or not. For instance, a postcard representing a town map from 1874
         (Instantiation 1) is digitized and kept as a JPEG file (Instantiation 2). The digital copy
         may be considered as instantiating the \"same\" Record by an Agent considering the
         information transmitted by the Record (e.g., the urban landscape displayed), but as a\"
         different\" Record by an antiquarian more focused on the materiality of the carrier.
         Successive instantiations may change the perceivable boundaries of a Record Resource. For
         instance, a case file comprising many records may be digitized and saved as one single PDF
         file, which, from management perspective, may be treated as one Record. Similarly, a large
         Record Set (a fonds or a series) may be maintained as one database. On the other hand, one
         record (main document and its annexes) may be digitized in separate files and each one may
         be managed as a discrete “physical” item. Instantiations may require mediation to
         communicate the information in the Record Resource. While a traditional Record on paper can
         simply be read by an Agent in order to understand the information, a vinyl recording, a
         video cassette or a digital file needs a device (mediator) to codify or decodify the
         information conveyed. This mediator may imply simple physical components (a turntable
         needle, for example), or a complex gallery of software and hardware elements.
         Instantiations are more than the mere informational content of Record Resource and may be
         the focus of preservation and physical management of records. The use of particular
         document types for records, such as a medieval charter, may have implications for the
         authenticity of the records. Hence, the way a Record Resource is instantiated contributes
         to the contextualizing of the content.record resource is instantiated contributes to the
         contextualizing the content. Distinguishing the message conveyed (Record Resource) and its
         physical representations (Instantiation) allows for the efficient management of their
         descriptions, and preserve information about a Record Resource even when no physical
         representation of it exists or is known to exist anymore. The relations between distinct
         instantiations can then be expressed wherever they coexist, and they can be related to the
         Record Resource they instantiate."""@en ;
    :RiCCMCorrespondingComponent """Corresponds to RiC-E06 (Instantiation
         entity)"""@en ;
    :closeTo "PREMIS Representation"@en .

:InstantiationExtent
    a owl:Class ;
    rdfs:comment """Countable characteristics of an Instantiation expressed as a
         quantity."""@en ;
    rdfs:isDefinedBy <https://www.ica.org/standards/RiC/ontology> ;
    rdfs:label "Extensión de la instanciación"@es, "Instantiation Extent"@en, "Mesure d’une instanciation"@fr, "Umfang der Instanz|Repräsentation"@de ;
    rdfs:subClassOf :Extent ;
    skos:changeNote [
        dc:date "2025-04-08" ;
        rdf:value "Added a new rdfs:label in German."@en
    ], [
        dc:date "2023-11-12" ;
        rdf:value """Aligned with RiC-CM 1.0: updated the description
               (rdfs:comment)."""@en
    ], [
        dc:date "2023-11-02" ;
        rdf:value "Added a new rdfs:label in Spanish."@en
    ], [
        dc:date "2023-08-25" ;
        rdf:value "Added a new rdfs:label in French."@en
    ], [
        dc:date "2020-11-21" ;
        rdf:value """Changed a bit the definition and added change
               notes."""@en
    ], [
        dc:date "2020-10-28" ;
        rdf:value """Class added in order to handle an accurate description of an
               instantiation extent"""@en
    ] ;
    :RiCCMCorrespondingComponent """Class implementation of RiC-A23 (Instantiation
         Extent attribute)"""@en .

:InstantiationToInstantiationRelation
    a owl:Class ;
    rdfs:comment """Connects at least two instantiations. This Relation is a generic,
         not oriented one."""@en ;
    rdfs:isDefinedBy <https://www.ica.org/standards/RiC/ontology> ;
    rdfs:label "Instantiation to Instantiation Relation"@en, "Instanz|Repräsentation-Instanz|Repräsentation"@de, "Relación entre instanciaciones"@es, "Relation entre instanciations"@fr ;
    rdfs:subClassOf :Relation, [
        a owl:Restriction ;
        owl:minQualifiedCardinality "2"^^xsd:nonNegativeInteger ;
        owl:onClass :Instantiation ;
        owl:onProperty :relationConnects
    ] ;
    owl:equivalentClass [
        a owl:Restriction ;
        owl:hasSelf true ;
        owl:onProperty :instantiationToInstantiationRelation_role
    ] ;
    skos:changeNote [
        dc:date "2025-04-08" ;
        rdf:value "Added a new rdfs:label in German."@en
    ], [
        dc:date "2023-12-06" ;
        rdf:value """Improved the description of the Relation class (rdfs:comment)
               by clearly specifying how it is directed."""@en
    ], [
        dc:date "2023-11-08" ;
        rdf:value """In order to get a system of rolified Relation classes: added an
               equivalentClass object property; replaced the specific object properties by the
               generic ones in the subClassOf declarations."""@en
    ], [
        dc:date "2023-11-02" ;
        rdf:value "Added a new rdfs:label in Spanish."@en
    ], [
        dc:date "2023-08-25" ;
        rdf:value "Added a new rdfs:label in French."@en
    ] .

:IntellectualPropertyRightsRelation
    a owl:Class ;
    rdfs:comment """Connects at least one Agent and one Record Resource or
         Instantiation on which the Agent has or had some intellectual property rights. The Agent(s)
         is the source of the Relation and the Record Resource(s) or Instantiation(s) is the
         target."""@en ;
    rdfs:isDefinedBy <https://www.ica.org/standards/RiC/ontology> ;
    rdfs:label "Akteur-Urheberschaft-Recordressource/Instanz"@de, "Intellectual Property Rights Relation"@en, "Relación de propiedad intelectual"@es, "Relation de propriété intellectuelle"@fr ;
    rdfs:subClassOf :AuthorityRelation, [
        a owl:Restriction ;
        owl:minQualifiedCardinality "1"^^xsd:nonNegativeInteger ;
        owl:onClass [
            a owl:Class ;
            owl:unionOf (:Group
                :Person
                :Position
            )
        ] ;
        owl:onProperty :relationHasSource
    ], [
        a owl:Restriction ;
        owl:minQualifiedCardinality "1"^^xsd:nonNegativeInteger ;
        owl:onClass [
            a owl:Class ;
            owl:unionOf (:Instantiation
                :RecordResource
            )
        ] ;
        owl:onProperty :relationHasTarget
    ] ;
    owl:equivalentClass [
        a owl:Restriction ;
        owl:hasSelf true ;
        owl:onProperty :intellectualPropertyRightsRelation_role
    ] ;
    skos:changeNote [
        dc:date "2025-04-08" ;
        rdf:value "Added a new rdfs:label in German."@en
    ], [
        dc:date "2023-12-06" ;
        rdf:value """Improved the description of the Relation class (rdfs:comment)
               by clearly specifying how it is directed."""@en
    ], [
        dc:date "2023-11-12" ;
        rdf:value """Aligned with RiC-CM 1.0: updated the description
               (rdfs:comment)."""@en
    ], [
        dc:date "2023-11-08" ;
        rdf:value """In order to get a system of rolified Relation classes: added an
               equivalentClass object property; replaced the specific object properties by the
               generic ones in the subClassOf declarations."""@en
    ], [
        dc:date "2023-11-02" ;
        rdf:value "Added a new rdfs:label in Spanish."@en
    ], [
        dc:date "2023-08-25" ;
        rdf:value "Added a new rdfs:label in French."@en
    ] ;
    skos:scopeNote """Can be used, when the record resource is a work, for specifying
         the connection between the record resource and its author(s)."""@en ;
    :RiCCMCorrespondingComponent """Class implementation of RiC-R040 and RiC-R040i
         relations"""@en .

:KnowingOfRelation
    a owl:Class ;
    rdfs:comment """Connects at least one Person to at least another one, when the
         first one has some knowledge of the second one through time or space. The first Person is
         the source of the Relation, and the second one is the target."""@en ;
    rdfs:isDefinedBy <https://www.ica.org/standards/RiC/ontology> ;
    rdfs:label "Knowing Of Relation"@en, "Person-Kenntnis-Person"@de, "Relación de conocimieto indirecto entre personas"@es, "Relation de connaissance à propos d’une personne"@fr ;
    rdfs:subClassOf :AgentToAgentRelation, [
        a owl:Restriction ;
        owl:minQualifiedCardinality "1"^^xsd:nonNegativeInteger ;
        owl:onClass :Person ;
        owl:onProperty :relationHasSource
    ], [
        a owl:Restriction ;
        owl:minQualifiedCardinality "1"^^xsd:nonNegativeInteger ;
        owl:onClass :Person ;
        owl:onProperty :relationHasTarget
    ] ;
    owl:equivalentClass [
        a owl:Restriction ;
        owl:hasSelf true ;
        owl:onProperty :knowingOfRelation_role
    ] ;
    skos:changeNote [
        dc:date "2025-04-08" ;
        rdf:value "Added a new rdfs:label in German."@en
    ], [
        dc:date "2023-12-06" ;
        rdf:value """Improved the description of the Relation class (rdfs:comment)
               by clearly specifying how it is directed."""@en
    ], [
        dc:date "2023-11-08" ;
        rdf:value """In order to get a system of rolified Relation classes: added an
               equivalentClass object property; replaced the specific object properties by the
               generic ones in the subClassOf declarations."""@en
    ], [
        dc:date "2023-11-02" ;
        rdf:value "Added a new rdfs:label in Spanish."@en
    ], [
        dc:date "2023-08-25" ;
        rdf:value "Added a new rdfs:label in French."@en
    ] ;
    :RiCCMCorrespondingComponent """Class implementation of RiC-R050 and RiC-R050i
         relations"""@en .

:KnowingRelation
    a owl:Class ;
    rdfs:comment """Connects at least two Persons who directly know each other during
         their existence. This Relation is not oriented."""@en ;
    rdfs:isDefinedBy <https://www.ica.org/standards/RiC/ontology> ;
    rdfs:label "Knowing Relation"@en, "Person-Bekanntschaft-Person"@de, "Relación de conocimiento directo entre personas"@es, "Relation de connaissance entre personnes"@fr ;
    rdfs:subClassOf :AgentToAgentRelation, [
        a owl:Restriction ;
        owl:minQualifiedCardinality "2"^^xsd:nonNegativeInteger ;
        owl:onClass :Person ;
        owl:onProperty :relationConnects
    ] ;
    owl:equivalentClass [
        a owl:Restriction ;
        owl:hasSelf true ;
        owl:onProperty :knowingRelation_role
    ] ;
    skos:changeNote [
        dc:date "2025-04-08" ;
        rdf:value "Added a new rdfs:label in German."@en
    ], [
        dc:date "2023-12-06" ;
        rdf:value """Improved the description of the Relation class (rdfs:comment)
               by clearly specifying how it is directed."""@en
    ], [
        dc:date "2023-11-12" ;
        rdf:value """Aligned with RiC-CM 1.0: updated the description
               (rdfs:comment), skos:scopeNote."""@en
    ], [
        dc:date "2023-11-08" ;
        rdf:value """In order to get a system of rolified Relation classes: added an
               equivalentClass object property; replaced the specific object properties by the
               generic ones in the subClassOf declarations."""@en
    ], [
        dc:date "2023-11-02" ;
        rdf:value "Added a new rdfs:label in Spanish."@en
    ], [
        dc:date "2023-08-25" ;
        rdf:value "Added a new rdfs:label in French."@en
    ] ;
    skos:scopeNote """The relation implies that the two persons met or at least
         corresponded with each other."""@en ;
    :RiCCMCorrespondingComponent """Class implementation of RiC-R051 and RiC—R051i
         relations"""@en .

:Language
    a owl:Class ;
    rdfs:comment """A spoken or written human language represented in a Record
         Resource or used by an Agent."""@en ;
    rdfs:isDefinedBy <https://www.ica.org/standards/RiC/ontology> ;
    rdfs:label "Language"@en, "Langue"@fr, "Lengua"@es, "Sprache"@de ;
    rdfs:subClassOf :Concept ;
    skos:changeNote [
        dc:date "2025-04-08" ;
        rdf:value "Added a new rdfs:label in German."@en
    ], [
        dc:date "2023-11-12" ;
        rdf:value """Aligned with RiC-CM 1.0: updated the description
               (rdfs:comment)."""@en
    ], [
        dc:date "2023-11-02" ;
        rdf:value "Added a new rdfs:label in Spanish."@en
    ], [
        dc:date "2023-08-25" ;
        rdf:value "Added a new rdfs:label in French."@en
    ], [
        dc:date "2020-12-28" ;
        rdf:value """Changed the definition (skos:comment annotation); so that it
               conforms to the RiC-CM one."""@en
    ], [
        dc:date "2020-10-23" ;
        rdf:value "Scope note from RiC-CM : deleted."@en
    ] ;
    :RiCCMCorrespondingComponent """Corresponds to RiC-A25 (Language
         attribute)"""@en .

:LeadershipRelation
    a owl:Class ;
    rdfs:comment """Connects at least one Person and at least one Group, when the
         first one(s) lead(s) or led the second one(s). The Relation is oriented from the leading
         Person to the Group: the leading Person(s) is the source of the Relation, and the Group(s)
         is the target."""@en ;
    rdfs:isDefinedBy <https://www.ica.org/standards/RiC/ontology> ;
    rdfs:label "Leadership Relation"@en, "Person-Führung-Person"@de, "Relación de liderazgo"@es, "Relation de direction"@fr ;
    rdfs:subClassOf :AgentControlRelation, [
        a owl:Restriction ;
        owl:maxQualifiedCardinality "1"^^xsd:nonNegativeInteger ;
        owl:onClass :Position ;
        owl:onProperty :leadershipWithPosition
    ], [
        a owl:Restriction ;
        owl:minQualifiedCardinality "1"^^xsd:nonNegativeInteger ;
        owl:onClass :Person ;
        owl:onProperty :relationHasSource
    ], [
        a owl:Restriction ;
        owl:minQualifiedCardinality "1"^^xsd:nonNegativeInteger ;
        owl:onClass :Group ;
        owl:onProperty :relationHasTarget
    ] ;
    owl:equivalentClass [
        a owl:Restriction ;
        owl:hasSelf true ;
        owl:onProperty :leadershipRelation_role
    ] ;
    skos:changeNote [
        dc:date "2025-04-08" ;
        rdf:value "Added a new rdfs:label in German."@en
    ], [
        dc:date "2023-12-06" ;
        rdf:value """Improved the description of the Relation class (rdfs:comment)
               by clearly specifying how it is directed."""@en
    ], [
        dc:date "2023-11-12" ;
        rdf:value """Aligned with RiC-CM 1.0: updated the description
               (rdfs:comment)."""@en
    ], [
        dc:date "2023-11-08" ;
        rdf:value """In order to get a system of rolified Relation classes: added an
               equivalentClass object property; replaced the specific object properties by the
               generic ones in the subClassOf declarations."""@en
    ], [
        dc:date "2023-11-02" ;
        rdf:value "Added a new rdfs:label in Spanish."@en
    ], [
        dc:date "2023-08-25" ;
        rdf:value "Added a new rdfs:label in French."@en
    ] ;
    :RiCCMCorrespondingComponent """Class implementation of RiC-R042 and RiC-R042i
         relations"""@en .

:LegalStatus
    a owl:Class ;
    rdfs:comment "A status defined by law."@en ;
    rdfs:isDefinedBy <https://www.ica.org/standards/RiC/ontology> ;
    rdfs:label "Legal Status"@en, "Rechtstatus"@de, "Status jurídico"@es, "Statut légal"@fr ;
    rdfs:subClassOf :Type ;
    skos:changeNote [
        dc:date "2025-04-08" ;
        rdf:value "Added a new rdfs:label in German."@en
    ], [
        dc:date "2023-11-02" ;
        rdf:value "Added a new rdfs:label in Spanish."@en
    ], [
        dc:date "2023-08-25" ;
        rdf:value "Added a new rdfs:label in French."@en
    ] ;
    :RiCCMCorrespondingComponent """Corresponds to RiC-A26 (Legal Status
         attribute)"""@en .

:ManagementRelation
    a owl:Class ;
    rdfs:comment """Connects at least one Agent and at least one Record Resource or
         Instantiation that the Agent manages or managed. The Agent(s) is the source of the
         Relation, and the Record Resource(s) or Instantiation(s) is the target."""@en ;
    rdfs:isDefinedBy <https://www.ica.org/standards/RiC/ontology> ;
    rdfs:label "Akteur-Management-Recordressource/Instanz"@de, "Management Relation"@en, "Relación de gestión"@es, "Relation de gestion"@fr ;
    rdfs:subClassOf :AuthorityRelation, [
        a owl:Restriction ;
        owl:minQualifiedCardinality "1"^^xsd:nonNegativeInteger ;
        owl:onClass :Agent ;
        owl:onProperty :relationHasSource
    ], [
        a owl:Restriction ;
        owl:minQualifiedCardinality "1"^^xsd:nonNegativeInteger ;
        owl:onClass [
            a owl:Class ;
            owl:unionOf (:Instantiation
                :RecordResource
            )
        ] ;
        owl:onProperty :relationHasTarget
    ] ;
    owl:equivalentClass [
        a owl:Restriction ;
        owl:hasSelf true ;
        owl:onProperty :managementRelation_role
    ] ;
    skos:changeNote [
        dc:date "2025-04-08" ;
        rdf:value "Added a new rdfs:label in German."@en
    ], [
        dc:date "2023-12-06" ;
        rdf:value """Improved the description of the Relation class (rdfs:comment)
               by clearly specifying how it is directed."""@en
    ], [
        dc:date "2023-11-12" ;
        rdf:value """Aligned with RiC-CM 1.0: updated the description
               (rdfs:comment)."""@en
    ], [
        dc:date "2023-11-08" ;
        rdf:value """In order to get a system of rolified Relation classes: added an
               equivalentClass object property; replaced the specific object properties by the
               generic ones in the subClassOf declarations."""@en
    ], [
        dc:date "2023-11-02" ;
        rdf:value "Added a new rdfs:label in Spanish."@en
    ], [
        dc:date "2023-08-25" ;
        rdf:value "Added a new rdfs:label in French."@en
    ] ;
    :RiCCMCorrespondingComponent """Class implementation of RiC-R038 and RiC-R038i
         relations"""@en .

:Mandate
    a owl:Class ;
    rdfs:comment """Delegation of responsibility or authority by an Agent to another
         Agent to perform an Activity."""@en ;
    rdfs:isDefinedBy <https://www.ica.org/standards/RiC/ontology> ;
    rdfs:label "Mandat"@de, "Mandat"@fr, "Mandate"@en, "Norma"@es ;
    rdfs:subClassOf :Rule ;
    skos:changeNote [
        dc:date "2025-04-08" ;
        rdf:value "Added a new rdfs:label in German."@en
    ], [
        dc:date "2023-11-12" ;
        rdf:value """Aligned with RiC-CM 1.0: updated the description
               (rdfs:comment), skos:scopeNote."""@en
    ], [
        dc:date "2023-11-02" ;
        rdf:value "Added a new rdfs:label in Spanish."@en
    ], [
        dc:date "2023-08-25" ;
        rdf:value "Added a new rdfs:label in French."@en
    ], [
        dc:date "2023-04-21" ;
        rdf:value "Removed the 0.2 existing unnecessary restriction."@en
    ], [
        dc:date "2020-10-23" ;
        rdf:value """Scope note: made separate paragraphs and updated. Objective: to
               make RiC-O compliant with RiC-CM v0.2."""@en
    ] ;
    skos:scopeNote """Mandate is a kind of Rule. A mandate confers the responsibility
         or authority of an agent to perform a specified activity. In addition to assigning an
         activity and delegating responsibility or authority to perform the activity to an agent, a
         mandate commonly limits the place (jurisdiction) and date (time period) within which an
         agent may perform the activity (where and when). Mandates exist in a specific social and
         cultural context, and within that context are subject to change over time. While a mandate
         may be tacit, in whole or part, it may be explicitly expressed in a variety of documentary
         sources (for example, constitutions, legislation, (legal) acts, statutes, legal codes,
         ordinances, charges, charters, or mission statements). The evidence for identifying a
         mandate may be found in its entirety in one documentary source (for example, a law or
         regulation), or may be found in two or more sources. A mandate should not be confused with
         the one or more documentary sources that serve as evidence of its identity. A documentary
         source is a record."""@en ;
    :RiCCMCorrespondingComponent """Corresponds to RiC-E17 (Mandate
         entity)"""@en .

:MandateRelation
    a owl:Class ;
    rdfs:comment """Connects at least one Mandate and at least one Agent, when the
         first gives or gave the second one the authority or competencies to act. May also involve
         one to many Activities that the Mandate(s) assign(s) or assigned to the Agent(s). The
         Mandate(s) is the source of the Relation and the Agent(s) is the target."""@en ;
    rdfs:isDefinedBy <https://www.ica.org/standards/RiC/ontology> ;
    rdfs:label "Mandat-Akteur"@de, "Mandate Relation"@en, "Relación normativa"@es, "Relation impliquant un mandat"@fr ;
    rdfs:subClassOf :RuleRelation, [
        a owl:Restriction ;
        owl:minQualifiedCardinality "1"^^xsd:nonNegativeInteger ;
        owl:onClass :Activity ;
        owl:onProperty :asConcernsActivity
    ], [
        a owl:Restriction ;
        owl:minQualifiedCardinality "1"^^xsd:nonNegativeInteger ;
        owl:onClass :Mandate ;
        owl:onProperty :relationHasSource
    ], [
        a owl:Restriction ;
        owl:minQualifiedCardinality "1"^^xsd:nonNegativeInteger ;
        owl:onClass :Agent ;
        owl:onProperty :relationHasTarget
    ] ;
    owl:equivalentClass [
        a owl:Restriction ;
        owl:hasSelf true ;
        owl:onProperty :mandateRelation_role
    ] ;
    skos:changeNote [
        dc:date "2025-04-08" ;
        rdf:value "Added a new rdfs:label in German."@en
    ], [
        dc:date "2023-12-06" ;
        rdf:value """Improved the description of the Relation class (rdfs:comment)
               by clearly specifying how it is directed."""@en
    ], [
        dc:date "2023-11-12" ;
        rdf:value """Aligned with RiC-CM 1.0: updated the description
               (rdfs:comment)."""@en
    ], [
        dc:date "2023-11-08" ;
        rdf:value """In order to get a system of rolified Relation classes: added an
               equivalentClass object property; replaced the specific object properties by the
               generic ones in the subClassOf declarations."""@en
    ], [
        dc:date "2023-11-02" ;
        rdf:value "Added a new rdfs:label in Spanish."@en
    ], [
        dc:date "2023-08-25" ;
        rdf:value "Added a new rdfs:label in French."@en
    ], [
        dc:date "2023-04-19" ;
        rdf:value "Removed a 0.2 existing unnecessary restriction."@en
    ] ;
    :RiCCMCorrespondingComponent """Class implementation of RiC-R067 and RiC-R067i
         relations"""@en .

:MandateType
    a owl:Class ;
    rdfs:comment "Categorization of a Mandate."@en ;
    rdfs:isDefinedBy <https://www.ica.org/standards/RiC/ontology> ;
    rdfs:label "Mandate Type"@en, "Mandatkategorie"@de, "Tipo de norma"@es, "Type de mandat"@fr ;
    rdfs:subClassOf :RuleType ;
    skos:changeNote [
        dc:date "2025-04-08" ;
        rdf:value "Added a new rdfs:label in German."@en
    ], [
        dc:date "2023-11-12" ;
        rdf:value """Added in RiC-0 1.0 as it has been added to RiC-CM
               1.0."""@en
    ] ;
    skos:scopeNote """For example : charter, treaty, contract, letter of appointment,
         papal mandate, episcopal mandate, ciurt mandate, election mandate, popular mandate, federal
         mandate, etc."""@en ;
    :RiCCMCorrespondingComponent """Corresponds to RiC-A44 (Mandate Type
         attribute)."""@en .

:Mechanism
    a owl:Class ;
    rdfs:comment """A process or system created by a Person or Group that performs an
         Activity."""@en ;
    rdfs:isDefinedBy <https://www.ica.org/standards/RiC/ontology> ;
    rdfs:label "Mecanismo"@es, "Mechanism"@en, "Mechanismus"@de, "Système"@fr ;
    rdfs:subClassOf :Agent ;
    owl:disjointWith :Person, :Position ;
    skos:changeNote [
        dc:date "2025-04-08" ;
        rdf:value "Added a new rdfs:label in German."@en
    ], [
        dc:date "2023-11-12" ;
        rdf:value """Aligned with RiC-CM 1.0: updated the
               skos:scopeNote."""@en
    ], [
        dc:date "2023-11-02" ;
        rdf:value "Added a new rdfs:label in Spanish."@en
    ], [
        dc:date "2023-08-25" ;
        rdf:value "Added a new rdfs:label in French."@en
    ], [
        dc:date "2020-10-23" ;
        rdf:value """scope note: made separate paragraphs. Disjoint with:
               enriched."""@en
    ] ;
    skos:scopeNote """Mechanism is a kind of Agent. A mechanism may have both
         mechanical and software components or may be exclusively software. A mechanism acts in the
         world producing physical or social effects and may generate or modify records. A mechanism
         performs activities based on rules determined by the agent that designed and created it. A
         mechanism has an essential, derivative relation with the designing and creating
         agent."""@en ;
    :RiCCMCorrespondingComponent """Corresponds to RiC-E13 (Mechanism
         entity)"""@en .

:MembershipRelation
    a owl:Class ;
    rdfs:comment """Connects a Group and at least one Person, when the first one has
         or had the second one(s) among its members. The Relation is oriented from the Group to its
         members: the Group(s) is the source of the Relation, and the Person(s) is the
         target."""@en ;
    rdfs:isDefinedBy <https://www.ica.org/standards/RiC/ontology> ;
    rdfs:label "Gruppe-Mitgliedschaft-Person"@de, "Membership Relation"@en, "Relación de membresía"@es, "Relation d’appartenance"@fr ;
    rdfs:subClassOf :AgentToAgentRelation, [
        a owl:Restriction ;
        owl:maxQualifiedCardinality "1"^^xsd:nonNegativeInteger ;
        owl:onClass :Position ;
        owl:onProperty :membershipWithPosition
    ], [
        a owl:Restriction ;
        owl:onClass :Group ;
        owl:onProperty :relationHasSource ;
        owl:qualifiedCardinality "1"^^xsd:nonNegativeInteger
    ], [
        a owl:Restriction ;
        owl:minQualifiedCardinality "1"^^xsd:nonNegativeInteger ;
        owl:onClass :Person ;
        owl:onProperty :relationHasTarget
    ] ;
    owl:equivalentClass [
        a owl:Restriction ;
        owl:hasSelf true ;
        owl:onProperty :membershipRelation_role
    ] ;
    skos:changeNote [
        dc:date "2025-04-08" ;
        rdf:value "Added a new rdfs:label in German."@en
    ], [
        dc:date "2023-12-06" ;
        rdf:value """Improved the description of the Relation class (rdfs:comment)
               by clearly specifying how it is directed."""@en
    ], [
        dc:date "2023-11-12" ;
        rdf:value """Aligned with RiC-CM 1.0: updated the description
               (rdfs:comment)."""@en
    ], [
        dc:date "2023-11-08" ;
        rdf:value """In order to get a system of rolified Relation classes: added an
               equivalentClass object property; replaced the specific object properties by the
               generic ones in the subClassOf declarations."""@en
    ], [
        dc:date "2023-11-02" ;
        rdf:value "Added a new rdfs:label in Spanish."@en
    ], [
        dc:date "2023-08-25" ;
        rdf:value "Added a new rdfs:label in French."@en
    ] ;
    :RiCCMCorrespondingComponent """Class implementation of RiC-R055 and RiC-R055i
         relations"""@en .

:MigrationRelation
    a owl:Class ;
    rdfs:comment """Connects an Instantiation and at least another Instantiation it
         has been migrated into. The Relation is oriented chronologically, from the first
         Instantiation in time (the migrated one) to the one which results from its migration: the
         first Instantiation in time is the source of the Relation, and the resulting Instantiation
         is the target."""@en ;
    rdfs:isDefinedBy <https://www.ica.org/standards/RiC/ontology> ;
    rdfs:label "Migration Relation"@en, "Relación de migración entre instanciaciones"@es, "Relation de migration"@fr, "Repräsentation-Migration-Repräsentation"@de ;
    rdfs:subClassOf :DerivationRelation, [
        a owl:Restriction ;
        owl:onClass :Instantiation ;
        owl:onProperty :relationHasSource ;
        owl:qualifiedCardinality "1"^^xsd:nonNegativeInteger
    ], [
        a owl:Restriction ;
        owl:minQualifiedCardinality "1"^^xsd:nonNegativeInteger ;
        owl:onClass :Instantiation ;
        owl:onProperty :relationHasTarget
    ] ;
    owl:equivalentClass [
        a owl:Restriction ;
        owl:hasSelf true ;
        owl:onProperty :migrationRelation_role
    ] ;
    skos:changeNote [
        dc:date "2025-04-08" ;
        rdf:value "Added a new rdfs:label in German."@en
    ], [
        dc:date "2023-12-06" ;
        rdf:value """Improved the description of the Relation class (rdfs:comment)
               by clearly specifying how it is directed."""@en
    ], [
        dc:date "2023-11-12" ;
        rdf:value """Aligned with RiC-CM 1.0: updated the description
               (rdfs:comment), skos:scopeNote."""@en
    ], [
        dc:date "2023-11-08" ;
        rdf:value """In order to get a system of rolified Relation classes: added an
               equivalentClass object property; replaced the specific object properties by the
               generic ones in the subClassOf declarations."""@en
    ], [
        dc:date "2023-11-02" ;
        rdf:value "Added a new rdfs:label in Spanish."@en
    ], [
        dc:date "2023-08-25" ;
        rdf:value "Added a new rdfs:label in French."@en
    ] ;
    skos:scopeNote "Use for digital instantiations."@en ;
    :RiCCMCorrespondingComponent """Class implementation of RiC-R015 and RiC-R015i
         relations"""@en .

:Name
    a owl:Class ;
    rdfs:comment """A label, title or term designating an entity in order to make it
         distinguishable from other similar entities."""@en ;
    rdfs:isDefinedBy <https://www.ica.org/standards/RiC/ontology> ;
    rdfs:label "Name"@de, "Name"@en, "Nom"@fr, "Nombre"@es ;
    rdfs:subClassOf :Appellation ;
    skos:changeNote [
        dc:date "2025-04-08" ;
        rdf:value "Added a new rdfs:label in German."@en
    ], [
        dc:date "2023-11-12" ;
        rdf:value """Aligned with RiC-CM 1.0: updated the description
               (rdfs:comment), skos:scopeNote."""@en
    ], [
        dc:date "2023-11-02" ;
        rdf:value "Added a new rdfs:label in Spanish."@en
    ], [
        dc:date "2023-08-25" ;
        rdf:value "Added a new rdfs:label in French."@en
    ] ;
    skos:scopeNote """Provides brief information about the content or other individual
         characteristics of the entity being described, necessary to distinguish it from other
         perhaps similar entities."""@en ;
    :RiCCMCorrespondingComponent """Class implementation of RiC-A28 (Name attribute)
         (see also the name datatype property)"""@en .

:OccupationType
    a owl:Class ;
    rdfs:comment """Categorization of a profession, trade, or craft pursued by a
         Person in fulfilment of an Activity."""@en ;
    rdfs:isDefinedBy <https://www.ica.org/standards/RiC/ontology> ;
    rdfs:label "Beschäftigungskategorie"@de, "Occupation Type"@en, "Tipo de ocupación"@es, "Type d’occupation"@fr ;
    rdfs:subClassOf :ActivityType, :DemographicGroup ;
    skos:changeNote [
        dc:date "2025-04-08" ;
        rdf:value "Added a new rdfs:label in German."@en
    ], [
        dc:date "2023-11-12" ;
        rdf:value """Aligned with RiC-CM 1.0: updated the description
               (rdfs:comment), skos:scopeNote."""@en
    ], [
        dc:date "2023-11-02" ;
        rdf:value "Added a new rdfs:label in Spanish."@en
    ], [
        dc:date "2023-08-25" ;
        rdf:value "Added a new rdfs:label in French."@en
    ], [
        dc:date "2023-04-19" ;
        rdf:value "Removed the 0.2 existing unnecessary restriction."@en
    ], [
        dc:date "2020-10-23" ;
        rdf:value "scope note: added."@en
    ] ;
    skos:scopeNote """The pursuit of an occupation involves the performance of an
         Activity. Successful performance of the Activity is based on the ability to perform related
         competencies successfully. Such competencies may be acquired through education or
         experience, or a combination of both. The authority of the Person to pursue the occupation
         may be derived tacitly or explicitly from an external Agent, based on a demonstrated
         mastery of the competency. An occupation may be pursued independently by a Person or a
         Group, thereby contributing to the fulfilment of the function (activity) of the group.
         Should not be confused with Position where, for example, an agent with the occupation type
         \"lawyer\" holds the position of \"legal counsel\" in an agency. Related to but should not be
         confused with the domain or field of activity, such as an archivist who works in the domain
         of archival science."""@en ;
    :RiCCMCorrespondingComponent """Corresponds to RiC-A30 (Occupation Type
         attribute)"""@en .

:OrganicOrFunctionalProvenanceRelation
    a owl:Class ;
    rdfs:comment """Connects at least one Record Resource or Instantiation to at least
         one Agent or Activity, when the Agent or Activity is the provenance of the Record Resource
         or Instantiation (i.e. when the Agent created, accumulated or maintained the Record
         Resource or Instantiation, or when the Activity resulted into them). The Record Resource(s)
         or Instantiation(s) is the source of the Relation, and the Agent(s) or Activity(-ies) is
         the target."""@en ;
    rdfs:isDefinedBy <https://www.ica.org/standards/RiC/ontology> ;
    rdfs:label "Organic or functional provenance Relation"@en, "Recordressource/Instanz-Herkunft-Akteur/Funktion"@de, "Relación de procedencia orgánica or funcional"@es, "Relation de provenance organique ou fonctionnelle"@fr ;
    rdfs:subClassOf :Relation, [
        a owl:Restriction ;
        owl:minQualifiedCardinality "1"^^xsd:nonNegativeInteger ;
        owl:onClass [
            a owl:Class ;
            owl:unionOf (:Instantiation
                :RecordResource
            )
        ] ;
        owl:onProperty :relationHasSource
    ], [
        a owl:Restriction ;
        owl:minQualifiedCardinality "1"^^xsd:nonNegativeInteger ;
        owl:onClass [
            a owl:Class ;
            owl:unionOf (:Activity
                :Agent
            )
        ] ;
        owl:onProperty :relationHasTarget
    ] ;
    owl:equivalentClass [
        a owl:Restriction ;
        owl:hasSelf true ;
        owl:onProperty :organicOrFunctionalProvenanceRelation_role
    ] ;
    skos:changeNote [
        dc:date "2025-04-08" ;
        rdf:value "Added a new rdfs:label in German."@en
    ], [
        dc:date "2023-12-06" ;
        rdf:value """Improved the description of the Relation class (rdfs:comment)
               by clearly specifying how it is directed."""@en
    ], [
        dc:date "2023-11-08" ;
        rdf:value """In order to get a system of rolified Relation classes: added an
               equivalentClass object property; replaced the specific object properties by the
               generic ones in the subClassOf declarations."""@en
    ], [
        dc:date "2023-11-07" ;
        rdf:value """Renamed the relation (its name was
               ProvenanceRelation)."""@en
    ], [
        dc:date "2023-11-02" ;
        rdf:value "Added a new rdfs:label in Spanish."@en
    ], [
        dc:date "2023-08-25" ;
        rdf:value "Added a new rdfs:label in French."@en
    ] ;
    skos:scopeNote """This relation stands for organic and for functional
         provenance."""@en .

:OrganicProvenanceRelation
    a owl:Class ;
    rdfs:comment """Connects at least one Record Resource or an Instantiation to at
         least one Agent that creates or accumulates the Record Resource, receives it, or sends it.
         The Record Resource(s) or Instantiation(s) is the source of the Relation, and the Agent(s)
         is the target."""@en ;
    rdfs:isDefinedBy <https://www.ica.org/standards/RiC/ontology> ;
    rdfs:label "Organic Provenance Relation"@en, "Recordressource/Instanz-Herkunft-Akteur"@de, "Relación de procedencia orgánica"@es, "Relation de provenance organique"@fr ;
    rdfs:subClassOf :OrganicOrFunctionalProvenanceRelation, [
        a owl:Restriction ;
        owl:minQualifiedCardinality "1"^^xsd:nonNegativeInteger ;
        owl:onClass [
            a owl:Class ;
            owl:unionOf (:Instantiation
                :RecordResource
            )
        ] ;
        owl:onProperty :relationHasSource
    ], [
        a owl:Restriction ;
        owl:minQualifiedCardinality "1"^^xsd:nonNegativeInteger ;
        owl:onClass :Agent ;
        owl:onProperty :relationHasTarget
    ] ;
    owl:equivalentClass [
        a owl:Restriction ;
        owl:hasSelf true ;
        owl:onProperty :organicProvenanceRelation_role
    ] ;
    skos:changeNote [
        dc:date "2025-04-08" ;
        rdf:value "Added a new rdfs:label in German."@en
    ], [
        dc:date "2023-12-06" ;
        rdf:value """Improved the description of the Relation class (rdfs:comment)
               by clearly specifying how it is directed."""@en
    ], [
        dc:date "2023-11-12" ;
        rdf:value """Aligned with RiC-CM 1.0: updated the description
               (rdfs:comment), skos:scopeNote."""@en
    ], [
        dc:date "2023-11-08" ;
        rdf:value """In order to get a system of rolified Relation classes: added an
               equivalentClass object property; replaced the specific object properties by the
               generic ones in the subClassOf declarations."""@en
    ], [
        dc:date "2023-11-07" ;
        rdf:value """Renamed the relation in order to make it clearer (its name was
               AgentOriginationRelation)."""@en
    ], [
        dc:date "2023-11-02" ;
        rdf:value "Added a new rdfs:label in Spanish."@en
    ], [
        dc:date "2023-08-25" ;
        rdf:value "Added a new rdfs:label in French."@en
    ] ;
    skos:scopeNote """This is the most general organic provenance relation. Use it to
         connect a record resource or instantiation with an agent only if it is not possible to use
         a narrower, more specific relation, for example Creation Relation."""@en ;
    :RiCCMCorrespondingComponent """Class implementation of RiC-R026 and RiC-R026i
         relations"""@en .

:OwnershipRelation
    a owl:Class ;
    rdfs:comment """Connects at least one Group, Person or Position and at least a
         Thing that these Agent(s) own(s) or owned. The Group(s), Person(s) or Position(s) is the
         source of the Relation, and the Agent(s) is the target."""@en ;
    rdfs:isDefinedBy <https://www.ica.org/standards/RiC/ontology> ;
    rdfs:label "Gruppe/Person/Position-Besitz-Ding"@de, "Ownership Relation"@en, "Relación de posesión"@es, "Relation de propriété"@fr ;
    rdfs:subClassOf :AuthorityRelation, [
        a owl:Restriction ;
        owl:minQualifiedCardinality "1"^^xsd:nonNegativeInteger ;
        owl:onClass [
            a owl:Class ;
            owl:unionOf (:Group
                :Person
                :Position
            )
        ] ;
        owl:onProperty :relationHasSource
    ], [
        a owl:Restriction ;
        owl:minQualifiedCardinality "1"^^xsd:nonNegativeInteger ;
        owl:onClass :Thing ;
        owl:onProperty :relationHasTarget
    ] ;
    owl:equivalentClass [
        a owl:Restriction ;
        owl:hasSelf true ;
        owl:onProperty :ownershipRelation_role
    ] ;
    skos:changeNote [
        dc:date "2025-04-08" ;
        rdf:value "Added a new rdfs:label in German."@en
    ], [
        dc:date "2023-12-06" ;
        rdf:value """Improved the description of the Relation class (rdfs:comment)
               by clearly specifying how it is directed."""@en
    ], [
        dc:date "2023-11-12" ;
        rdf:value """Aligned with RiC-CM 1.0: updated the description
               (rdfs:comment), skos:scopeNote."""@en
    ], [
        dc:date "2023-11-08" ;
        rdf:value """In order to get a system of rolified Relation classes: added an
               equivalentClass object property; replaced the specific object properties by the
               generic ones in the subClassOf declarations."""@en
    ], [
        dc:date "2023-11-02" ;
        rdf:value "Added a new rdfs:label in Spanish."@en
    ], [
        dc:date "2023-08-25" ;
        rdf:value "Added a new rdfs:label in French."@en
    ] ;
    skos:scopeNote """Among other probably more rare use cases for archival
         description, can be used between agents (a person owns a corporate body, a corporate body
         owns a mechanism), or between agents and record resources."""@en ;
    :RiCCMCorrespondingComponent """Class implementation of RiC-R037 and RiC-R037i
         relations"""@en .

:PerformanceRelation
    a owl:Class ;
    rdfs:comment """Connects at least one Activity to at least one Agent that performs
         or performed the activity. The Activity(-ies) is the source of the Relation and the
         Agent(s) is the target."""@en ;
    rdfs:isDefinedBy <https://www.ica.org/standards/RiC/ontology> ;
    rdfs:label "Aktivität-Ausführung-Akteur"@de, "Performance Relation"@en, "Relación de desarrollo funcional"@es, "Relation entre activités et agents"@fr ;
    rdfs:subClassOf :EventRelation, [
        a owl:Restriction ;
        owl:minQualifiedCardinality "1"^^xsd:nonNegativeInteger ;
        owl:onClass :Activity ;
        owl:onProperty :relationHasSource
    ], [
        a owl:Restriction ;
        owl:minQualifiedCardinality "1"^^xsd:nonNegativeInteger ;
        owl:onClass :Agent ;
        owl:onProperty :relationHasTarget
    ] ;
    owl:equivalentClass [
        a owl:Restriction ;
        owl:hasSelf true ;
        owl:onProperty :performanceRelation_role
    ] ;
    skos:changeNote [
        dc:date "2025-04-08" ;
        rdf:value "Added a new rdfs:label in German."@en
    ], [
        dc:date "2023-12-06" ;
        rdf:value """Improved the description of the Relation class (rdfs:comment)
               by clearly specifying how it is directed."""@en
    ], [
        dc:date "2023-11-12" ;
        rdf:value """Aligned with RiC-CM 1.0: updated the description
               (rdfs:comment)."""@en
    ], [
        dc:date "2023-11-08" ;
        rdf:value """In order to get a system of rolified Relation classes: added an
               equivalentClass object property; replaced the specific object properties by the
               generic ones in the subClassOf declarations."""@en
    ], [
        dc:date "2023-11-02" ;
        rdf:value "Added a new rdfs:label in Spanish."@en
    ], [
        dc:date "2023-08-25" ;
        rdf:value "Added a new rdfs:label in French."@en
    ] ;
    :RiCCMCorrespondingComponent """Class implementation of RiC-R060 and RiC-R060i
         relations"""@en .

:Person
    a owl:Class ;
    rdfs:comment "An individual human being."@en ;
    rdfs:isDefinedBy <https://www.ica.org/standards/RiC/ontology> ;
    rdfs:label "Person"@de, "Person"@en, "Persona"@es, "Personne"@fr ;
    rdfs:subClassOf :Agent ;
    owl:disjointWith :Position ;
    skos:changeNote [
        dc:date "2025-04-08" ;
        rdf:value "Added a new rdfs:label in German."@en
    ], [
        dc:date "2023-11-12" ;
        rdf:value """Aligned with RiC-CM 1.0: updated the description
               (rdfs:comment), skos:scopeNote."""@en
    ], [
        dc:date "2023-11-02" ;
        rdf:value "Added a new rdfs:label in Spanish."@en
    ], [
        dc:date "2023-08-25" ;
        rdf:value "Added a new rdfs:label in French."@en
    ], [
        dc:date "2023-04-19" ;
        rdf:value "Removed the 0.2 existing unnecessary restriction."@en
    ], [
        dc:date "2021-02-08" ;
        rdf:value "Removed one Restriction."@en
    ], [
        dc:date "2020-10-23" ;
        rdf:value """Scope note: made separate paragraphs and updated. Disjoint
               with: enriched. Objective: to make RiC-O compliant with RiC-CM v0.2."""@en
    ], [
        dc:date "2020-10-23" ;
        rdf:value """Scope note: made separate paragraphs and updated. Disjoint
               with: enriched. Objective: to make RiC-O compliant with RiC-CM v0.2."""@en
    ] ;
    skos:scopeNote """Person is a kind of Agent. Most commonly, a human being
         (biological person) has a single socially constructed identity or persona. Less common
         though not rare, one or more personae in addition to the original persona which emerges at
         or near birth may be associated with the human being over the course of that human being’s
         lifetime. Such \"alternative personae\" are most often created by the original person for
         specific purposes. The original persona may, in everyday discourse, be regarded as “the
         real person”. Under some circumstances, an alternative persona might eclipse or replace the
         original person (Mark Twain eclipsing Samuel Clemens; John Wayne eclipsing Marion Mitchell
         Morrison), that is, the alternative identity becomes the predominant identity. Less common
         is when two or more persons collaborate to create a shared persona. A persona shared by two
         or more persons constitutes a kind of group. Within the archival context, the description
         of a person commonly will focus on the original associated persona, with alternative
         personae noted. Exceptionally, an alternative persona may displace the original persona as
         the focus of the description. Under some circumstances, for example, when record resources
         are associated with two or more different personae of one person, describing the different
         personae as separate though related persons may be desirable. Alternatively, a person may
         change their identity over the course of their lifetime."""@en ;
    :RiCCMCorrespondingComponent """Corresponds to RiC-E08 (Person
         entity)"""@en .

:PhysicalLocation
    a owl:Class ;
    rdfs:comment """A delimitation of the physical territory of a
         Place."""@en ;
    rdfs:isDefinedBy <https://www.ica.org/standards/RiC/ontology> ;
    rdfs:label "Localisation physique"@fr, "Localización física de lugar"@es, "Physical Location"@en, "Standort"@de ;
    rdfs:subClassOf :Thing ;
    skos:changeNote [
        dc:date "2025-04-08" ;
        rdf:value "Added a new rdfs:label in German."@en
    ], [
        dc:date "2023-11-12" ;
        rdf:value """Aligned with RiC-CM 1.0: updated the
               skos:scopeNote."""@en
    ], [
        dc:date "2023-11-02" ;
        rdf:value "Added a new rdfs:label in Spanish."@en
    ], [
        dc:date "2023-08-25" ;
        rdf:value "Added a new rdfs:label in French."@en
    ], [
        dc:date "2023-04-19" ;
        rdf:value """Removed the two 0.2 existing unnecessary
               restrictions."""@en
    ] ;
    skos:scopeNote """Used to describe basic human-readable text such as an address, a
         cadastral reference, or less precise information found in a record. Use the coordinates
         datatype property, or the Coordinates class to capture the geographical coordinates of the
         Place. Use spatial relations (particularly 'has or had location') to capture a relation
         between two places."""@en ;
    :RiCCMCorrespondingComponent """Class implementation of RiC-A27 (Location
         attribute)"""@en .

:Place
    a owl:Class ;
    rdfs:comment "Bounded, named geographic area or region."@en ;
    rdfs:isDefinedBy <https://www.ica.org/standards/RiC/ontology> ;
    rdfs:label "Geografikum"@de, "Lieu"@fr, "Lugar"@es, "Place"@en ;
    rdfs:subClassOf :Thing ;
    skos:changeNote [
        dc:date "2025-04-08" ;
        rdf:value "Added a new rdfs:label in German."@en
    ], [
        dc:date "2023-11-12" ;
        rdf:value """Aligned with RiC-CM 1.0: updated the
               skos:scopeNote."""@en
    ], [
        dc:date "2023-11-02" ;
        rdf:value "Added a new rdfs:label in Spanish."@en
    ], [
        dc:date "2023-08-25" ;
        rdf:value "Added a new rdfs:label in French."@en
    ], [
        dc:date "2023-04-19" ;
        rdf:value "Removed the 0.2 existing unnecessary restriction."@en
    ], [
        dc:date "2020-10-23" ;
        rdf:value """Comment: updated. Scope note: updated and made several
               paragraphs. Objective: to make RiC-O compliant with RiC-CM v0.2."""@en
    ] ;
    skos:scopeNote """A jurisdiction is the bounded geographic area within which an
         Agent has the authority to perform specified activities constrained by rules.
         Jurisdictions, man-made structures, and natural features are historical entities. A Place
         thus may have a beginning date and ending date and changing boundaries that result from
         human or natural events. A Place may be systematically referenced to a location on the
         earth (geographic coordinates)."""@en ;
    :RiCCMCorrespondingComponent """Corresponds to RiC-E22 (Place
         entity)"""@en .

:PlaceName
    a owl:Class ;
    rdfs:comment """A label, title or term designating a Place in order to make it
         distinguishable from other similar entities."""@en ;
    rdfs:isDefinedBy <https://www.ica.org/standards/RiC/ontology> ;
    rdfs:label "Geografikumsname"@de, "Nom de lieu"@fr, "Nombre de lugar"@es, "Place Name"@en ;
    rdfs:subClassOf :Name ;
    skos:changeNote [
        dc:date "2025-04-08" ;
        rdf:value "Added a new rdfs:label in German."@en
    ], [
        dc:date "2023-11-02" ;
        rdf:value "Added a new rdfs:label in Spanish."@en
    ], [
        dc:date "2023-08-25" ;
        rdf:value "Added a new rdfs:label in French."@en
    ] ;
    :RiCCMCorrespondingComponent """Class implementation of a specialization of RiC-A28
         (Name attribute)"""@en .

:PlaceRelation
    a owl:Class ;
    rdfs:comment """Connects a Place and at least one Thing when the first is
         associated with the existence and lifecycle of the second one. The Place is the source of
         the Relation and the Thing(s) is the target."""@en ;
    rdfs:isDefinedBy <https://www.ica.org/standards/RiC/ontology> ;
    rdfs:label "Geografikum-Ding"@de, "Place Relation"@en, "Relación con lugar"@es, "Relation impliquant un lieu"@fr ;
    rdfs:subClassOf :Relation, [
        a owl:Restriction ;
        owl:onClass :Place ;
        owl:onProperty :relationHasSource ;
        owl:qualifiedCardinality "1"^^xsd:nonNegativeInteger
    ], [
        a owl:Restriction ;
        owl:minQualifiedCardinality "1"^^xsd:nonNegativeInteger ;
        owl:onClass :Thing ;
        owl:onProperty :relationHasTarget
    ] ;
    owl:equivalentClass [
        a owl:Restriction ;
        owl:hasSelf true ;
        owl:onProperty :placeRelation_role
    ] ;
    skos:changeNote [
        dc:date "2025-04-08" ;
        rdf:value "Added a new rdfs:label in German."@en
    ], [
        dc:date "2023-12-06" ;
        rdf:value """Improved the description of the Relation class (rdfs:comment)
               by clearly specifying how it is directed."""@en
    ], [
        dc:date "2023-11-08" ;
        rdf:value """In order to get a system of rolified Relation classes: added an
               equivalentClass object property; replaced the specific object properties by the
               generic ones in the subClassOf declarations."""@en
    ], [
        dc:date "2023-11-02" ;
        rdf:value "Added a new rdfs:label in Spanish."@en
    ], [
        dc:date "2023-08-25" ;
        rdf:value "Added a new rdfs:label in French."@en
    ] ;
    :RiCCMCorrespondingComponent """Class implementation of RiC-R074 and RiC-R074i
         relations"""@en .

:PlaceType
    a owl:Class ;
    rdfs:comment "Categorization of a Place."@en ;
    rdfs:isDefinedBy <https://www.ica.org/standards/RiC/ontology> ;
    rdfs:label "Geografikumskategorie"@de, "Place Type"@en, "Tipo de lugar"@es, "Type de lieu"@fr ;
    rdfs:subClassOf :Type ;
    skos:changeNote [
        dc:date "2025-04-08" ;
        rdf:value "Added a new rdfs:label in German."@en
    ], [
        dc:date "2023-11-02" ;
        rdf:value "Added a new rdfs:label in Spanish."@en
    ], [
        dc:date "2023-08-25" ;
        rdf:value "Added a new rdfs:label in French."@en
    ], [
        dc:date "2023-04-19" ;
        rdf:value "Removed the 0.2 existing unnecessary restriction."@en
    ] ;
    skos:scopeNote """Broadly, a Place may be a member of three broad categories:
         jurisdiction, manmade structure, or a natural feature. Each of these three categories can
         subdivided into narrower categories."""@en ;
    :RiCCMCorrespondingComponent """Corresponds to RiC-A32 (Place Type
         attribute)"""@en .

:Position
    a owl:Class ;
    rdfs:comment "The functional role of a Person within a Group."@en ;
    rdfs:isDefinedBy <https://www.ica.org/standards/RiC/ontology> ;
    rdfs:label "Position"@de, "Position"@en, "Poste occupé"@fr, "Puesto"@es ;
    rdfs:subClassOf :Agent ;
    skos:changeNote [
        dc:date "2025-04-08" ;
        rdf:value "Added a new rdfs:label in German."@en
    ], [
        dc:date "2023-11-02" ;
        rdf:value "Added a new rdfs:label in Spanish."@en
    ], [
        dc:date "2023-08-25" ;
        rdf:value "Added a new rdfs:label in French."@en
    ], [
        dc:date "2020-10-23" ;
        rdf:value """Scope note: made separate paragraphs and updated. Disjoint
               with: enriched. Objective: to make RiC-O compliant with RiC-CM v0.2."""@en
    ] ;
    skos:scopeNote """Position is a kind of Agent. Position is the intersection of a
         Person and a Group. Position exists independently of the Person that holds the Position
         within a Group. More than one Person may hold a Position. Position is commonly defined in a
         Mandate, often called a position description or job description. The Mandate may specify
         the work to be performed (Activity) as well as the competencies for performing the
         Activity. A Position is often given a Name. A Position may be tied to a project or to a set
         of tasks and thus have a defined duration. A Position may change over time, as the Group
         that establishes it changes over time. Position is not to be confused with Occupation or
         Activity. Within the records created by a Corporate Body, a Position may be used to
         identify the record sets resulting from activities performed by one or more persons holding
         the Position over time, without necessarily identifying or describing the Person or
         persons, or identifying which records were created by each Person."""@en ;
    :RiCCMCorrespondingComponent """Corresponds to RiC-E12 (Position
         entity)"""@en .

:PositionHoldingRelation
    a owl:Class ;
    rdfs:comment """Connects at least one Person and at least one Position that the
         Person(s) occupies or occupied. The Person is the source of the Relation and the Position
         is the target."""@en ;
    rdfs:isDefinedBy <https://www.ica.org/standards/RiC/ontology> ;
    rdfs:label "Person-Position"@de, "Position Holding Relation"@en, "Relación de ocupación entre una persona y un puesto"@es, "Relation entre une personne et un poste"@fr ;
    rdfs:subClassOf :AgentToAgentRelation, [
        a owl:Restriction ;
        owl:minQualifiedCardinality "1"^^xsd:nonNegativeInteger ;
        owl:onClass :Person ;
        owl:onProperty :relationHasSource
    ], [
        a owl:Restriction ;
        owl:minQualifiedCardinality "1"^^xsd:nonNegativeInteger ;
        owl:onClass :Position ;
        owl:onProperty :relationHasTarget
    ] ;
    owl:equivalentClass [
        a owl:Restriction ;
        owl:hasSelf true ;
        owl:onProperty :positionHoldingRelation_role
    ] ;
    skos:changeNote [
        dc:date "2025-04-08" ;
        rdf:value "Added a new rdfs:label in German."@en
    ], [
        dc:date "2023-12-06" ;
        rdf:value """Improved the description of the Relation class (rdfs:comment)
               by clearly specifying how it is directed."""@en
    ], [
        dc:date "2023-11-12" ;
        rdf:value """Aligned with RiC-CM 1.0: updated the description
               (rdfs:comment)."""@en
    ], [
        dc:date "2023-11-08" ;
        rdf:value """In order to get a system of rolified Relation classes: added an
               equivalentClass object property; replaced the specific object properties by the
               generic ones in the subClassOf declarations."""@en
    ], [
        dc:date "2023-11-02" ;
        rdf:value "Added a new rdfs:label in Spanish."@en
    ], [
        dc:date "2023-08-25" ;
        rdf:value "Added a new rdfs:label in French."@en
    ] ;
    :RiCCMCorrespondingComponent """Class implementation of RiC-R054 and RiC-R054i
         relations"""@en .

:PositionToGroupRelation
    a owl:Class ;
    rdfs:comment """Connects at least one Position and a Group in which the
         position(s) exist(s) or existed, or that is (are) defined by that group's organizational
         structure. The Position(s) is the source of the Relation and the Group is the
         target."""@en ;
    rdfs:isDefinedBy <https://www.ica.org/standards/RiC/ontology> ;
    rdfs:label "Position to Group Relation"@en, "Position-Gruppe"@de, "Relación de ocupación entre un grupo y un puesto"@es, "Relation entre un poste et un groupe"@fr ;
    rdfs:subClassOf :AgentToAgentRelation, [
        a owl:Restriction ;
        owl:minQualifiedCardinality "1"^^xsd:nonNegativeInteger ;
        owl:onClass :Position ;
        owl:onProperty :relationHasSource
    ], [
        a owl:Restriction ;
        owl:onClass :Group ;
        owl:onProperty :relationHasTarget ;
        owl:qualifiedCardinality "1"^^xsd:nonNegativeInteger
    ] ;
    owl:equivalentClass [
        a owl:Restriction ;
        owl:hasSelf true ;
        owl:onProperty :positionToGroupRelation_role
    ] ;
    skos:changeNote [
        dc:date "2025-04-08" ;
        rdf:value "Added a new rdfs:label in German."@en
    ], [
        dc:date "2023-12-06" ;
        rdf:value """Improved the description of the Relation class (rdfs:comment)
               by clearly specifying how it is directed."""@en
    ], [
        dc:date "2023-11-12" ;
        rdf:value """Aligned with RiC-CM 1.0: updated the description
               (rdfs:comment)."""@en
    ], [
        dc:date "2023-11-08" ;
        rdf:value """In order to get a system of rolified Relation classes: added an
               equivalentClass object property; replaced the specific object properties by the
               generic ones in the subClassOf declarations."""@en
    ], [
        dc:date "2023-11-02" ;
        rdf:value "Added a new rdfs:label in Spanish."@en
    ], [
        dc:date "2023-08-25" ;
        rdf:value "Added a new rdfs:label in French."@en
    ] ;
    :RiCCMCorrespondingComponent """Class implementation of RiC-R056 and RiC-R056i
         relations"""@en .

:ProductionTechniqueType
    a owl:Class ;
    rdfs:comment """The method used in the representation of information on an
         instantiation."""@en ;
    rdfs:isDefinedBy <https://www.ica.org/standards/RiC/ontology> ;
    rdfs:label "Herstellungstechnikkategorie"@de, "Production Technique Type"@en, "Tipo de técnica de producción"@es, "Type de technique de production"@fr ;
    rdfs:subClassOf :Type ;
    skos:changeNote [
        dc:date "2025-04-08" ;
        rdf:value "Added a new rdfs:label in German."@en
    ], [
        dc:date "2023-11-12" ;
        rdf:value """Aligned with RiC-CM 1.0: updated the description
               (rdfs:comment)."""@en
    ], [
        dc:date "2023-11-02" ;
        rdf:value "Added a new rdfs:label in Spanish."@en
    ], [
        dc:date "2023-08-25" ;
        rdf:value "Added a new rdfs:label in French."@en
    ], [
        dc:date "2023-04-19" ;
        rdf:value "Removed the 0.2 existing unnecessary restriction."@en
    ], [
        dc:date "2020-10-23" ;
        rdf:value """Comment: updated. Objective: to make RiC-O compliant with
               RiC-CM v0.2."""@en
    ] ;
    :RiCCMCorrespondingComponent """Class implementation of RiC-A33 (Production
         Technique attribute)"""@en .

:Proxy
    a owl:Class ;
    rdfs:comment """A Proxy represents (stands for) a Record Resource as it exists in
         a specific other Record Resource."""@en ;
    rdfs:isDefinedBy <https://www.ica.org/standards/RiC/ontology> ;
    rdfs:label "Proxy"@de, "Proxy"@en, "Proxy"@es, "Proxy"@fr ;
    rdfs:subClassOf :Concept, [
        a owl:Restriction ;
        owl:onClass :RecordResource ;
        owl:onProperty :proxyFor ;
        owl:qualifiedCardinality "1"^^xsd:nonNegativeInteger
    ], [
        a owl:Restriction ;
        owl:onClass :RecordResource ;
        owl:onProperty :proxyIn ;
        owl:qualifiedCardinality "1"^^xsd:nonNegativeInteger
    ] ;
    skos:changeNote [
        dc:date "2025-04-08" ;
        rdf:value "Added a new rdfs:label in German."@en
    ], [
        dc:date "2025-03-04" ;
        rdf:value """Changed range of proxyIn restriction and rdfs:comment to allow
               any Record Resource, not only a Record Set. Also tweaked the scope note to refer to
               the new datatype properties rico:rankInSequence and rico:rankInHierarchy, and to
               generalise it to different kinds of Record Resources."""@en
    ], [
        dc:date "2023-11-02" ;
        rdf:value "Added a new rdfs:label in Spanish."@en
    ], [
        dc:date "2023-08-25" ;
        rdf:value "Added a new rdfs:label in French."@en
    ] ;
    skos:scopeNote """Useful e.g. in conjunction with rico:rankInSequence for
         describing sequences of Records or Record Sets in the context of a Record Set, or of Record
         Parts and Records in the context of a Record; or in conjunction with rico:rankInHierarchy
         for describing hierarchies of Records and/or Record Parts in the context of a Record Set,
         Record, or Record Part. A Record Resource has only one Proxy in the context of one specific
         Record Set, Record, or Record Part. It may have many Proxies simultaneously or through
         time."""@en ;
    :closeTo "ORE Proxy (http://www.openarchives.org/ore/terms/Proxy)"@en .

:Record
    a owl:Class ;
    rdfs:comment """Discrete information content formed and inscribed, at least once,
         by any method on any carrier in any persistent, recoverable form by an Agent in the course
         of life or work activity."""@en ;
    rdfs:isDefinedBy <https://www.ica.org/standards/RiC/ontology> ;
    rdfs:label "Documento"@es, "Objet informationnel"@fr, "Record"@de, "Record"@en ;
    rdfs:subClassOf :RecordResource ;
    skos:changeNote [
        dc:date "2025-04-08" ;
        rdf:value "Added a new rdfs:label in German."@en
    ], [
        dc:date "2023-11-12" ;
        rdf:value """Aligned with RiC-CM 1.0: updated the description
               (rdfs:comment), skos:scopeNote."""@en
    ], [
        dc:date "2023-11-02" ;
        rdf:value "Added a new rdfs:label in Spanish."@en
    ], [
        dc:date "2023-08-25" ;
        rdf:value "Added a new rdfs:label in French."@en
    ], [
        dc:date "2021-02-08" ;
        rdf:value "Removed the Restriction."@en
    ], [
        dc:date "2020-10-23" ;
        rdf:value """Scope note: updated and made several paragraphs. Objective: to
               make RiC-O compliant with RiC-CM v0.2."""@en
    ] ;
    skos:scopeNote """Record is a kind of Record Resource. A Record may itself contain
         one or more Records, or may consist of one or more Record Parts. A Record must have or have
         had at least one Instantiation. A Record may have more than one Instantiation. An
         Instantiation derived from another Instantiation of a Record may be considered the
         instantiation of the same Record or an instantiation of a new Record, depending on the
         context. A Record may serve a variety of purposes, though it always documents or is
         evidence of Activity."""@en ;
    :RiCCMCorrespondingComponent """Corresponds to RiC-E04 (Record
         entity)"""@en .

:RecordPart
    a owl:Class ;
    rdfs:comment """Component of a Record with independent information content that
         contributes to the intellectual completeness of the Record."""@en ;
    rdfs:isDefinedBy <https://www.ica.org/standards/RiC/ontology> ;
    rdfs:label "Componente documental"@es, "Partie d’objet informationnel"@fr, "Record Part"@en, "Recordteil"@de ;
    rdfs:subClassOf :RecordResource ;
    skos:changeNote [
        dc:date "2025-04-08" ;
        rdf:value "Added a new rdfs:label in German."@en
    ], [
        dc:date "2023-11-12" ;
        rdf:value """Aligned with RiC-CM 1.0: updated the description
               (rdfs:comment)."""@en
    ], [
        dc:date "2023-11-02" ;
        rdf:value "Added a new rdfs:label in Spanish."@en
    ], [
        dc:date "2023-08-25" ;
        rdf:value "Added a new rdfs:label in French."@en
    ], [
        dc:date "2021-02-08" ;
        rdf:value "Removed the Restriction."@en
    ], [
        dc:date "2020-10-23" ;
        rdf:value """comment: updated. Scope note: made several paragraphs.
               Objective: to make RiC-O compliant with RiC-CM v0.2."""@en
    ] ;
    skos:scopeNote """Record Part is a kind of Record Resource. A Record Part may
         itself have Record Parts."""@en ;
    :RiCCMCorrespondingComponent """Corresponds to RiC-E05 (Record Part
         entity)"""@en .

:RecordResource
    a owl:Class ;
    rdfs:comment """Information produced or acquired and retained by an Agent in the
         course of life or work activity."""@en ;
    rdfs:isDefinedBy <https://www.ica.org/standards/RiC/ontology> ;
    rdfs:label "Record Resource"@en, "Recordressource"@de, "Recurso documental"@es, "Ressource archivistique"@fr ;
    rdfs:subClassOf :Thing ;
    skos:changeNote [
        dc:date "2025-04-08" ;
        rdf:value "Added a new rdfs:label in German."@en
    ], [
        dc:date "2023-11-12" ;
        rdf:value """Aligned with RiC-CM 1.0: updated the description
               (rdfs:comment), skos:scopeNote."""@en
    ], [
        dc:date "2023-11-02" ;
        rdf:value "Added a new rdfs:label in Spanish."@en
    ], [
        dc:date "2023-08-25" ;
        rdf:value "Added a new rdfs:label in French."@en
    ], [
        dc:date "2023-04-19" ;
        rdf:value "Removed the 0.2 existing unnecessary restriction."@en
    ], [
        dc:date "2021-02-08" ;
        rdf:value "Removed one Restriction."@en
    ], [
        dc:date "2020-10-23" ;
        rdf:value """Scope note: made separate paragraphs plus very few
               changes."""@en
    ] ;
    skos:scopeNote """Record resource is a kind of Thing. Producing a record resource
         may imply either its initial creation or a reuse of previous existing information by
         combination, rearrangement, selecting, reformatting, etc. Record set, record, and record
         part are kinds of record resource. A record resource is evidence of the activity of an
         agent. More than one agent may be involved in the creation of a record resource. The role
         of the agent in creating the record resource may take different forms, for example,
         authoring of an individual record, accumulating a record set, or arranging a record set.
         Though a record, record set, and record part, under most circumstances, may be easily
         distinguished from one another, identifying the boundary of each may frequently present
         particular challenges. Documentary forms provide the rules governing the structure of many
         types of records, providing criteria for identifying a record's boundary, and identifying
         its essential parts. Many records, though, do not have well-established documentary forms,
         particularly in the case of digital records, where it may be difficult to determine whether
         individual elements represented in separate bitstreams are record parts, records, or record
         sets. For example, is photographic information represented independently in a bitstream
         embedded in a text document a record or a record part? Or is the same photographic
         information attached to an email that maintains its independent representation, a record or
         a record part? Information grouped for some purpose, for example, ZIP or TAR \"file
         compression\" for saving storage space, presents a further challenge. One file comprises
         multiple bitstreams subjected to techniques that remove bits that can be losslessly
         recovered when decompressed. Under what circumstances is such a compressed bitstream a
         record or a record set? Determining when an information object is a record, record set, or
         record part is based on perspective and judgement exercised in a particular context. In one
         context, the agent describing an information object may designate it a record, while
         another agent in a different context may designate it a record part. Both designations are
         supported by RiC-CM, and the significance of the difference for users of the records is
         ameliorated by the fact that all of the attributes and relations employed in describing
         record and record part are shared, as are many of the attributes and relations employed in
         describing a record set."""@en ;
    :RiCCMCorrespondingComponent """Corresponds to RiC-E02 (Record Resource
         entity)"""@en .

:RecordResourceExtent
    a owl:Class ;
    rdfs:comment """The quantity of information content, as human experienced,
         contained in a Record Resource."""@en ;
    rdfs:isDefinedBy <https://www.ica.org/standards/RiC/ontology> ;
    rdfs:label "Extensión de recurso documental"@es, "Mesure d’une ressource archivistique"@fr, "Record Resource Extent"@en, "Recordressourceumfang"@de ;
    rdfs:subClassOf :Extent ;
    skos:changeNote [
        dc:date "2025-04-08" ;
        rdf:value "Added a new rdfs:label in German."@en
    ], [
        dc:date "2023-11-12" ;
        rdf:value """Aligned with RiC-CM 1.0: updated the description
               (rdfs:comment), skos:scopeNote."""@en
    ], [
        dc:date "2023-11-02" ;
        rdf:value "Added a new rdfs:label in Spanish."@en
    ], [
        dc:date "2023-08-25" ;
        rdf:value "Added a new rdfs:label in French."@en
    ], [
        dc:date "2020-11-21" ;
        rdf:value """Changed a bit the definition and added change
               notes."""@en
    ], [
        dc:date "2020-10-28" ;
        rdf:value """Class added in order to handle an accurate description of a
               record resource extent"""@en
    ] ;
    skos:scopeNote """The method and precision of expressing the quantity of
         information represented in a Record Resource will vary according to the kind of record
         resource being described, processing economy constraints, etc. For Record Sets, quantity
         may be expressed as number of records, or, for analogue records in particular, by the
         physical storage dimensions of the members of the Record Set. For individual Records or
         Record Parts, quantity may be expressed in more precise terms."""@en ;
    :RiCCMCorrespondingComponent """Class implementation of RiC-A35 (Record Resource
         extent attribute)"""@en .

:RecordResourceGeneticRelation
    a owl:Class ;
    rdfs:comment """Connects two or more record resources when there is a genetic link
         between them. Genetic in this sense is as defined by diplomatics, i.e., the process by
         which a record resource is developed. This Relation is a generic, not oriented
         one."""@en ;
    rdfs:isDefinedBy <https://www.ica.org/standards/RiC/ontology> ;
    rdfs:label "Record Resource Genetic Relation"@en, "Recordressource-Entstehungszusammenhang-Recordressource"@de, "Relación genética entre recursos documentales"@es, "Relation génétique entre des ressources archivistiques"@fr ;
    rdfs:subClassOf :RecordResourceToRecordResourceRelation, [
        a owl:Restriction ;
        owl:minQualifiedCardinality "2"^^xsd:nonNegativeInteger ;
        owl:onClass :RecordResource ;
        owl:onProperty :relationConnects
    ] ;
    owl:equivalentClass [
        a owl:Restriction ;
        owl:hasSelf true ;
        owl:onProperty :recordResourceGeneticRelation_role
    ] ;
    skos:changeNote [
        dc:date "2025-04-08" ;
        rdf:value "Added a new rdfs:label in German."@en
    ], [
        dc:date "2023-12-06" ;
        rdf:value """Improved the description of the Relation class (rdfs:comment)
               by clearly specifying how it is directed."""@en
    ], [
        dc:date "2023-11-12" ;
        rdf:value """Aligned with RiC-CM 1.0: updated the description
               (rdfs:comment)."""@en
    ], [
        dc:date "2023-11-08" ;
        rdf:value """In order to get a system of rolified Relation classes: added an
               equivalentClass object property; replaced the specific object properties by the
               generic ones in the subClassOf declarations."""@en
    ], [
        dc:date "2023-11-02" ;
        rdf:value "Added a new rdfs:label in Spanish."@en
    ], [
        dc:date "2023-08-25" ;
        rdf:value "Added a new rdfs:label in French."@en
    ] ;
    :RiCCMCorrespondingComponent """Class implementation of RiC-R023 and RiC-023i
         relations"""@en .

:RecordResourceHoldingRelation
    a owl:Class ;
    rdfs:comment """Connects at least one Agent and one or more Record Resource or
         Instantiation that the Agent(s) hold(s) or held. The Agent(s) is the source of the Relation
         and the Record Resource(s) or Instantiation is the target."""@en ;
    rdfs:isDefinedBy <https://www.ica.org/standards/RiC/ontology> ;
    rdfs:label "Akteur-Aufbewahrung-Recordressource/Instanz"@de, "Record Resource Holding Relation"@en, """Relación entre agentes y recursos documentales que
         conservan"""@es, """Relation entre agents et ressources archivistiques ou instanciations
         conservées"""@fr ;
    rdfs:subClassOf :ManagementRelation, [
        a owl:Restriction ;
        owl:minQualifiedCardinality "1"^^xsd:nonNegativeInteger ;
        owl:onClass :Agent ;
        owl:onProperty :relationHasSource
    ], [
        a owl:Restriction ;
        owl:minQualifiedCardinality "1"^^xsd:nonNegativeInteger ;
        owl:onClass [
            a owl:Class ;
            owl:unionOf (:Instantiation
                :RecordResource
            )
        ] ;
        owl:onProperty :relationHasTarget
    ] ;
    owl:equivalentClass [
        a owl:Restriction ;
        owl:hasSelf true ;
        owl:onProperty :recordResourceHoldingRelation_role
    ] ;
    skos:changeNote [
        dc:date "2025-04-08" ;
        rdf:value "Added a new rdfs:label in German."@en
    ], [
        dc:date "2023-12-30" ;
        rdf:value "Fixed a typo in the French label."@en
    ], [
        dc:date "2023-12-06" ;
        rdf:value """Improved the description of the Relation class (rdfs:comment)
               by clearly specifying how it is directed."""@en
    ], [
        dc:date "2023-11-12" ;
        rdf:value """Aligned with RiC-CM 1.0: updated the description
               (rdfs:comment)."""@en
    ], [
        dc:date "2023-11-08" ;
        rdf:value """In order to get a system of rolified Relation classes: added an
               equivalentClass object property; replaced the specific object properties by the
               generic ones in the subClassOf declarations."""@en
    ], [
        dc:date "2023-11-02" ;
        rdf:value "Added a new rdfs:label in Spanish."@en
    ], [
        dc:date "2023-08-25" ;
        rdf:value "Added a new rdfs:label in French."@en
    ] ;
    :RiCCMCorrespondingComponent """Class implementation of RiC-R039 and RiC-039i
         relations"""@en .

:RecordResourceToInstantiationRelation
    a owl:Class ;
    rdfs:comment """Connects a Record Resource to one or more Instantiations that
         instantiate it, and which either may exist or may have been lost or destroyed. The Record
         Resource is the source of the Relation and the Instantiation(s) is the
         target."""@en ;
    rdfs:isDefinedBy <https://www.ica.org/standards/RiC/ontology> ;
    rdfs:label "Record Resource to Instantiation Relation"@en, "Recordressource-Repräsentation"@de, "Relación de recurso documental a instanciación"@es, "Relation d’instanciation"@fr ;
    rdfs:subClassOf :Relation, [
        a owl:Restriction ;
        owl:onClass :RecordResource ;
        owl:onProperty :relationHasSource ;
        owl:qualifiedCardinality "1"^^xsd:nonNegativeInteger
    ], [
        a owl:Restriction ;
        owl:minQualifiedCardinality "1"^^xsd:nonNegativeInteger ;
        owl:onClass :Instantiation ;
        owl:onProperty :relationHasTarget
    ] ;
    owl:equivalentClass [
        a owl:Restriction ;
        owl:hasSelf true ;
        owl:onProperty :recordResourceToInstantiationRelation_role
    ] ;
    skos:changeNote [
        dc:date "2025-04-08" ;
        rdf:value "Added a new rdfs:label in German."@en
    ], [
        dc:date "2023-12-06" ;
        rdf:value """Improved the description of the Relation class (rdfs:comment)
               by clearly specifying how it is directed."""@en
    ], [
        dc:date "2023-11-12" ;
        rdf:value """Aligned with RiC-CM 1.0: updated the description
               (rdfs:comment), skos:scopeNote."""@en
    ], [
        dc:date "2023-11-08" ;
        rdf:value """In order to get a system of rolified Relation classes: added an
               equivalentClass object property; replaced the specific object properties by the
               generic ones in the subClassOf declarations."""@en
    ], [
        dc:date "2023-11-02" ;
        rdf:value "Added a new rdfs:label in Spanish."@en
    ], [
        dc:date "2023-08-25" ;
        rdf:value "Added a new rdfs:label in French."@en
    ] ;
    skos:scopeNote """In some situations, it may be useful or necessary to connect a
         record resource to an instantiation that no longer exists or has been lost, when some of
         its characteristics are known from a source, such as an old finding aid."""@en ;
    :RiCCMCorrespondingComponent """Class implementation of RiC-R025 and RiC-R025i
         relations"""@en .

:RecordResourceToRecordResourceRelation
    a owl:Class ;
    rdfs:comment """Connects at least two Record Resources. This Relation is a
         generic, not oriented one."""@en ;
    rdfs:isDefinedBy <https://www.ica.org/standards/RiC/ontology> ;
    rdfs:label "Record Resource to Record Resource Relation"@en, "Recordressource-Recordressource"@de, "Relación entre recursos documentales"@es, "Relation entre ressources archivistiques"@fr ;
    rdfs:subClassOf :Relation, [
        a owl:Restriction ;
        owl:minQualifiedCardinality "2"^^xsd:nonNegativeInteger ;
        owl:onClass :RecordResource ;
        owl:onProperty :relationConnects
    ] ;
    owl:equivalentClass [
        a owl:Restriction ;
        owl:hasSelf true ;
        owl:onProperty :recordResourceToRecordResourceRelation_role
    ] ;
    skos:changeNote [
        dc:date "2025-04-08" ;
        rdf:value "Added a new rdfs:label in German."@en
    ], [
        dc:date "2023-12-06" ;
        rdf:value """Improved the description of the Relation class (rdfs:comment)
               by clearly specifying how it is directed."""@en
    ], [
        dc:date "2023-11-12" ;
        rdf:value """Aligned with RiC-CM 1.0: updated the
               skos:scopeNote."""@en
    ], [
        dc:date "2023-11-08" ;
        rdf:value """In order to get a system of rolified Relation classes: added an
               equivalentClass object property; replaced the specific object properties by the
               generic ones in the subClassOf declarations."""@en
    ], [
        dc:date "2023-11-02" ;
        rdf:value "Added a new rdfs:label in Spanish."@en
    ], [
        dc:date "2023-08-25" ;
        rdf:value "Added a new rdfs:label in French."@en
    ] ;
    skos:scopeNote """Use to connect two record resources only if it is not possible
         to use a narrower, more specific relation, for example
         RecordResourceGeneticRelation."""@en ;
    :RiCCMCorrespondingComponent """Class implementation of RiC-R022 and RiC-022i
         relations"""@en .

:RecordSet
    a owl:Class ;
    rdfs:comment """One or more records that are grouped together by an Agent based on
         the records sharing one or more attributes or relations."""@en ;
    rdfs:isDefinedBy <https://www.ica.org/standards/RiC/ontology> ;
    rdfs:label "Agrupación documental"@es, "Ensemble d’objets informationnels"@fr, "Record Set"@en, "Recordgruppe"@de ;
    rdfs:subClassOf :RecordResource ;
    skos:changeNote [
        dc:date "2025-04-08" ;
        rdf:value "Added a new rdfs:label in German."@en
    ], [
        dc:date "2023-11-12" ;
        rdf:value """Aligned with RiC-CM 1.0: updated the description
               (rdfs:comment), skos:scopeNote."""@en
    ], [
        dc:date "2023-11-02" ;
        rdf:value "Added a new rdfs:label in Spanish."@en
    ], [
        dc:date "2023-08-25" ;
        rdf:value "Added a new rdfs:label in French."@en
    ], [
        dc:date "2023-04-19" ;
        rdf:value "Removed the 0.2 existing unnecessary restriction."@en
    ], [
        dc:date "2020-10-23" ;
        rdf:value """comment: updated. Scope note: updated and made several
               paragraphs. Objective: to make RiC-O compliant with RiC-CM v0.2."""@en
    ] ;
    skos:scopeNote """Record set is a kind of Record Resource. The member records in a
         Record Set may physically reside together, though physical proximity is not essential. In a
         particular context, an Agent (for example, administrator, records manager, archivist,
         end-user, etc.) may select the member records of a Record Set based on any shared attribute
         or attributes, or any shared relation or relations. The grouping of the records serves a
         purpose or purposes specific to the context of the Agent. For example, all member records
         of a Record Set have been accumulated by the same Agent; have the same Documentary Form
         Type; or are related to and document the same Activity. A Record Set may represent the act
         of classifying the records in accordance with a formal classification scheme that may be
         based on activity, subject, organizational structure, or other criteria; an act of archival
         arrangement (for example, based on common provenance); or some other selection and grouping
         that fulfils a particular purpose or purposes (for example, a classification that reflects
         or supports the purposes of a researcher). By exception, some records are brought together
         based on their not belonging in the context of selection to other designated groups: a
         'Miscellaneous' series, for example. A Record Sset accumulated by an Agent in the course of
         life or work activity should be described in a manner that preserves context and evidential
         value. Record Sets may also contain other Record Sets. A Record Set or Record may
         simultaneously be a member of more than one Record Set, and over the course of its
         existence, a Record Set or Record may be a member of an indeterminate number of Record Sets
         in an indeterminate number of contexts. Record Sets and Records contained within a Record
         Set may be ordered into a sequence based on a common property or relation, or common
         properties or relations (for example, alphabetical by agent or related place);
         chronological order by creation date; or some other criterion (for example, an imposed
         order by relevance)."""@en ;
    :RiCCMCorrespondingComponent """Corresponds to RiC-E03 (Record Set
         entity)"""@en .

:RecordSetType
    a owl:Class ;
    rdfs:comment "A broad categorization of the type of Record Set."@en ;
    rdfs:isDefinedBy <https://www.ica.org/standards/RiC/ontology> ;
    rdfs:label "Record Set Type"@en, "Recordgruppenkategorie"@de, "Tipo de agrupación documental"@es, "Type d’ensemble d’objets informationnels"@fr ;
    rdfs:subClassOf :Type ;
    skos:changeNote [
        dc:date "2025-04-08" ;
        rdf:value "Added a new rdfs:label in German."@en
    ], [
        dc:date "2023-11-12" ;
        rdf:value """Aligned with RiC-CM 1.0: updated the
               skos:scopeNote."""@en
    ], [
        dc:date "2023-11-02" ;
        rdf:value "Added a new rdfs:label in Spanish."@en
    ], [
        dc:date "2023-08-25" ;
        rdf:value "Added a new rdfs:label in French."@en
    ], [
        dc:date "2023-04-19" ;
        rdf:value "Removed the 0.2 existing unnecessary restriction."@en
    ], [
        dc:date "2020-10-23" ;
        rdf:value """scope note: updated. Objective: to make RiC-O compliant with
               RiC-CM v0.2."""@en
    ] ;
    skos:scopeNote """Four instances of Record Set Type are included for now in RiC-O;
         they also are instances of skos:Concept and, as such, part of a SKOS vocabulary. Record Set
         Type may also be used (or extended) to categorize types of Record Set that have not
         traditionally been considered archival, e.g. search result list."""@en ;
    :RiCCMCorrespondingComponent """Corresponds to RiC-A36 (Record Set Type
         attribute)"""@en .

:RecordState
    a owl:Class ;
    rdfs:comment """Description of the production or reproduction status of a Record
         or Record Part."""@en ;
    rdfs:isDefinedBy <https://www.ica.org/standards/RiC/ontology> ;
    rdfs:label "Estado de documento"@es, "Record State"@en, "Recordstatus"@de, "État d’un objet informationnel"@fr ;
    rdfs:subClassOf :Type ;
    skos:changeNote [
        dc:date "2025-04-08" ;
        rdf:value "Added a new rdfs:label in German."@en
    ], [
        dc:date "2023-11-12" ;
        rdf:value """Aligned with RiC-CM 1.0: updated the description
               (rdfs:comment), skos:scopeNote."""@en
    ], [
        dc:date "2023-11-02" ;
        rdf:value "Added a new rdfs:label in Spanish."@en
    ], [
        dc:date "2023-08-25" ;
        rdf:value "Added a new rdfs:label in French."@en
    ], [
        dc:date "2020-12-28" ;
        rdf:value """IRI and label changed (RecordResourceState to RecordState), as
               well as textual definition."""@en
    ], [
        dc:date "2020-10-23" ;
        rdf:value """scope note: updated. Objective: to make RiC-O compliant with
               RiC-CM v0.2."""@en
    ] ;
    skos:scopeNote """Can refer both to a record's stage of creation (for example
         \"draft\") and its form of transmission when the record was received (for example
         \"copy\")."""@en ;
    :RiCCMCorrespondingComponent """Corresponds to RiC-A39 (State
         attribute)"""@en .

:Relation
    a owl:Class ;
    rdfs:comment """The top level relation class. It connects at least two Things. An
         instance of a Relation may have some datatype and object properties: a general description
         (datatype property) like any Thing; a certainty (for 'certain', 'quite probable',
         'uncertain','unknown'); a date (use either the date datatype property or the Date class and
         isAssociatedWithDate object property); a state (relationState); a location (use the Place
         class and isAssociatedWithPlace object property); a source of information that can be used
         as an evidence for it (use either source datatype property or hasSource object property).
         This Relation is the most generic one; it is not oriented."""@en ;
    rdfs:isDefinedBy <https://www.ica.org/standards/RiC/ontology> ;
    rdfs:label "Beziehung"@de, "Relación"@es, "Relation"@en, "Relation"@fr ;
    rdfs:subClassOf :Thing ;
    owl:equivalentClass [
        a owl:Restriction ;
        owl:hasSelf true ;
        owl:onProperty :relation_role
    ] ;
    skos:changeNote [
        dc:date "2025-04-08" ;
        rdf:value "Added a new rdfs:label in German."@en
    ], [
        dc:date "2023-12-06" ;
        rdf:value """Improved the description of the Relation class (rdfs:comment)
               by clearly specifying how it is directed."""@en
    ], [
        dc:date "2023-11-12" ;
        rdf:value """Aligned with RiC-CM 1.0: updated the description
               (rdfs:comment)."""@en
    ], [
        dc:date "2023-11-08" ;
        rdf:value "added the equivalence to relation_role."@en
    ], [
        dc:date "2023-11-02" ;
        rdf:value "Added a new rdfs:label in Spanish."@en
    ], [
        dc:date "2023-08-25" ;
        rdf:value "Added a new rdfs:label in French."@en
    ], [
        dc:date "2021-02-08" ;
        rdf:value """Removed the restrictions; completed the definition and scope
               note."""@en
    ] ;
    skos:scopeNote """Use when direct, binary object properties are not enough, e.g.
         when you need to record a date, a location or any other descriptive element for a relation
         (till RDF-Star becomes a W3C recommendation and provides a lighter method for doing so); or
         when the relation invloves more than two entities (n-ary relation). It is recommended to
         use the subclasses of the Relation class."""@en .

:RepresentationType
    a owl:Class ;
    rdfs:comment """Method of recording the content type of an
         Instantiation"""@en ;
    rdfs:isDefinedBy <https://www.ica.org/standards/RiC/ontology> ;
    rdfs:label "Representation Type"@en, "Repräsentationskategorie"@de, "Tipo de grabación"@es, "Type de représentation"@fr ;
    rdfs:subClassOf :Type ;
    skos:changeNote [
        dc:date "2025-04-08" ;
        rdf:value "Added a new rdfs:label in German."@en
    ], [
        dc:date "2023-11-12" ;
        rdf:value """Aligned with RiC-CM 1.0: updated the description
               (rdfs:comment), skos:scopeNote."""@en
    ], [
        dc:date "2023-11-02" ;
        rdf:value "Added a new rdfs:label in Spanish."@en
    ], [
        dc:date "2023-08-25" ;
        rdf:value "Added a new rdfs:label in French."@en
    ], [
        dc:date "2023-04-19" ;
        rdf:value "Removed the 0.2 existing unnecessary restriction."@en
    ], [
        dc:date "2020-10-23" ;
        rdf:value """Comment and scope note: updated. Objective: to make RiC-O
               compliant with RiC-CM v0.2."""@en
    ] ;
    skos:scopeNote """Can be unmediated (which allows humans to receive the message
         communicated without an intermediation of a device) and mediated (which needs a device to
         decode the message). A lot of contemporary mediated types are digital. Each representation
         type may present specific features: bit rate for audio, resolution for digital images,
         encoding format for video etc. Depending on the type, specific attributes may be added to
         describe their characteristics."""@en ;
    :RiCCMCorrespondingComponent """Corresponds to RiC-A37 (Representation Type
         attribute)"""@en .

:RiCCMCorrespondingComponent
    a owl:AnnotationProperty ;
    rdfs:comment """When it exists, specifies the identifier and name of RiC-CM
         component that corresponds to the annotated class or property."""@en ;
    rdfs:isDefinedBy <https://www.ica.org/standards/RiC/ontology> ;
    rdfs:label "RiC-CM corresponding component"@en, "componente correspondiente en RiC-CM"@es, "composant correspondant dans RiC-CM"@fr ;
    rdfs:subPropertyOf rdfs:comment ;
    skos:changeNote [
        dc:date "2023-11-25" ;
        rdf:value "Added a new rdfs:label in Spanish."@en
    ], [
        dc:date "2023-08-28" ;
        rdf:value "Added a new rdfs:label in French."@en
    ] .

:RoleType
    a owl:Class ;
    rdfs:comment """The role an Agent plays in some context (usually in some creation
         relation). Not to be confused with a Position (position of an agent in some group). For
         example, a Person who is the head of some Corporate Body may play the role of annotator (of
         a record) in a creation relation."""@en ;
    rdfs:isDefinedBy <https://www.ica.org/standards/RiC/ontology> ;
    rdfs:label "Role Type"@en, "Rollenkategorie"@de, "Tipo de rol"@es, "Type de rôle"@fr ;
    rdfs:subClassOf :Type ;
    skos:changeNote [
        dc:date "2025-04-08" ;
        rdf:value "Added a new rdfs:label in German."@en
    ], [
        dc:date "2023-11-02" ;
        rdf:value "Added a new rdfs:label in Spanish."@en
    ], [
        dc:date "2023-08-25" ;
        rdf:value "Added a new rdfs:label in French."@en
    ] .

:Rule
    a owl:Class ;
    rdfs:comment """Conditions that govern the existence, responsibility, or authority
         of an Agent; or the performance of an Activity by an Agent; or that contribute to the
         distinct characteristics of things created or managed by an Agent."""@en ;
    rdfs:isDefinedBy <https://www.ica.org/standards/RiC/ontology> ;
    rdfs:label "Regel"@de, "Regla"@es, "Rule"@en, "Règle"@fr ;
    rdfs:subClassOf :Thing ;
    skos:changeNote [
        dc:date "2025-04-08" ;
        rdf:value "Added a new rdfs:label in German."@en
    ], [
        dc:date "2023-11-12" ;
        rdf:value """Aligned with RiC-CM 1.0: updated the description
               (rdfs:comment), skos:scopeNote."""@en
    ], [
        dc:date "2023-11-02" ;
        rdf:value "Added a new rdfs:label in Spanish."@en
    ], [
        dc:date "2023-08-25" ;
        rdf:value "Added a new rdfs:label in French."@en
    ], [
        dc:date "2023-04-19" ;
        rdf:value "Removed the 0.2 existing unnecessary restriction."@en
    ], [
        dc:date "2021-02-11" ;
        rdf:value """Updated the definition (rdfs:comment) and scope note, as they
               were recently changed in RiC-CM 0.2 full draft."""@en
    ], [
        dc:date "2020-10-23" ;
        rdf:value """Scope note: made separate paragraphs and updated. Objective: to
               make RiC-O compliant with RiC-CM v0.2."""@en
    ] ;
    skos:scopeNote """Rule is a kind of Thing. Rule can be related directly to agent,
         activity, or anything created or managed by agents, such as a record resource or
         instantiation. A rule may be unwritten or written or otherwise documented. Unwritten rules
         may include though are not limited to the following: social mores, customs, or community
         expectations. Written rules may include though are not limited to the following:
         constitutions, legislation, acts (legal), statutes, legal codes, ordinances, charters,
         mission statements, regulations, policies, procedures, instructions, codes of conduct or
         ethics, professional standards, work assignments, or work plans. The source or sources of
         some rules governing the existence or activity of an agent may be external (for example,
         expressed in elections, social mores, customs, community expectations, laws, regulations,
         standards, and best practice codes), while others may be expressed within the immediate
         context of an agent (for example, policies, or written or verbal instructions). The
         evidence for identifying rules may be found in their entirety in one documentary source
         (for example, a law or regulation) or may be found in two or more sources. Rule should not
         be confused with the one or more documentary sources that serve as evidence of its
         identity. A documentary source is a record."""@en ;
    :RiCCMCorrespondingComponent """Corresponds to RiC-E16 (Rule
         entity)"""@en .

:RuleRelation
    a owl:Class ;
    rdfs:comment """Connects at least one Rule to at least one Thing when it is
         associated with existence and lifecycle of the Thing. The Rule(s) is the source of the
         Relation, and the Thing(s) is the target."""@en ;
    rdfs:isDefinedBy <https://www.ica.org/standards/RiC/ontology> ;
    rdfs:label "Regel-Ding"@de, "Relación con regla"@es, "Relation impliquant une règle"@fr, "Rule Relation"@en ;
    rdfs:subClassOf :Relation, [
        a owl:Restriction ;
        owl:minQualifiedCardinality "1"^^xsd:nonNegativeInteger ;
        owl:onClass :Rule ;
        owl:onProperty :relationHasSource
    ], [
        a owl:Restriction ;
        owl:minQualifiedCardinality "1"^^xsd:nonNegativeInteger ;
        owl:onClass :Thing ;
        owl:onProperty :relationHasTarget
    ] ;
    owl:equivalentClass [
        a owl:Restriction ;
        owl:hasSelf true ;
        owl:onProperty :ruleRelation_role
    ] ;
    skos:changeNote [
        dc:date "2025-04-08" ;
        rdf:value "Added a new rdfs:label in German."@en
    ], [
        dc:date "2023-12-06" ;
        rdf:value """Improved the description of the Relation class (rdfs:comment)
               by clearly specifying how it is directed."""@en
    ], [
        dc:date "2023-11-08" ;
        rdf:value """In order to get a system of rolified Relation classes: added an
               equivalentClass object property; replaced the specific object properties by the
               generic ones in the subClassOf declarations."""@en
    ], [
        dc:date "2023-11-02" ;
        rdf:value "Added a new rdfs:label in Spanish."@en
    ], [
        dc:date "2023-08-25" ;
        rdf:value "Added a new rdfs:label in French."@en
    ] ;
    :RiCCMCorrespondingComponent """Class implementation of RiC-R062 and RiC-R062i
         relations"""@en .

:RuleType
    a owl:Class ;
    rdfs:comment "Categorization of a Rule."@en ;
    rdfs:isDefinedBy <https://www.ica.org/standards/RiC/ontology> ;
    rdfs:label "Regelkategorie"@de, "Rule Type"@en, "Tipo de regla"@es, "Type de règle"@fr ;
    rdfs:subClassOf :Type ;
    skos:changeNote [
        dc:date "2025-04-08" ;
        rdf:value "Added a new rdfs:label in German."@en
    ], [
        dc:date "2023-11-12" ;
        rdf:value """Aligned with RiC-CM 1.0: added a
               rico:RiCCMCorrespondingComponent."""@en
    ], [
        dc:date "2023-11-02" ;
        rdf:value "Added a new rdfs:label in Spanish."@en
    ], [
        dc:date "2023-08-25" ;
        rdf:value "Added a new rdfs:label in French."@en
    ], [
        dc:date "2023-04-19" ;
        rdf:value "Removed the 0.2 existing unnecessary restriction."@en
    ], [
        dc:date "2020-10-19" ;
        rdf:value """Class added along with hasRuleType and isRuleTypeOf object
               properties."""@en
    ] ;
    skos:scopeNote """For example, for rules that can be applied to record resources :
         access rule, use rule, etc."""@en ;
    :RiCCMCorrespondingComponent """Corresponds to RiC-A45 (Rule Type
         attribute)."""@en .

:SequentialRelation
    a owl:Class ;
    rdfs:comment """Connects at least one Thing to at least one other Thing that
         follows or followed it in some sequence. The Relation is oriented from the first Thing(s)
         in the sequence to the following one(s): the first Thing(s) is the source, and the
         following Thing(s) is the target."""@en ;
    rdfs:isDefinedBy <https://www.ica.org/standards/RiC/ontology> ;
    rdfs:label "Ding-Abfolge-Ding"@de, "Relación secuencial"@es, "Relation séquentielle"@fr, "Sequential Relation"@en ;
    rdfs:subClassOf :Relation, [
        a owl:Restriction ;
        owl:minQualifiedCardinality "1"^^xsd:nonNegativeInteger ;
        owl:onClass :Thing ;
        owl:onProperty :relationHasSource
    ], [
        a owl:Restriction ;
        owl:minQualifiedCardinality "1"^^xsd:nonNegativeInteger ;
        owl:onClass :Thing ;
        owl:onProperty :relationHasTarget
    ] ;
    owl:equivalentClass [
        a owl:Restriction ;
        owl:hasSelf true ;
        owl:onProperty :sequentialRelation_role
    ] ;
    skos:changeNote [
        dc:date "2025-04-08" ;
        rdf:value "Added a new rdfs:label in German."@en
    ], [
        dc:date "2023-12-06" ;
        rdf:value """Improved the description of the Relation class (rdfs:comment)
               by clearly specifying how it is directed."""@en
    ], [
        dc:date "2023-11-12" ;
        rdf:value """Aligned with RiC-CM 1.0: updated the description
               (rdfs:comment), skos:scopeNote."""@en
    ], [
        dc:date "2023-11-08" ;
        rdf:value """In order to get a system of rolified Relation classes: added an
               equivalentClass object property; replaced the specific object properties by the
               generic ones in the subClassOf declarations."""@en
    ], [
        dc:date "2023-11-02" ;
        rdf:value "Added a new rdfs:label in Spanish."@en
    ], [
        dc:date "2023-08-25" ;
        rdf:value "Added a new rdfs:label in French."@en
    ] ;
    skos:scopeNote """The relation does not specify the criteria used for ordering the
         sequence. There may be zero to many intermediate entities, ignored or unknown, in the
         sequence between the two connected things. Can be used, for example, for specifying that a
         record \"has next\" another record within a record set."""@en ;
    :RiCCMCorrespondingComponent """Class implementation of RiC-R008 and RiC-R008i
         relations"""@en .

:SiblingRelation
    a owl:Class ;
    rdfs:comment """Connects at least two Persons, when they are siblings. This
         Relation is not oriented."""@en ;
    rdfs:isDefinedBy <https://www.ica.org/standards/RiC/ontology> ;
    rdfs:label "Person-Geschwister"@de, "Relación familiar entre hermanos"@es, "Relation de fratrie"@fr, "Sibling Relation"@en ;
    rdfs:subClassOf :FamilyRelation, [
        a owl:Restriction ;
        owl:minQualifiedCardinality "2"^^xsd:nonNegativeInteger ;
        owl:onClass :Person ;
        owl:onProperty :relationConnects
    ] ;
    owl:equivalentClass [
        a owl:Restriction ;
        owl:hasSelf true ;
        owl:onProperty :siblingRelation_role
    ] ;
    skos:changeNote [
        dc:date "2025-04-08" ;
        rdf:value "Added a new rdfs:label in German."@en
    ], [
        dc:date "2023-12-06" ;
        rdf:value """Improved the description of the Relation class (rdfs:comment)
               by clearly specifying how it is directed."""@en
    ], [
        dc:date "2023-11-08" ;
        rdf:value """In order to get a system of rolified Relation classes: added an
               equivalentClass object property; replaced the specific object properties by the
               generic ones in the subClassOf declarations."""@en
    ], [
        dc:date "2023-11-02" ;
        rdf:value "Added a new rdfs:label in Spanish."@en
    ], [
        dc:date "2023-08-25" ;
        rdf:value "Added a new rdfs:label in French."@en
    ] ;
    :RiCCMCorrespondingComponent """Class implementation of RiC-R048 and RiC-R048i
         relations"""@en .

:SpouseRelation
    a owl:Class ;
    rdfs:comment """Connects at least two Persons, when they are spouses. This
         Relation is not oriented."""@en ;
    rdfs:isDefinedBy <https://www.ica.org/standards/RiC/ontology> ;
    rdfs:label "Person-Ehepartner"@de, "Relación matrimonial entre personas"@es, "Relation matrimoniale"@fr, "Spouse Relation"@en ;
    rdfs:subClassOf :FamilyRelation, [
        a owl:Restriction ;
        owl:minQualifiedCardinality "2"^^xsd:nonNegativeInteger ;
        owl:onClass :Person ;
        owl:onProperty :relationConnects
    ] ;
    owl:equivalentClass [
        a owl:Restriction ;
        owl:hasSelf true ;
        owl:onProperty :spouseRelation_role
    ] ;
    skos:changeNote [
        dc:date "2025-04-08" ;
        rdf:value "Added a new rdfs:label in German."@en
    ], [
        dc:date "2023-12-06" ;
        rdf:value """Improved the description of the Relation class (rdfs:comment)
               by clearly specifying how it is directed."""@en
    ], [
        dc:date "2023-11-08" ;
        rdf:value """In order to get a system of rolified Relation classes: added an
               equivalentClass object property; replaced the specific object properties by the
               generic ones in the subClassOf declarations."""@en
    ], [
        dc:date "2023-11-02" ;
        rdf:value "Added a new rdfs:label in Spanish."@en
    ], [
        dc:date "2023-08-25" ;
        rdf:value "Added a new rdfs:label in French."@en
    ] ;
    :RiCCMCorrespondingComponent """Class implementation of RiC-R049 and RiC-R049i
         relations"""@en .

:StudyAtRelation
    a owl:Class ;
    rdfs:comment """Connects a Group (as an educational institution) to at least one
         Person who studied or study at this group. Both 'institution' and 'at' can be interpreted
         broadly. The Relation is oriented from the educational institution to the student(s): the
         former is the source of the Relation, and the latter is/are the target."""@en ;
    rdfs:isDefinedBy <https://www.ica.org/standards/RiC/ontology> ;
    rdfs:label "Relación entre institución educativa y estudiantes"@es, "Relation entre institution d’enseignement et étudiants"@fr, "Studium-An-Beziehung"@de, "Study At Relation"@en ;
    rdfs:subClassOf :MembershipRelation, [
        a owl:Restriction ;
        owl:onClass :Group ;
        owl:onProperty :relationHasSource ;
        owl:qualifiedCardinality "1"^^xsd:nonNegativeInteger
    ], [
        a owl:Restriction ;
        owl:minQualifiedCardinality "1"^^xsd:nonNegativeInteger ;
        owl:onClass :Person ;
        owl:onProperty :relationHasTarget
    ] ;
    owl:equivalentClass [
        a owl:Restriction ;
        owl:hasSelf true ;
        owl:onProperty :studyAtRelation_role
    ] ;
    skos:changeNote [
        dc:date "2025-04-08" ;
        rdf:value "Added a new rdfs:label in German."@en
    ], [
        dc:date "2024-12-23" ;
        rdf:value """Fixed details in the definition. Added the French and Spanish
               labels."""@en
    ], [
        dc:date "2024-12-19" ;
        rdf:value "Added in RiC-O 1.1."@en
    ] .

:TeachingRelation
    a owl:Class ;
    rdfs:comment """Connects at least one Person to at least another Person who is or
         was their student. The Relation is oriented from the teacher(s) to the student(s): the
         teacher Person(s) is the source of the Relation, and the student Person(s) is the
         target."""@en ;
    rdfs:isDefinedBy <https://www.ica.org/standards/RiC/ontology> ;
    rdfs:label "Person-Student"@de, "Relación académica entre profesor y alumno"@es, "Relation entre enseignants et étudiants"@fr, "Teaching Relation"@en ;
    rdfs:subClassOf :KnowingRelation, [
        a owl:Restriction ;
        owl:minQualifiedCardinality "1"^^xsd:nonNegativeInteger ;
        owl:onClass :Person ;
        owl:onProperty :relationHasSource
    ], [
        a owl:Restriction ;
        owl:minQualifiedCardinality "1"^^xsd:nonNegativeInteger ;
        owl:onClass :Person ;
        owl:onProperty :relationHasTarget
    ] ;
    owl:equivalentClass [
        a owl:Restriction ;
        owl:hasSelf true ;
        owl:onProperty :teachingRelation_role
    ] ;
    skos:changeNote [
        dc:date "2025-04-08" ;
        rdf:value "Added a new rdfs:label in German."@en
    ], [
        dc:date "2023-12-06" ;
        rdf:value """Improved the description of the Relation class (rdfs:comment)
               by clearly specifying how it is directed."""@en
    ], [
        dc:date "2023-11-12" ;
        rdf:value """Aligned with RiC-CM 1.0: updated the description
               (rdfs:comment)."""@en
    ], [
        dc:date "2023-11-08" ;
        rdf:value """In order to get a system of rolified Relation classes: added an
               equivalentClass object property; replaced the specific object properties by the
               generic ones in the subClassOf declarations."""@en
    ], [
        dc:date "2023-11-02" ;
        rdf:value "Added a new rdfs:label in Spanish."@en
    ], [
        dc:date "2023-08-25" ;
        rdf:value "Added a new rdfs:label in French."@en
    ] ;
    :RiCCMCorrespondingComponent """Class implementation of RiC-R053 and RiC-R053i
         relations"""@en .

:TemporalRelation
    a owl:Class ;
    rdfs:comment """Connects at least one Thing to at least one other Thing that
         follows it in chronological order. The Relation is oriented chronologically: the preceding
         Thing(s) is the source of the Relation, the following Thing(s) is the
         target."""@en ;
    rdfs:isDefinedBy <https://www.ica.org/standards/RiC/ontology> ;
    rdfs:label "Ding-Zeitfolge-Ding"@de, "Relación temporal"@es, "Relation temporelle"@fr, "Temporal Relation"@en ;
    rdfs:subClassOf :SequentialRelation, [
        a owl:Restriction ;
        owl:minQualifiedCardinality "1"^^xsd:nonNegativeInteger ;
        owl:onClass :Thing ;
        owl:onProperty :relationHasSource
    ], [
        a owl:Restriction ;
        owl:minQualifiedCardinality "1"^^xsd:nonNegativeInteger ;
        owl:onClass :Thing ;
        owl:onProperty :relationHasTarget
    ] ;
    owl:equivalentClass [
        a owl:Restriction ;
        owl:hasSelf true ;
        owl:onProperty :temporalRelation_role
    ] ;
    skos:changeNote [
        dc:date "2025-04-08" ;
        rdf:value "Added a new rdfs:label in German."@en
    ], [
        dc:date "2023-12-06" ;
        rdf:value """Improved the description of the Relation class (rdfs:comment)
               by clearly specifying how it is directed."""@en
    ], [
        dc:date "2023-11-12" ;
        rdf:value """Aligned with RiC-CM 1.0: updated the
               skos:scopeNote."""@en
    ], [
        dc:date "2023-11-08" ;
        rdf:value """In order to get a system of rolified Relation classes: added an
               equivalentClass object property; replaced the specific object properties by the
               generic ones in the subClassOf declarations."""@en
    ], [
        dc:date "2023-11-02" ;
        rdf:value "Added a new rdfs:label in Spanish."@en
    ], [
        dc:date "2023-08-25" ;
        rdf:value "Added a new rdfs:label in French."@en
    ] ;
    skos:scopeNote """There may be zero to many intermediate entities, ignored or
         unknown, in the chronological sequence between the connected entities."""@en ;
    :RiCCMCorrespondingComponent """Class implementation of RiC-R009 and RiC-R009i
         relations"""@en .

:Thing
    a owl:Class ;
    rdfs:comment """Any idea, material thing, or event within the realm of human
         experience."""@en ;
    rdfs:isDefinedBy <https://www.ica.org/standards/RiC/ontology> ;
    rdfs:label "Chose"@fr, "Cosa"@es, "Ding"@de, "Thing"@en ;
    skos:changeNote [
        dc:date "2025-04-08" ;
        rdf:value "Added a new rdfs:label in German."@en
    ], [
        dc:date "2023-11-02" ;
        rdf:value "Added a new rdfs:label in Spanish."@en
    ], [
        dc:date "2023-08-25" ;
        rdf:value "Added a new rdfs:label in French."@en
    ], [
        dc:date "2020-10-23" ;
        rdf:value "made separate paragraphs in the scope note."@en
    ] ;
    skos:scopeNote """Includes all RiC entities as well as any concept, material
         thing, or event that may be the subject of a Record Resource or associated with an
         Activity. Examples of entities not explicitly addressed in RiC includes but is not limited
         to the following: abstract concepts; cultural movements, named periods and events; named
         things, objects and works; legendary, mythical or fictitious figures, characters or
         beings."""@en ;
    :RiCCMCorrespondingComponent """Corresponds to RiC-E01 (Thing
         entity)"""@en .

:Title
    a owl:Class ;
    rdfs:comment "A name that is used for a Record Resource or a Rule"@en ;
    rdfs:isDefinedBy <https://www.ica.org/standards/RiC/ontology> ;
    rdfs:label "Intitulé"@fr, "Titel"@de, "Title"@en, "Título"@es ;
    rdfs:subClassOf :Name ;
    skos:changeNote [
        dc:date "2025-04-08" ;
        rdf:value "Added a new rdfs:label in German."@en
    ], [
        dc:date "2023-11-02" ;
        rdf:value "Added a new rdfs:label in Spanish."@en
    ], [
        dc:date "2023-08-25" ;
        rdf:value "Added a new rdfs:label in French."@en
    ] ;
    :RiCCMCorrespondingComponent """Class implementation of a specialization of RiC-A28
         (Name attribute)"""@en .

:TitleType
    a owl:Class ;
    rdfs:comment "Categorization of a Title."@en ;
    rdfs:isDefinedBy <https://www.ica.org/standards/RiC/ontology> ;
    rdfs:label "Tipo de título"@es, "Titelkategorie"@de, "Title Type"@en, "Type de titre"@fr ;
    rdfs:subClassOf :Type ;
    skos:changeNote [
        dc:date "2025-04-08" ;
        rdf:value "Added a new rdfs:label in German."@en
    ], [
        dc:date "2024-10-04" ;
        rdf:value """Class added along with hasTitleType and isTitleTypeOf object
               properties."""@en
    ] ;
    skos:scopeNote """For example, 'obsolete title' ; 'title on the original' ;
         'anonimised title'"""@en .

:Type
    a owl:Class ;
    rdfs:comment """A superclass for any type of some thing. A type characterizes an
         entity."""@en ;
    rdfs:isDefinedBy <https://www.ica.org/standards/RiC/ontology> ;
    rdfs:label "Kategorie"@de, "Tipo"@es, "Type"@en, "Type"@fr ;
    rdfs:subClassOf :Concept ;
    skos:changeNote [
        dc:date "2025-04-08" ;
        rdf:value "Added a new rdfs:label in German."@en
    ], [
        dc:date "2024-10-10" ;
        rdf:value """Updated the rdfs:comment (replaced the word 'category' with
               'type')."""@en
    ], [
        dc:date "2023-11-02" ;
        rdf:value "Added a new rdfs:label in Spanish."@en
    ], [
        dc:date "2023-08-25" ;
        rdf:value "Added a new rdfs:label in French."@en
    ] .

:TypeRelation
    a owl:Class ;
    rdfs:comment """Connects a category (a Type) and at least one Thing that belongs
         to this category. The Type(s) is the source of the Relation, and the Thing(s) is the
         target."""@en ;
    rdfs:isDefinedBy <https://www.ica.org/standards/RiC/ontology> ;
    rdfs:label "Kategorie-Ding"@de, "Relation de catégorisation"@fr, "Tipo de relación"@es, "Type Relation"@en ;
    rdfs:subClassOf :Relation, [
        a owl:Restriction ;
        owl:onClass :Type ;
        owl:onProperty :relationHasSource ;
        owl:qualifiedCardinality "1"^^xsd:nonNegativeInteger
    ], [
        a owl:Restriction ;
        owl:minQualifiedCardinality "1"^^xsd:nonNegativeInteger ;
        owl:onClass :Thing ;
        owl:onProperty :relationHasTarget
    ] ;
    owl:equivalentClass [
        a owl:Restriction ;
        owl:hasSelf true ;
        owl:onProperty :typeRelation_role
    ] ;
    skos:changeNote [
        dc:date "2025-04-08" ;
        rdf:value "Added a new rdfs:label in German."@en
    ], [
        dc:date "2023-12-06" ;
        rdf:value """Improved the description of the Relation class (rdfs:comment)
               by clearly specifying how it is directed."""@en
    ], [
        dc:date "2023-11-08" ;
        rdf:value """In order to get a system of rolified Relation classes: added an
               equivalentClass object property; replaced the specific object properties by the
               generic ones in the subClassOf declarations."""@en
    ], [
        dc:date "2023-11-02" ;
        rdf:value "Added a new rdfs:label in Spanish."@en
    ], [
        dc:date "2023-08-25" ;
        rdf:value "Added a new rdfs:label in French."@en
    ] ;
    skos:scopeNote """May be useful at least for some types (e.g. demographic
         group)"""@en .

:UnitOfMeasurement
    a owl:Class ;
    rdfs:comment """A definite magnitude of a quantity, defined and adopted by
         convention or by law, that is used as a standard for measurement of the same kind of
         quantity. Can be spacial units (cm, m), weight (g, kg), time (s, h), storage (MB, TB) or
         more informal units used in the archival context like number of boxes, pages or
         words."""@en ;
    rdfs:isDefinedBy <https://www.ica.org/standards/RiC/ontology> ;
    rdfs:label "Masseinheit"@de, "Unidad de medida"@es, "Unit Of Measurement"@en, "Unité de mesure"@fr ;
    rdfs:subClassOf :Concept ;
    skos:changeNote [
        dc:date "2025-04-08" ;
        rdf:value "Added a new rdfs:label in German."@en
    ], [
        dc:date "2023-11-02" ;
        rdf:value "Added a new rdfs:label in Spanish."@en
    ], [
        dc:date "2023-08-28" ;
        rdf:value "Added an xml:lang attribute to the rdfs:comment."@en
    ], [
        dc:date "2023-08-25" ;
        rdf:value "Added a new rdfs:label in French."@en
    ], [
        dc:date "2020-10-28" ;
        rdf:value """Class added in order to be able to handle units of measurement
               as full entities."""@en
    ] .

:WholePartRelation
    a owl:Class ;
    rdfs:comment """Connects a Thing to at least one other Thing that is or was a
         portion or division of the whole Thing. The Relation is oriented from the Thing to its
         part(s): the Thing is the source of the Relation, and the part Thing(s) is the
         target."""@en ;
    rdfs:isDefinedBy <https://www.ica.org/standards/RiC/ontology> ;
    rdfs:label "Relación entre todo y parte"@es, "Relation partitive"@fr, "Teil-Ganzes-Beziehung"@de, "Whole Part Relation"@en ;
    rdfs:subClassOf :Relation, [
        a owl:Restriction ;
        owl:onClass :Thing ;
        owl:onProperty :relationHasSource ;
        owl:qualifiedCardinality "1"^^xsd:nonNegativeInteger
    ], [
        a owl:Restriction ;
        owl:minQualifiedCardinality "1"^^xsd:nonNegativeInteger ;
        owl:onClass :Thing ;
        owl:onProperty :relationHasTarget
    ] ;
    owl:equivalentClass [
        a owl:Restriction ;
        owl:hasSelf true ;
        owl:onProperty :wholePartRelation_role
    ] ;
    skos:changeNote [
        dc:date "2025-04-08" ;
        rdf:value "Added a new rdfs:label in German."@en
    ], [
        dc:date "2023-12-06" ;
        rdf:value """Improved the description of the Relation class (rdfs:comment)
               by clearly specifying how it is directed."""@en
    ], [
        dc:date "2023-11-12" ;
        rdf:value """Aligned with RiC-CM 1.0: updated the description
               (rdfs:comment)."""@en
    ], [
        dc:date "2023-11-08" ;
        rdf:value """In order to get a system of rolified Relation classes: added an
               equivalentClass object property; replaced the specific object properties by the
               generic ones in the subClassOf declarations."""@en
    ], [
        dc:date "2023-11-02" ;
        rdf:value "Added a new rdfs:label in Spanish."@en
    ], [
        dc:date "2023-08-25" ;
        rdf:value "Added a new rdfs:label in French."@en
    ] ;
    :RiCCMCorrespondingComponent """Class implementation of RiC-R002 and RiC-R002i
         relations"""@en .

:WorkRelation
    a owl:Class ;
    rdfs:comment """Connects at least two Agents that have or had some type of work
         relation in the course of their activities. This Relation is not oriented."""@en ;
    rdfs:isDefinedBy <https://www.ica.org/standards/RiC/ontology> ;
    rdfs:label "Akteur-Arbeit-Akteur"@de, "Relación profesional"@es, "Relation de travail"@fr, "Work Relation"@en ;
    rdfs:subClassOf :AgentToAgentRelation, [
        a owl:Restriction ;
        owl:minQualifiedCardinality "2"^^xsd:nonNegativeInteger ;
        owl:onClass :Agent ;
        owl:onProperty :relationConnects
    ] ;
    owl:equivalentClass [
        a owl:Restriction ;
        owl:hasSelf true ;
        owl:onProperty :workRelation_role
    ] ;
    skos:changeNote [
        dc:date "2025-04-08" ;
        rdf:value "Added a new rdfs:label in German."@en
    ], [
        dc:date "2023-12-06" ;
        rdf:value """Improved the description of the Relation class (rdfs:comment)
               by clearly specifying how it is directed."""@en
    ], [
        dc:date "2023-11-12" ;
        rdf:value """Aligned with RiC-CM 1.0: updated the description
               (rdfs:comment)."""@en
    ], [
        dc:date "2023-11-08" ;
        rdf:value """In order to get a system of rolified Relation classes: added an
               equivalentClass object property; replaced the specific object properties by the
               generic ones in the subClassOf declarations."""@en
    ], [
        dc:date "2023-11-02" ;
        rdf:value "Added a new rdfs:label in Spanish."@en
    ], [
        dc:date "2023-08-25" ;
        rdf:value "Added a new rdfs:label in French."@en
    ] ;
    :RiCCMCorrespondingComponent """Class implementation of RiC-R046 and RiR046i
         relations"""@en .

:accruals
    a owl:DatatypeProperty ;
    rdfs:comment """Information on the anticipated accession(s) to the Record
         Set."""@en ;
    rdfs:domain :RecordSet ;
    rdfs:isDefinedBy <https://www.ica.org/standards/RiC/ontology> ;
    rdfs:label "accroissements"@fr, "accruals"@en, "ingresos"@es ;
    rdfs:range rdfs:Literal ;
    skos:changeNote [
        dc:date "2023-11-11" ;
        rdf:value """Aligned with RiC-CM 1.0: updated the IRI, mapping to RiC-CM
               (rico:RiCCMCorrespondingComponent), labels, skos:scopeNote, examples
               (skos:example)."""@en
    ], [
        dc:date "2023-11-02" ;
        rdf:value "Added a new rdfs:label in Spanish."@en
    ], [
        dc:date "2023-08-25" ;
        rdf:value "Added a new rdfs:label in French."@en
    ] ;
    skos:example """Accruing - there is an agreement with the creator that additional
         snapshots of their email directory will be accessioned at yearly intervals"""@en, "Non-accruing"@en, "Unknown"@en ;
    skos:scopeNote "See also accrualsStatus"@en ;
    :RiCCMCorrespondingComponent """corresponds to RiC-A01 (Accruals
         attribute)"""@en .

:accrualsStatus
    a owl:DatatypeProperty ;
    rdfs:comment "Information on the status of possible accruals"@en ;
    rdfs:domain :RecordSet ;
    rdfs:isDefinedBy <https://www.ica.org/standards/RiC/ontology> ;
    rdfs:label "accruals status"@en, "estado de los ingresos"@es, "statut des accroissements"@fr ;
    rdfs:range rdfs:Literal ;
    skos:changeNote [
        dc:date "2023-11-11" ;
        rdf:value """Aligned with RiC-CM 1.0: updated the IRI, mapping to RiC-CM
               (rico:RiCCMCorrespondingComponent), labels, description (rdfs:comment),
               skos:scopeNote."""@en
    ], [
        dc:date "2023-11-02" ;
        rdf:value "Added a new rdfs:label in Spanish."@en
    ], [
        dc:date "2023-08-25" ;
        rdf:value "Added a new rdfs:label in French."@en
    ], [
        dc:date "2020-11-01" ;
        rdf:value """scope note : updated. Objective: to make RiC-O compliant with
               RiC-CM v0.2."""@en
    ] ;
    skos:scopeNote """A text statement or single words such as “Closed” to indicate
         that no additional Record Resource will (or is anticipated to) be added to the Record Set;
         “Open” to indicate that additional records or record sets will (or are expected to) be
         added to the Record Set; or “Unknown” to indicate that this information is not available,
         for example. See also accruals"""@en ;
    :RiCCMCorrespondingComponent """specialization of RiC-A01 (Accruals
         attribute)"""@en .

:accumulationDate
    a owl:DatatypeProperty ;
    rdfs:comment """A date at which a Record Resource or Instantiation was or will be
         accumulated."""@en ;
    rdfs:domain [
        a owl:Class ;
        owl:unionOf (:Instantiation
            :RecordResource
        )
    ] ;
    rdfs:isDefinedBy <https://www.ica.org/standards/RiC/ontology> ;
    rdfs:label "accumulation date"@en, "date d’accumulation"@fr, "fecha de acumulación"@es ;
    rdfs:range rdfs:Literal ;
    rdfs:subPropertyOf :date ;
    skos:changeNote [
        dc:date "2025-02-19" ;
        rdf:value "Changed definition (added \"or will be\")."@en
    ], [
        dc:date "2024-12-19" ;
        rdf:value "Added in RiC-O 1.1."@en
    ] ;
    skos:scopeNote """Datatype property analogue of 'hasAccumulationDate', which is
         provided for usability reasons. May be deprecated and removed later on. Use only if you
         don’t use Date classes for handling dates."""@en .

:accumulationRelation_role
    a owl:ObjectProperty ;
    rdfs:comment """Connects an AccumulationRelation to itself. It is a property that
         can stand for an instance of the class when necessary, e.g. when you explore a knowledge
         graph."""@en ;
    rdfs:domain :AccumulationRelation ;
    rdfs:isDefinedBy <https://www.ica.org/standards/RiC/ontology> ;
    rdfs:label "a le rôle de la Relation d’accumulation"@fr, "desempeña el papel de la Relación de Acumulación"@es, "has the role of the Accumulation Relation"@en ;
    rdfs:range :AccumulationRelation ;
    rdfs:subPropertyOf :organicProvenanceRelation_role ;
    skos:changeNote [
        dc:date "2024-08-02" ;
        rdf:value """Removed global reflexivity (leads to
               inconsistency)."""@en
    ], [
        dc:date "2023-11-08" ;
        rdf:value """In order to get a system of rolified Relation classes: created
               the object property, with domain and range the AccumulationRelation rolified class.
               Declared it as reflexive. Declared it(s) superproperty(ies)."""@en
    ] ;
    skos:scopeNote """This property \"rolifies\" the AccumulationRelation class. It
         should be used only when you have to manage instances of the AccumulationRelation class, to
         connect each instance to itself, in order to be able to infer, using OWL-RL and property
         paths, the two shortcuts corresponding to this n-ary class."""@en .

:activityDocumentationRelation_role
    a owl:ObjectProperty ;
    rdfs:comment """Connects an ActivityDocumentationRelation to itself. It is a
         property that can stand for an instance of the class when necessary, e.g. when you explore
         a knowledge graph."""@en ;
    rdfs:domain :ActivityDocumentationRelation ;
    rdfs:isDefinedBy <https://www.ica.org/standards/RiC/ontology> ;
    rdfs:label """a le rôle de la Relation entre activités et ressources
         archivistiques"""@fr, """desempeña el papel de la Relación de procedencia
         funcional"""@es, "has the role of the Activity Documentation Relation"@en ;
    rdfs:range :ActivityDocumentationRelation ;
    rdfs:subPropertyOf :eventRelation_role, :organicOrFunctionalProvenanceRelation_role ;
    skos:changeNote [
        dc:date "2024-08-02" ;
        rdf:value """Removed global reflexivity (leads to
               inconsistency)."""@en
    ], [
        dc:date "2023-11-08" ;
        rdf:value """In order to get a system of rolified Relation classes: created
               the object property, with domain and range the ActivityDocumentationRelation rolified
               class. Declared it as reflexive. Declared it(s) superproperty(ies)."""@en
    ] ;
    skos:scopeNote """This property \"rolifies\" the ActivityDocumentationRelation
         class. It should be used only when you have to manage instances of the
         ActivityDocumentationRelation class, to connect each instance to itself, in order to be
         able to infer, using OWL-RL and property paths, the two shortcuts corresponding to this
         n-ary class."""@en .

:activityIsContextOfRelation
    a owl:ObjectProperty ;
    rdfs:comment """Connects an Activity to an Agent Temporal Relation (when the
         Activity is transferred from an Agent to another one) or a Mandate Relation (the Mandate
         assigns the Activity to the Agent or defines it)."""@en ;
    rdfs:domain :Activity ;
    rdfs:isDefinedBy <https://www.ica.org/standards/RiC/ontology> ;
    rdfs:label "actividad es contexto de relación"@es, "activity is context of relation"@en, "activité est le contexte de la relation"@fr ;
    rdfs:range [
        a owl:Class ;
        owl:unionOf (:AgentTemporalRelation
            :MandateRelation
        )
    ] ;
    rdfs:subPropertyOf :thingIsContextOfRelation ;
    owl:inverseOf :asConcernsActivity ;
    skos:changeNote [
        dc:date "2023-11-02" ;
        rdf:value "Added a new rdfs:label in Spanish."@en
    ], [
        dc:date "2023-08-28" ;
        rdf:value "Added a new rdfs:label in French."@en
    ] .

:affectsOrAffected
    a owl:ObjectProperty ;
    rdfs:comment """Connects an Event to a Thing on which the Event has or had some
         significant impact."""@en ;
    rdfs:domain :Event ;
    rdfs:isDefinedBy <https://www.ica.org/standards/RiC/ontology> ;
    rdfs:label "afecta o afectaba a"@es, "affecte ou a affecté"@fr, "affects or affected"@en ;
    rdfs:range :Thing ;
    rdfs:subPropertyOf :hasOrHadParticipant ;
    owl:inverseOf :isOrWasAffectedBy ;
    skos:changeNote [
        dc:date "2023-11-02" ;
        rdf:value "Added a new rdfs:label in Spanish."@en
    ], [
        dc:date "2023-08-28" ;
        rdf:value "Added a new rdfs:label in French."@en
    ], [
        dc:date "2021-01-22" ;
        rdf:value """changed the IRI, label, inverse property IRI, text definition
               and corresponding CM component (changed made in order to make RiC-O compliant with
               RiC-CM 0.2; the name of this property in RiC-O 0.1 was \"affects\")."""@en
    ] ;
    :RiCCMCorrespondingComponent """RiC-R059 ('affects or affected'
         relation)"""@en .

:agentControlRelation_role
    a owl:ObjectProperty ;
    rdfs:comment """Connects an AgentControlRelation to itself. It is a property that
         can stand for an instance of the class when necessary, e.g. when you explore a knowledge
         graph."""@en ;
    rdfs:domain :AgentControlRelation ;
    rdfs:isDefinedBy <https://www.ica.org/standards/RiC/ontology> ;
    rdfs:label "a le rôle de la Relation de contrôle entre agents"@fr, """desempeña el papel de la Relación de control entre
         agentes"""@es, "has the role of the Agent Control Relation"@en ;
    rdfs:range :AgentControlRelation ;
    rdfs:subPropertyOf :agentHierarchicalRelation_role, :authorityRelation_role ;
    skos:changeNote [
        dc:date "2024-08-02" ;
        rdf:value """Removed global reflexivity (leads to
               inconsistency)."""@en
    ], [
        dc:date "2023-11-08" ;
        rdf:value """In order to get a system of rolified Relation classes: created
               the object property, with domain and range the AgentControlRelation rolified class.
               Declared it as reflexive. Declared it(s) superproperty(ies)."""@en
    ] ;
    skos:scopeNote """This property \"rolifies\" the AgentControlRelation class. It
         should be used only when you have to manage instances of the AgentControlRelation class, to
         connect each instance to itself, in order to be able to infer, using OWL-RL and property
         paths, the two shortcuts corresponding to this n-ary class."""@en .

:agentHasOrHadLocation
    a owl:ObjectProperty ;
    rdfs:comment """Inverse of 'is or was location of agent' object
         property."""@en ;
    rdfs:domain :Agent ;
    rdfs:isDefinedBy <https://www.ica.org/standards/RiC/ontology> ;
    rdfs:label "agent a ou a eu pour localisation"@fr, "agent has or had location"@en, "agente tiene o tenía como localización"@es ;
    rdfs:range :Place ;
    rdfs:subPropertyOf :hasOrHadLocation, :isAgentAssociatedWithPlace ;
    owl:inverseOf :isOrWasLocationOfAgent ;
    skos:changeNote [
        dc:date "2023-11-27" ;
        rdf:value "Added a new rdfs:label in Spanish."@en
    ], [
        dc:date "2023-10-26" ;
        rdf:value "Added a rdfs:comment."@en
    ], [
        dc:date "2023-10-20" ;
        rdf:value "Property created for RiC-0 1.0."@en
    ] .

:agentHierarchicalRelation_role
    a owl:ObjectProperty ;
    rdfs:comment """Connects an AgentHierarchicalRelation to itself. It is a property
         that can stand for an instance of the class when necessary, e.g. when you explore a
         knowledge graph."""@en ;
    rdfs:domain :AgentHierarchicalRelation ;
    rdfs:isDefinedBy <https://www.ica.org/standards/RiC/ontology> ;
    rdfs:label "a le rôle de la Relation hiérarchique entre agents"@fr, """desempeña el papel de la Relación jerárquica entre
         agentes"""@es, "has the role of the Agent Hierarchical Relation"@en ;
    rdfs:range :AgentHierarchicalRelation ;
    rdfs:subPropertyOf :agentToAgentRelation_role ;
    skos:changeNote [
        dc:date "2024-08-02" ;
        rdf:value """Removed global reflexivity (leads to
               inconsistency)."""@en
    ], [
        dc:date "2023-11-08" ;
        rdf:value """In order to get a system of rolified Relation classes: created
               the object property, with domain and range the AgentHierarchicalRelation rolified
               class. Declared it as reflexive. Declared it(s) superproperty(ies)."""@en
    ] ;
    skos:scopeNote """This property \"rolifies\" the AgentHierarchicalRelation class. It
         should be used only when you have to manage instances of the AgentHierarchicalRelation
         class, to connect each instance to itself, in order to be able to infer, using OWL-RL and
         property paths, the two shortcuts corresponding to this n-ary class."""@en .

:agentTemporalRelation_role
    a owl:ObjectProperty ;
    rdfs:comment """Connects an AgentTemporalRelation to itself. It is a property that
         can stand for an instance of the class when necessary, e.g. when you explore a knowledge
         graph."""@en ;
    rdfs:domain :AgentTemporalRelation ;
    rdfs:isDefinedBy <https://www.ica.org/standards/RiC/ontology> ;
    rdfs:label "a le rôle de la Relation temporelle entre agents"@fr, """desempeña el papel de la Relación temporal entre
         agentes"""@es, "has the role of the Agent Temporal Relation"@en ;
    rdfs:range :AgentTemporalRelation ;
    rdfs:subPropertyOf :agentToAgentRelation_role, :temporalRelation_role ;
    skos:changeNote [
        dc:date "2024-08-02" ;
        rdf:value """Removed global reflexivity (leads to
               inconsistency)."""@en
    ], [
        dc:date "2023-11-08" ;
        rdf:value """In order to get a system of rolified Relation classes: created
               the object property, with domain and range the AgentTemporalRelation rolified class.
               Declared it as reflexive. Declared it(s) superproperty(ies)."""@en
    ] ;
    skos:scopeNote """This property \"rolifies\" the AgentTemporalRelation class. It
         should be used only when you have to manage instances of the AgentTemporalRelation class,
         to connect each instance to itself, in order to be able to infer, using OWL-RL and property
         paths, the two shortcuts corresponding to this n-ary class."""@en .

:agentToAgentRelation_role
    a owl:ObjectProperty ;
    rdfs:comment """Connects an AgentToAgentRelation to itself. It is a property that
         can stand for an instance of the class when necessary, e.g. when you explore a knowledge
         graph."""@en ;
    rdfs:domain :AgentToAgentRelation ;
    rdfs:isDefinedBy <https://www.ica.org/standards/RiC/ontology> ;
    rdfs:label "a le rôle de la Relation entre agents"@fr, "desempeña el papel de la Relación entre agentes"@es, "has the role of the Agent Relation"@en ;
    rdfs:range :AgentToAgentRelation ;
    rdfs:subPropertyOf :relation_role ;
    skos:changeNote [
        dc:date "2024-08-02" ;
        rdf:value """Removed global reflexivity (leads to
               inconsistency)."""@en
    ], [
        dc:date "2023-11-08" ;
        rdf:value """In order to get a system of rolified Relation classes: created
               the object property, with domain and range the AgentToAgentRelation rolified class.
               Declared it as reflexive. Declared it(s) superproperty(ies)."""@en
    ] ;
    skos:scopeNote """This property \"rolifies\" the AgentToAgentRelation class. It
         should be used only when you have to manage instances of the AgentToAgentRelation class, to
         connect each instance to itself, in order to be able to infer, using OWL-RL and property
         paths, the two shortcuts corresponding to this n-ary class."""@en .

:allMembersWithAccumulationDate
    a owl:DatatypeProperty ;
    rdfs:comment """Date at which all of the present or past members of a Record Set
         were or will be accumulated."""@en ;
    rdfs:domain :RecordSet ;
    rdfs:isDefinedBy <https://www.ica.org/standards/RiC/ontology> ;
    rdfs:label "all members with accumulation date"@en, "des membres ayant tous pour date d’accumulation"@fr, "todos sus miembros como fecha de acumulación"@es ;
    rdfs:range rdfs:Literal ;
    rdfs:subPropertyOf :date ;
    skos:changeNote [
        dc:date "2025-02-19" ;
        rdf:value "Changed definition (added \"or will be\")."@en
    ], [
        dc:date "2024-12-19" ;
        rdf:value "Added in RiC-O 1.1."@en
    ] ;
    skos:scopeNote """Datatype property analogue of
         'hasOrHadAllMembersWithAccumulationDate', which is provided for usability reasons. May be
         deprecated and removed later on. Use only if you don’t use Date classes for handling
         dates."""@en .

:allMembersWithCreationDate
    a owl:DatatypeProperty ;
    rdfs:comment """Date at which all of the present or past members of a Record Set
         were or will be created."""@en ;
    rdfs:domain :RecordSet ;
    rdfs:isDefinedBy <https://www.ica.org/standards/RiC/ontology> ;
    rdfs:label "all members with creation date"@en, "des membres ayant tous pour date de création"@fr, "todos sus miembros como fecha de creación"@es ;
    rdfs:range rdfs:Literal ;
    rdfs:subPropertyOf :beginningDate ;
    skos:changeNote [
        dc:date "2025-02-19" ;
        rdf:value "Changed definition (added \"or will be\")."@en
    ], [
        dc:date "2024-12-19" ;
        rdf:value "Added in RiC-O 1.1."@en
    ] ;
    skos:scopeNote """Datatype property analogue of
         'hasOrHadAllMembersWithCreationDate', which is provided for usability reasons. May be
         deprecated and removed later on. Use only if you don’t use Date classes for handling
         dates."""@en ;
    :RiCCMCorrespondingComponent """RiC-R081i ('has or had all members with creation
         date' relation)."""@en .

:altimetricSystem
    a owl:DatatypeProperty ;
    rdfs:comment "Reference system used for altitude"@en ;
    rdfs:domain :Coordinates ;
    rdfs:isDefinedBy <https://www.ica.org/standards/RiC/ontology> ;
    rdfs:label "altimetric system"@en, "sistema altimétrico"@es, "système altimétrique"@fr ;
    rdfs:range rdfs:Literal ;
    rdfs:subPropertyOf :referenceSystem ;
    skos:changeNote [
        dc:date "2023-11-02" ;
        rdf:value "Added a new rdfs:label in Spanish."@en
    ], [
        dc:date "2023-08-25" ;
        rdf:value "Added a new rdfs:label in French."@en
    ] .

:altitude
    a owl:DatatypeProperty ;
    rdfs:comment """The height of a Place above a reference level, especially above
         sea level."""@en ;
    rdfs:domain :Coordinates ;
    rdfs:isDefinedBy <https://www.ica.org/standards/RiC/ontology> ;
    rdfs:label "altitud"@es, "altitude"@en, "altitude"@fr ;
    rdfs:range rdfs:Literal ;
    rdfs:subPropertyOf :measure ;
    skos:changeNote [
        dc:date "2023-11-02" ;
        rdf:value "Added a new rdfs:label in Spanish."@en
    ], [
        dc:date "2023-08-25" ;
        rdf:value "Added a new rdfs:label in French."@en
    ] ;
    skos:scopeNote """Property of the Coordinates class. If you don't use this class,
         use geographicalCoordinates property, a property of Place class."""@en .

:appellationRelation_role
    a owl:ObjectProperty ;
    rdfs:comment """Connects an AppellationRelation to itself. It is a property that
         can stand for an instance of the class when necessary, e.g. when you explore a knowledge
         graph."""@en ;
    rdfs:domain :AppellationRelation ;
    rdfs:isDefinedBy <https://www.ica.org/standards/RiC/ontology> ;
    rdfs:label "a le rôle de la Relation d’appellation"@fr, "desempeña el papel de la Relación de denominación"@es, "has the role of the Appellation Relation"@en ;
    rdfs:range :AppellationRelation ;
    rdfs:subPropertyOf :relation_role ;
    skos:changeNote [
        dc:date "2024-08-02" ;
        rdf:value """Removed global reflexivity (leads to
               inconsistency)."""@en
    ], [
        dc:date "2023-11-08" ;
        rdf:value """In order to get a system of rolified Relation classes: created
               the object property, with domain and range the AppellationRelation rolified class.
               Declared it as reflexive. Declared it(s) superproperty(ies)."""@en
    ] ;
    skos:scopeNote """This property \"rolifies\" the AppellationRelation class. It
         should be used only when you have to manage instances of the AppellationRelation class, to
         connect each instance to itself, in order to be able to infer, using OWL-RL and property
         paths, the two shortcuts corresponding to this n-ary class."""@en .

:asConcernsActivity
    a owl:ObjectProperty ;
    rdfs:comment """Connects an Agent Temporal Relation or Mandate Relation, to an
         Activity that is, either transferred from an Agent to another one, or assigned by a Mandate
         to an Agent."""@en ;
    rdfs:domain [
        a owl:Class ;
        owl:unionOf (:AgentTemporalRelation
            :MandateRelation
        )
    ] ;
    rdfs:isDefinedBy <https://www.ica.org/standards/RiC/ontology> ;
    rdfs:label "as concerns activity"@en, "en ce qui concerne l’activité"@fr, "en cuanto a actividad"@es ;
    rdfs:range :Activity ;
    rdfs:subPropertyOf :relationHasContext ;
    owl:inverseOf :activityIsContextOfRelation ;
    skos:changeNote [
        dc:date "2023-11-02" ;
        rdf:value "Added a new rdfs:label in Spanish."@en
    ], [
        dc:date "2023-08-28" ;
        rdf:value "Added a new rdfs:label in French."@en
    ] .

:authenticityNote
    a owl:DatatypeProperty ;
    rdfs:comment """Information on the evidence that a Record Resource or
         Instantiation is what it purports to be, was created or sent by the said Agent at the said
         time, and has not been tampered with, corrupted, or forged. """@en ;
    rdfs:domain [
        a owl:Class ;
        owl:unionOf (:Instantiation
            :RecordResource
        )
    ] ;
    rdfs:isDefinedBy <https://www.ica.org/standards/RiC/ontology> ;
    rdfs:label "authenticity note"@en, "nota de autenticidad"@es, "note sur l’authenticité"@fr ;
    rdfs:range rdfs:Literal ;
    rdfs:subPropertyOf :note ;
    skos:changeNote [
        dc:date "2025-01-17" ;
        rdf:value """Made this property a subproperty of the new rico:note datatype
               property. Slightly modified its definition (rdfs:comment)."""@en
    ], [
        dc:date "2023-11-11" ;
        rdf:value """Aligned with RiC-CM 1.0: updated the description
               (rdfs:comment), skos:scopeNote, examples (skos:example)."""@en
    ], [
        dc:date "2023-11-02" ;
        rdf:value "Added a new rdfs:label in Spanish."@en
    ], [
        dc:date "2023-08-25" ;
        rdf:value "Added a new rdfs:label in French."@en
    ], [
        dc:date "2020-11-01" ;
        rdf:value """examples added. Objective: to make RiC-O compliant with RiC-CM
               v0.2."""@en
    ] ;
    skos:example """The deed is digitally signed by the Notary. The electronic
         signature validity cannot be assessed, but the content was not modified from the moment of
         signing."""@en, "The letter is unsigned."@en, "The record bears signatures."@en, "The timestamp exists but cannot be verified."@en ;
    skos:scopeNote """May be used in a Record Set description when its value is shared
         by some or all members of the Record Set. For digital records, it may include results from
         automated means of checking the validity of signatures and timestamp. In particular cases
         it may be contextually related to the state attribute, for example, a document can be an
         original or a copy, either of which can be authentic or a forgery. """@en ;
    :RiCCMCorrespondingComponent """Corresponds to RiC-A03 (Authenticity Note
         attribute)"""@en .

:authorityRelation_role
    a owl:ObjectProperty ;
    rdfs:comment """Connects an AuthorityRelation to itself. It is a property that can
         stand for an instance of the class when necessary, e.g. when you explore a knowledge
         graph."""@en ;
    rdfs:domain :AuthorityRelation ;
    rdfs:isDefinedBy <https://www.ica.org/standards/RiC/ontology> ;
    rdfs:label "a le rôle de la Relation d’autorité"@fr, """desempeña el papel de la Relación de control por parte de
         agentes"""@es, "has the role of the Authority Relation"@en ;
    rdfs:range :AuthorityRelation ;
    rdfs:subPropertyOf :relation_role ;
    skos:changeNote [
        dc:date "2024-08-02" ;
        rdf:value """Removed global reflexivity (leads to
               inconsistency)."""@en
    ], [
        dc:date "2023-11-08" ;
        rdf:value """In order to get a system of rolified Relation classes: created
               the object property, with domain and range the AuthorityRelation rolified class.
               Declared it as reflexive. Declared it(s) superproperty(ies)."""@en
    ] ;
    skos:scopeNote """This property \"rolifies\" the AuthorityRelation class. It should
         be used only when you have to manage instances of the AuthorityRelation class, to connect
         each instance to itself, in order to be able to infer, using OWL-RL and property paths, the
         two shortcuts corresponding to this n-ary class."""@en .

:authorizedBy
    a owl:ObjectProperty ;
    rdfs:comment "Inverse of 'authorizes' object property."@en ;
    rdfs:domain :Agent ;
    rdfs:isDefinedBy <https://www.ica.org/standards/RiC/ontology> ;
    rdfs:label "authorized by"@en, "autorisé par"@fr, "controlado por"@es ;
    rdfs:range :Mandate ;
    rdfs:subPropertyOf :isAssociatedWithRule ;
    owl:inverseOf :authorizes ;
    owl:propertyChainAxiom (:thingIsTargetOfRelation
        :mandateRelation_role
        :relationHasSource
    ) ;
    skos:changeNote [
        dc:date "2023-11-08" ;
        rdf:value """In order to get a system of rolified Relation classes: modified
               the property chain axiom so that it now involves the new mandateRelation_role object
               property."""@en
    ], [
        dc:date "2023-11-02" ;
        rdf:value "Added a new rdfs:label in Spanish."@en
    ], [
        dc:date "2023-08-28" ;
        rdf:value "Added a new rdfs:label in French."@en
    ] ;
    :RiCCMCorrespondingComponent """RiC-R067i ('authorizedBy'
         relation)"""@en .

:authorizes
    a owl:ObjectProperty ;
    rdfs:comment """Connects a Mandate to the Agent that the Mandate gives the
         authority or competencies to act."""@en ;
    rdfs:domain :Mandate ;
    rdfs:isDefinedBy <https://www.ica.org/standards/RiC/ontology> ;
    rdfs:label "authorizes"@en, "autorise"@fr, "controla"@es ;
    rdfs:range :Agent ;
    rdfs:subPropertyOf :isRuleAssociatedWith ;
    owl:inverseOf :authorizedBy ;
    owl:propertyChainAxiom (:thingIsSourceOfRelation
        :mandateRelation_role
        :relationHasTarget
    ) ;
    skos:changeNote [
        dc:date "2023-11-08" ;
        rdf:value """In order to get a system of rolified Relation classes: modified
               the property chain axiom so that it now involves the new mandateRelation_role object
               property."""@en
    ], [
        dc:date "2023-11-02" ;
        rdf:value "Added a new rdfs:label in Spanish."@en
    ], [
        dc:date "2023-08-28" ;
        rdf:value "Added a new rdfs:label in French."@en
    ], [
        dc:date "2021-01-22" ;
        rdf:value "fixed the CM corresponding component name."@en
    ] ;
    :RiCCMCorrespondingComponent """RiC-R067 ('authorizes'
         relation)"""@en .

:authorizingAgent
    a owl:ObjectProperty ;
    rdfs:comment """Connects a Mandate Relation to an Agent that assigns the
         Mandate."""@en ;
    rdfs:domain :MandateRelation ;
    rdfs:isDefinedBy <https://www.ica.org/standards/RiC/ontology> ;
    rdfs:label "authorizing agent"@en, "autorisation donnée par l’agent"@fr, "autorización dada por el agente"@es ;
    rdfs:range :Agent ;
    rdfs:subPropertyOf :relationHasContext ;
    owl:inverseOf :isAuthorizingAgentInMandateRelation ;
    skos:changeNote [
        dc:date "2023-11-13" ;
        rdf:value "Fixed the rdfs:label in Spanish."@en
    ], [
        dc:date "2023-11-02" ;
        rdf:value "Added a new rdfs:label in Spanish."@en
    ], [
        dc:date "2023-08-28" ;
        rdf:value "Added a new rdfs:label in French."@en
    ] .

:authorizingMandate
    a owl:DatatypeProperty ;
    rdfs:comment """Information on a Mandate that authorizes an Agent to perform an
         Activity."""@en ;
    rdfs:domain :Agent ;
    rdfs:isDefinedBy <https://www.ica.org/standards/RiC/ontology> ;
    rdfs:label "authorizing mandate"@en, "mandat"@fr, "norma de control"@es ;
    rdfs:range rdfs:Literal ;
    rdfs:subPropertyOf :ruleFollowed ;
    skos:changeNote [
        dc:date "2023-11-02" ;
        rdf:value "Added a new rdfs:label in Spanish."@en
    ], [
        dc:date "2023-08-25" ;
        rdf:value "Added a new rdfs:label in French."@en
    ] ;
    skos:scopeNote """Provided for usability reasons. May be deprecated and removed
         later on. Use only if you don't use the Mandate class for handling
         mandates."""@en .

:authorshipRelation_role
    a owl:ObjectProperty ;
    rdfs:comment """Connects an AuthorshipRelation to itself. It is a property that
         can stand for an instance of the class when necessary, e.g. when you explore a knowledge
         graph."""@en ;
    rdfs:domain :AuthorshipRelation ;
    rdfs:isDefinedBy <https://www.ica.org/standards/RiC/ontology> ;
    rdfs:label """a le rôle de la Relation de responsabilité
         intellectuelle"""@fr, "desempeña el papel de la Relación de autoría"@es, "has the role of the Authorship Relation"@en ;
    rdfs:range :AuthorshipRelation ;
    rdfs:subPropertyOf :creationRelation_role ;
    skos:changeNote [
        dc:date "2024-08-02" ;
        rdf:value """Removed global reflexivity (leads to
               inconsistency)."""@en
    ], [
        dc:date "2023-11-08" ;
        rdf:value """In order to get a system of rolified Relation classes: created
               the object property, with domain and range the AuthorshipRelation rolified class.
               Declared it as reflexive. Declared it(s) superproperty(ies)."""@en
    ] ;
    skos:scopeNote """This property \"rolifies\" the AuthorshipRelation class. It should
         be used only when you have to manage instances of the AuthorshipRelation class, to connect
         each instance to itself, in order to be able to infer, using OWL-RL and property paths, the
         two shortcuts corresponding to this n-ary class."""@en .

:beginningDate
    a owl:DatatypeProperty ;
    rdfs:comment "Date at which something began."@en ;
    rdfs:domain :Thing ;
    rdfs:isDefinedBy <https://www.ica.org/standards/RiC/ontology> ;
    rdfs:label "beginning date"@en, "date de début"@fr, "fecha de inicio"@es ;
    rdfs:range rdfs:Literal ;
    rdfs:subPropertyOf :date ;
    skos:changeNote [
        dc:date "2023-11-02" ;
        rdf:value "Added a new rdfs:label in Spanish."@en
    ], [
        dc:date "2023-08-25" ;
        rdf:value "Added a new rdfs:label in French."@en
    ] ;
    skos:scopeNote """Provided for usability reasons. May be deprecated and removed
         later on. Use only if you don't use Date classes for handling dates."""@en ;
    :RiCCMCorrespondingComponent """Datatype property specialized implementation of
         RiC-E18 (Date entity)"""@en .

:birthDate
    a owl:DatatypeProperty ;
    rdfs:comment "Date at which a Person was born."@en ;
    rdfs:domain :Person ;
    rdfs:isDefinedBy <https://www.ica.org/standards/RiC/ontology> ;
    rdfs:label "birth date"@en, "date de naissance"@fr, "fecha de nacimiento"@es ;
    rdfs:range rdfs:Literal ;
    rdfs:subPropertyOf :beginningDate ;
    skos:changeNote [
        dc:date "2023-11-02" ;
        rdf:value "Added a new rdfs:label in Spanish."@en
    ], [
        dc:date "2023-08-25" ;
        rdf:value "Added a new rdfs:label in French."@en
    ] ;
    skos:scopeNote """Provided for usability reasons. May be deprecated and removed
         later on. Use only if you don't use Date classes for handling dates."""@en ;
    :RiCCMCorrespondingComponent """Datatype property specialized implementation of
         RiC-E18 (Date entity)"""@en .

:carrierExtent
    a owl:DatatypeProperty ;
    rdfs:comment """Number of physical units and/or physical dimensions of the carrier
         of an Instantiation. In order to manage an Instantiation of a record resource it is
         necessary to note the extent of the carrier as well as that of the Instantiation itself.
         Whether it is necessary to note dimensions, the number of relevant units, or both, depends
         on the nature of the carrier and particular business needs."""@en ;
    rdfs:domain :Instantiation ;
    rdfs:isDefinedBy <https://www.ica.org/standards/RiC/ontology> ;
    rdfs:label "carrier extent"@en, "extensión del soporte"@es, "mesure du support"@fr ;
    rdfs:range rdfs:Literal ;
    rdfs:subPropertyOf :physicalOrLogicalExtent ;
    skos:changeNote [
        dc:date "2023-11-11" ;
        rdf:value """Aligned with RiC-CM 1.0: updated the description
               (rdfs:comment), skos:scopeNote, examples (skos:example)."""@en
    ], [
        dc:date "2023-11-02" ;
        rdf:value "Added a new rdfs:label in Spanish."@en
    ], [
        dc:date "2023-08-25" ;
        rdf:value "Added a new rdfs:label in French."@en
    ], [
        dc:date "2020-11-01" ;
        rdf:value """Text definition and scope note updated. Examples added.
               Objective: to make RiC-O compliant with RiC-CM v0.2."""@en
    ] ;
    skos:example "1 page"@en, "3 GB (1 USB key)"@en, "32.5 x 49 cm (piece of parchment)"@en ;
    skos:scopeNote """For digital resources, it may be used to indicate the size of
         storage capacity (disk, tape, film, etc.). Carrier extent should not be confused with
         instantiation extent or record resource extent. For a given Record Resource, the
         instantiation extent may vary, based on format, density of information on the carrier, etc.
         For example, a CD with a storage capacity of 700 MB (carrier extent) might hold a record of
         1500 words (record resource extent) represented in two versions, one a Word document with
         an instantiation extent of 3 KB and the other a PDF file with an instantiation extent of 5
         KB. """@en ;
    :RiCCMCorrespondingComponent """Corresponds to RiC-A04 (Carrier Extent
         attribute)"""@en .

:childRelation_role
    a owl:ObjectProperty ;
    rdfs:comment """Connects a ChildRelation to itself. It is a property that can
         stand for an instance of the class when necessary, e.g. when you explore a knowledge
         graph."""@en ;
    rdfs:domain :ChildRelation ;
    rdfs:isDefinedBy <https://www.ica.org/standards/RiC/ontology> ;
    rdfs:label "a le rôle de la Relation de filiation"@fr, "desempeña el papel de la Relación de filiación"@es, "has the role of the Child Relation"@en ;
    rdfs:range :ChildRelation ;
    rdfs:subPropertyOf :descendanceRelation_role ;
    skos:changeNote [
        dc:date "2024-08-02" ;
        rdf:value """Removed global reflexivity (leads to
               inconsistency)."""@en
    ], [
        dc:date "2023-11-08" ;
        rdf:value """In order to get a system of rolified Relation classes: created
               the object property, with domain and range the ChildRelation rolified class. Declared
               it as reflexive. Declared it(s) superproperty(ies)."""@en
    ] ;
    skos:scopeNote """This property \"rolifies\" the ChildRelation class. It should be
         used only when you have to manage instances of the ChildRelation class, to connect each
         instance to itself, in order to be able to infer, using OWL-RL and property paths, the two
         shortcuts corresponding to this n-ary class."""@en .

:classification
    a owl:DatatypeProperty ;
    rdfs:comment """A term, number or alphanumeric string that is usually taken from
         an external classification vocabulary or scheme that qualifies a Record
         Resource."""@en ;
    rdfs:domain :RecordResource ;
    rdfs:isDefinedBy <https://www.ica.org/standards/RiC/ontology> ;
    rdfs:label "clasificación"@es, "classification"@en, "classification"@fr ;
    rdfs:range rdfs:Literal ;
    skos:changeNote [
        dc:date "2023-11-11" ;
        rdf:value """Aligned with RiC-CM 1.0: updated the description
               (rdfs:comment), skos:scopeNote, examples (skos:example)."""@en
    ], [
        dc:date "2023-11-02" ;
        rdf:value "Added a new rdfs:label in Spanish."@en
    ], [
        dc:date "2023-08-25" ;
        rdf:value "Added a new rdfs:label in French."@en
    ], [
        dc:date "2020-11-01" ;
        rdf:value """Text definition and scope note updated. Examples added.
               Objective: to make RiC-O compliant with RiC-CM v0.2."""@en
    ] ;
    skos:example """BUD-01-F002 (classification number from a corporate file
         plan)"""@en, "digitized items"@en, "financial affairs"@en, "human resource management"@en, "student registration"@en ;
    skos:scopeNote """May be used in a Record Set description when its value is shared
         by some or all members of the record set. This datatype property is not to be confused with
         Identifier although, in some cases, the information may be the same."""@en ;
    :RiCCMCorrespondingComponent """Corresponds to RiC-A07 (Classification
         attribute)"""@en .

:closeTo
    a owl:AnnotationProperty ;
    rdfs:comment """An annotation property for recording a possible mapping to a
         component in another model or ontology"""@en ;
    rdfs:isDefinedBy <https://www.ica.org/standards/RiC/ontology> ;
    rdfs:label "cerca de"@es, "close to"@en, "proche de"@fr ;
    rdfs:subPropertyOf rdfs:comment ;
    skos:changeNote [
        dc:date "2023-11-25" ;
        rdf:value "Added a new rdfs:label in Spanish."@en
    ], [
        dc:date "2023-08-28" ;
        rdf:value "Added a new rdfs:label in French."@en
    ] .

:conditionsOfAccess
    a owl:DatatypeProperty ;
    rdfs:comment """Terms and circumstances affecting the availability of a Record
         Resource or an Instantiation for consultation."""@en ;
    rdfs:domain [
        a owl:Class ;
        owl:unionOf (:Instantiation
            :RecordResource
        )
    ] ;
    rdfs:isDefinedBy <https://www.ica.org/standards/RiC/ontology> ;
    rdfs:label "condiciones de acceso"@es, "conditions d’accès"@fr, "conditions of access"@en ;
    rdfs:range rdfs:Literal ;
    skos:changeNote [
        dc:date "2023-11-11" ;
        rdf:value """Aligned with RiC-CM 1.0: updated the description
               (rdfs:comment), skos:scopeNote, examples (skos:example)."""@en
    ], [
        dc:date "2023-11-02" ;
        rdf:value "Added a new rdfs:label in Spanish."@en
    ], [
        dc:date "2023-08-25" ;
        rdf:value "Added a new rdfs:label in French."@en
    ], [
        dc:date "2020-11-01" ;
        rdf:value """Text definition and scope note updated. Examples added.
               Objective: to make RiC-O compliant with RiC-CM v0.2."""@en
    ] ;
    skos:example "Acceso libre a través de los terminales de consulta"@es, "Closed as awaiting conservation treatment"@en, "Closed for 30 years"@en, "Closed under data protection legislation"@en, "Open"@en, """Recognita software, min. version 3.0, is needed in order to open
         the file"""@en, """The Archives cannot provide VHS reader to access the content of
         the tape"""@en ;
    skos:scopeNote """May be used in a Record Set description when its value is shared
         by some or all members of the Record Set. The attribute provides information about the
         accessibility of a Record Resource, as well as the physical, technical or legal limitations
         that exist for providing access to it."""@en ;
    :RiCCMCorrespondingComponent """Corresponds to RiC-A08 (Conditions of Access
         attribute)"""@en .

:conditionsOfUse
    a owl:DatatypeProperty ;
    rdfs:comment """Terms and circumstances affecting the use of a Record Resource or
         an Instantiation after access has been provided. Includes conditions governing reproduction
         of the Record Resource under applicable copyright (intellectual property) and/or property
         legislation or due to conservation status."""@en ;
    rdfs:domain [
        a owl:Class ;
        owl:unionOf (:Instantiation
            :RecordResource
        )
    ] ;
    rdfs:isDefinedBy <https://www.ica.org/standards/RiC/ontology> ;
    rdfs:label "condiciones de uso"@es, "conditions d’utilisation"@fr, "conditions of use"@en ;
    rdfs:range rdfs:Literal ;
    skos:changeNote [
        dc:date "2023-11-11" ;
        rdf:value """Aligned with RiC-CM 1.0: updated the description
               (rdfs:comment), skos:scopeNote, examples (skos:example)."""@en
    ], [
        dc:date "2023-11-02" ;
        rdf:value "Added a new rdfs:label in Spanish."@en
    ], [
        dc:date "2023-08-25" ;
        rdf:value "Added a new rdfs:label in French."@en
    ], [
        dc:date "2020-11-01" ;
        rdf:value """Text definition updated. Examples added. Objective: to make
               RiC-O compliant with RiC-CM v0.2."""@en
    ] ;
    skos:example """Cannot be copied using warm light copying machines or photographed
         using flashlight"""@en, """Permission of the copyright owner must be obtained before
         use"""@en ;
    skos:scopeNote """May be used in a Record Set description when its value is shared
         by some or all members of the Record Set."""@en ;
    :RiCCMCorrespondingComponent """Corresponds to RiC-A09 (Conditions of Use
         attribute)"""@en .

:contained
    a owl:ObjectProperty ;
    rdfs:comment """Connects a Place to a Place that it contained in the
         past."""@en ;
    rdfs:domain :Place ;
    rdfs:isDefinedBy <https://www.ica.org/standards/RiC/ontology> ;
    rdfs:label "a contenu"@fr, "contained"@en, "contenía"@es ;
    rdfs:range :Place ;
    rdfs:subPropertyOf :containsOrContained, :hadPart ;
    owl:inverseOf :wasContainedBy ;
    skos:changeNote [
        dc:date "2023-11-27" ;
        rdf:value "Added a new rdfs:label in Spanish."@en
    ], [
        dc:date "2023-11-12" ;
        rdf:value "Updated the labels, description (rdfs:comment)."@en
    ], [
        dc:date "2023-09-05" ;
        rdf:value """Object property added, along with its inverse property, in
               order to enable to express past partitive relations between places (the current
               partitive relations being also added, including a transitive one)."""@en
    ] .

:containsOrContained
    a owl:ObjectProperty ;
    rdfs:comment """Connects a Place to a region that is or was within
         it."""@en ;
    rdfs:domain :Place ;
    rdfs:isDefinedBy <https://www.ica.org/standards/RiC/ontology> ;
    rdfs:label "contains or contained"@en, "contiene o contenía"@es, "contient ou a contenu"@fr ;
    rdfs:range :Place ;
    rdfs:subPropertyOf :hasOrHadPart, :isAssociatedWithPlace, :isPlaceAssociatedWith ;
    owl:inverseOf :isOrWasContainedBy ;
    skos:changeNote [
        dc:date "2023-11-02" ;
        rdf:value "Added a new rdfs:label in Spanish."@en
    ], [
        dc:date "2023-08-28" ;
        rdf:value "Added a new rdfs:label in French."@en
    ], [
        dc:date "2021-01-22" ;
        rdf:value """changed the IRI, label, inverse property IRI, text definition,
               corresponding CM component name ; added a scope note (changed made in order to make
               RiC-O compliant with RiC-CM 0.2; the name of this property in RiC-O 0.1 was
               \"contains\")."""@en
    ] ;
    skos:scopeNote """Use for connecting two geographical or administrative
         regions."""@en ;
    :RiCCMCorrespondingComponent """RiC-R007 ('contains or contained'
         relation)"""@en .

:containsTransitive
    a owl:ObjectProperty, owl:TransitiveProperty ;
    rdfs:comment """Connects a Place to a Place that it contains, directly or
         indirectly. This is a transitive relation."""@en ;
    rdfs:domain :Place ;
    rdfs:isDefinedBy <https://www.ica.org/standards/RiC/ontology> ;
    rdfs:label "contains transitive"@en, "contiene transitivo"@es, "contient transitif"@fr ;
    rdfs:range :Place ;
    rdfs:subPropertyOf :containsOrContained, :hasPartTransitive ;
    owl:inverseOf :isContainedByTransitive ;
    skos:changeNote [
        dc:date "2023-11-27" ;
        rdf:value "Added a new rdfs:label in Spanish."@en
    ], [
        dc:date "2023-11-12" ;
        rdf:value "Updated the description (rdfs:comment) and labels."@en
    ], [
        dc:date "2023-09-05" ;
        rdf:value """Object property added, along with its inverse property, in
               order to enable to express current partitive relations between places (the past
               partitive relation also being added)."""@en
    ] .

:correspondenceRelation_role
    a owl:ObjectProperty ;
    rdfs:comment """Connects a CorrespondenceRelation to itself. It is a property that
         can stand for an instance of the class when necessary, e.g. when you explore a knowledge
         graph."""@en ;
    rdfs:domain :CorrespondenceRelation ;
    rdfs:isDefinedBy <https://www.ica.org/standards/RiC/ontology> ;
    rdfs:label "a le rôle de la Relation épistolaire"@fr, """desempeña el papel de la Relación entre personas por
         correspondencia"""@es, "has the role of the Correspondence Relation"@en ;
    rdfs:range :CorrespondenceRelation ;
    rdfs:subPropertyOf :knowingRelation_role ;
    skos:changeNote [
        dc:date "2024-08-02" ;
        rdf:value """Removed global reflexivity (leads to
               inconsistency)."""@en
    ], [
        dc:date "2023-11-08" ;
        rdf:value """In order to get a system of rolified Relation classes: created
               the object property, with domain and range the CorrespondenceRelation rolified class.
               Declared it as reflexive. Declared it(s) superproperty(ies)."""@en
    ] ;
    skos:scopeNote """This property \"rolifies\" the CorrespondenceRelation class. It
         should be used only when you have to manage instances of the CorrespondenceRelation class,
         to connect each instance to itself, in order to be able to infer, using OWL-RL and property
         paths, the two shortcuts corresponding to this n-ary class."""@en .

:creationDate
    a owl:DatatypeProperty ;
    rdfs:comment """Date at which a Record Resource or Instantiation was or will be
         created."""@en ;
    rdfs:domain [
        a owl:Class ;
        owl:unionOf (:Instantiation
            :RecordResource
        )
    ] ;
    rdfs:isDefinedBy <https://www.ica.org/standards/RiC/ontology> ;
    rdfs:label "creation date"@en, "date de création"@fr, "fecha de creación"@es ;
    rdfs:range rdfs:Literal ;
    rdfs:subPropertyOf :beginningDate ;
    skos:changeNote [
        dc:date "2025-02-19" ;
        rdf:value "Changed definition (added \"or will be\")."@en
    ], [
        dc:date "2024-12-19" ;
        rdf:value "Narrowed the domain to match 'hasCreationDate'."@en
    ], [
        dc:date "2023-11-02" ;
        rdf:value "Added a new rdfs:label in Spanish."@en
    ], [
        dc:date "2023-08-25" ;
        rdf:value "Added a new rdfs:label in French."@en
    ] ;
    skos:scopeNote """Provided for usability reasons. May be deprecated and removed
         later on. Use only if you don't use Date classes for handling dates."""@en ;
    :RiCCMCorrespondingComponent """Datatype property specialized implementation of
         RiC-E18 (Date entity)"""@en .

:creationRelation_role
    a owl:ObjectProperty ;
    rdfs:comment """Connects a CreationRelation to itself. It is a property that can
         stand for an instance of the class when necessary, e.g. when you explore a knowledge
         graph."""@en ;
    rdfs:domain :CreationRelation ;
    rdfs:isDefinedBy <https://www.ica.org/standards/RiC/ontology> ;
    rdfs:label "a le rôle de la Relation de création"@fr, "desempeña el papel de la Relación de creación"@es, "has the role of the Creation Relation"@en ;
    rdfs:range :CreationRelation ;
    rdfs:subPropertyOf :organicProvenanceRelation_role ;
    skos:changeNote [
        dc:date "2024-08-02" ;
        rdf:value """Removed global reflexivity (leads to
               inconsistency)."""@en
    ], [
        dc:date "2023-11-08" ;
        rdf:value """In order to get a system of rolified Relation classes: created
               the object property, with domain and range the CreationRelation rolified class.
               Declared it as reflexive. Declared it(s) superproperty(ies)."""@en
    ] ;
    skos:scopeNote """This property \"rolifies\" the CreationRelation class. It should
         be used only when you have to manage instances of the CreationRelation class, to connect
         each instance to itself, in order to be able to infer, using OWL-RL and property paths, the
         two shortcuts corresponding to this n-ary class."""@en .

:creationWithRole
    a owl:ObjectProperty ;
    rdfs:comment """Connects a Creation Relation to the Role Type that the creator
         Agent(s) has in the creation process"""@en ;
    rdfs:domain :CreationRelation ;
    rdfs:isDefinedBy <https://www.ica.org/standards/RiC/ontology> ;
    rdfs:label "creación con el rol de"@es, "creation with role"@en, "création avec pour rôle"@fr ;
    rdfs:range :RoleType ;
    rdfs:subPropertyOf :relationHasContext ;
    owl:inverseOf :roleIsContextOfCreationRelation ;
    skos:changeNote [
        dc:date "2023-11-02" ;
        rdf:value "Added a new rdfs:label in Spanish."@en
    ], [
        dc:date "2023-08-28" ;
        rdf:value "Added a new rdfs:label in French."@en
    ] .

:date
    a owl:DatatypeProperty ;
    rdfs:comment """Chronological information associated with an entity that
         contributes to its identification and contextualization."""@en ;
    rdfs:domain :Thing ;
    rdfs:isDefinedBy <https://www.ica.org/standards/RiC/ontology> ;
    rdfs:label "date"@en, "date"@fr, "fecha"@es ;
    rdfs:range rdfs:Literal ;
    skos:changeNote [
        dc:date "2023-11-02" ;
        rdf:value "Added a new rdfs:label in Spanish."@en
    ], [
        dc:date "2023-08-25" ;
        rdf:value "Added a new rdfs:label in French."@en
    ] ;
    skos:scopeNote """Provided for usability reasons, like its subproperties. May be
         deprecated and removed later on. Use only if you don't use Date classes for handling
         dates."""@en ;
    :RiCCMCorrespondingComponent """Datatype property implementation of RiC-E18 (Date
         entity)"""@en .

:dateQualifier
    a owl:DatatypeProperty ;
    rdfs:comment """A human readable qualification of a Date to indicate the level of
         precision or certainty."""@en ;
    rdfs:domain :Date ;
    rdfs:isDefinedBy <https://www.ica.org/standards/RiC/ontology> ;
    rdfs:label "calificador de fecha"@es, "date qualifier"@en, "qualificatif de la date"@fr ;
    rdfs:range rdfs:Literal ;
    skos:changeNote [
        dc:date "2023-11-11" ;
        rdf:value """Aligned with RiC-CM 1.0: updated the description
               (rdfs:comment), skos:scopeNote."""@en
    ], [
        dc:date "2023-11-02" ;
        rdf:value "Added a new rdfs:label in Spanish."@en
    ], [
        dc:date "2023-10-10" ;
        rdf:value """Updated the rdfs:comment, skos:scopeNote and examples, in order
               to make this datatype property fully compliant with RiC-CM 1.0"""@en
    ], [
        dc:date "2023-08-25" ;
        rdf:value "Added a new rdfs:label in French."@en
    ], [
        dc:date "2020-11-01" ;
        rdf:value """examples added. Objective: to make RiC-O compliant with RiC-CM
               v0.2."""@en
    ] ;
    skos:example "approximate"@en, "circa"@en, "end unknown"@en ;
    skos:scopeNote """Most often, this human readable expression of the accuracy of
         the date is used along with an ISO 8601 representation of the date. The qualifier can also
         be expressed as a machine-readable value, using the EDTF standard (thus, a specialization
         of the normalizedDateValue datatype property)."""@en ;
    :RiCCMCorrespondingComponent """Corresponds to RiC-A13 (Date Qualifier
         attribute)"""@en .

:deathDate
    a owl:DatatypeProperty ;
    rdfs:comment "Date at which a Person died."@en ;
    rdfs:domain :Person ;
    rdfs:isDefinedBy <https://www.ica.org/standards/RiC/ontology> ;
    rdfs:label "date de décès"@fr, "death date"@en, "fecha de muerte"@es ;
    rdfs:range rdfs:Literal ;
    rdfs:subPropertyOf :endDate ;
    skos:changeNote [
        dc:date "2023-11-02" ;
        rdf:value "Added a new rdfs:label in Spanish."@en
    ], [
        dc:date "2023-08-25" ;
        rdf:value "Added a new rdfs:label in French."@en
    ] ;
    skos:scopeNote """Provided for usability reasons. May be deprecated and removed
         later on. Use only if you don't use Date classes for handling dates."""@en ;
    :RiCCMCorrespondingComponent """Datatype property specialized implementation of
         RiC-E18 (Date entity)"""@en .

:derivationDate
    a owl:DatatypeProperty ;
    rdfs:comment """Date at which an Instantiation was or will be derived from another
         Instantiation."""@en ;
    rdfs:domain :Instantiation ;
    rdfs:isDefinedBy <https://www.ica.org/standards/RiC/ontology> ;
    rdfs:label "date de dérivation"@fr, "derivation date"@en, "fecha de derivación"@es ;
    rdfs:range rdfs:Literal ;
    rdfs:subPropertyOf :date ;
    skos:changeNote [
        dc:date "2025-03-01" ;
        rdf:value "Added in RiC-O 1.1."@en
    ] ;
    skos:scopeNote """Provided for usability reasons. May be deprecated and removed
         later on. Use only if you don't use Date classes for handling dates."""@en ;
    :RiCCMCorrespondingComponent """Datatype property specialized implementation of
         RiC-E18 (Date entity)"""@en .

:derivationRelation_role
    a owl:ObjectProperty ;
    rdfs:comment """Connects a DerivationRelation to itself. It is a property that can
         stand for an instance of the class when necessary, e.g. when you explore a knowledge
         graph."""@en ;
    rdfs:domain :DerivationRelation ;
    rdfs:isDefinedBy <https://www.ica.org/standards/RiC/ontology> ;
    rdfs:label "a le rôle de la Relation de dérivation"@fr, "desempeña el papel de la Relación de derivación"@es, "has the role of the Derivation Relation"@en ;
    rdfs:range :DerivationRelation ;
    rdfs:subPropertyOf :instantiationToInstantiationRelation_role, :temporalRelation_role ;
    skos:changeNote [
        dc:date "2024-08-02" ;
        rdf:value """Removed global reflexivity (leads to
               inconsistency)."""@en
    ], [
        dc:date "2023-11-08" ;
        rdf:value """In order to get a system of rolified Relation classes: created
               the object property, with domain and range the DerivationRelation rolified class.
               Declared it as reflexive. Declared it(s) superproperty(ies)."""@en
    ] ;
    skos:scopeNote """This property \"rolifies\" the DerivationRelation class. It should
         be used only when you have to manage instances of the DerivationRelation class, to connect
         each instance to itself, in order to be able to infer, using OWL-RL and property paths, the
         two shortcuts corresponding to this n-ary class."""@en .

:descendanceRelation_role
    a owl:ObjectProperty ;
    rdfs:comment """Connects a DescendanceRelation to itself. It is a property that
         can stand for an instance of the class when necessary, e.g. when you explore a knowledge
         graph."""@en ;
    rdfs:domain :DescendanceRelation ;
    rdfs:isDefinedBy <https://www.ica.org/standards/RiC/ontology> ;
    rdfs:label "a le rôle de la Relation de descendance"@fr, "desempeña el papel de la Relación de descendencia"@es, "has the role of the Descendance Relation"@en ;
    rdfs:range :DescendanceRelation ;
    rdfs:subPropertyOf :agentTemporalRelation_role, :familyRelation_role ;
    skos:changeNote [
        dc:date "2024-08-02" ;
        rdf:value """Removed global reflexivity (leads to
               inconsistency)."""@en
    ], [
        dc:date "2023-11-08" ;
        rdf:value """In order to get a system of rolified Relation classes: created
               the object property, with domain and range the DescendanceRelation rolified class.
               Declared it as reflexive. Declared it(s) superproperty(ies)."""@en
    ] ;
    skos:scopeNote """This property \"rolifies\" the DescendanceRelation class. It
         should be used only when you have to manage instances of the DescendanceRelation class, to
         connect each instance to itself, in order to be able to infer, using OWL-RL and property
         paths, the two shortcuts corresponding to this n-ary class."""@en .

:describesOrDescribed
    a owl:ObjectProperty ;
    rdfs:comment """Connects a Record Resource to a Thing that it describes or
         described."""@en ;
    rdfs:domain :RecordResource ;
    rdfs:isDefinedBy <https://www.ica.org/standards/RiC/ontology> ;
    rdfs:label "describe o describía"@es, "describes or described"@en, "décrit ou a décrit"@fr ;
    rdfs:range :Thing ;
    rdfs:subPropertyOf :hasOrHadSubject ;
    owl:inverseOf :isOrWasDescribedBy ;
    skos:changeNote [
        dc:date "2023-11-12" ;
        rdf:value """Aligned with RiC-CM 1.0: updated the description
               (rdfs:comment)."""@en
    ], [
        dc:date "2023-11-02" ;
        rdf:value "Added a new rdfs:label in Spanish."@en
    ], [
        dc:date "2023-08-28" ;
        rdf:value "Added a new rdfs:label in French."@en
    ], [
        dc:date "2021-01-22" ;
        rdf:value """changed the IRI, label, inverse property IRI, text definition,
               corresponding CM component name (changed made in order to make RiC-O compliant with
               RiC-CM 0.2; the name of this property in RiC-O 0.1 was \"describes\")."""@en
    ] ;
    skos:scopeNote """Can be used, among other situations, for specifying that some
         finding aid (a Record that has Documentary Form Type Finding Aid) describes some Record
         Set."""@en ;
    :RiCCMCorrespondingComponent """RiC-R021 ('describes or described'
         relation)"""@en .

:destructionDate
    a owl:DatatypeProperty ;
    rdfs:comment """Date at which a Record Resource or Instantiation was or will be
         destructed."""@en ;
    rdfs:domain [
        a owl:Class ;
        owl:unionOf (:Instantiation
            :RecordResource
        )
    ] ;
    rdfs:isDefinedBy <https://www.ica.org/standards/RiC/ontology> ;
    rdfs:label "date de destruction"@fr, "destruction date"@en, "fecha de destrucción"@es ;
    rdfs:range rdfs:Literal ;
    rdfs:subPropertyOf :endDate ;
    skos:changeNote [
        dc:date "2025-02-19" ;
        rdf:value "Changed domain and definition (added \"or will be\")."@en
    ], [
        dc:date "2023-11-12" ;
        rdf:value "Added a new rdfs:label in Spanish."@en
    ], [
        dc:date "2023-10-12" ;
        rdf:value "Renamed deletion into destruction."@en
    ], [
        dc:date "2023-08-25" ;
        rdf:value "Added a new rdfs:label in French."@en
    ] ;
    skos:scopeNote """Provided for usability reasons. May be deprecated and removed
         later on. Use only if you don't use Date classes for handling dates."""@en ;
    :RiCCMCorrespondingComponent """Datatype property specialized implementation of
         RiC-E18 (Date entity)"""@en .

:directlyContains
    a owl:ObjectProperty ;
    rdfs:comment """Connects a Place to another Place that it directly
         contains."""@en ;
    rdfs:domain :Place ;
    rdfs:isDefinedBy <https://www.ica.org/standards/RiC/ontology> ;
    rdfs:label "contains directly"@en, "contiene directamente"@es, "contient directement"@fr ;
    rdfs:range :Place ;
    rdfs:subPropertyOf :containsTransitive, :hasDirectPart ;
    owl:inverseOf :isDirectlyContainedBy ;
    skos:changeNote [
        dc:date "2023-11-27" ;
        rdf:value "Added a new rdfs:label in Spanish."@en
    ], [
        dc:date "2023-11-12" ;
        rdf:value "Updated the description (rdfs:comment) and labels."@en
    ], [
        dc:date "2023-09-05" ;
        rdf:value """Object property added, along with its inverse property, in
               order to enable to express current, direct, partitive relations between places (the
               possibly indirect, transitive relation, superproperty of this one, being also
               added)."""@en
    ] .

:directlyFollowsInSequence
    a owl:ObjectProperty ;
    rdfs:comment """Inverse of 'directly precedes in sequence' object
         property."""@en ;
    rdfs:domain :Thing ;
    rdfs:isDefinedBy <https://www.ica.org/standards/RiC/ontology> ;
    rdfs:label "directly follows in sequence"@en, "sigue directamente en la secuencia"@es, "suit directement dans la séquence"@fr ;
    rdfs:range :Thing ;
    rdfs:subPropertyOf :followsInSequenceTransitive ;
    owl:inverseOf :directlyPrecedesInSequence ;
    owl:propertyChainAxiom (:hasProxy
        :proxyDirectlyFollowsInSequence
    ) ;
    skos:changeNote [
        dc:date "2025-04-02" ;
        rdf:value "Fixed the property chain axiom."@en
    ], [
        dc:date "2025-03-04" ;
        rdf:value """Tweaked the rdfs:comment to simply refer to its inverse
               property. Also added a property chain axiom relating it to use of
               rico:Proxy."""@en
    ], [
        dc:date "2023-11-27" ;
        rdf:value "Added a new rdfs:label in Spanish."@en
    ], [
        dc:date "2023-11-12" ;
        rdf:value "Updated the description (rdfs:comment) and labels."@en
    ], [
        dc:date "2023-09-22" ;
        rdf:value """Renamed the property and modified its definition (rdfs:comment)
               in order to better distinguish it from followsInTime."""@en
    ], [
        dc:date "2023-09-08" ;
        rdf:value """Added transitive super-property and both present direct and
               past sequential relations as well as their respective inverse relations."""@en
    ] .

:directlyFollowsProxyInSequence
    a owl:ObjectProperty ;
    rdfs:comment "Inverse of 'proxy directly precedes in sequence' object property. "@en ;
    rdfs:domain :RecordResource ;
    rdfs:isDefinedBy <https://www.ica.org/standards/RiC/ontology> ;
    rdfs:label "directly follows proxy in sequence"@en, "sigue directamente el proxy en la secuencia"@es, "suit directement le proxy dans la séquence"@fr ;
    rdfs:range :Proxy ;
    rdfs:subPropertyOf :directlyFollowsInSequence, :followsProxyInSequence ;
    owl:inverseOf :proxyDirectlyPrecedesInSequence ;
    skos:changeNote [
        dc:date "2025-04-02" ;
        rdf:value "Added the French and Spanish labels."@en
    ], [
        dc:date "2025-03-04" ;
        rdf:value "Introduced in RiC-O 1.1."@en
    ] .

:directlyIncludes
    a owl:ObjectProperty ;
    rdfs:comment """Connects a Record Set to a Record or Record Set which it includes
         directly."""@en ;
    rdfs:domain :RecordSet ;
    rdfs:isDefinedBy <https://www.ica.org/standards/RiC/ontology> ;
    rdfs:label "directly includes"@en, "inclut directement"@fr, "incluye directamente"@es ;
    rdfs:range [
        a owl:Class ;
        owl:unionOf (:Record
            :RecordSet
        )
    ] ;
    rdfs:subPropertyOf :hasDirectPart, :includesTransitive ;
    owl:inverseOf :isDirectlyIncludedIn ;
    skos:changeNote [
        dc:date "2023-11-27" ;
        rdf:value "Added a new rdfs:label in Spanish."@en
    ], [
        dc:date "2023-11-12" ;
        rdf:value "Updated the labels, description (rdfs:comment)."@en
    ], [
        dc:date "2023-09-08" ;
        rdf:value """Object property added, along with its inverse property, in
               order to enable to express current, direct, partitive relations between Record Sets
               and their members (the possibly indirect, transitive relation, superproperty of this
               one, being also added)."""@en
    ] .

:directlyIncludesProxy
    a owl:ObjectProperty ;
    rdfs:comment """Inverse of 'proxy is directly included in' object
         property."""@en ;
    rdfs:domain :RecordSet ;
    rdfs:isDefinedBy <https://www.ica.org/standards/RiC/ontology> ;
    rdfs:label "directly includes proxy"@en, "inclut directement le proxy"@fr, "incluye directamente el proxy"@es ;
    rdfs:range :Proxy ;
    rdfs:subPropertyOf :hasDirectPart, :includesProxy ;
    owl:inverseOf :proxyIsDirectlyIncludedIn ;
    skos:changeNote [
        dc:date "2025-03-04" ;
        rdf:value "Introduced in RiC-O 1.1."@en
    ], [
        dc:date "2025-04-02" ;
        rdf:value "Added the French and Spanish labels."@en
    ] .

:directlyPrecedesInSequence
    a owl:ObjectProperty ;
    rdfs:comment """Connects a Thing to a Thing that it precedes directly in some
         sequence (not necessarily defined or characterised chronologically)."""@en ;
    rdfs:domain :Thing ;
    rdfs:isDefinedBy <https://www.ica.org/standards/RiC/ontology> ;
    rdfs:label "directly precedes in sequence"@en, "precede directamente en la secuencia"@es, "précède directement dans la séquence"@fr ;
    rdfs:range :Thing ;
    rdfs:subPropertyOf :precedesInSequenceTransitive ;
    owl:inverseOf :directlyFollowsInSequence ;
    owl:propertyChainAxiom (:directlyPrecedesProxyInSequence
        :proxyFor
    ) ;
    skos:changeNote [
        dc:date "2025-03-04" ;
        rdf:value """Tweaked the rdfs:comment to try to clarify what is meant. Also
               added a property chain axiom relating it to use of rico:Proxy."""@en
    ], [
        dc:date "2023-11-27" ;
        rdf:value "Added a new rdfs:label in Spanish."@en
    ], [
        dc:date "2023-11-12" ;
        rdf:value "Updated the description (rdfs:comment) and labels."@en
    ], [
        dc:date "2023-09-22" ;
        rdf:value """Renamed the property and modified its definition (rdfs:comment)
               in order to better distinguish it from precedesInTime."""@en
    ], [
        dc:date "2023-09-08" ;
        rdf:value """Object property added, along with its inverse property, in
               order to enable to express current, direct, sequential relations between things (the
               possibly indirect, transitive relation, superproperty of this one, being also
               added)."""@en
    ] .

:directlyPrecedesProxyInSequence
    a owl:ObjectProperty ;
    rdfs:comment """Connects a Record Resource to a Proxy of a Record Resource that it
         precedes directly in some sequence (not necessarily defined or characterised
         chronologically)."""@en ;
    rdfs:domain :RecordResource ;
    rdfs:isDefinedBy <https://www.ica.org/standards/RiC/ontology> ;
    rdfs:label "directly precedes proxy in sequence"@en, "precede directamente el proxy en la secuencia"@es, "précède directement le proxy dans la séquence"@fr ;
    rdfs:range :Proxy ;
    rdfs:subPropertyOf :directlyPrecedesInSequence, :precedesProxyInSequence ;
    owl:inverseOf :proxyDirectlyFollowsInSequence ;
    skos:changeNote [
        dc:date "2025-04-02" ;
        rdf:value "Added the French and Spanish labels."@en
    ], [
        dc:date "2025-03-04" ;
        rdf:value "Introduced in RiC-O 1.1."@en
    ] .

:documentedBy
    a owl:ObjectProperty ;
    rdfs:comment "Inverse of 'documents' object property."@en ;
    rdfs:domain :Activity ;
    rdfs:isDefinedBy <https://www.ica.org/standards/RiC/ontology> ;
    rdfs:label "documented by"@en, "est documenté par"@fr, "se documenta en"@es ;
    rdfs:range [
        a owl:Class ;
        owl:unionOf (:Instantiation
            :RecordResource
        )
    ] ;
    rdfs:subPropertyOf :isOrganicOrFunctionalProvenanceOf, :resultsOrResultedIn ;
    owl:inverseOf :documents ;
    owl:propertyChainAxiom (:thingIsTargetOfRelation
        :activityDocumentationRelation_role
        :relationHasSource
    ) ;
    skos:changeNote [
        dc:date "2023-11-08" ;
        rdf:value """In order to get a system of rolified Relation classes: modified
               the property chain axiom so that it now involves the new
               activityDocumentationRelation_role object property."""@en
    ], [
        dc:date "2023-11-07" ;
        rdf:value """Made this property a subproperty of the new
               isOrganicOrFunctionalProvenanceOf property."""@en
    ], [
        dc:date "2023-11-02" ;
        rdf:value "Added a new rdfs:label in Spanish."@en
    ], [
        dc:date "2023-08-28" ;
        rdf:value "Added a new rdfs:label in French."@en
    ], [
        dc:date "2021-01-22" ;
        rdf:value """changed the inverse property IRI, the superproperty IRI and the
               corresponding CML component name"""@en
    ] ;
    :RiCCMCorrespondingComponent """RiC-R033i ('documented by'
         relation)"""@en .

:documents
    a owl:ObjectProperty ;
    rdfs:comment """Connects a Record Resource or an Instantiation to the Activity
         that generates the Record Resource or Instantiation."""@en ;
    rdfs:domain [
        a owl:Class ;
        owl:unionOf (:Instantiation
            :RecordResource
        )
    ] ;
    rdfs:isDefinedBy <https://www.ica.org/standards/RiC/ontology> ;
    rdfs:label "documenta"@es, "documente"@fr, "documents"@en ;
    rdfs:range :Activity ;
    rdfs:subPropertyOf :hasOrganicOrFunctionalProvenance, :resultsOrResultedFrom ;
    owl:inverseOf :documentedBy ;
    owl:propertyChainAxiom (:thingIsSourceOfRelation
        :activityDocumentationRelation_role
        :relationHasTarget
    ) ;
    skos:changeNote [
        dc:date "2023-11-12" ;
        rdf:value """Aligned with RiC-CM 1.0: updated the
               skos:scopeNote."""@en
    ], [
        dc:date "2023-11-08" ;
        rdf:value """In order to get a system of rolified Relation classes: modified
               the property chain axiom so that it now involves the new
               activityDocumentationRelation_role object property."""@en
    ], [
        dc:date "2023-11-07" ;
        rdf:value """Made this property a subproperty of the new
               hasOrganicOrFunctionalProvenance property."""@en
    ], [
        dc:date "2023-11-02" ;
        rdf:value "Added a new rdfs:label in Spanish."@en
    ], [
        dc:date "2023-08-28" ;
        rdf:value "Added a new rdfs:label in French."@en
    ], [
        dc:date "2021-01-22" ;
        rdf:value """changed the IRI, label, superproperty IRI, corresponding CM
               component name (changed made in order to make RiC-O compliant with RiC-CM 0.2; the
               name of this property in RiC-O 0.1 was \"isDocumentationOf\")."""@en
    ] ;
    skos:scopeNote """To be used to describe the functional provenance of a Record
         Resource or Instantiation."""@en ;
    :RiCCMCorrespondingComponent """RiC-R033 ('documents'
         relation)"""@en .

:endDate
    a owl:DatatypeProperty ;
    rdfs:comment "Date at which something ended."@en ;
    rdfs:domain :Thing ;
    rdfs:isDefinedBy <https://www.ica.org/standards/RiC/ontology> ;
    rdfs:label "date de fin"@fr, "end date"@en, "fecha final"@es ;
    rdfs:range rdfs:Literal ;
    rdfs:subPropertyOf :date ;
    skos:changeNote [
        dc:date "2023-11-02" ;
        rdf:value "Added a new rdfs:label in Spanish."@en
    ], [
        dc:date "2023-08-25" ;
        rdf:value "Added a new rdfs:label in French."@en
    ] ;
    skos:scopeNote """Provided for usability reasons. May be deprecated and removed
         later on. Use only if you don't use Date classes for handling dates."""@en ;
    :RiCCMCorrespondingComponent """Datatype property specialized implementation of
         RiC-E18 (Date entity)"""@en .

:eventRelation_role
    a owl:ObjectProperty ;
    rdfs:comment """Connects an EventRelation to itself. It is a property that can
         stand for an instance of the class when necessary, e.g. when you explore a knowledge
         graph."""@en ;
    rdfs:domain :EventRelation ;
    rdfs:isDefinedBy <https://www.ica.org/standards/RiC/ontology> ;
    rdfs:label "a le rôle de la Relation impliquant un événement"@fr, "desempeña el papel de la Relación con un evento"@es, "has the role of the Event Relation"@en ;
    rdfs:range :EventRelation ;
    rdfs:subPropertyOf :relation_role ;
    skos:changeNote [
        dc:date "2024-08-02" ;
        rdf:value """Removed global reflexivity (leads to
               inconsistency)."""@en
    ], [
        dc:date "2023-11-08" ;
        rdf:value """In order to get a system of rolified Relation classes: created
               the object property, with domain and range the EventRelation rolified class. Declared
               it as reflexive. Declared it(s) superproperty(ies)."""@en
    ] ;
    skos:scopeNote """This property \"rolifies\" the EventRelation class. It should be
         used only when you have to manage instances of the EventRelation class, to connect each
         instance to itself, in order to be able to infer, using OWL-RL and property paths, the two
         shortcuts corresponding to this n-ary class."""@en .

:evidences
    a owl:ObjectProperty ;
    rdfs:comment """Connects a Record Resource to a Relation, when the first is used
         for proving the existence of the second one, or for describing it."""@en ;
    rdfs:domain :RecordResource ;
    rdfs:isDefinedBy <https://www.ica.org/standards/RiC/ontology> ;
    rdfs:label "atteste de"@fr, "evidences"@en, "evidencia"@es ;
    rdfs:range :Relation ;
    rdfs:subPropertyOf :thingIsConnectedToRelation ;
    owl:inverseOf :isEvidencedBy ;
    skos:changeNote [
        dc:date "2023-12-27" ;
        rdf:value """Renamed the object property (was 'is source of') and reduced
               its domain to Record Resource (the domain was the union of Record Resource and Agent)
               and its range to Relation (the range was the union of Record Resource and Relation).
               Consequently updated the superproperty, the labels, and added a
               rico:RiCCMCorrespondingComponent. Same for the inverse object property."""@en
    ], [
        dc:date "2023-11-02" ;
        rdf:value "Added a new rdfs:label in Spanish."@en
    ], [
        dc:date "2023-08-28" ;
        rdf:value "Added a new rdfs:label in French."@en
    ] ;
    :RiCCMCorrespondingComponent """Inverse of 'is evidenced by' object
         property."""@en .

:existsOrExistedIn
    a owl:ObjectProperty ;
    rdfs:comment """Connects a Position to a Group in which that Position exists or
         existed, or that is defined by that Group's organizational structure."""@en ;
    rdfs:domain :Position ;
    rdfs:isDefinedBy <https://www.ica.org/standards/RiC/ontology> ;
    rdfs:label "existe o existía en"@es, "existe ou a existé dans"@fr, "exists or existed in"@en ;
    rdfs:range :Group ;
    rdfs:subPropertyOf :isAgentAssociatedWithAgent ;
    owl:inverseOf :hasOrHadPosition ;
    owl:propertyChainAxiom (:thingIsSourceOfRelation
        :positionToGroupRelation_role
        :relationHasTarget
    ) ;
    skos:changeNote [
        dc:date "2024-03-15" ;
        rdf:value "Corrected unparseable symbol in rdfs:comment"@en
    ], [
        dc:date "2023-11-08" ;
        rdf:value """In order to get a system of rolified Relation classes: modified
               the property chain axiom so that it now involves the new positionToGroupRelation_role
               object property."""@en
    ], [
        dc:date "2023-11-02" ;
        rdf:value "Added a new rdfs:label in Spanish."@en
    ], [
        dc:date "2023-08-28" ;
        rdf:value "Added a new rdfs:label in French."@en
    ], [
        dc:date "2021-01-22" ;
        rdf:value """changed the IRI, label, inverse property IRI, text definition,
               corresponding CM component name (changed made in order to make RiC-O compliant with
               RiC-CM 0.2; the name of this property in RiC-O 0.1 was \"existsIn\")."""@en
    ] ;
    :RiCCMCorrespondingComponent """RiC-R056 ('exists or existed in'
         relation)"""@en .

:expressedDate
    a owl:DatatypeProperty ;
    rdfs:comment """Natural language expression of a date. This property is a
         specialization of the name property. In order that the precise meaning of the date can be
         understood, information such as the calendar used or other specific context should be
         included."""@en ;
    rdfs:domain :Date ;
    rdfs:isDefinedBy <https://www.ica.org/standards/RiC/ontology> ;
    rdfs:label "date en langage naturel"@fr, "expressed date"@en, "fecha expresada"@es ;
    rdfs:range rdfs:Literal ;
    rdfs:subPropertyOf :name, :textualValue ;
    skos:changeNote [
        dc:date "2023-11-11" ;
        rdf:value """Aligned with RiC-CM 1.0: updated the description
               (rdfs:comment), examples (skos:example)."""@en
    ], [
        dc:date "2023-11-02" ;
        rdf:value "Added a new rdfs:label in Spanish."@en
    ], [
        dc:date "2023-10-10" ;
        rdf:value """Updated the rdfs:comment and skos:examples in order to make
               this property fully compliant with RiC-CM 1.0. Made it a subproperty of
               rico:name."""@en
    ], [
        dc:date "2023-08-25" ;
        rdf:value "Added a new rdfs:label in French."@en
    ], [
        dc:date "2020-11-01" ;
        rdf:value """examples added. Objective: to make RiC-O compliant with RiC-CM
               v0.2."""@en
    ] ;
    skos:example """15 thermidor an IV (calendrier révolutionnaire
         français)"""@fr, "1550-1553, 1555 (date range)"@en, "1925-1966 (date range)"@en, "8 avril 1258 (a. st., style de Pâques)"@fr, "All of the years 1550, 1551, 1553, 1555"@en, """Die jovis ultima mensis martii anno domini millesimo quingentesimo
         quadragesimo ante Pascha"""@la, "October 24, 1999 (month day, year)"@en, "One of the years 1550, 1551, 1553, 1555"@en, "The Middle Ages"@en, """The second semester of 1951 to 1952 (academic reference
         system)"""@en, "XVIIe siècle"@fr ;
    :RiCCMCorrespondingComponent """Corresponds to RiC-A19 (Expressed Date
         attribute)"""@en .

:expressesOrExpressed
    a owl:ObjectProperty ;
    rdfs:comment """Inverse of 'is or was expressed by' object
         property."""@en ;
    rdfs:domain :RecordResource ;
    rdfs:isDefinedBy <https://www.ica.org/standards/RiC/ontology> ;
    rdfs:label "expresa o expresaba"@es, "expresses or expressed"@en, "exprime ou a exprimé"@fr ;
    rdfs:range :Rule ;
    rdfs:subPropertyOf :isAssociatedWithRule ;
    owl:inverseOf :isOrWasExpressedBy ;
    skos:changeNote [
        dc:date "2023-11-02" ;
        rdf:value "Added a new rdfs:label in Spanish."@en
    ], [
        dc:date "2023-08-28" ;
        rdf:value "Added a new rdfs:label in French."@en
    ], [
        dc:date "2021-01-22" ;
        rdf:value """changed the IRI, label, inverse property IRI, text definition,
               corresponding CM component name (changed made in order to make RiC-O compliant with
               RiC-CM 0.2; the name of this property in RiC-O 0.1 was \"expresses\")."""@en
    ] ;
    :RiCCMCorrespondingComponent """RiC-R064i ('expresses or expressed'
         relation)"""@en .

:familyRelation_role
    a owl:ObjectProperty ;
    rdfs:comment """Connects a FamilyRelation to itself. It is a property that can
         stand for an instance of the class when necessary, e.g. when you explore a knowledge
         graph."""@en ;
    rdfs:domain :FamilyRelation ;
    rdfs:isDefinedBy <https://www.ica.org/standards/RiC/ontology> ;
    rdfs:label "a le rôle de la Relation familiale"@fr, "desempeña el papel de la Relación familiar"@es, "has the role of the Family Relation"@en ;
    rdfs:range :FamilyRelation ;
    rdfs:subPropertyOf :agentToAgentRelation_role ;
    skos:changeNote [
        dc:date "2024-08-02" ;
        rdf:value """Removed global reflexivity (leads to
               inconsistency)."""@en
    ], [
        dc:date "2024-03-15" ;
        rdf:value "Corrected unparseable symbol in rdfs:comment"@en
    ], [
        dc:date "2023-11-08" ;
        rdf:value """In order to get a system of rolified Relation classes: created
               the object property, with domain and range the FamilyRelation rolified class.
               Declared it as reflexive. Declared it(s) superproperty(ies)."""@en
    ] ;
    skos:scopeNote """This property \"rolifies\" the FamilyRelation class. It should be
         used only when you have to manage instances of the FamilyRelation class, to connect each
         instance to itself, in order to be able to infer, using OWL-RL and property paths, the two
         shortcuts corresponding to this n-ary class."""@en .

:followedInSequence
    a owl:ObjectProperty ;
    rdfs:comment """Connects a Thing to a Thing that it followed in some sequence (not
         necessarily defined or characterised chronologically) in the past."""@en ;
    rdfs:domain :Thing ;
    rdfs:isDefinedBy <https://www.ica.org/standards/RiC/ontology> ;
    rdfs:label "a suivi dans la séquence"@fr, "followed in sequence"@en, "seguía en la secuencia transitivo"@es ;
    rdfs:range :Thing ;
    rdfs:subPropertyOf :followsOrFollowed ;
    owl:inverseOf :precededInSequence ;
    skos:changeNote [
        dc:date "2025-03-04" ;
        rdf:value """Tweaked the rdfs:comment to try to clarify what is
               meant."""@en
    ], [
        dc:date "2023-11-27" ;
        rdf:value "Added a new rdfs:label in Spanish."@en
    ], [
        dc:date "2023-11-12" ;
        rdf:value "Updated the description (rdfs:comment) and labels."@en
    ], [
        dc:date "2023-09-22" ;
        rdf:value """Renamed the property and modified its definition (rdfs:comment)
               in order to better distinguish it from followsInTime."""@en
    ], [
        dc:date "2023-09-08" ;
        rdf:value """Added transitive super-property and both present direct and
               past sequential relations as well as their respective inverse relations."""@en
    ] .

:followsInSequenceTransitive
    a owl:ObjectProperty, owl:TransitiveProperty ;
    rdfs:comment """Inverse of 'precedes in sequence transitive' object
         property."""@en ;
    rdfs:domain :Thing ;
    rdfs:isDefinedBy <https://www.ica.org/standards/RiC/ontology> ;
    rdfs:label "follows in sequence transitive"@en, "sigue en la secuencia transitivo"@es, "suit dans la séquence transitif"@fr ;
    rdfs:range :Thing ;
    rdfs:subPropertyOf :followsOrFollowed ;
    owl:inverseOf :precedesInSequenceTransitive ;
    owl:propertyChainAxiom (:hasProxy
        :proxyFollowsInSequence
    ) ;
    skos:changeNote [
        dc:date "2025-03-04" ;
        rdf:value """Tweaked the rdfs:comment to simply refer to its inverse
               property. Also added a property chain axiom relating it to use of rico:Proxy.
            """@en
    ], [
        dc:date "2023-11-27" ;
        rdf:value "Added a new rdfs:label in Spanish."@en
    ], [
        dc:date "2023-11-12" ;
        rdf:value "Updated the description (rdfs:comment) and labels."@en
    ], [
        dc:date "2023-09-22" ;
        rdf:value """Renamed the property and modified its definition (rdfs:comment)
               in order to better distinguish it from followsInTime."""@en
    ], [
        dc:date "2023-09-08" ;
        rdf:value """Added transitive super-property and both present direct and
               past sequential relations as well as their respective inverse relations."""@en
    ] .

:followsInTime
    a owl:ObjectProperty, owl:TransitiveProperty ;
    rdfs:comment """Inverse of 'precedes in time' object property. This is a
         transitive relation."""@en ;
    rdfs:domain :Thing ;
    rdfs:isDefinedBy <https://www.ica.org/standards/RiC/ontology> ;
    rdfs:label "follows in time"@en, "sigue en el tiempo a"@es, "suit dans le temps"@fr ;
    rdfs:range :Thing ;
    rdfs:subPropertyOf :followsOrFollowed ;
    owl:inverseOf :precedesInTime ;
    owl:propertyChainAxiom (:thingIsTargetOfRelation
        :temporalRelation_role
        :relationHasSource
    ) ;
    skos:changeNote [
        dc:date "2023-11-08" ;
        rdf:value """In order to get a system of rolified Relation classes: modified
               the property chain axiom so that it now involves the new temporalRelation_role object
               property."""@en
    ], [
        dc:date "2023-11-02" ;
        rdf:value "Added a new rdfs:label in Spanish."@en
    ], [
        dc:date "2023-09-22" ;
        rdf:value "Property made transitive."@en
    ], [
        dc:date "2023-08-28" ;
        rdf:value "Added a new rdfs:label in French."@en
    ], [
        dc:date "2021-01-22" ;
        rdf:value "changed the superproperty IRI."@en
    ] ;
    :RiCCMCorrespondingComponent """RiC-R009i ('follows in time'
         relation)"""@en .

:followsOrFollowed
    a owl:ObjectProperty ;
    rdfs:comment "Inverse of 'precedes or preceded' object property."@en ;
    rdfs:domain :Thing ;
    rdfs:isDefinedBy <https://www.ica.org/standards/RiC/ontology> ;
    rdfs:label "follows or followed"@en, "sigue o seguía a"@es, "suit ou a suivi"@fr ;
    rdfs:range :Thing ;
    rdfs:subPropertyOf :isRelatedTo ;
    owl:inverseOf :precedesOrPreceded ;
    owl:propertyChainAxiom (:thingIsTargetOfRelation
        :sequentialRelation_role
        :relationHasSource
    ) ;
    skos:changeNote [
        dc:date "2023-11-08" ;
        rdf:value """In order to get a system of rolified Relation classes: modified
               the property chain axiom so that it now involves the new sequentialRelation_role
               object property."""@en
    ], [
        dc:date "2023-11-02" ;
        rdf:value "Added a new rdfs:label in Spanish."@en
    ], [
        dc:date "2023-08-28" ;
        rdf:value "Added a new rdfs:label in French."@en
    ], [
        dc:date "2021-01-22" ;
        rdf:value """changed the IRI, label, inverse property IRI, text definition,
               corresponding CM component name (changed made in order to make RiC-O compliant with
               RiC-CM 0.2; the name of this property in RiC-O 0.1 was \"follows\")."""@en
    ] ;
    :RiCCMCorrespondingComponent """RiC-R008i ('follows or followed'
         relation)"""@en .

:followsProxyInSequence
    a owl:ObjectProperty ;
    rdfs:comment """Inverse of 'proxy precedes in sequence' object
         property."""@en ;
    rdfs:domain :RecordResource ;
    rdfs:isDefinedBy <https://www.ica.org/standards/RiC/ontology> ;
    rdfs:label "follows proxy in sequence"@en, "sigue el proxy en la secuencia"@es, "suit le proxy dans la séquence"@fr ;
    rdfs:range :Proxy ;
    rdfs:subPropertyOf :followsInSequenceTransitive ;
    owl:inverseOf :proxyPrecedesInSequence ;
    skos:changeNote [
        dc:date "2025-04-02" ;
        rdf:value "Added the French and Spanish labels."@en
    ], [
        dc:date "2025-03-04" ;
        rdf:value "Introduced in RiC-O 1.1."@en
    ] .

:functionalEquivalenceRelation_role
    a owl:ObjectProperty ;
    rdfs:comment """Connects a FunctionalEquivalenceRelation to itself. It is a
         property that can stand for an instance of the class when necessary, e.g. when you explore
         a knowledge graph."""@en ;
    rdfs:domain :FunctionalEquivalenceRelation ;
    rdfs:isDefinedBy <https://www.ica.org/standards/RiC/ontology> ;
    rdfs:label "a le rôle de la Relation d’équivalence fonctionnelle"@fr, """desempeña el papel de la Relación de equivalencia
         funcional"""@es, "has the role of the Functional Equivalence Relation"@en ;
    rdfs:range :FunctionalEquivalenceRelation ;
    rdfs:subPropertyOf :instantiationToInstantiationRelation_role ;
    skos:changeNote [
        dc:date "2024-08-02" ;
        rdf:value """Removed global reflexivity (leads to
               inconsistency)."""@en
    ], [
        dc:date "2023-11-08" ;
        rdf:value """In order to get a system of rolified Relation classes: created
               the object property, with domain and range the FunctionalEquivalenceRelation rolified
               class. Declared it as reflexive. Declared it(s) superproperty(ies)."""@en
    ] ;
    skos:scopeNote """This property \"rolifies\" the FunctionalEquivalenceRelation
         class. It should be used only when you have to manage instances of the
         FunctionalEquivalenceRelation class, to connect each instance to itself, in order to be
         able to infer, using OWL-RL and property paths, the two shortcuts corresponding to this
         n-ary class."""@en .

:generalDescription
    a owl:DatatypeProperty ;
    rdfs:comment """General information about an entity. General description may be
         used to describe any entity. There are different appropriate uses for general description.
         First, while it is recommended that more specific properties be used in describing an
         entity, it may be desirable, for economic or other reasons, to describe two or more
         specific properties together. Second, general description may be used to describe one or
         more characteristics that are not otherwise accommodated in RiC-O. Third, it may be used to
         provide a succinct summary or abstract description in addition to more detailed specific
         description."""@en ;
    rdfs:domain :Thing ;
    rdfs:isDefinedBy <https://www.ica.org/standards/RiC/ontology> ;
    rdfs:label "descripción general"@es, "description générale"@fr, "general description"@en ;
    rdfs:range rdfs:Literal ;
    skos:changeNote [
        dc:date "2023-11-11" ;
        rdf:value """Aligned with RiC-CM 1.0: updated the IRI, mapping to RiC-CM
               (rico:RiCCMCorrespondingComponent), labels, description (rdfs:comment), examples
               (skos:example)."""@en
    ], [
        dc:date "2023-11-02" ;
        rdf:value "Added a new rdfs:label in Spanish."@en
    ], [
        dc:date "2023-08-25" ;
        rdf:value "Added a new rdfs:label in French."@en
    ] ;
    skos:example """Le massif du Mont-Blanc est un massif des Alpes partagé entre la
         France, l'Italie et la Suisse. Il abrite le mont Blanc, plus haut sommet d'Europe
         occidentale qui culmine à 4 809 mètres (altitude relevée en 2015). Il est traversé par le
         tunnel du Mont-Blanc, entre Chamonix dans la vallée de l'Arve et Courmayeur dans la vallée
         d'Aoste."""@fr, """The Senate is the academic governing body of the University of
         Strathclyde and is responsible for all academic matters including academic standards and
         quality. Meetings of the Senate are chaired by the Principal and the membership is drawn
         entirely from within the University, comprising academic and research staff. (about a
         corporate body, University of Strathclyde Senate)"""@en, """This activity involves regulating the nursing profession by
         conducting examinations and on-going education for nurses, maintaining rolls of those
         qualified as enrolled or registered nurses, midwives, psychiatric, and other specialised
         nurses. It also covers hearing disciplinary charges against nurses (and where necessary,
         removing them temporarily or permanently from the registers), as well as promoting the
         nursing profession. (about an activity, Nursing Profession Regulation)"""@en, """Thomas Blaikie (1750-1838) est un botaniste et jardinier écossais.
         Il a dessiné notamment les jardins de Malmaison et Bagatelle."""@fr ;
    :RiCCMCorrespondingComponent """Corresponds to RiC-A43 (General Description
         attribute)"""@en .

:geodesicSystem
    a owl:DatatypeProperty ;
    rdfs:comment "Reference system used for geographical coordinates."@en ;
    rdfs:domain :Coordinates ;
    rdfs:isDefinedBy <https://www.ica.org/standards/RiC/ontology> ;
    rdfs:label "geodesic system"@en, "sistema geodésico"@es, "système géodésique"@fr ;
    rdfs:range rdfs:Literal ;
    rdfs:subPropertyOf :referenceSystem ;
    skos:changeNote [
        dc:date "2023-11-02" ;
        rdf:value "Added a new rdfs:label in Spanish."@en
    ], [
        dc:date "2023-08-25" ;
        rdf:value "Added a new rdfs:label in French."@en
    ] .

:geographicalCoordinates
    a owl:DatatypeProperty ;
    rdfs:comment "Longitudinal and latitudinal information about a Place. "@en ;
    rdfs:domain :Place ;
    rdfs:isDefinedBy <https://www.ica.org/standards/RiC/ontology> ;
    rdfs:label "coordenadas geográficas"@es, "coordonnées géographiques"@fr, "geographical coordinates"@en ;
    rdfs:range rdfs:Literal ;
    skos:changeNote [
        dc:date "2023-11-11" ;
        rdf:value """Aligned with RiC-CM 1.0: updated the description
               (rdfs:comment), examples (skos:example)."""@en
    ], [
        dc:date "2023-11-02" ;
        rdf:value "Added a new rdfs:label in Spanish."@en
    ], [
        dc:date "2023-08-25" ;
        rdf:value "Added a new rdfs:label in French."@en
    ], [
        dc:date "2023-08-25" ;
        rdf:value "Added a new rdfs:label in French."@en
    ], [
        dc:date "2020-11-01" ;
        rdf:value """Text definition and scope note updated. Examples added.
               Objective: to make RiC-O compliant with RiC-CM v0.2."""@en
    ] ;
    skos:example """Latitude 35.89421911, Longitude 139.94637467 (ISO
         6709/F)"""@en, """Latitude 50°40′46,461″N, Longitude 95°48′26,533″W, Height 123,45m
         (ISO 6709/D)"""@en ;
    skos:scopeNote """Provided for usability reasons. May be deprecated and removed
         later on. Use only if you don't use PhysicalLocation and Coordinates classes with Place.
         Coordinates may be based on ISO 6709 Standard representation of geographic point location
         by coordinates."""@en ;
    :RiCCMCorrespondingComponent """Corresponds to RiC-A11 (Coordinates
         attribute)"""@en .

:groupSubdivisionRelation_role
    a owl:ObjectProperty ;
    rdfs:comment """Connects a GroupSubdivisionRelation to itself. It is a property
         that can stand for an instance of the class when necessary, e.g. when you explore a
         knowledge graph."""@en ;
    rdfs:domain :GroupSubdivisionRelation ;
    rdfs:isDefinedBy <https://www.ica.org/standards/RiC/ontology> ;
    rdfs:label """a le rôle de la Relation de subdivision entre groupes
         d’agents"""@fr, """desempeña el papel de la Relación de subdivisión entre grupos de
         agentes"""@es, "has the role of the Group Subdivision Relation"@en ;
    rdfs:range :GroupSubdivisionRelation ;
    rdfs:subPropertyOf :agentHierarchicalRelation_role, :wholePartRelation_role ;
    skos:changeNote [
        dc:date "2024-08-02" ;
        rdf:value """Removed global reflexivity (leads to
               inconsistency)."""@en
    ], [
        dc:date "2023-11-08" ;
        rdf:value """In order to get a system of rolified Relation classes: created
               the object property, with domain and range the GroupSubdivisionRelation rolified
               class. Declared it as reflexive. Declared it(s) superproperty(ies)."""@en
    ] ;
    skos:scopeNote """This property \"rolifies\" the GroupSubdivisionRelation class. It
         should be used only when you have to manage instances of the GroupSubdivisionRelation
         class, to connect each instance to itself, in order to be able to infer, using OWL-RL and
         property paths, the two shortcuts corresponding to this n-ary class."""@en .

:hadComponent
    a owl:ObjectProperty ;
    rdfs:comment """Connects an Instantiation to another Instantiation that was its
         component in the past."""@en ;
    rdfs:domain :Instantiation ;
    rdfs:isDefinedBy <https://www.ica.org/standards/RiC/ontology> ;
    rdfs:label "a eu pour composant"@fr, "had component"@en, "tenía como componente"@es ;
    rdfs:range :Instantiation ;
    rdfs:subPropertyOf :hadPart, :hasOrHadComponent ;
    owl:inverseOf :wasComponentOf ;
    skos:changeNote [
        dc:date "2023-11-27" ;
        rdf:value "Added a new rdfs:label in Spanish."@en
    ], [
        dc:date "2023-11-12" ;
        rdf:value "Updated the description (rdfs:comment) and labels."@en
    ], [
        dc:date "2023-09-08" ;
        rdf:value """Object property added, along with its inverse property, in
               order to enable to express past partitive relations between instantiations (the
               current partitive relations being also added, including a transitive
               one)."""@en
    ] .

:hadConstituent
    a owl:ObjectProperty ;
    rdfs:comment """Connects a Record or Record Part to another Record or Record Part
         that was its constituent in the past."""@en ;
    rdfs:domain [
        a owl:Class ;
        owl:unionOf (:Record
            :RecordPart
        )
    ] ;
    rdfs:isDefinedBy <https://www.ica.org/standards/RiC/ontology> ;
    rdfs:label "a eu pour constituant"@fr, "had constituent"@en, "tenía como elemento constitutivo"@es ;
    rdfs:range [
        a owl:Class ;
        owl:unionOf (:Record
            :RecordPart
        )
    ] ;
    rdfs:subPropertyOf :hadPart, :hasOrHadConstituent ;
    owl:inverseOf :wasConstituentOf ;
    skos:changeNote [
        dc:date "2023-11-27" ;
        rdf:value "Added a new rdfs:label in Spanish."@en
    ], [
        dc:date "2023-11-12" ;
        rdf:value "Updated the labels."@en
    ], [
        dc:date "2023-10-26" ;
        rdf:value "Added RecordPart to the domain."@en
    ], [
        dc:date "2023-09-08" ;
        rdf:value """Object property added, along with its inverse property, in
               order to enable to express past partitive relations between Record and Record or
               Record Part (the current partitive relations being also added, including a transitive
               one)."""@en
    ] .

:hadPart
    a owl:ObjectProperty ;
    rdfs:comment """Connects a Thing to a Thing that was a constitutive or component
         part of that Thing in the past."""@en ;
    rdfs:domain :Thing ;
    rdfs:isDefinedBy <https://www.ica.org/standards/RiC/ontology> ;
    rdfs:label "a eu pour partie"@fr, "had part"@en, "tenía como parte"@es ;
    rdfs:range :Thing ;
    rdfs:subPropertyOf :hasOrHadPart ;
    owl:inverseOf :wasPartOf ;
    skos:changeNote [
        dc:date "2023-11-27" ;
        rdf:value "Added a new rdfs:label in Spanish."@en
    ], [
        dc:date "2023-11-12" ;
        rdf:value "Updated the labels."@en
    ], [
        dc:date "2023-07-12" ;
        rdf:value """Object property added, along with its inverse property, in
               order to enable to express past partitive relations between things (the current
               partitive relations being also added, including a transitive one)."""@en
    ] .

:hadSubdivision
    a owl:ObjectProperty ;
    rdfs:comment "Connects a Group to one of its past subdivisions."@en ;
    rdfs:domain :Group ;
    rdfs:isDefinedBy <https://www.ica.org/standards/RiC/ontology> ;
    rdfs:label "a eu pour subdivision"@fr, "had subdivision"@en, "tenía como subdivisión"@es ;
    rdfs:range :Group ;
    rdfs:subPropertyOf :hadPart, :hadSubordinate, :hasOrHadSubdivision ;
    owl:inverseOf :wasSubdivisionOf ;
    skos:changeNote [
        dc:date "2023-11-27" ;
        rdf:value "Added a new rdfs:label in Spanish."@en
    ], [
        dc:date "2023-11-12" ;
        rdf:value "Updated the labels."@en
    ], [
        dc:date "2023-09-08" ;
        rdf:value """Object property added, along with its inverse property, in
               order to enable to express past partitive relations between groups (the current
               partitive relations being also added, including a transitive one)."""@en
    ] .

:hadSubevent
    a owl:ObjectProperty ;
    rdfs:comment """Connects a past Event to one of a series of past Events that
         constituted that original, broader, past Event."""@en ;
    rdfs:domain :Event ;
    rdfs:isDefinedBy <https://www.ica.org/standards/RiC/ontology> ;
    rdfs:label "a été constitué de l’événement"@fr, "had subevent"@en, "tenía como parte de evento"@es ;
    rdfs:range :Event ;
    rdfs:subPropertyOf :hadPart, :hasOrHadSubevent ;
    owl:inverseOf :wasSubeventOf ;
    skos:changeNote [
        dc:date "2023-11-27" ;
        rdf:value "Added a new rdfs:label in Spanish."@en
    ], [
        dc:date "2023-11-12" ;
        rdf:value "Updated the labels."@en
    ], [
        dc:date "2023-09-08" ;
        rdf:value """Object property added, along with its inverse property, in
               order to enable to express partitive relations between past Events (the partitive
               relations between ongoing events being also added, including a transitive
               one)."""@en
    ] .

:hadSubordinate
    a owl:ObjectProperty ;
    rdfs:comment """Connects an Agent to an Agent that was hierarchically inferior in
         the past."""@en ;
    rdfs:domain :Agent ;
    rdfs:isDefinedBy <https://www.ica.org/standards/RiC/ontology> ;
    rdfs:label "a eu pour subalterne"@fr, "had subordinate"@en, "tenía como subordinado o subordinada a"@es ;
    rdfs:range :Agent ;
    rdfs:subPropertyOf :hasOrHadSubordinate ;
    owl:inverseOf :wasSubordinateTo ;
    skos:changeNote [
        dc:date "2023-11-27" ;
        rdf:value "Added a new rdfs:label in Spanish."@en
    ], [
        dc:date "2023-11-12" ;
        rdf:value "Updated the labels."@en
    ], [
        dc:date "2023-09-08" ;
        rdf:value """Object property added, along with its inverse property, in
               order to enable to express past subordination relations between Agents (the current
               subordination relations being also added, including a transitive one)."""@en
    ] .

:hasAccumulationDate
    a owl:ObjectProperty ;
    rdfs:comment """Inverse of 'is accumulation date of' object
         property."""@en ;
    rdfs:domain [
        a owl:Class ;
        owl:unionOf (:Instantiation
            :RecordResource
        )
    ] ;
    rdfs:isDefinedBy <https://www.ica.org/standards/RiC/ontology> ;
    rdfs:label "a pour date d'accumulation"@fr, "has accumulation date"@en, "tiene como fecha de acumulación"@es ;
    rdfs:range :Date ;
    rdfs:subPropertyOf :hasOrganicProvenanceDate ;
    owl:inverseOf :isAccumulationDateOf ;
    owl:propertyChainAxiom (:thingIsSourceOfRelation
        :accumulationRelation_role
        :relationHasDate
    ) ;
    skos:changeNote [
        dc:date "2024-12-19" ;
        rdf:value """Connect to AccumulationRelation via a sub-property chain, and
               make a sub-property of the new object property
               'hasOrganicProvenanceDate'."""@en
    ], [
        dc:date "2024-10-04" ;
        rdf:value "Added in RiC-O 1.1."@en
    ] .

:hasAccumulator
    a owl:ObjectProperty ;
    rdfs:comment """Connects a Record Resource or an Instantiation to the Agent that
         accumulates it, be it intentionally (collecting) or not (receiving in the course of its
         activities)."""@en ;
    rdfs:domain [
        a owl:Class ;
        owl:unionOf (:Instantiation
            :RecordResource
        )
    ] ;
    rdfs:isDefinedBy <https://www.ica.org/standards/RiC/ontology> ;
    rdfs:label "est accumulé par"@fr, "has accumulator"@en, "tiene como acumulador a"@es ;
    rdfs:range :Agent ;
    rdfs:subPropertyOf :hasOrganicProvenance ;
    owl:inverseOf :isAccumulatorOf ;
    owl:propertyChainAxiom (:thingIsSourceOfRelation
        :accumulationRelation_role
        :relationHasTarget
    ) ;
    skos:changeNote [
        dc:date "2023-11-08" ;
        rdf:value """In order to get a system of rolified Relation classes: modified
               the property chain axiom so that it now involves the new accumulationRelation_role
               object property."""@en
    ], [
        dc:date "2023-11-02" ;
        rdf:value "Added a new rdfs:label in Spanish."@en
    ], [
        dc:date "2023-08-28" ;
        rdf:value "Added a new rdfs:label in French."@en
    ], [
        dc:date "2021-01-22" ;
        rdf:value """changed the IRI, label, inverse property IRI, text definition
               and corresponding CM component (changed made in order to make RiC-O compliant with
               RiC-CM 0.2; the name of this property in RiC-O 0.1 was \"accumulatedBy\")."""@en
    ] ;
    :RiCCMCorrespondingComponent """RiC-R028 ('has accumulator'
         relation)"""@en .

:hasActivityType
    a owl:ObjectProperty ;
    rdfs:comment """Connects an Activity to an Activity Type that categorizes
         it."""@en ;
    rdfs:domain :Activity ;
    rdfs:isDefinedBy <https://www.ica.org/standards/RiC/ontology> ;
    rdfs:label "a pour type d’activité"@fr, "has activity type"@en, "tiene como tipo de actividad"@es ;
    rdfs:range :ActivityType ;
    rdfs:subPropertyOf :hasOrHadType ;
    owl:inverseOf :isActivityTypeOf ;
    skos:changeNote [
        dc:date "2025-04-06" ;
        rdf:value "Fixed the Spanish label."@en
    ], [
        dc:date "2023-11-02" ;
        rdf:value "Added a new rdfs:label in Spanish."@en
    ], [
        dc:date "2023-08-28" ;
        rdf:value "Added a new rdfs:label in French."@en
    ], [
        dc:date "2021-01-22" ;
        rdf:value "changed the superproperty IRI."@en
    ] .

:hasAddressee
    a owl:ObjectProperty ;
    rdfs:comment """Connects a Record Resource or an Instantiation to the Agent that
         it is addressed to."""@en ;
    rdfs:domain [
        a owl:Class ;
        owl:unionOf (:Instantiation
            :RecordResource
        )
    ] ;
    rdfs:isDefinedBy <https://www.ica.org/standards/RiC/ontology> ;
    rdfs:label "a pour destinataire"@fr, "has addressee"@en, "se dirige a"@es ;
    rdfs:range :Agent ;
    rdfs:subPropertyOf :hasOrganicProvenance ;
    owl:inverseOf :isAddresseeOf ;
    skos:changeNote [
        dc:date "2023-11-02" ;
        rdf:value "Added a new rdfs:label in Spanish."@en
    ], [
        dc:date "2023-08-28" ;
        rdf:value "Added a new rdfs:label in French."@en
    ], [
        dc:date "2021-01-22" ;
        rdf:value "added a scope note"@en
    ] ;
    skos:scopeNote """The identity of the addressee is (usually) evidenced by the
         Record Resource or Instantiation itself."""@en ;
    :RiCCMCorrespondingComponent """RiC-R032 ('has addressee'
         relation)"""@en .

:hasAncestor
    a owl:ObjectProperty, owl:TransitiveProperty ;
    rdfs:comment """Inverse of 'has descendant' object property. This is a transitive
         relation."""@en ;
    rdfs:domain :Person ;
    rdfs:isDefinedBy <https://www.ica.org/standards/RiC/ontology> ;
    rdfs:label "a pour ancêtre"@fr, "has ancestor"@en, "tiene como ancestro a"@es ;
    rdfs:range :Person ;
    rdfs:subPropertyOf :hasFamilyAssociationWith, :isSuccessorOf ;
    owl:inverseOf :hasDescendant ;
    owl:propertyChainAxiom (:thingIsTargetOfRelation
        :descendanceRelation_role
        :relationHasSource
    ) ;
    skos:changeNote [
        dc:date "2023-11-08" ;
        rdf:value """In order to get a system of rolified Relation classes: modified
               the property chain axiom so that it now involves the new descendanceRelation_role
               object property."""@en
    ], [
        dc:date "2023-11-02" ;
        rdf:value "Added a new rdfs:label in Spanish."@en
    ], [
        dc:date "2023-09-08" ;
        rdf:value "made property transitive"@en
    ], [
        dc:date "2023-08-28" ;
        rdf:value "Added a new rdfs:label in French."@en
    ], [
        dc:date "2021-01-22" ;
        rdf:value "changed the superproperty IRIs."@en
    ] ;
    :RiCCMCorrespondingComponent """RiC-R017i (has ancestor
         relation)"""@en .

:hasAuthor
    a owl:ObjectProperty ;
    rdfs:comment """Connects a Record to the Group, Person or Position that is
         responsible for conceiving and formulating the information contained in the
         Record."""@en ;
    rdfs:domain :Record ;
    rdfs:isDefinedBy <https://www.ica.org/standards/RiC/ontology> ;
    rdfs:label "a pour responsable intellectuel"@fr, "has author"@en, "tiene como autor a"@es ;
    rdfs:range [
        a owl:Class ;
        owl:unionOf (:Group
            :Person
            :Position
        )
    ] ;
    rdfs:subPropertyOf :hasCreator ;
    owl:inverseOf :isAuthorOf ;
    owl:propertyChainAxiom (:thingIsSourceOfRelation
        :authorshipRelation_role
        :relationHasTarget
    ) ;
    skos:changeNote [
        dc:date "2023-11-12" ;
        rdf:value """Aligned with RiC-CM 1.0: updated the
               skos:scopeNote."""@en
    ], [
        dc:date "2023-11-08" ;
        rdf:value """In order to get a system of rolified Relation classes: modified
               the property chain axiom so that it now involves the new authorshipRelation_role
               object property."""@en
    ], [
        dc:date "2023-11-02" ;
        rdf:value "Added a new rdfs:label in Spanish."@en
    ], [
        dc:date "2023-08-28" ;
        rdf:value "Added a new rdfs:label in French."@en
    ], [
        dc:date "2020-12-29" ;
        rdf:value """Created following the addition of RiC-R079 relation in RiC-CM
               0.2"""@en
    ] ;
    skos:scopeNote """To be used for a Person, Group or Position that makes any
         contribution to the content of a record. Includes the Person, Group or Position in whose
         name or by whose command the content may have been formulated and first instantiated (for
         example the Person who signed the Record)."""@en ;
    :RiCCMCorrespondingComponent """RiC-R079 ('has author'
         relation)"""@en .

:hasBeginningDate
    a owl:ObjectProperty ;
    rdfs:comment "Inverse of 'is beginning date of' object property."@en ;
    rdfs:domain :Thing ;
    rdfs:isDefinedBy <https://www.ica.org/standards/RiC/ontology> ;
    rdfs:label "a pour date de début"@fr, "has beginning date"@en, "tiene como fecha de inicio"@es ;
    rdfs:range :Date ;
    rdfs:subPropertyOf :isAssociatedWithDate ;
    owl:inverseOf :isBeginningDateOf ;
    skos:changeNote [
        dc:date "2023-11-02" ;
        rdf:value "Added a new rdfs:label in Spanish."@en
    ], [
        dc:date "2023-08-28" ;
        rdf:value "Added a new rdfs:label in French."@en
    ] ;
    :RiCCMCorrespondingComponent """RiC-R069i ('has beginning date'
         relation)"""@en .

:hasBirthDate
    a owl:ObjectProperty ;
    rdfs:comment "Inverse of 'is birth date of' object property."@en ;
    rdfs:domain :Person ;
    rdfs:isDefinedBy <https://www.ica.org/standards/RiC/ontology> ;
    rdfs:label "a pour date de naissance"@fr, "has birth date"@en, "tiene como fecha de nacimiento"@es ;
    rdfs:range :Date ;
    rdfs:subPropertyOf :hasBeginningDate ;
    owl:inverseOf :isBirthDateOf ;
    skos:changeNote [
        dc:date "2023-11-02" ;
        rdf:value "Added a new rdfs:label in Spanish."@en
    ], [
        dc:date "2023-08-28" ;
        rdf:value "Added a new rdfs:label in French."@en
    ] ;
    :RiCCMCorrespondingComponent """RiC-R070i ('has birth date'
         relation)"""@en .

:hasBirthPlace
    a owl:ObjectProperty ;
    rdfs:comment "Inverse of 'is birth place of' object property."@en ;
    rdfs:domain :Person ;
    rdfs:isDefinedBy <https://www.ica.org/standards/RiC/ontology> ;
    rdfs:label "a pour lieu de naissance"@fr, "has birth place"@en, "tiene como lugar de nacimiento"@es ;
    rdfs:range :Place ;
    rdfs:subPropertyOf :isAgentAssociatedWithPlace ;
    owl:inverseOf :isBirthPlaceOf ;
    skos:changeNote [
        dc:date "2023-11-27" ;
        rdf:value "Added a new rdfs:label in Spanish."@en
    ], [
        dc:date "2023-11-12" ;
        rdf:value "Updated the description (rdfs:comment)."@en
    ], [
        dc:date "2023-10-26" ;
        rdf:value "Fixed the domain of the property."@en
    ], [
        dc:date "2023-10-19" ;
        rdf:value "Added for RiC-O 1.0."@en
    ] .

:hasCarrierType
    a owl:ObjectProperty ;
    rdfs:comment """Connects an Instantiation to a Carrier Type which categorizes its
         carrier."""@en ;
    rdfs:domain :Instantiation ;
    rdfs:isDefinedBy <https://www.ica.org/standards/RiC/ontology> ;
    rdfs:label "a pour type de support"@fr, "has carrier type"@en, "tiene como tipo de soporte"@es ;
    rdfs:range :CarrierType ;
    rdfs:subPropertyOf :hasOrHadType ;
    owl:inverseOf :isCarrierTypeOf ;
    skos:changeNote [
        dc:date "2023-11-02" ;
        rdf:value "Added a new rdfs:label in Spanish."@en
    ], [
        dc:date "2023-08-28" ;
        rdf:value "Added a new rdfs:label in French."@en
    ], [
        dc:date "2021-01-22" ;
        rdf:value "changed the superproperty IRI."@en
    ] .

:hasChild
    a owl:ObjectProperty ;
    rdfs:comment "Connects a Person to one of their children."@en ;
    rdfs:domain :Person ;
    rdfs:isDefinedBy <https://www.ica.org/standards/RiC/ontology> ;
    rdfs:label "a pour enfant"@fr, "has child"@en, "tiene como hijo o hija a"@es ;
    rdfs:range :Person ;
    rdfs:subPropertyOf :hasDescendant ;
    owl:inverseOf :isChildOf ;
    owl:propertyChainAxiom (:thingIsSourceOfRelation
        :childRelation_role
        :relationHasTarget
    ) ;
    skos:changeNote [
        dc:date "2023-11-08" ;
        rdf:value """In order to get a system of rolified Relation classes: modified
               the property chain axiom so that it now involves the new childRelation_role object
               property."""@en
    ], [
        dc:date "2023-11-02" ;
        rdf:value "Added a new rdfs:label in Spanish."@en
    ], [
        dc:date "2023-08-28" ;
        rdf:value "Added a new rdfs:label in French."@en
    ], [
        dc:date "2021-01-22" ;
        rdf:value "changed the inverse property IRI."@en
    ] ;
    :RiCCMCorrespondingComponent """RiC-R018 ('has child'
         relation)"""@en .

:hasCollector
    a owl:ObjectProperty ;
    rdfs:comment """Connects a Record Resource or an Instantiation to the Agent that
         collects it intentionally, i.e., the Agent is a collector."""@en ;
    rdfs:domain [
        a owl:Class ;
        owl:unionOf (:Instantiation
            :RecordResource
        )
    ] ;
    rdfs:isDefinedBy <https://www.ica.org/standards/RiC/ontology> ;
    rdfs:label "est collecté par"@fr, "has collector"@en, "tiene como coleccionista a"@es ;
    rdfs:range :Agent ;
    rdfs:subPropertyOf :hasAccumulator ;
    owl:inverseOf :isCollectorOf ;
    skos:changeNote [
        dc:date "2023-11-12" ;
        rdf:value """Aligned with RiC-CM 1.0: updated the description
               (rdfs:comment)."""@en
    ], [
        dc:date "2023-11-02" ;
        rdf:value "Added a new rdfs:label in Spanish."@en
    ], [
        dc:date "2023-08-28" ;
        rdf:value "Added a new rdfs:label in French."@en
    ], [
        dc:date "2021-01-22" ;
        rdf:value """changed the IRI, label, inverse property and super property
               IRI, text definition, domain (changed made in order to make RiC-O compliant with
               RiC-CM 0.2; the name of this property in RiC-O 0.1 was \"collectedBy\")."""@en
    ] ;
    :RiCCMCorrespondingComponent """RiC-R030 ('has collector'
         relation)"""@en .

:hasComponentTransitive
    a owl:ObjectProperty, owl:TransitiveProperty ;
    rdfs:comment """Connects an Instantiation to another Instantiation that is,
         directly or indirectly, a component of that Instantiation. This is a transitive
         relation."""@en ;
    rdfs:domain :Instantiation ;
    rdfs:isDefinedBy <https://www.ica.org/standards/RiC/ontology> ;
    rdfs:label "a pour composant transitif"@fr, "has component transitive"@en, "tiene como componente transitivo"@es ;
    rdfs:range :Instantiation ;
    rdfs:subPropertyOf :hasOrHadComponent, :hasPartTransitive ;
    owl:inverseOf :isComponentOfTransitive ;
    skos:changeNote [
        dc:date "2023-11-27" ;
        rdf:value "Added a new rdfs:label in Spanish."@en
    ], [
        dc:date "2023-11-12" ;
        rdf:value "Updated the description (rdfs:comment) and labels."@en
    ], [
        dc:date "2023-09-08" ;
        rdf:value """Object property added, along with its inverse property, in
               order to enable to express current partitive relations between instantiations (the
               past partitive relation also being added)."""@en
    ] .

:hasConstituentProxy
    a owl:ObjectProperty ;
    rdfs:comment """Inverse of 'proxy is constituent of' object
         property."""@en ;
    rdfs:domain [
        a owl:Class ;
        owl:unionOf (:Record
            :RecordPart
        )
    ] ;
    rdfs:isDefinedBy <https://www.ica.org/standards/RiC/ontology> ;
    rdfs:label "a pour constituant le proxy"@fr, "has constituent proxy"@en, "tiene como elemento constitutivo el proxy"@es ;
    rdfs:range :Proxy ;
    rdfs:subPropertyOf :hasPartTransitive ;
    owl:inverseOf :proxyIsConstituentOf ;
    owl:propertyChainAxiom (:hasConstituentProxy
        :proxyHasConstituentProxyTransitive
    ) ;
    skos:changeNote [
        dc:date "2025-04-02" ;
        rdf:value "Added the French and Spanish labels."@en
    ], [
        dc:date "2025-04-02" ;
        rdf:value """Fixed the owl:subPropertyOf (was set to
               isPartOfTransitive)."""@en
    ], [
        dc:date "2025-03-04" ;
        rdf:value "Introduced in RiC-O 1.1."@en
    ] .

:hasConstituentTransitive
    a owl:ObjectProperty, owl:TransitiveProperty ;
    rdfs:comment """Connects a Record or Record Part to another Record or Record Part
         that is its constituent, directly or indirectly. This is a transitive
         relation."""@en ;
    rdfs:domain [
        a owl:Class ;
        owl:unionOf (:Record
            :RecordPart
        )
    ] ;
    rdfs:isDefinedBy <https://www.ica.org/standards/RiC/ontology> ;
    rdfs:label "a pour constituant transitif"@fr, "has constituent transitive"@en, "tiene como elemento constitutivo transitivo"@es ;
    rdfs:range [
        a owl:Class ;
        owl:unionOf (:Record
            :RecordPart
        )
    ] ;
    rdfs:subPropertyOf :hasOrHadConstituent, :hasPartTransitive ;
    owl:inverseOf :isConstituentOfTransitive ;
    owl:propertyChainAxiom (:hasConstituentProxy
        :proxyHasConstituent
    ) ;
    skos:changeNote [
        dc:date "2025-03-04" ;
        rdf:value """Added a property chain axiom relating it to use of
               rico:Proxy."""@en
    ], [
        dc:date "2023-11-27" ;
        rdf:value "Added a new rdfs:label in Spanish."@en
    ], [
        dc:date "2023-11-12" ;
        rdf:value "Updated the description (rdfs:comment) and labels."@en
    ], [
        dc:date "2023-10-26" ;
        rdf:value "Added RecordPart to the domain."@en
    ], [
        dc:date "2023-09-08" ;
        rdf:value """Object property added, along with its inverse property, in
               order to enable to express current partitive relations between records and other
               records or record parts (the past partitive relation also being added)."""@en
    ] .

:hasContentOfType
    a owl:ObjectProperty ;
    rdfs:comment """Connects a Record or a Record Part to a Content Type which
         categorizes its content."""@en ;
    rdfs:domain [
        a owl:Class ;
        owl:unionOf (:Record
            :RecordPart
        )
    ] ;
    rdfs:isDefinedBy <https://www.ica.org/standards/RiC/ontology> ;
    rdfs:label "a pour type de contenu"@fr, "has content of type"@en, "tiene como tipo de contenido"@es ;
    rdfs:range :ContentType ;
    rdfs:subPropertyOf :hasOrHadType ;
    owl:inverseOf :isContentTypeOf ;
    skos:changeNote [
        dc:date "2023-11-02" ;
        rdf:value "Added a new rdfs:label in Spanish."@en
    ], [
        dc:date "2023-08-28" ;
        rdf:value "Added a new rdfs:label in French."@en
    ], [
        dc:date "2021-01-22" ;
        rdf:value "changed the text definition and superproperty IRI."@en
    ] .

:hasContentWhichMainlyRepresents
    a owl:ObjectProperty ;
    rdfs:comment """Connects a Record or a Record Part to a Thing that its content
         mainly represents."""@en ;
    rdfs:domain [
        a owl:Class ;
        owl:unionOf (:Record
            :RecordPart
        )
    ] ;
    rdfs:isDefinedBy <https://www.ica.org/standards/RiC/ontology> ;
    rdfs:label "a un contenu qui représente principalement"@fr, "has content which mainly represents"@en, "tiene contenido que representa principalmente"@es ;
    rdfs:range :Thing ;
    rdfs:subPropertyOf :hasContentWhichRepresents, :hasOrHadMainSubject ;
    owl:inverseOf :isMainThingRepresentedByContentOf ;
    skos:changeNote [
        dc:date "2025-04-04" ;
        rdf:value "Introduced in RiC-O 1.1."@en
    ] ;
    skos:scopeNote """A common use case would be to connect a photograph of a person
         (a portrait) and the person represented."""@en .

:hasContentWhichRepresents
    a owl:ObjectProperty ;
    rdfs:comment """Connects a Record or a Record Part to a Thing that its content
         represents."""@en ;
    rdfs:domain [
        a owl:Class ;
        owl:unionOf (:Record
            :RecordPart
        )
    ] ;
    rdfs:isDefinedBy <https://www.ica.org/standards/RiC/ontology> ;
    rdfs:label "a un contenu qui représente"@fr, "has content which represents"@en, "tiene contenido que representa"@es ;
    rdfs:range :Thing ;
    rdfs:subPropertyOf :hasOrHadSubject ;
    owl:inverseOf :isRepresentedByContentOf ;
    skos:changeNote [
        dc:date "2025-04-04" ;
        rdf:value "Introduced in RiC-O 1.1."@en
    ] ;
    skos:scopeNote """Can be used for visual Records or Record Parts, like
         photographs, drawings, engravings, miniatures..."""@en .

:hasCopy
    a owl:ObjectProperty ;
    rdfs:comment """Connects a Record Resource to a copy of that Record
         Resource."""@en ;
    rdfs:domain :RecordResource ;
    rdfs:isDefinedBy <https://www.ica.org/standards/RiC/ontology> ;
    rdfs:label "a pour copie"@fr, "has copy"@en, "tiene como copia"@es ;
    rdfs:range :RecordResource ;
    rdfs:subPropertyOf :hasGeneticLinkToRecordResource, :precedesInTime ;
    owl:inverseOf :isCopyOf ;
    skos:changeNote [
        dc:date "2023-11-12" ;
        rdf:value """Aligned with RiC-CM 1.0: updated the
               skos:scopeNote."""@en
    ], [
        dc:date "2023-11-02" ;
        rdf:value "Added a new rdfs:label in Spanish."@en
    ], [
        dc:date "2023-08-28" ;
        rdf:value "Added a new rdfs:label in French."@en
    ] ;
    skos:scopeNote """Is both a temporal and genetic relation between the two Record
         Resources."""@en ;
    :RiCCMCorrespondingComponent """RiC-R012 ('has copy'
         relation)"""@en .

:hasCreationDate
    a owl:ObjectProperty ;
    rdfs:comment "Inverse of 'is creation date of' object property"@en ;
    rdfs:domain [
        a owl:Class ;
        owl:unionOf (:Instantiation
            :RecordResource
        )
    ] ;
    rdfs:isDefinedBy <https://www.ica.org/standards/RiC/ontology> ;
    rdfs:label "a pour date de création"@fr, "has creation date"@en, "tiene como fecha de creación"@es ;
    rdfs:range :Date ;
    rdfs:subPropertyOf :hasBeginningDate, :hasOrganicProvenanceDate ;
    owl:inverseOf :isCreationDateOf ;
    owl:propertyChainAxiom (:thingIsSourceOfRelation
        :creationRelation_role
        :relationHasDate
    ) ;
    skos:changeNote [
        dc:date "2024-12-19" ;
        rdf:value """Connect to CreationRelation via a sub-property chain, and make
               a sub-property of the new object property 'hasOrganicProvenanceDate'."""@en
    ], [
        dc:date "2023-11-27" ;
        rdf:value "Added a new rdfs:label in Spanish."@en
    ], [
        dc:date "2023-09-22" ;
        rdf:value "Added in RiC-O 1.0."@en
    ] ;
    :RiCCMCorrespondingComponent """RiC-R080i ('has creation date'
         relation)"""@en .

:hasCreator
    a owl:ObjectProperty ;
    rdfs:comment """Connects a Record Resource or an Instantiation to an Agent that is
         either responsible for all or some of the content of the Record Resource or is a
         contributor to the genesis or production of an Instantiation."""@en ;
    rdfs:domain [
        a owl:Class ;
        owl:unionOf (:Instantiation
            :RecordResource
        )
    ] ;
    rdfs:isDefinedBy <https://www.ica.org/standards/RiC/ontology> ;
    rdfs:label "a pour créateur"@fr, "has creator"@en, "tiene como creador a"@es ;
    rdfs:range :Agent ;
    rdfs:subPropertyOf :hasOrganicProvenance ;
    owl:inverseOf :isCreatorOf ;
    owl:propertyChainAxiom (:thingIsSourceOfRelation
        :creationRelation_role
        :relationHasTarget
    ) ;
    skos:changeNote [
        dc:date "2023-12-29" ;
        rdf:value """Added the property chain axiom, that had been
               forgotten."""@en
    ], [
        dc:date "2023-11-02" ;
        rdf:value "Added a new rdfs:label in Spanish."@en
    ], [
        dc:date "2023-08-28" ;
        rdf:value "Added a new rdfs:label in French."@en
    ], [
        dc:date "2021-01-22" ;
        rdf:value """changed the IRI and label (changed made in order to make RiC-O
               compliant with RiC-CM 0.2; the name of this property in RiC-O 0.1 was
               \"createdBy\")."""@en
    ] ;
    skos:scopeNote """Covers the definition of author in diplomatics, and any
         contribution to the intellectual content of a Record Resource."""@en ;
    :RiCCMCorrespondingComponent """RiC-R027 ('has creator'
         relation)"""@en .

:hasDateType
    a owl:ObjectProperty ;
    rdfs:comment "Connects a Date to its Date Type."@en ;
    rdfs:domain :Date ;
    rdfs:isDefinedBy <https://www.ica.org/standards/RiC/ontology> ;
    rdfs:label "a pour type de date"@fr, "has date type"@en, "tiene como tipo de fecha"@es ;
    rdfs:range :DateType ;
    rdfs:subPropertyOf :hasOrHadType ;
    owl:inverseOf :isDateTypeOf ;
    skos:changeNote [
        dc:date "2023-11-27" ;
        rdf:value "Added a new rdfs:label in Spanish."@en
    ], [
        dc:date "2023-10-10" ;
        rdf:value "Added a rdfs:comment and a French rdfs:label."@en
    ], [
        dc:date "2023-09-22" ;
        rdf:value "Added in RiC-O 1.0."@en
    ] .

:hasDeathDate
    a owl:ObjectProperty ;
    rdfs:comment "Inverse of 'is death date of' object property."@en ;
    rdfs:domain :Person ;
    rdfs:isDefinedBy <https://www.ica.org/standards/RiC/ontology> ;
    rdfs:label "a pour date de décès"@fr, "has death date"@en, "tiene como fecha de muerte"@es ;
    rdfs:range :Date ;
    rdfs:subPropertyOf :hasEndDate ;
    owl:inverseOf :isDeathDateOf ;
    skos:changeNote [
        dc:date "2023-11-02" ;
        rdf:value "Added a new rdfs:label in Spanish."@en
    ], [
        dc:date "2023-08-28" ;
        rdf:value "Added a new rdfs:label in French."@en
    ] ;
    :RiCCMCorrespondingComponent """RiC-R072i ('has death date'
         relation)"""@en .

:hasDeathPlace
    a owl:ObjectProperty ;
    rdfs:comment "Inverse of 'is death place of' object property."@en ;
    rdfs:domain :Person ;
    rdfs:isDefinedBy <https://www.ica.org/standards/RiC/ontology> ;
    rdfs:label "a pour lieu de décès"@fr, "has death place"@en, "tiene como lugar de muerte"@es ;
    rdfs:range :Place ;
    rdfs:subPropertyOf :isAgentAssociatedWithPlace ;
    owl:inverseOf :isDeathPlaceOf ;
    skos:changeNote [
        dc:date "2023-11-27" ;
        rdf:value "Added a new rdfs:label in Spanish."@en
    ], [
        dc:date "2023-11-13" ;
        rdf:value "Added a rdfs:comment."@en
    ], [
        dc:date "2023-10-26" ;
        rdf:value "Fixed the domain of the property."@en
    ], [
        dc:date "2023-10-19" ;
        rdf:value "Added for RiC-O v1.0."@en
    ] .

:hasDerivationDate
    a owl:ObjectProperty ;
    rdfs:comment "Inverse of 'is derivation date of' object property."@en ;
    rdfs:domain :Instantiation ;
    rdfs:isDefinedBy <https://www.ica.org/standards/RiC/ontology> ;
    rdfs:label "a pour date de dérivation"@fr, "has derivation date"@en, "tiene como fecha de derivación"@es ;
    rdfs:range :Date ;
    rdfs:subPropertyOf :isAssociatedWithDate ;
    owl:inverseOf :isDerivationDateOf ;
    owl:propertyChainAxiom (:thingIsSourceOfRelation
        :derivationRelation_role
        :relationHasDate
    ) ;
    skos:changeNote [
        dc:date "2025-03-13" ;
        rdf:value "Added the property chain axiom."@en
    ], [
        dc:date "2025-03-01" ;
        rdf:value "Added in RiC-O 1.1."@en
    ] .

:hasDescendant
    a owl:ObjectProperty, owl:TransitiveProperty ;
    rdfs:comment """Connects a Person to one of their descendants. This is a
         transitive relation."""@en ;
    rdfs:domain :Person ;
    rdfs:isDefinedBy <https://www.ica.org/standards/RiC/ontology> ;
    rdfs:label "a pour descendant"@fr, "has descendant"@en, "tiene como descendiente a"@es ;
    rdfs:range :Person ;
    rdfs:subPropertyOf :hasFamilyAssociationWith, :hasSuccessor ;
    owl:inverseOf :hasAncestor ;
    owl:propertyChainAxiom (:thingIsSourceOfRelation
        :descendanceRelation_role
        :relationHasTarget
    ) ;
    skos:changeNote [
        dc:date "2023-11-12" ;
        rdf:value """Aligned with RiC-CM 1.0: updated the
               skos:scopeNote."""@en
    ], [
        dc:date "2023-11-08" ;
        rdf:value """In order to get a system of rolified Relation classes: modified
               the property chain axiom so that it now involves the new descendanceRelation_role
               object property."""@en
    ], [
        dc:date "2023-11-02" ;
        rdf:value "Added a new rdfs:label in Spanish."@en
    ], [
        dc:date "2023-09-08" ;
        rdf:value "made property transitive"@en
    ], [
        dc:date "2023-08-28" ;
        rdf:value "Added a new rdfs:label in French."@en
    ], [
        dc:date "2021-01-22" ;
        rdf:value "changed the superproperties IRIs."@en
    ] ;
    skos:scopeNote """There may be zero to many intermediate persons, ignored or
         unknown, between the two connected persons."""@en ;
    :RiCCMCorrespondingComponent """RiC-R017 ('has descendant'
         relation)"""@en .

:hasDestructionDate
    a owl:ObjectProperty ;
    rdfs:comment """Inverse of 'is destruction date of' object
         property."""@en ;
    rdfs:domain [
        a owl:Class ;
        owl:unionOf (:Instantiation
            :RecordResource
        )
    ] ;
    rdfs:isDefinedBy <https://www.ica.org/standards/RiC/ontology> ;
    rdfs:label "a pour date de destruction"@fr, "has destruction date"@en, "tiene como fecha de destrucción"@es ;
    rdfs:range :Date ;
    rdfs:subPropertyOf :hasEndDate ;
    owl:inverseOf :isDestructionDateOf ;
    skos:changeNote [
        dc:date "2025-02-19" ;
        rdf:value "Changed domain."@en
    ], [
        dc:date "2023-11-27" ;
        rdf:value "Added a new rdfs:label in Spanish."@en
    ], [
        dc:date "2023-10-14" ;
        rdf:value "Added a rdfs:comment; same to the inverse property."@en
    ], [
        dc:date "2023-10-12" ;
        rdf:value "Renamed deletion into destruction"@en
    ], [
        dc:date "2023-09-22" ;
        rdf:value "Added in RiC-O 1.0."@en
    ] .

:hasDirectComponent
    a owl:ObjectProperty ;
    rdfs:comment """Connects an Instantiation to another Instantiation that is its
         direct component."""@en ;
    rdfs:domain :Instantiation ;
    rdfs:isDefinedBy <https://www.ica.org/standards/RiC/ontology> ;
    rdfs:label "a directement pour composant"@fr, "has direct component"@en, "tiene directamente como componente"@es ;
    rdfs:range :Instantiation ;
    rdfs:subPropertyOf :hasComponentTransitive, :hasDirectPart ;
    owl:inverseOf :isDirectComponentOf ;
    skos:changeNote [
        dc:date "2023-11-27" ;
        rdf:value "Added a new rdfs:label in Spanish."@en
    ], [
        dc:date "2023-11-12" ;
        rdf:value "Updated the labels."@en
    ], [
        dc:date "2023-09-08" ;
        rdf:value """Object property added, along with its inverse property, in
               order to enable to express current, direct, partitive relations between
               instantiations (the possibly indirect, transitive relation, superproperty of this
               one, being also added)."""@en
    ] .

:hasDirectConstituent
    a owl:ObjectProperty ;
    rdfs:comment """Connects a Record or Record Part to another Record or Record Part
         that is its direct constituent."""@en ;
    rdfs:domain [
        a owl:Class ;
        owl:unionOf (:Record
            :RecordPart
        )
    ] ;
    rdfs:isDefinedBy <https://www.ica.org/standards/RiC/ontology> ;
    rdfs:label "a directement pour constituant"@fr, "has direct constituent"@en, "tiene directamente como elemento constitutivo"@es ;
    rdfs:range [
        a owl:Class ;
        owl:unionOf (:Record
            :RecordPart
        )
    ] ;
    rdfs:subPropertyOf :hasConstituentTransitive, :hasDirectPart ;
    owl:inverseOf :isDirectConstituentOf ;
    owl:propertyChainAxiom (:hasDirectConstituentProxy
        :proxyFor
    ) ;
    skos:changeNote [
        dc:date "2025-04-03" ;
        rdf:value "Fixed the property chain axiom."@en
    ], [
        dc:date "2025-03-04" ;
        rdf:value """Added a property chain axiom relating it to use of
               rico:Proxy."""@en
    ], [
        dc:date "2023-11-27" ;
        rdf:value "Added a new rdfs:label in Spanish."@en
    ], [
        dc:date "2023-11-12" ;
        rdf:value "Updated the labels."@en
    ], [
        dc:date "2023-10-26" ;
        rdf:value "Added RecordPart to the domain."@en
    ], [
        dc:date "2023-09-08" ;
        rdf:value """Object property added, along with its inverse property, in
               order to enable to express current, direct, partitive relations between records and
               other records or record parts (the possibly indirect, transitive relation,
               superproperty of this one, being also added)."""@en
    ] .

:hasDirectConstituentProxy
    a owl:ObjectProperty ;
    rdfs:comment """Inverse of 'proxy is direct constituent of' object
         property."""@en ;
    rdfs:domain [
        a owl:Class ;
        owl:unionOf (:Record
            :RecordPart
        )
    ] ;
    rdfs:isDefinedBy <https://www.ica.org/standards/RiC/ontology> ;
    rdfs:label "a pour constituant direct le proxy"@fr, "has direct constituent proxy"@en, "tiene como directo elemento constitutivo el proxy"@es ;
    rdfs:range :Proxy ;
    rdfs:subPropertyOf :hasConstituentProxy, :hasDirectPart ;
    owl:inverseOf :proxyIsDirectConstituentOf ;
    skos:changeNote [
        dc:date "2025-04-02" ;
        rdf:value "Added the French and Spanish labels."@en
    ], [
        dc:date "2025-03-04" ;
        rdf:value "Introduced in RiC-O 1.1."@en
    ] .

:hasDirectPart
    a owl:ObjectProperty ;
    rdfs:comment """Connects a Thing to a Thing that is a direct constitutive or
         component part of that Thing."""@en ;
    rdfs:domain :Thing ;
    rdfs:isDefinedBy <https://www.ica.org/standards/RiC/ontology> ;
    rdfs:label "a directement pour partie"@fr, "has direct part"@en, "tiene directamente como parte"@es ;
    rdfs:range :Thing ;
    rdfs:subPropertyOf :hasPartTransitive ;
    owl:inverseOf :isDirectPartOf ;
    skos:changeNote [
        dc:date "2023-11-27" ;
        rdf:value "Added a new rdfs:label in Spanish."@en
    ], [
        dc:date "2023-11-12" ;
        rdf:value "Updated the labels."@en
    ], [
        dc:date "2023-07-12" ;
        rdf:value """Object property added, along with its inverse property, in
               order to enable to express current, direct, partitive relations between things (the
               possibly indirect, transitive relation, superproperty of this one, being also
               added)."""@en
    ] ;
    skos:scopeNote """To be used only when the current partitive relation is direct,
         without any intermediate node between the related things."""@en .

:hasDirectSubdivision
    a owl:ObjectProperty ;
    rdfs:comment "Connects a Group to one of its direct subdivisions."@en ;
    rdfs:domain :Group ;
    rdfs:isDefinedBy <https://www.ica.org/standards/RiC/ontology> ;
    rdfs:label "a directement pour subdivision"@fr, "has direct subdivision"@en, "tiene directamente como subdivisión"@es ;
    rdfs:range :Group ;
    rdfs:subPropertyOf :hasDirectPart, :hasDirectSubordinate, :hasSubdivisionTransitive ;
    owl:inverseOf :isDirectSubdivisionOf ;
    skos:changeNote [
        dc:date "2023-11-27" ;
        rdf:value "Added a new rdfs:label in Spanish."@en
    ], [
        dc:date "2023-11-12" ;
        rdf:value "Updated the labels."@en
    ], [
        dc:date "2023-09-08" ;
        rdf:value """Object property added, along with its inverse property, in
               order to enable to express current, direct, partitive relations between groups (the
               possibly indirect, transitive relation, superproperty of this one, being also
               added)."""@en
    ] .

:hasDirectSubevent
    a owl:ObjectProperty ;
    rdfs:comment """Connects an ongoing Event to one of a series of Events that
         directly constitute that broader, ongoing Event."""@en ;
    rdfs:domain :Event ;
    rdfs:isDefinedBy <https://www.ica.org/standards/RiC/ontology> ;
    rdfs:label "est directement constitué de l’événement"@fr, "has direct subevent"@en, "tiene directamente como parte de evento"@es ;
    rdfs:range :Event ;
    rdfs:subPropertyOf :hasDirectPart, :hasSubeventTransitive ;
    owl:inverseOf :isDirectSubeventOf ;
    skos:changeNote [
        dc:date "2023-11-27" ;
        rdf:value "Added a new rdfs:label in Spanish."@en
    ], [
        dc:date "2023-11-12" ;
        rdf:value "Updated the labels."@en
    ], [
        dc:date "2023-09-08" ;
        rdf:value """Object property added, along with its inverse property, in
               order to enable to express current, direct, partitive relations between ongoing
               events (the possibly indirect, transitive relation, superproperty of this one, being
               also added)."""@en
    ] .

:hasDirectSubordinate
    a owl:ObjectProperty ;
    rdfs:comment """Connects an Agent to an Agent that is its direct
         subordinate."""@en ;
    rdfs:domain :Agent ;
    rdfs:isDefinedBy <https://www.ica.org/standards/RiC/ontology> ;
    rdfs:label "a directement pour subalterne"@fr, "has direct subordinate"@en, "tiene directamente como subordinado o subordinada a"@es ;
    rdfs:range :Agent ;
    rdfs:subPropertyOf :hasSubordinateTransitive ;
    owl:inverseOf :isDirectSubordinateTo ;
    skos:changeNote [
        dc:date "2023-11-27" ;
        rdf:value "Added a new rdfs:label in Spanish."@en
    ], [
        dc:date "2023-11-12" ;
        rdf:value "Updated the labels."@en
    ], [
        dc:date "2023-09-08" ;
        rdf:value """Object property added, along with its inverse property, in
               order to enable to express current, direct, subordination relations between agents
               (the possibly indirect, transitive relation, superproperty of this one, being also
               added)."""@en
    ] .

:hasDocumentaryFormType
    a owl:ObjectProperty ;
    rdfs:comment """Connects a Record or Record Part to its Documentary Form
         Type."""@en ;
    rdfs:domain [
        a owl:Class ;
        owl:unionOf (:Record
            :RecordPart
        )
    ] ;
    rdfs:isDefinedBy <https://www.ica.org/standards/RiC/ontology> ;
    rdfs:label "a pour type d’objet informationnel"@fr, "has documentary form type"@en, "tiene como tipo documental"@es ;
    rdfs:range :DocumentaryFormType ;
    rdfs:subPropertyOf :hasOrHadType ;
    owl:inverseOf :isDocumentaryFormTypeOf ;
    skos:changeNote [
        dc:date "2023-12-30" ;
        rdf:value "Fixed a typo in the French label."@en
    ], [
        dc:date "2023-11-02" ;
        rdf:value "Added a new rdfs:label in Spanish."@en
    ], [
        dc:date "2023-08-28" ;
        rdf:value "Added a new rdfs:label in French."@en
    ], [
        dc:date "2021-01-22" ;
        rdf:value "changed the superproperty IRI."@en
    ] .

:hasDraft
    a owl:ObjectProperty ;
    rdfs:comment "Inverse of 'is draft of' object property."@en ;
    rdfs:domain [
        a owl:Class ;
        owl:unionOf (:Record
            :RecordPart
        )
    ] ;
    rdfs:isDefinedBy <https://www.ica.org/standards/RiC/ontology> ;
    rdfs:label "a pour ébauche"@fr, "has draft"@en, "tiene como borrador"@es ;
    rdfs:range [
        a owl:Class ;
        owl:unionOf (:Record
            :RecordPart
        )
    ] ;
    rdfs:subPropertyOf :followsInTime, :hasGeneticLinkToRecordResource ;
    owl:inverseOf :isDraftOf ;
    skos:changeNote [
        dc:date "2023-11-02" ;
        rdf:value "Added a new rdfs:label in Spanish."@en
    ], [
        dc:date "2023-08-28" ;
        rdf:value "Added a new rdfs:label in French."@en
    ] ;
    :RiCCMCorrespondingComponent """RiC-011i ('has draft'
         relation)"""@en .

:hasEndDate
    a owl:ObjectProperty ;
    rdfs:comment "Inverse of 'is end date of' object property."@en ;
    rdfs:domain :Thing ;
    rdfs:isDefinedBy <https://www.ica.org/standards/RiC/ontology> ;
    rdfs:label "a pour date de fin"@fr, "has end date"@en, "tiene como fecha final"@es ;
    rdfs:range :Date ;
    rdfs:subPropertyOf :isAssociatedWithDate ;
    owl:inverseOf :isEndDateOf ;
    skos:changeNote [
        dc:date "2023-11-02" ;
        rdf:value "Added a new rdfs:label in Spanish."@en
    ], [
        dc:date "2023-08-28" ;
        rdf:value "Added a new rdfs:label in French."@en
    ] ;
    :RiCCMCorrespondingComponent """RiC-R071i ('has end date'
         relation)"""@en .

:hasEventType
    a owl:ObjectProperty ;
    rdfs:comment """Connects an Event to an Event Type which categorizes
         it."""@en ;
    rdfs:domain :Event ;
    rdfs:isDefinedBy <https://www.ica.org/standards/RiC/ontology> ;
    rdfs:label "a pour type d’événement"@fr, "has event type"@en, "tiene como tipo de evento"@es ;
    rdfs:range :EventType ;
    rdfs:subPropertyOf :hasOrHadType ;
    owl:inverseOf :isEventTypeOf ;
    skos:changeNote [
        dc:date "2023-11-02" ;
        rdf:value "Added a new rdfs:label in Spanish."@en
    ], [
        dc:date "2023-08-28" ;
        rdf:value "Added a new rdfs:label in French."@en
    ], [
        dc:date "2021-01-22" ;
        rdf:value "changed the superproperty IRI."@en
    ] .

:hasExtent
    a owl:ObjectProperty ;
    rdfs:comment """Connects a Record Resource or Instantiation to an
         Extent"""@en ;
    rdfs:domain :Thing ;
    rdfs:isDefinedBy <https://www.ica.org/standards/RiC/ontology> ;
    rdfs:label "a pour mesure"@fr, "has extent"@en, "tiene como extensión"@es ;
    rdfs:range :Extent ;
    rdfs:subPropertyOf :isRelatedTo ;
    owl:inverseOf :isExtentOf ;
    skos:changeNote [
        dc:date "2023-11-02" ;
        rdf:value "Added a new rdfs:label in Spanish."@en
    ], [
        dc:date "2023-08-28" ;
        rdf:value """Added a new rdfs:label in French; added an xml:lang attribute
               to the rdfs:comment."""@en
    ], [
        dc:date "2023-08-28" ;
        rdf:value """Changed the domain (was Instantiation or RecordResource) to
               Thing; changed the definition accordingly."""@en
    ], [
        dc:date "2020-10-28" ;
        rdf:value """Object property created along with the Extent class and its
               subclasses, in order to provide methods for handling extent accurately."""@en
    ] .

:hasExtentType
    a owl:ObjectProperty ;
    rdfs:comment """Connects an Extent to an Extent Type that categorizes what is
         being measured."""@en ;
    rdfs:domain :Extent ;
    rdfs:isDefinedBy <https://www.ica.org/standards/RiC/ontology> ;
    rdfs:label "a pour type de mesure"@fr, "has extent type"@en, "tiene como tipo de extensión"@es ;
    rdfs:range :ExtentType ;
    rdfs:subPropertyOf :hasOrHadType ;
    owl:inverseOf :isExtentTypeOf ;
    skos:changeNote [
        dc:date "2023-11-02" ;
        rdf:value "Added a new rdfs:label in Spanish."@en
    ], [
        dc:date "2023-08-28" ;
        rdf:value """Added a new rdfs:label in French; added an xml:lang attribute
               to the rdfs:comment."""@en
    ], [
        dc:date "2020-11-01" ;
        rdf:value """Object property added along with the Extent Type
               class."""@en
    ] .

:hasFamilyAssociationWith
    a owl:ObjectProperty, owl:SymmetricProperty ;
    rdfs:comment """Connects two Persons that have some type of family link, i.e.
         belong to the same family. This relation is symmetric."""@en ;
    rdfs:domain :Person ;
    rdfs:isDefinedBy <https://www.ica.org/standards/RiC/ontology> ;
    rdfs:label "a une relation familiale avec"@fr, "has family association with"@en, "tiene asociación familiar con"@es ;
    rdfs:range :Person ;
    rdfs:subPropertyOf :isAgentAssociatedWithAgent ;
    owl:propertyChainAxiom (:thingIsConnectedToRelation
        :familyRelation_role
        :relationConnects
    ) ;
    skos:changeNote [
        dc:date "2023-11-12" ;
        rdf:value """Aligned with RiC-CM 1.0: updated the
               skos:scopeNote."""@en
    ], [
        dc:date "2023-11-08" ;
        rdf:value """In order to get a system of rolified Relation classes: modified
               the property chain axiom so that it now involves the new familyRelation_role object
               property."""@en
    ], [
        dc:date "2023-11-02" ;
        rdf:value "Added a new rdfs:label in Spanish."@en
    ], [
        dc:date "2023-08-28" ;
        rdf:value "Added a new rdfs:label in French."@en
    ], [
        dc:date "2021-01-22" ;
        rdf:value """changed the IRI, label, textual definition (changed made in
               order to make RiC-O compliant with RiC-CM 0.2; the name of this property in RiC-O 0.1
               was \"hasFamilyLinkWith\")."""@en
    ] ;
    skos:scopeNote """Use hasOrHadMember for connecting a Family and a
         Person."""@en ;
    :RiCCMCorrespondingComponent """RiC-R047 ('has family association with'
         relation)"""@en .

:hasFamilyType
    a owl:ObjectProperty ;
    rdfs:comment """Connects a Family to a Family Type that categorizes
         it."""@en ;
    rdfs:domain :Family ;
    rdfs:isDefinedBy <https://www.ica.org/standards/RiC/ontology> ;
    rdfs:label "a pour type de famille"@fr, "has family type"@en, "tiene como tipo de familia"@es ;
    rdfs:range :FamilyType ;
    rdfs:subPropertyOf :hasOrHadType ;
    owl:inverseOf :isFamilyTypeOf ;
    skos:changeNote [
        dc:date "2023-11-02" ;
        rdf:value "Added a new rdfs:label in Spanish."@en
    ], [
        dc:date "2023-08-28" ;
        rdf:value "Added a new rdfs:label in French."@en
    ], [
        dc:date "2021-01-22" ;
        rdf:value "changed the superproperty IRI."@en
    ] .

:hasGeneticLinkToRecordResource
    a owl:ObjectProperty, owl:SymmetricProperty ;
    rdfs:comment """Connects two Record Resources when there is a genetic link between
         them. Genetic in this sense is as defined by diplomatics, i.e. the process by which a
         Record Resource is developed. This relation is symmetric."""@en ;
    rdfs:domain :RecordResource ;
    rdfs:isDefinedBy <https://www.ica.org/standards/RiC/ontology> ;
    rdfs:label """a une relation génétique avec la ressource
         archivistique"""@fr, "has genetic link to record resource"@en, "tiene vínculo de origen con recurso documental"@es ;
    rdfs:range :RecordResource ;
    rdfs:subPropertyOf :isRecordResourceAssociatedWithRecordResource ;
    owl:propertyChainAxiom (:thingIsConnectedToRelation
        :recordResourceGeneticRelation_role
        :relationConnects
    ) ;
    skos:changeNote [
        dc:date "2023-11-12" ;
        rdf:value """Aligned with RiC-CM 1.0: updated the
               skos:scopeNote."""@en
    ], [
        dc:date "2023-11-08" ;
        rdf:value """In order to get a system of rolified Relation classes: modified
               the property chain axiom so that it now involves the new
               recordResourceGeneticRelation_role object property."""@en
    ], [
        dc:date "2023-11-07" ;
        rdf:value """Added the property chain axiom so that this property is
               formally defined as a shortcut."""@en
    ], [
        dc:date "2023-11-02" ;
        rdf:value "Added a new rdfs:label in Spanish."@en
    ], [
        dc:date "2023-08-28" ;
        rdf:value "Added a new rdfs:label in French."@en
    ] ;
    skos:scopeNote """Use to connect two Record Resources only if it is not possible
         to use a narrower, more specific, asymmetric Record Resource to Record Resource relation,
         for example is original of."""@en ;
    :RiCCMCorrespondingComponent """RiC-R023 ('has genetic link to record resource'
         relation)"""@en .

:hasIdentifierType
    a owl:ObjectProperty ;
    rdfs:comment """Connects an Identifier and an Identifier Type that categorizes
         it."""@en ;
    rdfs:domain :Identifier ;
    rdfs:isDefinedBy <https://www.ica.org/standards/RiC/ontology> ;
    rdfs:label "a pour type d’identifiant"@fr, "has identifier type"@en, "tiene como tipo de identificador"@es ;
    rdfs:range :IdentifierType ;
    rdfs:subPropertyOf :hasOrHadType ;
    owl:inverseOf :isIdentifierTypeOf ;
    skos:changeNote [
        dc:date "2023-11-02" ;
        rdf:value "Added a new rdfs:label in Spanish."@en
    ], [
        dc:date "2023-08-28" ;
        rdf:value "Added a new rdfs:label in French."@en
    ], [
        dc:date "2021-01-22" ;
        rdf:value "changed the superproperty IRI."@en
    ], [
        dc:date "2020-10-19" ;
        rdf:value """Object property added along with IdentifierType class and
               isIdentifierTypeOf object property. """@en
    ] .

:hasMigrationDate
    a owl:ObjectProperty ;
    rdfs:comment "Inverse of 'is migration date of' object property."@en ;
    rdfs:domain :Instantiation ;
    rdfs:isDefinedBy <https://www.ica.org/standards/RiC/ontology> ;
    rdfs:label "a pour date de migration"@fr, "has migration date"@en, "tiene como fecha de migración"@es ;
    rdfs:range :Date ;
    rdfs:subPropertyOf :hasDerivationDate ;
    owl:inverseOf :isMigrationDateOf ;
    owl:propertyChainAxiom (:thingIsSourceOfRelation
        :migrationRelation_role
        :relationHasDate
    ) ;
    skos:changeNote [
        dc:date "2025-03-13" ;
        rdf:value "Added the property chain axiom."@en
    ], [
        dc:date "2025-03-01" ;
        rdf:value """Made this property a subproperty of the new 'hasDerivationDate'
               property."""@en
    ], [
        dc:date "2025-02-19" ;
        rdf:value "Added in RiC-O 1.1."@en
    ] .

:hasModificationDate
    a owl:ObjectProperty ;
    rdfs:comment """Inverse of 'is modification date of' object
         property."""@en ;
    rdfs:domain :Thing ;
    rdfs:isDefinedBy <https://www.ica.org/standards/RiC/ontology> ;
    rdfs:label "a pour date de modification"@fr, "has modification date"@en, "tiene como fecha de modificación"@es ;
    rdfs:range :Date ;
    rdfs:subPropertyOf :isAssociatedWithDate ;
    owl:inverseOf :isModificationDateOf ;
    skos:changeNote [
        dc:date "2023-11-02" ;
        rdf:value "Added a new rdfs:label in Spanish."@en
    ], [
        dc:date "2023-08-28" ;
        rdf:value "Added a new rdfs:label in French."@en
    ] ;
    :RiCCMCorrespondingComponent """RiC-R073i ('has modification date'
         relation)"""@en .

:hasOrHadAgentName
    a owl:ObjectProperty ;
    rdfs:comment """Connects an Agent and (one of) its present or past Agent
         Name."""@en ;
    rdfs:domain :Agent ;
    rdfs:isDefinedBy <https://www.ica.org/standards/RiC/ontology> ;
    rdfs:label "a ou a eu pour nom d’agent"@fr, "has or had agent name"@en, "tiene o tenía como nombre de agente"@es ;
    rdfs:range :AgentName ;
    rdfs:subPropertyOf :hasOrHadName ;
    owl:inverseOf :isOrWasAgentNameOf ;
    skos:changeNote [
        dc:date "2023-11-02" ;
        rdf:value "Added a new rdfs:label in Spanish."@en
    ], [
        dc:date "2023-08-28" ;
        rdf:value "Added a new rdfs:label in French."@en
    ], [
        dc:date "2021-01-22" ;
        rdf:value """changed the IRI, label, inverse property IRI, textual
               definition (the name of this property in RiC-O 0.1 was \"hasAgentName\")."""@en
    ] .

:hasOrHadAllMembersWithAccumulationDate
    a owl:ObjectProperty ;
    rdfs:comment """Inverse of 'is or was accumulation date of all members of' object
         property."""@en ;
    rdfs:domain :RecordSet ;
    rdfs:isDefinedBy <https://www.ica.org/standards/RiC/ontology> ;
    rdfs:label "has or had all members with accumulation date"@en, """inclut ou a inclus des membres ayant tous pour date
         d'accumulation"""@fr, """incluye o incluía miembros, todos como fecha de
         acumulación"""@es ;
    rdfs:range :Date ;
    rdfs:subPropertyOf :isAssociatedWithDate ;
    owl:inverseOf :isOrWasAccumulationDateOfAllMembersOf ;
    skos:changeNote [
        dc:date "2025-04-06" ;
        rdf:value "Adjusted the Spanish label."@en
    ], [
        dc:date "2024-10-04" ;
        rdf:value "Added in RiC-O 1.1."@en
    ] .

:hasOrHadAllMembersWithContentType
    a owl:ObjectProperty ;
    rdfs:comment """Connects a Record Set and a Content Type that categorizes all the
         Records or Record Parts that are or were included in the Record Set."""@en ;
    rdfs:domain :RecordSet ;
    rdfs:isDefinedBy <https://www.ica.org/standards/RiC/ontology> ;
    rdfs:label "has or had all members with content type"@en, """inclut ou a inclus des membres ayant tous pour type de
         contenu"""@fr, "incluye o incluía miembros, todos con tipo de contenido"@es ;
    rdfs:range :ContentType ;
    rdfs:subPropertyOf :hasOrHadAllMembersWithType ;
    owl:inverseOf :isOrWasContentTypeOfAllMembersOf ;
    skos:changeNote [
        dc:date "2025-04-06" ;
        rdf:value "Adjusted the Spanish label."@en
    ], [
        dc:date "2023-11-02" ;
        rdf:value "Added a new rdfs:label in Spanish."@en
    ], [
        dc:date "2023-08-28" ;
        rdf:value "Added a new rdfs:label in French."@en
    ], [
        dc:date "2020-12-28" ;
        rdf:value """Object property added for handling the case where a Record Set
               is described as having all or some members that belong to some category (see RiC-CM
               0.2 attributes section, #4.4 on Record Set, Record and Record Part
               attributes)."""@en
    ] .

:hasOrHadAllMembersWithCreationDate
    a owl:ObjectProperty ;
    rdfs:comment """Inverse of 'is or was creation date of all members of' object
         property."""@en ;
    rdfs:domain :RecordSet ;
    rdfs:isDefinedBy <https://www.ica.org/standards/RiC/ontology> ;
    rdfs:label "has or had all members with creation date"@en, """inclut ou a inclus des membres ayant tous pour date de
         création"""@fr, "incluye o incluía miembros, todos con fecha de creación"@es ;
    rdfs:range :Date ;
    rdfs:subPropertyOf :hasBeginningDate ;
    owl:inverseOf :isOrWasCreationDateOfAllMembersOf ;
    skos:changeNote [
        dc:date "2025-04-06" ;
        rdf:value "Adjusted the Spanish label."@en
    ], [
        dc:date "2023-11-27" ;
        rdf:value "Added a new rdfs:label in Spanish."@en
    ], [
        dc:date "2023-10-13" ;
        rdf:value """Renamed the property in order to take the past members of the
               record set into account. Adjusted the annotations accordingly."""@en
    ], [
        dc:date "2023-10-12" ;
        rdf:value "Added the French label"@en
    ], [
        dc:date "2023-09-22" ;
        rdf:value "Added in RiC-O 1.0."@en
    ] ;
    :RiCCMCorrespondingComponent """RiC-R081i ('has or had all members with creation
         date' relation)"""@en .

:hasOrHadAllMembersWithDocumentaryFormType
    a owl:ObjectProperty ;
    rdfs:comment """Connects a Record Set and a Documentary Form Type that categorizes
         all the Records or Record Parts that are or were included in the Record Set."""@en ;
    rdfs:domain :RecordSet ;
    rdfs:isDefinedBy <https://www.ica.org/standards/RiC/ontology> ;
    rdfs:label "has or had all members with documentary form type"@en, "inclut ou a inclus des membres ayant tous pour type"@fr, "incluye o incluía miembros, todos con tipo documental"@es ;
    rdfs:range :DocumentaryFormType ;
    rdfs:subPropertyOf :hasOrHadAllMembersWithType ;
    owl:inverseOf :isOrWasDocumentaryFormTypeOfAllMembersOf ;
    skos:changeNote [
        dc:date "2025-04-06" ;
        rdf:value "Adjusted the Spanish label."@en
    ], [
        dc:date "2023-11-02" ;
        rdf:value "Added a new rdfs:label in Spanish."@en
    ], [
        dc:date "2023-08-28" ;
        rdf:value "Added a new rdfs:label in French."@en
    ], [
        dc:date "2020-12-28" ;
        rdf:value """Object property added for handling the case where a Record Set
               is described as having all or some members that belong to some category (see RiC-CM
               0.2 attributes section, #4.4 on Record Set, Record and Record Part
               attributes)."""@en
    ] .

:hasOrHadAllMembersWithLanguage
    a owl:ObjectProperty ;
    rdfs:comment """Connects a Record Set and a Language used by all the Records or
         Record Parts that are or were included in the Record Set."""@en ;
    rdfs:domain :RecordSet ;
    rdfs:isDefinedBy <https://www.ica.org/standards/RiC/ontology> ;
    rdfs:label "has or had all members with language"@en, "inclut ou a inclus des membres ayant tous pour langue"@fr, "incluye o incluía miembros, todos con lengua"@es ;
    rdfs:range :Language ;
    rdfs:subPropertyOf :isRelatedTo ;
    owl:inverseOf :isOrWasLanguageOfAllMembersOf ;
    skos:changeNote [
        dc:date "2025-04-06" ;
        rdf:value "Adjusted the Spanish label."@en
    ], [
        dc:date "2023-11-02" ;
        rdf:value "Added a new rdfs:label in Spanish."@en
    ], [
        dc:date "2023-08-28" ;
        rdf:value "Added a new rdfs:label in French."@en
    ], [
        dc:date "2020-12-28" ;
        rdf:value """Object property added for handling the case where a Record Set
               is described as having all or some members that belong to some category (see RiC-CM
               0.2 attributes section, #4.4 on Record Set, Record and Record Part
               attributes)."""@en
    ] .

:hasOrHadAllMembersWithLegalStatus
    a owl:ObjectProperty ;
    rdfs:comment """Connects a Record Set and a Legal Status that categorizes all the
         Records or Record Parts that are or were included in the Record Set."""@en ;
    rdfs:domain :RecordSet ;
    rdfs:isDefinedBy <https://www.ica.org/standards/RiC/ontology> ;
    rdfs:label "has or had all members with legal status"@en, """inclut ou a inclus des membres ayant tous pour statut
         légal"""@fr, "incluye o incluía miembros, todos con status jurídico"@es ;
    rdfs:range :LegalStatus ;
    rdfs:subPropertyOf :hasOrHadAllMembersWithType ;
    owl:inverseOf :isOrWasLegalStatusOfAllMembersOf ;
    skos:changeNote [
        dc:date "2025-04-06" ;
        rdf:value "Adjusted the Spanish label."@en
    ], [
        dc:date "2023-11-02" ;
        rdf:value "Added a new rdfs:label in Spanish."@en
    ], [
        dc:date "2023-08-28" ;
        rdf:value "Added a new rdfs:label in French."@en
    ], [
        dc:date "2020-12-28" ;
        rdf:value """Object property added for handling the case where a Record Set
               is described as having all or some members that belong to some category (see RiC-CM
               0.2 attributes section, #4.4 on Record Set, Record and Record Part
               attributes)."""@en
    ] .

:hasOrHadAllMembersWithMainSubject
    a owl:ObjectProperty ;
    rdfs:comment """Connects a Record Set and a Thing that is the main subject of all
         the Records or Record Parts that are or were included in the Record Set."""@en ;
    rdfs:domain :RecordSet ;
    rdfs:isDefinedBy <https://www.ica.org/standards/RiC/ontology> ;
    rdfs:label "has or had all members with main subject"@en, """inclut ou a inclus des membres ayant tous pour principal
         sujet"""@fr, "incluye o incluía miembros, todos con matería principal"@es ;
    rdfs:range :Thing ;
    rdfs:subPropertyOf :hasOrHadAllMembersWithSubject, :hasOrHadMainSubject ;
    owl:inverseOf :isOrWasMainSubjectOfAllMembersOf ;
    skos:changeNote [
        dc:date "2025-04-05" ;
        rdf:value "Introduced in RiC-O 1.1."@en
    ] .

:hasOrHadAllMembersWithRecordState
    a owl:ObjectProperty ;
    rdfs:comment """Connects a Record Set and a Record State that categorizes all the
         Records or Record Parts that are or were included in the Record Set."""@en ;
    rdfs:domain :RecordSet ;
    rdfs:isDefinedBy <https://www.ica.org/standards/RiC/ontology> ;
    rdfs:label "has or had all members with record state"@en, "inclut ou a inclus des membres ayant tous pour état"@fr, """incluye o incluía miembros, todos con estado de
         documento"""@es ;
    rdfs:range :RecordState ;
    rdfs:subPropertyOf :hasOrHadAllMembersWithType ;
    owl:inverseOf :isOrWasRecordStateOfAllMembersOf ;
    skos:changeNote [
        dc:date "2025-04-06" ;
        rdf:value "Adjusted the Spanish label."@en
    ], [
        dc:date "2023-11-02" ;
        rdf:value "Added a new rdfs:label in Spanish."@en
    ], [
        dc:date "2023-08-28" ;
        rdf:value "Added a new rdfs:label in French."@en
    ], [
        dc:date "2020-12-28" ;
        rdf:value """Object property added for handling the case where a Record Set
               is described as having all or some members that belong to some category (see RiC-CM
               0.2 attributes section, #4.4 on Record Set, Record and Record Part
               attributes)."""@en
    ] .

:hasOrHadAllMembersWithSubject
    a owl:ObjectProperty ;
    rdfs:comment """Connects a Record Set and a Thing that is the subject of all the
         Records or Record Parts that are or were included in the Record Set."""@en ;
    rdfs:domain :RecordSet ;
    rdfs:isDefinedBy <https://www.ica.org/standards/RiC/ontology> ;
    rdfs:label "has or had all members with subject"@en, "inclut ou a inclus des membres ayant tous pour sujet"@fr, "incluye o incluía miembros, todos con matería"@es ;
    rdfs:range :Thing ;
    rdfs:subPropertyOf :hasOrHadSubject ;
    owl:inverseOf :isOrWasSubjectOfAllMembersOf ;
    skos:changeNote [
        dc:date "2025-04-05" ;
        rdf:value "Introduced in RiC-O 1.1."@en
    ] .

:hasOrHadAllMembersWithType
    a owl:ObjectProperty ;
    rdfs:comment """Connects a Record Set and a Type to which all the Records or
         Record Parts that are or were included in the Record Set belong."""@en ;
    rdfs:domain :RecordSet ;
    rdfs:isDefinedBy <https://www.ica.org/standards/RiC/ontology> ;
    rdfs:label "has or had all members with type"@en, "inclut ou a inclus des membres ayant tous pour type"@fr, "incluye o incluía miembros, todos con tipo"@es ;
    rdfs:range :Type ;
    rdfs:subPropertyOf :isRelatedTo ;
    owl:inverseOf :isOrWasTypeOfAllMembersOf ;
    skos:changeNote [
        dc:date "2025-04-06" ;
        rdf:value "Adjusted the Spanish label."@en
    ], [
        dc:date "2024-10-04" ;
        rdf:value """Changed the word 'category' into 'type' in all applicable
               properties names."""@en
    ], [
        dc:date "2023-11-02" ;
        rdf:value "Added a new rdfs:label in Spanish."@en
    ], [
        dc:date "2023-08-28" ;
        rdf:value "Added a new rdfs:label in French."@en
    ], [
        dc:date "2020-12-28" ;
        rdf:value """Object property added for handling the case where a Record Set
               is described as having all or some members that belong to some category (see RiC-CM
               0.2 attributes section, #4.4 on Record Set, Record and Record Part
               attributes)."""@en
    ] .

:hasOrHadAnalogueInstantiation
    a owl:ObjectProperty ;
    rdfs:comment """Connects a record resource to one of its analogue instantiations,
         whether it exists or has been lost or destroyed."""@en ;
    rdfs:domain :RecordResource ;
    rdfs:isDefinedBy <https://www.ica.org/standards/RiC/ontology> ;
    rdfs:label "a ou a eu pour instanciation analogique"@fr, "has or had analogue instantiation"@en, "tiene o tenía como instanciación analogica"@es ;
    rdfs:range :Instantiation ;
    rdfs:subPropertyOf :hasOrHadInstantiation ;
    owl:inverseOf :isOrWasAnalogueInstantiationOf ;
    skos:changeNote [
        dc:date "2023-11-27" ;
        rdf:value "Added a new rdfs:label in Spanish."@en
    ], [
        dc:date "2023-08-29" ;
        rdf:value "Added the property."@en
    ] ;
    skos:scopeNote """In some situations, it may be useful or necessary to connect a
         record resource to an analogue instantiation that no longer exists or has been
         lost."""@en .

:hasOrHadAppellation
    a owl:ObjectProperty ;
    rdfs:comment """Connects a Thing to an Appellation that is or was used for
         designating it."""@en ;
    rdfs:domain :Thing ;
    rdfs:isDefinedBy <https://www.ica.org/standards/RiC/ontology> ;
    rdfs:label "a ou a eu pour appellation"@fr, "has or had appellation"@en, "tiene o tenía como denominación"@es ;
    rdfs:range :Appellation ;
    rdfs:subPropertyOf :isRelatedTo ;
    owl:inverseOf :isOrWasAppellationOf ;
    owl:propertyChainAxiom (:thingIsTargetOfRelation
        :appellationRelation_role
        :relationHasSource
    ) ;
    skos:changeNote [
        dc:date "2023-11-08" ;
        rdf:value """In order to get a system of rolified Relation classes: modified
               the property chain axiom so that it now involves the new appellationRelation_role
               object property."""@en
    ], [
        dc:date "2023-11-02" ;
        rdf:value "Added a new rdfs:label in Spanish."@en
    ], [
        dc:date "2023-08-28" ;
        rdf:value "Added a new rdfs:label in French."@en
    ], [
        dc:date "2021-01-22" ;
        rdf:value """changed the IRI, label, inverse property IRI, textual
               definition (the name of this property in RiC-O 0.1 was \"hasAppellation\")."""@en
    ] .

:hasOrHadAuthorityOver
    a owl:ObjectProperty ;
    rdfs:comment """Connects an Agent to a Thing over which the Agent has or had some
         kind of authority."""@en ;
    rdfs:domain :Agent ;
    rdfs:isDefinedBy <https://www.ica.org/standards/RiC/ontology> ;
    rdfs:label "a ou a eu autorité sur"@fr, "has or had authority over"@en, "tiene o tenía control sobre"@es ;
    rdfs:range :Thing ;
    rdfs:subPropertyOf :isRelatedTo ;
    owl:inverseOf :isOrWasUnderAuthorityOf ;
    owl:propertyChainAxiom (:thingIsSourceOfRelation
        :authorityRelation_role
        :relationHasTarget
    ) ;
    skos:changeNote [
        dc:date "2023-11-12" ;
        rdf:value """Aligned with RiC-CM 1.0: updated the description
               (rdfs:comment), skos:scopeNote."""@en
    ], [
        dc:date "2023-11-08" ;
        rdf:value """In order to get a system of rolified Relation classes: modified
               the property chain axiom so that it now involves the new authorityRelation_role
               object property."""@en
    ], [
        dc:date "2023-11-02" ;
        rdf:value "Added a new rdfs:label in Spanish."@en
    ], [
        dc:date "2023-08-28" ;
        rdf:value "Added a new rdfs:label in French."@en
    ], [
        dc:date "2021-01-22" ;
        rdf:value """changed the IRI, label, inverse property IRI, textual
               definition (changed made in order to make RiC-O compliant with RiC-CM 0.2; the name
               of this property in RiC-O 0.1 was \"hasAuthorityOver\")."""@en
    ] ;
    skos:scopeNote """Use only if it is not possible to specify a narrower authority
         relation, for example is or was owner of."""@en ;
    :RiCCMCorrespondingComponent """RiC-R036 ('has or had authority over'
         relation)"""@en .

:hasOrHadComponent
    a owl:ObjectProperty ;
    rdfs:comment """Connects an Instantiation to one of its present or past component
         instantiations."""@en ;
    rdfs:domain :Instantiation ;
    rdfs:isDefinedBy <https://www.ica.org/standards/RiC/ontology> ;
    rdfs:label "a ou a eu pour composant"@fr, "has or had component"@en, "tiene o tenía como componente"@es ;
    rdfs:range :Instantiation ;
    rdfs:subPropertyOf :hasOrHadPart, :isInstantiationAssociatedWithInstantiation ;
    owl:inverseOf :isOrWasComponentOf ;
    skos:changeNote [
        dc:date "2023-11-02" ;
        rdf:value "Added a new rdfs:label in Spanish."@en
    ], [
        dc:date "2023-08-28" ;
        rdf:value "Added a new rdfs:label in French."@en
    ], [
        dc:date "2021-01-22" ;
        rdf:value """changed the IRI, label, inverse property IRI, textual
               definition (changed made in order to make RiC-O compliant with RiC-CM 0.2; the name
               of this property in RiC-O 0.1 was \"hasComponent\")."""@en
    ] ;
    :RiCCMCorrespondingComponent """RiC-R004 ('has or had component'
         relation)"""@en .

:hasOrHadConstituent
    a owl:ObjectProperty ;
    rdfs:comment """Connects a Record or Record Part to a Record or Record part that
         is or was a constituent of that Record or Record Part."""@en ;
    rdfs:domain [
        a owl:Class ;
        owl:unionOf (:Record
            :RecordPart
        )
    ] ;
    rdfs:isDefinedBy <https://www.ica.org/standards/RiC/ontology> ;
    rdfs:label "a ou a eu pour constituant"@fr, "has or had constituent"@en, "tiene o tenía como elemento constitutivo"@es ;
    rdfs:range [
        a owl:Class ;
        owl:unionOf (:Record
            :RecordPart
        )
    ] ;
    rdfs:subPropertyOf :hasOrHadPart, :isRecordResourceAssociatedWithRecordResource ;
    owl:inverseOf :isOrWasConstituentOf ;
    skos:changeNote [
        dc:date "2023-11-12" ;
        rdf:value """Aligned with RiC-CM 1.0: updated the description
               (rdfs:comment)."""@en
    ], [
        dc:date "2023-11-02" ;
        rdf:value "Added a new rdfs:label in Spanish."@en
    ], [
        dc:date "2023-10-19" ;
        rdf:value "Added Record Part to the domain."@en
    ], [
        dc:date "2023-08-28" ;
        rdf:value "Added a new rdfs:label in French."@en
    ], [
        dc:date "2021-01-22" ;
        rdf:value """changed the IRI, label, inverse property IRI, textual
               definition (changed made in order to make RiC-O compliant with RiC-CM 0.2; the name
               of this property in RiC-O 0.1 was \"hasConstituent\")."""@en
    ] ;
    :RiCCMCorrespondingComponent """RiC-R003 ('has or had constituent'
         relation)"""@en .

:hasOrHadController
    a owl:ObjectProperty ;
    rdfs:comment """Inverse of 'is or was controller of' object
         property."""@en ;
    rdfs:domain :Agent ;
    rdfs:isDefinedBy <https://www.ica.org/standards/RiC/ontology> ;
    rdfs:label "est ou a été contrôlé par"@fr, "has or had controller"@en, "tiene o tenía como controlador"@es ;
    rdfs:range :Agent ;
    rdfs:subPropertyOf :isOrWasSubordinateTo, :isOrWasUnderAuthorityOf ;
    owl:inverseOf :isOrWasControllerOf ;
    owl:propertyChainAxiom (:thingIsTargetOfRelation
        :agentControlRelation_role
        :relationHasSource
    ) ;
    skos:changeNote [
        dc:date "2024-09-02" ;
        rdf:value "Fixed the French label."@en
    ], [
        dc:date "2023-11-08" ;
        rdf:value """In order to get a system of rolified Relation classes: modified
               the property chain axiom so that it now involves the new agentControlRelation_role
               object property."""@en
    ], [
        dc:date "2023-11-02" ;
        rdf:value "Added a new rdfs:label in Spanish."@en
    ], [
        dc:date "2023-08-28" ;
        rdf:value "Added a new rdfs:label in French."@en
    ], [
        dc:date "2021-01-22" ;
        rdf:value """changed the IRI, label, inverse property IRI, text definition,
               corresponding CM component name (changed made in order to make RiC-O compliant with
               RiC-CM 0.2; the name of this property in RiC-O 0.1 was \"controlledBy\")."""@en
    ] ;
    :RiCCMCorrespondingComponent """RiC-R041i ('has or had controller'
         relation)"""@en .

:hasOrHadCoordinates
    a owl:ObjectProperty ;
    rdfs:comment """Connects a Physical Location to its past or present coordinates in
         a reference system."""@en ;
    rdfs:domain :PhysicalLocation ;
    rdfs:isDefinedBy <https://www.ica.org/standards/RiC/ontology> ;
    rdfs:label "a ou a eu pour coordonnées"@fr, "has or had coordinates"@en, "tiene como coordenadas de lugar"@es ;
    rdfs:range :Coordinates ;
    rdfs:subPropertyOf :isRelatedTo ;
    owl:inverseOf :isOrWasCoordinatesOf ;
    skos:changeNote [
        dc:date "2023-11-02" ;
        rdf:value "Added a new rdfs:label in Spanish."@en
    ], [
        dc:date "2023-08-29" ;
        rdf:value "fixed the English label (added the past tense.)"@en
    ], [
        dc:date "2023-08-28" ;
        rdf:value "Added a new rdfs:label in French."@en
    ], [
        dc:date "2021-01-22" ;
        rdf:value """changed the IRI, label, inverse property IRI, textual
               definition (the name of this property in RiC-O 0.1 was \"hasCoordinates\")."""@en
    ] .

:hasOrHadCorporateBodyType
    a owl:ObjectProperty ;
    rdfs:comment """Connects a Corporate Body to a Corporate Body Type which
         categorizes or categorized it."""@en ;
    rdfs:domain :CorporateBody ;
    rdfs:isDefinedBy <https://www.ica.org/standards/RiC/ontology> ;
    rdfs:label "a ou a eu pour type de collectivité"@fr, "has or had corporate body type"@en, "tiene o tenía como tipo de institucion"@es ;
    rdfs:range :CorporateBodyType ;
    rdfs:subPropertyOf :hasOrHadType ;
    owl:inverseOf :isOrWasCorporateBodyTypeOf ;
    skos:changeNote [
        dc:date "2023-11-02" ;
        rdf:value "Added a new rdfs:label in Spanish."@en
    ], [
        dc:date "2023-08-28" ;
        rdf:value "Added a new rdfs:label in French."@en
    ], [
        dc:date "2021-01-22" ;
        rdf:value """changed the IRI, label, inverse property IRI, textual
               definition (the name of this property in RiC-O 0.1 was
               \"hasCorporateBodyType\")."""@en
    ] .

:hasOrHadCorrespondent
    a owl:ObjectProperty, owl:SymmetricProperty ;
    rdfs:comment """Connects two Persons that correspond or have corresponded with
         each other. This relation is symmetric."""@en ;
    rdfs:domain :Person ;
    rdfs:isDefinedBy <https://www.ica.org/standards/RiC/ontology> ;
    rdfs:label "a ou a eu pour correspondant"@fr, "has or had correspondent"@en, "tiene o tenía como correspondiente"@es ;
    rdfs:range :Person ;
    rdfs:subPropertyOf :knows ;
    owl:propertyChainAxiom (:thingIsConnectedToRelation
        :correspondenceRelation_role
        :relationConnects
    ) ;
    skos:changeNote [
        dc:date "2023-11-08" ;
        rdf:value """In order to get a system of rolified Relation classes: modified
               the property chain axiom so that it now involves the new correspondenceRelation_role
               object property."""@en
    ], [
        dc:date "2023-11-02" ;
        rdf:value "Added a new rdfs:label in Spanish."@en
    ], [
        dc:date "2023-08-28" ;
        rdf:value "Added a new rdfs:label in French."@en
    ], [
        dc:date "2021-01-22" ;
        rdf:value """changed the IRI, label, textual definition (changed made in
               order to make RiC-O compliant with RiC-CM 0.2; the name of this property in RiC-O 0.1
               was \"hasCorrespondent\")."""@en
    ] ;
    :RiCCMCorrespondingComponent """RiC-R052 ('has or had correspondent'
         relation)"""@en .

:hasOrHadDemographicGroup
    a owl:ObjectProperty ;
    rdfs:comment """Connects a Person or a Group to a Demographic Group to which it
         belongs or belonged."""@en ;
    rdfs:domain [
        a owl:Class ;
        owl:unionOf (:Group
            :Person
        )
    ] ;
    rdfs:isDefinedBy <https://www.ica.org/standards/RiC/ontology> ;
    rdfs:label "a ou a eu pour groupe démographique"@fr, "has or had demographic group"@en, "tiene o tenía como grupo demográfico"@es ;
    rdfs:range :DemographicGroup ;
    rdfs:subPropertyOf :hasOrHadType ;
    owl:inverseOf :isOrWasDemographicGroupOf ;
    skos:changeNote [
        dc:date "2024-10-10" ;
        rdf:value """Changed the French and Spanish labels (replaced 'catégorie' and
               'categoria' with 'groupe' and 'grupo')."""@en
    ], [
        dc:date "2023-11-02" ;
        rdf:value "Added a new rdfs:label in Spanish."@en
    ], [
        dc:date "2023-08-28" ;
        rdf:value "Added a new rdfs:label in French."@en
    ], [
        dc:date "2021-01-22" ;
        rdf:value """changed the IRI, label, inverse property IRI, text definition,
               domain (the name of this property in RiC-O 0.1 was
               \"belongsToDemographicGroup\")."""@en
    ] .

:hasOrHadDerivedInstantiation
    a owl:ObjectProperty ;
    rdfs:comment """Connects an instantiation to an instantiation that is derived from
         it, whether it exists or has been lost or destroyed."""@en ;
    rdfs:domain :Instantiation ;
    rdfs:isDefinedBy <https://www.ica.org/standards/RiC/ontology> ;
    rdfs:label "a ou a eu pour instanciation dérivée"@fr, "has or had derived instantiation"@en, "tiene o tenía como instanciación derivada"@es ;
    rdfs:range :Instantiation ;
    rdfs:subPropertyOf :isInstantiationAssociatedWithInstantiation, :precedesInTime ;
    owl:inverseOf :isOrWasDerivedFromInstantiation ;
    owl:propertyChainAxiom (:thingIsSourceOfRelation
        :derivationRelation_role
        :relationHasTarget
    ) ;
    skos:changeNote [
        dc:date "2023-11-27" ;
        rdf:value "Added a new rdfs:label in Spanish."@en
    ], [
        dc:date "2023-11-08" ;
        rdf:value """In order to get a system of rolified Relation classes: modified
               the property chain axiom so that it now involves the new derivationRelation_role
               object property."""@en
    ], [
        dc:date "2023-08-29" ;
        rdf:value """Updated the IRI, inverse property, definition, labels and
               RiCMCorrespondingComponent, and added a skos:scopeNote; this in order to make the
               specification compliant with RiC-CM 1.0. The name of the property in RiC-O 0.2 was
               'has derived instantiation'."""@en
    ], [
        dc:date "2023-08-28" ;
        rdf:value "Added a new rdfs:label in French."@en
    ] ;
    skos:scopeNote """In some situations, it may be useful or necessary to connect an
         instantiation to an instantiation that was derived from it but no longer exists or or has
         been lost."""@en ;
    :RiCCMCorrespondingComponent """RiC-R014 ('has or had derived instantiation'
         relation)"""@en .

:hasOrHadDigitalInstantiation
    a owl:ObjectProperty ;
    rdfs:comment """Connects a record resource to one of its digital instantiations,
         whether it exists or has been lost or destroyed."""@en ;
    rdfs:domain :RecordResource ;
    rdfs:isDefinedBy <https://www.ica.org/standards/RiC/ontology> ;
    rdfs:label "a ou a eu pour instanciation numérique"@fr, "has or had digital instantiation"@en, "tiene o tenía como instanciación digital"@es ;
    rdfs:range :Instantiation ;
    rdfs:subPropertyOf :hasOrHadInstantiation ;
    owl:inverseOf :isOrWasDigitalInstantiationOf ;
    skos:changeNote [
        dc:date "2023-11-27" ;
        rdf:value "Added a new rdfs:label in Spanish."@en
    ], [
        dc:date "2023-08-29" ;
        rdf:value "Added the property."@en
    ] ;
    skos:scopeNote """This property can be used, among other cases, when you want to
         convert findings aids encoded in EAD/XML and need a simple and accurate migration path to
         process dao or daogrp EAD elements. Also, in some situations, it may be useful or necessary
         to connect a record resource to a digital instantiation that no longer exists or or has
         been lost."""@en .

:hasOrHadEmployer
    a owl:ObjectProperty ;
    rdfs:comment "Inverse of 'is or was employer of' object property."@en ;
    rdfs:domain :Person ;
    rdfs:isDefinedBy <https://www.ica.org/standards/RiC/ontology> ;
    rdfs:label "a ou a eu pour employeur"@fr, "has or had employer"@en, "tiene o tenía como empleador"@es ;
    rdfs:range [
        a owl:Class ;
        owl:unionOf (:CorporateBody
            :Person
        )
    ] ;
    rdfs:subPropertyOf :hasOrHadController ;
    owl:inverseOf :isOrWasEmployerOf ;
    skos:changeNote [
        dc:date "2023-11-27" ;
        rdf:value "Added a new rdfs:label in Spanish."@en
    ], [
        dc:date "2023-10-26" ;
        rdf:value """Changed the domain and range of the property. Added a
               rdfs:comment. Removed the isOrWasMemberOf super-property."""@en
    ], [
        dc:date "2023-10-19" ;
        rdf:value "Added for RiC-O 1.0."@en
    ], [
        dc:date "2023-10-13" ;
        rdf:value "Fixed the lang of the French label."@en
    ] .

:hasOrHadHolder
    a owl:ObjectProperty ;
    rdfs:comment "Inverse of 'is or was holder of' object property."@en ;
    rdfs:domain [
        a owl:Class ;
        owl:unionOf (:Instantiation
            :RecordResource
        )
    ] ;
    rdfs:isDefinedBy <https://www.ica.org/standards/RiC/ontology> ;
    rdfs:label "est ou a été détenu par"@fr, "has or had holder"@en, "tiene o tenía como conservador a"@es ;
    rdfs:range :Agent ;
    rdfs:subPropertyOf :hasOrHadManager ;
    owl:inverseOf :isOrWasHolderOf ;
    owl:propertyChainAxiom (:thingIsTargetOfRelation
        :recordResourceHoldingRelation_role
        :relationHasSource
    ) ;
    skos:changeNote [
        dc:date "2023-11-08" ;
        rdf:value """In order to get a system of rolified Relation classes: modified
               the property chain axiom so that it now involves the new
               recordResourceHoldingRelation_role object property."""@en
    ], [
        dc:date "2023-11-02" ;
        rdf:value "Added a new rdfs:label in Spanish."@en
    ], [
        dc:date "2023-08-28" ;
        rdf:value "Added a new rdfs:label in French."@en
    ], [
        dc:date "2021-01-22" ;
        rdf:value """changed the IRI, label, inverse property IRI, text definition,
               super property IRI (changed made in order to make RiC-O compliant with RiC-CM 0.2;
               the name of this property in RiC-O 0.1 was \"heldBy\")."""@en
    ] ;
    :RiCCMCorrespondingComponent """RiC-R039i ('has or had holder'
         relation)"""@en .

:hasOrHadIdentifier
    a owl:ObjectProperty ;
    rdfs:comment """Connects a Thing to one of its past or present
         Identifiers."""@en ;
    rdfs:domain :Thing ;
    rdfs:isDefinedBy <https://www.ica.org/standards/RiC/ontology> ;
    rdfs:label "a ou a eu pour identifiant"@fr, "has or had identifier"@en, "tiene o tenía como identificador"@es ;
    rdfs:range :Identifier ;
    rdfs:subPropertyOf :hasOrHadAppellation ;
    owl:inverseOf :isOrWasIdentifierOf ;
    skos:changeNote [
        dc:date "2023-11-02" ;
        rdf:value "Added a new rdfs:label in Spanish."@en
    ], [
        dc:date "2023-08-28" ;
        rdf:value "Added a new rdfs:label in French."@en
    ], [
        dc:date "2021-01-22" ;
        rdf:value """changed the IRI, label, inverse property IRI, text definition,
               super property IRI (the name of this property in RiC-O 0.1 was
               \"identifiedBy\")."""@en
    ] .

:hasOrHadInstantiation
    a owl:ObjectProperty ;
    rdfs:comment """Connects a Record Resource to an Instantiation, which either may
         exist or may have been lost or destroyed."""@en ;
    rdfs:domain :RecordResource ;
    rdfs:isDefinedBy <https://www.ica.org/standards/RiC/ontology> ;
    rdfs:label "a ou a eu pour instanciation"@fr, "has or had instantiation"@en, "tiene o tenía como instanciación"@es ;
    rdfs:range :Instantiation ;
    rdfs:subPropertyOf :isRelatedTo ;
    owl:inverseOf :isOrWasInstantiationOf ;
    owl:propertyChainAxiom (:thingIsSourceOfRelation
        :recordResourceToInstantiationRelation_role
        :relationHasTarget
    ) ;
    skos:changeNote [
        dc:date "2023-11-27" ;
        rdf:value "Added a new rdfs:label in Spanish."@en
    ], [
        dc:date "2023-11-12" ;
        rdf:value """Aligned with RiC-CM 1.0: updated the description
               (rdfs:comment)."""@en
    ], [
        dc:date "2023-11-08" ;
        rdf:value """In order to get a system of rolified Relation classes: modified
               the property chain axiom so that it now involves the new
               recordResourceToInstantiationRelation_role object property."""@en
    ], [
        dc:date "2023-08-29" ;
        rdf:value """Updated the IRI, inverse property, definition, labels and
               RiCMCorrespondingComponent, and added a skos:scopeNote; this in order to make the
               specification compliant with RiC-CM 1.0. The name of the property in RiC-O 0.2 was
               'has instantiation'."""@en
    ], [
        dc:date "2023-08-28" ;
        rdf:value "Added a new rdfs:label in French."@en
    ], [
        dc:date "2021-01-22" ;
        rdf:value "changed the inverse property IRI."@en
    ] ;
    skos:scopeNote """In some situations, it may be useful or necessary to connect a
         record resource to an instantiation that no longer exists or or has been lost, when some of
         its characteristics are known from some source, like an old finding aid."""@en ;
    :RiCCMCorrespondingComponent """RiC-R025 ('has or had instantiation'
         relation)"""@en .

:hasOrHadIntellectualPropertyRightsHolder
    a owl:ObjectProperty ;
    rdfs:comment """Inverse of 'is or was holder of intellectual property rights of'
         object property."""@en ;
    rdfs:domain [
        a owl:Class ;
        owl:unionOf (:Instantiation
            :RecordResource
        )
    ] ;
    rdfs:isDefinedBy <https://www.ica.org/standards/RiC/ontology> ;
    rdfs:label """a ou a eu comme détenteur des droits de propriété
         intellectuelle"""@fr, "has or had intellectual property rights holder"@en, """tiene o tenía como titular de derechos de propiedad intelectual
         a"""@es ;
    rdfs:range [
        a owl:Class ;
        owl:unionOf (:Group
            :Person
            :Position
        )
    ] ;
    rdfs:subPropertyOf :isOrWasUnderAuthorityOf ;
    owl:inverseOf :isOrWasHolderOfIntellectualPropertyRightsOf ;
    owl:propertyChainAxiom (:thingIsTargetOfRelation
        :intellectualPropertyRightsRelation_role
        :relationHasSource
    ) ;
    skos:changeNote [
        dc:date "2024-09-02" ;
        rdf:value "Fixed the French label."@en
    ], [
        dc:date "2023-11-08" ;
        rdf:value """In order to get a system of rolified Relation classes: modified
               the property chain axiom so that it now involves the new
               intellectualPropertyRightsRelation_role object property."""@en
    ], [
        dc:date "2023-11-02" ;
        rdf:value "Added a new rdfs:label in Spanish."@en
    ], [
        dc:date "2023-08-28" ;
        rdf:value "Added a new rdfs:label in French."@en
    ], [
        dc:date "2021-01-22" ;
        rdf:value """changed the IRI, label, inverse property IRI, textual
               definition (changed made in order to make RiC-O compliant with RiC-CM 0.2; the name
               of this property in RiC-O 0.1 was \"intellectualPropertyRightsHeldBy\")."""@en
    ] ;
    :RiCCMCorrespondingComponent """RiC-R040i ('has or had intellectual property rights
         holder ' relation)"""@en .

:hasOrHadJurisdiction
    a owl:ObjectProperty ;
    rdfs:comment """Inverse of 'is or was jurisdiction of' object
         property."""@en ;
    rdfs:domain :Agent ;
    rdfs:isDefinedBy <https://www.ica.org/standards/RiC/ontology> ;
    rdfs:label "a ou a eu pour ressort"@fr, "has or had jurisdiction"@en, "tiene o tenía como jurisdicción"@es ;
    rdfs:range :Place ;
    rdfs:subPropertyOf :isAgentAssociatedWithPlace ;
    owl:inverseOf :isOrWasJurisdictionOf ;
    skos:changeNote [
        dc:date "2023-11-02" ;
        rdf:value "Added a new rdfs:label in Spanish."@en
    ], [
        dc:date "2023-10-19" ;
        rdf:value """Made subproperty of new property isAgentAssociatedWithPlace
               instead of its parent isAssociatedWithPlace."""@en
    ], [
        dc:date "2023-08-28" ;
        rdf:value "Added a new rdfs:label in French."@en
    ], [
        dc:date "2021-01-22" ;
        rdf:value """changed the IRI, label, inverse property IRI and textual
               definition (changed made in order to make RiC-O compliant with RiC-CM 0.2; the name
               of this property in RiC-O 0.1 was \"hasJurisdiction\")."""@en
    ] ;
    :RiCCMCorrespondingComponent """RiC-R076i ('has or had jurisdiction'
         relation)"""@en .

:hasOrHadLanguage
    a owl:ObjectProperty ;
    rdfs:comment """Connects an Agent, Record or Record Part to a Language that uses
         or used it."""@en ;
    rdfs:domain [
        a owl:Class ;
        owl:unionOf (:Agent
            :Record
            :RecordPart
        )
    ] ;
    rdfs:isDefinedBy <https://www.ica.org/standards/RiC/ontology> ;
    rdfs:label "a ou a eu pour langue"@fr, "has or had language"@en, "tiene o tenía como lengua"@es ;
    rdfs:range :Language ;
    rdfs:subPropertyOf :isRelatedTo ;
    owl:inverseOf :isOrWasLanguageOf ;
    skos:changeNote [
        dc:date "2023-11-02" ;
        rdf:value "Added a new rdfs:label in Spanish."@en
    ], [
        dc:date "2023-08-28" ;
        rdf:value "Added a new rdfs:label in French."@en
    ], [
        dc:date "2023-07-25" ;
        rdf:value """changed the definition to be consistent with the inverse
               relation."""@en
    ], [
        dc:date "2021-01-22" ;
        rdf:value """changed the IRI, label, inverse property IRI and textual
               definition (the name of this property in RiC-O 0.1 was \"hasLanguage\")."""@en
    ] .

:hasOrHadLeader
    a owl:ObjectProperty ;
    rdfs:comment "Inverse of 'is or was leader of' object property."@en ;
    rdfs:domain :Group ;
    rdfs:isDefinedBy <https://www.ica.org/standards/RiC/ontology> ;
    rdfs:label "a ou a eu pour dirigeant"@fr, "has or had leader"@en, "tiene o tenía como líder a"@es ;
    rdfs:range :Person ;
    rdfs:subPropertyOf :hasOrHadController ;
    owl:inverseOf :isOrWasLeaderOf ;
    owl:propertyChainAxiom (:thingIsTargetOfRelation
        :leadershipRelation_role
        :relationHasSource
    ) ;
    skos:changeNote [
        dc:date "2023-11-08" ;
        rdf:value """In order to get a system of rolified Relation classes: modified
               the property chain axiom so that it now involves the new leadershipRelation_role
               object property."""@en
    ], [
        dc:date "2023-11-02" ;
        rdf:value "Added a new rdfs:label in Spanish."@en
    ], [
        dc:date "2023-08-28" ;
        rdf:value "Added a new rdfs:label in French."@en
    ], [
        dc:date "2021-01-22" ;
        rdf:value """changed the IRI, label, inverse property IRI, text definition,
               super property IRI (changed made in order to make RiC-O compliant with RiC-CM 0.2;
               the name of this property in RiC-O 0.1 was \"ledBy\")."""@en
    ] ;
    :RiCCMCorrespondingComponent """RiC-R042i ('has or had leader'
         relation)"""@en .

:hasOrHadLegalStatus
    a owl:ObjectProperty ;
    rdfs:comment """Connects an Agent or Record Resource to a Legal Status which
         categorized or categorizes it."""@en ;
    rdfs:domain [
        a owl:Class ;
        owl:unionOf (:Agent
            :Record
            :RecordPart
        )
    ] ;
    rdfs:isDefinedBy <https://www.ica.org/standards/RiC/ontology> ;
    rdfs:label "a ou a eu pour statut légal"@fr, "has or had legal status"@en, "tiene o tenía como status jurídico"@es ;
    rdfs:range :LegalStatus ;
    rdfs:subPropertyOf :hasOrHadType ;
    owl:inverseOf :isOrWasLegalStatusOf ;
    skos:changeNote [
        dc:date "2023-11-02" ;
        rdf:value "Added a new rdfs:label in Spanish."@en
    ], [
        dc:date "2023-08-28" ;
        rdf:value "Added a new rdfs:label in French."@en
    ], [
        dc:date "2021-01-22" ;
        rdf:value """changed the IRI, label, inverse property IRI and textual
               definition (the name of this property in RiC-O 0.1 was \"hasLegalStatus\")."""@en
    ] .

:hasOrHadLocation
    a owl:ObjectProperty ;
    rdfs:comment "Inverse of 'is or was location of' object property."@en ;
    rdfs:domain :Thing ;
    rdfs:isDefinedBy <https://www.ica.org/standards/RiC/ontology> ;
    rdfs:label "a ou a eu pour localisation"@fr, "has or had location"@en, "tiene o tenía como localización"@es ;
    rdfs:range :Place ;
    rdfs:subPropertyOf :isAssociatedWithPlace ;
    owl:inverseOf :isOrWasLocationOf ;
    skos:changeNote [
        dc:date "2023-11-02" ;
        rdf:value "Added a new rdfs:label in Spanish."@en
    ], [
        dc:date "2023-08-28" ;
        rdf:value "Added a new rdfs:label in French."@en
    ], [
        dc:date "2021-01-22" ;
        rdf:value """changed the IRI, label, inverse property IRI and textual
               definition (changed made in order to make RiC-O compliant with RiC-CM 0.2; the name
               of this property in RiC-O 0.1 was \"hasLocation\")."""@en
    ] ;
    :RiCCMCorrespondingComponent """RiC-R075i ('has or had location'
         relation)"""@en .

:hasOrHadMainSubject
    a owl:ObjectProperty ;
    rdfs:comment """Connects a Record Resource to a Thing that is or was its main
         subject."""@en ;
    rdfs:domain :RecordResource ;
    rdfs:isDefinedBy <https://www.ica.org/standards/RiC/ontology> ;
    rdfs:label "a ou a eu pour sujet principal"@fr, "has or had main subject"@en, "tiene o tenía como matería principal"@es ;
    rdfs:range :Thing ;
    rdfs:subPropertyOf :hasOrHadSubject ;
    owl:inverseOf :isOrWasMainSubjectOf ;
    skos:changeNote [
        dc:date "2023-11-02" ;
        rdf:value "Added a new rdfs:label in Spanish."@en
    ], [
        dc:date "2023-08-28" ;
        rdf:value "Added a new rdfs:label in French."@en
    ], [
        dc:date "2021-01-22" ;
        rdf:value """changed the IRI, label, inverse property IRI and textual
               definition (changed made in order to make RiC-O compliant with RiC-CM 0.2; the name
               of this property in RiC-O 0.1 was \"hasMainSubject\")."""@en
    ] ;
    skos:scopeNote """Use for specifying, for example, that a Record Set of type
         personal file has main subject some person, which would help end users to retrieve the main
         archival resources about this person."""@en ;
    :RiCCMCorrespondingComponent """RiC-R020 ('has or had main subject'
         relation)"""@en .

:hasOrHadManager
    a owl:ObjectProperty ;
    rdfs:comment "Inverse of 'is or was manager of' object property."@en ;
    rdfs:domain [
        a owl:Class ;
        owl:unionOf (:Instantiation
            :RecordResource
        )
    ] ;
    rdfs:isDefinedBy <https://www.ica.org/standards/RiC/ontology> ;
    rdfs:label "a ou a eu pour gestionnaire"@fr, "has or had manager"@en, "tiene o tenía como gestor a"@es ;
    rdfs:range :Agent ;
    rdfs:subPropertyOf :isOrWasUnderAuthorityOf ;
    owl:inverseOf :isOrWasManagerOf ;
    owl:propertyChainAxiom (:thingIsTargetOfRelation
        :managementRelation_role
        :relationHasSource
    ) ;
    skos:changeNote [
        dc:date "2023-11-08" ;
        rdf:value """In order to get a system of rolified Relation classes: modified
               the property chain axiom so that it now involves the new managementRelation_role
               object property."""@en
    ], [
        dc:date "2023-11-02" ;
        rdf:value "Added a new rdfs:label in Spanish."@en
    ], [
        dc:date "2023-08-28" ;
        rdf:value "Added a new rdfs:label in French."@en
    ], [
        dc:date "2021-01-22" ;
        rdf:value """changed the IRI, label, inverse property IRI, text definition,
               super property IRI (changed made in order to make RiC-O compliant with RiC-CM 0.2;
               the name of this property in RiC-O 0.1 was \"managedBy\")."""@en
    ] ;
    :RiCCMCorrespondingComponent """RiC-R038i ('is or was managed by'
         relation)"""@en .

:hasOrHadMandateType
    a owl:ObjectProperty ;
    rdfs:comment """Connects a Mandate to a Mandate Type that categorized or
         categorizes it."""@en ;
    rdfs:domain :Mandate ;
    rdfs:isDefinedBy <https://www.ica.org/standards/RiC/ontology> ;
    rdfs:label "a ou a eu pour type de mandat"@fr, "has or had mandate type"@en, "tiene o tenía como tipo de norma"@es ;
    rdfs:range :MandateType ;
    rdfs:subPropertyOf :hasOrHadRuleType ;
    owl:inverseOf :isOrWasMandateTypeOf ;
    skos:changeNote [
        dc:date "2023-11-13" ;
        rdf:value """Added the property, and its inverse one, following the creation
               of the MandateType class, that corresponds to the new Mandate Type attribute in
               RiC-CM 1.0."""@en
    ] .

:hasOrHadMember
    a owl:ObjectProperty ;
    rdfs:comment """Connects a Group to a Person that is or was a member of that
         Group."""@en ;
    rdfs:domain :Group ;
    rdfs:isDefinedBy <https://www.ica.org/standards/RiC/ontology> ;
    rdfs:label "a ou a eu pour membre"@fr, "has or had member"@en, "tiene o tenía como miembro a"@es ;
    rdfs:range :Person ;
    rdfs:subPropertyOf :isAgentAssociatedWithAgent ;
    owl:inverseOf :isOrWasMemberOf ;
    owl:propertyChainAxiom (:thingIsSourceOfRelation
        :membershipRelation_role
        :relationHasTarget
    ) ;
    skos:changeNote [
        dc:date "2023-11-08" ;
        rdf:value """In order to get a system of rolified Relation classes: modified
               the property chain axiom so that it now involves the new membershipRelation_role
               object property."""@en
    ], [
        dc:date "2023-11-02" ;
        rdf:value "Added a new rdfs:label in Spanish."@en
    ], [
        dc:date "2023-08-28" ;
        rdf:value "Added a new rdfs:label in French."@en
    ], [
        dc:date "2021-01-22" ;
        rdf:value """changed the IRI, label, inverse property IRI and textual
               definition (changed made in order to make RiC-O compliant with RiC-CM 0.2; the name
               of this property in RiC-O 0.1 was \"hasMember\")."""@en
    ] ;
    :RiCCMCorrespondingComponent """RiC-R055 ('has or had member'
         relation)"""@en .

:hasOrHadMostMembersWithAccumulationDate
    a owl:ObjectProperty ;
    rdfs:comment """Inverse of 'is or was accumulation date of most members of' object
         property."""@en ;
    rdfs:domain :RecordSet ;
    rdfs:isDefinedBy <https://www.ica.org/standards/RiC/ontology> ;
    rdfs:label "has or had most members with accumulation date"@en, """inclut ou a inclus des membres dont la plupart ont pour date
         d'accumulation"""@fr, """incluye o incluía miembros, la mayoría de los cuales con fecha de
         acumulación"""@es ;
    rdfs:range :Date ;
    rdfs:subPropertyOf :hasOrHadSomeMembersWithAccumulationDate ;
    owl:inverseOf :isOrWasAccumulationDateOfMostMembersOf ;
    skos:changeNote [
        dc:date "2025-04-06" ;
        rdf:value "Adjusted the Spanish label."@en
    ], [
        dc:date "2024-10-04" ;
        rdf:value "Added in RiC-O 1.1."@en
    ] .

:hasOrHadMostMembersWithCreationDate
    a owl:ObjectProperty ;
    rdfs:comment """Inverse of 'is or was creation date of most members of' object
         property."""@en ;
    rdfs:domain :RecordSet ;
    rdfs:isDefinedBy <https://www.ica.org/standards/RiC/ontology> ;
    rdfs:label "has or had most members with creation date"@en, """inclut ou a inclus des membres dont la plupart ont pour date de
         création"""@fr, """incluye o incluía miembros, la mayoría de los cuales con fecha de
         creación"""@es ;
    rdfs:range :Date ;
    rdfs:subPropertyOf :hasOrHadSomeMembersWithCreationDate ;
    owl:inverseOf :isOrWasCreationDateOfMostMembersOf ;
    skos:changeNote [
        dc:date "2025-04-06" ;
        rdf:value "Adjusted the Spanish label."@en
    ], [
        dc:date "2023-11-27" ;
        rdf:value "Added a new rdfs:label in Spanish."@en
    ], [
        dc:date "2023-10-13" ;
        rdf:value """Renamed the property in order to take the past members of the
               record set into account. Adjusted the annotations accordingly."""@en
    ], [
        dc:date "2023-10-12" ;
        rdf:value "Added the French label"@en
    ], [
        dc:date "2023-10-10" ;
        rdf:value """Made this property a subproperty of
               hasSomeMembersWithCreationDate."""@en
    ], [
        dc:date "2023-09-22" ;
        rdf:value "Added in RiC-O 1.0."@en
    ] ;
    :RiCCMCorrespondingComponent """RiC-R083i ('has or had most members with creation
         date' relation)"""@en .

:hasOrHadName
    a owl:ObjectProperty ;
    rdfs:comment """Connects a Thing to one of its past or present
         Names."""@en ;
    rdfs:domain :Thing ;
    rdfs:isDefinedBy <https://www.ica.org/standards/RiC/ontology> ;
    rdfs:label "a ou a eu pour nom"@fr, "has or had name"@en, "tiene o tenía como nombre"@es ;
    rdfs:range :Name ;
    rdfs:subPropertyOf :hasOrHadAppellation ;
    owl:inverseOf :isOrWasNameOf ;
    skos:changeNote [
        dc:date "2023-11-02" ;
        rdf:value "Added a new rdfs:label in Spanish."@en
    ], [
        dc:date "2023-08-28" ;
        rdf:value "Added a new rdfs:label in French."@en
    ], [
        dc:date "2021-01-22" ;
        rdf:value """changed the IRI, label, inverse property IRI, textual
               definition, super property IRI (the name of this property in RiC-O 0.1 was
               \"hasName\")."""@en
    ] .

:hasOrHadOccupationOfType
    a owl:ObjectProperty ;
    rdfs:comment """Connects a Person to an Occupation Type that categorized or
         categorizes his/her occupation (profession, trade or craft)."""@en ;
    rdfs:domain :Person ;
    rdfs:isDefinedBy <https://www.ica.org/standards/RiC/ontology> ;
    rdfs:label "a ou a eu pour type d’occupation"@fr, "has or had occupation of type"@en, "tiene o tenía como tipo de ocupación"@es ;
    rdfs:range :OccupationType ;
    rdfs:subPropertyOf :hasOrHadDemographicGroup ;
    owl:inverseOf :isOrWasOccupationTypeOf ;
    skos:changeNote [
        dc:date "2023-11-02" ;
        rdf:value "Added a new rdfs:label in Spanish."@en
    ], [
        dc:date "2023-08-28" ;
        rdf:value "Added a new rdfs:label in French."@en
    ], [
        dc:date "2021-01-22" ;
        rdf:value """changed the IRI, label, inverse property IRI, textual
               definition, super property IRI (the name of this property in RiC-O 0.1 was
               \"hasOccupationOfType\")."""@en
    ] .

:hasOrHadOwner
    a owl:ObjectProperty ;
    rdfs:comment "Inverse of 'is or was owner of' object property."@en ;
    rdfs:domain :Thing ;
    rdfs:isDefinedBy <https://www.ica.org/standards/RiC/ontology> ;
    rdfs:label "a ou a eu pour propriétaire"@fr, "has or had owner"@en, "tiene o tenía como poseedor a"@es ;
    rdfs:range [
        a owl:Class ;
        owl:unionOf (:Group
            :Person
            :Position
        )
    ] ;
    rdfs:subPropertyOf :isOrWasUnderAuthorityOf ;
    owl:inverseOf :isOrWasOwnerOf ;
    owl:propertyChainAxiom (:thingIsTargetOfRelation
        :ownershipRelation_role
        :relationHasSource
    ) ;
    skos:changeNote [
        dc:date "2023-11-08" ;
        rdf:value """In order to get a system of rolified Relation classes: modified
               the property chain axiom so that it now involves the new ownershipRelation_role
               object property."""@en
    ], [
        dc:date "2023-11-02" ;
        rdf:value "Added a new rdfs:label in Spanish."@en
    ], [
        dc:date "2023-08-28" ;
        rdf:value "Added a new rdfs:label in French."@en
    ], [
        dc:date "2021-01-22" ;
        rdf:value """changed the IRI, label, inverse property IRI, text definition,
               super property IRI (changed made in order to make RiC-O compliant with RiC-CM 0.2;
               the name of this property in RiC-O 0.1 was \"ownedBy\")."""@en
    ] ;
    :RiCCMCorrespondingComponent """RiC-R037i ('has or had owner'
         relation)"""@en .

:hasOrHadPart
    a owl:ObjectProperty ;
    rdfs:comment """Connects a Thing to a constitutive or component part of that
         Thing."""@en ;
    rdfs:domain :Thing ;
    rdfs:isDefinedBy <https://www.ica.org/standards/RiC/ontology> ;
    rdfs:label "a ou a eu pour partie"@fr, "has or had part"@en, "tiene o tenía como parte"@es ;
    rdfs:range :Thing ;
    rdfs:subPropertyOf :isRelatedTo ;
    owl:inverseOf :isOrWasPartOf ;
    owl:propertyChainAxiom (:thingIsSourceOfRelation
        :wholePartRelation_role
        :relationHasTarget
    ) ;
    skos:changeNote [
        dc:date "2023-11-12" ;
        rdf:value """Aligned with RiC-CM 1.0: updated the
               skos:scopeNote."""@en
    ], [
        dc:date "2023-11-08" ;
        rdf:value """In order to get a system of rolified Relation classes: modified
               the property chain axiom so that it now involves the new wholePartRelation_role
               object property."""@en
    ], [
        dc:date "2023-11-02" ;
        rdf:value "Added a new rdfs:label in Spanish."@en
    ], [
        dc:date "2023-08-28" ;
        rdf:value "Added a new rdfs:label in French."@en
    ], [
        dc:date "2021-01-22" ;
        rdf:value """changed the IRI, label, inverse property IRI, textual
               definition (changed made in order to make RiC-O compliant with RiC-CM 0.2; the name
               of this property in RiC-O 0.1 was \"hasPart\")."""@en
    ] ;
    skos:scopeNote """Use to connect a Thing to another Thing that is or was a part of
         the whole Thing only if it is not possible to use a narrower, more specific whole/part
         relation, for example has or had constituent. The end of existence of a whole/part relation
         may affect the integrity or nature of the domain entity."""@en ;
    :RiCCMCorrespondingComponent """RiC-R002 ('has or had part'
         relation)"""@en .

:hasOrHadParticipant
    a owl:ObjectProperty ;
    rdfs:comment """Connects an Event to a Thing that is or was actively or passively
         involved in it."""@en ;
    rdfs:domain :Event ;
    rdfs:isDefinedBy <https://www.ica.org/standards/RiC/ontology> ;
    rdfs:label "a ou a eu pour participant"@fr, "has or had participant"@en, "tiene o tenía como participante"@es ;
    rdfs:range :Thing ;
    rdfs:subPropertyOf :isEventAssociatedWith ;
    owl:inverseOf :isOrWasParticipantIn ;
    skos:changeNote [
        dc:date "2023-11-02" ;
        rdf:value "Added a new rdfs:label in Spanish."@en
    ], [
        dc:date "2023-08-28" ;
        rdf:value "Added a new rdfs:label in French."@en
    ], [
        dc:date "2021-01-22" ;
        rdf:value """changed the IRI, label, inverse property IRI, textual
               definition (changed made in order to make RiC-O compliant with RiC-CM 0.2; the name
               of this property in RiC-O 0.1 was \"involves\")."""@en
    ] ;
    :RiCCMCorrespondingComponent """RiC-R058 ('has or had participant'
         relation)"""@en .

:hasOrHadPhysicalLocation
    a owl:ObjectProperty ;
    rdfs:comment """Connects a Place to one of its past or present Physical
         Location."""@en ;
    rdfs:domain :Place ;
    rdfs:isDefinedBy <https://www.ica.org/standards/RiC/ontology> ;
    rdfs:label "a ou a eu pour localisation physique"@fr, "has or had physical location"@en, "tiene o tenía como localización física"@es ;
    rdfs:range :PhysicalLocation ;
    rdfs:subPropertyOf :isPlaceAssociatedWith ;
    owl:inverseOf :isOrWasPhysicalLocationOf ;
    skos:changeNote [
        dc:date "2023-11-02" ;
        rdf:value "Added a new rdfs:label in Spanish."@en
    ], [
        dc:date "2023-08-28" ;
        rdf:value "Added a new rdfs:label in French."@en
    ], [
        dc:date "2021-02-01" ;
        rdf:value """Property made a subproperty of
               'isPlaceAssociatedWith\"."""@en
    ], [
        dc:date "2021-01-22" ;
        rdf:value """changed the IRI, label, inverse property IRI, textual
               definition (the name of this property in RiC-O 0.1 was
               \"hasPhysicalLocation\")."""@en
    ] .

:hasOrHadPlaceName
    a owl:ObjectProperty ;
    rdfs:comment """Connects a Place to one of its past or present
         names."""@en ;
    rdfs:domain :Place ;
    rdfs:isDefinedBy <https://www.ica.org/standards/RiC/ontology> ;
    rdfs:label "a ou a eu pour nom de lieu"@fr, "has or had place name"@en, "tiene o tenía como nombre de lugar"@es ;
    rdfs:range :PlaceName ;
    rdfs:subPropertyOf :hasOrHadName ;
    owl:inverseOf :isOrWasPlaceNameOf ;
    skos:changeNote [
        dc:date "2023-11-02" ;
        rdf:value "Added a new rdfs:label in Spanish."@en
    ], [
        dc:date "2023-08-28" ;
        rdf:value "Added a new rdfs:label in French."@en
    ], [
        dc:date "2021-01-22" ;
        rdf:value """changed the IRI, label, inverse property IRI, text definition,
               super property IRI (the name of this property in RiC-O 0.1 was
               \"hasPlaceName\")."""@en
    ] .

:hasOrHadPlaceType
    a owl:ObjectProperty ;
    rdfs:comment """Connects a Place to a Place Type that categorized or categorizes
         it."""@en ;
    rdfs:domain :Place ;
    rdfs:isDefinedBy <https://www.ica.org/standards/RiC/ontology> ;
    rdfs:label "a ou a eu pour type de lieu"@fr, "has or had place type"@en, "tiene o tenía como tipo de lugar"@es ;
    rdfs:range :PlaceType ;
    rdfs:subPropertyOf :hasOrHadType ;
    owl:inverseOf :isOrWasPlaceTypeOf ;
    skos:changeNote [
        dc:date "2023-11-02" ;
        rdf:value "Added a new rdfs:label in Spanish."@en
    ], [
        dc:date "2023-08-28" ;
        rdf:value "Added a new rdfs:label in French."@en
    ], [
        dc:date "2021-01-22" ;
        rdf:value """changed the IRI, label, inverse property IRI, text definition,
               super property IRI (the name of this property in RiC-O 0.1 was
               \"hasPlaceType\")."""@en
    ] .

:hasOrHadPosition
    a owl:ObjectProperty ;
    rdfs:comment "Inverse of 'exists or existed in' object property."@en ;
    rdfs:domain :Group ;
    rdfs:isDefinedBy <https://www.ica.org/standards/RiC/ontology> ;
    rdfs:label "has or had position"@en, "occupe ou a occupé le poste"@fr, "tiene o tenía como puesto"@es ;
    rdfs:range :Position ;
    rdfs:subPropertyOf :isAgentAssociatedWithAgent ;
    owl:inverseOf :existsOrExistedIn ;
    owl:propertyChainAxiom (:thingIsTargetOfRelation
        :positionToGroupRelation_role
        :relationHasSource
    ) ;
    skos:changeNote [
        dc:date "2023-11-08" ;
        rdf:value """In order to get a system of rolified Relation classes: modified
               the property chain axiom so that it now involves the new positionToGroupRelation_role
               object property."""@en
    ], [
        dc:date "2023-11-07" ;
        rdf:value """Added the property chain axiom so that this property is
               formally defined as a shortcut (the inverse property already was)."""@en
    ], [
        dc:date "2023-11-02" ;
        rdf:value "Added a new rdfs:label in Spanish."@en
    ], [
        dc:date "2023-08-28" ;
        rdf:value "Added a new rdfs:label in French."@en
    ], [
        dc:date "2021-01-22" ;
        rdf:value """changed the IRI, label, inverse property IRI, text definition,
               corresponding CM component name (changed made in order to make RiC-O compliant with
               RiC-CM 0.2; the name of this property in RiC-O 0.1 was \"hasPosition\")."""@en
    ] ;
    :RiCCMCorrespondingComponent """RiC-R056i ('has or had position'
         relation)"""@en .

:hasOrHadRuleType
    a owl:ObjectProperty ;
    rdfs:comment """Connects a Rule to a Rule Type that categorized or categorizes
         it."""@en ;
    rdfs:domain :Rule ;
    rdfs:isDefinedBy <https://www.ica.org/standards/RiC/ontology> ;
    rdfs:label "a ou a eu pour type de règle"@fr, "has or had rule type"@en, "tiene o tenía como tipo de regla"@es ;
    rdfs:range :RuleType ;
    rdfs:subPropertyOf :hasOrHadType ;
    owl:inverseOf :isOrWasRuleTypeOf ;
    skos:changeNote [
        dc:date "2023-11-02" ;
        rdf:value "Added a new rdfs:label in Spanish."@en
    ], [
        dc:date "2023-08-28" ;
        rdf:value "Added a new rdfs:label in French."@en
    ], [
        dc:date "2021-01-22" ;
        rdf:value """changed the IRI, label, inverse property IRI, text definition,
               super property IRI (the name of this property in RiC-O 0.1 was
               \"hasRuleType\")."""@en
    ], [
        dc:date "2020-10-19" ;
        rdf:value """Object property added along with RuleType class and
               isRuleTypeOf object property. """@en
    ] .

:hasOrHadSomeMembersWhoseContentMainlyRepresents
    a owl:ObjectProperty ;
    rdfs:comment """Connects a Record Set and a Thing that is the main element
         represented by the content of some of the members of the Records or Record Parts that are
         or were included in the Record Set."""@en ;
    rdfs:domain :RecordSet ;
    rdfs:isDefinedBy <https://www.ica.org/standards/RiC/ontology> ;
    rdfs:label "has or had some members whose content mainly represents"@en, """inclut ou a inclus des membres dont le contenu représente
         principalement"""@fr, """incluye o incluía algunos miembros cuyo contenido representa
         principalmente"""@es ;
    rdfs:range :Thing ;
    rdfs:subPropertyOf :hasOrHadSomeMembersWhoseContentRepresents, :hasOrHadSomeMembersWithMainSubject ;
    owl:inverseOf :isOrWasMainThingRepresentedByContentOfSomeMembersOf ;
    skos:changeNote [
        dc:date "2025-04-06" ;
        rdf:value "Introduced in RiC-O 1.1."@en
    ] .

:hasOrHadSomeMembersWhoseContentRepresents
    a owl:ObjectProperty ;
    rdfs:comment """Connects a Record Set and a Thing that is represented by the
         content of some of the Records or Record Parts that are or were included in the Record
         Set."""@en ;
    rdfs:domain :RecordSet ;
    rdfs:isDefinedBy <https://www.ica.org/standards/RiC/ontology> ;
    rdfs:label "has or had some members whose content represents"@en, """inclut ou a inclus des membres dont le contenu
         représente"""@fr, """incluye o incluía algunos miembros cuyo contenido
         representa"""@es ;
    rdfs:range :Thing ;
    rdfs:subPropertyOf :hasOrHadSomeMembersWithSubject ;
    owl:inverseOf :isOrWasRepresentedByContentOfSomeMembersOf ;
    skos:changeNote [
        dc:date "2025-04-05" ;
        rdf:value "Introduced in RiC-O 1.1."@en
    ] .

:hasOrHadSomeMembersWithAccumulationDate
    a owl:ObjectProperty ;
    rdfs:comment """Inverse of 'is or was accumulation date of some members of' object
         property."""@en ;
    rdfs:domain :RecordSet ;
    rdfs:isDefinedBy <https://www.ica.org/standards/RiC/ontology> ;
    rdfs:label "has or had some members with accumulation date"@en, """inclut ou a inclus des membres ayant pour date
         d'accumulation"""@fr, """incluye o incluía algunos miembros con fecha de
         acumulación"""@es ;
    rdfs:range :Date ;
    rdfs:subPropertyOf :isAssociatedWithDate ;
    owl:inverseOf :isOrWasAccumulationDateOfSomeMembersOf ;
    skos:changeNote [
        dc:date "2025-04-06" ;
        rdf:value "Adjusted the Spanish label."@en
    ], [
        dc:date "2024-10-04" ;
        rdf:value "Added in RiC-O 1.1."@en
    ] .

:hasOrHadSomeMembersWithContentType
    a owl:ObjectProperty ;
    rdfs:comment """Connects a Record Set and a Content Type that categorizes some of
         the Records or Record Parts that are or were included in the Record Set."""@en ;
    rdfs:domain :RecordSet ;
    rdfs:isDefinedBy <https://www.ica.org/standards/RiC/ontology> ;
    rdfs:label "has or had some members with content type"@en, """inclut ou a inclus des membres ayant pour type de
         contenu"""@fr, """incluye o incluía algunos miembros con tipo de
         contenido"""@es ;
    rdfs:range :ContentType ;
    rdfs:subPropertyOf :hasOrHadSomeMembersWithType ;
    owl:inverseOf :isOrWasContentTypeOfSomeMembersOf ;
    skos:changeNote [
        dc:date "2025-04-06" ;
        rdf:value "Adjusted the Spanish label."@en
    ], [
        dc:date "2023-11-02" ;
        rdf:value "Added a new rdfs:label in Spanish."@en
    ], [
        dc:date "2023-08-28" ;
        rdf:value "Added a new rdfs:label in French."@en
    ], [
        dc:date "2020-12-28" ;
        rdf:value """Object property added for handling the case where a Record Set
               is described as having all or some members that belong to some category (see RiC-CM
               0.2 attributes section, #4.4 on Record Set, Record and Record Part
               attributes)."""@en
    ] .

:hasOrHadSomeMembersWithCreationDate
    a owl:ObjectProperty ;
    rdfs:comment """Inverse of 'is or was creation date of some members of' object
         property."""@en ;
    rdfs:domain :RecordSet ;
    rdfs:isDefinedBy <https://www.ica.org/standards/RiC/ontology> ;
    rdfs:label "has or had some members with creation date"@en, """inclut ou a inclus des membres ayant pour date de
         création"""@fr, """incluye o incluía algunos miembros con fecha de
         creación"""@es ;
    rdfs:range :Date ;
    rdfs:subPropertyOf :hasBeginningDate ;
    owl:inverseOf :isOrWasCreationDateOfSomeMembersOf ;
    skos:changeNote [
        dc:date "2025-04-06" ;
        rdf:value "Adjusted the Spanish label."@en
    ], [
        dc:date "2023-11-27" ;
        rdf:value "Added a new rdfs:label in Spanish."@en
    ], [
        dc:date "2023-10-13" ;
        rdf:value """Renamed the property in order to take the past members of the
               record set into account. Adjusted the annotations accordingly."""@en
    ], [
        dc:date "2023-10-12" ;
        rdf:value "Added the French label"@en
    ], [
        dc:date "2023-09-22" ;
        rdf:value "Added in RiC-O 1.0."@en
    ] ;
    :RiCCMCorrespondingComponent """RiC-R082i ('has or had some members with creation
         date' relation)"""@en .

:hasOrHadSomeMembersWithDocumentaryFormType
    a owl:ObjectProperty ;
    rdfs:comment """Connects a Record Set and a Documentary Form Type that categorizes
         some of the Records or Record Parts that are or were included in the Record
         Set."""@en ;
    rdfs:domain :RecordSet ;
    rdfs:isDefinedBy <https://www.ica.org/standards/RiC/ontology> ;
    rdfs:label "has or had some members with documentary form type"@en, """inclut ou a inclus des membres ayant pour type de
         document"""@fr, "incluye o incluía algunos miembros con tipo documental"@es ;
    rdfs:range :DocumentaryFormType ;
    rdfs:subPropertyOf :hasOrHadSomeMembersWithType ;
    owl:inverseOf :isOrWasDocumentaryFormTypeOfSomeMembersOf ;
    skos:changeNote [
        dc:date "2025-04-06" ;
        rdf:value "Adjusted the Spanish label."@en
    ], [
        dc:date "2024-03-15" ;
        rdf:value "Fixed a typo in IRI: changed 'with' to 'With'."@en
    ], [
        dc:date "2023-11-02" ;
        rdf:value "Added a new rdfs:label in Spanish."@en
    ], [
        dc:date "2023-08-28" ;
        rdf:value "Added a new rdfs:label in French."@en
    ], [
        dc:date "2020-12-28" ;
        rdf:value """Object property added for handling the case where a Record Set
               is described as having all or some members that belong to some category (see RiC-CM
               0.2 attributes section, #4.4 on Record Set, Record and Record Part
               attributes)."""@en
    ] .

:hasOrHadSomeMembersWithLanguage
    a owl:ObjectProperty ;
    rdfs:comment """Connects a Record Set and a Language used by some of the Records
         or Record Parts that are or were included in the Record Set."""@en ;
    rdfs:domain :RecordSet ;
    rdfs:isDefinedBy <https://www.ica.org/standards/RiC/ontology> ;
    rdfs:label "has or had some members with language"@en, "inclut ou a inclus des membres ayant pour langue"@fr, "incluye o incluía algunos miembros con lengua"@es ;
    rdfs:range :Language ;
    rdfs:subPropertyOf :isRelatedTo ;
    owl:inverseOf :isOrWasLanguageOfSomeMembersOf ;
    skos:changeNote [
        dc:date "2025-04-06" ;
        rdf:value "Adjusted the Spanish label."@en
    ], [
        dc:date "2023-11-02" ;
        rdf:value "Added a new rdfs:label in Spanish."@en
    ], [
        dc:date "2023-08-28" ;
        rdf:value "Added a new rdfs:label in French."@en
    ], [
        dc:date "2020-12-28" ;
        rdf:value """Object property added for handling the case where a Record Set
               is described as having all or some members that belong to some category (see RiC-CM
               0.2 attributes section, #4.4 on Record Set, Record and Record Part
               attributes)."""@en
    ] .

:hasOrHadSomeMembersWithLegalStatus
    a owl:ObjectProperty ;
    rdfs:comment """Connects a Record Set and a Legal Status that categorizes some of
         the Records or Record Parts that are or were included in the Record Set."""@en ;
    rdfs:domain :RecordSet ;
    rdfs:isDefinedBy <https://www.ica.org/standards/RiC/ontology> ;
    rdfs:label "has or had some members with legal status"@en, "inclut ou a inclus des membres ayant pour statut légal"@fr, "incluye o incluía algunos miembros con status jurídico"@es ;
    rdfs:range :LegalStatus ;
    rdfs:subPropertyOf :hasOrHadSomeMembersWithType ;
    owl:inverseOf :isOrWasLegalStatusOfSomeMembersOf ;
    skos:changeNote [
        dc:date "2025-04-06" ;
        rdf:value "Adjusted the Spanish label."@en
    ], [
        dc:date "2023-11-02" ;
        rdf:value "Added a new rdfs:label in Spanish."@en
    ], [
        dc:date "2023-08-28" ;
        rdf:value "Added a new rdfs:label in French."@en
    ], [
        dc:date "2020-12-28" ;
        rdf:value """Object property added for handling the case where a Record Set
               is described as having all or some members that belong to some category (see RiC-CM
               0.2 attributes section, #4.4 on Record Set, Record and Record Part
               attributes)."""@en
    ] .

:hasOrHadSomeMembersWithMainSubject
    a owl:ObjectProperty ;
    rdfs:comment """Connects a Record Set and a Thing that is the main subject of some
         of the Records or Record Parts that are or were included in the Record Set."""@en ;
    rdfs:domain :RecordSet ;
    rdfs:isDefinedBy <https://www.ica.org/standards/RiC/ontology> ;
    rdfs:label "has or had some members with main subject"@en, """inclut ou a inclus des membres ayant pour sujet
         principal"""@fr, """incluye o incluía algunos miembros con matería
         principal"""@es ;
    rdfs:range :Thing ;
    rdfs:subPropertyOf :hasOrHadSomeMembersWithSubject ;
    owl:inverseOf :isOrWasMainSubjectOfSomeMembersOf ;
    skos:changeNote [
        dc:date "2025-04-05" ;
        rdf:value "Introduced in RiC-O 1.1."@en
    ] .

:hasOrHadSomeMembersWithRecordState
    a owl:ObjectProperty ;
    rdfs:comment """Connects a Record Set and a Record State that categorizes some of
         the Records or Record Parts that are or were included in the Record Set."""@en ;
    rdfs:domain :RecordSet ;
    rdfs:isDefinedBy <https://www.ica.org/standards/RiC/ontology> ;
    rdfs:label "has or had some members with record state"@en, "inclut ou a inclus des membres ayant pour état"@fr, """incluye o incluía algunos miembros con estado de
         documento"""@es ;
    rdfs:range :RecordState ;
    rdfs:subPropertyOf :hasOrHadSomeMembersWithType ;
    owl:inverseOf :isOrWasRecordStateOfSomeMembersOf ;
    skos:changeNote [
        dc:date "2025-04-06" ;
        rdf:value "Adjusted the Spanish label."@en
    ], [
        dc:date "2023-11-02" ;
        rdf:value "Added a new rdfs:label in Spanish."@en
    ], [
        dc:date "2023-08-28" ;
        rdf:value "Added a new rdfs:label in French."@en
    ], [
        dc:date "2020-12-28" ;
        rdf:value """Object property added for handling the case where a Record Set
               is described as having all or some members that belong to some category (see RiC-CM
               0.2 attributes section, #4.4 on Record Set, Record and Record Part
               attributes)."""@en
    ] .

:hasOrHadSomeMembersWithSubject
    a owl:ObjectProperty ;
    rdfs:comment """Connects a Record Set and a Thing that is the subject of some of
         the Records or Record Parts that are or were included in the Record Set."""@en ;
    rdfs:domain :RecordSet ;
    rdfs:isDefinedBy <https://www.ica.org/standards/RiC/ontology> ;
    rdfs:label "has or had some members with subject"@en, "inclut ou a inclus des membres ayant pour sujet"@fr, "incluye o incluía algunos miembros con matería"@es ;
    rdfs:range :Thing ;
    rdfs:subPropertyOf :isRelatedTo ;
    owl:inverseOf :isOrWasSubjectOfSomeMembersOf ;
    skos:changeNote [
        dc:date "2025-04-06" ;
        rdf:value "Adjusted the Spanish label."@en
    ], [
        dc:date "2025-04-05" ;
        rdf:value "Introduced in RiC-O 1.1."@en
    ] .

:hasOrHadSomeMembersWithType
    a owl:ObjectProperty ;
    rdfs:comment """Connects a Record Set and a Type to which some of the Records or
         Record Parts that are or were included in the Record Set belong."""@en ;
    rdfs:domain :RecordSet ;
    rdfs:isDefinedBy <https://www.ica.org/standards/RiC/ontology> ;
    rdfs:label "has or had some members with type"@en, "inclut ou a inclus des membres ayant pour type"@fr, "incluye o incluía algunos miembros con tipo"@es ;
    rdfs:range :Type ;
    rdfs:subPropertyOf :isRelatedTo ;
    owl:inverseOf :isOrWasTypeOfSomeMembersOf ;
    skos:changeNote [
        dc:date "2025-04-06" ;
        rdf:value "Adjusted the Spanish label."@en
    ], [
        dc:date "2024-10-04" ;
        rdf:value """Changed the word 'category' into 'type' in all applicable
               properties names."""@en
    ], [
        dc:date "2023-11-02" ;
        rdf:value "Added a new rdfs:label in Spanish."@en
    ], [
        dc:date "2023-08-28" ;
        rdf:value "Added a new rdfs:label in French."@en
    ], [
        dc:date "2020-12-28" ;
        rdf:value """Object property added for handling the case where a Record Set
               is described as having all or some members that belong to some category (see RiC-CM
               0.2 attributes section, #4.4 on Record Set, Record and Record Part
               attributes)."""@en
    ] .

:hasOrHadSpouse
    a owl:ObjectProperty, owl:SymmetricProperty ;
    rdfs:comment """Connects two Persons who are or were married. This relation is
         symmetric."""@en ;
    rdfs:domain :Person ;
    rdfs:isDefinedBy <https://www.ica.org/standards/RiC/ontology> ;
    rdfs:label "a ou a eu pour conjoint"@fr, "has or had spouse"@en, "tiene o tenía como cónyuge a"@es ;
    rdfs:range :Person ;
    rdfs:subPropertyOf :hasFamilyAssociationWith ;
    owl:propertyChainAxiom (:thingIsConnectedToRelation
        :spouseRelation_role
        :relationConnects
    ) ;
    skos:changeNote [
        dc:date "2023-11-12" ;
        rdf:value """Aligned with RiC-CM 1.0: updated the description
               (rdfs:comment)."""@en
    ], [
        dc:date "2023-11-08" ;
        rdf:value """In order to get a system of rolified Relation classes: modified
               the property chain axiom so that it now involves the new spouseRelation_role object
               property."""@en
    ], [
        dc:date "2023-11-02" ;
        rdf:value "Added a new rdfs:label in Spanish."@en
    ], [
        dc:date "2023-08-28" ;
        rdf:value "Added a new rdfs:label in French."@en
    ], [
        dc:date "2021-01-22" ;
        rdf:value """changed the IRI, label, inverse property IRI, text definition,
               super property IRI (changed made in order to make RiC-O compliant with RiC-CM 0.2;
               the name of this property in RiC-O 0.1 was \"hasSpouse\")."""@en
    ] ;
    :RiCCMCorrespondingComponent """RiC-R049 ('has or had spouse'
         relation)"""@en .

:hasOrHadStudent
    a owl:ObjectProperty ;
    rdfs:comment "Inverse of 'has or had teacher' object property."@en ;
    rdfs:domain :Person ;
    rdfs:isDefinedBy <https://www.ica.org/standards/RiC/ontology> ;
    rdfs:label "a ou a eu pour étudiant"@fr, "has or had student"@en, "tiene o tenía como estudiante a"@es ;
    rdfs:range :Person ;
    rdfs:subPropertyOf :knows ;
    owl:inverseOf :hasOrHadTeacher ;
    owl:propertyChainAxiom (:thingIsSourceOfRelation
        :teachingRelation_role
        :relationHasTarget
    ) ;
    skos:changeNote [
        dc:date "2023-11-08" ;
        rdf:value """In order to get a system of rolified Relation classes: modified
               the property chain axiom so that it now involves the new teachingRelation_role object
               property."""@en
    ], [
        dc:date "2023-11-02" ;
        rdf:value "Added a new rdfs:label in Spanish."@en
    ], [
        dc:date "2023-08-28" ;
        rdf:value "Added a new rdfs:label in French."@en
    ], [
        dc:date "2021-01-22" ;
        rdf:value """changed the IRI, label, inverse property IRI, text definition
               (changed made in order to make RiC-O compliant with RiC-CM 0.2; the name of this
               property in RiC-O 0.1 was \"hasStudent\")."""@en
    ] ;
    :RiCCMCorrespondingComponent """RiC-R053i ('has or had student'
         relation)"""@en .

:hasOrHadSubdivision
    a owl:ObjectProperty ;
    rdfs:comment """Connects a Group to one of its present or past
         subdivisions."""@en ;
    rdfs:domain :Group ;
    rdfs:isDefinedBy <https://www.ica.org/standards/RiC/ontology> ;
    rdfs:label "a ou a eu pour subdivision"@fr, "has or had subdivision"@en, "tiene o tenía como subdivisión"@es ;
    rdfs:range :Group ;
    rdfs:subPropertyOf :hasOrHadPart, :hasOrHadSubordinate ;
    owl:inverseOf :isOrWasSubdivisionOf ;
    owl:propertyChainAxiom (:thingIsSourceOfRelation
        :groupSubdivisionRelation_role
        :relationHasTarget
    ) ;
    skos:changeNote [
        dc:date "2023-11-08" ;
        rdf:value """In order to get a system of rolified Relation classes: modified
               the property chain axiom so that it now involves the new
               groupSubdivisionRelation_role object property."""@en
    ], [
        dc:date "2023-11-02" ;
        rdf:value "Added a new rdfs:label in Spanish."@en
    ], [
        dc:date "2023-08-28" ;
        rdf:value "Added a new rdfs:label in French."@en
    ], [
        dc:date "2021-01-22" ;
        rdf:value """changed the IRI, label, inverse property IRI, text definition,
               super property IRIs (changed made in order to make RiC-O compliant with RiC-CM 0.2;
               the name of this property in RiC-O 0.1 was \"hasSubdivision\")."""@en
    ] ;
    :RiCCMCorrespondingComponent """RiC-R005 ('has or had subdivision'
         relation)"""@en .

:hasOrHadSubevent
    a owl:ObjectProperty ;
    rdfs:comment """Connects an Event to one of a series of Events that constitute the
         original, broader, past or ongoing Event."""@en ;
    rdfs:domain :Event ;
    rdfs:isDefinedBy <https://www.ica.org/standards/RiC/ontology> ;
    rdfs:label "est ou a été constitué de l’événement"@fr, "has or had subevent"@en, "tiene o tenía como parte de evento"@es ;
    rdfs:range :Event ;
    rdfs:subPropertyOf :hasOrHadPart, :isAssociatedWithEvent, :isEventAssociatedWith ;
    owl:inverseOf :isOrWasSubeventOf ;
    skos:changeNote [
        dc:date "2023-11-02" ;
        rdf:value "Added a new rdfs:label in Spanish."@en
    ], [
        dc:date "2023-08-28" ;
        rdf:value "Added a new rdfs:label in French."@en
    ], [
        dc:date "2021-01-22" ;
        rdf:value """changed the IRI, label, inverse property IRI, text definition,
               super property IRI (changed made in order to make RiC-O compliant with RiC-CM 0.2;
               the name of this property in RiC-O 0.1 was \"hasSubEvent\")."""@en
    ] ;
    skos:scopeNote """Since an Activity is a kind of Event, this Relation can also be
         used for Activity."""@en ;
    :RiCCMCorrespondingComponent """RiC-R006 ('has or had subevent'
         relation)"""@en .

:hasOrHadSubject
    a owl:ObjectProperty ;
    rdfs:comment """Connects a Record Resource to a Thing that is or was its
         subject."""@en ;
    rdfs:domain :RecordResource ;
    rdfs:isDefinedBy <https://www.ica.org/standards/RiC/ontology> ;
    rdfs:label "a ou a eu pour sujet"@fr, "has or had subject"@en, "tiene o tenía como materia"@es ;
    rdfs:range :Thing ;
    rdfs:subPropertyOf :isRelatedTo ;
    owl:inverseOf :isOrWasSubjectOf ;
    skos:changeNote [
        dc:date "2023-11-12" ;
        rdf:value """Aligned with RiC-CM 1.0: updated the
               skos:scopeNote."""@en
    ], [
        dc:date "2023-11-02" ;
        rdf:value "Added a new rdfs:label in Spanish."@en
    ], [
        dc:date "2023-08-28" ;
        rdf:value "Added a new rdfs:label in French."@en
    ], [
        dc:date "2021-01-22" ;
        rdf:value """changed the IRI, label, inverse property IRI, text definition
               (changed made in order to make RiC-O compliant with RiC-CM 0.2; the name of this
               property in RiC-O 0.1 was \"hasSubject\")."""@en
    ] ;
    skos:scopeNote """The subject of a Record Set may be affected if the Record Set
         loses some of the Records."""@en ;
    :RiCCMCorrespondingComponent """RiC-R019 ('has or had subject'
         relation)"""@en .

:hasOrHadSubordinate
    a owl:ObjectProperty ;
    rdfs:comment """Connects an Agent to an Agent that is hierarchically
         inferior."""@en ;
    rdfs:domain :Agent ;
    rdfs:isDefinedBy <https://www.ica.org/standards/RiC/ontology> ;
    rdfs:label "a ou a eu pour subalterne"@fr, "has or had subordinate"@en, "tiene o tenía como subordinado o subordinada a"@es ;
    rdfs:range :Agent ;
    rdfs:subPropertyOf :isAgentAssociatedWithAgent ;
    owl:inverseOf :isOrWasSubordinateTo ;
    owl:propertyChainAxiom (:thingIsSourceOfRelation
        :agentHierarchicalRelation_role
        :relationHasTarget
    ) ;
    skos:changeNote [
        dc:date "2023-11-12" ;
        rdf:value """Aligned with RiC-CM 1.0: updated the
               skos:scopeNote."""@en
    ], [
        dc:date "2023-11-08" ;
        rdf:value """In order to get a system of rolified Relation classes: modified
               the property chain axiom so that it now involves the new
               agentHierarchicalRelation_role object property."""@en
    ], [
        dc:date "2023-11-02" ;
        rdf:value "Added a new rdfs:label in Spanish."@en
    ], [
        dc:date "2023-08-28" ;
        rdf:value "Added a new rdfs:label in French."@en
    ], [
        dc:date "2021-01-22" ;
        rdf:value """changed the IRI, label, inverse property IRI (changed made in
               order to make RiC-O compliant with RiC-CM 0.2; the name of this property in RiC-O 0.1
               was \"isHierarchicallySuperiorTo\")."""@en
    ] ;
    skos:scopeNote """The hierarchical relation can be an authority relation, or a
         whole/part relation between two Agents."""@en ;
    :RiCCMCorrespondingComponent """RiC-R045 ('has or had subordinate '
         relation)"""@en .

:hasOrHadTeacher
    a owl:ObjectProperty ;
    rdfs:comment """Connects a Person to another Person who is or was their
         teacher."""@en ;
    rdfs:domain :Person ;
    rdfs:isDefinedBy <https://www.ica.org/standards/RiC/ontology> ;
    rdfs:label "a ou a eu pour enseignant"@fr, "has or had teacher"@en, "tiene o tenía como profesor(a) a"@es ;
    rdfs:range :Person ;
    rdfs:subPropertyOf :knows ;
    owl:inverseOf :hasOrHadStudent ;
    owl:propertyChainAxiom (:thingIsTargetOfRelation
        :teachingRelation_role
        :relationHasSource
    ) ;
    skos:changeNote [
        dc:date "2023-11-12" ;
        rdf:value """Aligned with RiC-CM 1.0: updated the description
               (rdfs:comment)."""@en
    ], [
        dc:date "2023-11-08" ;
        rdf:value """In order to get a system of rolified Relation classes: modified
               the property chain axiom so that it now involves the new teachingRelation_role object
               property."""@en
    ], [
        dc:date "2023-11-02" ;
        rdf:value "Added a new rdfs:label in Spanish."@en
    ], [
        dc:date "2023-08-28" ;
        rdf:value "Added a new rdfs:label in French."@en
    ], [
        dc:date "2021-01-22" ;
        rdf:value """changed the IRI, label, inverse property IRI, text definition
               (changed made in order to make RiC-O compliant with RiC-CM 0.2; the name of this
               property in RiC-O 0.1 was \"hasTeacher\")."""@en
    ] ;
    :RiCCMCorrespondingComponent """RiC-R053 ('has or had teacher'
         relation)"""@en .

:hasOrHadTitle
    a owl:ObjectProperty ;
    rdfs:comment """Connects a Record Resource, Instantiation or Rule to a title that
         is or was used for designating it."""@en ;
    rdfs:domain [
        a owl:Class ;
        owl:unionOf (:Instantiation
            :RecordResource
            :Rule
        )
    ] ;
    rdfs:isDefinedBy <https://www.ica.org/standards/RiC/ontology> ;
    rdfs:label "a ou a eu pour intitulé"@fr, "has or had title"@en, "tiene o tenía como título"@es ;
    rdfs:range :Title ;
    rdfs:subPropertyOf :hasOrHadName ;
    owl:inverseOf :isOrWasTitleOf ;
    skos:changeNote [
        dc:date "2023-11-02" ;
        rdf:value "Added a new rdfs:label in Spanish."@en
    ], [
        dc:date "2023-08-28" ;
        rdf:value "Added a new rdfs:label in French."@en
    ], [
        dc:date "2021-01-22" ;
        rdf:value """changed the IRI, label, inverse property IRI, text definition,
               super property IRI (the name of this property in RiC-O 0.1 was
               \"hasTitle\")."""@en
    ] .

:hasOrHadType
    a owl:ObjectProperty ;
    rdfs:comment """Connects a Thing to a Type that categorizes or categorized
         it."""@en ;
    rdfs:domain :Thing ;
    rdfs:isDefinedBy <https://www.ica.org/standards/RiC/ontology> ;
    rdfs:label "a ou a eu pour type"@fr, "has or had type"@en, "tiene o tenía como tipo"@es ;
    rdfs:range :Type ;
    rdfs:subPropertyOf :isRelatedTo ;
    owl:inverseOf :isOrWasTypeOf ;
    owl:propertyChainAxiom (:thingIsTargetOfRelation
        :typeRelation_role
        :relationHasSource
    ) ;
    skos:changeNote [
        dc:date "2024-10-04" ;
        rdf:value """Changed the word 'category' into 'type' in all applicable
               properties names."""@en
    ], [
        dc:date "2023-11-08" ;
        rdf:value """In order to get a system of rolified Relation classes: modified
               the property chain axiom so that it now involves the new typeRelation_role object
               property."""@en
    ], [
        dc:date "2023-11-02" ;
        rdf:value "Added a new rdfs:label in Spanish."@en
    ], [
        dc:date "2023-08-28" ;
        rdf:value "Added a new rdfs:label in French."@en
    ], [
        dc:date "2021-01-22" ;
        rdf:value """changed the IRI, label, inverse property IRI, text definition
               (the name of this property in RiC-O 0.1 was \"belongsToCategory\")."""@en
    ] .

:hasOrHadWorkRelationWith
    a owl:ObjectProperty, owl:SymmetricProperty ;
    rdfs:comment """Connects two Agents that have or had some type of work relation in
         the course of their activities. This relation is symmetric."""@en ;
    rdfs:domain :Agent ;
    rdfs:isDefinedBy <https://www.ica.org/standards/RiC/ontology> ;
    rdfs:label "a ou a eu une relation professionnelle avec"@fr, "has or had work relation with"@en, "tiene o tenía relación profesional con"@es ;
    rdfs:range :Agent ;
    rdfs:subPropertyOf :isAgentAssociatedWithAgent ;
    owl:propertyChainAxiom (:thingIsConnectedToRelation
        :workRelation_role
        :relationConnects
    ) ;
    skos:changeNote [
        dc:date "2023-11-08" ;
        rdf:value """In order to get a system of rolified Relation classes: modified
               the property chain axiom so that it now involves the new workRelation_role object
               property."""@en
    ], [
        dc:date "2023-11-07" ;
        rdf:value """Added the property chain axiom so that this property is
               formally defined as a shortcut."""@en
    ], [
        dc:date "2023-11-02" ;
        rdf:value "Added a new rdfs:label in Spanish."@en
    ], [
        dc:date "2023-08-28" ;
        rdf:value "Added a new rdfs:label in French."@en
    ], [
        dc:date "2021-01-22" ;
        rdf:value """changed the IRI, label, text definition (changed made in order
               to make RiC-O compliant with RiC-CM 0.2; the name of this property in RiC-O 0.1 was
               \"hasWorkRelationWith\")."""@en
    ] ;
    :RiCCMCorrespondingComponent """RiC-R046 ('has or had work relation with'
         relation)"""@en .

:hasOrganicOrFunctionalProvenance
    a owl:ObjectProperty ;
    rdfs:comment """Connects a Record Resource or an Instantiation to an Agent that
         creates or accumulates it, receives it, or sends it, or to an Activity that generates
         it."""@en ;
    rdfs:domain [
        a owl:Class ;
        owl:unionOf (:Instantiation
            :RecordResource
        )
    ] ;
    rdfs:isDefinedBy <https://www.ica.org/standards/RiC/ontology> ;
    rdfs:label "a pour provenance organique ou fonctionnelle"@fr, "has organic or functional provenance"@en, "tiene como procedencia orgánica o funcional"@es ;
    rdfs:range [
        a owl:Class ;
        owl:unionOf (:Activity
            :Agent
        )
    ] ;
    rdfs:subPropertyOf :isRelatedTo ;
    owl:inverseOf :isOrganicOrFunctionalProvenanceOf ;
    owl:propertyChainAxiom (:thingIsSourceOfRelation
        :organicOrFunctionalProvenanceRelation_role
        :relationHasTarget
    ) ;
    skos:changeNote [
        dc:date "2023-11-08" ;
        rdf:value """In order to get a system of rolified Relation classes: modified
               the property chain axiom so that it now involves the new
               organicOrFunctionalProvenanceRelation_role object property."""@en
    ], [
        dc:date "2023-11-07" ;
        rdf:value """Property added as a superproperty of hasProvenance and
               documents, along with its inverse property. Shortcut also added."""@en
    ] .

:hasOrganicProvenance
    a owl:ObjectProperty ;
    rdfs:comment """Connects a Record Resource or an Instantiation to an Agent that
         creates or accumulates the Record Resource, receives it, or sends it."""@en ;
    rdfs:domain [
        a owl:Class ;
        owl:unionOf (:Instantiation
            :RecordResource
        )
    ] ;
    rdfs:isDefinedBy <https://www.ica.org/standards/RiC/ontology> ;
    rdfs:label "a pour provenance organique"@fr, "has organic provenance"@en, "tiene como procedencia orgánica"@es ;
    rdfs:range :Agent ;
    rdfs:subPropertyOf :hasOrganicOrFunctionalProvenance ;
    owl:inverseOf :isOrganicProvenanceOf ;
    owl:propertyChainAxiom (:thingIsSourceOfRelation
        :organicProvenanceRelation_role
        :relationHasTarget
    ) ;
    skos:changeNote [
        dc:date "2023-11-12" ;
        rdf:value """Aligned with RiC-CM 1.0: updated the
               skos:scopeNote."""@en
    ], [
        dc:date "2023-11-08" ;
        rdf:value """In order to get a system of rolified Relation classes: modified
               the property chain axiom so that it now involves the new
               organicProvenanceRelation_role object property."""@en
    ], [
        dc:date "2023-11-07" ;
        rdf:value """Made this property a subproperty of the new
               hasOrganicOrFunctionalProvenance property. Renamed it to make things clearer.
               Adjusted its labels."""@en
    ], [
        dc:date "2023-11-02" ;
        rdf:value "Added a new rdfs:label in Spanish."@en
    ], [
        dc:date "2023-08-28" ;
        rdf:value "Added a new rdfs:label in French."@en
    ] ;
    skos:scopeNote """This is the most general organic provenance relation. Use it to
         connect a Record Resource or Instantiation with an Agent only if it is not possible to use
         a narrower, more specific relation, for example has creator."""@en ;
    :RiCCMCorrespondingComponent """RiC-R026 ('has provenance'
         relation)"""@en .

:hasOrganicProvenanceDate
    a owl:ObjectProperty ;
    rdfs:comment """Inverse of 'is date associated with organic provenance of' object
         property."""@en ;
    rdfs:domain [
        a owl:Class ;
        owl:unionOf (:Instantiation
            :RecordResource
        )
    ] ;
    rdfs:isDefinedBy <https://www.ica.org/standards/RiC/ontology> ;
    rdfs:label "a pour date de provenance organique"@fr, "has organic provenance date"@en, "tiene como fecha de procedencia orgánica"@es ;
    rdfs:range :Date ;
    rdfs:subPropertyOf :isAssociatedWithDate ;
    owl:inverseOf :isOrganicProvenanceDateOf ;
    owl:propertyChainAxiom (:thingIsSourceOfRelation
        :organicProvenanceRelation_role
        :relationHasDate
    ) ;
    skos:changeNote [
        dc:date "2025-03-13" ;
        rdf:value "Added French and Spanish labels."@en
    ], [
        dc:date "2024-12-19" ;
        rdf:value "Added in RiC-O 1.1."@en
    ] .

:hasOriginal
    a owl:ObjectProperty ;
    rdfs:comment "Inverse of 'is original of' object property."@en ;
    rdfs:domain [
        a owl:Class ;
        owl:unionOf (:Record
            :RecordPart
        )
    ] ;
    rdfs:isDefinedBy <https://www.ica.org/standards/RiC/ontology> ;
    rdfs:label "a pour original"@fr, "has original"@en, "tiene como original"@es ;
    rdfs:range [
        a owl:Class ;
        owl:unionOf (:Record
            :RecordPart
        )
    ] ;
    rdfs:subPropertyOf :followsInTime, :hasGeneticLinkToRecordResource ;
    owl:inverseOf :isOriginalOf ;
    skos:changeNote [
        dc:date "2023-11-02" ;
        rdf:value "Added a new rdfs:label in Spanish."@en
    ], [
        dc:date "2023-08-28" ;
        rdf:value "Added a new rdfs:label in French."@en
    ] ;
    :RiCCMCorrespondingComponent """RiC-R010i ('is original of'
         relation)"""@en .

:hasPartTransitive
    a owl:ObjectProperty, owl:TransitiveProperty ;
    rdfs:comment """Connects a Thing to a Thing that is, directly or indirectly, a
         constitutive or component part of that Thing. This is a transitive relation."""@en ;
    rdfs:domain :Thing ;
    rdfs:isDefinedBy <https://www.ica.org/standards/RiC/ontology> ;
    rdfs:label "a pour partie transitif"@fr, "has part transitive"@en, "tiene como parte transitivo"@es ;
    rdfs:range :Thing ;
    rdfs:subPropertyOf :hasOrHadPart ;
    owl:inverseOf :isPartOfTransitive ;
    skos:changeNote [
        dc:date "2023-11-27" ;
        rdf:value "Added a new rdfs:label in Spanish."@en
    ], [
        dc:date "2023-11-12" ;
        rdf:value "Updated the labels."@en
    ], [
        dc:date "2023-07-12" ;
        rdf:value """Object property added, along with its inverse property, in
               order to enable to express current partitive relations between things (the past
               partitive relation also being added)."""@en
    ] ;
    skos:scopeNote """To be used, either to infer, then query or browse, relations
         from existing direct 'hasDirectPart' relations between things, or to record a current
         partitive relation when you do not know if there are intermediate nodes between the related
         things."""@en .

:hasProductionTechniqueType
    a owl:ObjectProperty ;
    rdfs:comment """Connects an Instantiation to a Production Technique Type that
         categorizes its production technique."""@en ;
    rdfs:domain :Instantiation ;
    rdfs:isDefinedBy <https://www.ica.org/standards/RiC/ontology> ;
    rdfs:label "a pour type de technique de production"@fr, "has production technique type"@en, "tiene como técnica de producción"@es ;
    rdfs:range :ProductionTechniqueType ;
    rdfs:subPropertyOf :hasOrHadType ;
    owl:inverseOf :isProductionTechniqueTypeOf ;
    skos:changeNote [
        dc:date "2023-11-02" ;
        rdf:value "Added a new rdfs:label in Spanish."@en
    ], [
        dc:date "2023-08-28" ;
        rdf:value "Added a new rdfs:label in French."@en
    ], [
        dc:date "2021-01-22" ;
        rdf:value "changed the super property IRI."@en
    ] .

:hasProxy
    a owl:ObjectProperty ;
    rdfs:comment "Inverse of 'proxy for' object property."@en ;
    rdfs:domain :RecordResource ;
    rdfs:isDefinedBy <https://www.ica.org/standards/RiC/ontology> ;
    rdfs:label "a pour proxy"@fr, "has proxy"@en, "tiene como proxy"@es ;
    rdfs:range :Proxy ;
    rdfs:subPropertyOf :isRelatedTo ;
    owl:inverseOf :proxyFor ;
    skos:changeNote [
        dc:date "2025-04-02" ;
        rdf:value "Added the French and Spanish labels."@en
    ], [
        dc:date "2025-03-04" ;
        rdf:value "Introduced in RiC-O 1.1"@en
    ] .

:hasPublicationDate
    a owl:ObjectProperty ;
    rdfs:comment """Inverse of 'is publication date of' object
         property."""@en ;
    rdfs:domain :RecordResource ;
    rdfs:isDefinedBy <https://www.ica.org/standards/RiC/ontology> ;
    rdfs:label "a pour date de publication"@fr, "has publication date"@en, "tiene como fecha de publicación"@es ;
    rdfs:range :Date ;
    rdfs:subPropertyOf :isAssociatedWithDate ;
    owl:inverseOf :isPublicationDateOf ;
    skos:changeNote [
        dc:date "2023-11-27" ;
        rdf:value "Added a new rdfs:label in Spanish."@en
    ], [
        dc:date "2023-10-12" ;
        rdf:value "Added the French label"@en
    ], [
        dc:date "2023-09-22" ;
        rdf:value "Added in RiC-O 1.0."@en
    ] .

:hasPublisher
    a owl:ObjectProperty ;
    rdfs:comment """Connects a Record resource to an Agent who published
         it."""@en ;
    rdfs:domain :RecordResource ;
    rdfs:isDefinedBy <https://www.ica.org/standards/RiC/ontology> ;
    rdfs:label "a pour éditeur"@fr, "has publisher"@en, "tiene como editor(a) a"@es ;
    rdfs:range :Agent ;
    rdfs:subPropertyOf :isRelatedTo ;
    owl:inverseOf :isPublisherOf ;
    skos:changeNote [
        dc:date "2023-11-02" ;
        rdf:value "Added a new rdfs:label in Spanish."@en
    ], [
        dc:date "2023-08-28" ;
        rdf:value "Added a new rdfs:label in French."@en
    ], [
        dc:date "2021-01-22" ;
        rdf:value """changed the IRI, label, inverse property IRI (the name of this
               property in RiC-O 0.1 was \"publishedBy\")."""@en
    ] .

:hasReceiver
    a owl:ObjectProperty ;
    rdfs:comment """Connects a Record Resource or an Instantiation to the Agent that
         receives it in the course of the Agent's activities."""@en ;
    rdfs:domain [
        a owl:Class ;
        owl:unionOf (:Instantiation
            :RecordResource
        )
    ] ;
    rdfs:isDefinedBy <https://www.ica.org/standards/RiC/ontology> ;
    rdfs:label "est reçu par"@fr, "has receiver"@en, "tiene como receptor(a) a"@es ;
    rdfs:range :Agent ;
    rdfs:subPropertyOf :hasAccumulator ;
    owl:inverseOf :isReceiverOf ;
    skos:changeNote [
        dc:date "2023-11-12" ;
        rdf:value """Aligned with RiC-CM 1.0: updated the description
               (rdfs:comment)."""@en
    ], [
        dc:date "2023-11-02" ;
        rdf:value "Added a new rdfs:label in Spanish."@en
    ], [
        dc:date "2023-08-28" ;
        rdf:value "Added a new rdfs:label in French."@en
    ], [
        dc:date "2023-08-28" ;
        rdf:value "Added a new rdfs:label in French."@en
    ], [
        dc:date "2021-01-22" ;
        rdf:value """changed the IRI, label, inverse property IRI, super property
               IRI (changed made in order to make RiC-O compliant with RiC-CM 0.2; the name of this
               property in RiC-O 0.1 was \"receivedBy\")."""@en
    ] ;
    :RiCCMCorrespondingComponent """RiC-R029 ('has receiver'
         relation)"""@en .

:hasRecordSetType
    a owl:ObjectProperty ;
    rdfs:comment """Connects a Record Set to a Record Set Type that categorizes
         it."""@en ;
    rdfs:domain :RecordSet ;
    rdfs:isDefinedBy <https://www.ica.org/standards/RiC/ontology> ;
    rdfs:label "a pour type d’ensemble d’objets informationnels"@fr, "has record set type"@en, "tiene como tipo de agrupación documental"@es ;
    rdfs:range :RecordSetType ;
    rdfs:subPropertyOf :hasOrHadType ;
    owl:inverseOf :isRecordSetTypeOf ;
    skos:changeNote [
        dc:date "2023-11-02" ;
        rdf:value "Added a new rdfs:label in Spanish."@en
    ], [
        dc:date "2023-08-28" ;
        rdf:value "Added a new rdfs:label in French."@en
    ], [
        dc:date "2021-01-22" ;
        rdf:value "changed the super property IRI."@en
    ] .

:hasRecordState
    a owl:ObjectProperty ;
    rdfs:comment """Connects a Record or Record Part to a Record State that
         categorizes its state."""@en ;
    rdfs:domain [
        a owl:Class ;
        owl:unionOf (:Record
            :RecordPart
        )
    ] ;
    rdfs:isDefinedBy <https://www.ica.org/standards/RiC/ontology> ;
    rdfs:label "a pour état"@fr, "has record state"@en, "tiene como estado de documento"@es ;
    rdfs:range :RecordState ;
    rdfs:subPropertyOf :hasOrHadType ;
    owl:inverseOf :isRecordStateOf ;
    skos:changeNote [
        dc:date "2023-11-02" ;
        rdf:value "Added a new rdfs:label in Spanish."@en
    ], [
        dc:date "2023-08-28" ;
        rdf:value "Added a new rdfs:label in French."@en
    ], [
        dc:date "2020-12-28" ;
        rdf:value """Changed the IRI (hasRecordResourceState changed to
               hasRecordState), label, textual definition and domain (RecordResource replaced by
               Record or Record Part)."""@en
    ] .

:hasReply
    a owl:ObjectProperty ;
    rdfs:comment """Connects a Record Resource to a reply, usually in the form of
         correspondence."""@en ;
    rdfs:domain :RecordResource ;
    rdfs:isDefinedBy <https://www.ica.org/standards/RiC/ontology> ;
    rdfs:label "a pour réponse"@fr, "has reply"@en, "tiene como contestación"@es ;
    rdfs:range :RecordResource ;
    rdfs:subPropertyOf :isRecordResourceAssociatedWithRecordResource, :precedesInTime ;
    owl:inverseOf :isReplyTo ;
    skos:changeNote [
        dc:date "2023-11-02" ;
        rdf:value "Added a new rdfs:label in Spanish."@en
    ], [
        dc:date "2023-08-28" ;
        rdf:value "Added a new rdfs:label in French."@en
    ], [
        dc:date "2021-01-22" ;
        rdf:value """changed the IRI, label, inverse property IRI, text definition
               (changed made in order to make RiC-O compliant with RiC-CM 0.2; the name of this
               property in RiC-O 0.1 was \"isRepliedToBy\")."""@en
    ] ;
    :RiCCMCorrespondingComponent """RiC-R013 ('has reply'
         relation)"""@en .

:hasRepresentationType
    a owl:ObjectProperty ;
    rdfs:comment """Connects an Instantiation to a Representation Type that
         categorizes its representation type."""@en ;
    rdfs:domain :Instantiation ;
    rdfs:isDefinedBy <https://www.ica.org/standards/RiC/ontology> ;
    rdfs:label "a pour type de représentation"@fr, "has representation type"@en, "tiene como tipo de grabación"@es ;
    rdfs:range :RepresentationType ;
    rdfs:subPropertyOf :hasOrHadType ;
    owl:inverseOf :isRepresentationTypeOf ;
    skos:changeNote [
        dc:date "2023-11-02" ;
        rdf:value "Added a new rdfs:label in Spanish."@en
    ], [
        dc:date "2023-08-28" ;
        rdf:value "Added a new rdfs:label in French."@en
    ], [
        dc:date "2021-01-22" ;
        rdf:value "changed the super property IRI."@en
    ] .

:hasSender
    a owl:ObjectProperty ;
    rdfs:comment """Connects a Record Resource or an Instantiation to the Agent that
         sends it"""@en ;
    rdfs:domain [
        a owl:Class ;
        owl:unionOf (:Instantiation
            :RecordResource
        )
    ] ;
    rdfs:isDefinedBy <https://www.ica.org/standards/RiC/ontology> ;
    rdfs:label "a pour expéditeur"@fr, "has sender"@en, "tiene como remitente a"@es ;
    rdfs:range :Agent ;
    rdfs:subPropertyOf :hasOrganicProvenance ;
    owl:inverseOf :isSenderOf ;
    skos:changeNote [
        dc:date "2023-11-12" ;
        rdf:value """Aligned with RiC-CM 1.0: updated the
               skos:scopeNote."""@en
    ], [
        dc:date "2023-11-02" ;
        rdf:value "Added a new rdfs:label in Spanish."@en
    ], [
        dc:date "2023-08-28" ;
        rdf:value "Added a new rdfs:label in French."@en
    ] ;
    skos:scopeNote """The identity of the sender is (usually) evidenced by the Record
         Resource or Instantiation itself."""@en ;
    :RiCCMCorrespondingComponent """RiC-R031 ('has sender'
         relation)"""@en .

:hasSibling
    a owl:ObjectProperty, owl:SymmetricProperty ;
    rdfs:comment """Connects two Persons who are siblings. This relation is
         symmetric."""@en ;
    rdfs:domain :Person ;
    rdfs:isDefinedBy <https://www.ica.org/standards/RiC/ontology> ;
    rdfs:label "a pour frère ou sœur"@fr, "has sibling"@en, "tiene como hermano o hermana a"@es ;
    rdfs:range :Person ;
    rdfs:subPropertyOf :hasFamilyAssociationWith ;
    owl:propertyChainAxiom (:thingIsConnectedToRelation
        :siblingRelation_role
        :relationConnects
    ) ;
    skos:changeNote [
        dc:date "2023-11-12" ;
        rdf:value """Aligned with RiC-CM 1.0: updated the description
               (rdfs:comment)."""@en
    ], [
        dc:date "2023-11-08" ;
        rdf:value """In order to get a system of rolified Relation classes: modified
               the property chain axiom so that it now involves the new siblingRelation_role object
               property."""@en
    ], [
        dc:date "2023-11-02" ;
        rdf:value "Added a new rdfs:label in Spanish."@en
    ], [
        dc:date "2023-08-28" ;
        rdf:value "Added a new rdfs:label in French."@en
    ], [
        dc:date "2021-01-22" ;
        rdf:value "changed the super property IRI."@en
    ] ;
    :RiCCMCorrespondingComponent """RiC-R048 ('has sibling'
         relation)"""@en .

:hasSubdivisionTransitive
    a owl:ObjectProperty, owl:TransitiveProperty ;
    rdfs:comment """Connects a Group to another Group that is one of its direct or
         indirect subdivisions. This is a transitive relation."""@en ;
    rdfs:domain :Group ;
    rdfs:isDefinedBy <https://www.ica.org/standards/RiC/ontology> ;
    rdfs:label "a pour subdivision transitif"@fr, "has subdivision transitive"@en, "tiene como subdivisión transitivo"@es ;
    rdfs:range :Group ;
    rdfs:subPropertyOf :hasOrHadSubdivision, :hasPartTransitive, :hasSubordinateTransitive ;
    owl:inverseOf :isSubdivisionOfTransitive ;
    skos:changeNote [
        dc:date "2023-11-27" ;
        rdf:value "Added a new rdfs:label in Spanish."@en
    ], [
        dc:date "2023-11-25" ;
        rdf:value "Fixed the French label."@en
    ], [
        dc:date "2023-11-12" ;
        rdf:value "Updated the labels."@en
    ], [
        dc:date "2023-09-08" ;
        rdf:value """Object property added, along with its inverse property, in
               order to enable to express current partitive relations between groups (the past
               partitive relation also being added)."""@en
    ] .

:hasSubeventTransitive
    a owl:ObjectProperty, owl:TransitiveProperty ;
    rdfs:comment """Connects an ongoing Event to one of a series of Events that
         directly or indirectly constitute that broader, ongoing Event. This is a transitive
         relation."""@en ;
    rdfs:domain :Event ;
    rdfs:isDefinedBy <https://www.ica.org/standards/RiC/ontology> ;
    rdfs:label "est constitué de l’événement transitif"@fr, "has subevent transitive"@en, "tiene como parte de evento transitivo"@es ;
    rdfs:range :Event ;
    rdfs:subPropertyOf :hasOrHadSubevent, :hasPartTransitive ;
    owl:inverseOf :isSubeventOfTransitive ;
    skos:changeNote [
        dc:date "2024-10-21" ;
        rdf:value "Fixed the Spanish label."@en
    ], [
        dc:date "2023-11-27" ;
        rdf:value "Added a new rdfs:label in Spanish."@en
    ], [
        dc:date "2023-11-12" ;
        rdf:value "Updated the labels."@en
    ], [
        dc:date "2023-09-08" ;
        rdf:value """Object property added, along with its inverse property, in
               order to enable to express partitive relations between ongoing events (the past
               partitive relation also being added)."""@en
    ] .

:hasSubordinateTransitive
    a owl:ObjectProperty, owl:TransitiveProperty ;
    rdfs:comment """Connects an Agent to an Agent that is directly or indirectly
         hierarchically inferior. This is a transitive relation."""@en ;
    rdfs:domain :Agent ;
    rdfs:isDefinedBy <https://www.ica.org/standards/RiC/ontology> ;
    rdfs:label "a pour subalterne transitif"@fr, "has subordinate transitive"@en, "tiene como subordinado o subordinada a transitivo"@es ;
    rdfs:range :Agent ;
    rdfs:subPropertyOf :hasOrHadSubordinate ;
    owl:inverseOf :isSubordinateToTransitive ;
    skos:changeNote [
        dc:date "2023-11-27" ;
        rdf:value "Added a new rdfs:label in Spanish."@en
    ], [
        dc:date "2023-11-12" ;
        rdf:value "Updated the labels."@en
    ], [
        dc:date "2023-09-08" ;
        rdf:value """Object property added, along with its inverse property, in
               order to enable to express current subordination relations between agents (the past
               subordination relation also being added)."""@en
    ] .

:hasSuccessor
    a owl:ObjectProperty ;
    rdfs:comment """Connects an Agent to another Agent that succeeds it
         chronologically."""@en ;
    rdfs:domain :Agent ;
    rdfs:isDefinedBy <https://www.ica.org/standards/RiC/ontology> ;
    rdfs:label "a pour successeur"@fr, "has successor"@en, "tiene como sucesor(a) a"@es ;
    rdfs:range :Agent ;
    rdfs:subPropertyOf :isAgentAssociatedWithAgent, :precedesInTime ;
    owl:inverseOf :isSuccessorOf ;
    owl:propertyChainAxiom (:thingIsSourceOfRelation
        :agentTemporalRelation_role
        :relationHasTarget
    ) ;
    skos:changeNote [
        dc:date "2023-11-08" ;
        rdf:value """In order to get a system of rolified Relation classes: modified
               the property chain axiom so that it now involves the new agentTemporalRelation_role
               object property."""@en
    ], [
        dc:date "2023-11-02" ;
        rdf:value "Added a new rdfs:label in Spanish."@en
    ], [
        dc:date "2023-08-28" ;
        rdf:value "Added a new rdfs:label in French."@en
    ], [
        dc:date "2021-01-22" ;
        rdf:value """changed the IRI and label (changed made in order to make RiC-O
               compliant with RiC-CM 0.2; the name of this property in RiC-O 0.1 was
               \"isAntecedentOf\")."""@en
    ] ;
    skos:scopeNote """There may be zero to many intermediate Agents, ignored or
         unknown, between the two connected Agents. Can be used when there is a transfer of function
         from the first Agent to the second Agent."""@en ;
    :RiCCMCorrespondingComponent """RIC-R016 ('has successor'
         relation)"""@en .

:hasTitleType
    a owl:ObjectProperty ;
    rdfs:comment """Connects a Title and a Title Type that categorizes
         it."""@en ;
    rdfs:domain :Title ;
    rdfs:isDefinedBy <https://www.ica.org/standards/RiC/ontology> ;
    rdfs:label "a pour type de titre"@fr, "has title type"@en, "tiene como tipo de título"@es ;
    rdfs:range :TitleType ;
    rdfs:subPropertyOf :hasOrHadType ;
    owl:inverseOf :isTitleTypeOf ;
    skos:changeNote [
        dc:date "2024-10-04" ;
        rdf:value """Object property added along with TitleType class and
               isTitleTypeOf object property. """@en
    ] .

:hasUnitOfMeasurement
    a owl:ObjectProperty ;
    rdfs:comment "Connects an Extent to a Unit Of Measurement"@en ;
    rdfs:domain :Extent ;
    rdfs:isDefinedBy <https://www.ica.org/standards/RiC/ontology> ;
    rdfs:label "a pour unité de mesure"@fr, "has unit of measurement"@en, "tiene como unidad de medida"@es ;
    rdfs:range :UnitOfMeasurement ;
    rdfs:subPropertyOf :isRelatedTo ;
    owl:inverseOf :isUnitOfMeasurementOf ;
    skos:changeNote [
        dc:date "2023-11-02" ;
        rdf:value "Added a new rdfs:label in Spanish."@en
    ], [
        dc:date "2023-08-28" ;
        rdf:value """Added a new rdfs:label in French; added an xml:lang attribute
               to the rdfs:comment."""@en
    ], [
        dc:date "2020-10-28" ;
        rdf:value """Object property created along with Extent and UnitOfMeasurement
               classes, in order to provide methods for handling extent accurately."""@en
    ] .

:hasWithin
    a owl:ObjectProperty ;
    rdfs:comment "Inverse of 'is within' object property."@en ;
    rdfs:domain :Date ;
    rdfs:isDefinedBy <https://www.ica.org/standards/RiC/ontology> ;
    rdfs:label "contient"@fr, "has within"@en, "tiene dentro"@es ;
    rdfs:range :Date ;
    rdfs:subPropertyOf :hasOrHadPart, :isAssociatedWithDate, :isDateAssociatedWith ;
    owl:inverseOf :isWithin ;
    skos:changeNote [
        dc:date "2023-11-27" ;
        rdf:value "Added a new rdfs:label in Spanish."@en
    ], [
        dc:date "2023-10-13" ;
        rdf:value """made this property a subproperty of both isDateAssociatedWith
               and isAssociatedWithdate, and of hasOrHadPart."""@en
    ], [
        dc:date "2023-10-12" ;
        rdf:value "Added the property"@en
    ] ;
    :RiCCMCorrespondingComponent """RiC-R085i ('has within'
         relation)"""@en .

:height
    a owl:DatatypeProperty ;
    rdfs:comment "Vertical dimension of an entity."@en ;
    rdfs:domain :Thing ;
    rdfs:isDefinedBy <https://www.ica.org/standards/RiC/ontology> ;
    rdfs:label "altura"@es, "hauteur"@fr, "height"@en ;
    rdfs:range rdfs:Literal ;
    rdfs:subPropertyOf :measure ;
    skos:changeNote [
        dc:date "2023-11-02" ;
        rdf:value "Added a new rdfs:label in Spanish."@en
    ], [
        dc:date "2023-08-25" ;
        rdf:value "Added a new rdfs:label in French."@en
    ] .

:history
    a owl:DatatypeProperty ;
    rdfs:comment """Summary of the development of an entity throughout its
         existence."""@en ;
    rdfs:domain [
        a owl:Class ;
        owl:unionOf (:Agent
            :Event
            :Instantiation
            :Place
            :RecordResource
            :Rule
        )
    ] ;
    rdfs:isDefinedBy <https://www.ica.org/standards/RiC/ontology> ;
    rdfs:label "histoire"@fr, "historia"@es, "history"@en ;
    rdfs:range rdfs:Literal ;
    skos:changeNote [
        dc:date "2023-11-11" ;
        rdf:value """Aligned with RiC-CM 1.0: updated the description
               (rdfs:comment), skos:scopeNote, domain, examples (skos:example)."""@en
    ], [
        dc:date "2023-11-02" ;
        rdf:value "Added a new rdfs:label in Spanish."@en
    ], [
        dc:date "2023-08-25" ;
        rdf:value "Added a new rdfs:label in French."@en
    ], [
        dc:date "2020-11-01" ;
        rdf:value """Domains updated. Examples added. Objective: to make RiC-O
               compliant with RiC-CM v0.2."""@en
    ] ;
    skos:example """El primer sorteo de lotería se celebró el 13 de mayo de 1771,
         siendo desarrollado por la Real Lotería General de Nueva España… (sobre una
         actividad)"""@es, """Nacido en Barbastro en 1892, donde realizó sus primeros estudios
         con los escolapios. Licenciado en Derecho por la Universidad de Zaragoza, aprobó las
         oposiciones al cuerpo nacional de notarios… (sobre una persona)"""@es, """The manuscripts are part of the collections of Robert Harley (d
         1724) and Edward Harley (d 1741), 1st and 2nd Earls of Oxford, that were brought by
         Parliament and transferred to the British Museum in 1753. Those materials were then
         separated into this collection and those for Harley Charters and Harley Rolls and became
         part of the collections of the British Library in 1972. (about a Record Set)"""@en ;
    skos:scopeNote """For a record set, may be used to summarize the history of the
         Record Set itself, or additionally to summarize the history of some or all members of the
         Record Set. Should not be confused with the scope and content property."""@en ;
    :RiCCMCorrespondingComponent """Corresponds to RiC-A21 (History
         attribute)"""@en .

:identifier
    a owl:DatatypeProperty ;
    rdfs:comment """A word, number, letter, symbol, or any combination of these used
         to uniquely identify or reference an individual instance of an entity within a specific
         information domain. Can include Global Persistent Identifiers (globally unique and
         persistently resolvable identifier for the entity) and/or Local Identifiers. Both the
         domain within which the identifier is unique, and the rules used in forming the identifier
         value should be provided with the identifier value."""@en ;
    rdfs:domain :Thing ;
    rdfs:isDefinedBy <https://www.ica.org/standards/RiC/ontology> ;
    rdfs:label "identifiant"@fr, "identificador"@es, "identifier"@en ;
    rdfs:range rdfs:Literal ;
    skos:changeNote [
        dc:date "2023-11-11" ;
        rdf:value """Aligned with RiC-CM 1.0: updated the description
               (rdfs:comment), skos:scopeNote, examples (skos:example)."""@en
    ], [
        dc:date "2023-11-02" ;
        rdf:value "Added a new rdfs:label in Spanish."@en
    ], [
        dc:date "2023-08-25" ;
        rdf:value "Added a new rdfs:label in French."@en
    ], [
        dc:date "2020-11-01" ;
        rdf:value """Text definition and scope note updated. Examples added.
               Objective: to make RiC-O compliant with RiC-CM v0.2."""@en
    ] ;
    skos:example """B-000091 (example of a unique identifier for an instantiation
         assigned by a repository)"""@en, """BUD-01-F002 (example of a classification number from a corporate
         file plan)"""@en, """F 1204 (example of a local identifier for a record set assigned by
         a repository)"""@en, """NAS1/A/1.1 (example of a local identifier for a
         record)"""@en, """http://isni.org/0000000073572182 (example of a persistent
         International Standard Name Identifier for a person)"""@en, """http://n2t.net/ark:/99166/w6tz44ht (example of an Archival
         Resource Key for a person)"""@en, """http://n2t.net/ark:/99166/w6v1266v (example of an Archival
         Resource Key for a record)"""@en ;
    skos:scopeNote """Use only if you don't use Identifier class for handling
         identifiers. Within a given domain (a closed system), identifiers are used to uniquely
         reference instances of an entity. Identifiers are instruments of control that facilitate
         management of the entities within the domain. The formulation of identifiers commonly is
         based on rules. In addition to an identifier needing to be unique within a domain, it is
         also highly desirable that it be persistent, that is, that the identifier uniquely
         identifies the entity over time. A variety of organizations provide rules for the formation
         of identifiers, and services designed to facilitate the persistence of identifiers. Such
         identifiers are commonly referred to as Persistent Identifiers (or PIDs). PIDs conform to
         RFC 3986, but impose additional rules. Common examples are Archival Resource Keys (ARKs)
         and Digital Object Identifiers (DOIs). Within the global environment of the Internet, there
         are special rules for the formation of identifiers to ensure that they are unique within
         the domain of the Internet. Such identifiers must conform to the Internet Engineering Task
         Force (IETF) Uniform Resource Identifier rules (RFC 3986)."""@en ;
    :RiCCMCorrespondingComponent """Corresponds to RiC-A22 (Identifier
         attribute)"""@en .

:included
    a owl:ObjectProperty ;
    rdfs:comment """Connects a Record Set to a Record or Record Set which it included
         in the past."""@en ;
    rdfs:domain :RecordSet ;
    rdfs:isDefinedBy <https://www.ica.org/standards/RiC/ontology> ;
    rdfs:label "a inclus"@fr, "included"@en, "incluía"@es ;
    rdfs:range [
        a owl:Class ;
        owl:unionOf (:Record
            :RecordSet
        )
    ] ;
    rdfs:subPropertyOf :hadPart, :includesOrIncluded ;
    owl:inverseOf :wasIncludedIn ;
    skos:changeNote [
        dc:date "2023-11-27" ;
        rdf:value "Added a new rdfs:label in Spanish."@en
    ], [
        dc:date "2023-11-13" ;
        rdf:value "Added a French label."@en
    ], [
        dc:date "2023-09-08" ;
        rdf:value """Object property added, along with its inverse property, in
               order to enable to express past partitive relations between Record Sets and their
               members (the current partitive relations being also added, including a transitive
               one)."""@en
    ] .

:includesOrIncluded
    a owl:ObjectProperty ;
    rdfs:comment """Connects a Record Set to a Record or Record Set it aggregates, or
         aggregated in the past."""@en ;
    rdfs:domain :RecordSet ;
    rdfs:isDefinedBy <https://www.ica.org/standards/RiC/ontology> ;
    rdfs:label "includes or included"@en, "inclut ou a inclus"@fr, "incluye o incluía"@es ;
    rdfs:range [
        a owl:Class ;
        owl:unionOf (:Record
            :RecordSet
        )
    ] ;
    rdfs:subPropertyOf :hasOrHadPart, :isRecordResourceAssociatedWithRecordResource ;
    owl:inverseOf :isOrWasIncludedIn ;
    skos:changeNote [
        dc:date "2023-11-02" ;
        rdf:value "Added a new rdfs:label in Spanish."@en
    ], [
        dc:date "2023-08-28" ;
        rdf:value "Added a new rdfs:label in French."@en
    ], [
        dc:date "2023-06-05" ;
        rdf:value """Made this object property a subproperty of
               hasOrHadPart."""@en
    ], [
        dc:date "2021-01-22" ;
        rdf:value """changed the IRI, label, inverse property IRI, text definition
               (changed made in order to make RiC-O compliant with RiC-CM 0.2; the name of this
               property in RiC-O 0.1 was \"includes\")."""@en
    ] ;
    skos:scopeNote """A Record or Record Set can be aggregated in one or many Record
         Sets simultaneously or through time."""@en ;
    :RiCCMCorrespondingComponent """RiC-R024 ('includes or included'
         relation)"""@en .

:includesProxy
    a owl:ObjectProperty ;
    rdfs:comment "Inverse of 'proxy is included in' object property."@en ;
    rdfs:domain :RecordSet ;
    rdfs:isDefinedBy <https://www.ica.org/standards/RiC/ontology> ;
    rdfs:label "includes proxy"@en, "inclut le proxy"@fr, "incluye el proxy"@es ;
    rdfs:range :Proxy ;
    rdfs:subPropertyOf :hasPartTransitive ;
    owl:inverseOf :proxyIsIncludedIn ;
    owl:propertyChainAxiom (:includesProxy
        :proxyIncludesProxyTransitive
    ) ;
    skos:changeNote [
        dc:date "2025-04-02" ;
        rdf:value "Added the French and Spanish labels."@en
    ], [
        dc:date "2025-04-02" ;
        rdf:value """Fixed the owl:inverseOf (was set to
               isPartOfTransitive)."""@en
    ], [
        dc:date "2025-03-04" ;
        rdf:value "Introduced in RiC-O 1.1."@en
    ] .

:includesTransitive
    a owl:ObjectProperty, owl:TransitiveProperty ;
    rdfs:comment """Connects a Record Set to a Record or Record Set which it includes
         directly or indirectly. This is a transitive relation."""@en ;
    rdfs:domain :RecordSet ;
    rdfs:isDefinedBy <https://www.ica.org/standards/RiC/ontology> ;
    rdfs:label "includes transitive"@en, "inclut transitif"@fr, "incluye transitivo"@es ;
    rdfs:range [
        a owl:Class ;
        owl:unionOf (:Record
            :RecordSet
        )
    ] ;
    rdfs:subPropertyOf :hasPartTransitive, :includesOrIncluded ;
    owl:inverseOf :isIncludedInTransitive ;
    owl:propertyChainAxiom (:includesProxy
        :proxyIncludes
    ) ;
    skos:changeNote [
        dc:date "2025-03-04" ;
        rdf:value """Added a property chain axiom relating it to use of
               rico:Proxy"""@en
    ], [
        dc:date "2023-11-27" ;
        rdf:value "Added a new rdfs:label in Spanish."@en
    ], [
        dc:date "2023-11-13" ;
        rdf:value "Added two labels."@en
    ], [
        dc:date "2023-09-08" ;
        rdf:value """Object property added, along with its inverse property, in
               order to enable to express current partitive relations between Record Sets and their
               members (the past partitive relation also being added)."""@en
    ] .

:instantiationExtent
    a owl:DatatypeProperty ;
    rdfs:comment """Countable characteristics of an Instantiation expressed as a
         quantity."""@en ;
    rdfs:domain :Instantiation ;
    rdfs:isDefinedBy <https://www.ica.org/standards/RiC/ontology> ;
    rdfs:label "Instantiation extent"@en, "mesure de l’instanciation"@fr, "soporte de instanciación"@es ;
    rdfs:range rdfs:Literal ;
    rdfs:subPropertyOf :physicalOrLogicalExtent ;
    skos:changeNote [
        dc:date "2023-11-11" ;
        rdf:value """Aligned with RiC-CM 1.0: updated the description
               (rdfs:comment), skos:scopeNote, examples (skos:example)."""@en
    ], [
        dc:date "2023-11-02" ;
        rdf:value "Added a new rdfs:label in Spanish."@en
    ], [
        dc:date "2023-08-25" ;
        rdf:value "Added a new rdfs:label in French."@en
    ], [
        dc:date "2020-11-01" ;
        rdf:value """Scope note updated. Examples added. Objective: to make RiC-O
               compliant with RiC-CM v0.2."""@en
    ] ;
    skos:example "234 linear metres"@en, "Size of PDF file: 1.5 MB"@en, "The register has 345 written folios"@en ;
    skos:scopeNote """Instantiation extent should not be confused with record resource
         extent or carrier extent. For a given Record Resource, the instantiation extent may vary,
         based on format, density of information on the carrier, etc. For example, a CD with a
         storage capacity of 700 MB (carrier extent) might hold a record of 1500 words (record
         resource extent) represented in two versions, one a Word document with an instantiation
         extent of 3 KB and the other a PDF file with an instantiation extent of 5
         KB."""@en ;
    :RiCCMCorrespondingComponent """Corresponds to RiC-A23 (Instantiation Extent
         attribute)"""@en .

:instantiationStructure
    a owl:DatatypeProperty ;
    rdfs:comment """Information about the physical arrangement and composition of an
         Instantiation."""@en ;
    rdfs:domain :Instantiation ;
    rdfs:isDefinedBy <https://www.ica.org/standards/RiC/ontology> ;
    rdfs:label "Instantiation structure"@en, "estructura de la instanciación"@es, "structure de l’instanciation"@fr ;
    rdfs:range rdfs:Literal ;
    rdfs:subPropertyOf :structure ;
    skos:changeNote [
        dc:date "2023-11-02" ;
        rdf:value "Added a new rdfs:label in Spanish."@en
    ], [
        dc:date "2023-08-25" ;
        rdf:value "Added a new rdfs:label in French."@en
    ], [
        dc:date "2020-11-01" ;
        rdf:value """Text definition fixed. Objective: to make RiC-O compliant with
               RiC-CM v0.2."""@en
    ] ;
    :RiCCMCorrespondingComponent """Specialization of RiC-A40 (Structure
         attribute)"""@en .

:instantiationToInstantiationRelation_role
    a owl:ObjectProperty ;
    rdfs:comment """Connects an InstantiationToInstantiationRelation to itself. It is
         a property that can stand for an instance of the class when necessary, e.g. when you
         explore a knowledge graph."""@en ;
    rdfs:domain :InstantiationToInstantiationRelation ;
    rdfs:isDefinedBy <https://www.ica.org/standards/RiC/ontology> ;
    rdfs:label "a le rôle de la Relation entre instanciations"@fr, "desempeña el papel de la Relación entre instanciaciones"@es, """has the role of the Instantiation to Instantiation
         Relation"""@en ;
    rdfs:range :InstantiationToInstantiationRelation ;
    rdfs:subPropertyOf :relation_role ;
    skos:changeNote [
        dc:date "2024-08-02" ;
        rdf:value """Removed global reflexivity (leads to
               inconsistency)."""@en
    ], [
        dc:date "2023-11-08" ;
        rdf:value """In order to get a system of rolified Relation classes: created
               the object property, with domain and range the InstantiationToInstantiationRelation
               rolified class. Declared it as reflexive. Declared it(s)
               superproperty(ies)."""@en
    ] ;
    skos:scopeNote """This property \"rolifies\" the
         InstantiationToInstantiationRelation class. It should be used only when you have to manage
         instances of the InstantiationToInstantiationRelation class, to connect each instance to
         itself, in order to be able to infer, using OWL-RL and property paths, the two shortcuts
         corresponding to this n-ary class."""@en .

:integrityNote
    a owl:DatatypeProperty ;
    rdfs:comment """Information about the known intellectual completeness of a Record
         Resource."""@en ;
    rdfs:domain :RecordResource ;
    rdfs:isDefinedBy <https://www.ica.org/standards/RiC/ontology> ;
    rdfs:label "integrity note"@en, "nota de integridad"@es, "note sur l'intégrité"@fr ;
    rdfs:range rdfs:Literal ;
    rdfs:subPropertyOf :note ;
    skos:changeNote [
        dc:date "2025-01-17" ;
        rdf:value """Made this property a subproperty of the new rico:note datatype
               property."""@en
    ], [
        dc:date "2023-11-11" ;
        rdf:value """Aligned with RiC-CM 1.0: updated the IRI, mapping to RiC-CM
               (rico:RiCCMCorrespondingComponent), labels, description (rdfs:comment),
               skos:scopeNote, domain, examples (skos:example)."""@en
    ], [
        dc:date "2023-11-02" ;
        rdf:value "Added a new rdfs:label in Spanish."@en
    ], [
        dc:date "2023-08-25" ;
        rdf:value "Added a new rdfs:label in French."@en
    ], [
        dc:date "2020-11-01" ;
        rdf:value """Scope note and examples added. Objective: to make RiC-O
               compliant with RiC-CM v0.2."""@en
    ] ;
    skos:example """A web page (HTML, 15 images, 2 CSS, 1 javascript), with 5 images
         missing."""@en, """For record set: series of letters, one is missing so the integrity
         is compromised."""@en, """Line three of a hand-written letter was cut out and a replacement
         text was inserted by an unknown person."""@en, """Part of the text is missing (because a corner on the instantiation
         was cut out, which is a physical characteristic). See also the examples of
         physicalCharacteristics."""@en ;
    skos:scopeNote """May be used in a Record Set description when its value is shared
         by some or all members of the Record Set. The information about integrity may be generated
         manually or automatically. Not to be confused with the physical completeness of the
         instantiation, which is covered by the physical characteristics note attribute. The
         integrity of a Record Resource and the physical characteristics note of an Instantiation
         may be complementary. This attribute also covers any additions to or removal of original
         information."""@en ;
    :RiCCMCorrespondingComponent """Corresponds to RiC-A24 (Integrity Note
         attribute)"""@en .

:intellectualPropertyRightsRelation_role
    a owl:ObjectProperty ;
    rdfs:comment """Connects an IntellectualPropertyRightsRelation to itself. It is a
         property that can stand for an instance of the class when necessary, e.g. when you explore
         a knowledge graph."""@en ;
    rdfs:domain :IntellectualPropertyRightsRelation ;
    rdfs:isDefinedBy <https://www.ica.org/standards/RiC/ontology> ;
    rdfs:label "a le rôle de la Relation de propriété intellectuelle"@fr, """desempeña el papel de la Relación de propiedad
         intelectual"""@es, """has the role of the Intellectual Property Rights
         Relation"""@en ;
    rdfs:range :IntellectualPropertyRightsRelation ;
    rdfs:subPropertyOf :authorityRelation_role ;
    skos:changeNote [
        dc:date "2024-08-02" ;
        rdf:value """Removed global reflexivity (leads to
               inconsistency)."""@en
    ], [
        dc:date "2023-11-08" ;
        rdf:value """In order to get a system of rolified Relation classes: created
               the object property, with domain and range the IntellectualPropertyRightsRelation
               rolified class. Declared it as reflexive. Declared it(s)
               superproperty(ies)."""@en
    ] ;
    skos:scopeNote """This property \"rolifies\" the IntellectualPropertyRightsRelation
         class. It should be used only when you have to manage instances of the
         IntellectualPropertyRightsRelation class, to connect each instance to itself, in order to
         be able to infer, using OWL-RL and property paths, the two shortcuts corresponding to this
         n-ary class."""@en .

:intersects
    a owl:ObjectProperty, owl:SymmetricProperty ;
    rdfs:comment """Connects two Dates that overlap. This relation is
         symmetric."""@en ;
    rdfs:domain :Date ;
    rdfs:isDefinedBy <https://www.ica.org/standards/RiC/ontology> ;
    rdfs:label "cruza"@es, "intersecte"@fr, "intersects"@en ;
    rdfs:range :Date ;
    rdfs:subPropertyOf :isAssociatedWithDate, :isDateAssociatedWith ;
    skos:changeNote [
        dc:date "2023-11-27" ;
        rdf:value "Added a new rdfs:label in Spanish."@en
    ], [
        dc:date "2023-10-13" ;
        rdf:value """made this property a subproperty of
               isAssociatedWithdate."""@en
    ], [
        dc:date "2023-10-12" ;
        rdf:value "Added the property"@en
    ] ;
    :RiCCMCorrespondingComponent """RiC-R086 ('intersects'
         relation)"""@en .

:isAccumulationDateOf
    a owl:ObjectProperty ;
    rdfs:comment """Connects a Date to a Record Resource or Instantiation that was or
         will be accumulated at this Date."""@en ;
    rdfs:domain :Date ;
    rdfs:isDefinedBy <https://www.ica.org/standards/RiC/ontology> ;
    rdfs:label "es fecha de acumulación de"@es, "est la date d'accumulation de"@fr, "is accumulation date of"@en ;
    rdfs:range [
        a owl:Class ;
        owl:unionOf (:Instantiation
            :RecordResource
        )
    ] ;
    rdfs:subPropertyOf :isOrganicProvenanceDateOf ;
    owl:inverseOf :hasAccumulationDate ;
    owl:propertyChainAxiom (:isDateAssociatedWithRelation
        :accumulationRelation_role
        :relationHasSource
    ) ;
    skos:changeNote [
        dc:date "2025-02-19" ;
        rdf:value "Changed definition (added \"or will be\")."@en
    ], [
        dc:date "2024-12-19" ;
        rdf:value """Connect to AccumulationRelation via a sub-property chain, and
               make a sub-property of the new 'isOrganicProvenanceDateOf' object
               property."""@en
    ], [
        dc:date "2024-10-04" ;
        rdf:value "Added in RiC-O 1.1."@en
    ] ;
    skos:scopeNote """When used for a Record Set (e.g. a file), it is the accumulation
         date of the Record Set itself rather than the accumulation date of the members of the
         Record Set. To record the accumulation date of members of the Record Set, use 'is or was
         accumulation date of all members of', 'is or was accumulation date of most members of’ or
         'is or was accumulation date of some members of’."""@en .

:isAccumulatorOf
    a owl:ObjectProperty ;
    rdfs:comment "Inverse of 'has accumulator' object property."@en ;
    rdfs:domain :Agent ;
    rdfs:isDefinedBy <https://www.ica.org/standards/RiC/ontology> ;
    rdfs:label "accumule"@fr, "es acumulador(a) de"@es, "is accumulator of"@en ;
    rdfs:range [
        a owl:Class ;
        owl:unionOf (:Instantiation
            :RecordResource
        )
    ] ;
    rdfs:subPropertyOf :isOrganicProvenanceOf ;
    owl:inverseOf :hasAccumulator ;
    owl:propertyChainAxiom (:thingIsTargetOfRelation
        :accumulationRelation_role
        :relationHasSource
    ) ;
    skos:changeNote [
        dc:date "2023-11-08" ;
        rdf:value """In order to get a system of rolified Relation classes: modified
               the property chain axiom so that it now involves the new accumulationRelation_role
               object property."""@en
    ], [
        dc:date "2023-11-02" ;
        rdf:value "Added a new rdfs:label in Spanish."@en
    ], [
        dc:date "2023-08-28" ;
        rdf:value "Added a new rdfs:label in French."@en
    ], [
        dc:date "2021-01-22" ;
        rdf:value """changed the IRI, label, inverse property IRI, text definition
               and corresponding CM component (changed made in order to make RiC-O compliant with
               RiC-CM 0.2; the name of this property in RiC-O 0.1 was \"accumulates\")."""@en
    ] ;
    :RiCCMCorrespondingComponent """RiC-R028i ('is accumulator of'
         relation)"""@en .

:isActivityTypeOf
    a owl:ObjectProperty ;
    rdfs:comment """Connects an Activity Type to an Activity that it
         categorizes."""@en ;
    rdfs:domain :ActivityType ;
    rdfs:isDefinedBy <https://www.ica.org/standards/RiC/ontology> ;
    rdfs:label "es tipo de actividad de"@es, "est le type d’activité de"@fr, "is activity type of"@en ;
    rdfs:range :Activity ;
    rdfs:subPropertyOf :isOrWasTypeOf ;
    owl:inverseOf :hasActivityType ;
    skos:changeNote [
        dc:date "2023-11-02" ;
        rdf:value "Added a new rdfs:label in Spanish."@en
    ], [
        dc:date "2023-08-28" ;
        rdf:value "Added a new rdfs:label in French."@en
    ], [
        dc:date "2021-01-22" ;
        rdf:value "changed the super property IRI."@en
    ] .

:isAddresseeOf
    a owl:ObjectProperty ;
    rdfs:comment "Inverse of 'has addressee' object property."@en ;
    rdfs:domain :Agent ;
    rdfs:isDefinedBy <https://www.ica.org/standards/RiC/ontology> ;
    rdfs:label "es destino de"@es, "est le destinataire de"@fr, "is addressee of"@en ;
    rdfs:range [
        a owl:Class ;
        owl:unionOf (:Instantiation
            :RecordResource
        )
    ] ;
    rdfs:subPropertyOf :isOrganicProvenanceOf ;
    owl:inverseOf :hasAddressee ;
    skos:changeNote [
        dc:date "2023-11-02" ;
        rdf:value "Added a new rdfs:label in Spanish."@en
    ], [
        dc:date "2023-08-28" ;
        rdf:value "Added a new rdfs:label in French."@en
    ] ;
    :RiCCMCorrespondingComponent """RiC-032i ('is addressee of'
         relation)"""@en .

:isAgentAssociatedWithAgent
    a owl:ObjectProperty, owl:SymmetricProperty ;
    rdfs:comment """Connects two Agents. This object property is
         symmetric."""@en ;
    rdfs:domain :Agent ;
    rdfs:isDefinedBy <https://www.ica.org/standards/RiC/ontology> ;
    rdfs:label "agente está asociado con agente"@es, "est un agent associé à l’agent"@fr, "is agent associated with agent"@en ;
    rdfs:range :Agent ;
    rdfs:subPropertyOf :isRelatedTo ;
    owl:propertyChainAxiom (:thingIsConnectedToRelation
        :agentToAgentRelation_role
        :relationConnects
    ) ;
    skos:changeNote [
        dc:date "2023-11-25" ;
        rdf:value "Fixed the French label."@en
    ], [
        dc:date "2023-11-12" ;
        rdf:value """Aligned with RiC-CM 1.0: updated the
               skos:scopeNote."""@en
    ], [
        dc:date "2023-11-08" ;
        rdf:value """In order to get a system of rolified Relation classes: modified
               the property chain axiom so that it now involves the new agentToAgentRelation_role
               object property."""@en
    ], [
        dc:date "2023-11-02" ;
        rdf:value "Added a new rdfs:label in Spanish."@en
    ], [
        dc:date "2023-08-28" ;
        rdf:value "Added a new rdfs:label in French."@en
    ] ;
    skos:scopeNote """Use only if it is not possible to specify a narrower Agent to
         Agent relation, for example has or had work relation with."""@en ;
    :RiCCMCorrespondingComponent """RiC-R044 ('is agent associated with agent'
         relation)"""@en .

:isAgentAssociatedWithPlace
    a owl:ObjectProperty ;
    rdfs:comment """Inverse of 'is place associated with agent' object
         property."""@en ;
    rdfs:domain :Agent ;
    rdfs:isDefinedBy <https://www.ica.org/standards/RiC/ontology> ;
    rdfs:label "agente está asociado con lugar"@es, "est un agent associé au lieu"@fr, "is agent associated with place"@en ;
    rdfs:range :Place ;
    rdfs:subPropertyOf :isAssociatedWithPlace ;
    owl:inverseOf :isPlaceAssociatedWithAgent ;
    skos:changeNote [
        dc:date "2023-11-27" ;
        rdf:value "Added a new rdfs:label in Spanish."@en
    ], [
        dc:date "2023-10-26" ;
        rdf:value "Added a rdfs:comment."@en
    ], [
        dc:date "2023-10-19" ;
        rdf:value "Added for RiC-O v1.0."@en
    ] .

:isAssociatedWithDate
    a owl:ObjectProperty ;
    rdfs:comment """Inverse of 'is date associated with' object
         property."""@en ;
    rdfs:domain :Thing ;
    rdfs:isDefinedBy <https://www.ica.org/standards/RiC/ontology> ;
    rdfs:label "est associé à la date"@fr, "está asociado con fecha"@es, "is associated with date"@en ;
    rdfs:range :Date ;
    rdfs:subPropertyOf :isRelatedTo ;
    owl:inverseOf :isDateAssociatedWith ;
    skos:changeNote [
        dc:date "2023-11-02" ;
        rdf:value "Added a new rdfs:label in Spanish."@en
    ], [
        dc:date "2023-08-28" ;
        rdf:value "Added a new rdfs:label in French."@en
    ] ;
    :RiCCMCorrespondingComponent """RiC-R068i ('is associated with date'
         relation)"""@en .

:isAssociatedWithEvent
    a owl:ObjectProperty ;
    rdfs:comment """Inverse of 'is event associated with' object
         property."""@en ;
    rdfs:domain :Thing ;
    rdfs:isDefinedBy <https://www.ica.org/standards/RiC/ontology> ;
    rdfs:label "est associé à l’événement"@fr, "está asociado con evento"@es, "is associated with event"@en ;
    rdfs:range :Event ;
    rdfs:subPropertyOf :isRelatedTo ;
    owl:inverseOf :isEventAssociatedWith ;
    owl:propertyChainAxiom (:thingIsTargetOfRelation
        :eventRelation_role
        :relationHasSource
    ) ;
    skos:changeNote [
        dc:date "2023-11-08" ;
        rdf:value """In order to get a system of rolified Relation classes: modified
               the property chain axiom so that it now involves the new eventRelation_role object
               property."""@en
    ], [
        dc:date "2023-11-02" ;
        rdf:value "Added a new rdfs:label in Spanish."@en
    ], [
        dc:date "2023-08-28" ;
        rdf:value "Added a new rdfs:label in French."@en
    ] ;
    :RiCCMCorrespondingComponent """RiC-R057i ('is associated with event'
         relation)"""@en .

:isAssociatedWithPlace
    a owl:ObjectProperty ;
    rdfs:comment """Inverse of 'is place associated with' object
         property."""@en ;
    rdfs:domain :Thing ;
    rdfs:isDefinedBy <https://www.ica.org/standards/RiC/ontology> ;
    rdfs:label "est associé au lieu"@fr, "está asociado con lugar"@es, "is associated with place"@en ;
    rdfs:range :Place ;
    rdfs:subPropertyOf :isRelatedTo ;
    owl:inverseOf :isPlaceAssociatedWith ;
    owl:propertyChainAxiom (:thingIsTargetOfRelation
        :placeRelation_role
        :relationHasSource
    ) ;
    skos:changeNote [
        dc:date "2023-11-08" ;
        rdf:value """In order to get a system of rolified Relation classes: modified
               the property chain axiom so that it now involves the new placeRelation_role object
               property."""@en
    ], [
        dc:date "2023-11-02" ;
        rdf:value "Added a new rdfs:label in Spanish."@en
    ], [
        dc:date "2023-08-28" ;
        rdf:value "Added a new rdfs:label in French."@en
    ] ;
    :RiCCMCorrespondingComponent """RiC-R074i ('is associated with place'
         relation)"""@en .

:isAssociatedWithRule
    a owl:ObjectProperty ;
    rdfs:comment """Inverse of 'is rule associated with' object
         property."""@en ;
    rdfs:domain :Thing ;
    rdfs:isDefinedBy <https://www.ica.org/standards/RiC/ontology> ;
    rdfs:label "est associé à la règle"@fr, "está asociado con regla"@es, "is associated with rule"@en ;
    rdfs:range :Rule ;
    rdfs:subPropertyOf :isRelatedTo ;
    owl:inverseOf :isRuleAssociatedWith ;
    owl:propertyChainAxiom (:thingIsTargetOfRelation
        :ruleRelation_role
        :relationHasSource
    ) ;
    skos:changeNote [
        dc:date "2023-11-08" ;
        rdf:value """In order to get a system of rolified Relation classes: modified
               the property chain axiom so that it now involves the new ruleRelation_role object
               property."""@en
    ], [
        dc:date "2023-11-02" ;
        rdf:value "Added a new rdfs:label in Spanish."@en
    ], [
        dc:date "2023-08-28" ;
        rdf:value "Added a new rdfs:label in French."@en
    ] ;
    :RiCCMCorrespondingComponent """RiC-R062i ('is associated with rule'
         relation)"""@en .

:isAuthorOf
    a owl:ObjectProperty ;
    rdfs:comment "Inverse of 'has author' object property."@en ;
    rdfs:domain [
        a owl:Class ;
        owl:unionOf (:Group
            :Person
            :Position
        )
    ] ;
    rdfs:isDefinedBy <https://www.ica.org/standards/RiC/ontology> ;
    rdfs:label "es autor(a) de"@es, "est le responsable intellectuel de"@fr, "is author of"@en ;
    rdfs:range :Record ;
    rdfs:subPropertyOf :isCreatorOf ;
    owl:inverseOf :hasAuthor ;
    owl:propertyChainAxiom (:thingIsTargetOfRelation
        :authorshipRelation_role
        :relationHasSource
    ) ;
    skos:changeNote [
        dc:date "2023-11-08" ;
        rdf:value """In order to get a system of rolified Relation classes: modified
               the property chain axiom so that it now involves the new authorshipRelation_role
               object property."""@en
    ], [
        dc:date "2023-11-02" ;
        rdf:value "Added a new rdfs:label in Spanish."@en
    ], [
        dc:date "2023-08-28" ;
        rdf:value "Added a new rdfs:label in French."@en
    ], [
        dc:date "2020-12-29" ;
        rdf:value """Created following the addition of RiC-R079 relation in RiC-CM
               0.2"""@en
    ] ;
    :RiCCMCorrespondingComponent """RiC-R079i ('is author of'
         relation)"""@en .

:isAuthorizingAgentInMandateRelation
    a owl:ObjectProperty ;
    rdfs:comment """Connects an Agent that assigns the Mandate, to a Mandate
         Relation."""@en ;
    rdfs:domain :Agent ;
    rdfs:isDefinedBy <https://www.ica.org/standards/RiC/ontology> ;
    rdfs:label "es el agente autorizador en la relación normativa"@es, """est l’agent donnant l’autorisation dans la relation impliquant un
         mandat"""@fr, "is authorizing agent in mandate relation"@en ;
    rdfs:range :MandateRelation ;
    rdfs:subPropertyOf :thingIsContextOfRelation ;
    owl:inverseOf :authorizingAgent ;
    skos:changeNote [
        dc:date "2023-11-13" ;
        rdf:value """Added a new rdfs:label in French and fixed the Spanish
               label."""@en
    ], [
        dc:date "2023-11-02" ;
        rdf:value "Added a new rdfs:label in Spanish."@en
    ] .

:isBeginningDateOf
    a owl:ObjectProperty ;
    rdfs:comment """Connects a Date to a Thing that came into existence on that
         Date."""@en ;
    rdfs:domain :Date ;
    rdfs:isDefinedBy <https://www.ica.org/standards/RiC/ontology> ;
    rdfs:label "es fecha de inicio de"@es, "est la date de début de"@fr, "is beginning date of"@en ;
    rdfs:range :Thing ;
    rdfs:subPropertyOf :isDateAssociatedWith ;
    owl:inverseOf :hasBeginningDate ;
    skos:changeNote [
        dc:date "2023-11-02" ;
        rdf:value "Added a new rdfs:label in Spanish."@en
    ], [
        dc:date "2023-08-28" ;
        rdf:value "Added a new rdfs:label in French."@en
    ] ;
    :RiCCMCorrespondingComponent """RiC-R069 ('is beginning date of'
         relation)"""@en .

:isBirthDateOf
    a owl:ObjectProperty ;
    rdfs:comment """Connects a Date to a Person that was born on that
         Date."""@en ;
    rdfs:domain :Date ;
    rdfs:isDefinedBy <https://www.ica.org/standards/RiC/ontology> ;
    rdfs:label "es fecha de nacimiento de"@es, "est la date de naissance de"@fr, "is birth date of"@en ;
    rdfs:range :Person ;
    rdfs:subPropertyOf :isBeginningDateOf ;
    owl:inverseOf :hasBirthDate ;
    skos:changeNote [
        dc:date "2023-11-02" ;
        rdf:value "Added a new rdfs:label in Spanish."@en
    ], [
        dc:date "2023-08-28" ;
        rdf:value "Added a new rdfs:label in French."@en
    ] ;
    :RiCCMCorrespondingComponent """RiC-R070 ('is birth date of'
         relation)"""@en .

:isBirthPlaceOf
    a owl:ObjectProperty ;
    rdfs:comment """Connects a Place to a Person who was born in that
         Place."""@en ;
    rdfs:domain :Place ;
    rdfs:isDefinedBy <https://www.ica.org/standards/RiC/ontology> ;
    rdfs:label "es lugar de nacimiento de"@es, "est le lieu de naissance de"@fr, "is birth place of"@en ;
    rdfs:range :Person ;
    rdfs:subPropertyOf :isPlaceAssociatedWithAgent ;
    owl:inverseOf :hasBirthPlace ;
    skos:changeNote [
        dc:date "2023-11-27" ;
        rdf:value "Added a new rdfs:label in Spanish."@en
    ], [
        dc:date "2023-11-12" ;
        rdf:value "Updated the description (rdfs:comment)."@en
    ], [
        dc:date "2023-10-26" ;
        rdf:value "Fixed the range."@en
    ], [
        dc:date "2023-10-19" ;
        rdf:value "Added for RiC-O v1.0."@en
    ] .

:isCarrierTypeOf
    a owl:ObjectProperty ;
    rdfs:comment """Connects a Carrier Type to an Instantiation whose carrier it
         categorizes."""@en ;
    rdfs:domain :CarrierType ;
    rdfs:isDefinedBy <https://www.ica.org/standards/RiC/ontology> ;
    rdfs:label "es tipo de soporte de"@es, "est le type de support de"@fr, "is carrier type of"@en ;
    rdfs:range :Instantiation ;
    rdfs:subPropertyOf :isOrWasTypeOf ;
    owl:inverseOf :hasCarrierType ;
    skos:changeNote [
        dc:date "2023-11-02" ;
        rdf:value "Added a new rdfs:label in Spanish."@en
    ], [
        dc:date "2023-08-28" ;
        rdf:value "Added a new rdfs:label in French."@en
    ], [
        dc:date "2021-01-22" ;
        rdf:value "Changed the super property IRI."@en
    ] .

:isChildOf
    a owl:ObjectProperty ;
    rdfs:comment "Inverse of 'has child' object property."@en ;
    rdfs:domain :Person ;
    rdfs:isDefinedBy <https://www.ica.org/standards/RiC/ontology> ;
    rdfs:label "es hijo o hija de"@es, "est l’enfant de"@fr, "is child of"@en ;
    rdfs:range :Person ;
    rdfs:subPropertyOf :hasAncestor ;
    owl:inverseOf :hasChild ;
    owl:propertyChainAxiom (:thingIsTargetOfRelation
        :childRelation_role
        :relationHasSource
    ) ;
    skos:changeNote [
        dc:date "2023-11-08" ;
        rdf:value """In order to get a system of rolified Relation classes: modified
               the property chain axiom so that it now involves the new childRelation_role object
               property."""@en
    ], [
        dc:date "2023-11-07" ;
        rdf:value """Added the property chain axiom so that this property is
               formally defined as a shortcut (the inverse property already was)."""@en
    ], [
        dc:date "2023-11-02" ;
        rdf:value "Added a new rdfs:label in Spanish."@en
    ], [
        dc:date "2023-08-28" ;
        rdf:value "Added a new rdfs:label in French."@en
    ], [
        dc:date "2021-01-22" ;
        rdf:value """changed the IRI and label (changed made in order to make RiC-O
               compliant with RiC-CM 0.2; the name of this property in RiC-O 0.1 was
               \"hasParent\")."""@en
    ] ;
    :RiCCMCorrespondingComponent """RiC-R018i ('is child of'
         relation)"""@en .

:isCollectorOf
    a owl:ObjectProperty ;
    rdfs:comment "Inverse of 'has collector' object property."@en ;
    rdfs:domain :Agent ;
    rdfs:isDefinedBy <https://www.ica.org/standards/RiC/ontology> ;
    rdfs:label "collecte"@fr, "es coleccionista de"@es, "is collector of"@en ;
    rdfs:range [
        a owl:Class ;
        owl:unionOf (:Instantiation
            :RecordResource
        )
    ] ;
    rdfs:subPropertyOf :isAccumulatorOf ;
    owl:inverseOf :hasCollector ;
    skos:changeNote [
        dc:date "2023-11-02" ;
        rdf:value "Added a new rdfs:label in Spanish."@en
    ], [
        dc:date "2023-08-28" ;
        rdf:value "Added a new rdfs:label in French."@en
    ], [
        dc:date "2021-01-22" ;
        rdf:value """changed the IRI, label, inverse property and super property
               IRI, text definition, domain (changed made in order to make RiC-O compliant with
               RiC-CM 0.2; the name of this property in RiC-O 0.1 was \"collects\")."""@en
    ] ;
    :RiCCMCorrespondingComponent """RiC-R030i ('is collector of'
         relation)"""@en .

:isComponentOfTransitive
    a owl:ObjectProperty, owl:TransitiveProperty ;
    rdfs:comment """Connects an Instantiation to another Instantiation of which it is,
         directly or indirectly, a component. This is a transitive relation."""@en ;
    rdfs:domain :Instantiation ;
    rdfs:isDefinedBy <https://www.ica.org/standards/RiC/ontology> ;
    rdfs:label "es componente de transitivo"@es, "est un composant de transitif"@fr, "is component of transitive"@en ;
    rdfs:range :Instantiation ;
    rdfs:subPropertyOf :isOrWasComponentOf, :isPartOfTransitive ;
    owl:inverseOf :hasComponentTransitive ;
    skos:changeNote [
        dc:date "2023-11-27" ;
        rdf:value "Added a new rdfs:label in Spanish."@en
    ], [
        dc:date "2023-11-12" ;
        rdf:value "Updated the labels."@en
    ], [
        dc:date "2023-09-08" ;
        rdf:value """Object property added, along with its inverse property, in
               order to enable to express current partitive relations between instantiations (the
               past partitive relation also being added)."""@en
    ] .

:isConstituentOfProxy
    a owl:ObjectProperty ;
    rdfs:comment """Connects a Record or Record Part to a Proxy of a Record or Record
         Part of which it is a constituent, directly or indirectly."""@en ;
    rdfs:domain [
        a owl:Class ;
        owl:unionOf (:Record
            :RecordPart
        )
    ] ;
    rdfs:isDefinedBy <https://www.ica.org/standards/RiC/ontology> ;
    rdfs:label "es elemento constitutivo del proxy"@es, "est le constituant du proxy"@fr, "is constituent of proxy"@en ;
    rdfs:range :Proxy ;
    rdfs:subPropertyOf :isPartOfTransitive ;
    owl:inverseOf :proxyHasConstituent ;
    owl:propertyChainAxiom (:isConstituentOfProxy
        :proxyIsConstituentOfProxyTransitive
    ) ;
    skos:changeNote [
        dc:date "2025-04-02" ;
        rdf:value "Added the French and Spanish labels."@en
    ], [
        dc:date "2025-03-04" ;
        rdf:value "Introduced in RiC-O 1.1."@en
    ] .

:isConstituentOfTransitive
    a owl:ObjectProperty, owl:TransitiveProperty ;
    rdfs:comment """Connects a Record or Record Part to another Record or Record Part
         of which it is a constituent, directly or indirectly. This is a transitive
         relation."""@en ;
    rdfs:domain [
        a owl:Class ;
        owl:unionOf (:Record
            :RecordPart
        )
    ] ;
    rdfs:isDefinedBy <https://www.ica.org/standards/RiC/ontology> ;
    rdfs:label "es elemento constitutivo de transitivo"@es, "est le constituant de transitif"@fr, "is constituent of transitive"@en ;
    rdfs:range [
        a owl:Class ;
        owl:unionOf (:Record
            :RecordPart
        )
    ] ;
    rdfs:subPropertyOf :isOrWasConstituentOf, :isPartOfTransitive ;
    owl:inverseOf :hasConstituentTransitive ;
    owl:propertyChainAxiom (:hasProxy
        :proxyInRecord
    ), (:isConstituentOfProxy
        :proxyIsConstituentOf
    ) ;
    skos:changeNote [
        dc:date "2025-03-04" ;
        rdf:value """Added two property chain axioms relating it to use of
               rico:Proxy."""@en
    ], [
        dc:date "2023-11-27" ;
        rdf:value "Added a new rdfs:label in Spanish."@en
    ], [
        dc:date "2023-11-12" ;
        rdf:value "Updated the labels."@en
    ], [
        dc:date "2023-10-26" ;
        rdf:value "Added RecordPart to the range."@en
    ], [
        dc:date "2023-09-08" ;
        rdf:value """Object property added, along with its inverse property, in
               order to enable to express current partitive relations between records and other
               records or record parts (the past partitive relation also being added)."""@en
    ] .

:isContainedByTransitive
    a owl:ObjectProperty, owl:TransitiveProperty ;
    rdfs:comment """Connects a Place to a Place that is, directly or indirectly,
         contained by it. This is a transitive relation."""@en ;
    rdfs:domain :Place ;
    rdfs:isDefinedBy <https://www.ica.org/standards/RiC/ontology> ;
    rdfs:label "est contenu par transitif"@fr, "está contenido en transitivo"@es, "is contained by transitive"@en ;
    rdfs:range :Place ;
    rdfs:subPropertyOf :isOrWasContainedBy, :isPartOfTransitive ;
    owl:inverseOf :containsTransitive ;
    skos:changeNote [
        dc:date "2023-11-27" ;
        rdf:value "Added a new rdfs:label in Spanish."@en
    ], [
        dc:date "2023-11-12" ;
        rdf:value "Updated the labels."@en
    ], [
        dc:date "2023-09-08" ;
        rdf:value """Object property added, along with its inverse property, in
               order to enable to express current partitive relations between places (the past
               partitive relation also being added)."""@en
    ] .

:isContentTypeOf
    a owl:ObjectProperty ;
    rdfs:comment """Connects a Content Type to a Record or Record Part whose content
         it categorizes."""@en ;
    rdfs:domain :ContentType ;
    rdfs:isDefinedBy <https://www.ica.org/standards/RiC/ontology> ;
    rdfs:label "es tipo de contenido de"@es, "est le type de contenu de"@fr, "is content type of"@en ;
    rdfs:range [
        a owl:Class ;
        owl:unionOf (:Record
            :RecordPart
        )
    ] ;
    rdfs:subPropertyOf :isOrWasTypeOf ;
    owl:inverseOf :hasContentOfType ;
    skos:changeNote [
        dc:date "2023-11-02" ;
        rdf:value "Added a new rdfs:label in Spanish."@en
    ], [
        dc:date "2023-08-28" ;
        rdf:value "Added a new rdfs:label in French."@en
    ], [
        dc:date "2021-01-22" ;
        rdf:value "changed the text definition and super property IRI."@en
    ] .

:isCopyOf
    a owl:ObjectProperty ;
    rdfs:comment "Inverse of 'has copy' object property."@en ;
    rdfs:domain :RecordResource ;
    rdfs:isDefinedBy <https://www.ica.org/standards/RiC/ontology> ;
    rdfs:label "es copia de"@es, "est la copie de"@fr, "is copy of"@en ;
    rdfs:range :RecordResource ;
    rdfs:subPropertyOf :followsInTime, :hasGeneticLinkToRecordResource ;
    owl:inverseOf :hasCopy ;
    skos:changeNote [
        dc:date "2023-11-02" ;
        rdf:value "Added a new rdfs:label in Spanish."@en
    ], [
        dc:date "2023-08-28" ;
        rdf:value "Added a new rdfs:label in French."@en
    ] ;
    :RiCCMCorrespondingComponent """RiC-R012i ('is copy of'
         relation)"""@en .

:isCreationDateOf
    a owl:ObjectProperty ;
    rdfs:comment """Connects a Date to a Record Resource or Instantiation that was or
         will be created at this Date."""@en ;
    rdfs:domain :Date ;
    rdfs:isDefinedBy <https://www.ica.org/standards/RiC/ontology> ;
    rdfs:label "es fecha de creación de"@es, "est la date de création de"@fr, "is creation date of"@en ;
    rdfs:range [
        a owl:Class ;
        owl:unionOf (:Instantiation
            :RecordResource
        )
    ] ;
    rdfs:subPropertyOf :isBeginningDateOf, :isOrganicProvenanceDateOf ;
    owl:inverseOf :hasCreationDate ;
    owl:propertyChainAxiom (:isDateAssociatedWithRelation
        :creationRelation_role
        :relationHasSource
    ) ;
    skos:changeNote [
        dc:date "2025-02-19" ;
        rdf:value "Changed definition (added \"or will be\")."@en
    ], [
        dc:date "2024-12-19" ;
        rdf:value """Connect to CreationRelation via a sub-property chain, and make
               a sub-property of the new 'isOrganicProvenanceDateOf' object property."""@en
    ], [
        dc:date "2023-11-27" ;
        rdf:value "Added a new rdfs:label in Spanish."@en
    ], [
        dc:date "2023-11-12" ;
        rdf:value """Aligned with RiC-CM 1.0: updated the
               skos:scopeNote."""@en
    ], [
        dc:date "2023-10-12" ;
        rdf:value "Added the French label"@en
    ], [
        dc:date "2023-09-22" ;
        rdf:value "Added in RiC-O 1.0."@en
    ] ;
    skos:scopeNote """When used for a Record Set (e.g. a file), it is the creation
         date of the Record Set itself rather than the creation date of the members of the Record
         Set. To record the creation date of members of the Record Set, use 'is or was creation date
         of all members of', 'is or was creation date of most members of’ or 'is or was creation
         date of some members of’."""@en ;
    :RiCCMCorrespondingComponent """RiC-R080 ('is creation date of'
         relation)"""@en .

:isCreatorOf
    a owl:ObjectProperty ;
    rdfs:comment "Inverse of 'has creator' object property."@en ;
    rdfs:domain :Agent ;
    rdfs:isDefinedBy <https://www.ica.org/standards/RiC/ontology> ;
    rdfs:label "es creador(a) de"@es, "est le créateur de"@fr, "is creator of"@en ;
    rdfs:range [
        a owl:Class ;
        owl:unionOf (:Instantiation
            :RecordResource
        )
    ] ;
    rdfs:subPropertyOf :isOrganicProvenanceOf ;
    owl:inverseOf :hasCreator ;
    owl:propertyChainAxiom (:thingIsTargetOfRelation
        :creationRelation_role
        :relationHasSource
    ) ;
    skos:changeNote [
        dc:date "2023-11-08" ;
        rdf:value """In order to get a system of rolified Relation classes: modified
               the property chain axiom so that it now involves the new creationRelation_role object
               property."""@en
    ], [
        dc:date "2023-11-02" ;
        rdf:value "Added a new rdfs:label in Spanish."@en
    ], [
        dc:date "2023-08-28" ;
        rdf:value "Added a new rdfs:label in French."@en
    ], [
        dc:date "2021-01-22" ;
        rdf:value "change the inverse property IRI."@en
    ] ;
    :RiCCMCorrespondingComponent """RiC-R027i ('is creator of
         'relation')"""@en .

:isDateAssociatedWith
    a owl:ObjectProperty ;
    rdfs:comment """Connects a Date to a Thing with whose existence and lifecycle the
         Date is associated."""@en ;
    rdfs:domain :Date ;
    rdfs:isDefinedBy <https://www.ica.org/standards/RiC/ontology> ;
    rdfs:label "es fecha asociada con"@es, "est une date associée a"@fr, "is date associated with"@en ;
    rdfs:range :Thing ;
    rdfs:subPropertyOf :isRelatedTo ;
    owl:inverseOf :isAssociatedWithDate ;
    skos:changeNote [
        dc:date "2023-11-12" ;
        rdf:value """Aligned with RiC-CM 1.0: updated the description
               (rdfs:comment), skos:scopeNote."""@en
    ], [
        dc:date "2023-11-02" ;
        rdf:value "Added a new rdfs:label in Spanish."@en
    ], [
        dc:date "2023-08-28" ;
        rdf:value "Added a new rdfs:label in French."@en
    ] ;
    skos:scopeNote """Use to connect a date and an entity only if it is not possible
         to specify a narrower date relation, for example, is beginning date of."""@en ;
    :RiCCMCorrespondingComponent """RiC-R068 ('is date associated with'
         relation)"""@en .

:isDateAssociatedWithRelation
    a owl:ObjectProperty ;
    rdfs:comment "Connects a Date to an n-ary Relation."@en ;
    rdfs:domain :Date ;
    rdfs:isDefinedBy <https://www.ica.org/standards/RiC/ontology> ;
    rdfs:label "es fecha asociada con la relación"@es, "est une date associée à la relation"@fr, "is date associated with Relation"@en ;
    rdfs:range :Relation ;
    rdfs:subPropertyOf :isDateAssociatedWith, :thingIsContextOfRelation ;
    owl:inverseOf :relationHasDate ;
    skos:changeNote [
        dc:date "2025-03-13" ;
        rdf:value """Added French and Spanish labels; fixed the first
               rdfs:subPropertyOf and the rdfs:domain."""@en
    ], [
        dc:date "2024-12-19" ;
        rdf:value "Added in RiC-O 1.1."@en
    ] .

:isDateOfOccurrenceOf
    a owl:ObjectProperty ;
    rdfs:comment """Connects a Date to an Event that occurred at this Date. An event
         or activity can be recurrent, which implies that one single event can be related to several
         dates."""@en ;
    rdfs:domain :Date ;
    rdfs:isDefinedBy <https://www.ica.org/standards/RiC/ontology> ;
    rdfs:label "es fecha de ocurrencia de"@es, "est la date d'occurrence de"@fr, "is date of occurrence of"@en ;
    rdfs:range :Event ;
    rdfs:subPropertyOf :isAssociatedWithEvent, :isDateAssociatedWith ;
    owl:inverseOf :occurredAtDate ;
    skos:changeNote [
        dc:date "2023-11-27" ;
        rdf:value "Added a new rdfs:label in Spanish."@en
    ], [
        dc:date "2023-10-17" ;
        rdf:value """Made this property a subproperty of
               isAssociatedWithEvent"""@en
    ], [
        dc:date "2023-10-13" ;
        rdf:value """Renamed the property to correct a spelling mistake. Also
               corrected the annotations when necessary."""@en
    ], [
        dc:date "2023-10-12" ;
        rdf:value "Added the property"@en
    ] ;
    :RiCCMCorrespondingComponent """RiC-R084 ('is date of occurrence of'
         relation)"""@en .

:isDateTypeOf
    a owl:ObjectProperty ;
    rdfs:comment "Connects a Date Type to a Date that it categorizes."@en ;
    rdfs:domain :DateType ;
    rdfs:isDefinedBy <https://www.ica.org/standards/RiC/ontology> ;
    rdfs:label "es tipo de fecha de"@es, "est le type de date de"@fr, "is date type of"@en ;
    rdfs:range :Date ;
    rdfs:subPropertyOf :isOrWasTypeOf ;
    owl:inverseOf :hasDateType ;
    skos:changeNote [
        dc:date "2023-11-27" ;
        rdf:value "Added a new rdfs:label in Spanish."@en
    ], [
        dc:date "2023-10-10" ;
        rdf:value "Added a rdfs:comment and a French rdfs:label."@en
    ], [
        dc:date "2023-09-22" ;
        rdf:value "Added in RiC-O 1.0."@en
    ] .

:isDeathDateOf
    a owl:ObjectProperty ;
    rdfs:comment "Connects a Date to a Person who died on that Date."@en ;
    rdfs:domain :Date ;
    rdfs:isDefinedBy <https://www.ica.org/standards/RiC/ontology> ;
    rdfs:label "es fecha de muerte de"@es, "est la date de décès de"@fr, "is death date of"@en ;
    rdfs:range :Person ;
    rdfs:subPropertyOf :isEndDateOf ;
    owl:inverseOf :hasDeathDate ;
    skos:changeNote [
        dc:date "2023-11-02" ;
        rdf:value "Added a new rdfs:label in Spanish."@en
    ], [
        dc:date "2023-08-28" ;
        rdf:value "Added a new rdfs:label in French."@en
    ] ;
    :RiCCMCorrespondingComponent """RiC-R072 ('is death date of'
         relation)"""@en .

:isDeathPlaceOf
    a owl:ObjectProperty ;
    rdfs:comment """Connects a Place to a Person who died in that
         Place."""@en ;
    rdfs:domain :Place ;
    rdfs:isDefinedBy <https://www.ica.org/standards/RiC/ontology> ;
    rdfs:label "es lugar de muerte de"@es, "est le lieu de décès de"@fr, "is death place of"@en ;
    rdfs:range :Person ;
    rdfs:subPropertyOf :isPlaceAssociatedWithAgent ;
    owl:inverseOf :hasDeathPlace ;
    skos:changeNote [
        dc:date "2023-11-27" ;
        rdf:value "Added a new rdfs:label in Spanish."@en
    ], [
        dc:date "2023-11-12" ;
        rdf:value "Updated the description (rdfs:comment)."@en
    ], [
        dc:date "2023-10-26" ;
        rdf:value """Fixed the range and the French label of the
               property."""@en
    ], [
        dc:date "2023-10-19" ;
        rdf:value "Property added to RiC-0 1.0"@en
    ] .

:isDerivationDateOf
    a owl:ObjectProperty ;
    rdfs:comment """Connects a Date to an Instantiation from which a new Instantiation
         was or will be derived at that Date."""@en ;
    rdfs:domain :Date ;
    rdfs:isDefinedBy <https://www.ica.org/standards/RiC/ontology> ;
    rdfs:label "es fecha de derivación de"@es, "est la date de dérivation de"@fr, "is derivation date of"@en ;
    rdfs:range :Instantiation ;
    rdfs:subPropertyOf :isDateAssociatedWith ;
    owl:inverseOf :hasDerivationDate ;
    owl:propertyChainAxiom (:isDateAssociatedWithRelation
        :derivationRelation_role
        :relationHasSource
    ) ;
    skos:changeNote [
        dc:date "2025-03-13" ;
        rdf:value "Added the property chain axiom."@en
    ], [
        dc:date "2025-03-01" ;
        rdf:value "Added in RiC-O 1.1."@en
    ] .

:isDestructionDateOf
    a owl:ObjectProperty ;
    rdfs:comment """Connects a Date to a Record Resource or Instantiation that was or
         will be destructed at that Date."""@en ;
    rdfs:domain :Date ;
    rdfs:isDefinedBy <https://www.ica.org/standards/RiC/ontology> ;
    rdfs:label "es fecha de destrucción de"@es, "est la date de destruction de"@fr, "is destruction date of"@en ;
    rdfs:range [
        a owl:Class ;
        owl:unionOf (:Instantiation
            :RecordResource
        )
    ] ;
    rdfs:subPropertyOf :isEndDateOf ;
    owl:inverseOf :hasDestructionDate ;
    skos:changeNote [
        dc:date "2025-02-19" ;
        rdf:value "Changed definition (added \"or will be\") and range."@en
    ], [
        dc:date "2023-11-27" ;
        rdf:value "Added a new rdfs:label in Spanish."@en
    ], [
        dc:date "2023-10-14" ;
        rdf:value "Added a rdfs:comment; same to the inverse property."@en
    ], [
        dc:date "2023-10-12" ;
        rdf:value "Renamed deletion into destruction."@en
    ], [
        dc:date "2023-09-22" ;
        rdf:value "Added in RiC-O 1.0."@en
    ] .

:isDirectComponentOf
    a owl:ObjectProperty ;
    rdfs:comment """Connects an Instantiation to another Instantiation of which it is
         a direct component."""@en ;
    rdfs:domain :Instantiation ;
    rdfs:isDefinedBy <https://www.ica.org/standards/RiC/ontology> ;
    rdfs:label "es componente directo de"@es, "est le composant direct de"@fr, "is direct component of"@en ;
    rdfs:range :Instantiation ;
    rdfs:subPropertyOf :isComponentOfTransitive, :isDirectPartOf ;
    owl:inverseOf :hasDirectComponent ;
    skos:changeNote [
        dc:date "2023-11-27" ;
        rdf:value "Added a new rdfs:label in Spanish."@en
    ], [
        dc:date "2023-11-12" ;
        rdf:value "Updated the labels."@en
    ], [
        dc:date "2023-09-08" ;
        skos:changeNote """Object property added, along with its inverse property,
               in order to enable to express current, direct, partitive relations between
               instantiations (the possibly indirect, transitive relation, superproperty of this
               one, being also added)."""@en
    ] .

:isDirectConstituentOf
    a owl:ObjectProperty ;
    rdfs:comment """Connects a Record or Record Part to another Record or Record Part
         of which it is a direct constituent."""@en ;
    rdfs:domain [
        a owl:Class ;
        owl:unionOf (:Record
            :RecordPart
        )
    ] ;
    rdfs:isDefinedBy <https://www.ica.org/standards/RiC/ontology> ;
    rdfs:label "es elemento constitutivo directo de"@es, "est un constituant direct de"@fr, "is direct constituent of"@en ;
    rdfs:range [
        a owl:Class ;
        owl:unionOf (:Record
            :RecordPart
        )
    ] ;
    rdfs:subPropertyOf :isConstituentOfTransitive, :isDirectPartOf ;
    owl:inverseOf :hasDirectConstituent ;
    owl:propertyChainAxiom (:isDirectConstituentOfProxy
        :proxyFor
    ) ;
    skos:changeNote [
        dc:date "2025-03-04" ;
        rdf:value """Added a property chain axiom relating it to use of
               rico:Proxy."""@en
    ], [
        dc:date "2023-11-27" ;
        rdf:value "Added a new rdfs:label in Spanish."@en
    ], [
        dc:date "2023-11-12" ;
        rdf:value "Updated the labels."@en
    ], [
        dc:date "2023-10-26" ;
        rdf:value "Added RecordPart to the range."@en
    ], [
        dc:date "2023-09-08" ;
        rdf:value """Object property added, along with its inverse property, in
               order to enable to express current, direct, partitive relations between records and
               other records or record parts (the possibly indirect, transitive relation,
               superproperty of this one, being also added)."""@en
    ] .

:isDirectConstituentOfProxy
    a owl:ObjectProperty ;
    rdfs:comment """Connects a Record or Record Part to a Proxy of a Record or Record
         Part which it is a direct constituent of."""@en ;
    rdfs:domain [
        a owl:Class ;
        owl:unionOf (:Record
            :RecordPart
        )
    ] ;
    rdfs:isDefinedBy <https://www.ica.org/standards/RiC/ontology> ;
    rdfs:label "es elemento constitutivo directo del proxy"@es, "est un constituant direct du proxy"@fr, "is direct constituent of proxy"@en ;
    rdfs:range :Proxy ;
    rdfs:subPropertyOf :isConstituentOfProxy, :isDirectPartOf ;
    owl:inverseOf :proxyHasDirectConstituent ;
    skos:changeNote [
        dc:date "2025-04-02" ;
        rdf:value "Added the French and Spanish labels."@en
    ], [
        dc:date "2025-03-04" ;
        rdf:value "Introduced in RiC-O 1.1."@en
    ] .

:isDirectPartOf
    a owl:ObjectProperty ;
    rdfs:comment """Connects a Thing to a Thing of which it is direct constitutive or
         component part."""@en ;
    rdfs:domain :Thing ;
    rdfs:isDefinedBy <https://www.ica.org/standards/RiC/ontology> ;
    rdfs:label "es parte directa de"@es, "fait directement partie de"@fr, "is direct part of"@en ;
    rdfs:range :Thing ;
    rdfs:subPropertyOf :isPartOfTransitive ;
    owl:inverseOf :hasDirectPart ;
    skos:changeNote [
        dc:date "2023-11-27" ;
        rdf:value "Added a new rdfs:label in Spanish."@en
    ], [
        dc:date "2023-11-12" ;
        rdf:value "Updated the labels."@en
    ], [
        dc:date "2023-07-12" ;
        rdf:value """Object property added, along with its inverse property, in
               order to enable to express current, direct, partitive relations between things (the
               possibly indirect, transitive relation, superproperty of this one, being also
               added)."""@en
    ] ;
    skos:scopeNote """To be used only when the current partitive relation is direct,
         without any intermediate node between the related things."""@en .

:isDirectSubdivisionOf
    a owl:ObjectProperty ;
    rdfs:comment """Connects a Group to the Group it is a direct subdivision
         of."""@en ;
    rdfs:domain :Group ;
    rdfs:isDefinedBy <https://www.ica.org/standards/RiC/ontology> ;
    rdfs:label "es subdivisión directa de"@es, "est la subdivision directe de"@fr, "is direct subdivision of"@en ;
    rdfs:range :Group ;
    rdfs:subPropertyOf :isDirectPartOf, :isDirectSubordinateTo, :isSubdivisionOfTransitive ;
    owl:inverseOf :hasDirectSubdivision ;
    skos:changeNote [
        dc:date "2023-11-27" ;
        rdf:value "Added a new rdfs:label in Spanish."@en
    ], [
        dc:date "2023-11-12" ;
        rdf:value "Updated the labels."@en
    ], [
        dc:date "2023-09-08" ;
        rdf:value """Object property added, along with its inverse property, in
               order to enable to express current, direct, partitive relations between groups (the
               possibly indirect, transitive relation, superproperty of this one, being also
               added)."""@en
    ] .

:isDirectSubeventOf
    a owl:ObjectProperty ;
    rdfs:comment """Connects an ongoing Event to the Event it is a direct part
         of."""@en ;
    rdfs:domain :Event ;
    rdfs:isDefinedBy <https://www.ica.org/standards/RiC/ontology> ;
    rdfs:label "es parte directa de evento de"@es, "est un événement constituant directement l’événement"@fr, "is direct subevent of"@en ;
    rdfs:range :Event ;
    rdfs:subPropertyOf :isDirectPartOf, :isSubeventOfTransitive ;
    owl:inverseOf :hasDirectSubevent ;
    skos:changeNote [
        dc:date "2023-11-27" ;
        rdf:value "Added a new rdfs:label in Spanish."@en
    ], [
        dc:date "2023-11-12" ;
        rdf:value "Updated the labels."@en
    ], [
        dc:date "2023-09-08" ;
        rdf:value """Object property added, along with its inverse property, in
               order to enable to express current, direct, partitive relations between ongoing
               events (the possibly indirect, transitive relation, superproperty of this one, being
               also added)."""@en
    ] .

:isDirectSubordinateTo
    a owl:ObjectProperty ;
    rdfs:comment """Connects an Agent to an Agent that is directly hierarchically
         superior."""@en ;
    rdfs:domain :Agent ;
    rdfs:isDefinedBy <https://www.ica.org/standards/RiC/ontology> ;
    rdfs:label "est directement subalterne de"@fr, "está directamente subordinado(a) a"@es, "is direct subordinate to"@en ;
    rdfs:range :Agent ;
    rdfs:subPropertyOf :isSubordinateToTransitive ;
    owl:inverseOf :hasDirectSubordinate ;
    skos:changeNote [
        dc:date "2023-11-27" ;
        rdf:value "Added a new rdfs:label in Spanish."@en
    ], [
        dc:date "2023-11-12" ;
        rdf:value "Updated the labels."@en
    ], [
        dc:date "2023-09-08" ;
        rdf:value """Object property added, along with its inverse property, in
               order to enable to express current, direct, subordination relations between agents
               (the possibly indirect, transitive relation, superproperty of this one, being also
               added)."""@en
    ] .

:isDirectlyContainedBy
    a owl:ObjectProperty ;
    rdfs:comment """Connects a Place to a Place that directly contains
         it."""@en ;
    rdfs:domain :Place ;
    rdfs:isDefinedBy <https://www.ica.org/standards/RiC/ontology> ;
    rdfs:label "est directement contenu par"@fr, "está directamente contenido en"@es, "is directly contained by"@en ;
    rdfs:range :Place ;
    rdfs:subPropertyOf :isContainedByTransitive, :isDirectPartOf ;
    owl:inverseOf :directlyContains ;
    skos:changeNote [
        dc:date "2023-11-27" ;
        rdf:value "Added a new rdfs:label in Spanish."@en
    ], [
        dc:date "2023-11-12" ;
        rdf:value "Updated the labels."@en
    ], [
        dc:date "2023-09-08" ;
        rdf:value """Object property added, along with its inverse property, in
               order to enable to express current, direct, partitive relations between places (the
               possibly indirect, transitive relation, superproperty of this one, being also
               added)."""@en
    ] .

:isDirectlyIncludedIn
    a owl:ObjectProperty ;
    rdfs:comment """Connects a Record to a Record or Record Set in which it is
         directly included."""@en ;
    rdfs:domain [
        a owl:Class ;
        owl:unionOf (:Record
            :RecordSet
        )
    ] ;
    rdfs:isDefinedBy <https://www.ica.org/standards/RiC/ontology> ;
    rdfs:label "est directement inclus dans"@fr, "está directamente incluido en"@es, "is directly included in"@en ;
    rdfs:range :RecordSet ;
    rdfs:subPropertyOf :isDirectPartOf, :isIncludedInTransitive ;
    owl:inverseOf :directlyIncludes ;
    skos:changeNote [
        dc:date "2023-11-27" ;
        rdf:value "Added a new rdfs:label in Spanish."@en
    ], [
        dc:date "2023-11-12" ;
        rdf:value "Updated the labels."@en
    ], [
        dc:date "2023-09-08" ;
        rdf:value """Object property added, along with its inverse property, in
               order to enable to express current, direct, partitive relations between Record Sets
               and their members (the possibly indirect, transitive relation, superproperty of this
               one, being also added)."""@en
    ] .

:isDirectlyIncludedInProxy
    a owl:ObjectProperty ;
    rdfs:comment """Connects a Record or Record Set to a Proxy of a Record Set which
         it is directly included in."""@en ;
    rdfs:domain [
        a owl:Class ;
        owl:unionOf (:Record
            :RecordSet
        )
    ] ;
    rdfs:isDefinedBy <https://www.ica.org/standards/RiC/ontology> ;
    rdfs:label "est directement inclus dans le proxy"@fr, "está directamente incluido en el proxy"@es, "is directly included in proxy"@en ;
    rdfs:range :Proxy ;
    rdfs:subPropertyOf :isDirectPartOf, :isIncludedInProxy ;
    owl:inverseOf :proxyDirectlyIncludes ;
    skos:changeNote [
        dc:date "2025-04-02" ;
        rdf:value "Added the French and Spanish labels."@en
    ], [
        dc:date "2025-03-04" ;
        rdf:value "Introduced in RiC-O 1.1."@en
    ] .

:isDocumentaryFormTypeOf
    a owl:ObjectProperty ;
    rdfs:comment """Connects a Documentary Form Type to a Record or Record Part that
         it categorizes."""@en ;
    rdfs:domain :DocumentaryFormType ;
    rdfs:isDefinedBy <https://www.ica.org/standards/RiC/ontology> ;
    rdfs:label "es tipo documental de"@es, "est le type de document de"@fr, "is documentary form type of"@en ;
    rdfs:range [
        a owl:Class ;
        owl:unionOf (:Record
            :RecordPart
        )
    ] ;
    rdfs:subPropertyOf :isOrWasTypeOf ;
    owl:inverseOf :hasDocumentaryFormType ;
    skos:changeNote [
        dc:date "2023-11-02" ;
        rdf:value "Added a new rdfs:label in Spanish."@en
    ], [
        dc:date "2023-08-28" ;
        rdf:value "Added a new rdfs:label in French."@en
    ], [
        dc:date "2021-01-22" ;
        rdf:value "changed the superproperty IRI."@en
    ] .

:isDraftOf
    a owl:ObjectProperty ;
    rdfs:comment "Connects a draft to the final version of a Record."@en ;
    rdfs:domain [
        a owl:Class ;
        owl:unionOf (:Record
            :RecordPart
        )
    ] ;
    rdfs:isDefinedBy <https://www.ica.org/standards/RiC/ontology> ;
    rdfs:label "es borrador de"@es, "est l’ébauche de"@fr, "is draft of"@en ;
    rdfs:range [
        a owl:Class ;
        owl:unionOf (:Record
            :RecordPart
        )
    ] ;
    rdfs:subPropertyOf :hasGeneticLinkToRecordResource, :precedesInTime ;
    owl:inverseOf :hasDraft ;
    skos:changeNote [
        dc:date "2023-11-12" ;
        rdf:value """Aligned with RiC-CM 1.0: updated the
               skos:scopeNote."""@en
    ], [
        dc:date "2023-11-02" ;
        rdf:value "Added a new rdfs:label in Spanish."@en
    ], [
        dc:date "2023-08-28" ;
        rdf:value "Added a new rdfs:label in French."@en
    ] ;
    skos:scopeNote """There may be zero to many intermediate records, ignored or
         unknown, between the two connected Records."""@en ;
    :RiCCMCorrespondingComponent """RiC-R011 ('is draft of'
         relation)"""@en .

:isEndDateOf
    a owl:ObjectProperty ;
    rdfs:comment """Connects a Date to a Thing whose existence ended on that
         Date."""@en ;
    rdfs:domain :Date ;
    rdfs:isDefinedBy <https://www.ica.org/standards/RiC/ontology> ;
    rdfs:label "es fecha final de"@es, "est la date de fin de"@fr, "is end date of"@en ;
    rdfs:range :Thing ;
    rdfs:subPropertyOf :isDateAssociatedWith ;
    owl:inverseOf :hasEndDate ;
    skos:changeNote [
        dc:date "2023-11-02" ;
        rdf:value "Added a new rdfs:label in Spanish."@en
    ], [
        dc:date "2023-08-28" ;
        rdf:value "Added a new rdfs:label in French."@en
    ] ;
    :RiCCMCorrespondingComponent """RiC-R071 ('is end date of'
         relation)"""@en .

:isEquivalentTo
    a owl:ObjectProperty, owl:SymmetricProperty ;
    rdfs:comment "Connects two Things that are considered equivalent."@en ;
    rdfs:domain :Thing ;
    rdfs:isDefinedBy <https://www.ica.org/standards/RiC/ontology> ;
    rdfs:label "equivale a"@es, "est l’équivalent de"@fr, "is equivalent to"@en ;
    rdfs:range :Thing ;
    rdfs:subPropertyOf :isRelatedTo ;
    skos:changeNote [
        dc:date "2023-11-02" ;
        rdf:value "Added a new rdfs:label in Spanish."@en
    ], [
        dc:date "2023-08-28" ;
        rdf:value "Added a new rdfs:label in French."@en
    ] .

:isEventAssociatedWith
    a owl:ObjectProperty ;
    rdfs:comment """Connects an Event to a Thing that is associated with the existence
         and lifecycle of the Event."""@en ;
    rdfs:domain :Event ;
    rdfs:isDefinedBy <https://www.ica.org/standards/RiC/ontology> ;
    rdfs:label "es evento asociado con"@es, "est un événement associé a"@fr, "is event associated with"@en ;
    rdfs:range :Thing ;
    rdfs:subPropertyOf :isRelatedTo ;
    owl:inverseOf :isAssociatedWithEvent ;
    owl:propertyChainAxiom (:thingIsSourceOfRelation
        :eventRelation_role
        :relationHasTarget
    ) ;
    skos:changeNote [
        dc:date "2023-11-12" ;
        rdf:value """Aligned with RiC-CM 1.0: updated the
               skos:scopeNote."""@en
    ], [
        dc:date "2023-11-08" ;
        rdf:value """In order to get a system of rolified Relation classes: modified
               the property chain axiom so that it now involves the new eventRelation_role object
               property."""@en
    ], [
        dc:date "2023-11-02" ;
        rdf:value "Added a new rdfs:label in Spanish."@en
    ], [
        dc:date "2023-08-28" ;
        rdf:value "Added a new rdfs:label in French."@en
    ] ;
    skos:scopeNote """Use to connect an Event and an entity only if it is not possible
         to specify a narrower Event relation, for example has or had participant."""@en ;
    :RiCCMCorrespondingComponent """RiC-R057 ('is event associated with'
         relation)"""@en .

:isEventTypeOf
    a owl:ObjectProperty ;
    rdfs:comment """Connects an Event Type to an Event that it
         categorizes."""@en ;
    rdfs:domain :EventType ;
    rdfs:isDefinedBy <https://www.ica.org/standards/RiC/ontology> ;
    rdfs:label "es tipo de evento de"@es, "est le type d’événement de"@fr, "is event type of"@en ;
    rdfs:range :Event ;
    rdfs:subPropertyOf :isOrWasTypeOf ;
    owl:inverseOf :hasEventType ;
    skos:changeNote [
        dc:date "2024-03-15" ;
        rdf:value "Fixed typo in rdfs:comment"@en
    ], [
        dc:date "2023-11-02" ;
        rdf:value "Added a new rdfs:label in Spanish."@en
    ], [
        dc:date "2023-08-28" ;
        rdf:value "Added a new rdfs:label in French."@en
    ], [
        dc:date "2021-01-22" ;
        rdf:value "changed the superproperty IRI."@en
    ] .

:isEvidencedBy
    a owl:ObjectProperty ;
    rdfs:comment """Connects a Relation to a Record Resource that is used for proving
         is existence or describing it."""@en ;
    rdfs:domain :Relation ;
    rdfs:isDefinedBy <https://www.ica.org/standards/RiC/ontology> ;
    rdfs:label "est attestée par"@fr, "is evidenced by"@en, "se evidencia en"@es ;
    rdfs:range :RecordResource ;
    rdfs:subPropertyOf :relationConnects ;
    owl:inverseOf :evidences ;
    skos:changeNote [
        dc:date "2023-12-27" ;
        rdf:value """Renamed the object property (was 'has source') and reduced its
               domain to Relation (the domain was the union of Record Resource and Relation) and its
               range to Record Resource (the range was the union of Agent and Record Resource).
               Consequently updated the superproperty, the labels, and added a
               rico:RiCCMCorrespondingComponent. Same for the inverse object property."""@en
    ], [
        dc:date "2023-11-02" ;
        rdf:value "Added a new rdfs:label in Spanish."@en
    ], [
        dc:date "2023-08-28" ;
        rdf:value "Added a new rdfs:label in French."@en
    ] ;
    :RiCCMCorrespondingComponent """Object property implementation of RiC-RA05 (Source
         of Relation attribute)."""@en .

:isExtentOf
    a owl:ObjectProperty ;
    rdfs:comment "Connects an Extent to a Thing"@en ;
    rdfs:domain :Extent ;
    rdfs:isDefinedBy <https://www.ica.org/standards/RiC/ontology> ;
    rdfs:label "es extensión de"@es, "est la mesure de"@fr, "is extent of"@en ;
    rdfs:range :Thing ;
    rdfs:subPropertyOf :isRelatedTo ;
    owl:inverseOf :hasExtent ;
    skos:changeNote [
        dc:date "2023-11-08" ;
        rdf:value "Fixed the range."@en
    ], [
        dc:date "2023-11-02" ;
        rdf:value "Added a new rdfs:label in Spanish."@en
    ], [
        dc:date "2023-08-28" ;
        rdf:value """Added a new rdfs:label in French; added an xml:lang attribute
               to the rdfs:comment."""@en
    ], [
        dc:date "2023-08-28" ;
        rdf:value """Changed the range (was Instantiation or RecordResource) to
               Thing ; changed the definition accordingly"""@en
    ], [
        dc:date "2020-10-28" ;
        rdf:value """Object property created along with the Extent class and its
               subclasses, in order to provide methods for handling extent accurately."""@en
    ] .

:isExtentTypeOf
    a owl:ObjectProperty ;
    rdfs:comment """Connects an Extent Type to an Extent that it
         categorizes."""@en ;
    rdfs:domain :ExtentType ;
    rdfs:isDefinedBy <https://www.ica.org/standards/RiC/ontology> ;
    rdfs:label "es tipo de extensión de"@es, "est le type de mesure de"@fr, "is extent type of"@en ;
    rdfs:range :Extent ;
    rdfs:subPropertyOf :isOrWasTypeOf ;
    owl:inverseOf :hasExtentType ;
    skos:changeNote [
        dc:date "2023-11-02" ;
        rdf:value "Added a new rdfs:label in Spanish."@en
    ], [
        dc:date "2023-08-28" ;
        rdf:value "Added a new rdfs:label in French."@en
    ], [
        dc:date "2020-11-21" ;
        rdf:value "Added a rdfs:comment."@en
    ], [
        dc:date "2020-11-01" ;
        rdf:value """Object property added along with the Extent Type
               class."""@en
    ] .

:isFamilyTypeOf
    a owl:ObjectProperty ;
    rdfs:comment """Connects a Family Type to a Family that it
         categorizes."""@en ;
    rdfs:domain :FamilyType ;
    rdfs:isDefinedBy <https://www.ica.org/standards/RiC/ontology> ;
    rdfs:label "es tipo de familia de"@es, "est le type de famille de"@fr, "is family type of"@en ;
    rdfs:range :Family ;
    rdfs:subPropertyOf :isOrWasTypeOf ;
    owl:inverseOf :hasFamilyType ;
    skos:changeNote [
        dc:date "2024-03-15" ;
        rdf:value "Fixed typo in rdfs:comment"@en
    ], [
        dc:date "2023-11-02" ;
        rdf:value "Added a new rdfs:label in Spanish."@en
    ], [
        dc:date "2023-08-28" ;
        rdf:value "Added a new rdfs:label in French."@en
    ], [
        dc:date "2021-01-22" ;
        rdf:value "changed the superproperty IRI."@en
    ] .

:isFromUseDateOf
    a owl:ObjectProperty ;
    rdfs:comment """Connects a Date to an Appellation, when it is the date at which
         the Appellation was first used."""@en ;
    rdfs:domain :Date ;
    rdfs:isDefinedBy <https://www.ica.org/standards/RiC/ontology> ;
    rdfs:label "es fecha desde la que se usa de"@es, "est la date à partir de laquelle est utilisé"@fr, "is from use date of"@en ;
    rdfs:range :Appellation ;
    rdfs:subPropertyOf :isBeginningDateOf ;
    owl:inverseOf :wasUsedFromDate ;
    skos:changeNote [
        dc:date "2023-11-02" ;
        rdf:value "Added a new rdfs:label in Spanish."@en
    ], [
        dc:date "2023-10-19" ;
        rdf:value "Made this property subPropertyOf isBeginningDateOf."@en
    ], [
        dc:date "2023-08-28" ;
        rdf:value "Added a new rdfs:label in French."@en
    ] .

:isFunctionallyEquivalentTo
    a owl:ObjectProperty, owl:SymmetricProperty ;
    rdfs:comment """Connects two Instantiations which may be considered as equivalent.
         This relation is symmetric."""@en ;
    rdfs:domain :Instantiation ;
    rdfs:isDefinedBy <https://www.ica.org/standards/RiC/ontology> ;
    rdfs:label "equivale funcionalmente a"@es, "est fonctionnellement équivalente à"@fr, "is functionally equivalent to"@en ;
    rdfs:range :Instantiation ;
    rdfs:subPropertyOf :isEquivalentTo, :isInstantiationAssociatedWithInstantiation ;
    owl:propertyChainAxiom (:thingIsConnectedToRelation
        :functionalEquivalenceRelation_role
        :relationConnects
    ) ;
    skos:changeNote [
        dc:date "2023-11-08" ;
        rdf:value """In order to get a system of rolified Relation classes: modified
               the property chain axiom so that it now involves the new
               functionalEquivalenceRelation_role object property."""@en
    ], [
        dc:date "2023-11-02" ;
        rdf:value "Added a new rdfs:label in Spanish."@en
    ], [
        dc:date "2023-08-28" ;
        rdf:value "Added a new rdfs:label in French."@en
    ], [
        dc:date "2021-01-22" ;
        rdf:value "changed the scope note."@en
    ] ;
    skos:scopeNote """Two Instantiations, from some point of view, may be considered
         as equivalent. This equivalence is usually based upon the fact that the Instantiations have
         at least the same intellectual content (they instantiate the same Record
         Resource)."""@en ;
    :RiCCMCorrespondingComponent """RiC-R035 ('is functionally equivalent to'
         relation)"""@en .

:isIdentifierTypeOf
    a owl:ObjectProperty ;
    rdfs:comment """Connects an Identifier Type and an Identifier that it
         categorizes."""@en ;
    rdfs:domain :IdentifierType ;
    rdfs:isDefinedBy <https://www.ica.org/standards/RiC/ontology> ;
    rdfs:label "es tipo de identificador de"@es, "est le type d’identifiant de"@fr, "is identifier type of"@en ;
    rdfs:range :Identifier ;
    rdfs:subPropertyOf :isOrWasTypeOf ;
    owl:inverseOf :hasIdentifierType ;
    skos:changeNote [
        dc:date "2023-11-02" ;
        rdf:value "Added a new rdfs:label in Spanish."@en
    ], [
        dc:date "2023-08-28" ;
        rdf:value "Added a new rdfs:label in French."@en
    ], [
        dc:date "2021-01-22" ;
        rdf:value "changed the superproperty IRI."@en
    ], [
        dc:date "2020-10-19" ;
        rdf:value """Object property added along with IdentifierType class and
               hasIdentifierType object property. """@en
    ] .

:isIncludedInProxy
    a owl:ObjectProperty ;
    rdfs:comment """Connects a Record or Record Set to a Proxy of a Record Set which
         it is included in, directly or indirectly."""@en ;
    rdfs:domain [
        a owl:Class ;
        owl:unionOf (:Record
            :RecordSet
        )
    ] ;
    rdfs:isDefinedBy <https://www.ica.org/standards/RiC/ontology> ;
    rdfs:label "est inclus dans le proxy"@fr, "está incluido en el proxy"@es, "is included in proxy"@en ;
    rdfs:range :Proxy ;
    rdfs:subPropertyOf :isPartOfTransitive ;
    owl:inverseOf :proxyIncludes ;
    owl:propertyChainAxiom (:isIncludedInProxy
        :proxyIsIncludedInProxyTransitive
    ) ;
    skos:changeNote [
        dc:date "2025-04-02" ;
        rdf:value "Added the French and Spanish labels."@en
    ], [
        dc:date "2025-03-04" ;
        rdf:value "Introduced in RiC-O 1.1."@en
    ] .

:isIncludedInTransitive
    a owl:ObjectProperty, owl:TransitiveProperty ;
    rdfs:comment """Connects a Record to a Record or Record Set in which it is
         directly or indirectly included. This is a transitive relation."""@en ;
    rdfs:domain [
        a owl:Class ;
        owl:unionOf (:Record
            :RecordSet
        )
    ] ;
    rdfs:isDefinedBy <https://www.ica.org/standards/RiC/ontology> ;
    rdfs:label "est inclus dans transitif"@fr, "está incluido en transitivo"@es, "is included in transitive"@en ;
    rdfs:range :RecordSet ;
    rdfs:subPropertyOf :isOrWasIncludedIn, :isPartOfTransitive ;
    owl:inverseOf :includesTransitive ;
    owl:propertyChainAxiom (:hasProxy
        :proxyInRecordSet
    ), (:isIncludedInProxy
        :proxyIsIncludedIn
    ) ;
    skos:changeNote [
        dc:date "2025-03-04" ;
        rdf:value """Added two property chain axioms relating it to use of
               rico:Proxy."""@en
    ], [
        dc:date "2023-11-27" ;
        rdf:value "Added a new rdfs:label in Spanish."@en
    ], [
        dc:date "2023-11-13" ;
        rdf:value "Added a French label."@en
    ], [
        dc:date "2023-09-08" ;
        rdf:value """Object property added, along with its inverse property, in
               order to enable to express current partitive relations between Record Sets and their
               members (the past partitive relation also being added)."""@en
    ] .

:isInstantiationAssociatedWithInstantiation
    a owl:ObjectProperty, owl:SymmetricProperty ;
    rdfs:comment """Connects two Instantiations. This relation is
         symmetric."""@en ;
    rdfs:domain :Instantiation ;
    rdfs:isDefinedBy <https://www.ica.org/standards/RiC/ontology> ;
    rdfs:label "est associée à l’instanciation"@fr, "is instantiation associated with instantiation"@en, "se asocia con la instanciación"@es ;
    rdfs:range :Instantiation ;
    rdfs:subPropertyOf :isRelatedTo ;
    owl:propertyChainAxiom (:thingIsConnectedToRelation
        :instantiationToInstantiationRelation_role
        :relationConnects
    ) ;
    skos:changeNote [
        dc:date "2023-11-12" ;
        rdf:value """Aligned with RiC-CM 1.0: updated the description
               (rdfs:comment), skos:scopeNote."""@en
    ], [
        dc:date "2023-11-08" ;
        rdf:value """In order to get a system of rolified Relation classes: modified
               the property chain axiom so that it now involves the new
               instantiationToInstantiationRelation_role object property."""@en
    ], [
        dc:date "2023-11-02" ;
        rdf:value "Added a new rdfs:label in Spanish."@en
    ], [
        dc:date "2023-08-28" ;
        rdf:value "Added a new rdfs:label in French."@en
    ] ;
    skos:scopeNote """Use only if it is not possible to specify a narrower
         Instantiation to Instantiation relation, for example is functionally equivalent
         to."""@en ;
    :RiCCMCorrespondingComponent """RiC-R034 ('is instantiation associated with
         instantiation' relation)"""@en .

:isLastUpdateDateOf
    a owl:ObjectProperty ;
    rdfs:comment """Connects a Date and a Thing that was last modified at this
         Date."""@en ;
    rdfs:domain :Date ;
    rdfs:isDefinedBy <https://www.ica.org/standards/RiC/ontology> ;
    rdfs:label "es fecha de última actualización de"@es, "est la date de dernière mise à jour de"@fr, "is last update date of"@en ;
    rdfs:range :Thing ;
    rdfs:subPropertyOf :isModificationDateOf ;
    owl:inverseOf :wasLastUpdatedAtDate ;
    skos:changeNote [
        dc:date "2023-11-02" ;
        rdf:value "Added a new rdfs:label in Spanish."@en
    ], [
        dc:date "2023-08-28" ;
        rdf:value "Added a new rdfs:label in French."@en
    ] .

:isMainThingRepresentedByContentOf
    a owl:ObjectProperty ;
    rdfs:comment """Inverse of 'has content which mainly represents' object
         property."""@en ;
    rdfs:domain :Thing ;
    rdfs:isDefinedBy <https://www.ica.org/standards/RiC/ontology> ;
    rdfs:label "es lo principal representado por el contenido de"@es, "est la chose principale représentée par le contenu de"@fr, "is main thing represented by content of"@en ;
    rdfs:range [
        a owl:Class ;
        owl:unionOf (:Record
            :RecordPart
        )
    ] ;
    rdfs:subPropertyOf :isOrWasMainSubjectOf, :isRepresentedByContentOf ;
    owl:inverseOf :hasContentWhichMainlyRepresents ;
    skos:changeNote [
        dc:date "2025-04-04" ;
        rdf:value "Introduced in RiC-O 1.1."@en
    ] .

:isMigrationDateOf
    a owl:ObjectProperty ;
    rdfs:comment """Connects a Date to an Instantiation that was or will be migrated
         at that Date."""@en ;
    rdfs:domain :Date ;
    rdfs:isDefinedBy <https://www.ica.org/standards/RiC/ontology> ;
    rdfs:label "es fecha de migración de"@es, "est la date de migration de"@fr, "is migration date of"@en ;
    rdfs:range :Instantiation ;
    rdfs:subPropertyOf :isDerivationDateOf ;
    owl:inverseOf :hasMigrationDate ;
    owl:propertyChainAxiom (:isDateAssociatedWithRelation
        :migrationRelation_role
        :relationHasSource
    ) ;
    skos:changeNote [
        dc:date "2025-03-13" ;
        rdf:value "Added the property chain axiom."@en
    ], [
        dc:date "2025-03-01" ;
        rdf:value """Removed 'Record Resource' from the definition and made this
               property a subproperty of the new 'isDerivationDateOf' property."""@en
    ], [
        dc:date "2025-02-19" ;
        rdf:value "Added in RiC-O 1.1."@en
    ] .

:isModificationDateOf
    a owl:ObjectProperty ;
    rdfs:comment """Connects a Date to a Thing that was modified on that
         Date."""@en ;
    rdfs:domain :Date ;
    rdfs:isDefinedBy <https://www.ica.org/standards/RiC/ontology> ;
    rdfs:label "es fecha de modificación de"@es, "est une date de modification de"@fr, "is modification date of"@en ;
    rdfs:range :Thing ;
    rdfs:subPropertyOf :isDateAssociatedWith ;
    owl:inverseOf :hasModificationDate ;
    skos:changeNote [
        dc:date "2023-11-02" ;
        rdf:value "Added a new rdfs:label in Spanish."@en
    ], [
        dc:date "2023-08-28" ;
        rdf:value "Added a new rdfs:label in French."@en
    ] ;
    :RiCCMCorrespondingComponent """RiC-R073 ('is modification date of'
         relation)"""@en .

:isOrWasAccumulationDateOfAllMembersOf
    a owl:ObjectProperty ;
    rdfs:comment """Connects a Date to a Record Set all of whose present or past
         members were or will be accumulated at this Date."""@en ;
    rdfs:domain :Date ;
    rdfs:isDefinedBy <https://www.ica.org/standards/RiC/ontology> ;
    rdfs:label "es o era fecha de acumulación de todos los miembros de"@es, """est ou a été la date de accumulation de tous les membres
         de"""@fr, "is or was accumulation date of all members of"@en ;
    rdfs:range :RecordSet ;
    rdfs:subPropertyOf :isDateAssociatedWith ;
    owl:inverseOf :hasOrHadAllMembersWithAccumulationDate ;
    skos:changeNote [
        dc:date "2025-02-19" ;
        rdf:value "Changed definition (added \"or will be\")."@en
    ], [
        dc:date "2024-10-04" ;
        rdf:value "Added in RiC-O 1.1."@en
    ] .

:isOrWasAccumulationDateOfMostMembersOf
    a owl:ObjectProperty ;
    rdfs:comment """Connects a Date to a Record Set most of whose present or past
         members were or will be accumulated at this Date."""@en ;
    rdfs:domain :Date ;
    rdfs:isDefinedBy <https://www.ica.org/standards/RiC/ontology> ;
    rdfs:label """es o era fecha de acumulación de la mayoría de los miembros
         de"""@es, """est ou a été la date d'accumulation de la plupart des membres
         de"""@fr, "is or was accumulation date of most members of"@en ;
    rdfs:range :RecordSet ;
    rdfs:subPropertyOf :isOrWasAccumulationDateOfSomeMembersOf ;
    owl:inverseOf :hasOrHadMostMembersWithAccumulationDate ;
    skos:changeNote [
        dc:date "2025-02-19" ;
        rdf:value "Changed definition (added \"or will be\")."@en
    ], [
        dc:date "2024-10-04" ;
        rdf:value "Added in RiC-O 1.1."@en
    ] ;
    skos:scopeNote """To be used for specifying a bulk date, i.e. the predominant date
         of the members of the record set."""@en .

:isOrWasAccumulationDateOfSomeMembersOf
    a owl:ObjectProperty ;
    rdfs:comment """Connects a Date to a Record Set some of whose present or past
         members were or will be accumulated at this Date."""@en ;
    rdfs:domain :Date ;
    rdfs:isDefinedBy <https://www.ica.org/standards/RiC/ontology> ;
    rdfs:label "es o era fecha de acumulación de algunos miembros de"@es, """est ou a été la date d'accumulation de certains membres
         de"""@fr, "is or was accumulation date of some members of"@en ;
    rdfs:range :RecordSet ;
    rdfs:subPropertyOf :isDateAssociatedWith ;
    owl:inverseOf :hasOrHadSomeMembersWithAccumulationDate ;
    skos:changeNote [
        dc:date "2025-02-19" ;
        rdf:value "Changed definition (added \"or will be\")."@en
    ], [
        dc:date "2024-10-04" ;
        rdf:value "Added in RiC-O 1.1."@en
    ] .

:isOrWasActiveAtDate
    a owl:ObjectProperty ;
    rdfs:comment """Inverse of 'is or was activity date of' object
         property."""@en ;
    rdfs:domain :Agent ;
    rdfs:isDefinedBy <https://www.ica.org/standards/RiC/ontology> ;
    rdfs:label "est ou a été actif à la date"@fr, "está o estuvo activo en la fecha"@es, "is or was active at date"@en ;
    rdfs:range :Date ;
    rdfs:subPropertyOf :isAssociatedWithDate ;
    owl:inverseOf :isOrWasActivityDateOf ;
    owl:propertyChainAxiom (:thingIsTargetOfRelation
        :performanceRelation_role
        :relationHasDate
    ) ;
    skos:changeNote [
        dc:date "2025-04-03" ;
        rdf:value """Adjusted the rdfs:comment and added French and Spanish
               labels."""@en
    ], [
        dc:date "2025-03-06" ;
        rdf:value "Introduced in RiC-O 1.1."@en
    ] .

:isOrWasActivityDateOf
    a owl:ObjectProperty ;
    rdfs:comment """Connects a Date to an Agent that is or was active at that
         Date."""@en ;
    rdfs:domain :Date ;
    rdfs:isDefinedBy <https://www.ica.org/standards/RiC/ontology> ;
    rdfs:label "es o era fecha de actividad de"@es, "est ou a été la date d’activité de"@fr, "is or was date of activity of"@en ;
    rdfs:range :Agent ;
    rdfs:subPropertyOf :isDateAssociatedWith ;
    owl:inverseOf :isOrWasActiveAtDate ;
    owl:propertyChainAxiom (:isDateAssociatedWithRelation
        :performanceRelation_role
        :relationHasTarget
    ) ;
    skos:changeNote [
        dc:date "2025-04-03" ;
        rdf:value """Renamed the property, changed its rdfs:comment, added the
               property chain axiom and French and Spanish labels."""@en
    ], [
        dc:date "2025-03-06" ;
        rdf:value "Introduced in RiC-O 1.1."@en
    ] .

:isOrWasAdjacentTo
    a owl:ObjectProperty, owl:SymmetricProperty ;
    rdfs:comment """Connects two Places that are or were geographically adjacent. This
         relation is symmetric."""@en ;
    rdfs:domain :Place ;
    rdfs:isDefinedBy <https://www.ica.org/standards/RiC/ontology> ;
    rdfs:label "es o era un lugar contiguo a"@es, "est ou a été adjacent à"@fr, "is or was adjacent to"@en ;
    rdfs:range :Place ;
    rdfs:subPropertyOf :isAssociatedWithPlace, :isPlaceAssociatedWith ;
    skos:changeNote [
        dc:date "2023-11-12" ;
        rdf:value """Aligned with RiC-CM 1.0: updated the description
               (rdfs:comment), skos:scopeNote."""@en
    ], [
        dc:date "2023-11-02" ;
        rdf:value "Added a new rdfs:label in Spanish."@en
    ], [
        dc:date "2023-08-28" ;
        rdf:value "Added a new rdfs:label in French."@en
    ], [
        dc:date "2021-01-22" ;
        rdf:value """changed the IRI, label, textual definition (changed made in
               order to make RiC-O compliant with RiC-CM 0.2; the name of this property in RiC-O 0.1
               was \"isAdjacentTo\")."""@en
    ] ;
    skos:scopeNote """Use for connecting two adjacent geographical or administrative
         regions."""@en ;
    :RiCCMCorrespondingComponent """RiC-R077 ('is or was adjacent to'
         relation)"""@en .

:isOrWasAffectedBy
    a owl:ObjectProperty ;
    rdfs:comment "Inverse of 'affects or affected' object property."@en ;
    rdfs:domain :Thing ;
    rdfs:isDefinedBy <https://www.ica.org/standards/RiC/ontology> ;
    rdfs:label "es o era afectado por"@es, "est ou a été affecté par"@fr, "is or was affected by"@en ;
    rdfs:range :Event ;
    rdfs:subPropertyOf :isOrWasParticipantIn ;
    owl:inverseOf :affectsOrAffected ;
    skos:changeNote [
        dc:date "2023-11-02" ;
        rdf:value "Added a new rdfs:label in Spanish."@en
    ], [
        dc:date "2023-08-28" ;
        rdf:value "Added a new rdfs:label in French."@en
    ], [
        dc:date "2021-01-22" ;
        rdf:value """changed the IRI, label, inverse property IRI, text definition
               and corresponding CM component (changed made in order to make RiC-O compliant with
               RiC-CM 0.2; the name of this property in RiC-O 0.1 was \"affectedBy\")."""@en
    ] ;
    :RiCCMCorrespondingComponent """RiC-R059i ('is or was affected by'
         relation)"""@en .

:isOrWasAgentNameOf
    a owl:ObjectProperty ;
    rdfs:comment """Connects an Agent Name to an Agent it designates or
         designated."""@en ;
    rdfs:domain :AgentName ;
    rdfs:isDefinedBy <https://www.ica.org/standards/RiC/ontology> ;
    rdfs:label "es o era el nombre de agente de"@es, "est ou a été le nom de"@fr, "is or was agent name of"@en ;
    rdfs:range :Agent ;
    rdfs:subPropertyOf :isOrWasNameOf ;
    owl:inverseOf :hasOrHadAgentName ;
    skos:changeNote [
        dc:date "2023-11-02" ;
        rdf:value "Added a new rdfs:label in Spanish."@en
    ], [
        dc:date "2023-08-28" ;
        rdf:value "Added a new rdfs:label in French."@en
    ], [
        dc:date "2021-01-22" ;
        rdf:value """changed the IRI, label, inverse property IRI, textual
               definition (the name of this property in RiC-O 0.1 was \"isAgentNameOf\")."""@en
    ] .

:isOrWasAnalogueInstantiationOf
    a owl:ObjectProperty ;
    rdfs:comment """Inverse of 'has or had analogue instantiation' object
         property."""@en ;
    rdfs:domain :Instantiation ;
    rdfs:isDefinedBy <https://www.ica.org/standards/RiC/ontology> ;
    rdfs:label "es or era instanciación analogica de"@es, "est ou a été une instanciation analogique de"@fr, "is or was analogue instantiation of"@en ;
    rdfs:range :RecordResource ;
    rdfs:subPropertyOf :isOrWasInstantiationOf ;
    owl:inverseOf :hasOrHadAnalogueInstantiation ;
    skos:changeNote [
        dc:date "2023-12-30" ;
        rdf:value "Fixed a typo in the French label."@en
    ], [
        dc:date "2023-11-27" ;
        rdf:value "Added a new rdfs:label in Spanish."@en
    ], [
        dc:date "2023-08-29" ;
        rdf:value "Added the property."@en
    ] .

:isOrWasAppellationOf
    a owl:ObjectProperty ;
    rdfs:comment """Connects an Appellation to a Thing that it designates or
         designated."""@en ;
    rdfs:domain :Appellation ;
    rdfs:isDefinedBy <https://www.ica.org/standards/RiC/ontology> ;
    rdfs:label "es o era la denominación de"@es, "est ou a été l’appellation de"@fr, "is or was appellation of"@en ;
    rdfs:range :Thing ;
    rdfs:subPropertyOf :isRelatedTo ;
    owl:inverseOf :hasOrHadAppellation ;
    owl:propertyChainAxiom (:thingIsSourceOfRelation
        :appellationRelation_role
        :relationHasTarget
    ) ;
    skos:changeNote [
        dc:date "2023-11-08" ;
        rdf:value """In order to get a system of rolified Relation classes: modified
               the property chain axiom so that it now involves the new appellationRelation_role
               object property."""@en
    ], [
        dc:date "2023-11-07" ;
        rdf:value """Added the property chain axiom so that this property is
               formally defined as a shortcut (the inverse property already was)."""@en
    ], [
        dc:date "2023-11-02" ;
        rdf:value "Added a new rdfs:label in Spanish."@en
    ], [
        dc:date "2023-08-28" ;
        rdf:value "Added a new rdfs:label in French."@en
    ], [
        dc:date "2021-01-22" ;
        rdf:value """changed the IRI, label, inverse property IRI, text definition
               (the name of this property in RiC-O 0.1 was \"isAppellationOf\")."""@en
    ] .

:isOrWasAttendedByStudent
    a owl:ObjectProperty ;
    rdfs:comment "Inverse of 'studies or studied at' object property."@en ;
    rdfs:domain :Group ;
    rdfs:isDefinedBy <https://www.ica.org/standards/RiC/ontology> ;
    rdfs:label "es o fue atendido por el estudiante"@es, "est ou a été fréquenté par l’étudiant"@fr, "is or was attended by student"@en ;
    rdfs:range :Person ;
    rdfs:subPropertyOf :hasOrHadMember ;
    owl:inverseOf :studiesOrStudiedAt ;
    owl:propertyChainAxiom (:thingIsSourceOfRelation
        :studyAtRelation_role
        :relationHasTarget
    ) ;
    skos:changeNote [
        dc:date "2024-12-23" ;
        rdf:value "Added the French and Spanish labels."@en
    ], [
        dc:date "2024-12-19" ;
        rdf:value "Added in RiC-O 1.1."@en
    ] .

:isOrWasComponentOf
    a owl:ObjectProperty ;
    rdfs:comment "Inverse of 'has or had component' object property."@en ;
    rdfs:domain :Instantiation ;
    rdfs:isDefinedBy <https://www.ica.org/standards/RiC/ontology> ;
    rdfs:label "es o era componente de"@es, "est ou a été un composant de"@fr, "is or was component of"@en ;
    rdfs:range :Instantiation ;
    rdfs:subPropertyOf :isInstantiationAssociatedWithInstantiation, :isOrWasPartOf ;
    owl:inverseOf :hasOrHadComponent ;
    skos:changeNote [
        dc:date "2023-11-02" ;
        rdf:value "Added a new rdfs:label in Spanish."@en
    ], [
        dc:date "2023-08-28" ;
        rdf:value "Added a new rdfs:label in French."@en
    ], [
        dc:date "2021-01-22" ;
        rdf:value """changed the IRI, label, inverse property IRI, text definition
               (changed made in order to make RiC-O compliant with RiC-CM 0.2; the name of this
               property in RiC-O 0.1 was \"isComponentOf\")."""@en
    ] ;
    :RiCCMCorrespondingComponent """RiC-R004i ('is or was component of'
         relation)"""@en .

:isOrWasConstituentOf
    a owl:ObjectProperty ;
    rdfs:comment """Inverse of 'has or had constituent' object
         property."""@en ;
    rdfs:domain [
        a owl:Class ;
        owl:unionOf (:Record
            :RecordPart
        )
    ] ;
    rdfs:isDefinedBy <https://www.ica.org/standards/RiC/ontology> ;
    rdfs:label "es o era elemento constitutivo de"@es, "est ou a été un constituant de"@fr, "is or was constituent of"@en ;
    rdfs:range [
        a owl:Class ;
        owl:unionOf (:Record
            :RecordPart
        )
    ] ;
    rdfs:subPropertyOf :isOrWasPartOf, :isRecordResourceAssociatedWithRecordResource ;
    owl:inverseOf :hasOrHadConstituent ;
    skos:changeNote [
        dc:date "2023-11-02" ;
        rdf:value "Added a new rdfs:label in Spanish."@en
    ], [
        dc:date "2023-10-26" ;
        rdf:value "Added RecordPart to the range."@en
    ], [
        dc:date "2023-08-28" ;
        rdf:value "Added a new rdfs:label in French."@en
    ], [
        dc:date "2021-01-22" ;
        rdf:value """changed the IRI, label, inverse property IRI, text definition
               (changed made in order to make RiC-O compliant with RiC-CM 0.2; the name of this
               property in RiC-O 0.1 was \"isConstituentOf\")."""@en
    ] ;
    :RiCCMCorrespondingComponent """RiC-R003i ('is or was constituent of'
         relation)"""@en .

:isOrWasContainedBy
    a owl:ObjectProperty ;
    rdfs:comment "Inverse of 'contains or contained' object property."@en ;
    rdfs:domain :Place ;
    rdfs:isDefinedBy <https://www.ica.org/standards/RiC/ontology> ;
    rdfs:label "est ou a été contenu par"@fr, "está o estaba contenido en"@es, "is or was contained by"@en ;
    rdfs:range :Place ;
    rdfs:subPropertyOf :isAssociatedWithPlace, :isOrWasPartOf, :isPlaceAssociatedWith ;
    owl:inverseOf :containsOrContained ;
    skos:changeNote [
        dc:date "2023-11-02" ;
        rdf:value "Added a new rdfs:label in Spanish."@en
    ], [
        dc:date "2023-08-28" ;
        rdf:value "Added a new rdfs:label in French."@en
    ], [
        dc:date "2021-01-22" ;
        rdf:value """changed the IRI, label, inverse property IRI, text definition,
               corresponding CM component name (changed made in order to make RiC-O compliant with
               RiC-CM 0.2; the name of this property in RiC-O 0.1 was \"containedBy\")."""@en
    ] ;
    :RiCCMCorrespondingComponent """RiC-R007i ('is or was contained by'
         relation)"""@en .

:isOrWasContentTypeOfAllMembersOf
    a owl:ObjectProperty ;
    rdfs:comment """Connects a Content Type and a Record Set whose all past or present
         Record or Record Part members have that Content Type."""@en ;
    rdfs:domain :ContentType ;
    rdfs:isDefinedBy <https://www.ica.org/standards/RiC/ontology> ;
    rdfs:label "es o era tipo de contenido de todos los miembros de"@es, "est ou a été le type de contenu de tous les membres de"@fr, "is or was content type of all members of"@en ;
    rdfs:range :RecordSet ;
    rdfs:subPropertyOf :isOrWasTypeOfAllMembersOf ;
    owl:inverseOf :hasOrHadAllMembersWithContentType ;
    skos:changeNote [
        dc:date "2023-11-02" ;
        rdf:value "Added a new rdfs:label in Spanish."@en
    ], [
        dc:date "2023-08-28" ;
        rdf:value "Added a new rdfs:label in French."@en
    ], [
        dc:date "2020-12-28" ;
        rdf:value """Object property added for handling the case where a Record Set
               is described as having all or some members that belong to some category (see RiC-CM
               0.2 attributes section, #4.4 on Record Set, Record and Record Part
               attributes)."""@en
    ] .

:isOrWasContentTypeOfSomeMembersOf
    a owl:ObjectProperty ;
    rdfs:comment """Connects a Content Type and a Record Set whose some past or
         present Record or Record Part members have that Content Type."""@en ;
    rdfs:domain :ContentType ;
    rdfs:isDefinedBy <https://www.ica.org/standards/RiC/ontology> ;
    rdfs:label "es o era tipo de contenido de algunos miembros de"@es, "est ou a été le type de contenu de certains membres de"@fr, "is or was content type of some members of"@en ;
    rdfs:range :RecordSet ;
    rdfs:subPropertyOf :isOrWasTypeOfSomeMembersOf ;
    owl:inverseOf :hasOrHadSomeMembersWithContentType ;
    skos:changeNote [
        dc:date "2023-11-02" ;
        rdf:value "Added a new rdfs:label in Spanish."@en
    ], [
        dc:date "2023-08-28" ;
        rdf:value "Added a new rdfs:label in French."@en
    ], [
        dc:date "2020-12-28" ;
        rdf:value """Object property added for handling the case where a Record Set
               is described as having all or some members that belong to some category (see RiC-CM
               0.2 attributes section, #4.4 on Record Set, Record and Record Part
               attributes)."""@en
    ] .

:isOrWasControllerOf
    a owl:ObjectProperty ;
    rdfs:comment """Connects an Agent to another Agent it controls or
         controlled."""@en ;
    rdfs:domain :Agent ;
    rdfs:isDefinedBy <https://www.ica.org/standards/RiC/ontology> ;
    rdfs:label "contrôle ou a contrôlé"@fr, "es o era controlador de"@es, "is or was controller of"@en ;
    rdfs:range :Agent ;
    rdfs:subPropertyOf :hasOrHadAuthorityOver, :hasOrHadSubordinate ;
    owl:inverseOf :hasOrHadController ;
    owl:propertyChainAxiom (:thingIsSourceOfRelation
        :agentControlRelation_role
        :relationHasTarget
    ) ;
    skos:changeNote [
        dc:date "2024-09-02" ;
        rdf:value "Fixed the French label."@en
    ], [
        dc:date "2023-11-12" ;
        rdf:value """Aligned with RiC-CM 1.0: updated the description
               (rdfs:comment)."""@en
    ], [
        dc:date "2023-11-08" ;
        rdf:value """In order to get a system of rolified Relation classes: modified
               the property chain axiom so that it now involves the new agentControlRelation_role
               object property."""@en
    ], [
        dc:date "2023-11-02" ;
        rdf:value "Added a new rdfs:label in Spanish."@en
    ], [
        dc:date "2023-08-28" ;
        rdf:value "Added a new rdfs:label in French."@en
    ], [
        dc:date "2021-01-22" ;
        rdf:value """changed the IRI, label, inverse property IRI, text definition,
               corresponding CM component name (changed made in order to make RiC-O compliant with
               RiC-CM 0.2; the name of this property in RiC-O 0.1 was \"controls\")."""@en
    ] ;
    :RiCCMCorrespondingComponent """RiC-R041 ('is or was controller of'
         relation)"""@en .

:isOrWasCoordinatesOf
    a owl:ObjectProperty ;
    rdfs:comment """Connects an instance of Coordinates to a Physical Location it
         locates or located on earth, according to some reference system."""@en ;
    rdfs:domain :Coordinates ;
    rdfs:isDefinedBy <https://www.ica.org/standards/RiC/ontology> ;
    rdfs:label "is or was coordinates of"@en, "ont ou ont été les coordonnées de"@fr, "son o eran coordenadas de lugar de"@es ;
    rdfs:range :PhysicalLocation ;
    rdfs:subPropertyOf :isRelatedTo ;
    owl:inverseOf :hasOrHadCoordinates ;
    skos:changeNote [
        dc:date "2023-11-02" ;
        rdf:value "Added a new rdfs:label in Spanish."@en
    ], [
        dc:date "2023-08-28" ;
        rdf:value "Added a new rdfs:label in French."@en
    ], [
        dc:date "2021-01-22" ;
        rdf:value """changed the IRI, label, inverse property IRI, text definition
               (the name of this property in RiC-O 0.1 was \"isCoordinatesOf\")."""@en
    ] .

:isOrWasCorporateBodyTypeOf
    a owl:ObjectProperty ;
    rdfs:comment """Connects a Corporate Body Type to a Corporate Body that it
         categorizes or categorized."""@en ;
    rdfs:domain :CorporateBodyType ;
    rdfs:isDefinedBy <https://www.ica.org/standards/RiC/ontology> ;
    rdfs:label "es o era tipo de institución de"@es, "est ou a été le type de collectivité de"@fr, "is or was corporate body type of"@en ;
    rdfs:range :CorporateBody ;
    rdfs:subPropertyOf :isOrWasTypeOf ;
    owl:inverseOf :hasOrHadCorporateBodyType ;
    skos:changeNote [
        dc:date "2023-11-02" ;
        rdf:value "Added a new rdfs:label in Spanish."@en
    ], [
        dc:date "2023-08-28" ;
        rdf:value "Added a new rdfs:label in French."@en
    ], [
        dc:date "2021-01-22" ;
        rdf:value """changed the IRI, label, inverse property IRI, text definition
               (the name of this property in RiC-O 0.1 was \"isCorporateBodyTypeOf\")."""@en
    ] .

:isOrWasCreationDateOfAllMembersOf
    a owl:ObjectProperty ;
    rdfs:comment """Connects a Date to a Record Set all of whose present or past
         members were or will be created at this Date."""@en ;
    rdfs:domain :Date ;
    rdfs:isDefinedBy <https://www.ica.org/standards/RiC/ontology> ;
    rdfs:label "es o era fecha de creación de todos los miembros de"@es, "est ou a été la date de création de tous les membres de"@fr, "is or was creation date of all members of"@en ;
    rdfs:range :RecordSet ;
    rdfs:subPropertyOf :isBeginningDateOf ;
    owl:inverseOf :hasOrHadAllMembersWithCreationDate ;
    skos:changeNote [
        dc:date "2025-02-19" ;
        rdf:value "Changed definition (added \"or will be\")."@en
    ], [
        dc:date "2023-11-27" ;
        rdf:value "Added a new rdfs:label in Spanish."@en
    ], [
        dc:date "2023-10-13" ;
        rdf:value """renamed the property in order to take the past members of the
               record set into account. Adjusted the annotations accordingly."""@en
    ], [
        dc:date "2023-10-12" ;
        rdf:value "Added the French label"@en
    ], [
        dc:date "2023-09-22" ;
        rdf:value "Added in RiC-O 1.0."@en
    ] ;
    :RiCCMCorrespondingComponent """RiC-R081 ('is or was creation date of all members
         of' relation)"""@en .

:isOrWasCreationDateOfMostMembersOf
    a owl:ObjectProperty ;
    rdfs:comment """Connects a Date to a Record Set most of whose present or past
         members were or will be created at this Date."""@en ;
    rdfs:domain :Date ;
    rdfs:isDefinedBy <https://www.ica.org/standards/RiC/ontology> ;
    rdfs:label """es o era fecha de creación de la mayoría de los miembros
         de"""@es, """est ou a été la date de création de la plupart des membres
         de"""@fr, "is or was creation date of most members of"@en ;
    rdfs:range :RecordSet ;
    rdfs:subPropertyOf :isOrWasCreationDateOfSomeMembersOf ;
    owl:inverseOf :hasOrHadMostMembersWithCreationDate ;
    skos:changeNote [
        dc:date "2025-02-19" ;
        rdf:value "Changed definition (added \"or will be\")."@en
    ], [
        dc:date "2023-11-27" ;
        rdf:value "Added a new rdfs:label in Spanish."@en
    ], [
        dc:date "2023-10-13" ;
        rdf:value """Renamed the property in order to take the past members of the
               record set into account. Adjusted the annotations accordingly."""@en
    ], [
        dc:date "2023-10-12" ;
        rdf:value "Added the French label"@en
    ], [
        dc:date "2023-10-10" ;
        rdf:value """Made this property a subproperty of
               isCreationDateOfSomeMembersOf."""@en
    ], [
        dc:date "2023-09-22" ;
        rdf:value "Added in RiC-O 1.0."@en
    ] ;
    skos:scopeNote """To be used for specifying a bulk date, i.e. the predominant date
         of the members of the record set."""@en ;
    :RiCCMCorrespondingComponent """RiC-R083 ('is or was creation date of most members
         of' relation)"""@en .

:isOrWasCreationDateOfSomeMembersOf
    a owl:ObjectProperty ;
    rdfs:comment """Connects a Date to a Record Set some of whose present or past
         members were or will be created at this Date."""@en ;
    rdfs:domain :Date ;
    rdfs:isDefinedBy <https://www.ica.org/standards/RiC/ontology> ;
    rdfs:label "es o era fecha de creación de algunos miembros de"@es, "est ou a été la date de création de certains membres de"@fr, "is or was creation date of some members of"@en ;
    rdfs:range :RecordSet ;
    rdfs:subPropertyOf :isBeginningDateOf ;
    owl:inverseOf :hasOrHadSomeMembersWithCreationDate ;
    skos:changeNote [
        dc:date "2025-02-19" ;
        rdf:value "Changed definition (added \"or will be\")."@en
    ], [
        dc:date "2023-11-27" ;
        rdf:value "Added a new rdfs:label in Spanish."@en
    ], [
        dc:date "2023-10-13" ;
        rdf:value """Renamed the property in order to take the past members of the
               record set into account. Adjusted the annotations accordingly."""@en
    ], [
        dc:date "2023-10-12" ;
        rdf:value "Added the French label and the rdfs:comment"@en
    ], [
        dc:date "2023-09-22" ;
        rdf:value "Added in RiC-O 1.0."@en
    ] ;
    :RiCCMCorrespondingComponent """RiC-R082 ('is or was creation date of some members
         of' relation)"""@en .

:isOrWasDemographicGroupOf
    a owl:ObjectProperty ;
    rdfs:comment """Connects a Demographic Group to a Person or Group which belongs or
         belonged to it."""@en ;
    rdfs:domain :DemographicGroup ;
    rdfs:isDefinedBy <https://www.ica.org/standards/RiC/ontology> ;
    rdfs:label "es o era grupo demográfico de"@es, "est ou a été le groupe démographique de"@fr, "is or was demographic group of"@en ;
    rdfs:range [
        a owl:Class ;
        owl:unionOf (:Group
            :Person
        )
    ] ;
    rdfs:subPropertyOf :isOrWasTypeOf ;
    owl:inverseOf :hasOrHadDemographicGroup ;
    skos:changeNote [
        dc:date "2024-10-10" ;
        rdf:value """Changed the French label (replaced 'catégorie' with
               'groupe')."""@en
    ], [
        dc:date "2023-11-02" ;
        rdf:value "Added a new rdfs:label in Spanish."@en
    ], [
        dc:date "2023-08-28" ;
        rdf:value "Added a new rdfs:label in French."@en
    ], [
        dc:date "2021-01-22" ;
        rdf:value """changed the IRI, label, inverse property IRI, text definition,
               range (the name of this property in RiC-O 0.1 was
               \"isDemographicGroupOf\")."""@en
    ] .

:isOrWasDerivedFromInstantiation
    a owl:ObjectProperty ;
    rdfs:comment """Inverse of 'has or had derived instantiation' object
         property."""@en ;
    rdfs:domain :Instantiation ;
    rdfs:isDefinedBy <https://www.ica.org/standards/RiC/ontology> ;
    rdfs:label "es o era un derivado de instanciación"@es, "est ou a été une instanciation dérivée de"@fr, "is or was derived from instantiation"@en ;
    rdfs:range :Instantiation ;
    rdfs:subPropertyOf :followsInTime, :isInstantiationAssociatedWithInstantiation ;
    owl:inverseOf :hasOrHadDerivedInstantiation ;
    owl:propertyChainAxiom (:thingIsTargetOfRelation
        :derivationRelation_role
        :relationHasSource
    ) ;
    skos:changeNote [
        dc:date "2023-11-27" ;
        rdf:value "Added a new rdfs:label in Spanish."@en
    ], [
        dc:date "2023-11-08" ;
        rdf:value """In order to get a system of rolified Relation classes: modified
               the property chain axiom so that it now involves the new derivationRelation_role
               object property."""@en
    ], [
        dc:date "2023-11-07" ;
        rdf:value """Added the property chain axiom so that this property is
               formally defined as a shortcut (the inverse property already was)."""@en
    ], [
        dc:date "2023-08-29" ;
        rdf:value """Updated the IRI, inverse property, definition, labels and
               RiCMCorrespondingComponent; this in order to make the specification compliant with
               RiC-CM 1.0. The name of the property in RiC-O 0.2 was 'is derived from
               instantiation'."""@en
    ], [
        dc:date "2023-08-28" ;
        rdf:value "Added a new rdfs:label in French."@en
    ] ;
    :RiCCMCorrespondingComponent """RiC-R014i ('is or was derived from instantiation'
         relation)"""@en .

:isOrWasDescribedBy
    a owl:ObjectProperty ;
    rdfs:comment """Inverse of 'describes or described' object
         property."""@en ;
    rdfs:domain :Thing ;
    rdfs:isDefinedBy <https://www.ica.org/standards/RiC/ontology> ;
    rdfs:label "es o fue descrito por"@es, "est ou a été décrit par"@fr, "is or was described by"@en ;
    rdfs:range :RecordResource ;
    rdfs:subPropertyOf :isOrWasSubjectOf ;
    owl:inverseOf :describesOrDescribed ;
    skos:changeNote [
        dc:date "2023-11-02" ;
        rdf:value "Added a new rdfs:label in Spanish."@en
    ], [
        dc:date "2023-08-28" ;
        rdf:value "Added a new rdfs:label in French."@en
    ], [
        dc:date "2023-08-28" ;
        rdf:value "Added a new rdfs:label in French."@en
    ], [
        dc:date "2021-01-22" ;
        rdf:value """changed the IRI, label, inverse property IRI, text definition,
               corresponding CM component name (changed made in order to make RiC-O compliant with
               RiC-CM 0.2; the name of this property in RiC-O 0.1 was \"describedBy\")."""@en
    ] ;
    :RiCCMCorrespondingComponent """RiC-R021i ('is or was described by'
         relation)"""@en .

:isOrWasDigitalInstantiationOf
    a owl:ObjectProperty ;
    rdfs:comment """Inverse of 'has or had digital instantiation' object
         property."""@en ;
    rdfs:domain :Instantiation ;
    rdfs:isDefinedBy <https://www.ica.org/standards/RiC/ontology> ;
    rdfs:label "es o era instanciación digital de"@es, "est ou a été une instanciation numérique de"@fr, "is or was digital instantiation of"@en ;
    rdfs:range :RecordResource ;
    rdfs:subPropertyOf :isOrWasInstantiationOf ;
    owl:inverseOf :hasOrHadDigitalInstantiation ;
    skos:changeNote [
        dc:date "2023-11-27" ;
        rdf:value "Added a new rdfs:label in Spanish."@en
    ], [
        dc:date "2023-08-29" ;
        rdf:value "Added the property."@en
    ] .

:isOrWasDocumentaryFormTypeOfAllMembersOf
    a owl:ObjectProperty ;
    rdfs:comment """Connects a Documentary Form Type and a Record Set whose all past
         or present Record or Record Part members have that Documentary Form Type."""@en ;
    rdfs:domain :DocumentaryFormType ;
    rdfs:isDefinedBy <https://www.ica.org/standards/RiC/ontology> ;
    rdfs:label "es o era tipo documental de todos los miembros de"@es, "est ou a été le type de document de tous les membres de"@fr, "is or was documentary form type of all members of"@en ;
    rdfs:range :RecordSet ;
    rdfs:subPropertyOf :isOrWasTypeOfAllMembersOf ;
    owl:inverseOf :hasOrHadAllMembersWithDocumentaryFormType ;
    skos:changeNote [
        dc:date "2023-11-02" ;
        rdf:value "Added a new rdfs:label in Spanish."@en
    ], [
        dc:date "2023-08-28" ;
        rdf:value "Added a new rdfs:label in French."@en
    ], [
        dc:date "2020-12-28" ;
        rdf:value """Object property added for handling the case where a Record Set
               is described as having all or some members that belong to some category (see RiC-CM
               0.2 attributes section, #4.4 on Record Set, Record and Record Part
               attributes)."""@en
    ] .

:isOrWasDocumentaryFormTypeOfSomeMembersOf
    a owl:ObjectProperty ;
    rdfs:comment """Connects a Documentary Form Type and a Record Set whose some past
         or present Record or Record Part members have that Documentary Form Type."""@en ;
    rdfs:domain :DocumentaryFormType ;
    rdfs:isDefinedBy <https://www.ica.org/standards/RiC/ontology> ;
    rdfs:label "es o era tipo documental de algunos miembros de"@es, "est ou a été le type de document de certains membres de"@fr, "is or was documentary form type of some members of"@en ;
    rdfs:range :RecordSet ;
    rdfs:subPropertyOf :isOrWasTypeOfSomeMembersOf ;
    owl:inverseOf :hasOrHadSomeMembersWithDocumentaryFormType ;
    skos:changeNote [
        dc:date "2023-11-02" ;
        rdf:value "Added a new rdfs:label in Spanish."@en
    ], [
        dc:date "2023-08-28" ;
        rdf:value "Added a new rdfs:label in French."@en
    ], [
        dc:date "2020-12-28" ;
        rdf:value """Object property added for handling the case where a Record Set
               is described as having all or some members that belong to some category (see RiC-CM
               0.2 attributes section, #4.4 on Record Set, Record and Record Part
               attributes)."""@en
    ] .

:isOrWasEmployerOf
    a owl:ObjectProperty ;
    rdfs:comment """Connects a Corporate Body or a Person to a Person who is or was
         their employee."""@en ;
    rdfs:domain [
        a owl:Class ;
        owl:unionOf (:CorporateBody
            :Person
        )
    ] ;
    rdfs:isDefinedBy <https://www.ica.org/standards/RiC/ontology> ;
    rdfs:label "a ou a été l'employeur de"@fr, "es o era empleador(a) de"@es, "is or was employer of"@en ;
    rdfs:range :Person ;
    rdfs:subPropertyOf :isOrWasControllerOf ;
    owl:inverseOf :hasOrHadEmployer ;
    skos:changeNote [
        dc:date "2023-11-27" ;
        rdf:value "Added a new rdfs:label in Spanish."@en
    ], [
        dc:date "2023-10-26" ;
        rdf:value """Changed the domain and range of the property. Added a
               rdfs:comment. Removed the 'has or had member' super-property."""@en
    ], [
        dc:date "2023-10-19" ;
        rdf:value "Adder for RiC-O v1.0."@en
    ] .

:isOrWasEnforcedBy
    a owl:ObjectProperty ;
    rdfs:comment """Connects a Rule to an Agent that enforces or enforced the
         Rule."""@en ;
    rdfs:domain :Rule ;
    rdfs:isDefinedBy <https://www.ica.org/standards/RiC/ontology> ;
    rdfs:label "es o era una regla aplicada por"@es, "est ou a été imposé par"@fr, "is or was enforced by"@en ;
    rdfs:range :Agent ;
    rdfs:subPropertyOf :isRuleAssociatedWith ;
    owl:inverseOf :isOrWasResponsibleForEnforcing ;
    skos:changeNote [
        dc:date "2024-09-02" ;
        rdf:value "Fixed the French label."@en
    ], [
        dc:date "2023-11-02" ;
        rdf:value "Added a new rdfs:label in Spanish."@en
    ], [
        dc:date "2023-08-28" ;
        rdf:value "Added a new rdfs:label in French."@en
    ], [
        dc:date "2021-01-22" ;
        rdf:value """changed the IRI, label, inverse property IRI, text definition,
               corresponding CM component name (changed made in order to make RiC-O compliant with
               RiC-CM 0.2; the name of this property in RiC-O 0.1 was \"enforcedBy\")."""@en
    ] ;
    :RiCCMCorrespondingComponent """RiC-R066 ('is or was enforced by'
         relation)"""@en .

:isOrWasExpressedBy
    a owl:ObjectProperty ;
    rdfs:comment """Connects a Rule to a Record Resource that expresses or expressed
         the Rule."""@en ;
    rdfs:domain :Rule ;
    rdfs:isDefinedBy <https://www.ica.org/standards/RiC/ontology> ;
    rdfs:label "es o era una regla expresada en"@es, "est ou a été exprimé par"@fr, "is or was expressed by"@en ;
    rdfs:range :RecordResource ;
    rdfs:subPropertyOf :isRuleAssociatedWith ;
    owl:inverseOf :expressesOrExpressed ;
    skos:changeNote [
        dc:date "2023-11-02" ;
        rdf:value "Added a new rdfs:label in Spanish."@en
    ], [
        dc:date "2023-08-28" ;
        rdf:value "Added a new rdfs:label in French."@en
    ], [
        dc:date "2021-01-22" ;
        rdf:value """changed the IRI, label, inverse property IRI, text definition,
               corresponding CM component name (changed made in order to make RiC-O compliant with
               RiC-CM 0.2; the name of this property in RiC-O 0.1 was \"expressedBy\")."""@en
    ] ;
    :RiCCMCorrespondingComponent """RiC-R064 ('is or was expressed by'
         relation)"""@en .

:isOrWasHolderOf
    a owl:ObjectProperty ;
    rdfs:comment """Connects an Agent to a Record Resource or Instantiation that the
         Agent holds or held."""@en ;
    rdfs:domain :Agent ;
    rdfs:isDefinedBy <https://www.ica.org/standards/RiC/ontology> ;
    rdfs:label "détient ou a détenu"@fr, "es o era conservador de"@es, "is or was holder of"@en ;
    rdfs:range [
        a owl:Class ;
        owl:unionOf (:Instantiation
            :RecordResource
        )
    ] ;
    rdfs:subPropertyOf :isOrWasManagerOf ;
    owl:inverseOf :hasOrHadHolder ;
    owl:propertyChainAxiom (:thingIsSourceOfRelation
        :recordResourceHoldingRelation_role
        :relationHasTarget
    ) ;
    skos:changeNote [
        dc:date "2023-11-08" ;
        rdf:value """In order to get a system of rolified Relation classes: modified
               the property chain axiom so that it now involves the new
               recordResourceHoldingRelation_role object property."""@en
    ], [
        dc:date "2023-11-02" ;
        rdf:value "Added a new rdfs:label in Spanish."@en
    ], [
        dc:date "2023-08-28" ;
        rdf:value "Added a new rdfs:label in French."@en
    ], [
        dc:date "2021-01-22" ;
        rdf:value """changed the IRI, label, inverse property IRI, super = property
               IRI and text definition (changed made in order to make RiC-O compliant with RiC-CM
               0.2; the name of this property in RiC-O 0.1 was \"isHolderOf\")."""@en
    ] ;
    :RiCCMCorrespondingComponent """RiC-R039 ('is or was holder of'
         relation)"""@en .

:isOrWasHolderOfIntellectualPropertyRightsOf
    a owl:ObjectProperty ;
    rdfs:comment """Connects an Agent to a Record Resource or Instantiation on which
         the Agent has or had some intellectual property rights."""@en ;
    rdfs:domain [
        a owl:Class ;
        owl:unionOf (:Group
            :Person
            :Position
        )
    ] ;
    rdfs:isDefinedBy <https://www.ica.org/standards/RiC/ontology> ;
    rdfs:label """détient ou a détenu les droits de propriété intellectuelle
         sur"""@fr, """es o era conservador de derechos de propiedad intelectual
         de"""@es, "is or was holder of intellectual property rights of"@en ;
    rdfs:range [
        a owl:Class ;
        owl:unionOf (:Instantiation
            :RecordResource
        )
    ] ;
    rdfs:subPropertyOf :hasOrHadAuthorityOver ;
    owl:inverseOf :hasOrHadIntellectualPropertyRightsHolder ;
    owl:propertyChainAxiom (:thingIsSourceOfRelation
        :intellectualPropertyRightsRelation_role
        :relationHasTarget
    ) ;
    skos:changeNote [
        dc:date "2023-11-08" ;
        rdf:value """In order to get a system of rolified Relation classes: modified
               the property chain axiom so that it now involves the new
               intellectualPropertyRightsRelation_role object property."""@en
    ], [
        dc:date "2023-11-02" ;
        rdf:value "Added a new rdfs:label in Spanish."@en
    ], [
        dc:date "2023-08-28" ;
        rdf:value "Added a new rdfs:label in French."@en
    ], [
        dc:date "2021-01-22" ;
        rdf:value """changed the IRI, label, inverse property IRI and textual
               definition (changed made in order to make RiC-O compliant with RiC-CM 0.2; the name
               of this property in RiC-O 0.1 was \"hasIntellectualPropertyRightsOn\")."""@en
    ] ;
    :RiCCMCorrespondingComponent """RiC-R040 ('is or was holder of intellectual
         property rights of' relation)"""@en .

:isOrWasIdentifierOf
    a owl:ObjectProperty ;
    rdfs:comment """Connects an Identifier to a Thing that it identified or
         identifies."""@en ;
    rdfs:domain :Identifier ;
    rdfs:isDefinedBy <https://www.ica.org/standards/RiC/ontology> ;
    rdfs:label "es o era identificador de"@es, "est ou a été l’identifiant de"@fr, "is or was identifier of"@en ;
    rdfs:range :Thing ;
    rdfs:subPropertyOf :isOrWasAppellationOf ;
    owl:inverseOf :hasOrHadIdentifier ;
    skos:changeNote [
        dc:date "2023-11-02" ;
        rdf:value "Added a new rdfs:label in Spanish."@en
    ], [
        dc:date "2023-08-28" ;
        rdf:value "Added a new rdfs:label in French."@en
    ], [
        dc:date "2021-01-22" ;
        rdf:value """changed the IRI, label, inverse property IRI, text definition,
               super property IRI (the name of this property in RiC-O 0.1 was
               \"identifies\")."""@en
    ] .

:isOrWasIncludedIn
    a owl:ObjectProperty ;
    rdfs:comment "Inverse of 'includes or included' object property."@en ;
    rdfs:domain [
        a owl:Class ;
        owl:unionOf (:Record
            :RecordSet
        )
    ] ;
    rdfs:isDefinedBy <https://www.ica.org/standards/RiC/ontology> ;
    rdfs:label "est ou a été inclus dans"@fr, "está o estaba incluido en"@es, "is or was included in"@en ;
    rdfs:range :RecordSet ;
    rdfs:subPropertyOf :isOrWasPartOf, :isRecordResourceAssociatedWithRecordResource ;
    owl:inverseOf :includesOrIncluded ;
    skos:changeNote [
        dc:date "2023-11-02" ;
        rdf:value "Added a new rdfs:label in Spanish."@en
    ], [
        dc:date "2023-08-28" ;
        rdf:value "Added a new rdfs:label in French."@en
    ], [
        dc:date "2023-06-05" ;
        rdf:value """Made this object property a subproperty of
               isOrWasPartOf."""@en
    ], [
        dc:date "2021-01-22" ;
        rdf:value """changed the IRI, label, inverse property IRI, text definition
               (changed made in order to make RiC-O compliant with RiC-CM 0.2; the name of this
               property in RiC-O 0.1 was \"includedIn\")."""@en
    ] ;
    :RiCCMCorrespondingComponent """RiC-R024i ('is or was included in'
         relation)"""@en .

:isOrWasInstantiationOf
    a owl:ObjectProperty ;
    rdfs:comment """Inverse of 'has or had instantiation' object
         property."""@en ;
    rdfs:domain :Instantiation ;
    rdfs:isDefinedBy <https://www.ica.org/standards/RiC/ontology> ;
    rdfs:label "es o era instanciación de"@es, "est ou a été une instanciation de"@fr, "is or was instantiation of"@en ;
    rdfs:range :RecordResource ;
    rdfs:subPropertyOf :isRelatedTo ;
    owl:inverseOf :hasOrHadInstantiation ;
    owl:propertyChainAxiom (:thingIsTargetOfRelation
        :recordResourceToInstantiationRelation_role
        :relationHasSource
    ) ;
    skos:changeNote [
        dc:date "2023-11-27" ;
        rdf:value "Added a new rdfs:label in Spanish."@en
    ], [
        dc:date "2023-11-08" ;
        rdf:value """In order to get a system of rolified Relation classes: modified
               the property chain axiom so that it now involves the new
               recordResourceToInstantiationRelation_role object property."""@en
    ], [
        dc:date "2023-08-29" ;
        rdf:value """Updated the IRI, inverse property, definition, labels and
               RiCMCorrespondingComponent; this in order to make the specification compliant with
               RiC-CM 1.0. The name of the property in RiC-O 0.2 was 'is instantiation
               of'."""@en
    ], [
        dc:date "2023-08-28" ;
        rdf:value "Added a new rdfs:label in French."@en
    ], [
        dc:date "2021-01-22" ;
        rdf:value """changed the IRI and label (changed made in order to make RiC-O
               compliant with RiC-CM 0.2; the name of this property in RiC-O 0.1 was
               \"instantiates\")."""@en
    ] ;
    :RiCCMCorrespondingComponent """RiC-R025i ('is or was instantiation of'
         relation)"""@en .

:isOrWasJurisdictionOf
    a owl:ObjectProperty ;
    rdfs:comment """Connects a Place to an Agent that has or had jurisdiction over the
         Place."""@en ;
    rdfs:domain :Place ;
    rdfs:isDefinedBy <https://www.ica.org/standards/RiC/ontology> ;
    rdfs:label "es o era jurisdicción de"@es, "est ou a été le ressort de"@fr, "is or was jurisdiction of"@en ;
    rdfs:range :Agent ;
    rdfs:subPropertyOf :isPlaceAssociatedWithAgent ;
    owl:inverseOf :hasOrHadJurisdiction ;
    skos:changeNote [
        dc:date "2024-09-02" ;
        rdf:value "Fixed the French label."@en
    ], [
        dc:date "2023-11-02" ;
        rdf:value "Added a new rdfs:label in Spanish."@en
    ], [
        dc:date "2023-10-19" ;
        rdf:value """Made subproperty of new property isPlaceAssociatedWithAgent
               instead of its parent isPlaceAssociatedWith."""@en
    ], [
        dc:date "2023-08-28" ;
        rdf:value "Added a new rdfs:label in French."@en
    ], [
        dc:date "2021-01-22" ;
        rdf:value """changed the IRI, label, inverse property IRI, textual
               definition (changed made in order to make RiC-O compliant with RiC-CM 0.2; the name
               of this property in RiC-O 0.1 was \"isJurisdictionOf\")."""@en
    ] ;
    :RiCCMCorrespondingComponent """RiC-R076 ('is or was jurisdiction of'
         relation)"""@en .

:isOrWasLanguageOf
    a owl:ObjectProperty ;
    rdfs:comment """Connects a Language to an Agent, Record or Record Part that uses
         or used it."""@en ;
    rdfs:domain :Language ;
    rdfs:isDefinedBy <https://www.ica.org/standards/RiC/ontology> ;
    rdfs:label "es o era lengua de"@es, "est ou a été la langue de"@fr, "is or was language of"@en ;
    rdfs:range [
        a owl:Class ;
        owl:unionOf (:Agent
            :Record
            :RecordPart
        )
    ] ;
    rdfs:subPropertyOf :isRelatedTo ;
    owl:inverseOf :hasOrHadLanguage ;
    skos:changeNote [
        dc:date "2023-11-02" ;
        rdf:value "Added a new rdfs:label in Spanish."@en
    ], [
        dc:date "2023-08-28" ;
        rdf:value "Added a new rdfs:label in French."@en
    ], [
        dc:date "2021-01-22" ;
        rdf:value """changed the IRI, label, inverse property IRI, textual
               definition (the name of this property in RiC-O 0.1 was \"isLanguageOf\")."""@en
    ] .

:isOrWasLanguageOfAllMembersOf
    a owl:ObjectProperty ;
    rdfs:comment """Connects a Language and a Record Set whose all present or past
         Record or Record Part members use that Language."""@en ;
    rdfs:domain :Language ;
    rdfs:isDefinedBy <https://www.ica.org/standards/RiC/ontology> ;
    rdfs:label "es o era lengua de todos los miembros de"@es, "est ou a été la langue de tous les membres de"@fr, "is or was language of all members of"@en ;
    rdfs:range :RecordSet ;
    rdfs:subPropertyOf :isRelatedTo ;
    owl:inverseOf :hasOrHadAllMembersWithLanguage ;
    skos:changeNote [
        dc:date "2023-11-02" ;
        rdf:value "Added a new rdfs:label in Spanish."@en
    ], [
        dc:date "2023-08-28" ;
        rdf:value "Added a new rdfs:label in French."@en
    ], [
        dc:date "2020-12-28" ;
        rdf:value """Object property added for handling the case where a Record Set
               is described as having all or some members that belong to some category (see RiC-CM
               0.2 attributes section, #4.4 on Record Set, Record and Record Part
               attributes)."""@en
    ] .

:isOrWasLanguageOfSomeMembersOf
    a owl:ObjectProperty ;
    rdfs:comment """Connects a Language and a Record Set whose some present or past
         Record or Record Part members use that Language."""@en ;
    rdfs:domain :Language ;
    rdfs:isDefinedBy <https://www.ica.org/standards/RiC/ontology> ;
    rdfs:label "es o era lengua de algunos miembros de"@es, "est ou a été la langue de certains membres de"@fr, "is or was language of some members of"@en ;
    rdfs:range :RecordSet ;
    rdfs:subPropertyOf :isRelatedTo ;
    owl:inverseOf :hasOrHadSomeMembersWithLanguage ;
    skos:changeNote [
        dc:date "2023-11-02" ;
        rdf:value "Added a new rdfs:label in Spanish."@en
    ], [
        dc:date "2023-08-28" ;
        rdf:value "Added a new rdfs:label in French."@en
    ], [
        dc:date "2020-12-28" ;
        rdf:value """Object property added for handling the case where a Record Set
               is described as having all or some members that belong to some category (see RiC-CM
               0.2 attributes section, #4.4 on Record Set, Record and Record Part
               attributes)."""@en
    ] .

:isOrWasLeaderOf
    a owl:ObjectProperty ;
    rdfs:comment """Connects a Person to the Group that Person leads or led in the
         past."""@en ;
    rdfs:domain :Person ;
    rdfs:isDefinedBy <https://www.ica.org/standards/RiC/ontology> ;
    rdfs:label "es o era líder de"@es, "est ou a été le dirigeant de"@fr, "is or was leader of"@en ;
    rdfs:range :Group ;
    rdfs:subPropertyOf :isOrWasControllerOf ;
    owl:inverseOf :hasOrHadLeader ;
    owl:propertyChainAxiom (:thingIsSourceOfRelation
        :leadershipRelation_role
        :relationHasTarget
    ) ;
    skos:changeNote [
        dc:date "2023-11-08" ;
        rdf:value """In order to get a system of rolified Relation classes: modified
               the property chain axiom so that it now involves the new leadershipRelation_role
               object property."""@en
    ], [
        dc:date "2023-11-02" ;
        rdf:value "Added a new rdfs:label in Spanish."@en
    ], [
        dc:date "2023-08-28" ;
        rdf:value "Added a new rdfs:label in French."@en
    ], [
        dc:date "2021-01-22" ;
        rdf:value """changed the IRI, label, inverse property IRI, super property
               IRI, textual definition (changed made in order to make RiC-O compliant with RiC-CM
               0.2; the name of this property in RiC-O 0.1 was \"isLeaderOf\")."""@en
    ] ;
    :RiCCMCorrespondingComponent """RiC-R042 ('is or was leader of'
         relation)"""@en .

:isOrWasLegalStatusOf
    a owl:ObjectProperty ;
    rdfs:comment """Connects a Legal Status to an Agent or Record Resource that it
         categorizes."""@en ;
    rdfs:domain :LegalStatus ;
    rdfs:isDefinedBy <https://www.ica.org/standards/RiC/ontology> ;
    rdfs:label "es o era status jurídico de"@es, "est ou a été le statut légal de"@fr, "is or was legal status of"@en ;
    rdfs:range [
        a owl:Class ;
        owl:unionOf (:Agent
            :Record
            :RecordPart
        )
    ] ;
    rdfs:subPropertyOf :isOrWasTypeOf ;
    owl:inverseOf :hasOrHadLegalStatus ;
    skos:changeNote [
        dc:date "2023-11-02" ;
        rdf:value "Added a new rdfs:label in Spanish."@en
    ], [
        dc:date "2023-08-28" ;
        rdf:value "Added a new rdfs:label in French."@en
    ], [
        dc:date "2021-01-22" ;
        rdf:value """changed the IRI, label, inverse property IRI, textual
               definition (the name of this property in RiC-O 0.1 was
               \"isLegalStatusOf\")."""@en
    ] ;
    skos:scopeNote """Connects a Legal Status to an Agent, Record or Record Part that
         it categorized or categorizes."""@en .

:isOrWasLegalStatusOfAllMembersOf
    a owl:ObjectProperty ;
    rdfs:comment """Connects a Legal Status and a Record Set whose all past or present
         Record or Record Part members have that Legal Status."""@en ;
    rdfs:domain :LegalStatus ;
    rdfs:isDefinedBy <https://www.ica.org/standards/RiC/ontology> ;
    rdfs:label "es o era status jurídico de todos los miembros de"@es, "est ou a été le statut légal de tous les membres de"@fr, "is or was legal status of all members of"@en ;
    rdfs:range :RecordSet ;
    rdfs:subPropertyOf :isOrWasTypeOfAllMembersOf ;
    owl:inverseOf :hasOrHadAllMembersWithLegalStatus ;
    skos:changeNote [
        dc:date "2023-11-02" ;
        rdf:value "Added a new rdfs:label in Spanish."@en
    ], [
        dc:date "2023-08-28" ;
        rdf:value "Added a new rdfs:label in French."@en
    ], [
        dc:date "2020-12-28" ;
        rdf:value """Object property added for handling the case where a Record Set
               is described as having all or some members that belong to some category (see RiC-CM
               0.2 attributes section, #4.4 on Record Set, Record and Record Part
               attributes)."""@en
    ] .

:isOrWasLegalStatusOfSomeMembersOf
    a owl:ObjectProperty ;
    rdfs:comment """Connects a Legal Status and a Record Set whose some past or
         present Record or Record Part members have that Legal Status."""@en ;
    rdfs:domain :LegalStatus ;
    rdfs:isDefinedBy <https://www.ica.org/standards/RiC/ontology> ;
    rdfs:label "es o era status jurídico de algunos miembros de"@es, "est ou a été le statut légal de certains membres de"@fr, "is or was legal status of some members of"@en ;
    rdfs:range :RecordSet ;
    rdfs:subPropertyOf :isOrWasTypeOfSomeMembersOf ;
    owl:inverseOf :hasOrHadSomeMembersWithLegalStatus ;
    skos:changeNote [
        dc:date "2023-11-02" ;
        rdf:value "Added a new rdfs:label in Spanish."@en
    ], [
        dc:date "2023-08-28" ;
        rdf:value "Added a new rdfs:label in French."@en
    ], [
        dc:date "2020-12-28" ;
        rdf:value """Object property added for handling the case where a Record Set
               is described as having all or some members that belong to some category (see RiC-CM
               0.2 attributes section, #4.4 on Record Set, Record and Record Part
               attributes)."""@en
    ] .

:isOrWasLocationOf
    a owl:ObjectProperty ;
    rdfs:comment """Connects a Place to a Thing that is or was located in the
         Place."""@en ;
    rdfs:domain :Place ;
    rdfs:isDefinedBy <https://www.ica.org/standards/RiC/ontology> ;
    rdfs:label "es o era localización de"@es, "est ou a été la localisation de"@fr, "is or was location of"@en ;
    rdfs:range :Thing ;
    rdfs:subPropertyOf :isPlaceAssociatedWith ;
    owl:inverseOf :hasOrHadLocation ;
    skos:changeNote [
        dc:date "2023-11-02" ;
        rdf:value "Added a new rdfs:label in Spanish."@en
    ], [
        dc:date "2023-08-28" ;
        rdf:value "Added a new rdfs:label in French."@en
    ], [
        dc:date "2021-01-22" ;
        rdf:value """changed the IRI, label, inverse property IRI, textual
               definition (changed made in order to make RiC-O compliant with RiC-CM 0.2; the name
               of this property in RiC-O 0.1 was \"isLocationOf\")."""@en
    ] ;
    :RiCCMCorrespondingComponent """RiC-R075 ('is or was location of'
         relation)"""@en .

:isOrWasLocationOfAgent
    a owl:ObjectProperty ;
    rdfs:comment """Connects a Place to an Agent that is or was located in this
         Place."""@en ;
    rdfs:domain :Place ;
    rdfs:isDefinedBy <https://www.ica.org/standards/RiC/ontology> ;
    rdfs:label "es o era localización de agente"@es, "est ou a été la localisation de l'agent"@fr, "is or was location of agent"@en ;
    rdfs:range :Agent ;
    rdfs:subPropertyOf :isOrWasLocationOf, :isPlaceAssociatedWithAgent ;
    owl:inverseOf :agentHasOrHadLocation ;
    skos:changeNote [
        dc:date "2023-11-27" ;
        rdf:value "Added a new rdfs:label in Spanish."@en
    ], [
        dc:date "2023-10-26" ;
        rdf:value "Renamed the property and added an rdfs:comment."@en
    ], [
        dc:date "2023-10-20" ;
        rdf:value "Added for RiC-O 1.0."@en
    ] .

:isOrWasMainSubjectOf
    a owl:ObjectProperty ;
    rdfs:comment """Inverse of 'has or had main subject' object
         property."""@en ;
    rdfs:domain :Thing ;
    rdfs:isDefinedBy <https://www.ica.org/standards/RiC/ontology> ;
    rdfs:label "es o era la materia principal de"@es, "est ou a été le sujet principal de"@fr, "is or was main subject of"@en ;
    rdfs:range :RecordResource ;
    rdfs:subPropertyOf :isOrWasSubjectOf ;
    owl:inverseOf :hasOrHadMainSubject ;
    skos:changeNote [
        dc:date "2023-11-02" ;
        rdf:value "Added a new rdfs:label in Spanish."@en
    ], [
        dc:date "2023-08-28" ;
        rdf:value "Added a new rdfs:label in French."@en
    ], [
        dc:date "2021-01-22" ;
        rdf:value """changed the IRI, label, inverse property IRI, super property
               IRI, textual definition (changed made in order to make RiC-O compliant with RiC-CM
               0.2; the name of this property in RiC-O 0.1 was \"isMainSubjectOf\")."""@en
    ] ;
    :RiCCMCorrespondingComponent """RiC-R020i ('is or was main subject of'
         relation)"""@en .

:isOrWasMainSubjectOfAllMembersOf
    a owl:ObjectProperty ;
    rdfs:comment """Inverse of 'has or had all members with main subject' object
         property."""@en ;
    rdfs:domain :Thing ;
    rdfs:isDefinedBy <https://www.ica.org/standards/RiC/ontology> ;
    rdfs:label "es o era la materia principal de todos los miembros de"@es, "est ou a été le sujet principal de tous les membres de"@fr, "is or was main subject of all members of"@en ;
    rdfs:range :RecordSet ;
    rdfs:subPropertyOf :isOrWasMainSubjectOf, :isOrWasSubjectOfAllMembersOf ;
    owl:inverseOf :hasOrHadAllMembersWithMainSubject ;
    skos:changeNote [
        dc:date "2025-04-05" ;
        rdf:value "Introduced in RiC-O 1.1."@en
    ] .

:isOrWasMainSubjectOfSomeMembersOf
    a owl:ObjectProperty ;
    rdfs:comment """Inverse of 'has or had some members with main subject' object
         property."""@en ;
    rdfs:domain :Thing ;
    rdfs:isDefinedBy <https://www.ica.org/standards/RiC/ontology> ;
    rdfs:label "es o era la materia principal de algunos miembros de"@es, "est ou a été le sujet principal de certains membres de"@fr, "is or was main subject of some members of"@en ;
    rdfs:range :RecordSet ;
    rdfs:subPropertyOf :isOrWasSubjectOfSomeMembersOf ;
    owl:inverseOf :hasOrHadSomeMembersWithMainSubject ;
    skos:changeNote [
        dc:date "2025-04-05" ;
        rdf:value "Introduced in RiC-O 1.1."@en
    ] .

:isOrWasMainThingRepresentedByContentOfSomeMembersOf
    a owl:ObjectProperty ;
    rdfs:comment """Inverse of 'has or had some members whose content mainly
         represents' object property."""@en ;
    rdfs:domain :Thing ;
    rdfs:isDefinedBy <https://www.ica.org/standards/RiC/ontology> ;
    rdfs:label """es o era lo principal representado por el contenido de algunos
         miembros de"""@es, """est ou a été la chose principale représentée par le contenu de
         certains membres de"""@fr, """is or was main thing represented by content of some members
         of"""@en ;
    rdfs:range :RecordSet ;
    rdfs:subPropertyOf :isOrWasMainSubjectOfSomeMembersOf, :isOrWasRepresentedByContentOfSomeMembersOf ;
    owl:inverseOf :hasOrHadSomeMembersWhoseContentMainlyRepresents ;
    skos:changeNote [
        dc:date "2025-04-06" ;
        rdf:value "Introduced in RiC-O 1.1."@en
    ] .

:isOrWasManagerOf
    a owl:ObjectProperty ;
    rdfs:comment """Connects an Agent to a Record Resource or Instantiation that the
         Agent managed or manages."""@en ;
    rdfs:domain :Agent ;
    rdfs:isDefinedBy <https://www.ica.org/standards/RiC/ontology> ;
    rdfs:label "es o era gestor de"@es, "est ou a été le gestionnaire de"@fr, "is or was manager of"@en ;
    rdfs:range [
        a owl:Class ;
        owl:unionOf (:Instantiation
            :RecordResource
        )
    ] ;
    rdfs:subPropertyOf :hasOrHadAuthorityOver ;
    owl:inverseOf :hasOrHadManager ;
    owl:propertyChainAxiom (:thingIsSourceOfRelation
        :managementRelation_role
        :relationHasTarget
    ) ;
    skos:changeNote [
        dc:date "2023-11-08" ;
        rdf:value """In order to get a system of rolified Relation classes: modified
               the property chain axiom so that it now involves the new managementRelation_role
               object property."""@en
    ], [
        dc:date "2023-11-02" ;
        rdf:value "Added a new rdfs:label in Spanish."@en
    ], [
        dc:date "2023-08-28" ;
        rdf:value "Added a new rdfs:label in French."@en
    ], [
        dc:date "2021-01-22" ;
        rdf:value """changed the IRI, label, inverse property IRI, super property
               IRI, textual definition (changed made in order to make RiC-O compliant with RiC-CM
               0.2; the name of this property in RiC-O 0.1 was \"isManagerOf\")."""@en
    ] ;
    :RiCCMCorrespondingComponent """RiC-R038 ('is or was manager of'
         relation)"""@en .

:isOrWasMandateTypeOf
    a owl:ObjectProperty ;
    rdfs:comment """Connects a Mandate Type to a Mandate that it categorized or
         categorizes."""@en ;
    rdfs:domain :MandateType ;
    rdfs:isDefinedBy <https://www.ica.org/standards/RiC/ontology> ;
    rdfs:label "es o era tipo de norma de"@es, "est ou a été le type de mandat de"@fr, "is or was mandate type of"@en ;
    rdfs:range :Mandate ;
    rdfs:subPropertyOf :isOrWasRuleTypeOf ;
    owl:inverseOf :hasOrHadMandateType ;
    skos:changeNote [
        dc:date "2024-03-15" ;
        rdf:value "Make capitalisation of rdfs:comment consistent."@en
    ], [
        dc:date "2023-11-13" ;
        rdf:value """Added the property, and its inverse one, following the creation
               of the MandateType class, that corresponds to the new Mandate Type attribute in
               RiC-CM 1.0."""@en
    ] .

:isOrWasMemberOf
    a owl:ObjectProperty ;
    rdfs:comment "Inverse of 'has or had member' object property."@en ;
    rdfs:domain :Person ;
    rdfs:isDefinedBy <https://www.ica.org/standards/RiC/ontology> ;
    rdfs:label "es o era miembro de"@es, "est ou a été membre de"@fr, "is or was member of"@en ;
    rdfs:range :Group ;
    rdfs:subPropertyOf :isAgentAssociatedWithAgent ;
    owl:inverseOf :hasOrHadMember ;
    owl:propertyChainAxiom (:thingIsTargetOfRelation
        :membershipRelation_role
        :relationHasSource
    ) ;
    skos:changeNote [
        dc:date "2023-11-08" ;
        rdf:value """In order to get a system of rolified Relation classes: modified
               the property chain axiom so that it now involves the new membershipRelation_role
               object property."""@en
    ], [
        dc:date "2023-11-02" ;
        rdf:value "Added a new rdfs:label in Spanish."@en
    ], [
        dc:date "2023-08-28" ;
        rdf:value "Added a new rdfs:label in French."@en
    ], [
        dc:date "2021-01-22" ;
        rdf:value """changed the IRI, label, inverse property IRI, textual
               definition (changed made in order to make RiC-O compliant with RiC-CM 0.2; the name
               of this property in RiC-O 0.1 was \"isMemberOf\")."""@en
    ] ;
    :RiCCMCorrespondingComponent """RiC-R055i ('is or was member of'
         relation)"""@en .

:isOrWasNameOf
    a owl:ObjectProperty ;
    rdfs:comment """Connects a Name to a Thing that it designated or
         designates."""@en ;
    rdfs:domain :Name ;
    rdfs:isDefinedBy <https://www.ica.org/standards/RiC/ontology> ;
    rdfs:label "es o era nombre de"@es, "est ou a été le nom de"@fr, "is or was name of"@en ;
    rdfs:range :Thing ;
    rdfs:subPropertyOf :isOrWasAppellationOf ;
    owl:inverseOf :hasOrHadName ;
    skos:changeNote [
        dc:date "2023-11-02" ;
        rdf:value "Added a new rdfs:label in Spanish."@en
    ], [
        dc:date "2023-08-28" ;
        rdf:value "Added a new rdfs:label in French."@en
    ], [
        dc:date "2021-01-22" ;
        rdf:value """changed the IRI, label, inverse property IRI, textual
               definition, super property IRI (the name of this property in RiC-O 0.1 was
               \"isNameOf\")."""@en
    ] .

:isOrWasOccupationTypeOf
    a owl:ObjectProperty ;
    rdfs:comment """Connects an Occupation Type to a Person whose occupation is or was
         categorized by it."""@en ;
    rdfs:domain :OccupationType ;
    rdfs:isDefinedBy <https://www.ica.org/standards/RiC/ontology> ;
    rdfs:label "es o era tipo de ocupación de"@es, "est ou a été le type d’occupation de"@fr, "is or was occupation type of"@en ;
    rdfs:range :Person ;
    rdfs:subPropertyOf :isOrWasDemographicGroupOf ;
    owl:inverseOf :hasOrHadOccupationOfType ;
    skos:changeNote [
        dc:date "2023-11-02" ;
        rdf:value "Added a new rdfs:label in Spanish."@en
    ], [
        dc:date "2023-08-28" ;
        rdf:value "Added a new rdfs:label in French."@en
    ], [
        dc:date "2021-01-22" ;
        rdf:value """changed the IRI, label, inverse property IRI, textual
               definition, super property IRI (the name of this property in RiC-O 0.1 was
               \"isOccupationTypeOf\")."""@en
    ] .

:isOrWasOccupiedBy
    a owl:ObjectProperty ;
    rdfs:comment "Inverse of 'occupies or occupied' object property."@en ;
    rdfs:domain :Position ;
    rdfs:isDefinedBy <https://www.ica.org/standards/RiC/ontology> ;
    rdfs:label "est ou a été occupé par"@fr, "está o estaba ocupado por"@es, "is or was occupied by"@en ;
    rdfs:range :Person ;
    rdfs:subPropertyOf :isAgentAssociatedWithAgent ;
    owl:inverseOf :occupiesOrOccupied ;
    owl:propertyChainAxiom (:thingIsTargetOfRelation
        :positionHoldingRelation_role
        :relationHasSource
    ) ;
    skos:changeNote [
        dc:date "2023-11-08" ;
        rdf:value """In order to get a system of rolified Relation classes: modified
               the property chain axiom so that it now involves the new positionHoldingRelation_role
               object property."""@en
    ], [
        dc:date "2023-11-02" ;
        rdf:value "Added a new rdfs:label in Spanish."@en
    ], [
        dc:date "2023-08-28" ;
        rdf:value "Added a new rdfs:label in French."@en
    ], [
        dc:date "2021-01-22" ;
        rdf:value """changed the IRI, label, inverse property IRI, text definition
               (changed made in order to make RiC-O compliant with RiC-CM 0.2; the name of this
               property in RiC-O 0.1 was \"occupiedBy\")."""@en
    ] ;
    :RiCCMCorrespondingComponent """RiC-R054i ('is or was occupied by'
         relation)"""@en .

:isOrWasOwnerOf
    a owl:ObjectProperty ;
    rdfs:comment """Connects a Group, Person or Position to a Thing that this Agent
         owns or owned."""@en ;
    rdfs:domain [
        a owl:Class ;
        owl:unionOf (:Group
            :Person
            :Position
        )
    ] ;
    rdfs:isDefinedBy <https://www.ica.org/standards/RiC/ontology> ;
    rdfs:label "es o era poseedor(a) de"@es, "est ou a été propriétaire de"@fr, "is or was owner of"@en ;
    rdfs:range :Thing ;
    rdfs:subPropertyOf :hasOrHadAuthorityOver ;
    owl:inverseOf :hasOrHadOwner ;
    owl:propertyChainAxiom (:thingIsSourceOfRelation
        :ownershipRelation_role
        :relationHasTarget
    ) ;
    skos:changeNote [
        dc:date "2023-11-08" ;
        rdf:value """In order to get a system of rolified Relation classes: modified
               the property chain axiom so that it now involves the new ownershipRelation_role
               object property."""@en
    ], [
        dc:date "2023-11-02" ;
        rdf:value "Added a new rdfs:label in Spanish."@en
    ], [
        dc:date "2023-08-28" ;
        rdf:value "Added a new rdfs:label in French."@en
    ], [
        dc:date "2021-01-22" ;
        rdf:value """changed the IRI, label, inverse property IRI, textual
               definition, super property IRI (changed made in order to make RiC-O compliant with
               RiC-CM 0.2; the name of this property in RiC-O 0.1 was \"isOwnerOf\")."""@en
    ] ;
    :RiCCMCorrespondingComponent """RiC-R037 ('is or was owner of'
         relation)"""@en .

:isOrWasPartOf
    a owl:ObjectProperty ;
    rdfs:comment "Inverse of 'has or had part' relation."@en ;
    rdfs:domain :Thing ;
    rdfs:isDefinedBy <https://www.ica.org/standards/RiC/ontology> ;
    rdfs:label "es o era parte de"@es, "est ou a été une partie de"@fr, "is or was part of"@en ;
    rdfs:range :Thing ;
    rdfs:subPropertyOf :isRelatedTo ;
    owl:inverseOf :hasOrHadPart ;
    owl:propertyChainAxiom (:thingIsTargetOfRelation
        :wholePartRelation_role
        :relationHasSource
    ) ;
    skos:changeNote [
        dc:date "2023-11-08" ;
        rdf:value """In order to get a system of rolified Relation classes: modified
               the property chain axiom so that it now involves the new wholePartRelation_role
               object property."""@en
    ], [
        dc:date "2023-11-02" ;
        rdf:value "Added a new rdfs:label in Spanish."@en
    ], [
        dc:date "2023-08-28" ;
        rdf:value "Added a new rdfs:label in French."@en
    ], [
        dc:date "2021-01-22" ;
        rdf:value """changed the IRI, label, inverse property IRI, textual
               definition (changed made in order to make RiC-O compliant with RiC-CM 0.2; the name
               of this property in RiC-O 0.1 was \"isPartOf\")."""@en
    ] ;
    :RiCCMCorrespondingComponent """RiC-R002i ('is or was part of'
         relation)"""@en .

:isOrWasParticipantIn
    a owl:ObjectProperty ;
    rdfs:comment """Inverse of 'has or had participant' object
         property."""@en ;
    rdfs:domain :Thing ;
    rdfs:isDefinedBy <https://www.ica.org/standards/RiC/ontology> ;
    rdfs:label "es o era participante de"@es, "is or was participant in"@en, "participe ou a participé à"@fr ;
    rdfs:range :Event ;
    rdfs:subPropertyOf :isAssociatedWithEvent ;
    owl:inverseOf :hasOrHadParticipant ;
    skos:changeNote [
        dc:date "2023-11-02" ;
        rdf:value "Added a new rdfs:label in Spanish."@en
    ], [
        dc:date "2023-08-28" ;
        rdf:value "Added a new rdfs:label in French."@en
    ], [
        dc:date "2021-01-22" ;
        rdf:value """changed the IRI, label, inverse property IRI, textual
               definition (changed made in order to make RiC-O compliant with RiC-CM 0.2; the name
               of this property in RiC-O 0.1 was \"involvedIn\")."""@en
    ] ;
    :RiCCMCorrespondingComponent """RiC-R058i ('is or was participant in'
         relation)"""@en .

:isOrWasPerformedBy
    a owl:ObjectProperty ;
    rdfs:comment """Connects an Activity to an Agent that performed or performs the
         Activity."""@en ;
    rdfs:domain :Activity ;
    rdfs:isDefinedBy <https://www.ica.org/standards/RiC/ontology> ;
    rdfs:label "es o fue desarrollado por"@es, "est ou a été réalisée par"@fr, "is or was performed by"@en ;
    rdfs:range :Agent ;
    rdfs:subPropertyOf :hasOrHadParticipant ;
    owl:inverseOf :performsOrPerformed ;
    owl:propertyChainAxiom (:thingIsSourceOfRelation
        :performanceRelation_role
        :relationHasTarget
    ) ;
    skos:changeNote [
        dc:date "2023-11-08" ;
        rdf:value """In order to get a system of rolified Relation classes: modified
               the property chain axiom so that it now involves the new performanceRelation_role
               object property."""@en
    ], [
        dc:date "2023-11-02" ;
        rdf:value "Added a new rdfs:label in Spanish."@en
    ], [
        dc:date "2023-08-28" ;
        rdf:value "Added a new rdfs:label in French."@en
    ], [
        dc:date "2021-01-22" ;
        rdf:value """changed the IRI, label, inverse property IRI, text definition,
               super property IRI (changed made in order to make RiC-O compliant with RiC-CM 0.2;
               the name of this property in RiC-O 0.1 was \"performedBy\")."""@en
    ] ;
    :RiCCMCorrespondingComponent """RiC-R060 ('is or was performed by'
         relation)"""@en .

:isOrWasPhysicalLocationOf
    a owl:ObjectProperty ;
    rdfs:comment """Connects a Physical Location to a Place, when it is or was its
         location."""@en ;
    rdfs:domain :PhysicalLocation ;
    rdfs:isDefinedBy <https://www.ica.org/standards/RiC/ontology> ;
    rdfs:label "a ou a été la localisation physique de"@fr, "es o era localización física de"@es, "is or was physical location of"@en ;
    rdfs:range :Place ;
    rdfs:subPropertyOf :isAssociatedWithPlace ;
    owl:inverseOf :hasOrHadPhysicalLocation ;
    skos:changeNote [
        dc:date "2023-11-02" ;
        rdf:value "Added a new rdfs:label in Spanish."@en
    ], [
        dc:date "2023-08-28" ;
        rdf:value "Added a new rdfs:label in French."@en
    ], [
        dc:date "2021-02-01" ;
        rdf:value """Property made a subproperty of
               'isAssociatedWithPlace\"."""@en
    ], [
        dc:date "2021-01-22" ;
        rdf:value """changed the IRI, label, inverse property IRI, textual
               definition (the name of this property in RiC-O 0.1 was
               \"isPhysicalLocationOf\")."""@en
    ] .

:isOrWasPlaceNameOf
    a owl:ObjectProperty ;
    rdfs:comment """Connects a Place Name to a Place that was or is designated by
         it."""@en ;
    rdfs:domain :PlaceName ;
    rdfs:isDefinedBy <https://www.ica.org/standards/RiC/ontology> ;
    rdfs:label "a ou a été le nom de lieu de"@fr, "es o era nombre de lugar de"@es, "is or was place name of"@en ;
    rdfs:range :Place ;
    rdfs:subPropertyOf :isOrWasNameOf ;
    owl:inverseOf :hasOrHadPlaceName ;
    skos:changeNote [
        dc:date "2023-11-02" ;
        rdf:value "Added a new rdfs:label in Spanish."@en
    ], [
        dc:date "2023-08-28" ;
        rdf:value "Added a new rdfs:label in French."@en
    ], [
        dc:date "2021-01-22" ;
        rdf:value """changed the IRI, label, inverse property IRI, text definition,
               super property IRI (the name of this property in RiC-O 0.1 was
               \"isPlaceNameOf\")."""@en
    ] .

:isOrWasPlaceTypeOf
    a owl:ObjectProperty ;
    rdfs:comment """Connects a Place Type to a Place that is or was categorized by
         it."""@en ;
    rdfs:domain :PlaceType ;
    rdfs:isDefinedBy <https://www.ica.org/standards/RiC/ontology> ;
    rdfs:label "a ou a été le type de lieu de"@fr, "es o era tipo de lugar de"@es, "is or was place type of"@en ;
    rdfs:range :Place ;
    rdfs:subPropertyOf :isOrWasTypeOf ;
    owl:inverseOf :hasOrHadPlaceType ;
    skos:changeNote [
        dc:date "2023-11-02" ;
        rdf:value "Added a new rdfs:label in Spanish."@en
    ], [
        dc:date "2023-08-28" ;
        rdf:value "Added a new rdfs:label in French."@en
    ], [
        dc:date "2021-01-22" ;
        rdf:value """changed the IRI, label, inverse property IRI, text definition,
               super property IRI (the name of this property in RiC-O 0.1 was
               \"isPlaceTypeOf\")."""@en
    ] .

:isOrWasRecordStateOfAllMembersOf
    a owl:ObjectProperty ;
    rdfs:comment """Connects a Record State and a Record Set whose all past or present
         Record or Record Part members have that Record State."""@en ;
    rdfs:domain :RecordState ;
    rdfs:isDefinedBy <https://www.ica.org/standards/RiC/ontology> ;
    rdfs:label "a ou a été l’état de tous les membres de"@fr, "es o era estado de documento de todos los miembros de"@es, "is or was record state of all members of"@en ;
    rdfs:range :RecordSet ;
    rdfs:subPropertyOf :isOrWasTypeOfAllMembersOf ;
    owl:inverseOf :hasOrHadAllMembersWithRecordState ;
    skos:changeNote [
        dc:date "2023-11-02" ;
        rdf:value "Added a new rdfs:label in Spanish."@en
    ], [
        dc:date "2023-08-28" ;
        rdf:value "Added a new rdfs:label in French."@en
    ], [
        dc:date "2020-12-28" ;
        rdf:value """Object property added for handling the case where a Record Set
               is described as having all or some members that belong to some category (see RiC-CM
               0.2 attributes section, #4.4 on Record Set, Record and Record Part
               attributes)."""@en
    ] .

:isOrWasRecordStateOfSomeMembersOf
    a owl:ObjectProperty ;
    rdfs:comment """Connects a Record State and a Record Set whose some past or
         present Record or Record Part members have that Record State."""@en ;
    rdfs:domain :RecordState ;
    rdfs:isDefinedBy <https://www.ica.org/standards/RiC/ontology> ;
    rdfs:label "a ou a été l’état de certains membres de"@fr, "es o era estado de documento de algunos miembros de"@es, "is or was record state of some members of"@en ;
    rdfs:range :RecordSet ;
    rdfs:subPropertyOf :isOrWasTypeOfSomeMembersOf ;
    owl:inverseOf :hasOrHadSomeMembersWithRecordState ;
    skos:changeNote [
        dc:date "2023-11-02" ;
        rdf:value "Added a new rdfs:label in Spanish."@en
    ], [
        dc:date "2023-08-28" ;
        rdf:value "Added a new rdfs:label in French."@en
    ], [
        dc:date "2020-12-28" ;
        rdf:value """Object property added for handling the case where a Record Set
               is described as having all or some members that belong to some category (see RiC-CM
               0.2 attributes section, #4.4 on Record Set, Record and Record Part
               attributes)."""@en
    ] .

:isOrWasRegulatedBy
    a owl:ObjectProperty ;
    rdfs:comment """Inverse of 'regulates or regulated' object
         property."""@en ;
    rdfs:domain :Thing ;
    rdfs:isDefinedBy <https://www.ica.org/standards/RiC/ontology> ;
    rdfs:label "est ou a été régulé par"@fr, "está o estaba regulado por"@es, "is or was regulated by"@en ;
    rdfs:range :Rule ;
    rdfs:subPropertyOf :isAssociatedWithRule ;
    owl:inverseOf :regulatesOrRegulated ;
    skos:changeNote [
        dc:date "2023-11-02" ;
        rdf:value "Added a new rdfs:label in Spanish."@en
    ], [
        dc:date "2023-08-28" ;
        rdf:value "Added a new rdfs:label in French."@en
    ], [
        dc:date "2021-01-22" ;
        rdf:value """changed the IRI, label, inverse property IRI (changed made in
               order to make RiC-O compliant with RiC-CM 0.2; the name of this property in RiC-O 0.1
               was \"regulatedBy\")."""@en
    ] ;
    :RiCCMCorrespondingComponent """RiC-R063i ('is or was regulated by'
         relation)"""@en .

:isOrWasRepresentedByContentOfSomeMembersOf
    a owl:ObjectProperty ;
    rdfs:comment """Inverse of 'has or had some members whose content represents'
         object property."""@en ;
    rdfs:domain :Thing ;
    rdfs:isDefinedBy <https://www.ica.org/standards/RiC/ontology> ;
    rdfs:label """es o era representado por el contenido de algunos miembros
         de"""@es, """est ou a été représenté par le contenu de certains membres
         de"""@fr, "is or was represented by content of some members of"@en ;
    rdfs:range :RecordSet ;
    rdfs:subPropertyOf :isOrWasSubjectOfSomeMembersOf ;
    owl:inverseOf :hasOrHadSomeMembersWhoseContentRepresents ;
    skos:changeNote [
        dc:date "2025-04-05" ;
        rdf:value "Introduced in RiC-O 1.1."@en
    ] .

:isOrWasResponsibleForEnforcing
    a owl:ObjectProperty ;
    rdfs:comment "Inverse of 'is or was enforced by' object property."@en ;
    rdfs:domain :Agent ;
    rdfs:isDefinedBy <https://www.ica.org/standards/RiC/ontology> ;
    rdfs:label "es o era responsable de aplicar"@es, "impose ou a imposé"@fr, "is or was responsible for enforcing"@en ;
    rdfs:range :Rule ;
    rdfs:subPropertyOf :isAssociatedWithRule ;
    owl:inverseOf :isOrWasEnforcedBy ;
    skos:changeNote [
        dc:date "2024-09-02" ;
        rdf:value "Fixed the French label."@en
    ], [
        dc:date "2023-11-02" ;
        rdf:value "Added a new rdfs:label in Spanish."@en
    ], [
        dc:date "2023-08-28" ;
        rdf:value "Added a new rdfs:label in French."@en
    ], [
        dc:date "2021-01-22" ;
        rdf:value """changed the IRI, label, inverse property IRI, text definition,
               corresponding CM component name (changed made in order to make RiC-O compliant with
               RiC-CM 0.2; the name of this property in RiC-O 0.1 was
               \"isResponsibleForEnforcing\")."""@en
    ] ;
    :RiCCMCorrespondingComponent """RiC-R066i ('is or was responsible for enforcing'
         relation)"""@en .

:isOrWasRuleTypeOf
    a owl:ObjectProperty ;
    rdfs:comment """Connects a Rule Type to a Rule that it categorized or
         categorizes."""@en ;
    rdfs:domain :RuleType ;
    rdfs:isDefinedBy <https://www.ica.org/standards/RiC/ontology> ;
    rdfs:label "es o era tipo de regla de"@es, "est ou a été le type de règle de"@fr, "is or was rule type of"@en ;
    rdfs:range :Rule ;
    rdfs:subPropertyOf :isOrWasTypeOf ;
    owl:inverseOf :hasOrHadRuleType ;
    skos:changeNote [
        dc:date "2024-03-15" ;
        rdf:value "Make capitalisation of rdfs:comment consistent."@en
    ], [
        dc:date "2023-11-02" ;
        rdf:value "Added a new rdfs:label in Spanish."@en
    ], [
        dc:date "2023-08-28" ;
        rdf:value "Added a new rdfs:label in French."@en
    ], [
        dc:date "2021-01-22" ;
        rdf:value """changed the IRI, label, inverse property IRI, text definition,
               super property URI (the name of this property in RiC-O 0.1 was
               \"isRuleTypeOf\")."""@en
    ], [
        dc:date "2020-10-19" ;
        rdf:value """Object property added along with RuleType class and hasRuleType
               object property. """@en
    ] .

:isOrWasSubdivisionOf
    a owl:ObjectProperty ;
    rdfs:comment """Inverse of 'has or had subdivision' object
         property."""@en ;
    rdfs:domain :Group ;
    rdfs:isDefinedBy <https://www.ica.org/standards/RiC/ontology> ;
    rdfs:label "es o era subdivisión de"@es, "est ou a été une subdivision de"@fr, "is or was subdivision of"@en ;
    rdfs:range :Group ;
    rdfs:subPropertyOf :isOrWasPartOf, :isOrWasSubordinateTo ;
    owl:inverseOf :hasOrHadSubdivision ;
    owl:propertyChainAxiom (:thingIsTargetOfRelation
        :groupSubdivisionRelation_role
        :relationHasSource
    ) ;
    skos:changeNote [
        dc:date "2023-11-08" ;
        rdf:value """In order to get a system of rolified Relation classes: modified
               the property chain axiom so that it now involves the new
               groupSubdivisionRelation_role object property."""@en
    ], [
        dc:date "2023-11-02" ;
        rdf:value "Added a new rdfs:label in Spanish."@en
    ], [
        dc:date "2023-08-28" ;
        rdf:value "Added a new rdfs:label in French."@en
    ], [
        dc:date "2021-01-22" ;
        rdf:value """changed the IRI, label, inverse property IRI, text definition,
               super property IRIs (changed made in order to make RiC-O compliant with RiC-CM 0.2;
               the name of this property in RiC-O 0.1 was \"isSubdivisionOf\")."""@en
    ] ;
    :RiCCMCorrespondingComponent """RiC-R005i ('is or was subdivision'
         relation)"""@en .

:isOrWasSubeventOf
    a owl:ObjectProperty ;
    rdfs:comment "Inverse of 'has or had subevent' object property."@en ;
    rdfs:domain :Event ;
    rdfs:isDefinedBy <https://www.ica.org/standards/RiC/ontology> ;
    rdfs:label "es o era parte de evento de"@es, "est ou a été un événement constituant de"@fr, "is or was subevent of"@en ;
    rdfs:range :Event ;
    rdfs:subPropertyOf :isAssociatedWithEvent, :isEventAssociatedWith, :isOrWasPartOf ;
    owl:inverseOf :hasOrHadSubevent ;
    skos:changeNote [
        dc:date "2023-11-02" ;
        rdf:value "Added a new rdfs:label in Spanish."@en
    ], [
        dc:date "2023-08-28" ;
        rdf:value "Added a new rdfs:label in French."@en
    ], [
        dc:date "2021-01-22" ;
        rdf:value """changed the IRI, label, inverse property IRI, text definition,
               super property URI (changed made in order to make RiC-O compliant with RiC-CM 0.2;
               the name of this property in RiC-O 0.1 was \"isSubEventOf\")."""@en
    ] ;
    :RiCCMCorrespondingComponent """RiC-R006i ('is or was subevent of'
         relation)"""@en .

:isOrWasSubjectOf
    a owl:ObjectProperty ;
    rdfs:comment "Inverse of 'has or had subject' object property."@en ;
    rdfs:domain :Thing ;
    rdfs:isDefinedBy <https://www.ica.org/standards/RiC/ontology> ;
    rdfs:label "es o era materia de"@es, "est ou a été le sujet de"@fr, "is or was subject of"@en ;
    rdfs:range :RecordResource ;
    rdfs:subPropertyOf :isRelatedTo ;
    owl:inverseOf :hasOrHadSubject ;
    skos:changeNote [
        dc:date "2023-11-02" ;
        rdf:value "Added a new rdfs:label in Spanish."@en
    ], [
        dc:date "2023-08-28" ;
        rdf:value "Added a new rdfs:label in French."@en
    ], [
        dc:date "2021-01-22" ;
        rdf:value """changed the IRI, label, inverse property IRI, text definition
               (changed made in order to make RiC-O compliant with RiC-CM 0.2; the name of this
               property in RiC-O 0.1 was \"isSubjectOf\")."""@en
    ] ;
    :RiCCMCorrespondingComponent """RIc-R019i ('is or was subject of'
         relation)"""@en .

:isOrWasSubjectOfAllMembersOf
    a owl:ObjectProperty ;
    rdfs:comment """Inverse of 'has or had all members with subject' object
         property."""@en ;
    rdfs:domain :Thing ;
    rdfs:isDefinedBy <https://www.ica.org/standards/RiC/ontology> ;
    rdfs:label "es o era la matería de todos los miembros de"@es, "est ou a été le sujet de tous les membres de"@fr, "is or was subject of all members of"@en ;
    rdfs:range :RecordSet ;
    rdfs:subPropertyOf :isOrWasSubjectOf ;
    owl:inverseOf :hasOrHadAllMembersWithSubject ;
    skos:changeNote [
        dc:date "2025-04-05" ;
        rdf:value "Introduced in RiC-O 1.1."@en
    ] .

:isOrWasSubjectOfSomeMembersOf
    a owl:ObjectProperty ;
    rdfs:comment """Inverse of 'has or had some members with subject' object
         property."""@en ;
    rdfs:domain :Thing ;
    rdfs:isDefinedBy <https://www.ica.org/standards/RiC/ontology> ;
    rdfs:label "es o era la matería de algunos miembros de"@es, "est ou a été le sujet de certains membres de"@fr, "is or was subject of some members of"@en ;
    rdfs:range :RecordSet ;
    rdfs:subPropertyOf :isRelatedTo ;
    owl:inverseOf :hasOrHadSomeMembersWithSubject ;
    skos:changeNote [
        dc:date "2025-04-05" ;
        rdf:value "Introduced in RiC-O 1.1."@en
    ] .

:isOrWasSubordinateTo
    a owl:ObjectProperty ;
    rdfs:comment """Inverse of 'has or had subordinate' object
         property."""@en ;
    rdfs:domain :Agent ;
    rdfs:isDefinedBy <https://www.ica.org/standards/RiC/ontology> ;
    rdfs:label "est ou a été le subalterne de"@fr, "está o estaba subordinado(a) a"@es, "is or was subordinate to"@en ;
    rdfs:range :Agent ;
    rdfs:subPropertyOf :isAgentAssociatedWithAgent ;
    owl:inverseOf :hasOrHadSubordinate ;
    owl:propertyChainAxiom (:thingIsTargetOfRelation
        :agentHierarchicalRelation_role
        :relationHasSource
    ) ;
    skos:changeNote [
        dc:date "2023-11-08" ;
        rdf:value """In order to get a system of rolified Relation classes: modified
               the property chain axiom so that it now involves the new
               agentHierarchicalRelation_role object property."""@en
    ], [
        dc:date "2023-11-02" ;
        rdf:value "Added a new rdfs:label in Spanish."@en
    ], [
        dc:date "2023-08-28" ;
        rdf:value "Added a new rdfs:label in French."@en
    ], [
        dc:date "2021-01-22" ;
        rdf:value """changed the IRI, label, inverse property IRI (changed made in
               order to make RiC-O compliant with RiC-CM 0.2; the name of this property in RiC-O 0.1
               was \"isHierarchicallyInferiorTo\")."""@en
    ] ;
    :RiCCMCorrespondingComponent """RiC-R045i ('is or was subordinate to'
         relation)"""@en .

:isOrWasTitleOf
    a owl:ObjectProperty ;
    rdfs:comment """Connects a Title to a Record Resource, Instantiation or Rule that
         it designated or designates."""@en ;
    rdfs:domain :Title ;
    rdfs:isDefinedBy <https://www.ica.org/standards/RiC/ontology> ;
    rdfs:label "es o era título de"@es, "est ou a été l’intitulé de"@fr, "is or was title of"@en ;
    rdfs:range [
        a owl:Class ;
        owl:unionOf (:Instantiation
            :RecordResource
            :Rule
        )
    ] ;
    rdfs:subPropertyOf :isOrWasNameOf ;
    owl:inverseOf :hasOrHadTitle ;
    skos:changeNote [
        dc:date "2023-11-02" ;
        rdf:value "Added a new rdfs:label in Spanish."@en
    ], [
        dc:date "2023-08-28" ;
        rdf:value "Added a new rdfs:label in French."@en
    ], [
        dc:date "2021-01-22" ;
        rdf:value """changed the IRI, label, inverse property IRI, text definition,
               super property IRI (the name of this property in RiC-O 0.1 was
               \"isTitleOf\")."""@en
    ] .

:isOrWasTypeOf
    a owl:ObjectProperty ;
    rdfs:comment """Connects a Type to a Thing that it categorizes or
         categorized."""@en ;
    rdfs:domain :Type ;
    rdfs:isDefinedBy <https://www.ica.org/standards/RiC/ontology> ;
    rdfs:label "es o era lo tipo de"@es, "est ou a été le type de"@fr, "is or was type of"@en ;
    rdfs:range :Thing ;
    rdfs:subPropertyOf :isRelatedTo ;
    owl:inverseOf :hasOrHadType ;
    owl:propertyChainAxiom (:thingIsSourceOfRelation
        :typeRelation_role
        :relationHasTarget
    ) ;
    skos:changeNote [
        dc:date "2024-10-04" ;
        rdf:value """Changed the word 'category' into 'type' in all applicable
               properties names."""@en
    ], [
        dc:date "2023-11-08" ;
        rdf:value """In order to get a system of rolified Relation classes: modified
               the property chain axiom so that it now involves the new typeRelation_role object
               property."""@en
    ], [
        dc:date "2023-11-02" ;
        rdf:value "Added a new rdfs:label in Spanish."@en
    ], [
        dc:date "2023-08-28" ;
        rdf:value "Added a new rdfs:label in French."@en
    ], [
        dc:date "2021-01-22" ;
        rdf:value """changed the IRI, label, inverse property IRI, text definition
               (the name of this property in RiC-O 0.1 was \"isCategoryOf\")."""@en
    ] .

:isOrWasTypeOfAllMembersOf
    a owl:ObjectProperty ;
    rdfs:comment """Connects a Type and a Record Set whose all present or past Record
         or Record Part members belong to that Type."""@en ;
    rdfs:domain :Type ;
    rdfs:isDefinedBy <https://www.ica.org/standards/RiC/ontology> ;
    rdfs:label "es o era lo tipo de todos los miembros de"@es, "est ou a été le type de tous les membres de"@fr, "is or was type of all members of"@en ;
    rdfs:range :RecordSet ;
    rdfs:subPropertyOf :isRelatedTo ;
    owl:inverseOf :hasOrHadAllMembersWithType ;
    skos:changeNote [
        dc:date "2024-10-04" ;
        rdf:value """Changed the word 'category' into 'type' in all applicable
               properties names."""@en
    ], [
        dc:date "2023-11-02" ;
        rdf:value "Added a new rdfs:label in Spanish."@en
    ], [
        dc:date "2023-08-28" ;
        rdf:value "Added a new rdfs:label in French."@en
    ], [
        dc:date "2020-12-28" ;
        rdf:value """Object property added for handling the case where a Record Set
               is described as having all or some members that belong to some category (see RiC-CM
               0.2 attributes section, #4.4 on Record Set, Record and Record Part
               attributes)."""@en
    ] .

:isOrWasTypeOfSomeMembersOf
    a owl:ObjectProperty ;
    rdfs:comment """Connects a Type and a Record Set whose some present or past Record
         or Record Part members belong to that Type."""@en ;
    rdfs:domain :Type ;
    rdfs:isDefinedBy <https://www.ica.org/standards/RiC/ontology> ;
    rdfs:label "es o era lo tipo de algunos miembros de"@es, "est ou a été le type de certains membres de"@fr, "is or was type of some members of"@en ;
    rdfs:range :RecordSet ;
    rdfs:subPropertyOf :isRelatedTo ;
    owl:inverseOf :hasOrHadSomeMembersWithType ;
    skos:changeNote [
        dc:date "2024-10-04" ;
        rdf:value """Changed the word 'category' into 'type' in all applicable
               properties names."""@en
    ], [
        dc:date "2023-11-02" ;
        rdf:value "Added a new rdfs:label in Spanish."@en
    ], [
        dc:date "2023-08-28" ;
        rdf:value "Added a new rdfs:label in French."@en
    ], [
        dc:date "2020-12-28" ;
        rdf:value """Object property added for handling the case where a Record Set
               is described as having all or some members that belong to some category (see RiC-CM
               0.2 attributes section, #4.4 on Record Set, Record and Record Part
               attributes)."""@en
    ] .

:isOrWasUnderAuthorityOf
    a owl:ObjectProperty ;
    rdfs:comment """Inverse of 'has or had authority over' object
         property."""@en ;
    rdfs:domain :Thing ;
    rdfs:isDefinedBy <https://www.ica.org/standards/RiC/ontology> ;
    rdfs:label "est ou a été sous l’autorité de"@fr, "está o estaba bajo control de"@es, "is or was under authority of"@en ;
    rdfs:range :Agent ;
    rdfs:subPropertyOf :isRelatedTo ;
    owl:inverseOf :hasOrHadAuthorityOver ;
    owl:propertyChainAxiom (:thingIsTargetOfRelation
        :authorityRelation_role
        :relationHasSource
    ) ;
    skos:changeNote [
        dc:date "2023-11-08" ;
        rdf:value """In order to get a system of rolified Relation classes: modified
               the property chain axiom so that it now involves the new authorityRelation_role
               object property."""@en
    ], [
        dc:date "2023-11-02" ;
        rdf:value "Added a new rdfs:label in Spanish."@en
    ], [
        dc:date "2023-08-28" ;
        rdf:value "Added a new rdfs:label in French."@en
    ], [
        dc:date "2021-01-22" ;
        rdf:value """changed the IRI, label, inverse property IRI, text definition
               (changed made in order to make RiC-O compliant with RiC-CM 0.2; the name of this
               property in RiC-O 0.1 was \"isUnderAuthorityOf\")."""@en
    ] ;
    :RiCCMCorrespondingComponent """RiC-R036i ('is or was under authority of'
         relation)"""@en .

:isOrganicOrFunctionalProvenanceOf
    a owl:ObjectProperty ;
    rdfs:comment """Inverse of 'has organic or functional provenance' object
         property."""@en ;
    rdfs:domain [
        a owl:Class ;
        owl:unionOf (:Activity
            :Agent
        )
    ] ;
    rdfs:isDefinedBy <https://www.ica.org/standards/RiC/ontology> ;
    rdfs:label "es procedencia orgánica o funcional de"@es, "est la provenance organique ou fonctionnelle de"@fr, "is organic or functional provenance of"@en ;
    rdfs:range [
        a owl:Class ;
        owl:unionOf (:Instantiation
            :RecordResource
        )
    ] ;
    rdfs:subPropertyOf :isRelatedTo ;
    owl:inverseOf :hasOrganicOrFunctionalProvenance ;
    owl:propertyChainAxiom (:thingIsTargetOfRelation
        :organicOrFunctionalProvenanceRelation_role
        :relationHasSource
    ) ;
    skos:changeNote [
        dc:date "2023-11-08" ;
        rdf:value """In order to get a system of rolified Relation classes: modified
               the property chain axiom so that it now involves the new
               organicOrFunctionalProvenanceRelation_role object property."""@en
    ], [
        dc:date "2023-11-07" ;
        rdf:value """Property added as a superproperty of isProvenance and
               documentedBy, along with its inverse property. Shortcut also added."""@en
    ] .

:isOrganicProvenanceDateOf
    a owl:ObjectProperty ;
    rdfs:comment """Connects a Date associated with the organic provenance of a Record
         Resource or Instantiation to that Record Resource or Instantiation."""@en ;
    rdfs:domain :Date ;
    rdfs:isDefinedBy <https://www.ica.org/standards/RiC/ontology> ;
    rdfs:label "es la fecha de procedencia orgánica de"@es, "est la date de provenance organique de"@fr, "is organic provenance date of"@en ;
    rdfs:range [
        a owl:Class ;
        owl:unionOf (:Instantiation
            :RecordResource
        )
    ] ;
    rdfs:subPropertyOf :isDateAssociatedWith ;
    owl:inverseOf :hasOrganicProvenanceDate ;
    owl:propertyChainAxiom (:isDateAssociatedWithRelation
        :organicProvenanceRelation_role
        :relationHasSource
    ) ;
    skos:changeNote [
        dc:date "2025-03-13" ;
        rdf:value "Added French and Spanish labels."@en
    ], [
        dc:date "2024-12-19" ;
        rdf:value "Added in RiC-O 1.1."@en
    ] .

:isOrganicProvenanceOf
    a owl:ObjectProperty ;
    rdfs:comment """Inverse of 'has organic provenance' object
         property."""@en ;
    rdfs:domain :Agent ;
    rdfs:isDefinedBy <https://www.ica.org/standards/RiC/ontology> ;
    rdfs:label "es procedencia orgánica de"@es, "est la provenance organique de"@fr, "is organic provenance of"@en ;
    rdfs:range [
        a owl:Class ;
        owl:unionOf (:Instantiation
            :RecordResource
        )
    ] ;
    rdfs:subPropertyOf :isOrganicOrFunctionalProvenanceOf ;
    owl:inverseOf :hasOrganicProvenance ;
    owl:propertyChainAxiom (:thingIsTargetOfRelation
        :organicProvenanceRelation_role
        :relationHasSource
    ) ;
    skos:changeNote [
        dc:date "2024-03-15" ;
        rdf:value "Make capitalisation of rdfs:comment consistent."@en
    ], [
        dc:date "2023-11-08" ;
        rdf:value """In order to get a system of rolified Relation classes: modified
               the property chain axiom so that it now involves the new
               organicProvenanceRelation_role object property."""@en
    ], [
        dc:date "2023-11-07" ;
        rdf:value """Made this property a subproperty of the new
               isOrganicOrFunctionalProvenanceOf property. Renamed it to make things clearer.
               Adjusted its labels."""@en
    ], [
        dc:date "2023-11-02" ;
        rdf:value "Added a new rdfs:label in Spanish."@en
    ], [
        dc:date "2023-08-28" ;
        rdf:value "Added a new rdfs:label in French."@en
    ] ;
    :RiCCMCorrespondingComponent """RiC-R026i ('is provenance of'
         relation)"""@en .

:isOriginalOf
    a owl:ObjectProperty ;
    rdfs:comment """Connects the original version of a Record to a copy or a later
         version."""@en ;
    rdfs:domain [
        a owl:Class ;
        owl:unionOf (:Record
            :RecordPart
        )
    ] ;
    rdfs:isDefinedBy <https://www.ica.org/standards/RiC/ontology> ;
    rdfs:label "es original de"@es, "est l’original de"@fr, "is original of"@en ;
    rdfs:range [
        a owl:Class ;
        owl:unionOf (:Record
            :RecordPart
        )
    ] ;
    rdfs:subPropertyOf :hasGeneticLinkToRecordResource, :precedesInTime ;
    owl:inverseOf :hasOriginal ;
    skos:changeNote [
        dc:date "2023-11-02" ;
        rdf:value "Added a new rdfs:label in Spanish."@en
    ], [
        dc:date "2023-08-28" ;
        rdf:value "Added a new rdfs:label in French."@en
    ] ;
    skos:scopeNote """There may be zero to many intermediate Records, ignored or
         unknown, between the two connected Records"""@en ;
    :RiCCMCorrespondingComponent """RiC-R010 (is original of
         relation)"""@en .

:isPartOfTransitive
    a owl:ObjectProperty, owl:TransitiveProperty ;
    rdfs:comment """Connects a Thing to a Thing of which it is a a constitutive or
         component part, directly or indirectly. This is a transitive relation."""@en ;
    rdfs:domain :Thing ;
    rdfs:isDefinedBy <https://www.ica.org/standards/RiC/ontology> ;
    rdfs:label "es parte de transitivo"@es, "est une partie de transitif"@fr, "is part of transitive"@en ;
    rdfs:range :Thing ;
    rdfs:subPropertyOf :isOrWasPartOf ;
    owl:inverseOf :hasPartTransitive ;
    skos:changeNote [
        dc:date "2023-11-27" ;
        rdf:value "Added a new rdfs:label in Spanish."@en
    ], [
        dc:date "2023-11-13" ;
        rdf:value "Added a French label."@en
    ], [
        dc:date "2023-07-12" ;
        rdf:value """Object property added, along with its inverse property, in
               order to enable to express current partitive relations between things (the past
               partitive relation also being added)."""@en
    ] ;
    skos:scopeNote """To be used, either to infer, then query or browse, relations
         from existing direct 'isDirectPartOf' relations between things, or to record a current
         partitive relation when you do not know if there are intermediate nodes between the related
         things."""@en .

:isPlaceAssociatedWith
    a owl:ObjectProperty ;
    rdfs:comment """Connects a Place to a Thing with whose existence and lifecycle the
         Place is associated."""@en ;
    rdfs:domain :Place ;
    rdfs:isDefinedBy <https://www.ica.org/standards/RiC/ontology> ;
    rdfs:label "es lugar asociado con"@es, "est un lieu associé à"@fr, "is place associated with"@en ;
    rdfs:range :Thing ;
    rdfs:subPropertyOf :isRelatedTo ;
    owl:inverseOf :isAssociatedWithPlace ;
    owl:propertyChainAxiom (:thingIsSourceOfRelation
        :placeRelation_role
        :relationHasTarget
    ) ;
    skos:changeNote [
        dc:date "2023-11-12" ;
        rdf:value """Aligned with RiC-CM 1.0: updated the description
               (rdfs:comment), skos:scopeNote."""@en
    ], [
        dc:date "2023-11-08" ;
        rdf:value """In order to get a system of rolified Relation classes: modified
               the property chain axiom so that it now involves the new placeRelation_role object
               property."""@en
    ], [
        dc:date "2023-11-02" ;
        rdf:value "Added a new rdfs:label in Spanish."@en
    ], [
        dc:date "2023-08-28" ;
        rdf:value "Added a new rdfs:label in French."@en
    ] ;
    skos:scopeNote """Use to connect a Place to an entity only if it is not possible
         to specify a narrower spatial relation, for example, is or was location
         of."""@en ;
    :RiCCMCorrespondingComponent """RiC-R074 ('is place associated with'
         relation)"""@en .

:isPlaceAssociatedWithAgent
    a owl:ObjectProperty ;
    rdfs:comment """Connects a Place to an Agent which is related to that
         Place."""@en ;
    rdfs:domain :Place ;
    rdfs:isDefinedBy <https://www.ica.org/standards/RiC/ontology> ;
    rdfs:label "es lugar asociado con agente"@es, "est un lieu associé à l'agent"@fr, "is place associated with agent"@en ;
    rdfs:range :Agent ;
    rdfs:subPropertyOf :isPlaceAssociatedWith ;
    owl:inverseOf :isAgentAssociatedWithPlace ;
    skos:changeNote [
        dc:date "2023-11-27" ;
        rdf:value "Added a new rdfs:label in Spanish."@en
    ], [
        dc:date "2023-10-26" ;
        rdf:value """fixed the domain and range, added a rdfs:comment and English
               and French labels."""@en
    ], [
        dc:date "2023-10-19" ;
        rdf:value "Added for RiC-O v1.0."@en
    ] .

:isProductionTechniqueTypeOf
    a owl:ObjectProperty ;
    rdfs:comment """Connects a Production Technique Type to an Instantiation whose
         production technique is categorized by it."""@en ;
    rdfs:domain :ProductionTechniqueType ;
    rdfs:isDefinedBy <https://www.ica.org/standards/RiC/ontology> ;
    rdfs:label "es tipo de técnica de producción de"@es, "est le type de technique de production de"@fr, "is production technique type of"@en ;
    rdfs:range :Instantiation ;
    rdfs:subPropertyOf :isOrWasTypeOf ;
    owl:inverseOf :hasProductionTechniqueType ;
    skos:changeNote [
        dc:date "2023-11-02" ;
        rdf:value "Added a new rdfs:label in Spanish."@en
    ], [
        dc:date "2023-08-28" ;
        rdf:value "Added a new rdfs:label in French."@en
    ], [
        dc:date "2021-01-22" ;
        rdf:value "changed the super property IRI."@en
    ] .

:isPublicationDateOf
    a owl:ObjectProperty ;
    rdfs:comment """Connects a Date to a Record Resource that was or will be made
         public at this Date."""@en ;
    rdfs:domain :Date ;
    rdfs:isDefinedBy <https://www.ica.org/standards/RiC/ontology> ;
    rdfs:label "es fecha de publicación de"@es, "est la date de publication de"@fr, "is publication date of"@en ;
    rdfs:range :RecordResource ;
    rdfs:subPropertyOf :isDateAssociatedWith ;
    owl:inverseOf :hasPublicationDate ;
    skos:changeNote [
        dc:date "2025-03-01" ;
        rdf:value """Made the property a subproperty of isDateAssociatedWith
               (instead of isBeginningDateOf)."""@en
    ], [
        dc:date "2025-02-19" ;
        rdf:value "Changed definition (added \"or will be\")."@en
    ], [
        dc:date "2023-11-27" ;
        rdf:value "Added a new rdfs:label in Spanish."@en
    ], [
        dc:date "2023-10-12" ;
        rdf:value "Added the French label"@en
    ], [
        dc:date "2023-09-22" ;
        rdf:value "Added in RiC-O 1.0."@en
    ] .

:isPublisherOf
    a owl:ObjectProperty ;
    rdfs:comment """Connects an Agent to a Record Resource that it
         published."""@en ;
    rdfs:domain :Agent ;
    rdfs:isDefinedBy <https://www.ica.org/standards/RiC/ontology> ;
    rdfs:label "es editor(a) de"@es, "est l’éditeur de"@fr, "is publisher of"@en ;
    rdfs:range :RecordResource ;
    rdfs:subPropertyOf :isRelatedTo ;
    owl:inverseOf :hasPublisher ;
    skos:changeNote [
        dc:date "2023-11-02" ;
        rdf:value "Added a new rdfs:label in Spanish."@en
    ], [
        dc:date "2023-08-28" ;
        rdf:value "Added a new rdfs:label in French."@en
    ], [
        dc:date "2021-01-22" ;
        rdf:value """changed the IRI, label, inverse property IRI (the name of this
               property in RiC-O 0.1 was \"publishes\")."""@en
    ] .

:isReceiverOf
    a owl:ObjectProperty ;
    rdfs:comment "Inverse of 'received by' object property."@en ;
    rdfs:domain :Agent ;
    rdfs:isDefinedBy <https://www.ica.org/standards/RiC/ontology> ;
    rdfs:label "es receptor(a) de"@es, "is receiver of"@en, "reçoit"@fr ;
    rdfs:range [
        a owl:Class ;
        owl:unionOf (:Instantiation
            :RecordResource
        )
    ] ;
    rdfs:subPropertyOf :isAccumulatorOf ;
    owl:inverseOf :hasReceiver ;
    skos:changeNote [
        dc:date "2023-11-02" ;
        rdf:value "Added a new rdfs:label in Spanish."@en
    ], [
        dc:date "2023-08-28" ;
        rdf:value "Added a new rdfs:label in French."@en
    ], [
        dc:date "2021-01-22" ;
        rdf:value """changed the IRI, label, inverse property IRI, super property
               IRI (changed made in order to make RiC-O compliant with RiC-CM 0.2; the name of this
               property in RiC-O 0.1 was \"receives\")."""@en
    ] ;
    :RiCCMCorrespondingComponent """RiC-R029i ('is receiver of'
         relation)"""@en .

:isRecordResourceAssociatedWithRecordResource
    a owl:ObjectProperty, owl:SymmetricProperty ;
    rdfs:comment """Connects two Record Resources. This relation is
         symmetric."""@en ;
    rdfs:domain :RecordResource ;
    rdfs:isDefinedBy <https://www.ica.org/standards/RiC/ontology> ;
    rdfs:label "es recurso documental asociado con"@es, """est une ressource archivistique associée avec la ressource
         archivistique"""@fr, "is record resource associated with record resource"@en ;
    rdfs:range :RecordResource ;
    rdfs:subPropertyOf :isRelatedTo ;
    owl:propertyChainAxiom (:thingIsConnectedToRelation
        :recordResourceToRecordResourceRelation_role
        :relationConnects
    ) ;
    skos:changeNote [
        dc:date "2023-11-25" ;
        rdf:value "Fixed the French label."@en
    ], [
        dc:date "2023-11-12" ;
        rdf:value """Aligned with RiC-CM 1.0: updated the description
               (rdfs:comment), skos:scopeNote."""@en
    ], [
        dc:date "2023-11-08" ;
        rdf:value """In order to get a system of rolified Relation classes: modified
               the property chain axiom so that it now involves the new
               recordResourceToRecordResourceRelation_role object property."""@en
    ], [
        dc:date "2023-11-02" ;
        rdf:value "Added a new rdfs:label in Spanish."@en
    ], [
        dc:date "2023-08-28" ;
        rdf:value "Added a new rdfs:label in French."@en
    ] ;
    skos:scopeNote """Use to connect two Record Resources only if it is not possible
         to use a narrower, more specific relation, for example has genetic link
         to."""@en ;
    :RiCCMCorrespondingComponent """RiC-R022 ('is record resource associated with
         record resource' relation)"""@en .

:isRecordSetTypeOf
    a owl:ObjectProperty ;
    rdfs:comment """Connects a Record Set Type to a Record Set that it
         categorizes."""@en ;
    rdfs:domain :RecordSetType ;
    rdfs:isDefinedBy <https://www.ica.org/standards/RiC/ontology> ;
    rdfs:label "es tipo de agrupación documental de"@es, "est le type d’ensemble d’objets informationnels de"@fr, "is record set type of"@en ;
    rdfs:range :RecordSet ;
    rdfs:subPropertyOf :isOrWasTypeOf ;
    owl:inverseOf :hasRecordSetType ;
    skos:changeNote [
        dc:date "2023-11-02" ;
        rdf:value "Added a new rdfs:label in Spanish."@en
    ], [
        dc:date "2023-08-28" ;
        rdf:value "Added a new rdfs:label in French."@en
    ], [
        dc:date "2021-01-22" ;
        rdf:value "changed the super property IRI."@en
    ] .

:isRecordStateOf
    a owl:ObjectProperty ;
    rdfs:comment """Connects a Record State to a Record or Record Part whose state it
         categorizes."""@en ;
    rdfs:domain :RecordState ;
    rdfs:isDefinedBy <https://www.ica.org/standards/RiC/ontology> ;
    rdfs:label "es estado de documento de"@es, "est l’état de"@fr, "is record state of"@en ;
    rdfs:range [
        a owl:Class ;
        owl:unionOf (:Record
            :RecordPart
        )
    ] ;
    rdfs:subPropertyOf :isOrWasTypeOf ;
    owl:inverseOf :hasRecordState ;
    skos:changeNote [
        dc:date "2023-11-02" ;
        rdf:value "Added a new rdfs:label in Spanish."@en
    ], [
        dc:date "2023-08-28" ;
        rdf:value "Added a new rdfs:label in French."@en
    ], [
        dc:date "2020-12-28" ;
        rdf:value """Changed the IRI, label, textual definition and range (Record
               Resource removed, replaced by Record or Record Part)."""@en
    ] .

:isRelatedTo
    a owl:ObjectProperty, owl:SymmetricProperty ;
    rdfs:comment """The most generic relation, is related to, connects any Thing to
         any other Thing. This relation is symmetric."""@en ;
    rdfs:domain :Thing ;
    rdfs:isDefinedBy <https://www.ica.org/standards/RiC/ontology> ;
    rdfs:label "est relié à"@fr, "está relacionado con"@es, "is related to"@en ;
    rdfs:range :Thing ;
    owl:propertyChainAxiom (:thingIsConnectedToRelation
        :relation_role
        :relationConnects
    ) ;
    skos:changeNote [
        dc:date "2023-11-12" ;
        rdf:value """Aligned with RiC-CM 1.0: updated the description
               (rdfs:comment)."""@en
    ], [
        dc:date "2023-11-08" ;
        rdf:value """Added the property chain axiom in order to make this property a
               shortcut."""@en
    ], [
        dc:date "2023-11-02" ;
        rdf:value "Added a new rdfs:label in Spanish."@en
    ], [
        dc:date "2023-08-28" ;
        rdf:value "Added a new rdfs:label in French."@en
    ] ;
    :RiCCMCorrespondingComponent """RiC-R001 ('is related to'
         relation)"""@en .

:isReplyTo
    a owl:ObjectProperty ;
    rdfs:comment "Inverse of 'has reply' object property."@en ;
    rdfs:domain :RecordResource ;
    rdfs:isDefinedBy <https://www.ica.org/standards/RiC/ontology> ;
    rdfs:label "es contestación de"@es, "est une réponse à"@fr, "is reply to"@en ;
    rdfs:range :RecordResource ;
    rdfs:subPropertyOf :followsInTime, :isRecordResourceAssociatedWithRecordResource ;
    owl:inverseOf :hasReply ;
    skos:changeNote [
        dc:date "2023-11-02" ;
        rdf:value "Added a new rdfs:label in Spanish."@en
    ], [
        dc:date "2023-08-28" ;
        rdf:value "Added a new rdfs:label in French."@en
    ], [
        dc:date "2021-01-22" ;
        rdf:value """changed the IRI, label, inverse property IRI, text definition
               (changed made in order to make RiC-O compliant with RiC-CM 0.2; the name of this
               property in RiC-O 0.1 was \"repliesTo\")."""@en
    ] ;
    :RiCCMCorrespondingComponent """RiC-R013i ('is reply to'
         relation)"""@en .

:isRepresentationTypeOf
    a owl:ObjectProperty ;
    rdfs:comment """Connects a Representation Type to an Instantiation that it
         categorizes."""@en ;
    rdfs:domain :RepresentationType ;
    rdfs:isDefinedBy <https://www.ica.org/standards/RiC/ontology> ;
    rdfs:label "es tipo de grabación de"@es, "est le type de représentation de"@fr, "is representation type of"@en ;
    rdfs:range :Instantiation ;
    rdfs:subPropertyOf :isOrWasTypeOf ;
    owl:inverseOf :hasRepresentationType ;
    skos:changeNote [
        dc:date "2023-11-02" ;
        rdf:value "Added a new rdfs:label in Spanish."@en
    ], [
        dc:date "2023-08-28" ;
        rdf:value "Added a new rdfs:label in French."@en
    ], [
        dc:date "2021-01-22" ;
        rdf:value "changed the super property IRI."@en
    ] .

:isRepresentedByContentOf
    a owl:ObjectProperty ;
    rdfs:comment """Inverse of 'has content which represents' object
         property."""@en ;
    rdfs:domain :Thing ;
    rdfs:isDefinedBy <https://www.ica.org/standards/RiC/ontology> ;
    rdfs:label "es representado por el contenido de"@es, "est représenté par le contenu de"@fr, "is represented by content of"@en ;
    rdfs:range [
        a owl:Class ;
        owl:unionOf (:Record
            :RecordPart
        )
    ] ;
    rdfs:subPropertyOf :isOrWasSubjectOf ;
    owl:inverseOf :hasContentWhichRepresents ;
    skos:changeNote [
        dc:date "2025-04-04" ;
        rdf:value "Introduced in RiC-O 1.1."@en
    ] .

:isResponsibleForIssuing
    a owl:ObjectProperty ;
    rdfs:comment "Inverse of 'issued by' object property."@en ;
    rdfs:domain :Agent ;
    rdfs:isDefinedBy <https://www.ica.org/standards/RiC/ontology> ;
    rdfs:label "es responsable de emisión de"@es, "est chargé de rendre publique"@fr, "is responsible for issuing"@en ;
    rdfs:range :Rule ;
    rdfs:subPropertyOf :isAssociatedWithRule ;
    owl:inverseOf :issuedBy ;
    skos:changeNote [
        dc:date "2023-11-02" ;
        rdf:value "Added a new rdfs:label in Spanish."@en
    ], [
        dc:date "2023-08-28" ;
        rdf:value "Added a new rdfs:label in French."@en
    ] ;
    :RiCCMCorrespondingComponent """RiC-R065i ('is responsible for issuing'
         relation)"""@en .

:isRuleAssociatedWith
    a owl:ObjectProperty ;
    rdfs:comment """Connects a Rule to a Thing that is associated with the
         Rule."""@en ;
    rdfs:domain :Rule ;
    rdfs:isDefinedBy <https://www.ica.org/standards/RiC/ontology> ;
    rdfs:label "es regla asociada con"@es, "est une règle associée à"@fr, "is rule associated with"@en ;
    rdfs:range :Thing ;
    rdfs:subPropertyOf :isRelatedTo ;
    owl:inverseOf :isAssociatedWithRule ;
    owl:propertyChainAxiom (:thingIsSourceOfRelation
        :ruleRelation_role
        :relationHasTarget
    ) ;
    skos:changeNote [
        dc:date "2023-11-12" ;
        rdf:value """Aligned with RiC-CM 1.0: updated the description
               (rdfs:comment), skos:scopeNote."""@en
    ], [
        dc:date "2023-11-08" ;
        rdf:value """In order to get a system of rolified Relation classes: modified
               the property chain axiom so that it now involves the new ruleRelation_role object
               property."""@en
    ], [
        dc:date "2023-11-02" ;
        rdf:value "Added a new rdfs:label in Spanish."@en
    ], [
        dc:date "2023-08-28" ;
        rdf:value "Added a new rdfs:label in French."@en
    ] ;
    skos:scopeNote """Use only if it is not possible to specify a narrower Rule
         relation, for example, regulates or regulated."""@en ;
    :RiCCMCorrespondingComponent """RiC-R062 ('is rule associated with'
         relation)"""@en .

:isSenderOf
    a owl:ObjectProperty ;
    rdfs:comment "Inverse of 'has sender' object property."@en ;
    rdfs:domain :Agent ;
    rdfs:isDefinedBy <https://www.ica.org/standards/RiC/ontology> ;
    rdfs:label "es remitente de"@es, "est l’expéditeur de"@fr, "is sender of"@en ;
    rdfs:range [
        a owl:Class ;
        owl:unionOf (:Instantiation
            :RecordResource
        )
    ] ;
    rdfs:subPropertyOf :isOrganicProvenanceOf ;
    owl:inverseOf :hasSender ;
    skos:changeNote [
        dc:date "2023-11-02" ;
        rdf:value "Added a new rdfs:label in Spanish."@en
    ], [
        dc:date "2023-08-28" ;
        rdf:value "Added a new rdfs:label in French."@en
    ] ;
    :RiCCMCorrespondingComponent """RiC-R031i ('is sender of'
         relation)"""@en .

:isSourceOfInformationOfRecordResource
    a owl:ObjectProperty ;
    rdfs:comment """Connects a Record Resource to a Record Resource, when the first is
         used as a source of information for producing the content of the second one."""@en ;
    rdfs:domain :RecordResource ;
    rdfs:isDefinedBy <https://www.ica.org/standards/RiC/ontology> ;
    rdfs:label "es fuente de información de recurso documental"@es, """est une source d’information de la ressource
         archivistique"""@fr, "is source of information of Record Resource"@en ;
    rdfs:range :RecordResource ;
    rdfs:subPropertyOf :isRecordResourceAssociatedWithRecordResource ;
    owl:inverseOf :recordResourceHasSourceOfInformation ;
    skos:changeNote [
        dc:date "2025-01-17" ;
        rdf:value """Object property added in RiC-O 1.1, with its inverse one. It
               replaces, as concerns Record Resources, the former 'isSourceOf' object property, that
               was available in RiC-0 0.1 and RiC-O 0.2, and was removed in RiC-O 1.0."""@en
    ] ;
    skos:scopeNote """Can be used, for example, for a Record Resource used to produce
         a Record having documentary form type Authority Record or Finding Aid. Not to be confused
         with the 'hasGeneticLinkToRecordResource' object property."""@en .

:isSubdivisionOfTransitive
    a owl:ObjectProperty, owl:TransitiveProperty ;
    rdfs:comment """Connects a Group to the Group it is a direct or indirect
         subdivision of. This is a transitive relation."""@en ;
    rdfs:domain :Group ;
    rdfs:isDefinedBy <https://www.ica.org/standards/RiC/ontology> ;
    rdfs:label "es subdivisión de transitivo"@es, "est une subdivision de transitif"@fr, "is subdivision of transitive"@en ;
    rdfs:range :Group ;
    rdfs:subPropertyOf :isOrWasSubdivisionOf, :isPartOfTransitive, :isSubordinateToTransitive ;
    owl:inverseOf :hasSubdivisionTransitive ;
    skos:changeNote [
        dc:date "2023-11-27" ;
        rdf:value "Added a new rdfs:label in Spanish."@en
    ], [
        dc:date "2023-11-12" ;
        rdf:value "Updated the labels."@en
    ], [
        dc:date "2023-09-08" ;
        rdf:value """Object property added, along with its inverse property, in
               order to enable to express current partitive relations between groups (the past
               partitive relation also being added)."""@en
    ] .

:isSubeventOfTransitive
    a owl:ObjectProperty, owl:TransitiveProperty ;
    rdfs:comment """Connects an ongoing Event to an Event of which it is a direct or
         indirect part. This is a transitive relation."""@en ;
    rdfs:domain :Event ;
    rdfs:isDefinedBy <https://www.ica.org/standards/RiC/ontology> ;
    rdfs:label "es elemento constitutivo de transitivo"@es, "est un événement constituant de transitif"@fr, "is subevent of transitive"@en ;
    rdfs:range :Event ;
    rdfs:subPropertyOf :isOrWasSubeventOf, :isPartOfTransitive ;
    owl:inverseOf :hasSubeventTransitive ;
    skos:changeNote [
        dc:date "2023-11-27" ;
        rdf:value "Added a new rdfs:label in Spanish."@en
    ], [
        dc:date "2023-11-12" ;
        rdf:value "Updated the labels."@en
    ], [
        dc:date "2023-09-08" ;
        rdf:value """Object property added, along with its inverse property, in
               order to enable to express partitive relations between ongoing events (the past
               partitive relation also being added)."""@en
    ] .

:isSubordinateToTransitive
    a owl:ObjectProperty, owl:TransitiveProperty ;
    rdfs:comment """Connects an Agent to an Agent that is directly or indirectly
         hierarchically superior. This is a transitive relation."""@en ;
    rdfs:domain :Agent ;
    rdfs:isDefinedBy <https://www.ica.org/standards/RiC/ontology> ;
    rdfs:label "est subalterne de transitif"@fr, "está subordinado(a) a transitivo"@es, "is subordinate to transitive"@en ;
    rdfs:range :Agent ;
    rdfs:subPropertyOf :isOrWasSubordinateTo ;
    owl:inverseOf :hasSubordinateTransitive ;
    skos:changeNote [
        dc:date "2023-11-27" ;
        rdf:value "Added a new rdfs:label in Spanish."@en
    ], [
        dc:date "2023-11-12" ;
        rdf:value "Updated the labels."@en
    ], [
        dc:date "2023-09-08" ;
        rdf:value """Object property added, along with its inverse property, in
               order to enable to express current subordination relations between agents (the past
               subordination relation also being added)."""@en
    ] .

:isSuccessorOf
    a owl:ObjectProperty ;
    rdfs:comment "Inverse of 'has successor' object property."@en ;
    rdfs:domain :Agent ;
    rdfs:isDefinedBy <https://www.ica.org/standards/RiC/ontology> ;
    rdfs:label "es sucesor(a) de"@es, "est le successeur de"@fr, "is successor of"@en ;
    rdfs:range :Agent ;
    rdfs:subPropertyOf :followsInTime, :isAgentAssociatedWithAgent ;
    owl:inverseOf :hasSuccessor ;
    owl:propertyChainAxiom (:thingIsTargetOfRelation
        :agentTemporalRelation_role
        :relationHasSource
    ) ;
    skos:changeNote [
        dc:date "2023-11-08" ;
        rdf:value """In order to get a system of rolified Relation classes: modified
               the property chain axiom so that it now involves the new agentTemporalRelation_role
               object property."""@en
    ], [
        dc:date "2023-11-02" ;
        rdf:value "Added a new rdfs:label in Spanish."@en
    ], [
        dc:date "2023-08-28" ;
        rdf:value "Added a new rdfs:label in French."@en
    ], [
        dc:date "2021-01-22" ;
        rdf:value """changed the inverse property IRI and the text
               definition."""@en
    ] ;
    :RiCCMCorrespondingComponent """RiC-R016i ('is successor of'
         relation)"""@en .

:isTitleTypeOf
    a owl:ObjectProperty ;
    rdfs:comment """Connects a Title Type and a Title that it
         categorizes."""@en ;
    rdfs:domain :TitleType ;
    rdfs:isDefinedBy <https://www.ica.org/standards/RiC/ontology> ;
    rdfs:label "es tipo de título de"@es, "est le type de titre de"@fr, "is title type of"@en ;
    rdfs:range :Title ;
    rdfs:subPropertyOf :isOrWasTypeOf ;
    owl:inverseOf :hasTitleType ;
    skos:changeNote [
        dc:date "2024-10-04" ;
        rdf:value """Object property added along with TitleType class and
               hasTitleType object property. """@en
    ] .

:isToUseDateOf
    a owl:ObjectProperty ;
    rdfs:comment """Connects a Date to an Appellation, when it is the date till which
         the Appellation was used."""@en ;
    rdfs:domain :Date ;
    rdfs:isDefinedBy <https://www.ica.org/standards/RiC/ontology> ;
    rdfs:label "es fecha hasta la que se usa"@es, "est la date jusqu’à laquelle est utilisé"@fr, "is to use date of"@en ;
    rdfs:range :Appellation ;
    rdfs:subPropertyOf :isEndDateOf ;
    owl:inverseOf :wasUsedToDate ;
    skos:changeNote [
        dc:date "2023-11-02" ;
        rdf:value "Added a new rdfs:label in Spanish."@en
    ], [
        dc:date "2023-10-19" ;
        rdf:value "Made this property a subPropertyOf isEndDateOf."@en
    ], [
        dc:date "2023-08-28" ;
        rdf:value "Added a new rdfs:label in French."@en
    ] .

:isUnitOfMeasurementOf
    a owl:ObjectProperty ;
    rdfs:comment """Inverse of 'has unit of measurement' object
         property."""@en ;
    rdfs:domain :UnitOfMeasurement ;
    rdfs:isDefinedBy <https://www.ica.org/standards/RiC/ontology> ;
    rdfs:label "es unidad de medida de"@es, "est l’unité de mesure de"@fr, "is unit of measurement of"@en ;
    rdfs:range :Extent ;
    rdfs:subPropertyOf :isRelatedTo ;
    owl:inverseOf :hasUnitOfMeasurement ;
    skos:changeNote [
        dc:date "2023-11-02" ;
        rdf:value "Added a new rdfs:label in Spanish."@en
    ], [
        dc:date "2023-08-28" ;
        rdf:value """Added a new rdfs:label in French; added an xml:lang attribute
               to the rdfs:comment."""@en
    ], [
        dc:date "2020-10-28" ;
        rdf:value """Object property created along with Extent and UnitOfMeasurement
               classes, in order to provide methods for handling extent accurately."""@en
    ] .

:isWithin
    a owl:ObjectProperty ;
    rdfs:comment "Connects a Date to a Date in which it is contained."@en ;
    rdfs:domain :Date ;
    rdfs:isDefinedBy <https://www.ica.org/standards/RiC/ontology> ;
    rdfs:label "est contenu dans"@fr, "está dentro"@es, "is within"@en ;
    rdfs:range :Date ;
    rdfs:subPropertyOf :isAssociatedWithDate, :isDateAssociatedWith, :isOrWasPartOf ;
    owl:inverseOf :hasWithin ;
    skos:changeNote [
        dc:date "2023-11-27" ;
        rdf:value "Added a new rdfs:label in Spanish."@en
    ], [
        dc:date "2023-10-13" ;
        rdf:value """made this property a subproperty of both isDateAssociatedWith
               and isAssociatedWithdate, and of isOrWasPartOf."""@en
    ], [
        dc:date "2023-10-12" ;
        rdf:value "Added the property"@en
    ] ;
    :RiCCMCorrespondingComponent """RiC-R085 ('is within'
         relation)"""@en .

:issuedBy
    a owl:ObjectProperty ;
    rdfs:comment """Connects a Rule to the Agent that issued or published the
         Rule."""@en ;
    rdfs:domain :Rule ;
    rdfs:isDefinedBy <https://www.ica.org/standards/RiC/ontology> ;
    rdfs:label "emitido por"@es, "issued by"@en, "rendue publique par"@fr ;
    rdfs:range :Agent ;
    rdfs:subPropertyOf :isRuleAssociatedWith ;
    owl:inverseOf :isResponsibleForIssuing ;
    skos:changeNote [
        dc:date "2023-11-02" ;
        rdf:value "Added a new rdfs:label in Spanish."@en
    ], [
        dc:date "2023-08-28" ;
        rdf:value "Added a new rdfs:label in French."@en
    ] ;
    :RiCCMCorrespondingComponent """RiC-R065 ('issued by'
         relation)"""@en .

:knowingOfRelation_role
    a owl:ObjectProperty ;
    rdfs:comment """Connects a KnowingOfRelation to itself. It is a property that can
         stand for an instance of the class when necessary, e.g. when you explore a knowledge
         graph."""@en ;
    rdfs:domain :KnowingOfRelation ;
    rdfs:isDefinedBy <https://www.ica.org/standards/RiC/ontology> ;
    rdfs:label """a le rôle de la Relation de connaissance à propos d’une
         personne"""@fr, """desempeña el papel de la Relación de conocimieto indirecto entre
         personas"""@es, "has the role of the Knowing Of Relation"@en ;
    rdfs:range :KnowingOfRelation ;
    rdfs:subPropertyOf :agentToAgentRelation_role ;
    skos:changeNote [
        dc:date "2024-08-02" ;
        rdf:value """Removed global reflexivity (leads to
               inconsistency)."""@en
    ], [
        dc:date "2023-11-08" ;
        rdf:value """In order to get a system of rolified Relation classes: created
               the object property, with domain and range the KnowingOfRelation rolified class.
               Declared it as reflexive. Declared it(s) superproperty(ies)."""@en
    ] ;
    skos:scopeNote """This property \"rolifies\" the KnowingOfRelation class. It should
         be used only when you have to manage instances of the KnowingOfRelation class, to connect
         each instance to itself, in order to be able to infer, using OWL-RL and property paths, the
         two shortcuts corresponding to this n-ary class."""@en .

:knowingRelation_role
    a owl:ObjectProperty ;
    rdfs:comment """Connects a KnowingRelation to itself. It is a property that can
         stand for an instance of the class when necessary, e.g. when you explore a knowledge
         graph."""@en ;
    rdfs:domain :KnowingRelation ;
    rdfs:isDefinedBy <https://www.ica.org/standards/RiC/ontology> ;
    rdfs:label """a le rôle de la Relation de connaissance entre
         personnes"""@fr, """desempeña el papel de la Relación de conocimiento directo entre
         personas"""@es, "has the role of the Knowing Relation"@en ;
    rdfs:range :KnowingRelation ;
    rdfs:subPropertyOf :agentToAgentRelation_role ;
    skos:changeNote [
        dc:date "2024-08-02" ;
        rdf:value """Removed global reflexivity (leads to
               inconsistency)."""@en
    ], [
        dc:date "2023-11-08" ;
        rdf:value """In order to get a system of rolified Relation classes: created
               the object property, with domain and range the KnowingRelation rolified class.
               Declared it as reflexive. Declared it(s) superproperty(ies)."""@en
    ] ;
    skos:scopeNote """This property \"rolifies\" the KnowingRelation class. It should be
         used only when you have to manage instances of the KnowingRelation class, to connect each
         instance to itself, in order to be able to infer, using OWL-RL and property paths, the two
         shortcuts corresponding to this n-ary class."""@en .

:knownBy
    a owl:ObjectProperty ;
    rdfs:comment "Inverse of 'knows of' object property."@en ;
    rdfs:domain :Person ;
    rdfs:isDefinedBy <https://www.ica.org/standards/RiC/ontology> ;
    rdfs:label "conocido por"@es, "est connue par"@fr, "known by"@en ;
    rdfs:range :Person ;
    rdfs:subPropertyOf :isAgentAssociatedWithAgent ;
    owl:inverseOf :knowsOf ;
    owl:propertyChainAxiom (:thingIsTargetOfRelation
        :knowingOfRelation_role
        :relationHasSource
    ) ;
    skos:changeNote [
        dc:date "2023-11-08" ;
        rdf:value """In order to get a system of rolified Relation classes: modified
               the property chain axiom so that it now involves the new knowingOfRelation_role
               object property."""@en
    ], [
        dc:date "2023-11-02" ;
        rdf:value "Added a new rdfs:label in Spanish."@en
    ], [
        dc:date "2023-08-28" ;
        rdf:value "Added a new rdfs:label in French."@en
    ] ;
    :RiCCMCorrespondingComponent """RiC-R050i ('known by'
         relation)"""@en .

:knows
    a owl:ObjectProperty, owl:SymmetricProperty ;
    rdfs:comment """Connects two Persons that directly know each other during their
         existence. This relation is symmetric."""@en ;
    rdfs:domain :Person ;
    rdfs:isDefinedBy <https://www.ica.org/standards/RiC/ontology> ;
    rdfs:label "connaît"@fr, "conoce a"@es, "knows"@en ;
    rdfs:range :Person ;
    rdfs:subPropertyOf :isAgentAssociatedWithAgent ;
    owl:propertyChainAxiom (:thingIsConnectedToRelation
        :knowingRelation_role
        :relationConnects
    ) ;
    skos:changeNote [
        dc:date "2023-11-12" ;
        rdf:value """Aligned with RiC-CM 1.0: updated the description
               (rdfs:comment), skos:scopeNote."""@en
    ], [
        dc:date "2023-11-08" ;
        rdf:value """In order to get a system of rolified Relation classes: modified
               the property chain axiom so that it now involves the new knowingRelation_role object
               property."""@en
    ], [
        dc:date "2023-11-02" ;
        rdf:value "Added a new rdfs:label in Spanish."@en
    ], [
        dc:date "2023-08-28" ;
        rdf:value "Added a new rdfs:label in French."@en
    ] ;
    skos:scopeNote """The relation implies that the two Persons met or at least
         corresponded with each other."""@en ;
    :RiCCMCorrespondingComponent """RiC-R051 ('knows'
         relation)"""@en .

:knowsOf
    a owl:ObjectProperty ;
    rdfs:comment """Connects a Person to another Person they have some knowledge of
         through time or space."""@en ;
    rdfs:domain :Person ;
    rdfs:isDefinedBy <https://www.ica.org/standards/RiC/ontology> ;
    rdfs:label "a connaissance de la personne"@fr, "conoce indirectamente a"@es, "knows of"@en ;
    rdfs:range :Person ;
    rdfs:subPropertyOf :isAgentAssociatedWithAgent ;
    owl:inverseOf :knownBy ;
    owl:propertyChainAxiom (:thingIsSourceOfRelation
        :knowingOfRelation_role
        :relationHasTarget
    ) ;
    skos:changeNote [
        dc:date "2023-11-08" ;
        rdf:value """In order to get a system of rolified Relation classes: modified
               the property chain axiom so that it now involves the new knowingOfRelation_role
               object property."""@en
    ], [
        dc:date "2023-11-02" ;
        rdf:value "Added a new rdfs:label in Spanish."@en
    ], [
        dc:date "2023-08-28" ;
        rdf:value "Added a new rdfs:label in French."@en
    ] ;
    :RiCCMCorrespondingComponent """RiC-R050 ('knows of'
         relation)"""@en .

:lastModificationDate
    a owl:DatatypeProperty ;
    rdfs:comment "Date at which an entity was last updated."@en ;
    rdfs:domain :Thing ;
    rdfs:isDefinedBy <https://www.ica.org/standards/RiC/ontology> ;
    rdfs:label "date de dernière modification"@fr, "fecha de última modificación"@es, "last modification date"@en ;
    rdfs:range rdfs:Literal ;
    rdfs:subPropertyOf :modificationDate ;
    skos:changeNote [
        dc:date "2023-11-02" ;
        rdf:value "Added a new rdfs:label in Spanish."@en
    ], [
        dc:date "2023-08-25" ;
        rdf:value "Added a new rdfs:label in French."@en
    ] ;
    skos:scopeNote """Provided for usability reasons. May be deprecated and removed
         later on. Use only if you don't use Date classes for handling dates."""@en ;
    :RiCCMCorrespondingComponent """Datatype property specialized implementation of
         RiC-E18 (Date entity)"""@en .

:latitude
    a owl:DatatypeProperty ;
    rdfs:comment "Distance in degrees north or south of the equator."@en ;
    rdfs:domain :Coordinates ;
    rdfs:isDefinedBy <https://www.ica.org/standards/RiC/ontology> ;
    rdfs:label "latitud"@es, "latitude"@en, "latitude"@fr ;
    rdfs:range rdfs:Literal ;
    rdfs:subPropertyOf :measure ;
    skos:changeNote [
        dc:date "2023-11-02" ;
        rdf:value "Added a new rdfs:label in Spanish."@en
    ], [
        dc:date "2023-08-25" ;
        rdf:value "Added a new rdfs:label in French."@en
    ] ;
    skos:scopeNote """Property of the Coordinates class. If you don't use this class,
         use geographicalCoordinates property, a property of Place class."""@en .

:leadershipRelation_role
    a owl:ObjectProperty ;
    rdfs:comment """Connects a LeadershipRelation to itself. It is a property that can
         stand for an instance of the class when necessary, e.g. when you explore a knowledge
         graph."""@en ;
    rdfs:domain :LeadershipRelation ;
    rdfs:isDefinedBy <https://www.ica.org/standards/RiC/ontology> ;
    rdfs:label "a le rôle de la Relation de direction"@fr, "desempeña el papel de la Relación de liderazgo"@es, "has the role of the Leadership Relation"@en ;
    rdfs:range :LeadershipRelation ;
    rdfs:subPropertyOf :agentControlRelation_role ;
    skos:changeNote [
        dc:date "2024-08-02" ;
        rdf:value """Removed global reflexivity (leads to
               inconsistency)."""@en
    ], [
        dc:date "2023-11-08" ;
        rdf:value """In order to get a system of rolified Relation classes: created
               the object property, with domain and range the LeadershipRelation rolified class.
               Declared it as reflexive. Declared it(s) superproperty(ies)."""@en
    ] ;
    skos:scopeNote """This property \"rolifies\" the LeadershipRelation class. It should
         be used only when you have to manage instances of the LeadershipRelation class, to connect
         each instance to itself, in order to be able to infer, using OWL-RL and property paths, the
         two shortcuts corresponding to this n-ary class."""@en .

:leadershipWithPosition
    a owl:ObjectProperty ;
    rdfs:comment """Connects a Leadership Relation to the Position occupied by the
         leading Person."""@en ;
    rdfs:domain :LeadershipRelation ;
    rdfs:isDefinedBy <https://www.ica.org/standards/RiC/ontology> ;
    rdfs:label "leadership with position"@en, "liderazgo en puesto"@es, "relation de direction dans le cadre du poste"@fr ;
    rdfs:range :Position ;
    rdfs:subPropertyOf :relationHasContext ;
    owl:inverseOf :positionIsContextOfLeadershipRelation ;
    skos:changeNote [
        dc:date "2023-11-02" ;
        rdf:value "Added a new rdfs:label in Spanish."@en
    ], [
        dc:date "2023-08-28" ;
        rdf:value "Added a new rdfs:label in French."@en
    ] .

:length
    a owl:DatatypeProperty ;
    rdfs:comment "Length of an entity."@en ;
    rdfs:domain :Thing ;
    rdfs:isDefinedBy <https://www.ica.org/standards/RiC/ontology> ;
    rdfs:label "length"@en, "longitud"@es, "longueur"@fr ;
    rdfs:range rdfs:Literal ;
    rdfs:subPropertyOf :measure ;
    skos:changeNote [
        dc:date "2023-11-12" ;
        rdf:value "Added a new rdfs:label in Spanish."@en
    ], [
        dc:date "2023-08-28" ;
        rdf:value """Added for enabling to describe entities that have such a
               dimension."""@en
    ] ;
    skos:scopeNote """May be used, among other cases, for storing the length of some
         places like streets."""@en .

:location
    a owl:DatatypeProperty ;
    rdfs:comment """A delimitation of the physical territory of a Place. Used to
         describe basic human-readable text such as an address, a cadastral reference, or less
         precise information found in a Record."""@en ;
    rdfs:domain :Place ;
    rdfs:isDefinedBy <https://www.ica.org/standards/RiC/ontology> ;
    rdfs:label "localisation"@fr, "localización"@es, "location"@en ;
    rdfs:range rdfs:Literal ;
    skos:changeNote [
        dc:date "2023-11-11" ;
        rdf:value """Aligned with RiC-CM 1.0: updated the description
               (rdfs:comment), skos:scopeNote, examples (skos:example)."""@en
    ], [
        dc:date "2023-11-02" ;
        rdf:value "Added a new rdfs:label in Spanish."@en
    ], [
        dc:date "2023-08-25" ;
        rdf:value "Added a new rdfs:label in French."@en
    ], [
        dc:date "2020-11-01" ;
        rdf:value """Text definition and scope note updated. Examples added.
               Objective: to make RiC-O compliant with RiC-CM v0.2."""@en
    ] ;
    skos:example "25 rue Saint-Denis à Paris"@fr, "Montreal (city in Canada)"@en ;
    skos:scopeNote """Use only if you don't use PhysicalLocation class with Place. Use
         the geographicalCoordinates property, or the Coordinates class, to record the geographical
         coordinates of the Place. Use the spatial relations (particularly 'has or had location') to
         capture a relation between two places."""@en ;
    :RiCCMCorrespondingComponent """Corresponds to RiC-A27 (Location
         attribute)"""@en .

:longitude
    a owl:DatatypeProperty ;
    rdfs:comment """Distance in degrees east or west of a prime
         meridian."""@en ;
    rdfs:domain :Coordinates ;
    rdfs:isDefinedBy <https://www.ica.org/standards/RiC/ontology> ;
    rdfs:label "longitud"@es, "longitude"@en, "longitude"@fr ;
    rdfs:range rdfs:Literal ;
    rdfs:subPropertyOf :measure ;
    skos:changeNote [
        dc:date "2023-11-02" ;
        rdf:value "Added a new rdfs:label in Spanish."@en
    ], [
        dc:date "2023-08-25" ;
        rdf:value "Added a new rdfs:label in French."@en
    ] ;
    skos:scopeNote """Property of the Coordinates class. If you don't use this class,
         use geographicalCoordinates property, a property of Place class."""@en .

:managementRelation_role
    a owl:ObjectProperty ;
    rdfs:comment """Connects a ManagementRelation to itself. It is a property that can
         stand for an instance of the class when necessary, e.g. when you explore a knowledge
         graph."""@en ;
    rdfs:domain :ManagementRelation ;
    rdfs:isDefinedBy <https://www.ica.org/standards/RiC/ontology> ;
    rdfs:label "a le rôle de la Relation de gestion"@fr, "desempeña el papel de la Relación de gestión"@es, "has the role of the Management Relation"@en ;
    rdfs:range :ManagementRelation ;
    rdfs:subPropertyOf :authorityRelation_role ;
    skos:changeNote [
        dc:date "2024-08-02" ;
        rdf:value """Removed global reflexivity (leads to
               inconsistency)."""@en
    ], [
        dc:date "2023-11-08" ;
        rdf:value """In order to get a system of rolified Relation classes: created
               the object property, with domain and range the ManagementRelation rolified class.
               Declared it as reflexive. Declared it(s) superproperty(ies)."""@en
    ] ;
    skos:scopeNote """This property \"rolifies\" the ManagementRelation class. It should
         be used only when you have to manage instances of the ManagementRelation class, to connect
         each instance to itself, in order to be able to infer, using OWL-RL and property paths, the
         two shortcuts corresponding to this n-ary class."""@en .

:mandateRelation_role
    a owl:ObjectProperty ;
    rdfs:comment """Connects a MandateRelation to itself. It is a property that can
         stand for an instance of the class when necessary, e.g. when you explore a knowledge
         graph."""@en ;
    rdfs:domain :MandateRelation ;
    rdfs:isDefinedBy <https://www.ica.org/standards/RiC/ontology> ;
    rdfs:label "a le rôle de la Relation impliquant un mandat"@fr, "desempeña el papel de la Relación normativa"@es, "has the role of the Mandate Relation"@en ;
    rdfs:range :MandateRelation ;
    rdfs:subPropertyOf :ruleRelation_role ;
    skos:changeNote [
        dc:date "2024-08-02" ;
        rdf:value """Removed global reflexivity (leads to
               inconsistency)."""@en
    ], [
        dc:date "2023-11-08" ;
        rdf:value """In order to get a system of rolified Relation classes: created
               the object property, with domain and range the MandateRelation rolified class.
               Declared it as reflexive. Declared it(s) superproperty(ies)."""@en
    ] ;
    skos:scopeNote """This property \"rolifies\" the MandateRelation class. It should be
         used only when you have to manage instances of the MandateRelation class, to connect each
         instance to itself, in order to be able to infer, using OWL-RL and property paths, the two
         shortcuts corresponding to this n-ary class."""@en .

:measure
    a owl:DatatypeProperty ;
    rdfs:comment """The extent, quantity, amount, or degree of an entity, as
         determined by measurement or calculation."""@en ;
    rdfs:domain :Thing ;
    rdfs:isDefinedBy <https://www.ica.org/standards/RiC/ontology> ;
    rdfs:label "measure"@en, "medida"@es, "mesure"@fr ;
    rdfs:range rdfs:Literal ;
    skos:changeNote [
        dc:date "2023-11-02" ;
        rdf:value "Added a new rdfs:label in Spanish."@en
    ], [
        dc:date "2023-08-25" ;
        rdf:value "Added a new rdfs:label in French."@en
    ] .

:membershipRelation_role
    a owl:ObjectProperty ;
    rdfs:comment """Connects a MembershipRelation to itself. It is a property that can
         stand for an instance of the class when necessary, e.g. when you explore a knowledge
         graph."""@en ;
    rdfs:domain :MembershipRelation ;
    rdfs:isDefinedBy <https://www.ica.org/standards/RiC/ontology> ;
    rdfs:label "a le rôle de la Relation d’appartenance"@fr, "desempeña el papel de la Relación de membresía"@es, "has the role of the Membership Relation"@en ;
    rdfs:range :MembershipRelation ;
    rdfs:subPropertyOf :agentToAgentRelation_role ;
    skos:changeNote [
        dc:date "2024-08-02" ;
        rdf:value """Removed global reflexivity (leads to
               inconsistency)."""@en
    ], [
        dc:date "2023-11-08" ;
        rdf:value """In order to get a system of rolified Relation classes: created
               the object property, with domain and range the MembershipRelation rolified class.
               Declared it as reflexive. Declared it(s) superproperty(ies)."""@en
    ] ;
    skos:scopeNote """This property \"rolifies\" the MembershipRelation class. It should
         be used only when you have to manage instances of the MembershipRelation class, to connect
         each instance to itself, in order to be able to infer, using OWL-RL and property paths, the
         two shortcuts corresponding to this n-ary class."""@en .

:membershipWithPosition
    a owl:ObjectProperty ;
    rdfs:comment """Connects a Membership Relation to the Position occupied by the
         member Person(s)."""@en ;
    rdfs:domain :MembershipRelation ;
    rdfs:isDefinedBy <https://www.ica.org/standards/RiC/ontology> ;
    rdfs:label "membership with position"@en, "membresía en puesto"@es, "relation d’appartenance dans le cadre du poste"@fr ;
    rdfs:range :Position ;
    rdfs:subPropertyOf :relationHasContext ;
    owl:inverseOf :positionIsContextOfMembershipRelation ;
    skos:changeNote [
        dc:date "2023-11-02" ;
        rdf:value "Added a new rdfs:label in Spanish."@en
    ], [
        dc:date "2023-08-28" ;
        rdf:value "Added a new rdfs:label in French."@en
    ] .

:migratedFrom
    a owl:ObjectProperty ;
    rdfs:comment "Inverse of 'migrated into' object property."@en ;
    rdfs:domain :Instantiation ;
    rdfs:isDefinedBy <https://www.ica.org/standards/RiC/ontology> ;
    rdfs:label "a été produite par migration de"@fr, "migrado desde"@es, "migrated from"@en ;
    rdfs:range :Instantiation ;
    rdfs:subPropertyOf :isOrWasDerivedFromInstantiation ;
    owl:inverseOf :migratedInto ;
    owl:propertyChainAxiom (:thingIsTargetOfRelation
        :migrationRelation_role
        :relationHasSource
    ) ;
    skos:changeNote [
        dc:date "2023-11-08" ;
        rdf:value """In order to get a system of rolified Relation classes: modified
               the property chain axiom so that it now involves the new migrationRelation_role
               object property."""@en
    ], [
        dc:date "2023-11-02" ;
        rdf:value "Added a new rdfs:label in Spanish."@en
    ], [
        dc:date "2023-08-29" ;
        rdf:value """Updated subpropertyOf; this in order to make the specification
               compliant with RiC-CM 1.0."""@en
    ], [
        dc:date "2023-08-28" ;
        rdf:value "Added a new rdfs:label in French."@en
    ], [
        dc:date "2021-01-22" ;
        rdf:value """changed the IRI, label, inverse property IRI, text definition,
               corresponding CM component name (changed made in order to make RiC-O compliant with
               RiC-CM 0.2; the name of this property in RiC-O 0.1 was
               \"createdByMigrationFromInstantiation\")."""@en
    ] ;
    :RiCCMCorrespondingComponent """RiC-R015i ('migrated from'
         relation)"""@en .

:migratedInto
    a owl:ObjectProperty ;
    rdfs:comment """Connects an Instantiation to a version it has been migrated
         into."""@en ;
    rdfs:domain :Instantiation ;
    rdfs:isDefinedBy <https://www.ica.org/standards/RiC/ontology> ;
    rdfs:label "a été migrée vers"@fr, "migrado a"@es, "migrated into"@en ;
    rdfs:range :Instantiation ;
    rdfs:subPropertyOf :hasOrHadDerivedInstantiation ;
    owl:inverseOf :migratedFrom ;
    owl:propertyChainAxiom (:thingIsSourceOfRelation
        :migrationRelation_role
        :relationHasTarget
    ) ;
    skos:changeNote [
        dc:date "2023-11-12" ;
        rdf:value """Aligned with RiC-CM 1.0: updated the description
               (rdfs:comment)."""@en
    ], [
        dc:date "2023-11-08" ;
        rdf:value """In order to get a system of rolified Relation classes: modified
               the property chain axiom so that it now involves the new migrationRelation_role
               object property."""@en
    ], [
        dc:date "2023-11-02" ;
        rdf:value "Added a new rdfs:label in Spanish."@en
    ], [
        dc:date "2023-08-29" ;
        rdf:value """Updated subpropertyOf; this in order to make the specification
               compliant with RiC-CM 1.0."""@en
    ], [
        dc:date "2023-08-28" ;
        rdf:value "Added a new rdfs:label in French."@en
    ], [
        dc:date "2021-01-22" ;
        rdf:value """changed the IRI, label and inverse property IRI (changed made
               in order to make RiC-O compliant with RiC-CM 0.2; the name of this property in RiC-O
               0.1 was \"isMigratedIntoInstantiation\")."""@en
    ] ;
    skos:scopeNote "Use for digital instantiations."@en ;
    :RiCCMCorrespondingComponent """RiC-R015 ('migrated into'
         relation)"""@en .

:migrationDate
    a owl:DatatypeProperty ;
    rdfs:comment """Date at which an Instantiation was or will be
         migrated."""@en ;
    rdfs:domain :Instantiation ;
    rdfs:isDefinedBy <https://www.ica.org/standards/RiC/ontology> ;
    rdfs:label "date de migration"@fr, "fecha de migración"@es, "migration date"@en ;
    rdfs:range rdfs:Literal ;
    rdfs:subPropertyOf :derivationDate ;
    skos:changeNote [
        dc:date "2025-03-01" ;
        rdf:value """Removed 'Record Resource' from the definition and made the
               property a subproperty of the new 'derivationDate' property."""@en
    ], [
        dc:date "2025-02-19" ;
        rdf:value "Added in RiC-O 1.1."@en
    ] ;
    skos:scopeNote """Provided for usability reasons. May be deprecated and removed
         later on. Use only if you don't use Date classes for handling dates."""@en ;
    :RiCCMCorrespondingComponent """Datatype property specialized implementation of
         RiC-E18 (Date entity)"""@en .

:migrationRelation_role
    a owl:ObjectProperty ;
    rdfs:comment """Connects a MigrationRelation to itself. It is a property that can
         stand for an instance of the class when necessary, e.g. when you explore a knowledge
         graph."""@en ;
    rdfs:domain :MigrationRelation ;
    rdfs:isDefinedBy <https://www.ica.org/standards/RiC/ontology> ;
    rdfs:label "a le rôle de la Relation de migration"@fr, """desempeña el papel de la Relación de migración entre
         instanciaciones"""@es, "has the role of the Migration Relation"@en ;
    rdfs:range :MigrationRelation ;
    rdfs:subPropertyOf :derivationRelation_role ;
    skos:changeNote [
        dc:date "2024-08-02" ;
        rdf:value """Removed global reflexivity (leads to
               inconsistency)."""@en
    ], [
        dc:date "2023-11-08" ;
        rdf:value """In order to get a system of rolified Relation classes: created
               the object property, with domain and range the MigrationRelation rolified class.
               Declared it as reflexive. Declared it(s) superproperty(ies)."""@en
    ] ;
    skos:scopeNote """This property \"rolifies\" the MigrationRelation class. It should
         be used only when you have to manage instances of the MigrationRelation class, to connect
         each instance to itself, in order to be able to infer, using OWL-RL and property paths, the
         two shortcuts corresponding to this n-ary class."""@en .

:modificationDate
    a owl:DatatypeProperty ;
    rdfs:comment "Date of the modification of an entity."@en ;
    rdfs:domain :Thing ;
    rdfs:isDefinedBy <https://www.ica.org/standards/RiC/ontology> ;
    rdfs:label "date de modification"@fr, "fecha de modificación"@es, "modification date"@en ;
    rdfs:range rdfs:Literal ;
    rdfs:subPropertyOf :date ;
    skos:changeNote [
        dc:date "2023-11-02" ;
        rdf:value "Added a new rdfs:label in Spanish."@en
    ], [
        dc:date "2023-08-25" ;
        rdf:value "Added a new rdfs:label in French."@en
    ] ;
    skos:scopeNote """Provided for usability reasons. May be deprecated and removed
         later on. Use only if you don't use Date classes for handling dates."""@en ;
    :RiCCMCorrespondingComponent """Datatype property specialized implementation of
         RiC-E18 (Date entity)"""@en .

:mostMembersWithAccumulationDate
    a owl:DatatypeProperty ;
    rdfs:comment """Date at which most of the present or past members of a Record Set
         were or will be accumulated."""@en ;
    rdfs:domain :RecordSet ;
    rdfs:isDefinedBy <https://www.ica.org/standards/RiC/ontology> ;
    rdfs:label """des membres dont la plupart ont pour date
         d’accumulation"""@fr, "la mayoría de sus miembros como fecha de acumulación"@es, "most members with accumulation date"@en ;
    rdfs:range rdfs:Literal ;
    rdfs:subPropertyOf :someMembersWithAccumulationDate ;
    skos:changeNote [
        dc:date "2025-02-19" ;
        rdf:value "Changed definition (added \"or will be\")."@en
    ], [
        dc:date "2024-12-19" ;
        rdf:value "Added in RiC-O 1.1."@en
    ] ;
    skos:scopeNote """Datatype property analogue of
         'hasOrHadMostMembersWithAccumulationDate', which is provided for usability reasons. May be
         deprecated and removed later on. Use only if you don’t use Date classes for handling
         dates."""@en .

:mostMembersWithCreationDate
    a owl:DatatypeProperty ;
    rdfs:comment """Date at which most of the present or past members of a Record Set
         were or will be created."""@en ;
    rdfs:domain :RecordSet ;
    rdfs:isDefinedBy <https://www.ica.org/standards/RiC/ontology> ;
    rdfs:label "des membres dont la plupart ont pour date de création"@fr, "la mayoría de sus miembros como fecha de creación"@es, "most members with creation date"@en ;
    rdfs:range rdfs:Literal ;
    rdfs:subPropertyOf :someMembersWithCreationDate ;
    skos:changeNote [
        dc:date "2025-02-19" ;
        rdf:value "Changed definition (added \"or will be\")."@en
    ], [
        dc:date "2024-12-19" ;
        rdf:value "Added in RiC-O 1.1."@en
    ] ;
    skos:scopeNote """Datatype property analogue of
         'hasOrHadMostMembersWithCreationDate', which is provided for usability reasons. May be
         deprecated and removed later on. Use only if you don’t use Date classes for handling
         dates."""@en ;
    :RiCCMCorrespondingComponent """RiC-R083i ('has or had most members with creation
         date' relation)."""@en .

:name
    a owl:DatatypeProperty ;
    rdfs:comment """A label, title or term designating an entity in order to make it
         distinguishable from other similar entities."""@en ;
    rdfs:domain :Thing ;
    rdfs:isDefinedBy <https://www.ica.org/standards/RiC/ontology> ;
    rdfs:label "name"@en, "nom"@fr, "nombre"@es ;
    rdfs:range rdfs:Literal ;
    skos:changeNote [
        dc:date "2023-11-11" ;
        rdf:value """Aligned with RiC-CM 1.0: updated the description
               (rdfs:comment), skos:scopeNote, examples (skos:example)."""@en
    ], [
        dc:date "2023-11-02" ;
        rdf:value "Added a new rdfs:label in Spanish."@en
    ], [
        dc:date "2023-08-25" ;
        rdf:value "Added a new rdfs:label in French."@en
    ], [
        dc:date "2020-11-01" ;
        rdf:value """Text definition updated. Examples added. Objective: to make
               RiC-O compliant with RiC-CM v0.2."""@en
    ] ;
    skos:example "D-Day (about a Date or Event)"@en, """Digital copy of the Pomarius archival inventory from 1575 (about
         an Instantiation)"""@en, """Fundraising, University of Glasgow (about an
         Activity)"""@en, "Halloween 2016 (about a Date)"@en, "Nelson Mandela (about a Person)"@en, """Papers of the Earls of Liverpool (about a Record
         Set)"""@en, "Paris (about a Place)"@en, "Prime Minister (about a Position)"@en, "Providing hearing services (about an Activity)"@en, "Sketch Map of the Qatar Peninsula (about a Record)"@en, """The Letter of Neacsu from Campulung to the Mayor of Brasov (about
         a Record)"""@en ;
    skos:scopeNote """Use only if you don't use Name class for handling names.
         Provides brief information about the content or other individual characteristics of the
         entity being described, necessary to distinguish it from other perhaps similar
         entities."""@en ;
    :RiCCMCorrespondingComponent """Corrresponds to RiC-A28 (Name
         attribute)"""@en .

:normalizedDateValue
    a owl:DatatypeProperty ;
    rdfs:comment """Machine readable representation of the date based on a public
         technical standard."""@en ;
    rdfs:domain :Date ;
    rdfs:isDefinedBy <https://www.ica.org/standards/RiC/ontology> ;
    rdfs:label "normalized date value"@en, "valeur normalisée de la date"@fr, "valor normalizado de fecha"@es ;
    rdfs:range rdfs:Literal ;
    rdfs:subPropertyOf :normalizedValue ;
    skos:changeNote [
        dc:date "2024-09-02" ;
        rdf:value "Fixed a typo in two of the EDTF examples."@en
    ], [
        dc:date "2023-11-11" ;
        rdf:value """Aligned with RiC-CM 1.0: updated the examples
               (skos:example)."""@en
    ], [
        dc:date "2023-11-02" ;
        rdf:value "Added a new rdfs:label in Spanish."@en
    ], [
        dc:date "2023-10-10" ;
        rdf:value """Updated the rdfs:comment and examples, and added a scopeNote,
               in order to make this property fully compliant with RiC-CM 1.0."""@en
    ], [
        dc:date "2023-08-25" ;
        rdf:value "Added a new rdfs:label in French."@en
    ], [
        dc:date "2020-11-01" ;
        rdf:value """Examples added. Objective: to make RiC-O compliant with RiC-CM
               v0.2."""@en
    ] ;
    skos:example """1550,1551,1553,1555 (a date set in EDTF, meaning one of the years
         1550, 1551, 1553, 1555)"""@en, "1948-03 (an ISO 8601 form of a single date)"@en, "1948-03-08 (an ISO 8601 form of a single date)"@en, """1948-03~ (a single date in ETDF, meaning March 1948
         approximately)"""@en, """1948/ (a date range in EDTF, starting in 1948, end
         unknown)"""@en, """1948/.. (an open date range in EDTF, starting in
         1948)"""@en, """2012-02-14/2015-03-08 (an ISO 8601 form of a date
         range)"""@en, "2012/2015-03 (an ISO 8601 form of a date range)"@en, """{1550,1551,1553,1555} (a date set in EDTF, meaning all of the
         years 1550, 1551, 1553, 1555)"""@en, """{1805,1815..1820} (a date set in EDTF, meaning all of the years
         1805, 1815, 1816, 1817, 1818, 1819, 1820)"""@en ;
    skos:scopeNote """Used to represent the date in a standardized format that can be
         processed programmatically. The main standard used today is ISO 8601, which is based on the
         Gregorian calendar. See also the Extended Date Time Format (EDTF), which is an extension of
         ISO 8601, and enables, among other features, to represent a date set, and to indicate the
         date is approximate."""@en ;
    :RiCCMCorrespondingComponent """Corresponds to RiC-A29 (Normalized Date
         attribute)"""@en .

:normalizedValue
    a owl:DatatypeProperty ;
    rdfs:comment """Value representation based on a standard, preferably
         machine-readable."""@en ;
    rdfs:domain [
        a owl:Class ;
        owl:unionOf (:Appellation
            :Date
        )
    ] ;
    rdfs:isDefinedBy <https://www.ica.org/standards/RiC/ontology> ;
    rdfs:label "normalized value"@en, "valeur normalisée"@fr, "valor normalizado"@es ;
    rdfs:range rdfs:Literal ;
    rdfs:subPropertyOf :textualValue ;
    skos:changeNote [
        dc:date "2023-11-02" ;
        rdf:value "Added a new rdfs:label in Spanish."@en
    ], [
        dc:date "2023-08-25" ;
        rdf:value "Added a new rdfs:label in French."@en
    ] .

:note
    a owl:DatatypeProperty ;
    rdfs:comment """A short textual statement, that gives a little information on a
         specific feature of a Thing."""@en ;
    rdfs:domain :Thing ;
    rdfs:isDefinedBy <https://www.ica.org/standards/RiC/ontology> ;
    rdfs:label "nota"@es, "note"@en, "note"@fr ;
    rdfs:range rdfs:Literal ;
    skos:changeNote [
        dc:date "2025-01-17" ;
        rdf:value """Added in RiC-0 1.1, as a superproperty of any possible kind of
               note."""@en
    ] ;
    skos:scopeNote """Not to be confused with the rico:generalDescription datatype
         property, which is used to provide a textual description of a Thing. Use the subproperties
         of rico:note when they are appropriate."""@en .

:occupiesOrOccupied
    a owl:ObjectProperty ;
    rdfs:comment """Connects a Person to a Position they occupy or
         occupied."""@en ;
    rdfs:domain :Person ;
    rdfs:isDefinedBy <https://www.ica.org/standards/RiC/ontology> ;
    rdfs:label "occupe ou a occupé"@fr, "occupies or occupied"@en, "ocupa u ocupaba"@es ;
    rdfs:range :Position ;
    rdfs:subPropertyOf :isAgentAssociatedWithAgent ;
    owl:inverseOf :isOrWasOccupiedBy ;
    owl:propertyChainAxiom (:thingIsSourceOfRelation
        :positionHoldingRelation_role
        :relationHasTarget
    ) ;
    skos:changeNote [
        dc:date "2023-11-08" ;
        rdf:value """In order to get a system of rolified Relation classes: modified
               the property chain axiom so that it now involves the new positionHoldingRelation_role
               object property."""@en
    ], [
        dc:date "2023-11-02" ;
        rdf:value "Added a new rdfs:label in Spanish."@en
    ], [
        dc:date "2023-08-28" ;
        rdf:value "Added a new rdfs:label in French."@en
    ], [
        dc:date "2021-01-22" ;
        rdf:value """changed the IRI, label, inverse property IRI, text definition
               (changed made in order to make RiC-O compliant with RiC-CM 0.2; the name of this
               property in RiC-O 0.1 was \"occupies\")."""@en
    ] ;
    :RiCCMCorrespondingComponent """RiC-R054 ('occupies or occupied'
         relation)"""@en .

:occurredAtDate
    a owl:ObjectProperty ;
    rdfs:comment """Inverse of 'is date of occurrence of' object
         property."""@en ;
    rdfs:domain :Event ;
    rdfs:isDefinedBy <https://www.ica.org/standards/RiC/ontology> ;
    rdfs:label "a pour date d'occurrence"@fr, "occurred at date"@en, "tiene como fecha de ocurrencia"@es ;
    rdfs:range :Date ;
    rdfs:subPropertyOf :isAssociatedWithDate, :isEventAssociatedWith ;
    owl:inverseOf :isDateOfOccurrenceOf ;
    skos:changeNote [
        dc:date "2023-11-27" ;
        rdf:value "Added a new rdfs:label in Spanish."@en
    ], [
        dc:date "2023-10-17" ;
        rdf:value """Made this property a subproperty of
               isEventAssociatedWith"""@en
    ], [
        dc:date "2023-10-13" ;
        rdf:value """Renamed the property to correct a spelling mistake. Also
               corrected the annotations when necessary."""@en
    ] ;
    :RiCCMCorrespondingComponent """RiC-R084i ('occurred at date'
         relation)"""@en .

:organicOrFunctionalProvenanceRelation_role
    a owl:ObjectProperty ;
    rdfs:comment """Connects an OrganicOrFunctionalProvenanceRelation to itself. It is
         a property that can stand for an instance of the class when necessary, e.g. when you
         explore a knowledge graph."""@en ;
    rdfs:domain :OrganicOrFunctionalProvenanceRelation ;
    rdfs:isDefinedBy <https://www.ica.org/standards/RiC/ontology> ;
    rdfs:label """a le rôle de la Relation de provenance organique ou
         fonctionnelle"""@fr, """desempeña el papel de la Relación de procedencia orgánica or
         funcional"""@es, """has the role of the Organic or functional provenance
         Relation"""@en ;
    rdfs:range :OrganicOrFunctionalProvenanceRelation ;
    rdfs:subPropertyOf :relation_role ;
    skos:changeNote [
        dc:date "2024-08-02" ;
        rdf:value """Removed global reflexivity (leads to
               inconsistency)."""@en
    ], [
        dc:date "2023-11-08" ;
        rdf:value """In order to get a system of rolified Relation classes: created
               the object property, with domain and range the OrganicOrFunctionalProvenanceRelation
               rolified class. Declared it as reflexive. Declared it(s)
               superproperty(ies)."""@en
    ] ;
    skos:scopeNote """This property \"rolifies\" the
         OrganicOrFunctionalProvenanceRelation class. It should be used only when you have to manage
         instances of the OrganicOrFunctionalProvenanceRelation class, to connect each instance to
         itself, in order to be able to infer, using OWL-RL and property paths, the two shortcuts
         corresponding to this n-ary class."""@en .

:organicProvenanceRelation_role
    a owl:ObjectProperty ;
    rdfs:comment """Connects an OrganicProvenanceRelation to itself. It is a property
         that can stand for an instance of the class when necessary, e.g. when you explore a
         knowledge graph."""@en ;
    rdfs:domain :OrganicProvenanceRelation ;
    rdfs:isDefinedBy <https://www.ica.org/standards/RiC/ontology> ;
    rdfs:label "a le rôle de la Relation de provenance organique"@fr, """desempeña el papel de la Relación de procedencia
         orgánica"""@es, "has the role of the Organic Provenance Relation"@en ;
    rdfs:range :OrganicProvenanceRelation ;
    rdfs:subPropertyOf :organicOrFunctionalProvenanceRelation_role ;
    skos:changeNote [
        dc:date "2024-08-02" ;
        rdf:value """Removed global reflexivity (leads to
               inconsistency)."""@en
    ], [
        dc:date "2023-11-08" ;
        rdf:value """In order to get a system of rolified Relation classes: created
               the object property, with domain and range the OrganicProvenanceRelation rolified
               class. Declared it as reflexive. Declared it(s) superproperty(ies)."""@en
    ] ;
    skos:scopeNote """This property \"rolifies\" the OrganicProvenanceRelation class. It
         should be used only when you have to manage instances of the OrganicProvenanceRelation
         class, to connect each instance to itself, in order to be able to infer, using OWL-RL and
         property paths, the two shortcuts corresponding to this n-ary class."""@en .

:overlapsOrOverlapped
    a owl:ObjectProperty, owl:SymmetricProperty ;
    rdfs:comment """Connects two Places that geographically overlap or overlapped.
         This relation is symmetric."""@en ;
    rdfs:domain :Place ;
    rdfs:isDefinedBy <https://www.ica.org/standards/RiC/ontology> ;
    rdfs:label "chevauche ou a chevauché"@fr, "overlaps or overlapped"@en, "se superpone o superponía con"@es ;
    rdfs:range :Place ;
    rdfs:subPropertyOf :isAssociatedWithPlace, :isPlaceAssociatedWith ;
    skos:changeNote [
        dc:date "2023-11-12" ;
        rdf:value """Aligned with RiC-CM 1.0: updated the description
               (rdfs:comment)."""@en
    ], [
        dc:date "2023-11-02" ;
        rdf:value "Added a new rdfs:label in Spanish."@en
    ], [
        dc:date "2023-08-28" ;
        rdf:value "Added a new rdfs:label in French."@en
    ], [
        dc:date "2021-01-22" ;
        rdf:value """changed the IRI, label, text definition (changed made in order
               to make RiC-O compliant with RiC-CM 0.2; the name of this property in RiC-O 0.1 was
               \"overlaps\")."""@en
    ] ;
    :RiCCMCorrespondingComponent """RiC-R078 ('overlaps or overlapped'
         relation)"""@en .

:ownershipRelation_role
    a owl:ObjectProperty ;
    rdfs:comment """Connects an OwnershipRelation to itself. It is a property that can
         stand for an instance of the class when necessary, e.g. when you explore a knowledge
         graph."""@en ;
    rdfs:domain :OwnershipRelation ;
    rdfs:isDefinedBy <https://www.ica.org/standards/RiC/ontology> ;
    rdfs:label "a le rôle de la Relation de propriété"@fr, "desempeña el papel de la Relación de posesión"@es, "has the role of the Ownership Relation"@en ;
    rdfs:range :OwnershipRelation ;
    rdfs:subPropertyOf :authorityRelation_role ;
    skos:changeNote [
        dc:date "2024-08-02" ;
        rdf:value """Removed global reflexivity (leads to
               inconsistency)."""@en
    ], [
        dc:date "2023-11-08" ;
        rdf:value """In order to get a system of rolified Relation classes: created
               the object property, with domain and range the OwnershipRelation rolified class.
               Declared it as reflexive. Declared it(s) superproperty(ies)."""@en
    ] ;
    skos:scopeNote """This property \"rolifies\" the OwnershipRelation class. It should
         be used only when you have to manage instances of the OwnershipRelation class, to connect
         each instance to itself, in order to be able to infer, using OWL-RL and property paths, the
         two shortcuts corresponding to this n-ary class."""@en .

:performanceRelation_role
    a owl:ObjectProperty ;
    rdfs:comment """Connects a PerformanceRelation to itself. It is a property that
         can stand for an instance of the class when necessary, e.g. when you explore a knowledge
         graph."""@en ;
    rdfs:domain :PerformanceRelation ;
    rdfs:isDefinedBy <https://www.ica.org/standards/RiC/ontology> ;
    rdfs:label "a le rôle de la Relation entre activités et agents"@fr, """desempeña el papel de la Relación de desarrollo
         funcional"""@es, "has the role of the Performance Relation"@en ;
    rdfs:range :PerformanceRelation ;
    rdfs:subPropertyOf :eventRelation_role ;
    skos:changeNote [
        dc:date "2024-08-02" ;
        rdf:value """Removed global reflexivity (leads to
               inconsistency)."""@en
    ], [
        dc:date "2023-11-08" ;
        rdf:value """In order to get a system of rolified Relation classes: created
               the object property, with domain and range the PerformanceRelation rolified class.
               Declared it as reflexive. Declared it(s) superproperty(ies)."""@en
    ] ;
    skos:scopeNote """This property \"rolifies\" the PerformanceRelation class. It
         should be used only when you have to manage instances of the PerformanceRelation class, to
         connect each instance to itself, in order to be able to infer, using OWL-RL and property
         paths, the two shortcuts corresponding to this n-ary class."""@en .

:performsOrPerformed
    a owl:ObjectProperty ;
    rdfs:comment """Inverse of 'is or was performed by' object
         property."""@en ;
    rdfs:domain :Agent ;
    rdfs:isDefinedBy <https://www.ica.org/standards/RiC/ontology> ;
    rdfs:label "desarrolla o desarrollaba"@es, "exerce ou a exercé"@fr, "performs or performed"@en ;
    rdfs:range :Activity ;
    rdfs:subPropertyOf :isOrWasParticipantIn ;
    owl:inverseOf :isOrWasPerformedBy ;
    owl:propertyChainAxiom (:thingIsTargetOfRelation
        :performanceRelation_role
        :relationHasSource
    ) ;
    skos:changeNote [
        dc:date "2023-11-08" ;
        rdf:value """In order to get a system of rolified Relation classes: modified
               the property chain axiom so that it now involves the new performanceRelation_role
               object property."""@en
    ], [
        dc:date "2023-11-02" ;
        rdf:value "Added a new rdfs:label in Spanish."@en
    ], [
        dc:date "2023-08-28" ;
        rdf:value "Added a new rdfs:label in French."@en
    ], [
        dc:date "2021-01-22" ;
        rdf:value """changed the IRI, label, inverse property IRI, text definition,
               super property IRI (changed made in order to make RiC-O compliant with RiC-CM 0.2;
               the name of this property in RiC-O 0.1 was \"performs\")."""@en
    ] ;
    :RiCCMCorrespondingComponent """RiC-R060i ('performs or performed'
         relation)"""@en .

:physicalCharacteristicsNote
    a owl:DatatypeProperty ;
    rdfs:comment """Information about the physical features, completeness, or
         conservation status of an Instantiation. Includes information about the physical nature and
         condition such as conservation status or the deterioration of an Instantiation (for example
         its carrier) affecting the ability to recover information. """@en ;
    rdfs:domain :Instantiation ;
    rdfs:isDefinedBy <https://www.ica.org/standards/RiC/ontology> ;
    rdfs:label "nota sobre las características físicas"@es, "note sur les caractéristiques physiques"@fr, "physical characteristics note"@en ;
    rdfs:range rdfs:Literal ;
    rdfs:subPropertyOf :note ;
    skos:changeNote [
        dc:date "2025-01-17" ;
        rdf:value """Made this property a subproperty of the new rico:note datatype
               property."""@en
    ], [
        dc:date "2023-11-11" ;
        rdf:value """Aligned with RiC-CM 1.0: updated the IRI, mapping to RiC-CM
               (rico:RiCCMCorrespondingComponent), labels, description (rdfs:comment),
               skos:scopeNote, examples (skos:example)."""@en
    ], [
        dc:date "2023-11-02" ;
        rdf:value "Added a new rdfs:label in Spanish."@en
    ], [
        dc:date "2023-08-25" ;
        rdf:value "Added a new rdfs:label in French."@en
    ], [
        dc:date "2020-11-01" ;
        rdf:value """Text definition updated. Examples added. Objective: to make
               RiC-O compliant with RiC-CM v0.2."""@en
    ] ;
    skos:example """A web page (HTML, 15 images, 2 CSS, 1 JavaScript), with 1 CSS
         missing."""@en, "British Library binding"@en, "Digital file format: JPEG-2000"@en, """For carrier: hard drives on which the author wrote physically
         (using a pen)."""@en, """Letter physical characteristics: corner without text missing – the
         carrier is damaged, but no information of the content is missing"""@en, "The charter is missing the seal."@en, "Watermarked"@en, "carrier heavily foxed"@en, "some loss of text due to rodent damage"@en ;
    skos:scopeNote """Not to be confused with the intellectual completeness of a
         Record Resource and its sub-entities, which is covered by the Integrity attribute. May
         include digital file fixity. """@en ;
    :RiCCMCorrespondingComponent """Corresponds to RiC-A31 (Physical Characteristics
         Note attribute)"""@en .

:physicalOrLogicalExtent
    a owl:DatatypeProperty ;
    rdfs:comment """Countable characteristics of the content of an entity expressed as
         a quantity."""@en ;
    rdfs:domain [
        a owl:Class ;
        owl:unionOf (:Instantiation
            :RecordResource
        )
    ] ;
    rdfs:isDefinedBy <https://www.ica.org/standards/RiC/ontology> ;
    rdfs:label "importance physique ou logique"@fr, "physical or logical extent"@en, "soporte físico o lógico"@es ;
    rdfs:range rdfs:Literal ;
    skos:changeNote [
        dc:date "2023-11-02" ;
        rdf:value "Added a new rdfs:label in Spanish."@en
    ], [
        dc:date "2023-08-25" ;
        rdf:value "Added a new rdfs:label in French."@en
    ] ;
    skos:scopeNote """Provided for usability reasons. Use only if you cannot use the
         subproperties (particularly if the same free text is being used in your current metadata
         for describing the record resource, carrier and instantiation extent)."""@en .

:placeRelation_role
    a owl:ObjectProperty ;
    rdfs:comment """Connects a PlaceRelation to itself. It is a property that can
         stand for an instance of the class when necessary, e.g. when you explore a knowledge
         graph."""@en ;
    rdfs:domain :PlaceRelation ;
    rdfs:isDefinedBy <https://www.ica.org/standards/RiC/ontology> ;
    rdfs:label "a le rôle de la Relation impliquant un lieu"@fr, "desempeña el papel de la Relación con lugar"@es, "has the role of the Place Relation"@en ;
    rdfs:range :PlaceRelation ;
    rdfs:subPropertyOf :relation_role ;
    skos:changeNote [
        dc:date "2024-08-02" ;
        rdf:value """Removed global reflexivity (leads to
               inconsistency)."""@en
    ], [
        dc:date "2023-11-08" ;
        rdf:value """In order to get a system of rolified Relation classes: created
               the object property, with domain and range the PlaceRelation rolified class. Declared
               it as reflexive. Declared it(s) superproperty(ies)."""@en
    ] ;
    skos:scopeNote """This property \"rolifies\" the PlaceRelation class. It should be
         used only when you have to manage instances of the PlaceRelation class, to connect each
         instance to itself, in order to be able to infer, using OWL-RL and property paths, the two
         shortcuts corresponding to this n-ary class."""@en .

:positionHoldingRelation_role
    a owl:ObjectProperty ;
    rdfs:comment """Connects a PositionHoldingRelation to itself. It is a property
         that can stand for an instance of the class when necessary, e.g. when you explore a
         knowledge graph."""@en ;
    rdfs:domain :PositionHoldingRelation ;
    rdfs:isDefinedBy <https://www.ica.org/standards/RiC/ontology> ;
    rdfs:label "a le rôle de la Relation entre une personne et un poste"@fr, """desempeña el papel de la Relación de ocupación entre una persona y
         un puesto"""@es, "has the role of the Position Holding Relation"@en ;
    rdfs:range :PositionHoldingRelation ;
    rdfs:subPropertyOf :agentToAgentRelation_role ;
    skos:changeNote [
        dc:date "2024-08-02" ;
        rdf:value """Removed global reflexivity (leads to
               inconsistency)."""@en
    ], [
        dc:date "2023-11-08" ;
        rdf:value """In order to get a system of rolified Relation classes: created
               the object property, with domain and range the PositionHoldingRelation rolified
               class. Declared it as reflexive. Declared it(s) superproperty(ies)."""@en
    ] ;
    skos:scopeNote """This property \"rolifies\" the PositionHoldingRelation class. It
         should be used only when you have to manage instances of the PositionHoldingRelation class,
         to connect each instance to itself, in order to be able to infer, using OWL-RL and property
         paths, the two shortcuts corresponding to this n-ary class."""@en .

:positionIsContextOfLeadershipRelation
    a owl:ObjectProperty ;
    rdfs:comment """Connects a Position to a Leadership Relation (the leading Person
         occupies that Position)."""@en ;
    rdfs:domain :Position ;
    rdfs:isDefinedBy <https://www.ica.org/standards/RiC/ontology> ;
    rdfs:label "position is context of leadership relation"@en, "poste est le contexte de la relation de direction"@fr, "puesto es contexto de relación de liderazgo"@es ;
    rdfs:range :LeadershipRelation ;
    rdfs:subPropertyOf :thingIsContextOfRelation ;
    owl:inverseOf :leadershipWithPosition ;
    skos:changeNote [
        dc:date "2023-11-12" ;
        rdf:value "Updated the labels."@en
    ], [
        dc:date "2023-11-02" ;
        rdf:value "Added a new rdfs:label in Spanish."@en
    ] .

:positionIsContextOfMembershipRelation
    a owl:ObjectProperty ;
    rdfs:comment """Connects a Position to a Membership Relation (the member Person
         occupies that Position)."""@en ;
    rdfs:domain :Position ;
    rdfs:isDefinedBy <https://www.ica.org/standards/RiC/ontology> ;
    rdfs:label "position is context of membership relation"@en, "poste est le contexte de la relation d'appartenance"@fr, "puesto es contexto de relación de membresía"@es ;
    rdfs:range :MembershipRelation ;
    rdfs:subPropertyOf :thingIsContextOfRelation ;
    owl:inverseOf :membershipWithPosition ;
    skos:changeNote [
        dc:date "2023-11-12" ;
        rdf:value "Updated the labels."@en
    ], [
        dc:date "2023-11-02" ;
        rdf:value "Added a new rdfs:label in Spanish."@en
    ] .

:positionToGroupRelation_role
    a owl:ObjectProperty ;
    rdfs:comment """Connects a PositionToGroupRelation to itself. It is a property
         that can stand for an instance of the class when necessary, e.g. when you explore a
         knowledge graph."""@en ;
    rdfs:domain :PositionToGroupRelation ;
    rdfs:isDefinedBy <https://www.ica.org/standards/RiC/ontology> ;
    rdfs:label "a le rôle de la Relation entre un poste et un groupe"@fr, """desempeña el papel de la Relación de ocupación entre un grupo y un
         puesto"""@es, "has the role of the Position to Group Relation"@en ;
    rdfs:range :PositionToGroupRelation ;
    rdfs:subPropertyOf :agentToAgentRelation_role ;
    skos:changeNote [
        dc:date "2024-08-02" ;
        rdf:value """Removed global reflexivity (leads to
               inconsistency)."""@en
    ], [
        dc:date "2023-11-08" ;
        rdf:value """In order to get a system of rolified Relation classes: created
               the object property, with domain and range the PositionToGroupRelation rolified
               class. Declared it as reflexive. Declared it(s) superproperty(ies)."""@en
    ] ;
    skos:scopeNote """This property \"rolifies\" the PositionToGroupRelation class. It
         should be used only when you have to manage instances of the PositionToGroupRelation class,
         to connect each instance to itself, in order to be able to infer, using OWL-RL and property
         paths, the two shortcuts corresponding to this n-ary class."""@en .

:precededInSequence
    a owl:ObjectProperty ;
    rdfs:comment """Connects a Thing to a Thing that followed it in some sequence (not
         necessarily defined or characterised chronologically) in the past."""@en ;
    rdfs:domain :Thing ;
    rdfs:isDefinedBy <https://www.ica.org/standards/RiC/ontology> ;
    rdfs:label "a précédé dans la séquence"@fr, "preceded in sequence"@en, "precedía secuencialmente a"@es ;
    rdfs:range :Thing ;
    rdfs:subPropertyOf :precedesOrPreceded ;
    owl:inverseOf :followedInSequence ;
    skos:changeNote [
        dc:date "2025-03-04" ;
        rdf:value """Tweaked the rdfs:comment to try to clarify what is
               meant."""@en
    ], [
        dc:date "2023-11-27" ;
        rdf:value "Added a new rdfs:label in Spanish."@en
    ], [
        dc:date "2023-11-12" ;
        rdf:value "Updated the labels."@en
    ], [
        dc:date "2023-09-22" ;
        rdf:value """Renamed the property and modified its definition (rdfs:comment)
               in order to better distinguish it from precedesInTime."""@en
    ], [
        dc:date "2023-09-08" ;
        rdf:value """Object property added, along with its inverse property, in
               order to enable to express past sequential relations between things (the current
               sequential relations being also added, including a transitive one)."""@en
    ] .

:precedesInSequenceTransitive
    a owl:ObjectProperty, owl:TransitiveProperty ;
    rdfs:comment """Connects a Thing to a Thing that follows it directly or indirectly
         in some sequence (not necessarily defined or characterised chronologically). This is a
         transitive relation."""@en ;
    rdfs:domain :Thing ;
    rdfs:isDefinedBy <https://www.ica.org/standards/RiC/ontology> ;
    rdfs:label "precede secuencialmente a transitivo"@es, "precedes in sequence transitive"@en, "précède dans la séquence transitif"@fr ;
    rdfs:range :Thing ;
    rdfs:subPropertyOf :precedesOrPreceded ;
    owl:inverseOf :followsInSequenceTransitive ;
    owl:propertyChainAxiom (:precedesProxyInSequence
        :proxyFor
    ) ;
    skos:changeNote [
        dc:date "2025-03-04" ;
        rdf:value """Tweaked the rdfs:comment to try to clarify what is meant. Also
               added a property chain axiom relating it to use of rico:Proxy."""@en
    ], [
        dc:date "2023-11-27" ;
        rdf:value "Added a new rdfs:label in Spanish."@en
    ], [
        dc:date "2023-11-12" ;
        rdf:value "Updated the labels."@en
    ], [
        dc:date "2023-09-22" ;
        rdf:value """Renamed the property and modified its definition (rdfs:comment)
               in order to better distinguish it from precedesInTime."""@en
    ], [
        dc:date "2023-09-08" ;
        rdf:value """Object property added, along with its inverse property, in
               order to enable to express current, direct or indirect, sequential relations between
               things (the past sequential relation also being added)."""@en
    ] .

:precedesInTime
    a owl:ObjectProperty, owl:TransitiveProperty ;
    rdfs:comment """Connects a Thing to a Thing that follows it in chronological
         order. This is a transitive relation."""@en ;
    rdfs:domain :Thing ;
    rdfs:isDefinedBy <https://www.ica.org/standards/RiC/ontology> ;
    rdfs:label "precede en el tiempo a"@es, "precedes in time"@en, "précède dans le temps"@fr ;
    rdfs:range :Thing ;
    rdfs:subPropertyOf :precedesOrPreceded ;
    owl:inverseOf :followsInTime ;
    owl:propertyChainAxiom (:thingIsSourceOfRelation
        :temporalRelation_role
        :relationHasTarget
    ) ;
    skos:changeNote [
        dc:date "2023-11-08" ;
        rdf:value """In order to get a system of rolified Relation classes: modified
               the property chain axiom so that it now involves the new temporalRelation_role object
               property."""@en
    ], [
        dc:date "2023-11-02" ;
        rdf:value "Added a new rdfs:label in Spanish."@en
    ], [
        dc:date "2023-09-21" ;
        rdf:value "Property made transitive."@en
    ], [
        dc:date "2023-08-28" ;
        rdf:value "Added a new rdfs:label in French."@en
    ], [
        dc:date "2021-01-22" ;
        rdf:value "changed the superproperty IRI"@en
    ] ;
    skos:scopeNote """There may actually be zero to many intermediate Entities,
         ignored or unknown, in the chronological sequence between the two connected
         Entities."""@en ;
    :RiCCMCorrespondingComponent """RiC-R009 ('precedes in time'
         relation)"""@en .

:precedesOrPreceded
    a owl:ObjectProperty ;
    rdfs:comment """Connects a Thing to a Thing that follows or followed it in some
         sequence."""@en ;
    rdfs:domain :Thing ;
    rdfs:isDefinedBy <https://www.ica.org/standards/RiC/ontology> ;
    rdfs:label "precede o precedía secuencialmente a"@es, "precedes or preceded"@en, "précède ou a précédé"@fr ;
    rdfs:range :Thing ;
    rdfs:subPropertyOf :isRelatedTo ;
    owl:inverseOf :followsOrFollowed ;
    owl:propertyChainAxiom (:thingIsSourceOfRelation
        :sequentialRelation_role
        :relationHasTarget
    ) ;
    skos:changeNote [
        dc:date "2023-11-08" ;
        rdf:value """In order to get a system of rolified Relation classes: modified
               the property chain axiom so that it now involves the new sequentialRelation_role
               object property."""@en
    ], [
        dc:date "2023-11-02" ;
        rdf:value "Added a new rdfs:label in Spanish."@en
    ], [
        dc:date "2023-08-28" ;
        rdf:value "Added a new rdfs:label in French."@en
    ], [
        dc:date "2021-01-22" ;
        rdf:value """changed the IRI, label, inverse property IRI, text definition,
               corresponding CM component name (changed made in order to make RiC-O compliant with
               RiC-CM 0.2; the name of this property in RiC-O 0.1 was \"precedes\")."""@en
    ] ;
    skos:scopeNote """The relation does not specify by itself what criteria are used
         for ordering the sequence. There may actually be zero to many intermediate Entities,
         ignored or unkown, in the sequence between the two connected Things. Can be used, for
         example, for specifying that some Record 'precedes' (has next) some Record within a Record
         Set."""@en ;
    :RiCCMCorrespondingComponent """RiC-R008 ('precedes or preceded'
         relation)"""@en .

:precedesProxyInSequence
    a owl:ObjectProperty ;
    rdfs:comment """Connects a Record Resource to a Proxy of a Record Resource that it
         precedes directly or indirectly in some sequence (not necessarily defined or characterised
         chronologically)."""@en ;
    rdfs:domain :RecordResource ;
    rdfs:isDefinedBy <https://www.ica.org/standards/RiC/ontology> ;
    rdfs:label "precede el proxy en la secuencia"@es, "precedes proxy in sequence"@en, "précède le proxy dans la séquence"@fr ;
    rdfs:range :Proxy ;
    rdfs:subPropertyOf :precedesInSequenceTransitive ;
    owl:inverseOf :proxyFollowsInSequence ;
    owl:propertyChainAxiom (:precedesProxyInSequence
        :proxyPrecedesProxyInSequenceTransitive
    ) ;
    skos:changeNote [
        dc:date "2025-04-02" ;
        rdf:value "Added the French and Spanish labels."@en
    ], [
        dc:date "2025-03-04" ;
        rdf:value "Introduced in RiC-O 1.1."@en
    ] .

:productionTechnique
    a owl:DatatypeProperty ;
    rdfs:comment """The method used in the representation of information on an
         Instantiation."""@en ;
    rdfs:domain :Instantiation ;
    rdfs:isDefinedBy <https://www.ica.org/standards/RiC/ontology> ;
    rdfs:label "production technique"@en, "technique de production"@fr, "técnica de produccióon"@es ;
    rdfs:range rdfs:Literal ;
    skos:changeNote [
        dc:date "2023-11-11" ;
        rdf:value """Aligned with RiC-CM 1.0: updated the description
               (rdfs:comment)."""@en
    ], [
        dc:date "2023-11-02" ;
        rdf:value "Added a new rdfs:label in Spanish."@en
    ], [
        dc:date "2023-08-25" ;
        rdf:value "Added a new rdfs:label in French."@en
    ], [
        dc:date "2020-11-01" ;
        rdf:value """Examples added. Objective: to make RiC-O compliant with RiC-CM
               v0.2."""@en
    ] ;
    skos:example "engraving"@en, "handwriting"@en, "magnetic recording"@en, "optical recording"@en ;
    skos:scopeNote """Use only if you have free text or don't have a controlled
         vocabulary for production techniques (in this case, use the ProductionTechniqueType
         class)"""@en ;
    :RiCCMCorrespondingComponent """Corresponds to RiC-A33 (Production Technique
         attribute)"""@en .

:proxyDirectlyFollowsInSequence
    a owl:ObjectProperty ;
    rdfs:comment """Inverse of 'directly precedes proxy in sequence' object
         property."""@en ;
    rdfs:domain :Proxy ;
    rdfs:isDefinedBy <https://www.ica.org/standards/RiC/ontology> ;
    rdfs:label "proxy directly follows in sequence"@en, "proxy sigue directamente en la secuencia"@es, "proxy suit directement dans la séquence"@fr ;
    rdfs:range :RecordResource ;
    rdfs:subPropertyOf :directlyFollowsInSequence, :proxyFollowsInSequence ;
    owl:inverseOf :directlyPrecedesProxyInSequence ;
    skos:changeNote [
        dc:date "2025-04-02" ;
        rdf:value "Added the French and Spanish labels."@en
    ], [
        dc:date "2025-03-04" ;
        rdf:value "Introduced in RiC-O 1.1."@en
    ] .

:proxyDirectlyFollowsProxyInSequence
    a owl:ObjectProperty ;
    rdfs:comment """Inverse of 'proxy directly precedes proxy in sequence' object
         property."""@en ;
    rdfs:domain :Proxy ;
    rdfs:isDefinedBy <https://www.ica.org/standards/RiC/ontology> ;
    rdfs:label "proxy directly follows proxy in sequence"@en, "proxy sigue directamente el proxy en la secuencia"@es, "proxy suit directement le proxy dans la séquence"@fr ;
    rdfs:range :Proxy ;
    rdfs:subPropertyOf :directlyFollowsInSequence, :proxyFollowsProxyInSequenceTransitive ;
    owl:inverseOf :proxyDirectlyPrecedesProxyInSequence ;
    skos:changeNote [
        dc:date "2025-04-02" ;
        rdf:value "Added the French and Spanish labels."@en
    ], [
        dc:date "2025-03-04" ;
        rdf:value "Introduced in RiC-O 1.1."@en
    ] .

:proxyDirectlyIncludes
    a owl:ObjectProperty ;
    rdfs:comment """Inverse of 'is directly included in proxy' object
         property."""@en ;
    rdfs:domain :Proxy ;
    rdfs:isDefinedBy <https://www.ica.org/standards/RiC/ontology> ;
    rdfs:label "proxy directly includes"@en, "proxy inclut directement"@fr, "proxy incluye directamente"@es ;
    rdfs:range [
        a owl:Class ;
        owl:unionOf (:Record
            :RecordSet
        )
    ] ;
    rdfs:subPropertyOf :hasDirectPart, :proxyIncludes ;
    owl:inverseOf :isDirectlyIncludedInProxy ;
    skos:changeNote [
        dc:date "2025-04-02" ;
        rdf:value "Added the French and Spanish labels."@en
    ], [
        dc:date "2025-03-04" ;
        rdf:value "Introduced in RiC-O 1.1."@en
    ] .

:proxyDirectlyIncludesProxy
    a owl:ObjectProperty ;
    rdfs:comment """Inverse of 'proxy is directly included in' object
         property."""@en ;
    rdfs:domain :Proxy ;
    rdfs:isDefinedBy <https://www.ica.org/standards/RiC/ontology> ;
    rdfs:label "proxy directly includes proxy"@en, "proxy inclut directement le proxy"@fr, "proxy incluye directamente el proxy"@es ;
    rdfs:range :Proxy ;
    rdfs:subPropertyOf :hasDirectPart, :proxyIncludesProxyTransitive ;
    owl:inverseOf :proxyIsDirectlyIncludedInProxy ;
    skos:changeNote [
        dc:date "2025-04-02" ;
        rdf:value "Added the French and Spanish labels."@en
    ], [
        dc:date "2025-03-04" ;
        rdf:value "Introduced in RiC-O 1.1."@en
    ] .

:proxyDirectlyPrecedesInSequence
    a owl:ObjectProperty ;
    rdfs:comment """Connects a Proxy of a Record Resource to a Record Resource which
         it precedes directly in some sequence (not necessarily defined or characterised
         chronologically)."""@en ;
    rdfs:domain :Proxy ;
    rdfs:isDefinedBy <https://www.ica.org/standards/RiC/ontology> ;
    rdfs:label "proxy directly precedes in sequence"@en, "proxy precede directamente en la secuencia"@es, "proxy précède directement dans la séquence"@fr ;
    rdfs:range :RecordResource ;
    rdfs:subPropertyOf :directlyPrecedesInSequence, :proxyPrecedesInSequence ;
    owl:inverseOf :directlyFollowsProxyInSequence ;
    skos:changeNote [
        dc:date "2025-04-02" ;
        rdf:value "Added the French and Spanish labels."@en
    ], [
        dc:date "2025-03-04" ;
        rdf:value "Introduced in RiC-O 1.1."@en
    ] .

:proxyDirectlyPrecedesProxyInSequence
    a owl:ObjectProperty ;
    rdfs:comment """Connects a Proxy of a Record Resource to a Proxy of another Record
         Resource that it precedes directly in some sequence (not necessarily defined or
         characterised chronologically)."""@en ;
    rdfs:domain :Proxy ;
    rdfs:isDefinedBy <https://www.ica.org/standards/RiC/ontology> ;
    rdfs:label "proxy directly precedes proxy in sequence"@en, "proxy precede directamente el proxy en la secuencia"@es, "proxy précède directement le proxy dans la séquence"@fr ;
    rdfs:range :Proxy ;
    rdfs:subPropertyOf :directlyPrecedesInSequence, :proxyPrecedesProxyInSequenceTransitive ;
    owl:inverseOf :proxyDirectlyFollowsProxyInSequence ;
    skos:changeNote [
        dc:date "2025-04-02" ;
        rdf:value "Added the French and Spanish labels."@en
    ], [
        dc:date "2025-04-01" ;
        rdf:value """Added a second owl:subPropertyOf with target
               'proxyPrecedesProxyInSequenceTransitive'."""@en
    ], [
        dc:date "2025-03-04" ;
        rdf:value "Introduced in RiC-O 1.1."@en
    ] .

:proxyFollowsInSequence
    a owl:ObjectProperty ;
    rdfs:comment """Inverse of 'precedes proxy in sequence' object
         property."""@en ;
    rdfs:domain :Proxy ;
    rdfs:isDefinedBy <https://www.ica.org/standards/RiC/ontology> ;
    rdfs:label "proxy follows in sequence"@en, "proxy sigue en la secuencia"@es, "proxy suit dans la séquence"@fr ;
    rdfs:range :RecordResource ;
    rdfs:subPropertyOf :followsInSequenceTransitive ;
    owl:inverseOf :precedesProxyInSequence ;
    owl:propertyChainAxiom (:proxyFollowsProxyInSequenceTransitive
        :proxyFollowsInSequence
    ) ;
    skos:changeNote [
        dc:date "2025-04-02" ;
        rdf:value "Added the French and Spanish labels."@en
    ], [
        dc:date "2025-03-04" ;
        rdf:value "Introduced in RiC-O 1.1."@en
    ] .

:proxyFollowsProxyInSequenceTransitive
    a owl:ObjectProperty, owl:TransitiveProperty ;
    rdfs:comment """Inverse of 'proxy recedes proxy in sequence transitive' object
         property."""@en ;
    rdfs:domain :Proxy ;
    rdfs:isDefinedBy <https://www.ica.org/standards/RiC/ontology> ;
    rdfs:label "proxy follows proxy in sequence transitive"@en, "proxy sigue el proxy en la secuencia transitivo"@es, "proxy suit le proxy dans la séquence transitif"@fr ;
    rdfs:range :Proxy ;
    rdfs:subPropertyOf :followsInSequenceTransitive ;
    owl:inverseOf :proxyPrecedesProxyInSequenceTransitive ;
    skos:changeNote [
        dc:date "2025-04-02" ;
        rdf:value "Added the French and Spanish labels."@en
    ], [
        dc:date "2025-03-04" ;
        rdf:value "Introduced in RiC-O 1.1."@en
    ] .

:proxyFor
    a owl:ObjectProperty ;
    rdfs:comment """Connects a Proxy to the Record Resource it stands for in the
         context of a specific Record Resource."""@en ;
    rdfs:domain :Proxy ;
    rdfs:isDefinedBy <https://www.ica.org/standards/RiC/ontology> ;
    rdfs:label "es proxy para"@es, "proxy for"@en, "proxy pour"@fr ;
    rdfs:range :RecordResource ;
    rdfs:subPropertyOf :isRelatedTo ;
    owl:inverseOf :hasProxy ;
    skos:changeNote [
        dc:date "2025-03-04" ;
        rdf:value """Changed the rdfs:comment to allow for a context of a Record
               Resource of any kind, not only a Record Set."""@en
    ], [
        dc:date "2023-11-02" ;
        rdf:value "Added a new rdfs:label in Spanish."@en
    ], [
        dc:date "2023-08-28" ;
        rdf:value "Added a new rdfs:label in French."@en
    ] .

:proxyHasConstituent
    a owl:ObjectProperty ;
    rdfs:comment """Inverse of 'is constituent of proxy' object
         property."""@en ;
    rdfs:domain :Proxy ;
    rdfs:isDefinedBy <https://www.ica.org/standards/RiC/ontology> ;
    rdfs:label "proxy a pour constituant"@fr, "proxy has constituent"@en, "proxy tiene como elemento constitutivo"@es ;
    rdfs:range [
        a owl:Class ;
        owl:unionOf (:Record
            :RecordPart
        )
    ] ;
    rdfs:subPropertyOf :hasPartTransitive ;
    owl:inverseOf :isConstituentOfProxy ;
    owl:propertyChainAxiom (:proxyHasConstituentProxyTransitive
        :proxyHasConstituent
    ) ;
    skos:changeNote [
        dc:date "2025-04-02" ;
        rdf:value "Added the French and Spanish labels."@en
    ], [
        dc:date "2025-03-04" ;
        rdf:value "Introduced in RiC-O 1.1."@en
    ] .

:proxyHasConstituentProxyTransitive
    a owl:ObjectProperty, owl:TransitiveProperty ;
    rdfs:comment """Inverse of 'proxy is constituent of proxy transitive' object
         property. This is a transitive relation."""@en ;
    rdfs:domain :Proxy ;
    rdfs:isDefinedBy <https://www.ica.org/standards/RiC/ontology> ;
    rdfs:label "proxy a pour constituant le proxy (transitif)"@fr, "proxy has constituent proxy transitive"@en, """proxy tiene como elemento constitutivo el proxy
         (transitivo)"""@es ;
    rdfs:range :Proxy ;
    rdfs:subPropertyOf :hasPartTransitive ;
    owl:inverseOf :proxyIsConstituentOfProxyTransitive ;
    skos:changeNote [
        dc:date "2025-04-02" ;
        rdf:value "Added the French and Spanish labels."@en
    ], [
        dc:date "2025-03-04" ;
        rdf:value "Introduced in RiC-O 1.1."@en
    ] .

:proxyHasDirectConstituent
    a owl:ObjectProperty ;
    rdfs:comment """Inverse of 'is direct constituent of proxy' object
         property."""@en ;
    rdfs:domain :Proxy ;
    rdfs:isDefinedBy <https://www.ica.org/standards/RiC/ontology> ;
    rdfs:label "proxy a pour constituant direct"@fr, "proxy has direct constituent"@en, "proxy tiene como directo elemento constitutivo"@es ;
    rdfs:range [
        a owl:Class ;
        owl:unionOf (:Record
            :RecordPart
        )
    ] ;
    rdfs:subPropertyOf :hasDirectPart, :proxyHasConstituent ;
    owl:inverseOf :isDirectConstituentOfProxy ;
    skos:changeNote [
        dc:date "2025-04-02" ;
        rdf:value "Added the French and Spanish labels."@en
    ], [
        dc:date "2025-03-04" ;
        rdf:value "Introduced in RiC-O 1.1."@en
    ] .

:proxyHasDirectConstituentProxy
    a owl:ObjectProperty ;
    rdfs:comment """Inverse of 'proxy is direct constituent of' object
         property."""@en ;
    rdfs:domain :Proxy ;
    rdfs:isDefinedBy <https://www.ica.org/standards/RiC/ontology> ;
    rdfs:label "proxy a pour constituant direct le proxy"@fr, "proxy has direct constituent proxy"@en, "proxy tiene como directo elemento constitutivo el proxy"@es ;
    rdfs:range :Proxy ;
    rdfs:subPropertyOf :hasDirectPart, :proxyHasConstituentProxyTransitive ;
    owl:inverseOf :proxyIsDirectConstituentOfProxy ;
    skos:changeNote [
        dc:date "2025-04-02" ;
        rdf:value "Added the French and Spanish labels."@en
    ], [
        dc:date "2025-03-04" ;
        rdf:value "Introduced in RiC-O 1.1."@en
    ] .

:proxyIn
    a owl:ObjectProperty ;
    rdfs:comment """Connects a Proxy to the Record Resource in which it stands for
         (represents) another Record Resource."""@en ;
    rdfs:domain :Proxy ;
    rdfs:isDefinedBy <https://www.ica.org/standards/RiC/ontology> ;
    rdfs:label "es proxy en"@es, "proxy dans"@fr, "proxy in"@en ;
    rdfs:range :RecordResource ;
    rdfs:subPropertyOf :isRelatedTo ;
    skos:changeNote [
        dc:date "2025-03-04" ;
        rdf:value """Changed the range and rdfs:comment to allow any Record
               Resource, not only a Record Set."""@en
    ], [
        dc:date "2023-11-02" ;
        rdf:value "Added a new rdfs:label in Spanish."@en
    ], [
        dc:date "2023-08-28" ;
        rdf:value "Added a new rdfs:label in French."@en
    ] .

:proxyInRecord
    a owl:ObjectProperty ;
    rdfs:comment """Connects a Proxy to a Record in which it stands for (represents) a
         Record Part or another Record."""@en ;
    rdfs:domain :Proxy ;
    rdfs:isDefinedBy <https://www.ica.org/standards/RiC/ontology> ;
    rdfs:label "proxy dans l’objet informationnel"@fr, "proxy en el documento"@es, "proxy in record"@en ;
    rdfs:range :Record ;
    rdfs:subPropertyOf :proxyIn ;
    skos:changeNote [
        dc:date "2025-04-02" ;
        rdf:value "Added the French and Spanish labels."@en
    ], [
        dc:date "2025-03-04" ;
        rdf:value "Introduced in RiC-O 1.1."@en
    ] .

:proxyInRecordSet
    a owl:ObjectProperty ;
    rdfs:comment """Connects a Proxy to a Record Set in which it stands for
         (represents) a Record or another Record Set."""@en ;
    rdfs:domain :Proxy ;
    rdfs:isDefinedBy <https://www.ica.org/standards/RiC/ontology> ;
    rdfs:label "proxy dans l’ensemble d’objets informationnels"@fr, "proxy en la agrupación documental"@es, "proxy in record set"@en ;
    rdfs:range :RecordSet ;
    rdfs:subPropertyOf :proxyIn ;
    skos:changeNote [
        dc:date "2025-04-02" ;
        rdf:value "Added the French and Spanish labels."@en
    ], [
        dc:date "2025-03-04" ;
        rdf:value "Introduced in RiC-O 1.1."@en
    ] .

:proxyIncludes
    a owl:ObjectProperty ;
    rdfs:comment "Inverse of 'is included in proxy' object property."@en ;
    rdfs:domain :Proxy ;
    rdfs:isDefinedBy <https://www.ica.org/standards/RiC/ontology> ;
    rdfs:label "proxy includes"@en, "proxy inclut"@fr, "proxy incluye"@es ;
    rdfs:range [
        a owl:Class ;
        owl:unionOf (:Record
            :RecordSet
        )
    ] ;
    rdfs:subPropertyOf :hasPartTransitive ;
    owl:inverseOf :isIncludedInProxy ;
    owl:propertyChainAxiom (:proxyIncludesProxyTransitive
        :proxyIncludes
    ) ;
    skos:changeNote [
        dc:date "2025-04-02" ;
        rdf:value "Added the French and Spanish labels."@en
    ], [
        dc:date "2025-03-04" ;
        rdf:value "Introduced in RiC-O 1.1."@en
    ] .

:proxyIncludesProxyTransitive
    a owl:ObjectProperty, owl:TransitiveProperty ;
    rdfs:comment """Inverse of 'proxy is included in proxy transitive' object
         property. This is a transitive relation."""@en ;
    rdfs:domain :Proxy ;
    rdfs:isDefinedBy <https://www.ica.org/standards/RiC/ontology> ;
    rdfs:label "proxy includes proxy transitive"@en, "proxy inclut le proxy (transitif)"@fr, "proxy incluye el proxy (transitivo)"@es ;
    rdfs:range :Proxy ;
    rdfs:subPropertyOf :hasPartTransitive ;
    owl:inverseOf :proxyIsIncludedInProxyTransitive ;
    skos:changeNote [
        dc:date "2025-04-02" ;
        rdf:value "Added the French and Spanish labels."@en
    ], [
        dc:date "2025-03-04" ;
        rdf:value "Introduced in RiC-O 1.1."@en
    ] .

:proxyIsConstituentOf
    a owl:ObjectProperty ;
    rdfs:comment """Connects a Proxy of a Record or Record Part to a Record or Record
         Part which it is a constituent of, directly or indirectly."""@en ;
    rdfs:domain :Proxy ;
    rdfs:isDefinedBy <https://www.ica.org/standards/RiC/ontology> ;
    rdfs:label "proxy es un elemento constitutivo de"@es, "proxy est un constituant de"@fr, "proxy is constituent of"@en ;
    rdfs:range [
        a owl:Class ;
        owl:unionOf (:Record
            :RecordPart
        )
    ] ;
    rdfs:subPropertyOf :isPartOfTransitive ;
    owl:inverseOf :hasConstituentProxy ;
    owl:propertyChainAxiom (:proxyIsConstituentOfProxyTransitive
        :proxyIsConstituentOf
    ) ;
    skos:changeNote [
        dc:date "2025-04-02" ;
        rdf:value "Added the French and Spanish labels."@en
    ], [
        dc:date "2025-03-04" ;
        rdf:value "Introduced in RiC-O 1.1."@en
    ] .

:proxyIsConstituentOfProxyTransitive
    a owl:ObjectProperty, owl:TransitiveProperty ;
    rdfs:comment """Connects a Proxy of a Record or Record Part to a Proxy of another
         Record or Record Part which it is a constituent of, directly or indirectly. This is a
         transitive relation."""@en ;
    rdfs:domain :Proxy ;
    rdfs:isDefinedBy <https://www.ica.org/standards/RiC/ontology> ;
    rdfs:label "proxy es elemento constitutivo del proxy (transitivo)"@es, "proxy est un constituant du proxy (transitif)"@fr, "proxy is constituent of proxy transitive"@en ;
    rdfs:range :Proxy ;
    rdfs:subPropertyOf :isPartOfTransitive ;
    owl:inverseOf :proxyHasConstituentProxyTransitive ;
    skos:changeNote [
        dc:date "2025-04-02" ;
        rdf:value "Added the French and Spanish labels."@en
    ], [
        dc:date "2025-03-04" ;
        rdf:value "Introduced in RiC-O 1.1."@en
    ] .

:proxyIsDirectConstituentOf
    a owl:ObjectProperty ;
    rdfs:comment """Connects a Proxy of a Record or Record Part to another Record or
         Record Part which the first is a direct constituent of."""@en ;
    rdfs:domain :Proxy ;
    rdfs:isDefinedBy <https://www.ica.org/standards/RiC/ontology> ;
    rdfs:label "proxy es elemento constitutivo directo de"@es, "proxy est un constituant direct de"@fr, "proxy is direct constituent of"@en ;
    rdfs:range [
        a owl:Class ;
        owl:unionOf (:Record
            :RecordPart
        )
    ] ;
    rdfs:subPropertyOf :isDirectPartOf, :proxyIsConstituentOf ;
    owl:inverseOf :hasDirectConstituentProxy ;
    skos:changeNote [
        dc:date "2025-04-02" ;
        rdf:value """Fixed the owl:inverseOf property (was hasConstituentProxy).
               Added the French and Spanish labels."""@en
    ], [
        dc:date "2025-03-04" ;
        rdf:value "Introduced in RiC-O 1.1."@en
    ] .

:proxyIsDirectConstituentOfProxy
    a owl:ObjectProperty ;
    rdfs:comment """Connects a Proxy of a Record or Record Part to a Proxy of another
         Record or Record Part of which the first is a direct constituent."""@en ;
    rdfs:domain :Proxy ;
    rdfs:isDefinedBy <https://www.ica.org/standards/RiC/ontology> ;
    rdfs:label "proxy es elemento constitutivo directo del proxy"@es, "proxy est un constituant direct du proxy"@fr, "proxy is direct constituent of proxy"@en ;
    rdfs:range :Proxy ;
    rdfs:subPropertyOf :isDirectPartOf, :proxyIsConstituentOfProxyTransitive ;
    owl:inverseOf :proxyHasDirectConstituentProxy ;
    skos:changeNote [
        dc:date "2025-04-02" ;
        rdf:value "Added the French and Spanish labels."@en
    ], [
        dc:date "2025-03-04" ;
        rdf:value "Introduced in RiC-O 1.1."@en
    ] .

:proxyIsDirectlyIncludedIn
    a owl:ObjectProperty ;
    rdfs:comment """Connects a Proxy of a Record or Record Set to another Record Set
         which the first is directly included in."""@en ;
    rdfs:domain :Proxy ;
    rdfs:isDefinedBy <https://www.ica.org/standards/RiC/ontology> ;
    rdfs:label "proxy est directement inclus dans"@fr, "proxy está directamente incluido en"@es, "proxy is directly included in"@en ;
    rdfs:range :RecordSet ;
    rdfs:subPropertyOf :isDirectPartOf, :proxyIsIncludedIn ;
    owl:inverseOf :directlyIncludesProxy ;
    skos:changeNote [
        dc:date "2025-04-02" ;
        rdf:value "Added the French and Spanish labels."@en
    ], [
        dc:date "2025-03-04" ;
        rdf:value "Introduced in RiC-O 1.1."@en
    ] .

:proxyIsDirectlyIncludedInProxy
    a owl:ObjectProperty ;
    rdfs:comment """Connects a Proxy of a Record or Record Set to a Proxy of a Record
         Set which it is directly included in."""@en ;
    rdfs:domain :Proxy ;
    rdfs:isDefinedBy <https://www.ica.org/standards/RiC/ontology> ;
    rdfs:label "proxy est directement inclus dans le proxy"@fr, "proxy está directamente incluido en el proxy"@es, "proxy is directly included in proxy"@en ;
    rdfs:range :Proxy ;
    rdfs:subPropertyOf :isDirectPartOf, :proxyIsIncludedInProxyTransitive ;
    owl:inverseOf :proxyDirectlyIncludesProxy ;
    skos:changeNote [
        dc:date "2025-04-02" ;
        rdf:value "Added the French and Spanish labels."@en
    ], [
        dc:date "2025-03-04" ;
        rdf:value "Introduced in RiC-O 1.1."@en
    ] .

:proxyIsIncludedIn
    a owl:ObjectProperty ;
    rdfs:comment """Connects a Proxy of a Record or Record Set to a Record Set which
         it is included in, directly or indirectly."""@en ;
    rdfs:domain :Proxy ;
    rdfs:isDefinedBy <https://www.ica.org/standards/RiC/ontology> ;
    rdfs:label "proxy est inclus dans"@fr, "proxy está incluido en"@es, "proxy is included in"@en ;
    rdfs:range :RecordSet ;
    rdfs:subPropertyOf :isPartOfTransitive ;
    owl:inverseOf :includesProxy ;
    owl:propertyChainAxiom (:proxyIsIncludedInProxyTransitive
        :proxyIsIncludedIn
    ) ;
    skos:changeNote [
        dc:date "2025-04-02" ;
        rdf:value "Added the French and Spanish labels."@en
    ], [
        dc:date "2025-03-04" ;
        rdf:value "Introduced in RiC-O 1.1."@en
    ] .

:proxyIsIncludedInProxyTransitive
    a owl:ObjectProperty, owl:TransitiveProperty ;
    rdfs:comment """Connects a Proxy of a Record or Record Set to a Proxy of a Record
         Set which it is included in, directly or indirectly. This is a transitive
         relation."""@en ;
    rdfs:domain :Proxy ;
    rdfs:isDefinedBy <https://www.ica.org/standards/RiC/ontology> ;
    rdfs:label "proxy est inclus dans le proxy (transitif)"@fr, "proxy está incluido en el proxy (transitivo)"@es, "proxy is included in proxy transitive"@en ;
    rdfs:range :Proxy ;
    rdfs:subPropertyOf :isPartOfTransitive ;
    owl:inverseOf :proxyIncludesProxyTransitive ;
    skos:changeNote [
        dc:date "2025-04-02" ;
        rdf:value "Added the French and Spanish labels."@en
    ], [
        dc:date "2025-03-04" ;
        rdf:value "Introduced in RiC-O 1.1."@en
    ] .

:proxyPrecedesInSequence
    a owl:ObjectProperty ;
    rdfs:comment """Connects a Proxy of a Record Resource to a Record Resource which
         the first precedes directly or indirectly in some sequence (not necessarily defined or
         characterised chronologically)."""@en ;
    rdfs:domain :Proxy ;
    rdfs:isDefinedBy <https://www.ica.org/standards/RiC/ontology> ;
    rdfs:label "proxy precede en la secuencia"@es, "proxy precedes in sequence"@en, "proxy précède dans la séquence"@fr ;
    rdfs:range :RecordResource ;
    rdfs:subPropertyOf :precedesInSequenceTransitive ;
    owl:inverseOf :followsProxyInSequence ;
    owl:propertyChainAxiom (:proxyPrecedesProxyInSequenceTransitive
        :proxyPrecedesInSequence
    ) ;
    skos:changeNote [
        dc:date "2025-04-02" ;
        rdf:value "Added the French and Spanish labels."@en
    ], [
        dc:date "2025-03-04" ;
        rdf:value "Introduced in RiC-O 1.1."@en
    ] .

:proxyPrecedesProxyInSequenceTransitive
    a owl:ObjectProperty, owl:TransitiveProperty ;
    rdfs:comment """Connects a Proxy of a Record Resource to a Proxy of another Record
         Resource which directly or indirectly follows the first in some sequence (not necessarily
         defined or characterised chronologically). This is a transitive relation."""@en ;
    rdfs:domain :Proxy ;
    rdfs:isDefinedBy <https://www.ica.org/standards/RiC/ontology> ;
    rdfs:label "proxy precede el proxy en la secuencia (transitivo)"@es, "proxy precedes proxy in sequence transitive"@en, "proxy précède le proxy dans la séquence (transitif)"@fr ;
    rdfs:range :Proxy ;
    rdfs:subPropertyOf :precedesInSequenceTransitive ;
    owl:inverseOf :proxyFollowsProxyInSequenceTransitive ;
    skos:changeNote [
        dc:date "2025-04-02" ;
        rdf:value "Added the French and Spanish labels."@en
    ], [
        dc:date "2025-03-04" ;
        rdf:value "Introduced in RiC-O 1.1."@en
    ] .

:publicationDate
    a owl:DatatypeProperty ;
    rdfs:comment """Date of the publication, in the past or in the future, of a Record
         Resource."""@en ;
    rdfs:domain :RecordResource ;
    rdfs:isDefinedBy <https://www.ica.org/standards/RiC/ontology> ;
    rdfs:label "date de publication"@fr, "fecha de publicación"@es, "publication date"@en ;
    rdfs:range rdfs:Literal ;
    rdfs:subPropertyOf :date ;
    skos:changeNote [
        dc:date "2025-02-19" ;
        rdf:value """Changed definition (added \"in the past or in the
               future\")."""@en
    ], [
        dc:date "2023-11-02" ;
        rdf:value "Added a new rdfs:label in Spanish."@en
    ], [
        dc:date "2023-08-25" ;
        rdf:value "Added a new rdfs:label in French."@en
    ] ;
    skos:scopeNote """Provided for usability reasons. May be deprecated and removed
         later on. Use only if you don't use Date classes for handling dates."""@en ;
    :RiCCMCorrespondingComponent """Datatype property specialized implementation of
         RiC-E18 (Date entity)"""@en .

:qualityOfRepresentationNote
    a owl:DatatypeProperty ;
    rdfs:comment """Characteristics of an Instantiation that affect the ability to
         recover the intellectual content. Such characteristics may be related to the methods used
         in creating the Instantiation or introduced subsequent to the creation through
         accident."""@en ;
    rdfs:domain :Instantiation ;
    rdfs:isDefinedBy <https://www.ica.org/standards/RiC/ontology> ;
    rdfs:label "nota sobre la calidad de representación"@es, "note sur la qualité de la représentation"@fr, "quality of representation note"@en ;
    rdfs:range rdfs:Literal ;
    rdfs:subPropertyOf :physicalCharacteristicsNote ;
    skos:changeNote [
        dc:date "2023-11-11" ;
        rdf:value """Aligned with RiC-CM 1.0: updated the IRI, mapping to RiC-CM
               (rico:RiCCMCorrespondingComponent), labels, description (rdfs:comment),
               skos:scopeNote, rdfs:subpropertyOf."""@en
    ], [
        dc:date "2023-11-02" ;
        rdf:value "Added a new rdfs:label in Spanish."@en
    ], [
        dc:date "2023-08-25" ;
        rdf:value "Added a new rdfs:label in French."@en
    ], [
        dc:date "2020-11-01" ;
        rdf:value """Text definition updated. Examples added. Objective: to make
               RiC-O compliant with RiC-CM v0.2."""@en
    ] ;
    skos:example """Black and white digitization may have led to loss of some
         information."""@en, """some loss of information due to poor quality of image
         capture"""@en, "some loss of text due to rodent damage"@en ;
    skos:scopeNote """Quality of representation note is a specialization of physical
         characteristics note. Quality of representation note should be used in conjunction with
         physical characteristics note when the physical characteristics impact the ability to
         recover the intellectual content."""@en ;
    :RiCCMCorrespondingComponent """Corresponds to RiC-A34 (Quality of Representation
         Note attribute)"""@en .

:quantity
    a owl:DatatypeProperty ;
    rdfs:comment "Machine-readable quantity."@en ;
    rdfs:domain :Extent ;
    rdfs:isDefinedBy <https://www.ica.org/standards/RiC/ontology> ;
    rdfs:label "cantidad"@es, "quantity"@en, "quantité"@fr ;
    rdfs:range xsd:decimal ;
    rdfs:subPropertyOf :textualValue ;
    skos:changeNote [
        dc:date "2023-11-02" ;
        rdf:value "Added a new rdfs:label in Spanish."@en
    ], [
        dc:date "2023-08-28" ;
        rdf:value "Added an xml:lang attribute to the rdfs:comment."@en
    ], [
        dc:date "2023-08-25" ;
        rdf:value "Added a new rdfs:label in French."@en
    ], [
        dc:date "2020-11-21" ;
        rdf:value "Added a scope note."@en
    ], [
        dc:date "2020-10-28" ;
        rdf:value """Datatype property created along with unitOfMeasurement, Extent
               and UnitOfMeasurement classes, in order to provide methods for handling extent
               accurately."""@en
    ] ;
    skos:scopeNote """Use if you use the Extent class and its properties for handling
         an accurate description of the extent of a resource."""@en .

:rankInHierarchy
    a owl:DatatypeProperty ;
    rdfs:comment """The rank of a Record Resource, or of a Proxy that stands for it,
         in a hierarchy."""@en ;
    rdfs:domain [
        a owl:Class ;
        owl:unionOf (:RecordResource
            :Proxy
        )
    ] ;
    rdfs:isDefinedBy <https://www.ica.org/standards/RiC/ontology> ;
    rdfs:label "rang dans la hiérarchie"@fr, "rango en la jerarquía"@es, "rank in hierarchy"@en ;
    rdfs:range xsd:int ;
    rdfs:subPropertyOf :textualValue ;
    skos:changeNote [
        dc:date "2025-03-04" ;
        rdf:value "Introduced in RiC-O 1.1."@en
    ] ;
    skos:scopeNote """The object properties rico:directlyIncludes and
         rico:hasDirectConstituent, or variants of these which are sub-properties of
         rico:hasOrHadPart, should always be used to express hierarchies in RiC-O. The
         rico:rankInHierarchy datatype property should only be used in addition (never
         independently), for convenience (for example to help display or query a graph). But it
         should be ensured that it reflects and is compatible with (e.g. computed using) the
         hierarchical object properties in the intended context (e.g. a hierarchy of Record Parts in
         a given Record). Thus, if, for example, Record Part A rico:hasDirectConstituent Record Part
         B, then the rico:rankInHierarchy of Record Part B must be strictly greater than
         rico:rankInHierarchy of Record Part A, and no other Record Part in that context should have
         rico:rankInHierarchy between that of Record Part A and Record Part B. For a given Record
         Resource, rico:rankInHierarchy should never be used more than once. If a Record Resource
         belongs to more than one hierarchy, a rico:Proxy of the Record Resource should be
         introduced, and rico:rankInHierarchy have source such a proxy, in all cases except
         (possibly) the first."""@en .

:rankInSequence
    a owl:DatatypeProperty ;
    rdfs:comment """The rank of a Record Resource, or of a Proxy that stands for it,
         in a sequence."""@en ;
    rdfs:domain [
        a owl:Class ;
        owl:unionOf (:RecordResource
            :Proxy
        )
    ] ;
    rdfs:isDefinedBy <https://www.ica.org/standards/RiC/ontology> ;
    rdfs:label "rang dans la séquence"@fr, "rango en la secuencia"@es, "rank in sequence"@en ;
    rdfs:range xsd:int ;
    rdfs:subPropertyOf :textualValue ;
    skos:changeNote [
        dc:date "2025-03-04" ;
        rdf:value "Introduced in RiC-O 1.1."@en
    ] ;
    skos:scopeNote """The object property rico:precedesOrPreceded or one of its
         sub-properties should always be used to express sequences in RiC-O. The rico:rankInSequence
         datatype property should only be used in addition (never independently), for convenience
         (for example to help display or query a graph). But it should be ensured that it reflects
         and is compatible with (e.g. computed using) the sequential object properties in the
         intended context (e.g. the Records in a given Record Set). Thus, if, for example, Record
         Resource A rico:precedesOrPreceded Record Resource B, then the rico:rankInSequence of
         Record Resource B must be strictly greater than rico:rankInSequence of Record Resource A,
         and no other Record Resource in that context should have rico:rankInSequence between that
         of Record Resource A and Record Resource B. For a given Record Resource,
         rico:rankInSequence should never be used more than once. If a Record Resource belongs to
         more than one sequence, a rico:Proxy of the Record Resource should be introduced, and
         rico:rankInSequence have source such a proxy, in all cases except (possibly) the
         first."""@en .

:recordResourceExtent
    a owl:DatatypeProperty ;
    rdfs:comment """The quantity of information content, as human experienced,
         contained in a Record Resource. The method and precision of expressing the quantity of
         information represented in a Record Resource will vary according to the kind of Record
         Resource being described, processing economy constraints, etc. For record sets, quantity
         may be expressed as number of records, or, for analogue records in particular, by the
         physical storage dimensions of the members of the Record Set. For individual records or
         record parts, quantity may be expressed in more precise terms. """@en ;
    rdfs:domain :RecordResource ;
    rdfs:isDefinedBy <https://www.ica.org/standards/RiC/ontology> ;
    rdfs:label "Record Resource Extent"@en, "mesure de la ressource archivistique"@fr, "soporte de recurso documental"@es ;
    rdfs:range rdfs:Literal ;
    rdfs:subPropertyOf :physicalOrLogicalExtent ;
    skos:changeNote [
        dc:date "2024-03-15" ;
        rdf:value "Fix capitalisation in English label."@en
    ], [
        dc:date "2023-11-11" ;
        rdf:value """Aligned with RiC-CM 1.0: updated the description
               (rdfs:comment), skos:scopeNote, examples (skos:example)."""@en
    ], [
        dc:date "2023-11-02" ;
        rdf:value "Added a new rdfs:label in Spanish."@en
    ], [
        dc:date "2023-08-25" ;
        rdf:value "Added a new rdfs:label in French."@en
    ], [
        dc:date "2020-11-21" ;
        rdf:value """Updated the scope note, as a RecordResourceExtent class has
               been created."""@en
    ], [
        dc:date "2020-11-01" ;
        rdf:value """Text definition and scope note updated. Examples added.
               Objective: to make RiC-O compliant with RiC-CM v0.2."""@en
    ] ;
    skos:example "1,500 words"@en, "2 films"@en, "2.065.735 characters"@en, "3 minutes and 24 seconds"@en, "6 maps"@en, "6 photographs"@en ;
    skos:scopeNote """Use if you don't use RecordResourceExtent class and its
         properties for handling such information. Record resource extent should not be confused
         with instantiation extent or carrier extent. The number, size or duration of the
         information content unit(s) remains the same even if the information is instantiated in
         various carriers. For example, a CD with a storage capacity of 700 MB (carrier extent)
         might hold a record of 1,500 words (record resource extent) represented in two versions,
         one a Word document with an instantiation extent of 3 KB and the other a PDF file with an
         instantiation extent of 5 KB."""@en ;
    :RiCCMCorrespondingComponent """Corresponds to RiC-A35 (Record Resource Extent
         attribute)"""@en .

:recordResourceGeneticRelation_role
    a owl:ObjectProperty ;
    rdfs:comment """Connects a RecordResourceGeneticRelation to itself. It is a
         property that can stand for an instance of the class when necessary, e.g. when you explore
         a knowledge graph."""@en ;
    rdfs:domain :RecordResourceGeneticRelation ;
    rdfs:isDefinedBy <https://www.ica.org/standards/RiC/ontology> ;
    rdfs:label """a le rôle de la Relation génétique entre des ressources
         archivistiques"""@fr, """desempeña el papel de la Relación genética entre recursos
         documentales"""@es, "has the role of the Record Resource Genetic Relation"@en ;
    rdfs:range :RecordResourceGeneticRelation ;
    rdfs:subPropertyOf :recordResourceToRecordResourceRelation_role ;
    skos:changeNote [
        dc:date "2024-08-02" ;
        rdf:value """Removed global reflexivity (leads to
               inconsistency)."""@en
    ], [
        dc:date "2023-11-08" ;
        rdf:value """In order to get a system of rolified Relation classes: created
               the object property, with domain and range the RecordResourceGeneticRelation rolified
               class. Declared it as reflexive. Declared it(s) superproperty(ies)."""@en
    ] ;
    skos:scopeNote """This property \"rolifies\" the RecordResourceGeneticRelation
         class. It should be used only when you have to manage instances of the
         RecordResourceGeneticRelation class, to connect each instance to itself, in order to be
         able to infer, using OWL-RL and property paths, the two shortcuts corresponding to this
         n-ary class."""@en .

:recordResourceHasSourceOfInformation
    a owl:ObjectProperty ;
    rdfs:comment """Connects a Record Resource to a Record Resource, when the second
         one is used as a source of information for producing the content of the first
         one."""@en ;
    rdfs:domain :RecordResource ;
    rdfs:isDefinedBy <https://www.ica.org/standards/RiC/ontology> ;
    rdfs:label "Record Resource has source of information"@en, """est une ressource archivistique qui a pour source
         d’information"""@fr, "recurso documental tiene como fuente de información"@es ;
    rdfs:range :RecordResource ;
    rdfs:subPropertyOf :isRecordResourceAssociatedWithRecordResource ;
    owl:inverseOf :isSourceOfInformationOfRecordResource ;
    skos:changeNote [
        dc:date "2025-01-17" ;
        rdf:value """Object property added in RiC-O 1.1, with its inverse one. It
               replaces, as concerns Record Resources, the former 'hasSource' object property, that
               was available in RiC-0 0.1 and RiC-O 0.2, and was removed in RiC-O 1.0."""@en
    ] ;
    skos:scopeNote """Can be used, for example, to connect a Record that has
         documentary form type Authority Record or Finding Aid, and a Record Resource used as a
         source of information for it. Not to be confused with the 'hasGeneticLinkToRecordResource'
         object property."""@en .

:recordResourceHoldingRelation_role
    a owl:ObjectProperty ;
    rdfs:comment """Connects a RecordResourceHoldingRelation to itself. It is a
         property that can stand for an instance of the class when necessary, e.g. when you explore
         a knowledge graph."""@en ;
    rdfs:domain :RecordResourceHoldingRelation ;
    rdfs:isDefinedBy <https://www.ica.org/standards/RiC/ontology> ;
    rdfs:label """a le rôle de la Relation entre agents et ressources archivistiques
         ou instanciations conservées"""@fr, """desempeña el papel de la Relación entre agentes y recursos
         documentales que conservan"""@es, "has the role of the Record Resource Holding Relation"@en ;
    rdfs:range :RecordResourceHoldingRelation ;
    rdfs:subPropertyOf :managementRelation_role ;
    skos:changeNote [
        dc:date "2024-08-02" ;
        rdf:value """Removed global reflexivity (leads to
               inconsistency)."""@en
    ], [
        dc:date "2023-12-30" ;
        rdf:value "Fixed a typo in the French label."@en
    ], [
        dc:date "2023-11-08" ;
        rdf:value """In order to get a system of rolified Relation classes: created
               the object property, with domain and range the RecordResourceHoldingRelation rolified
               class. Declared it as reflexive. Declared it(s) superproperty(ies)."""@en
    ] ;
    skos:scopeNote """This property \"rolifies\" the RecordResourceHoldingRelation
         class. It should be used only when you have to manage instances of the
         RecordResourceHoldingRelation class, to connect each instance to itself, in order to be
         able to infer, using OWL-RL and property paths, the two shortcuts corresponding to this
         n-ary class."""@en .

:recordResourceSourceOfInformation
    a owl:DatatypeProperty ;
    rdfs:comment """Information about some source on which the content of a Record
         Resource is based."""@en ;
    rdfs:domain :RecordResource ;
    rdfs:isDefinedBy <https://www.ica.org/standards/RiC/ontology> ;
    rdfs:label "Record Resource source of information"@en, "fuente de información de recurso documental"@es, "source d’information de la ressource archivistique"@fr ;
    rdfs:range rdfs:Literal ;
    skos:changeNote [
        dc:date "2025-01-16" ;
        rdf:value """Datatype property added in RiC-O 1.1. It replaces, as concerns
               Record Resources, the former 'source' datatype property, that was available in RiC-0
               0.1 and RiC-O 0.2, and was removed in RiC-O 1.0."""@en
    ] ;
    skos:example """Dardy-Cretin (Michèle), Histoire administrative du ministère de la
         culture et de la communication (1959-2012). Paris: Collection du Comité d’histoire du
         ministère de la culture et de la communication, 2012."""@fr ;
    skos:scopeNote """Can be used, for example, for Records having documentary form
         type Authority Record or Finding Aid. Use only if you don't use the
         'recordResourceHasSourceOfInformation' object property."""@en .

:recordResourceStructure
    a owl:DatatypeProperty ;
    rdfs:comment """Information about the intellectual arrangement and composition of
         a Record Resource. For Record and Record Part, it encompasses information about the
         intellectual composition of the record, the presence of record parts and their functions.
         For Record Set, it encompasses information about the methodology or criteria used for
         arranging the Record Set members or Record members within the containing Record
         Set"""@en ;
    rdfs:domain :RecordResource ;
    rdfs:isDefinedBy <https://www.ica.org/standards/RiC/ontology> ;
    rdfs:label "Record Resource structure"@en, "estructura de recurso documental"@es, "structure de la ressource archivistique"@fr ;
    rdfs:range rdfs:Literal ;
    rdfs:subPropertyOf :structure ;
    skos:changeNote [
        dc:date "2023-11-02" ;
        rdf:value "Added a new rdfs:label in Spanish."@en
    ], [
        dc:date "2023-08-25" ;
        rdf:value "Added a new rdfs:label in French."@en
    ], [
        dc:date "2020-11-01" ;
        rdf:value """Text definition updated. Examples added. Objective: to make
               RiC-O compliant with RiC-CM v0.2."""@en
    ] ;
    skos:example """Inside each file, the records are arranged
         chronologically."""@en, """The database has 3 related tables: names, addresses, and passport
         numbers."""@en, """The record has 2 appendixes, comprising a full account of the
         income from car taxes and real estate taxes."""@en, """The series have the files arranged according to the alphabetical
         order of the places concerned."""@en ;
    :RiCCMCorrespondingComponent """Specialization of RiC-A40 (Structure
         attribute)"""@en .

:recordResourceToInstantiationRelation_role
    a owl:ObjectProperty ;
    rdfs:comment """Connects a RecordResourceToInstantiationRelation to itself. It is
         a property that can stand for an instance of the class when necessary, e.g. when you
         explore a knowledge graph."""@en ;
    rdfs:domain :RecordResourceToInstantiationRelation ;
    rdfs:isDefinedBy <https://www.ica.org/standards/RiC/ontology> ;
    rdfs:label "a le rôle de la Relation d’instanciation"@fr, """desempeña el papel de la Relación de recurso documental a
         instanciación"""@es, """has the role of the Record Resource to Instantiation
         Relation"""@en ;
    rdfs:range :RecordResourceToInstantiationRelation ;
    rdfs:subPropertyOf :relation_role ;
    skos:changeNote [
        dc:date "2024-08-02" ;
        rdf:value """Removed global reflexivity (leads to
               inconsistency)."""@en
    ], [
        dc:date "2023-11-08" ;
        rdf:value """In order to get a system of rolified Relation classes: created
               the object property, with domain and range the RecordResourceToInstantiationRelation
               rolified class. Declared it as reflexive. Declared it(s)
               superproperty(ies)."""@en
    ] ;
    skos:scopeNote """This property \"rolifies\" the
         RecordResourceToInstantiationRelation class. It should be used only when you have to manage
         instances of the RecordResourceToInstantiationRelation class, to connect each instance to
         itself, in order to be able to infer, using OWL-RL and property paths, the two shortcuts
         corresponding to this n-ary class."""@en .

:recordResourceToRecordResourceRelation_role
    a owl:ObjectProperty ;
    rdfs:comment """Connects a RecordResourceToRecordResourceRelation to itself. It is
         a property that can stand for an instance of the class when necessary, e.g. when you
         explore a knowledge graph."""@en ;
    rdfs:domain :RecordResourceToRecordResourceRelation ;
    rdfs:isDefinedBy <https://www.ica.org/standards/RiC/ontology> ;
    rdfs:label """a le rôle de la Relation entre ressources
         archivistiques"""@fr, """desempeña el papel de la Relación entre recursos
         documentales"""@es, """has the role of the Record Resource to Record Resource
         Relation"""@en ;
    rdfs:range :RecordResourceToRecordResourceRelation ;
    rdfs:subPropertyOf :relation_role ;
    skos:changeNote [
        dc:date "2024-08-02" ;
        rdf:value """Removed global reflexivity (leads to
               inconsistency)."""@en
    ], [
        dc:date "2023-11-08" ;
        rdf:value """In order to get a system of rolified Relation classes: created
               the object property, with domain and range the RecordResourceToRecordResourceRelation
               rolified class. Declared it as reflexive. Declared it(s)
               superproperty(ies)."""@en
    ] ;
    skos:scopeNote """This property \"rolifies\" the
         RecordResourceToRecordResourceRelation class. It should be used only when you have to
         manage instances of the RecordResourceToRecordResourceRelation class, to connect each
         instance to itself, in order to be able to infer, using OWL-RL and property paths, the two
         shortcuts corresponding to this n-ary class."""@en .

:referenceSystem
    a owl:DatatypeProperty ;
    rdfs:comment """Framework or standard used to represent an
         information."""@en ;
    rdfs:domain :Thing ;
    rdfs:isDefinedBy <https://www.ica.org/standards/RiC/ontology> ;
    rdfs:label "reference system"@en, "sistema de referencia"@es, "système de référence"@fr ;
    rdfs:range rdfs:Literal ;
    skos:changeNote [
        dc:date "2023-11-02" ;
        rdf:value "Added a new rdfs:label in Spanish."@en
    ], [
        dc:date "2023-08-25" ;
        rdf:value "Added a new rdfs:label in French."@en
    ] .

:regulatesOrRegulated
    a owl:ObjectProperty ;
    rdfs:comment """Connects a Rule to a Thing that it regulates or
         regulated."""@en ;
    rdfs:domain :Rule ;
    rdfs:isDefinedBy <https://www.ica.org/standards/RiC/ontology> ;
    rdfs:label "regula o regulaba"@es, "regulates or regulated"@en, "régule ou a régulé"@fr ;
    rdfs:range :Thing ;
    rdfs:subPropertyOf :isRuleAssociatedWith ;
    owl:inverseOf :isOrWasRegulatedBy ;
    skos:changeNote [
        dc:date "2023-11-02" ;
        rdf:value "Added a new rdfs:label in Spanish."@en
    ], [
        dc:date "2023-08-28" ;
        rdf:value "Added a new rdfs:label in French."@en
    ], [
        dc:date "2021-01-22" ;
        rdf:value """changed the IRI, label, inverse property IRI (changed made in
               order to make RiC-O compliant with RiC-CM 0.2; the name of this property in RiC-O 0.1
               was \"regulates\")."""@en
    ] ;
    :RiCCMCorrespondingComponent """RiC-R063 ('regulates or regulated'
         relation)"""@en .

:relationCertainty
    a owl:DatatypeProperty ;
    rdfs:comment """Qualifies the level of certitude of the accuracy of a
         Relation."""@en ;
    rdfs:domain :Relation ;
    rdfs:isDefinedBy <https://www.ica.org/standards/RiC/ontology> ;
    rdfs:label "certeza de la relación"@es, "degré de certitude de la relation"@fr, "relation certainty "@en ;
    rdfs:range rdfs:Literal ;
    skos:changeNote [
        dc:date "2023-12-27" ;
        rdf:value """Renamed the datatype property (was 'certainty') and reduced its
               domain to Relation (the dmain was the union of Event and Relation). Consequently
               updated the labels."""@en
    ], [
        dc:date "2023-11-02" ;
        rdf:value "Added a new rdfs:label in Spanish."@en
    ], [
        dc:date "2023-10-14" ;
        rdf:value """Reintroduced this datatype property, with the definition
               assigned to it in RiC-CM 1.0, apart from its domain that also includes
               Event."""@en
    ] ;
    skos:example "certain"@en, "uncertain"@en, "unknown"@en ;
    :RiCCMCorrespondingComponent """Corresponds to RiC-RA01 (Certainty of Relation
         attribute)"""@en .

:relationConnects
    a owl:ObjectProperty ;
    rdfs:comment """Connects an n-ary Relation to any of the Things
         involved."""@en ;
    rdfs:domain :Relation ;
    rdfs:isDefinedBy <https://www.ica.org/standards/RiC/ontology> ;
    rdfs:label "relación conecta"@es, "relation connecte"@fr, "relation connects"@en ;
    rdfs:range :Thing ;
    rdfs:subPropertyOf :isRelatedTo ;
    owl:inverseOf :thingIsConnectedToRelation ;
    skos:changeNote [
        dc:date "2023-11-02" ;
        rdf:value "Added a new rdfs:label in Spanish."@en
    ], [
        dc:date "2023-08-28" ;
        rdf:value "Added a new rdfs:label in French."@en
    ] .

:relationHasContext
    a owl:ObjectProperty ;
    rdfs:comment """Connects an n-ary Relation to a Thing that is a secondary,
         contextual entity during the existence of the Relation."""@en ;
    rdfs:domain :Relation ;
    rdfs:isDefinedBy <https://www.ica.org/standards/RiC/ontology> ;
    rdfs:label "relación tiene como contexto"@es, "relation a pour contexte"@fr, "relation has context"@en ;
    rdfs:range :Thing ;
    rdfs:subPropertyOf :relationConnects ;
    owl:inverseOf :thingIsContextOfRelation ;
    skos:changeNote [
        dc:date "2023-11-02" ;
        rdf:value "Added a new rdfs:label in Spanish."@en
    ], [
        dc:date "2023-08-28" ;
        rdf:value "Added a new rdfs:label in French."@en
    ] ;
    skos:scopeNote """The secondary entity may be, for instance, a Position or a Role
         Type."""@en .

:relationHasDate
    a owl:ObjectProperty ;
    rdfs:comment "Connects an n-ary Relation to a Date."@en ;
    rdfs:domain :Relation ;
    rdfs:isDefinedBy <https://www.ica.org/standards/RiC/ontology> ;
    rdfs:label "relación tiene como fecha"@es, "relation a pour date"@fr, "relation has date"@en ;
    rdfs:range :Date ;
    rdfs:subPropertyOf :isAssociatedWithDate, :relationHasContext ;
    owl:inverseOf :isDateAssociatedWithRelation ;
    skos:changeNote [
        dc:date "2025-03-13" ;
        rdf:value "Added French and Spanish labels."@en
    ], [
        dc:date "2024-12-19" ;
        rdf:value "Added in RiC-O 1.1."@en
    ] .

:relationHasSource
    a owl:ObjectProperty ;
    rdfs:comment """Connects an n-ary Relation to a Thing that is its
         source."""@en ;
    rdfs:domain :Relation ;
    rdfs:isDefinedBy <https://www.ica.org/standards/RiC/ontology> ;
    rdfs:label "relación tiene como fuente"@es, "relation a pour source"@fr, "relation has source"@en ;
    rdfs:range :Thing ;
    rdfs:subPropertyOf :relationConnects ;
    owl:inverseOf :thingIsSourceOfRelation ;
    skos:changeNote [
        dc:date "2023-11-02" ;
        rdf:value "Added a new rdfs:label in Spanish."@en
    ], [
        dc:date "2023-08-28" ;
        rdf:value "Added a new rdfs:label in French."@en
    ] .

:relationHasTarget
    a owl:ObjectProperty ;
    rdfs:comment """Connects an n-ary Relation to a Thing that is its
         target."""@en ;
    rdfs:domain :Relation ;
    rdfs:isDefinedBy <https://www.ica.org/standards/RiC/ontology> ;
    rdfs:label "relación tiene como objetivo"@es, "relation a pour cible"@fr, "relation has target"@en ;
    rdfs:range :Thing ;
    rdfs:subPropertyOf :relationConnects ;
    owl:inverseOf :thingIsTargetOfRelation ;
    skos:changeNote [
        dc:date "2023-11-02" ;
        rdf:value "Added a new rdfs:label in Spanish."@en
    ], [
        dc:date "2023-08-28" ;
        rdf:value "Added a new rdfs:label in French."@en
    ] .

:relationSource
    a owl:DatatypeProperty ;
    rdfs:comment """A source of information used for identifying and describing a
         Relation."""@en ;
    rdfs:domain :Relation ;
    rdfs:isDefinedBy <https://www.ica.org/standards/RiC/ontology> ;
    rdfs:label "fuente de la relación"@es, "relation source"@en, "source de la relation"@fr ;
    rdfs:range rdfs:Literal ;
    skos:changeNote [
        dc:date "2023-12-27" ;
        rdf:value """Renamed the datatype property (was 'source') and reduced its
               domain to Relation (the domain was the union of Record Resource and Relation).
               Consequently updated the rdfs:comment, labels and scope note. Added a
               rico:RiCCMCorrespondingComponent annotation."""@en
    ], [
        dc:date "2023-11-02" ;
        rdf:value "Added a new rdfs:label in Spanish."@en
    ], [
        dc:date "2023-08-25" ;
        rdf:value "Added a new rdfs:label in French."@en
    ] ;
    skos:scopeNote """Use only if you don't use the 'isEvidencedBy' object
         property."""@en ;
    :RiCCMCorrespondingComponent """Corresponds to RiC-RA05 (Source of Relation
         attribute)."""@en .

:relationState
    a owl:DatatypeProperty ;
    rdfs:comment """Used to qualify the state of a Relation (e. g. present, past,
         ongoing, unknown)."""@en ;
    rdfs:domain :Relation ;
    rdfs:isDefinedBy <https://www.ica.org/standards/RiC/ontology> ;
    rdfs:label "estado de la relación"@es, "relation state"@en, "statut de la relation"@fr ;
    rdfs:range rdfs:Literal ;
    skos:changeNote [
        dc:date "2023-11-02" ;
        rdf:value "Added a new rdfs:label in Spanish."@en
    ], [
        dc:date "2023-08-25" ;
        rdf:value "Added a new rdfs:label in French."@en
    ] .

:relation_role
    a owl:ObjectProperty ;
    rdfs:comment """Connects a Relation to itself. It is a property that can stand for
         an instance of the class when necessary, e.g. when you explore a knowledge
         graph."""@en ;
    rdfs:domain :Relation ;
    rdfs:isDefinedBy <https://www.ica.org/standards/RiC/ontology> ;
    rdfs:label "a le rôle de la Relation"@fr, "desempeña el papel de la Relación"@es, "has the role of the Relation"@en ;
    rdfs:range :Relation ;
    skos:changeNote [
        dc:date "2024-08-02" ;
        rdf:value """Removed global reflexivity (leads to
               inconsistency)."""@en
    ], [
        dc:date "2023-11-08" ;
        rdf:value """In order to get a system of rolified Relation classes: created
               the object property, with domain and range the Relation rolified class. Declared it
               as reflexive."""@en
    ] ;
    skos:scopeNote """This property \"rolifies\" the generic Relation class. It should
         be used only when you have to manage instances of this Relation class, to connect each
         instance to itself, in order to be able to infer, using OWL-RL and property paths, the two
         shortcuts corresponding to this n-ary class."""@en .

:resultedFromTheMergerOf
    a owl:ObjectProperty ;
    rdfs:comment "Inverse of 'was merged into' object property."@en ;
    rdfs:domain :CorporateBody ;
    rdfs:isDefinedBy <https://www.ica.org/standards/RiC/ontology> ;
    rdfs:label "resultado de la fusión de"@es, "resulted from the merger of"@en, "résulte de la fusion de"@fr ;
    rdfs:range :CorporateBody ;
    rdfs:subPropertyOf :isSuccessorOf ;
    owl:inverseOf :wasMergedInto ;
    skos:changeNote [
        dc:date "2024-03-15" ;
        rdf:value "Make capitalisation of rdfs:comment consistent."@en
    ], [
        dc:date "2023-11-12" ;
        rdf:value "Updated the labels."@en
    ], [
        dc:date "2023-11-02" ;
        rdf:value "Added a new rdfs:label in Spanish."@en
    ], [
        dc:date "2023-06-21" ;
        rdf:value """Object property created in order to enable an accurate
               representation of mergers between corporate bodies."""@en
    ] .

:resultedFromTheSplitOf
    a owl:ObjectProperty ;
    rdfs:comment "Inverse of 'was split into' object property."@en ;
    rdfs:domain :CorporateBody ;
    rdfs:isDefinedBy <https://www.ica.org/standards/RiC/ontology> ;
    rdfs:label "resultado de la separación de"@es, "resulted from the split of"@en, "résulte de la séparation de"@fr ;
    rdfs:range :CorporateBody ;
    rdfs:subPropertyOf :isSuccessorOf ;
    owl:inverseOf :wasSplitInto ;
    skos:changeNote [
        dc:date "2023-11-12" ;
        rdf:value "Updated the labels."@en
    ], [
        dc:date "2023-11-02" ;
        rdf:value "Added a new rdfs:label in Spanish."@en
    ], [
        dc:date "2023-06-21" ;
        rdf:value """Object property created in order to enable an accurate
               representation of the split of a corporate body into two or more new corporate
               bodies."""@en
    ] .

:resultsOrResultedFrom
    a owl:ObjectProperty ;
    rdfs:comment """Inverse of 'results or resulted in' object
         property."""@en ;
    rdfs:domain :Thing ;
    rdfs:isDefinedBy <https://www.ica.org/standards/RiC/ontology> ;
    rdfs:label "resulta o resultaba"@es, "results or resulted from"@en, "résulte ou a résulté de"@fr ;
    rdfs:range :Event ;
    rdfs:subPropertyOf :isAssociatedWithEvent ;
    owl:inverseOf :resultsOrResultedIn ;
    skos:changeNote [
        dc:date "2023-11-02" ;
        rdf:value "Added a new rdfs:label in Spanish."@en
    ], [
        dc:date "2023-08-28" ;
        rdf:value "Added a new rdfs:label in French."@en
    ], [
        dc:date "2021-01-22" ;
        rdf:value """changed the IRI, label, inverse property IRI, text definition
               (changed made in order to make RiC-O compliant with RiC-CM 0.2; the name of this
               property in RiC-O 0.1 was \"resultsFrom\")."""@en
    ] ;
    :RiCCMCorrespondingComponent """RiC-R061i ('results or resulted from'
         relation)"""@en .

:resultsOrResultedIn
    a owl:ObjectProperty ;
    rdfs:comment """Connects an Event to a Thing that results or resulted from the
         Event."""@en ;
    rdfs:domain :Event ;
    rdfs:isDefinedBy <https://www.ica.org/standards/RiC/ontology> ;
    rdfs:label "a ou a eu pour résultat"@fr, "results or resulted in"@en, "tiene o tenía como resultado a"@es ;
    rdfs:range :Thing ;
    rdfs:subPropertyOf :isEventAssociatedWith ;
    owl:inverseOf :resultsOrResultedFrom ;
    skos:changeNote [
        dc:date "2023-11-02" ;
        rdf:value "Added a new rdfs:label in Spanish."@en
    ], [
        dc:date "2023-08-28" ;
        rdf:value "Added a new rdfs:label in French."@en
    ], [
        dc:date "2021-01-22" ;
        rdf:value """changed the IRI, label, inverse property IRI, text definition
               (changed made in order to make RiC-O compliant with RiC-CM 0.2; the name of this
               property in RiC-O 0.1 was \"resultsIn\")."""@en
    ] ;
    :RiCCMCorrespondingComponent """RiC-R061 ('results or resulted in'
         relation)"""@en .

:roleIsContextOfCreationRelation
    a owl:ObjectProperty ;
    rdfs:comment """Connects a Role Type to a Creation Relation (this Role Type being
         the specific role played by the creating Person in the context of this
         Relation)."""@en ;
    rdfs:domain :RoleType ;
    rdfs:isDefinedBy <https://www.ica.org/standards/RiC/ontology> ;
    rdfs:label "rol es contexto de relación de creación"@es, "role is context of creation relation"@en, "rôle est le contexte de la relation de création"@fr ;
    rdfs:range :CreationRelation ;
    rdfs:subPropertyOf :thingIsContextOfRelation ;
    owl:inverseOf :creationWithRole ;
    skos:changeNote [
        dc:date "2023-11-02" ;
        rdf:value "Added a new rdfs:label in Spanish."@en
    ], [
        dc:date "2023-08-28" ;
        rdf:value "Added a new rdfs:label in French."@en
    ] .

:ruleFollowed
    a owl:DatatypeProperty ;
    rdfs:comment """The rule or conditions that govern the existence or lifecycle of a
         Thing."""@en ;
    rdfs:domain :Thing ;
    rdfs:isDefinedBy <https://www.ica.org/standards/RiC/ontology> ;
    rdfs:label "regla aplicada"@es, "rule followed"@en, "règle suivie"@fr ;
    rdfs:range rdfs:Literal ;
    skos:changeNote [
        dc:date "2023-11-02" ;
        rdf:value "Added a new rdfs:label in Spanish."@en
    ], [
        dc:date "2023-08-25" ;
        rdf:value "Added a new rdfs:label in French."@en
    ] ;
    skos:scopeNote """Provided for usability reasons. May be deprecated and removed
         later on. Use only if you don't use the Rule class for handling rules."""@en .

:ruleRelation_role
    a owl:ObjectProperty ;
    rdfs:comment """Connects a RuleRelation to itself. It is a property that can stand
         for an instance of the class when necessary, e.g. when you explore a knowledge
         graph."""@en ;
    rdfs:domain :RuleRelation ;
    rdfs:isDefinedBy <https://www.ica.org/standards/RiC/ontology> ;
    rdfs:label "a le rôle de la Relation impliquant une règle"@fr, "desempeña el papel de la Relación con regla"@es, "has the role of the Rule Relation"@en ;
    rdfs:range :RuleRelation ;
    rdfs:subPropertyOf :relation_role ;
    skos:changeNote [
        dc:date "2024-08-02" ;
        rdf:value """Removed global reflexivity (leads to
               inconsistency)."""@en
    ], [
        dc:date "2023-11-08" ;
        rdf:value """In order to get a system of rolified Relation classes: created
               the object property, with domain and range the RuleRelation rolified class. Declared
               it as reflexive. Declared it(s) superproperty(ies)."""@en
    ] ;
    skos:scopeNote """This property \"rolifies\" the RuleRelation class. It should be
         used only when you have to manage instances of the RuleRelation class, to connect each
         instance to itself, in order to be able to infer, using OWL-RL and property paths, the two
         shortcuts corresponding to this n-ary class."""@en .

:scopeAndContent
    a owl:DatatypeProperty ;
    rdfs:comment """Summary of the scope (such as time periods, geography) and content
         (such as subject matter, administrative processes) of a Record Resource. Provides a more
         complete summary of the informational content of the Record Resource highlighting the
         information conveyed in the Record Resource, why it was created, received, and/or
         maintained, and the agents connected to it. It may include description of relations with
         agents, activities, dates and places, or with other record resources."""@en ;
    rdfs:domain :RecordResource ;
    rdfs:isDefinedBy <https://www.ica.org/standards/RiC/ontology> ;
    rdfs:label "alcance y contenido"@es, "portée et contenu"@fr, "scope and content"@en ;
    rdfs:range rdfs:Literal ;
    rdfs:subPropertyOf :generalDescription ;
    skos:changeNote [
        dc:date "2023-11-11" ;
        rdf:value """Aligned with RiC-CM 1.0: updated the description
               (rdfs:comment), skos:scopeNote, rdfs:subpropertyOf, examples
               (skos:example)."""@en
    ], [
        dc:date "2023-11-02" ;
        rdf:value "Added a new rdfs:label in Spanish."@en
    ], [
        dc:date "2023-08-25" ;
        rdf:value "Added a new rdfs:label in French."@en
    ], [
        dc:date "2023-08-25" ;
        rdf:value "Added a new rdfs:label in French."@en
    ], [
        dc:date "2020-11-01" ;
        rdf:value """Text definition updated. Examples added. Objective: to make
               RiC-O compliant with RiC-CM v0.2."""@en
    ] ;
    skos:example "Among the witnesses, the Duke of Normandy."@en, """Includes a detailed list of the lands and villages given by the
         King to the Abbey."""@en, """Letter from Vlad the Impaler (Dracula) to the Council of Kronstadt
         asking them to send military support against the Ottomans, within the framework of their
         alliance treaty."""@en, """Se hace referencia a construcción del Gran Hotel, iniciada en 1899
         bajo el nombre de Casa Celestino. Tras su interrupción en 1902, continuó la obra ya con su
         nombre actual."""@es, """The author explains why he does not agree with the decision made
         and adds that it cannot be applied."""@en ;
    skos:scopeNote """Scope and content is a specialization of general description.
         For a Record Set, may be used to summarize the scope and content of the Record Set itself,
         or additionally to summarize the scope and content of some or all members of the Record
         Set. It is not to be confused with the history dataytpe property which focuses on the
         origination and subsequent changes to a Record Resource. """@en ;
    :RiCCMCorrespondingComponent """Corresponds to RiC-A38 (Scope and Content
         attribute)"""@en .

:sentimentOrEmotionExpressed
    a owl:DatatypeProperty ;
    rdfs:comment """Specification of, or information about, the sentiment(s) or
         emotion(s) expressed by the content of a Record or a Record Part."""@en ;
    rdfs:domain [
        a owl:Class ;
        owl:unionOf (:Record
            :RecordPart
        )
    ] ;
    rdfs:isDefinedBy <https://www.ica.org/standards/RiC/ontology> ;
    rdfs:label "sentiment or emotion expressed"@en, "sentiment ou émotion exprimés"@fr, "sentimiento o emoción expresados"@es ;
    rdfs:range rdfs:Literal ;
    rdfs:subPropertyOf :scopeAndContent ;
    skos:changeNote [
        dc:date "2025-04-05" ;
        rdf:value "Introduced in RiC-O 1.1."@en
    ] ;
    skos:scopeNote """Can in particular be used for textual or visual Records or
         Record Parts."""@en .

:sequentialRelation_role
    a owl:ObjectProperty ;
    rdfs:comment """Connects a SequentialRelation to itself. It is a property that can
         stand for an instance of the class when necessary, e.g. when you explore a knowledge
         graph."""@en ;
    rdfs:domain :SequentialRelation ;
    rdfs:isDefinedBy <https://www.ica.org/standards/RiC/ontology> ;
    rdfs:label "a le rôle de la Relation séquentielle"@fr, "desempeña el papel de la Relación secuencial"@es, "has the role of the Sequential Relation"@en ;
    rdfs:range :SequentialRelation ;
    rdfs:subPropertyOf :relation_role ;
    skos:changeNote [
        dc:date "2024-08-02" ;
        rdf:value """Removed global reflexivity (leads to
               inconsistency)."""@en
    ], [
        dc:date "2023-11-08" ;
        rdf:value """In order to get a system of rolified Relation classes: created
               the object property, with domain and range the SequentialRelation rolified class.
               Declared it as reflexive. Declared it(s) superproperty(ies)."""@en
    ] ;
    skos:scopeNote """This property \"rolifies\" the SequentialRelation class. It should
         be used only when you have to manage instances of the SequentialRelation class, to connect
         each instance to itself, in order to be able to infer, using OWL-RL and property paths, the
         two shortcuts corresponding to this n-ary class."""@en .

:siblingRelation_role
    a owl:ObjectProperty ;
    rdfs:comment """Connects a SiblingRelation to itself. It is a property that can
         stand for an instance of the class when necessary, e.g. when you explore a knowledge
         graph."""@en ;
    rdfs:domain :SiblingRelation ;
    rdfs:isDefinedBy <https://www.ica.org/standards/RiC/ontology> ;
    rdfs:label "a le rôle de la Relation de fratrie"@fr, """desempeña el papel de la Relación familiar entre
         hermanos"""@es, "has the role of the Sibling Relation"@en ;
    rdfs:range :SiblingRelation ;
    rdfs:subPropertyOf :familyRelation_role ;
    skos:changeNote [
        dc:date "2024-08-02" ;
        rdf:value """Removed global reflexivity (leads to
               inconsistency)."""@en
    ], [
        dc:date "2023-11-08" ;
        rdf:value """In order to get a system of rolified Relation classes: created
               the object property, with domain and range the SiblingRelation rolified class.
               Declared it as reflexive. Declared it(s) superproperty(ies)."""@en
    ] ;
    skos:scopeNote """This property \"rolifies\" the SiblingRelation class. It should be
         used only when you have to manage instances of the SiblingRelation class, to connect each
         instance to itself, in order to be able to infer, using OWL-RL and property paths, the two
         shortcuts corresponding to this n-ary class."""@en .

:someMembersWithAccumulationDate
    a owl:DatatypeProperty ;
    rdfs:comment """Date at which some of the present or past members of a Record Set
         were or will be accumulated."""@en ;
    rdfs:domain :RecordSet ;
    rdfs:isDefinedBy <https://www.ica.org/standards/RiC/ontology> ;
    rdfs:label "algunos de sus miembros como fecha de acumulación"@es, "des membres ayant pour date d’accumulation"@fr, "some members with accumulation date"@en ;
    rdfs:range rdfs:Literal ;
    rdfs:subPropertyOf :date ;
    skos:changeNote [
        dc:date "2025-02-19" ;
        rdf:value "Changed definition (added \"or will be\")."@en
    ], [
        dc:date "2024-12-19" ;
        rdf:value "Added in RiC-O 1.1."@en
    ] ;
    skos:scopeNote """Datatype property analogue of
         'hasOrHadSomeMembersWithAccumulationDate', which is provided for usability reasons. May be
         deprecated and removed later on. Use only if you don’t use Date classes for handling
         dates."""@en .

:someMembersWithCreationDate
    a owl:DatatypeProperty ;
    rdfs:comment """Date at which some of the present or past members of a Record Set
         were or will be created."""@en ;
    rdfs:domain :RecordSet ;
    rdfs:isDefinedBy <https://www.ica.org/standards/RiC/ontology> ;
    rdfs:label "algunos de sus miembros como fecha de creación"@es, "des membres ayant pour date de création"@fr, "some members with creation date"@en ;
    rdfs:range rdfs:Literal ;
    rdfs:subPropertyOf :beginningDate ;
    skos:changeNote [
        dc:date "2025-02-19" ;
        rdf:value "Changed definition (added \"or will be\")."@en
    ], [
        dc:date "2024-12-19" ;
        rdf:value "Added in RiC-O 1.1."@en
    ] ;
    skos:scopeNote """Datatype property analogue of
         'hasOrHadSomeMembersWithCreationDate', which is provided for usability reasons. May be
         deprecated and removed later on. Use only if you don’t use Date classes for handling
         dates."""@en ;
    :RiCCMCorrespondingComponent """RiC-R082i ('has or had some members with creation
         date' relation)."""@en .

:spouseRelation_role
    a owl:ObjectProperty ;
    rdfs:comment """Connects a SpouseRelation to itself. It is a property that can
         stand for an instance of the class when necessary, e.g. when you explore a knowledge
         graph."""@en ;
    rdfs:domain :SpouseRelation ;
    rdfs:isDefinedBy <https://www.ica.org/standards/RiC/ontology> ;
    rdfs:label "a le rôle de la Relation matrimoniale"@fr, """desempeña el papel de la Relación matrimonial entre
         personas"""@es, "has the role of the Spouse Relation"@en ;
    rdfs:range :SpouseRelation ;
    rdfs:subPropertyOf :familyRelation_role ;
    skos:changeNote [
        dc:date "2024-08-02" ;
        rdf:value """Removed global reflexivity (leads to
               inconsistency)."""@en
    ], [
        dc:date "2023-11-08" ;
        rdf:value """In order to get a system of rolified Relation classes: created
               the object property, with domain and range the SpouseRelation rolified class.
               Declared it as reflexive. Declared it(s) superproperty(ies)."""@en
    ] ;
    skos:scopeNote """This property \"rolifies\" the SpouseRelation class. It should be
         used only when you have to manage instances of the SpouseRelation class, to connect each
         instance to itself, in order to be able to infer, using OWL-RL and property paths, the two
         shortcuts corresponding to this n-ary class."""@en .

:structure
    a owl:DatatypeProperty ;
    rdfs:comment """Information about the intellectual arrangement and composition of
         a Record Resource or the physical arrangement and composition of an Instantiation. For
         Record and Record Part, it encompasses information about the intellectual composition of
         the record, the presence of record parts and their functions. For Record Set, it
         encompasses information about the methodology or criteria used for arranging the Record Set
         members or Record members within the containing Record Set. For Instantiation, it may
         comprise information about the composition of the physical elements of the
         instantiation"""@en ;
    rdfs:domain [
        a owl:Class ;
        owl:unionOf (:Instantiation
            :RecordResource
        )
    ] ;
    rdfs:isDefinedBy <https://www.ica.org/standards/RiC/ontology> ;
    rdfs:label "estructura"@es, "structure"@en, "structure"@fr ;
    rdfs:range rdfs:Literal ;
    skos:changeNote [
        dc:date "2023-11-11" ;
        rdf:value """Aligned with RiC-CM 1.0: updated the skos:scopeNote, examples
               (skos:example)."""@en
    ], [
        dc:date "2023-11-02" ;
        rdf:value "Added a new rdfs:label in Spanish."@en
    ], [
        dc:date "2023-08-25" ;
        rdf:value "Added a new rdfs:label in French."@en
    ], [
        dc:date "2020-11-01" ;
        rdf:value """Text definition updated. Objective: to make RiC-O compliant
               with RiC-CM v0.2."""@en
    ] ;
    skos:example """Inside each file, the records are arranged chronologically (about
         a record set)"""@en, """The database has three related tables: names, addresses, and
         passport numbers (about a record)"""@en, """The record has two appendices, comprising a full account of the
         income from car taxes and real estate taxes"""@en, """The series have the files arranged according to the alphabetical
         order of the places concerned"""@en ;
    skos:scopeNote """Use only if you cannot use the subproperties (particularly if
         the same free text is being used in your current metadata for describing the record
         resource and the instantiation structure). For a Record Set, may be used to summarize the
         structure of the Record Set itself, or additionally to summarize the structure of some or
         all members of the Record Set. Should not be confused with the classification datatype
         property, which provides information about the category which the Record Set belongs to
         within a classification scheme. """@en ;
    :RiCCMCorrespondingComponent """Corresponds to RiC-A40 (Structure
         attribute)"""@en .

:studiesOrStudiedAt
    a owl:ObjectProperty ;
    rdfs:comment """Connects a Person to an educational institution at which they
         studied or study. Both 'institution' and 'at' can be interpreted broadly."""@en ;
    rdfs:domain :Person ;
    rdfs:isDefinedBy <https://www.ica.org/standards/RiC/ontology> ;
    rdfs:label "estudia o estudió en"@es, "studies or studied at"@en, "étudie ou a étudié à"@fr ;
    rdfs:range :Group ;
    rdfs:subPropertyOf :isOrWasMemberOf ;
    owl:inverseOf :isOrWasAttendedByStudent ;
    owl:propertyChainAxiom (:thingIsTargetOfRelation
        :studyAtRelation_role
        :relationHasSource
    ) ;
    skos:changeNote [
        dc:date "2024-12-23" ;
        rdf:value "Added the French and Spanish labels."@en
    ], [
        dc:date "2024-12-19" ;
        rdf:value "Added in RiC-O 1.1."@en
    ] .

:studyAtRelation_role
    a owl:ObjectProperty ;
    rdfs:comment """Connects a StudyAtRelation to itself. It is a property that can
         stand for an instance of the class when necessary, e.g. when you explore a knowledge
         graph."""@en ;
    rdfs:domain :StudyAtRelation ;
    rdfs:isDefinedBy <https://www.ica.org/standards/RiC/ontology> ;
    rdfs:label """a le rôle de la Relation entre institution d’enseignement et
         étudiants"""@fr, """desempeña el papel de la Relación entre institución educativa y
         estudiantes"""@es, "has the role of the Study At Relation"@en ;
    rdfs:range :StudyAtRelation ;
    rdfs:subPropertyOf :membershipRelation_role ;
    skos:changeNote [
        dc:date "2024-12-23" ;
        rdf:value "Added the French and Spanish labels."@en
    ], [
        dc:date "2024-12-19" ;
        rdf:value "Added in RiC-O 1.1."@en
    ] .

:teachingRelation_role
    a owl:ObjectProperty ;
    rdfs:comment """Connects a TeachingRelation to itself. It is a property that can
         stand for an instance of the class when necessary, e.g. when you explore a knowledge
         graph."""@en ;
    rdfs:domain :TeachingRelation ;
    rdfs:isDefinedBy <https://www.ica.org/standards/RiC/ontology> ;
    rdfs:label "a le rôle de la Relation entre enseignants et étudiants"@fr, """desempeña el papel de la Relación académica entre profesor y
         alumno"""@es, "has the role of the Teaching Relation"@en ;
    rdfs:range :TeachingRelation ;
    rdfs:subPropertyOf :knowingRelation_role ;
    skos:changeNote [
        dc:date "2024-08-02" ;
        rdf:value """Removed global reflexivity (leads to
               inconsistency)."""@en
    ], [
        dc:date "2023-11-08" ;
        rdf:value """In order to get a system of rolified Relation classes: created
               the object property, with domain and range the TeachingRelation rolified class.
               Declared it as reflexive. Declared it(s) superproperty(ies)."""@en
    ] ;
    skos:scopeNote """This property \"rolifies\" the TeachingRelation class. It should
         be used only when you have to manage instances of the TeachingRelation class, to connect
         each instance to itself, in order to be able to infer, using OWL-RL and property paths, the
         two shortcuts corresponding to this n-ary class."""@en .

:technicalCharacteristics
    a owl:DatatypeProperty ;
    rdfs:comment """Describes any relevant physical or software feature of any device
         involved in the creation or management of a Record Resource."""@en ;
    rdfs:domain :Mechanism ;
    rdfs:isDefinedBy <https://www.ica.org/standards/RiC/ontology> ;
    rdfs:label "características técnicas"@es, "caractéristiques techniques"@fr, "technical characteristics"@en ;
    rdfs:range rdfs:Literal ;
    skos:changeNote [
        dc:date "2023-11-11" ;
        rdf:value """Aligned with RiC-CM 1.0: updated the description
               (rdfs:comment), skos:scopeNote."""@en
    ], [
        dc:date "2023-11-02" ;
        rdf:value "Added a new rdfs:label in Spanish."@en
    ], [
        dc:date "2023-08-25" ;
        rdf:value "Added a new rdfs:label in French."@en
    ], [
        dc:date "2020-11-01" ;
        rdf:value """Scope note and examples added. Objective: to make RiC-O
               compliant with RiC-CM v0.2."""@en
    ] ;
    skos:example """Hubble Space Telescope had until 2002 a flawed mirror that
         introduced severe spherical aberration for the images."""@en ;
    skos:scopeNote """Does not include references to the workflow that the Mechanism
         is involved in, which is described under the Activity entity. It emphasizes those features
         that provide a better understanding of the impact of the Mechanism on the
         records."""@en ;
    :RiCCMCorrespondingComponent """Corresponds to RiC-A41 (Technical Characteristics
         attribute)"""@en .

:temporalRelation_role
    a owl:ObjectProperty ;
    rdfs:comment """Connects a TemporalRelation to itself. It is a property that can
         stand for an instance of the class when necessary, e.g. when you explore a knowledge
         graph."""@en ;
    rdfs:domain :TemporalRelation ;
    rdfs:isDefinedBy <https://www.ica.org/standards/RiC/ontology> ;
    rdfs:label "a le rôle de la Relation temporelle"@fr, "desempeña el papel de la Relación temporal"@es, "has the role of the Temporal Relation"@en ;
    rdfs:range :TemporalRelation ;
    rdfs:subPropertyOf :sequentialRelation_role ;
    skos:changeNote [
        dc:date "2024-08-02" ;
        rdf:value """Removed global reflexivity (leads to
               inconsistency)."""@en
    ], [
        dc:date "2023-11-08" ;
        rdf:value """In order to get a system of rolified Relation classes: created
               the object property, with domain and range the TemporalRelation rolified class.
               Declared it as reflexive. Declared it(s) superproperty(ies)."""@en
    ] ;
    skos:scopeNote """This property \"rolifies\" the TemporalRelation class. It should
         be used only when you have to manage instances of the TemporalRelation class, to connect
         each instance to itself, in order to be able to infer, using OWL-RL and property paths, the
         two shortcuts corresponding to this n-ary class."""@en .

:textualValue
    a owl:DatatypeProperty ;
    rdfs:comment "A textual expression of an Appellation or Date."@en ;
    rdfs:domain [
        a owl:Class ;
        owl:unionOf (:Appellation
            :Date
            :Extent
        )
    ] ;
    rdfs:isDefinedBy <https://www.ica.org/standards/RiC/ontology> ;
    rdfs:label "textual value"@en, "valeur textuelle"@fr, "valor textual"@es ;
    rdfs:range rdfs:Literal ;
    skos:changeNote [
        dc:date "2023-11-02" ;
        rdf:value "Added a new rdfs:label in Spanish."@en
    ], [
        dc:date "2023-08-25" ;
        rdf:value "Added a new rdfs:label in French."@en
    ] .

:thingIsConnectedToRelation
    a owl:ObjectProperty ;
    rdfs:comment "Connects a Thing to an n-ary Relation."@en ;
    rdfs:domain :Thing ;
    rdfs:isDefinedBy <https://www.ica.org/standards/RiC/ontology> ;
    rdfs:label "chose est connectée à la relation"@fr, "cosa está conectada con relación"@es, "thing is connected to relation"@en ;
    rdfs:range :Relation ;
    rdfs:subPropertyOf :isRelatedTo ;
    owl:inverseOf :relationConnects ;
    skos:changeNote [
        dc:date "2023-12-30" ;
        rdf:value "Fixed a typo in the French label."@en
    ], [
        dc:date "2023-11-12" ;
        rdf:value "Updated the labels."@en
    ], [
        dc:date "2023-11-02" ;
        rdf:value "Added a new rdfs:label in Spanish."@en
    ] .

:thingIsContextOfRelation
    a owl:ObjectProperty ;
    rdfs:comment """Connects a Thing (that is a secondary, contextual entity during
         the existence of the Relation) to an n-ary Relation."""@en ;
    rdfs:domain :Thing ;
    rdfs:isDefinedBy <https://www.ica.org/standards/RiC/ontology> ;
    rdfs:label "chose est le contexte de la relation"@fr, "cosa es contexto de relación"@es, "thing is context of relation"@en ;
    rdfs:range :Relation ;
    rdfs:subPropertyOf :thingIsConnectedToRelation ;
    owl:inverseOf :relationHasContext ;
    skos:changeNote [
        dc:date "2023-11-12" ;
        rdf:value "Updated the labels."@en
    ], [
        dc:date "2023-11-02" ;
        rdf:value "Added a new rdfs:label in Spanish."@en
    ] .

:thingIsSourceOfRelation
    a owl:ObjectProperty ;
    rdfs:comment """Connects a Thing (that is the source of a Relation) to a
         Relation."""@en ;
    rdfs:domain :Thing ;
    rdfs:isDefinedBy <https://www.ica.org/standards/RiC/ontology> ;
    rdfs:label "chose est la source de la relation"@fr, "cosa es fuente de relación"@es, "thing is source of relation"@en ;
    rdfs:range :Relation ;
    rdfs:subPropertyOf :thingIsConnectedToRelation ;
    owl:inverseOf :relationHasSource ;
    skos:changeNote [
        dc:date "2023-11-27" ;
        rdf:value "Added a new rdfs:label in Spanish."@en
    ], [
        dc:date "2023-11-12" ;
        rdf:value "Updated the labels."@en
    ] .

:thingIsTargetOfRelation
    a owl:ObjectProperty ;
    rdfs:comment """Connects a Thing (that is the target of a Relation) to an n-ary
         Relation."""@en ;
    rdfs:domain :Thing ;
    rdfs:isDefinedBy <https://www.ica.org/standards/RiC/ontology> ;
    rdfs:label "chose est la cible de la relation"@fr, "cosa es objetivo de relación"@es, "thing is target of relation"@en ;
    rdfs:range :Relation ;
    rdfs:subPropertyOf :thingIsConnectedToRelation ;
    owl:inverseOf :relationHasTarget ;
    skos:changeNote [
        dc:date "2023-11-27" ;
        rdf:value "Added a new rdfs:label in Spanish."@en
    ], [
        dc:date "2023-11-12" ;
        rdf:value "Updated the description (rdfs:comment) and labels."@en
    ] .

:title
    a owl:DatatypeProperty ;
    rdfs:comment """An identifying name of a Record Resource, Instantiation or
         Rule."""@en ;
    rdfs:domain [
        a owl:Class ;
        owl:unionOf (:Instantiation
            :RecordResource
            :Rule
        )
    ] ;
    rdfs:isDefinedBy <https://www.ica.org/standards/RiC/ontology> ;
    rdfs:label "intitulé"@fr, "title"@en, "título"@es ;
    rdfs:range rdfs:Literal ;
    rdfs:subPropertyOf :name ;
    skos:changeNote [
        dc:date "2023-11-02" ;
        rdf:value "Added a new rdfs:label in Spanish."@en
    ], [
        dc:date "2023-08-25" ;
        rdf:value "Added a new rdfs:label in French."@en
    ] ;
    skos:scopeNote """Use only if you don't use Title class for handling
         titles."""@en ;
    :RiCCMCorrespondingComponent """Specialization of RiC-A28 (Name
         attribute)"""@en .

:type
    a owl:DatatypeProperty ;
    rdfs:comment "A term used to characterize an entity."@en ;
    rdfs:domain :Thing ;
    rdfs:isDefinedBy <https://www.ica.org/standards/RiC/ontology> ;
    rdfs:label "tipo"@es, "type"@en, "type"@fr ;
    rdfs:range rdfs:Literal ;
    skos:changeNote [
        dc:date "2023-11-02" ;
        rdf:value "Added a new rdfs:label in Spanish."@en
    ], [
        dc:date "2023-08-25" ;
        rdf:value "Added a new rdfs:label in French."@en
    ] ;
    skos:scopeNote """Provided for usability reasons. May be deprecated and removed
         later on. Use only if you don't use Type subclasses for handling
         categories."""@en .

:typeRelation_role
    a owl:ObjectProperty ;
    rdfs:comment """Connects a TypeRelation to itself. It is a property that can stand
         for an instance of the class when necessary, e.g. when you explore a knowledge
         graph."""@en ;
    rdfs:domain :TypeRelation ;
    rdfs:isDefinedBy <https://www.ica.org/standards/RiC/ontology> ;
    rdfs:label "a le rôle de la Relation de catégorisation"@fr, "desempeña el papel de la Tipo de relación"@es, "has the role of the Type Relation"@en ;
    rdfs:range :TypeRelation ;
    rdfs:subPropertyOf :relation_role ;
    skos:changeNote [
        dc:date "2024-08-02" ;
        rdf:value """Removed global reflexivity (leads to
               inconsistency)."""@en
    ], [
        dc:date "2023-11-08" ;
        rdf:value """In order to get a system of rolified Relation classes: created
               the object property, with domain and range the TypeRelation rolified class. Declared
               it as reflexive. Declared it(s) superproperty(ies)."""@en
    ] ;
    skos:scopeNote """This property \"rolifies\" the TypeRelation class. It should be
         used only when you have to manage instances of the TypeRelation class, to connect each
         instance to itself, in order to be able to infer, using OWL-RL and property paths, the two
         shortcuts corresponding to this n-ary class."""@en .

:unitOfMeasurement
    a owl:DatatypeProperty ;
    rdfs:comment """A definite magnitude of a quantity, defined and adopted by
         convention or by law, that is used as a standard for measurement of the same kind of
         quantity. Can be spacial units (cm, m), weight (g, kg), time (s, h), storage (MB, TB) or
         more informal units used in the archival context like number of boxes, pages or
         words."""@en ;
    rdfs:domain :Extent ;
    rdfs:isDefinedBy <https://www.ica.org/standards/RiC/ontology> ;
    rdfs:label "unidad de medida"@es, "unit of measurement"@en, "unité de mesure"@fr ;
    rdfs:range rdfs:Literal ;
    skos:changeNote [
        dc:date "2023-11-02" ;
        rdf:value "Added a new rdfs:label in Spanish."@en
    ], [
        dc:date "2023-08-28" ;
        rdf:value "Added an xml:lang attribute to the rdfs:comment."@en
    ], [
        dc:date "2023-08-25" ;
        rdf:value "Added a new rdfs:label in French."@en
    ], [
        dc:date "2020-11-21" ;
        rdf:value "Added a scope note."@en
    ], [
        dc:date "2020-10-28" ;
        rdf:value """Datatype property created along with quantity, Extent and
               UnitOfMeasurement classes, in order to provide methods for handling extent
               accurately."""@en
    ] ;
    skos:scopeNote """Use if you do not use the UnitOfMeasurement class for handling
         units of measurement along with Extent."""@en .

:usedFromDate
    a owl:DatatypeProperty ;
    rdfs:comment "Date at which an Appellation was first used."@en ;
    rdfs:domain :Appellation ;
    rdfs:isDefinedBy <https://www.ica.org/standards/RiC/ontology> ;
    rdfs:label "usado desde la fecha"@es, "used from date"@en, "utilisé à partir de"@fr ;
    rdfs:range rdfs:Literal ;
    rdfs:subPropertyOf :beginningDate ;
    skos:changeNote [
        dc:date "2023-11-12" ;
        rdf:value "Made this property a subproperty of beginningDate."@en
    ], [
        dc:date "2023-11-02" ;
        rdf:value "Added a new rdfs:label in Spanish."@en
    ], [
        dc:date "2023-08-25" ;
        rdf:value "Added a new rdfs:label in French."@en
    ] ;
    skos:scopeNote """Provided for usability reasons. May be deprecated and removed
         later on. Use only if you don't use Date classes for handling dates."""@en ;
    :RiCCMCorrespondingComponent """Datatype property specialized implementation of
         RiC-E18 (Date entity)"""@en .

:usedToDate
    a owl:DatatypeProperty ;
    rdfs:comment "Date until an Appellation was used."@en ;
    rdfs:domain :Appellation ;
    rdfs:isDefinedBy <https://www.ica.org/standards/RiC/ontology> ;
    rdfs:label "usado hasta la fecha"@es, "used to date"@en, "utilisé jusqu’à"@fr ;
    rdfs:range rdfs:Literal ;
    rdfs:subPropertyOf :endDate ;
    skos:changeNote [
        dc:date "2023-11-12" ;
        rdf:value "Made this property a subproperty of endDate."@en
    ], [
        dc:date "2023-11-02" ;
        rdf:value "Added a new rdfs:label in Spanish."@en
    ], [
        dc:date "2023-08-25" ;
        rdf:value "Added a new rdfs:label in French."@en
    ] ;
    skos:scopeNote """Provided for usability reasons. May be deprecated and removed
         later on. Use only if you don't use Date classes for handling dates."""@en ;
    :RiCCMCorrespondingComponent """Datatype property specialized implementation of
         RiC-E18 (Date entity)"""@en .

:wasComponentOf
    a owl:ObjectProperty ;
    rdfs:comment """Connects an Instantiation to another Instantiation of which it was
         a component in the past."""@en ;
    rdfs:domain :Instantiation ;
    rdfs:isDefinedBy <https://www.ica.org/standards/RiC/ontology> ;
    rdfs:label "a été le composant de"@fr, "era componente de"@es, "was component of"@en ;
    rdfs:range :Instantiation ;
    rdfs:subPropertyOf :isOrWasComponentOf, :wasPartOf ;
    owl:inverseOf :hadComponent ;
    skos:changeNote [
        dc:date "2023-11-27" ;
        rdf:value "Added a new rdfs:label in Spanish."@en
    ], [
        dc:date "2023-11-12" ;
        rdf:value "Updated the description (rdfs:comment) and labels."@en
    ], [
        dc:date "2023-09-08" ;
        rdf:value """Object property added, along with its inverse property, in
               order to enable to express past partitive relations between instantiations (the
               current partitive relations being also added, including a transitive
               one)."""@en
    ] .

:wasConstituentOf
    a owl:ObjectProperty ;
    rdfs:comment """Connects a Record or Record Part to another Record or Record Part
         of which it was a constituent in the past."""@en ;
    rdfs:domain [
        a owl:Class ;
        owl:unionOf (:Record
            :RecordPart
        )
    ] ;
    rdfs:isDefinedBy <https://www.ica.org/standards/RiC/ontology> ;
    rdfs:label "a été un constituant de"@fr, "era elemento constitutivo de"@es, "was constituent of"@en ;
    rdfs:range [
        a owl:Class ;
        owl:unionOf (:Record
            :RecordPart
        )
    ] ;
    rdfs:subPropertyOf :isOrWasConstituentOf, :wasPartOf ;
    owl:inverseOf :hadConstituent ;
    skos:changeNote [
        dc:date "2023-11-27" ;
        rdf:value "Added a new rdfs:label in Spanish."@en
    ], [
        dc:date "2023-11-12" ;
        rdf:value "Updated the labels."@en
    ], [
        dc:date "2023-10-26" ;
        rdf:value "Added RecordPart to the range."@en
    ], [
        dc:date "2023-09-08" ;
        rdf:value """Object property added, along with its inverse property, in
               order to enable to express past partitive relations between Record and Record or
               Record Part (the current partitive relations being also added, including a transitive
               one)."""@en
    ] .

:wasContainedBy
    a owl:ObjectProperty ;
    rdfs:comment """Connects a Place to a Place within which it was
         contained."""@en ;
    rdfs:domain :Place ;
    rdfs:isDefinedBy <https://www.ica.org/standards/RiC/ontology> ;
    rdfs:label "a été contenu par"@fr, "estaba contenido en"@es, "was contained by"@en ;
    rdfs:range :Place ;
    rdfs:subPropertyOf :isOrWasContainedBy, :wasPartOf ;
    owl:inverseOf :contained ;
    skos:changeNote [
        dc:date "2023-11-27" ;
        rdf:value "Added a new rdfs:label in Spanish."@en
    ], [
        dc:date "2023-11-12" ;
        rdf:value "Updated the description (rdfs:comment) and labels."@en
    ], [
        dc:date "2023-09-08" ;
        rdf:value """Object property added, along with its inverse property, in
               order to enable to express past partitive relations between places (the current
               partitive relations being also added, including a transitive one)."""@en
    ] .

:wasIncludedIn
    a owl:ObjectProperty ;
    rdfs:comment """Connects a Record to a Record or Record Set in which it was
         included in the past."""@en ;
    rdfs:domain [
        a owl:Class ;
        owl:unionOf (:Record
            :RecordSet
        )
    ] ;
    rdfs:isDefinedBy <https://www.ica.org/standards/RiC/ontology> ;
    rdfs:label "a été inclus dans"@fr, "estaba incluido en"@es, "was included in"@en ;
    rdfs:range :RecordSet ;
    rdfs:subPropertyOf :isOrWasIncludedIn, :wasPartOf ;
    owl:inverseOf :included ;
    skos:changeNote [
        dc:date "2023-11-27" ;
        rdf:value "Added a new rdfs:label in Spanish."@en
    ], [
        dc:date "2023-11-12" ;
        rdf:value "Updated the labels."@en
    ], [
        dc:date "2023-09-08" ;
        rdf:value """Object property added, along with its inverse property, in
               order to enable to express past partitive relations between Record Sets and their
               members (the current partitive relations being also added, including a transitive
               one)."""@en
    ] .

:wasLastUpdatedAtDate
    a owl:ObjectProperty ;
    rdfs:comment """Connects a Thing to the Date when it was last
         modified."""@en ;
    rdfs:domain :Thing ;
    rdfs:isDefinedBy <https://www.ica.org/standards/RiC/ontology> ;
    rdfs:label "a pour date de dernière mise à jour"@fr, "fue actualizado por última vez en fecha"@es, "was last updated at date"@en ;
    rdfs:range :Date ;
    rdfs:subPropertyOf :hasModificationDate ;
    owl:inverseOf :isLastUpdateDateOf ;
    skos:changeNote [
        dc:date "2023-11-02" ;
        rdf:value "Added a new rdfs:label in Spanish."@en
    ], [
        dc:date "2023-08-28" ;
        rdf:value "Added a new rdfs:label in French."@en
    ] .

:wasMergedInto
    a owl:ObjectProperty ;
    rdfs:comment """Connects a Corporate Body to another Corporate Body that is the
         result of a merger of the previous one with one to many other corporate
         bodies."""@en ;
    rdfs:domain :CorporateBody ;
    rdfs:isDefinedBy <https://www.ica.org/standards/RiC/ontology> ;
    rdfs:label "a été fusionné dans"@fr, "se fusionó en"@es, "was merged into"@en ;
    rdfs:range :CorporateBody ;
    rdfs:subPropertyOf :hasSuccessor ;
    owl:inverseOf :resultedFromTheMergerOf ;
    skos:changeNote [
        dc:date "2023-11-12" ;
        rdf:value "Updated the labels."@en
    ], [
        dc:date "2023-11-02" ;
        rdf:value "Added a new rdfs:label in Spanish."@en
    ], [
        dc:date "2023-06-21" ;
        rdf:value """Object property created in order to enable an accurate
               representation of mergers between corporate bodies."""@en
    ] .

:wasPartOf
    a owl:ObjectProperty ;
    rdfs:comment """Connects a Thing to a Thing of which it was a constitutive or
         component part in the past."""@en ;
    rdfs:domain :Thing ;
    rdfs:isDefinedBy <https://www.ica.org/standards/RiC/ontology> ;
    rdfs:label "a fait partie de"@fr, "era parte de"@es, "was part of"@en ;
    rdfs:range :Thing ;
    rdfs:subPropertyOf :isOrWasPartOf ;
    owl:inverseOf :hadPart ;
    skos:changeNote [
        dc:date "2023-11-27" ;
        rdf:value "Added a new rdfs:label in Spanish."@en
    ], [
        dc:date "2023-11-12" ;
        rdf:value "Updated the labels."@en
    ], [
        dc:date "2023-07-12" ;
        rdf:value """Object property added, along with its inverse property, in
               order to enable to express past partitive relations between things (the current
               partitive relations being also added, including a transitive one)."""@en
    ] .

:wasSplitInto
    a owl:ObjectProperty ;
    rdfs:comment """Connects a Corporate Body to one of the Corporate Bodies that
         results from the split of the previous one into two to many corporate
         bodies."""@en ;
    rdfs:domain :CorporateBody ;
    rdfs:isDefinedBy <https://www.ica.org/standards/RiC/ontology> ;
    rdfs:label "a été séparé en"@fr, "se separó en"@es, "was split into"@en ;
    rdfs:range :CorporateBody ;
    rdfs:subPropertyOf :hasSuccessor ;
    owl:inverseOf :resultedFromTheSplitOf ;
    skos:changeNote [
        dc:date "2023-11-12" ;
        rdf:value "Updated the labels."@en
    ], [
        dc:date "2023-11-02" ;
        rdf:value "Added a new rdfs:label in Spanish."@en
    ], [
        dc:date "2023-06-21" ;
        rdf:value """Object property created in order to enable an accurate
               representation of the split of a corporate body into two or more new corporate
               bodies."""@en
    ] .

:wasSubdivisionOf
    a owl:ObjectProperty ;
    rdfs:comment """Connects a subdivision to the Group it was a part of in the
         past."""@en ;
    rdfs:domain :Group ;
    rdfs:isDefinedBy <https://www.ica.org/standards/RiC/ontology> ;
    rdfs:label "a été une subdivision de"@fr, "era subdivisión de"@es, "was subdivision of"@en ;
    rdfs:range :Group ;
    rdfs:subPropertyOf :isOrWasSubdivisionOf, :wasPartOf, :wasSubordinateTo ;
    owl:inverseOf :hadSubdivision ;
    skos:changeNote [
        dc:date "2023-11-27" ;
        rdf:value "Added a new rdfs:label in Spanish."@en
    ], [
        dc:date "2023-11-12" ;
        rdf:value "Updated the labels."@en
    ], [
        dc:date "2023-09-08" ;
        rdf:value """Object property added, along with its inverse property, in
               order to enable to express past partitive relations between Groups (the current
               partitive relations being also added, including a transitive one)."""@en
    ] .

:wasSubeventOf
    a owl:ObjectProperty ;
    rdfs:comment """Connects a past Event to the broader Event of which it was a
         part."""@en ;
    rdfs:domain :Event ;
    rdfs:isDefinedBy <https://www.ica.org/standards/RiC/ontology> ;
    rdfs:label "a été un événement constitutif de l'événement"@fr, "era parte de evento de"@es, "was subevent of"@en ;
    rdfs:range :Event ;
    rdfs:subPropertyOf :isOrWasSubeventOf, :wasPartOf ;
    owl:inverseOf :hadSubevent ;
    skos:changeNote [
        dc:date "2023-11-27" ;
        rdf:value "Added a new rdfs:label in Spanish."@en
    ], [
        dc:date "2023-11-12" ;
        rdf:value "Updated the labels."@en
    ], [
        dc:date "2023-09-08" ;
        rdf:value """Object property added, along with its inverse property, in
               order to enable to express partitive relations between past Events (the partitive
               relations between ongoing events being also added, including a transitive
               one)."""@en
    ] .

:wasSubordinateTo
    a owl:ObjectProperty ;
    rdfs:comment """Connects an Agent to an Agent that was hierarchically superior in
         the past."""@en ;
    rdfs:domain :Agent ;
    rdfs:isDefinedBy <https://www.ica.org/standards/RiC/ontology> ;
    rdfs:label "a été subalterne de"@fr, "estaba subordinado(a) a"@es, "was subordinate to"@en ;
    rdfs:range :Agent ;
    rdfs:subPropertyOf :isOrWasSubordinateTo ;
    owl:inverseOf :hadSubordinate ;
    skos:changeNote [
        dc:date "2023-11-27" ;
        rdf:value "Added a new rdfs:label in Spanish."@en
    ], [
        dc:date "2023-11-12" ;
        rdf:value "Updated the labels."@en
    ], [
        dc:date "2023-09-08" ;
        rdf:value """Object property added, along with its inverse property, in
               order to enable to express past subordination relations between Agents (the current
               subordination relations being also added, including a transitive one)."""@en
    ] .

:wasUsedFromDate
    a owl:ObjectProperty ;
    rdfs:comment """Connects an Appellation to the Date from which it was
         used."""@en ;
    rdfs:domain :Appellation ;
    rdfs:isDefinedBy <https://www.ica.org/standards/RiC/ontology> ;
    rdfs:label "a été utilisé à partir de la date"@fr, "fue usado desde"@es, "was used from date"@en ;
    rdfs:range :Date ;
    rdfs:subPropertyOf :hasBeginningDate ;
    owl:inverseOf :isFromUseDateOf ;
    skos:changeNote [
        dc:date "2023-11-02" ;
        rdf:value "Added a new rdfs:label in Spanish."@en
    ], [
        dc:date "2023-10-19" ;
        rdf:value "Made this property subPropertyOf hasBeginningDate."@en
    ], [
        dc:date "2023-08-28" ;
        rdf:value "Added a new rdfs:label in French."@en
    ] .

:wasUsedToDate
    a owl:ObjectProperty ;
    rdfs:comment """Connects an Appellation to the Date till when it was
         used."""@en ;
    rdfs:domain :Appellation ;
    rdfs:isDefinedBy <https://www.ica.org/standards/RiC/ontology> ;
    rdfs:label "a été utilisé jusqu’à la date"@fr, "fue usado hasta"@es, "was used to date"@en ;
    rdfs:range :Date ;
    rdfs:subPropertyOf :hasEndDate ;
    owl:inverseOf :isToUseDateOf ;
    skos:changeNote [
        dc:date "2023-11-02" ;
        rdf:value "Added a new rdfs:label in Spanish."@en
    ], [
        dc:date "2023-10-19" ;
        rdf:value "Made this property subPropertyOf hasEndDate."@en
    ], [
        dc:date "2023-08-28" ;
        rdf:value "Added a new rdfs:label in French."@en
    ] .

:wholePartRelation_role
    a owl:ObjectProperty ;
    rdfs:comment """Connects a WholePartRelation to itself. It is a property that can
         stand for an instance of the class when necessary, e.g. when you explore a knowledge
         graph."""@en ;
    rdfs:domain :WholePartRelation ;
    rdfs:isDefinedBy <https://www.ica.org/standards/RiC/ontology> ;
    rdfs:label "a le rôle de la Relation partitive"@fr, "desempeña el papel de la Relación entre todo y parte"@es, "has the role of the Whole Part Relation"@en ;
    rdfs:range :WholePartRelation ;
    rdfs:subPropertyOf :relation_role ;
    skos:changeNote [
        dc:date "2024-08-02" ;
        rdf:value """Removed global reflexivity (leads to
               inconsistency)."""@en
    ], [
        dc:date "2023-11-08" ;
        rdf:value """In order to get a system of rolified Relation classes: created
               the object property, with domain and range the WholePartRelation rolified class.
               Declared it as reflexive. Declared it(s) superproperty(ies)."""@en
    ] ;
    skos:scopeNote """This property \"rolifies\" the WholePartRelation class. It should
         be used only when you have to manage instances of the WholePartRelation class, to connect
         each instance to itself, in order to be able to infer, using OWL-RL and property paths, the
         two shortcuts corresponding to this n-ary class."""@en .

:width
    a owl:DatatypeProperty ;
    rdfs:comment "Horizontal dimension of an entity."@en ;
    rdfs:domain :Thing ;
    rdfs:isDefinedBy <https://www.ica.org/standards/RiC/ontology> ;
    rdfs:label "anchura"@es, "largeur"@fr, "width"@en ;
    rdfs:range rdfs:Literal ;
    rdfs:subPropertyOf :measure ;
    skos:changeNote [
        dc:date "2023-11-02" ;
        rdf:value "Added a new rdfs:label in Spanish."@en
    ], [
        dc:date "2023-08-25" ;
        rdf:value "Added a new rdfs:label in French."@en
    ] .

:workRelation_role
    a owl:ObjectProperty ;
    rdfs:comment """Connects a WorkRelation to itself. It is a property that can stand
         for an instance of the class when necessary, e.g. when you explore a knowledge
         graph."""@en ;
    rdfs:domain :WorkRelation ;
    rdfs:isDefinedBy <https://www.ica.org/standards/RiC/ontology> ;
    rdfs:label "a le rôle de la Relation de travail"@fr, "desempeña el papel de la Relación profesional"@es, "has the role of the Work Relation"@en ;
    rdfs:range :WorkRelation ;
    rdfs:subPropertyOf :agentToAgentRelation_role ;
    skos:changeNote [
        dc:date "2024-08-02" ;
        rdf:value """Removed global reflexivity (leads to
               inconsistency)."""@en
    ], [
        dc:date "2023-11-08" ;
        rdf:value """In order to get a system of rolified Relation classes: created
               the object property, with domain and range the WorkRelation rolified class. Declared
               it as reflexive. Declared it(s) superproperty(ies)."""@en
    ] ;
    skos:scopeNote """This property \"rolifies\" the WorkRelation class. It should be
         used only when you have to manage instances of the WorkRelation class, to connect each
         instance to itself, in order to be able to infer, using OWL-RL and property paths, the two
         shortcuts corresponding to this n-ary class."""@en .

<https://www.ica.org/standards/RiC/vocabularies/documentaryFormTypes>
    dc:creator """International Coucil on Archives Expert Group on Archival
         Description (ICA EGAD)"""@en ;
    dc:language "en", "es", "fr" ;
    dc:title """International Council on Archives Records in Contexts Vocabulary for
         Documentary Form Types"""@en ;
    a owl:NamedIndividual, skos:ConceptScheme ;
    rdfs:label "Documentary Form Types"@en, "Tipos documentales"@es, "Types de documents"@fr ;
    skos:changeNote [
        dc:date "2025-05-14" ;
        rdf:value "Added a dcat:version property."@en
    ], [
        dc:date "2025-01-30" ;
        rdf:value """Added the IIIF manifest documentary form type, with broader
               concept finding aid. Updated the scope note of the vocabulary."""@en
    ], [
        dc:date "2023-12-13" ;
        rdf:value """Completed the metadata of the vocabulary: added dc:language, a
               history note and a scope note."""@en
    ], [
        dc:date "2023-11-25" ;
        rdf:value "Added a new rdfs:label in Spanish."@en
    ], [
        dc:date "2023-08-28" ;
        rdf:value "Added a new rdfs:label in French."@en
    ] ;
    skos:definition """A vocabulary that provides URIs for describing documentary form
         types of RiC Records and Record Parts."""@en ;
    skos:hasTopConcept ric-dft:AuthorityRecord, ric-dft:FindingAid ;
    skos:scopeNote """For now this vocabulary only defines three concepts; it should
         hopefully be completed later. The concepts defined in this vocabulary can be used in
         combination with RiC-O classes and properties, whenever necessary and appropriate, to
         assign a documentary form type to a Record or a Record Part, using the
         rico:hasDocumentaryFormType object property, or its inverse one. They also can be used to
         specify that a rico:RecordSet included or includes members whose some
         (rico:hasOrHadSomeMembersWithDocumentaryFormType) or all
         (rico:hasOrHadAllMembersWithDocumentaryFormType) have some Documentary Form Type. Each
         concept is both defined as a skos:Concept and a rico:DocumentaryFormType, so that it is
         possible to extend the classic definition of such concepts using RiC-O properties. For
         example, you can use rico:history, rico:date, or rico:isAssociatedWithPlace,
         rico:precedesInTime, if you consider a documentary form type as being a historical entity,
         known and used in some known space or time region."""@en ;
    dcat:version "1.1" .

ric-dft:AuthorityRecord
    a owl:NamedIndividual, skos:Concept, :DocumentaryFormType ;
    rdfs:label "authority record"@en, "notice d’autorité"@fr, "registro de autoridad"@es ;
    skos:changeNote [
        dc:date "2023-11-25" ;
        rdf:value "Added a new rdfs:label in Spanish."@en
    ], [
        dc:date "2023-08-28" ;
        rdf:value "Added a new rdfs:label in French."@en
    ] ;
    skos:definition """This category can be used for records that describe an
         entity."""@en ;
    skos:inScheme <https://www.ica.org/standards/RiC/vocabularies/documentaryFormTypes> ;
    skos:topConceptOf <https://www.ica.org/standards/RiC/vocabularies/documentaryFormTypes> .

ric-dft:FindingAid
    a owl:NamedIndividual, skos:Concept, :DocumentaryFormType ;
    rdfs:label "finding aid"@en, "instrument de recherche"@fr, "instrumento de descripción"@es ;
    skos:changeNote [
        dc:date "2025-01-30" ;
        rdf:value """Added a skos:narrower with object the IIIF Manifest
               concept."""@en
    ], [
        dc:date "2023-11-25" ;
        rdf:value "Added a new rdfs:label in Spanish."@en
    ], [
        dc:date "2023-08-28" ;
        rdf:value "Added a new rdfs:label in French."@en
    ] ;
    skos:definition """This documentary form type can be used for records that
         aggregate and organizes metadata on some record(s) or record set(s)."""@en ;
    skos:inScheme <https://www.ica.org/standards/RiC/vocabularies/documentaryFormTypes> ;
    skos:narrower ric-dft:IIIFManifest ;
    skos:topConceptOf <https://www.ica.org/standards/RiC/vocabularies/documentaryFormTypes> .

ric-dft:IIIFManifest
    a owl:NamedIndividual, skos:Concept, :DocumentaryFormType ;
    rdfs:label "IIIF manifest"@en, "manifeste IIIF"@fr ;
    skos:broader ric-dft:FindingAid ;
    skos:changeNote [
        dc:date "2025-01-30" ;
        rdf:value "Added to RiC-O 1.1."@en
    ] ;
    skos:definition """Can be used to categorize records which describe collections of
         cultural heritage objects, or of a single cultural object, and whose instantiations are
         compliant to the IIIF Presentation API."""@en ;
    skos:inScheme <https://www.ica.org/standards/RiC/vocabularies/documentaryFormTypes> .

<https://www.ica.org/standards/RiC/vocabularies/recordSetTypes>
    dc:creator """International Coucil on Archives Expert Group on Archival
         Description (ICA EGAD)"""@en ;
    dc:language "en", "es", "fr" ;
    dc:title """International Council on Archives Records in Contexts Vocabulary for
         Record Set Types"""@en ;
    a owl:NamedIndividual, skos:ConceptScheme ;
    rdfs:label "Record Set Types"@en, "Tipos de agrupación documental"@es, "Types d’ensembles d’objets informationnels"@fr ;
    skos:changeNote [
        dc:date "2025-05-14" ;
        rdf:value "Added a dcat:version property."@en
    ], [
        dc:date "2023-12-13" ;
        rdf:value """Completed the metadata of the vocabulary: added dc:language, a
               history note and a scope note."""@en
    ], [
        dc:date "2023-11-25" ;
        rdf:value "Added a new rdfs:label in Spanish."@en
    ], [
        dc:date "2023-08-28" ;
        rdf:value "Added a new rdfs:label in French."@en
    ] ;
    skos:definition """A vocabulary that provides URIs for describing types of RiC
         Record Sets."""@en ;
    skos:hasTopConcept ric-rst:Collection, ric-rst:File, ric-rst:Fonds, ric-rst:Series ;
    skos:scopeNote """For now this vocabulary only defines four top concepts; it
         should hopefully be completed later. The concepts defined in this vocabulary can be used in
         combination with RiC-O classes and properties, whenever necessary and appropriate, to
         assign a record set type to a Record Set, using the rico:hasRecordSetType object property,
         or its inverse one. Each concept is both defined as a skos:Concept and a
         rico:RecordSetType, so that it is possible to extend the classic definition of such
         concepts using RiC-O properties. For example, you can use rico:history, rico:date, or
         rico:isAssociatedWithPlace, rico:precedesInTime, if you consider a record set type as being
         a historical entity, known and used in some known space or time region."""@en ;
    dcat:version "1.1" .

ric-rst:Collection
    a owl:NamedIndividual, skos:Concept, :RecordSetType ;
    rdfs:label "colección"@es, "collection"@en, "collection"@fr ;
    skos:changeNote [
        dc:date "2023-11-25" ;
        rdf:value "Added a new rdfs:label in Spanish."@en
    ], [
        dc:date "2023-08-28" ;
        rdf:value "Added a new rdfs:label in French."@en
    ] ;
    skos:definition """An artificial assemblage of documents accumulated on the basis
         of some common characteristic without regard to the provenance of those documents. Not to
         be confused with an archival fonds. (From ICA ISAD(G))"""@en ;
    skos:inScheme <https://www.ica.org/standards/RiC/vocabularies/recordSetTypes> ;
    skos:topConceptOf <https://www.ica.org/standards/RiC/vocabularies/recordSetTypes> .

ric-rst:File
    a owl:NamedIndividual, skos:Concept, :RecordSetType ;
    rdfs:label "dossier"@fr, "expediente"@es, "file"@en ;
    skos:changeNote [
        dc:date "2023-11-25" ;
        rdf:value "Added a new rdfs:label in Spanish."@en
    ], [
        dc:date "2023-08-28" ;
        rdf:value "Added a new rdfs:label in French."@en
    ] ;
    skos:definition """An organized unit of documents grouped together either for
         current use by the creator or in the process of archival arrangement, because they relate
         to the same subject, activity, or transaction. A file is usually the basic unit within a
         record series. (From ICA ISAD(G))"""@en ;
    skos:inScheme <https://www.ica.org/standards/RiC/vocabularies/recordSetTypes> ;
    skos:topConceptOf <https://www.ica.org/standards/RiC/vocabularies/recordSetTypes> .

ric-rst:Fonds
    a owl:NamedIndividual, skos:Concept, :RecordSetType ;
    rdfs:label "fondo"@es, "fonds"@en, "fonds"@fr ;
    skos:changeNote [
        dc:date "2023-11-25" ;
        rdf:value "Added a new rdfs:label in Spanish."@en
    ], [
        dc:date "2023-08-28" ;
        rdf:value "Added a new rdfs:label in French."@en
    ] ;
    skos:definition """The whole of the records, regardless of form or medium,
         organically created and/or accumulated and used by a particular person, family, or
         corporate body in the course of that creator's activities and functions. (From ICA
         ISAD(G))"""@en ;
    skos:inScheme <https://www.ica.org/standards/RiC/vocabularies/recordSetTypes> ;
    skos:topConceptOf <https://www.ica.org/standards/RiC/vocabularies/recordSetTypes> .

ric-rst:Series
    a owl:NamedIndividual, skos:Concept, :RecordSetType ;
    rdfs:label "serie"@es, "series"@en, "série organique"@fr ;
    skos:changeNote [
        dc:date "2023-11-25" ;
        rdf:value "Added a new rdfs:label in Spanish."@en
    ], [
        dc:date "2023-08-28" ;
        rdf:value "Added a new rdfs:label in French."@en
    ] ;
    skos:definition """Documents arranged in accordance with a filing system or
         maintained as a unit because they result from the same accumulation or filing process, or
         the same activity; have a particular form; or because of some other relationship arising
         out of their creation, receipt, or use. A series is also known as a records series. (From
         ICA ISAD(G))"""@en ;
    skos:inScheme <https://www.ica.org/standards/RiC/vocabularies/recordSetTypes> ;
    skos:topConceptOf <https://www.ica.org/standards/RiC/vocabularies/recordSetTypes> .

